<?xml version='1.0' encoding='UTF-8'?>
<rdf:RDF xmlns:rdf="http://www.w3.org/1999/02/22-rdf-syntax-ns#" xmlns:dcterms="http://purl.org/dc/terms/" xmlns:owl="http://www.w3.org/2002/07/owl#" xmlns:skos="http://www.w3.org/2004/02/skos/core#">
<skos:ConceptScheme rdf:about="http://partage.vocnet.org/Activities">
	<rdf:type rdf:resource="http://www.w3.org/2004/02/skos/core#ConceptScheme"/>
</skos:ConceptScheme>
<skos:Concept rdf:about="http://partage.vocnet.org/part00211">
	<skos:prefLabel xml:lang="en">typography</skos:prefLabel>
	<skos:prefLabel xml:lang="pt">tipografia</skos:prefLabel>
	<skos:prefLabel xml:lang="de">Typografie</skos:prefLabel>
	<skos:prefLabel xml:lang="sv">typografi</skos:prefLabel>
	<skos:prefLabel xml:lang="fi">typografia</skos:prefLabel>
	<skos:prefLabel xml:lang="hr">tipografija</skos:prefLabel>
	<skos:inScheme rdf:resource="http://partage.vocnet.org/Activities"/>
	<skos:exactMatch rdf:resource="http://vocab.getty.edu/aat/300195853"/>
	<skos:scopeNote xml:lang="en">Various processes of dealing with type and typefaces, including setting type, designing typefaces, and designing layouts of printed characters.</skos:scopeNote>
	<skos:editorialNote xml:lang="en">PPTechnique</skos:editorialNote>
</skos:Concept>
<skos:Concept rdf:about="http://partage.vocnet.org/part00340">
	<skos:prefLabel xml:lang="en">slip trailing</skos:prefLabel>
	<skos:prefLabel xml:lang="pt">barbotina</skos:prefLabel>
	<skos:prefLabel xml:lang="de">Schlickermalerei</skos:prefLabel>
	<skos:prefLabel xml:lang="sv">slicker</skos:prefLabel>
	<skos:prefLabel xml:lang="fi">savilietekoristelu</skos:prefLabel>
	<skos:prefLabel xml:lang="hr">nanošenje angobe</skos:prefLabel>
	<skos:inScheme rdf:resource="http://partage.vocnet.org/Activities"/>
	<skos:exactMatch rdf:resource="http://vocab.getty.edu/aat/300053919"/>
	<skos:editorialNote xml:lang="en">PPTechnique</skos:editorialNote>
	<skos:scopeNote xml:lang="en">The application of slip to a piece of pottery with a syringelike device so as to create slightly raised linear decoration.</skos:scopeNote>
</skos:Concept>
<skos:Concept rdf:about="http://partage.vocnet.org/part00417">
	<skos:prefLabel xml:lang="en">etching (corroding)</skos:prefLabel>
	<skos:prefLabel xml:lang="pt">gravar a ácido</skos:prefLabel>
	<skos:prefLabel xml:lang="de">geätzt</skos:prefLabel>
	<skos:prefLabel xml:lang="sv">etsning (korrodering)</skos:prefLabel>
	<skos:prefLabel xml:lang="hr">jetkanje</skos:prefLabel>
	<skos:prefLabel xml:lang="fi">etsaus</skos:prefLabel>
	<skos:inScheme rdf:resource="http://partage.vocnet.org/Activities"/>
	<skos:exactMatch rdf:resource="http://vocab.getty.edu/aat/300053840"/>
	<skos:editorialNote xml:lang="en">PPTechnique</skos:editorialNote>
	<skos:scopeNote xml:lang="en">Creating marks on the surface of a hard material such as metal or glass, by the controlled corrosive action of acid. Use "etching (printing process)" for the series of steps that includes printing from a bitten plate.</skos:scopeNote>
</skos:Concept>
<skos:Concept rdf:about="http://partage.vocnet.org/part00449">
	<skos:altLabel xml:lang="en">carving (processes)</skos:altLabel>
	<skos:prefLabel xml:lang="en">carving</skos:prefLabel>
	<skos:prefLabel xml:lang="pt">entalhamento</skos:prefLabel>
	<skos:altLabel xml:lang="pt">escultura.</skos:altLabel>
	<skos:altLabel xml:lang="de">gemeisselt</skos:altLabel>
	<skos:prefLabel xml:lang="de">geschnitzt</skos:prefLabel>
	<skos:altLabel xml:lang="sv">täljning</skos:altLabel>
	<skos:prefLabel xml:lang="sv">snidning</skos:prefLabel>
	<skos:prefLabel xml:lang="hr">rezbarenje</skos:prefLabel>
	<skos:prefLabel xml:lang="fi">veisto</skos:prefLabel>
	<skos:inScheme rdf:resource="http://partage.vocnet.org/Activities"/>
	<skos:exactMatch rdf:resource="http://vocab.getty.edu/aat/300053149"/>
	<skos:editorialNote xml:lang="en">PPTechnique</skos:editorialNote>
	<skos:scopeNote xml:lang="en">The act of shaping, marking, or decorating wood, stone, or another material by cutting or incising, typically using tools such as chisels and other blades. It refers to this process as it is applied to small-scale objects or to objects that are not considered art. "Carving" may also be considered a sculpture technique that is employed in the creation of art.</skos:scopeNote>
</skos:Concept>
<skos:Concept rdf:about="http://partage.vocnet.org/part00450">
	<skos:altLabel xml:lang="en">casting (process)</skos:altLabel>
	<skos:prefLabel xml:lang="en">casting</skos:prefLabel>
	<skos:prefLabel xml:lang="pt">molde</skos:prefLabel>
	<skos:prefLabel xml:lang="de">gegossen</skos:prefLabel>
	<skos:prefLabel xml:lang="sv">gjutning (process)</skos:prefLabel>
	<skos:prefLabel xml:lang="fi">valaminen</skos:prefLabel>
	<skos:prefLabel xml:lang="hr">lijevanje</skos:prefLabel>
	<skos:inScheme rdf:resource="http://partage.vocnet.org/Activities"/>
	<skos:broader rdf:resource="http://partage.vocnet.org/part01037"/>
	<skos:exactMatch rdf:resource="http://vocab.getty.edu/aat/300053104"/>
	<skos:editorialNote xml:lang="en">PPTechnique</skos:editorialNote>
	<skos:scopeNote xml:lang="en">The act or process of making casts or of shaping in a mold; usually refers to pouring liquid material into a mold, as distinguished from pressing a material into a mold, for which prefer "molding."</skos:scopeNote>
</skos:Concept>
<skos:Concept rdf:about="http://partage.vocnet.org/part00451">
	<skos:prefLabel xml:lang="en">chasing</skos:prefLabel>
	<skos:prefLabel xml:lang="pt">cinzelar</skos:prefLabel>
	<skos:altLabel xml:lang="de">getrieben</skos:altLabel>
	<skos:prefLabel xml:lang="sv">ciselering</skos:prefLabel>
	<skos:prefLabel xml:lang="de">ziseliert</skos:prefLabel>
	<skos:prefLabel xml:lang="ca">cizeliranje</skos:prefLabel>
	<skos:prefLabel xml:lang="fi">pakotus</skos:prefLabel>
	<skos:inScheme rdf:resource="http://partage.vocnet.org/Activities"/>
	<skos:exactMatch rdf:resource="http://vocab.getty.edu/aat/300054016"/>
	<skos:editorialNote xml:lang="en">PPTechnique</skos:editorialNote>
	<skos:scopeNote xml:lang="en">The process of adding detail or ornament on metal by indenting with a hammer and tools without a cutting edge.</skos:scopeNote>
</skos:Concept>
<skos:Concept rdf:about="http://partage.vocnet.org/part00452">
	<skos:altLabel xml:lang="en">cutting (dividing)</skos:altLabel>
	<skos:prefLabel xml:lang="en">cutting</skos:prefLabel>
	<skos:prefLabel xml:lang="pt">corte</skos:prefLabel>
	<skos:prefLabel xml:lang="de">geschnitten</skos:prefLabel>
	<skos:prefLabel xml:lang="fi">hionta</skos:prefLabel>
	<skos:prefLabel xml:lang="hr">rezanje</skos:prefLabel>
	<skos:inScheme rdf:resource="http://partage.vocnet.org/Activities"/>
	<skos:exactMatch rdf:resource="http://vocab.getty.edu/aat/300053069"/>
	<skos:editorialNote xml:lang="en">PPTechnique</skos:editorialNote>
	<skos:scopeNote xml:lang="en">Making an incision with a sharp-edged instrument, thus removing material or dividing an object into parts.</skos:scopeNote>
</skos:Concept>
<skos:Concept rdf:about="http://partage.vocnet.org/part00453">
	<skos:prefLabel xml:lang="en">embossing</skos:prefLabel>
	<skos:prefLabel xml:lang="pt">gravar em relevo</skos:prefLabel>
	<skos:prefLabel xml:lang="de">geprägt</skos:prefLabel>
	<skos:prefLabel xml:lang="sv">prägling</skos:prefLabel>
	<skos:prefLabel xml:lang="hr">iskucavanje</skos:prefLabel>
	<skos:prefLabel xml:lang="fi">sokeapainatus</skos:prefLabel>
	<skos:inScheme rdf:resource="http://partage.vocnet.org/Activities"/>
	<skos:narrower rdf:resource="http://partage.vocnet.org/part01232"/>
	<skos:exactMatch rdf:resource="http://vocab.getty.edu/aat/300053826"/>
	<skos:editorialNote xml:lang="en">PPTechnique</skos:editorialNote>
	<skos:scopeNote xml:lang="en">Producing raised letters or designs on a surface, typically by means of stamping or molding.</skos:scopeNote>
</skos:Concept>
<skos:Concept rdf:about="http://partage.vocnet.org/part00454">
	<skos:prefLabel xml:lang="en">enameling</skos:prefLabel>
	<skos:prefLabel xml:lang="pt">esmaltar</skos:prefLabel>
	<skos:prefLabel xml:lang="de">emailliert</skos:prefLabel>
	<skos:prefLabel xml:lang="sv">emaljering</skos:prefLabel>
	<skos:prefLabel xml:lang="fi">emalointi</skos:prefLabel>
	<skos:prefLabel xml:lang="hr">emajliranje</skos:prefLabel>
	<skos:inScheme rdf:resource="http://partage.vocnet.org/Activities"/>
	<skos:broader rdf:resource="http://partage.vocnet.org/part00480"/>
	<skos:exactMatch rdf:resource="http://vocab.getty.edu/aat/300053773"/>
	<skos:editorialNote xml:lang="en">PPTechnique</skos:editorialNote>
	<skos:scopeNote xml:lang="en">The process of applying a vitreous coating to metal, ceramic, glass, or other surfaces by fusion using heat in a kiln or furnace, with the result of creating a smooth, hard surface.</skos:scopeNote>
</skos:Concept>
<skos:Concept rdf:about="http://partage.vocnet.org/part00455">
	<skos:prefLabel xml:lang="en">gilding</skos:prefLabel>
	<skos:prefLabel xml:lang="pt">dourar</skos:prefLabel>
	<skos:prefLabel xml:lang="de">vergoldet</skos:prefLabel>
	<skos:prefLabel xml:lang="sv">förgyllning</skos:prefLabel>
	<skos:prefLabel xml:lang="hr">pozlaćivanje</skos:prefLabel>
	<skos:prefLabel xml:lang="fi">kultaus</skos:prefLabel>
	<skos:inScheme rdf:resource="http://partage.vocnet.org/Activities"/>
	<skos:broader rdf:resource="http://partage.vocnet.org/part00483"/>
	<skos:exactMatch rdf:resource="http://vocab.getty.edu/aat/300053789"/>
	<skos:editorialNote xml:lang="en">PPTechnique</skos:editorialNote>
	<skos:scopeNote xml:lang="en">Surface application of metal in the form of leaf, powder applied directly to the surface, powder mixed with a binder, or other forms to approximate the effect of solid or inlaid metal.</skos:scopeNote>
</skos:Concept>
<skos:Concept rdf:about="http://partage.vocnet.org/part00456">
	<skos:altLabel xml:lang="en">glazing (coating)</skos:altLabel>
	<skos:prefLabel xml:lang="en">glazing</skos:prefLabel>
	<skos:prefLabel xml:lang="pt">vidrar</skos:prefLabel>
	<skos:prefLabel xml:lang="de">Glasur</skos:prefLabel>
	<skos:altLabel xml:lang="de">glasiert</skos:altLabel>
	<skos:prefLabel xml:lang="sv">glasering</skos:prefLabel>
	<skos:prefLabel xml:lang="fi">lasitus</skos:prefLabel>
	<skos:prefLabel xml:lang="hr">glaziranje</skos:prefLabel>
	<skos:inScheme rdf:resource="http://partage.vocnet.org/Activities"/>
	<skos:broader rdf:resource="http://partage.vocnet.org/part00480"/>
	<skos:exactMatch rdf:resource="http://vocab.getty.edu/aat/300053914"/>
	<skos:editorialNote xml:lang="en">PPTechnique</skos:editorialNote>
	<skos:scopeNote xml:lang="en">Covering with a thin, usually glossy, sometimes transparent, coating; includes the application of transparent, colored paint over areas of other paint to alter the appearance or color.</skos:scopeNote>
</skos:Concept>
<skos:Concept rdf:about="http://partage.vocnet.org/part00457">
	<skos:altLabel xml:lang="en">inlay (process)</skos:altLabel>
	<skos:prefLabel xml:lang="en">inlay</skos:prefLabel>
	<skos:prefLabel xml:lang="pt">incrustar</skos:prefLabel>
	<skos:prefLabel xml:lang="de">Einlegearbeit</skos:prefLabel>
	<skos:prefLabel xml:lang="sv">inläggning</skos:prefLabel>
	<skos:altLabel xml:lang="hr">inkrustacija</skos:altLabel>
	<skos:prefLabel xml:lang="fi">koristeupotus</skos:prefLabel>
	<skos:prefLabel xml:lang="hr">ulaganje.</skos:prefLabel>
	<skos:inScheme rdf:resource="http://partage.vocnet.org/Activities"/>
	<skos:narrower rdf:resource="http://partage.vocnet.org/part00662"/>
	<skos:narrower rdf:resource="http://partage.vocnet.org/part01250"/>
	<skos:exactMatch rdf:resource="http://vocab.getty.edu/aat/300053850"/>
	<skos:editorialNote xml:lang="en">PPTechnique</skos:editorialNote>
	<skos:scopeNote xml:lang="en">Any process by which small pieces of one material are inserted into a larger piece of another so as to create a design.</skos:scopeNote>
</skos:Concept>
<skos:Concept rdf:about="http://partage.vocnet.org/part00458">
	<skos:prefLabel xml:lang="en">layering</skos:prefLabel>
	<skos:prefLabel xml:lang="pt">colocar às camadas</skos:prefLabel>
	<skos:altLabel xml:lang="de">übereinander gelegt</skos:altLabel>
	<skos:prefLabel xml:lang="de">geschichtet</skos:prefLabel>
	<skos:prefLabel xml:lang="sv">skiktning</skos:prefLabel>
	<skos:prefLabel xml:lang="fi">kerrostus</skos:prefLabel>
	<skos:prefLabel xml:lang="hr">uslojavanje</skos:prefLabel>
	<skos:inScheme rdf:resource="http://partage.vocnet.org/Activities"/>
	<skos:exactMatch rdf:resource="http://vocab.getty.edu/aat/300123034"/>
	<skos:editorialNote xml:lang="en">PPTechnique</skos:editorialNote>
	<skos:scopeNote xml:lang="en">Forming or arranging in layers.</skos:scopeNote>
</skos:Concept>
<skos:Concept rdf:about="http://partage.vocnet.org/part00459">
	<skos:prefLabel xml:lang="en">marquetry</skos:prefLabel>
	<skos:altLabel xml:lang="hr">ulaganje</skos:altLabel>
	<skos:prefLabel xml:lang="hr">marketarija</skos:prefLabel>
	<skos:prefLabel xml:lang="de">Marketerie</skos:prefLabel>
	<skos:prefLabel xml:lang="sv">intarsia</skos:prefLabel>
	<skos:prefLabel xml:lang="pt">embutido.</skos:prefLabel>
	<skos:prefLabel xml:lang="fi">intarsia</skos:prefLabel>
	<skos:inScheme rdf:resource="http://partage.vocnet.org/Activities"/>
	<skos:narrower rdf:resource="http://partage.vocnet.org/part01239"/>
	<skos:exactMatch rdf:resource="http://vocab.getty.edu/aat/300053853"/>
	<skos:editorialNote xml:lang="en">PPTechnique</skos:editorialNote>
	<skos:scopeNote xml:lang="en">The technique in which small pieces of wood or other materials are overlaid or inlaid onto another wood surface to form a decorative veneer.</skos:scopeNote>
</skos:Concept>
<skos:Concept rdf:about="http://partage.vocnet.org/part00460">
	<skos:prefLabel xml:lang="en">printing (process)</skos:prefLabel>
	<skos:prefLabel xml:lang="pt">impressão</skos:prefLabel>
	<skos:prefLabel xml:lang="de">gedruckt</skos:prefLabel>
	<skos:prefLabel xml:lang="sv">tryckning (process)</skos:prefLabel>
	<skos:prefLabel xml:lang="hr">tiskanje</skos:prefLabel>
	<skos:prefLabel xml:lang="fi">painaminen</skos:prefLabel>
	<skos:inScheme rdf:resource="http://partage.vocnet.org/Activities"/>
	<skos:exactMatch rdf:resource="http://vocab.getty.edu/aat/300053319"/>
	<skos:editorialNote xml:lang="en">PPTechnique</skos:editorialNote>
	<skos:scopeNote xml:lang="en">Various means of reproducing identical copies of graphic matter in a fixed form. Processes by which an image, pictorial or textual, is transferred, usually to paper or cloth, most often by means of a plate, block, stone, or screen. Use also for the making of photographic prints and, with computers, for the production of a paper copy of stored data. For the production of prints in a fine arts context, prefer "printmaking."</skos:scopeNote>
</skos:Concept>
<skos:Concept rdf:about="http://partage.vocnet.org/part00461">
	<skos:prefLabel xml:lang="en">sewing</skos:prefLabel>
	<skos:prefLabel xml:lang="pt">cozer</skos:prefLabel>
	<skos:prefLabel xml:lang="de">genäht</skos:prefLabel>
	<skos:prefLabel xml:lang="sv">sömnad</skos:prefLabel>
	<skos:prefLabel xml:lang="fi">ompelu</skos:prefLabel>
	<skos:prefLabel xml:lang="hr">šivanje</skos:prefLabel>
	<skos:inScheme rdf:resource="http://partage.vocnet.org/Activities"/>
	<skos:broader rdf:resource="http://partage.vocnet.org/part00492"/>
	<skos:exactMatch rdf:resource="http://vocab.getty.edu/aat/300053658"/>
	<skos:editorialNote xml:lang="en">PPTechnique</skos:editorialNote>
	<skos:scopeNote xml:lang="en">Refers to the stitching of materials with thread, cord, or other filament by means of a needle or awl for the purpose of joining, attaching, repairing, enclosing, securing or decorating. In the context of textiles and needleworking, its meaning overlaps with "stitching." In the context of bookbinding, it refers specifically to the joining of leaves or gatherings together one by one by drawing thread or wire backwards and forwards through the back folds of each sheet to attach it to the cords; it is distinct from "stitching," which, in the context of bookbinding, is used for fastening together a number of leaves or gatherings by passing the thread or wire through all of them at once.</skos:scopeNote>
</skos:Concept>
<skos:Concept rdf:about="http://partage.vocnet.org/part00462">
	<skos:prefLabel xml:lang="en">staining</skos:prefLabel>
	<skos:prefLabel xml:lang="pt">manchar</skos:prefLabel>
	<skos:prefLabel xml:lang="de">eingefärbt (Glas)</skos:prefLabel>
	<skos:prefLabel xml:lang="sv">betsning</skos:prefLabel>
	<skos:prefLabel xml:lang="hr">bajcanje</skos:prefLabel>
	<skos:prefLabel xml:lang="fi">värjäys.</skos:prefLabel>
	<skos:inScheme rdf:resource="http://partage.vocnet.org/Activities"/>
	<skos:broader rdf:resource="http://partage.vocnet.org/part00497"/>
	<skos:exactMatch rdf:resource="http://vocab.getty.edu/aat/300053058"/>
	<skos:editorialNote xml:lang="en">PPTechnique</skos:editorialNote>
	<skos:scopeNote xml:lang="en">Process of applying a coloring matter that tinges and penetrates or combines with the substance.</skos:scopeNote>
</skos:Concept>
<skos:Concept rdf:about="http://partage.vocnet.org/part00463">
	<skos:prefLabel xml:lang="en">stitching</skos:prefLabel>
	<skos:prefLabel xml:lang="pt">costura</skos:prefLabel>
	<skos:prefLabel xml:lang="de">geheftet</skos:prefLabel>
	<skos:prefLabel xml:lang="sv">sömnad.</skos:prefLabel>
	<skos:prefLabel xml:lang="hr">šivanje.</skos:prefLabel>
	<skos:prefLabel xml:lang="fi">nidonta</skos:prefLabel>
	<skos:inScheme rdf:resource="http://partage.vocnet.org/Activities"/>
	<skos:exactMatch rdf:resource="http://vocab.getty.edu/aat/300053660"/>
	<skos:editorialNote xml:lang="en">PPTechnique</skos:editorialNote>
	<skos:scopeNote xml:lang="en">Refers to the process of fastening, joining, closing, uniting, mending, or creating ornamentation by stitches, which are the portions of thread left in fabric or another material by the in and out movement of a threaded needle through the thickness or surface of the material, or the loops of thread created on a needle in knitting or other needlework. In the context of textiles and needleworking, its meaning overlaps with "sewing." In the context of bookbinding, it refers to the fastening together a number of leaves or gatherings by passing the thread or wire through all of the sheets at once; it is distinct from "sewing," which, in the context of bookbinding, is used for the joining of leaves or gatherings together one by one by drawing thread or wire backwards and forwards through the back fold of each sheet to attach it to the cords.</skos:scopeNote>
</skos:Concept>
<skos:Concept rdf:about="http://partage.vocnet.org/part00464">
	<skos:prefLabel xml:lang="en">weaving</skos:prefLabel>
	<skos:prefLabel xml:lang="pt">tecer</skos:prefLabel>
	<skos:prefLabel xml:lang="de">gewebt</skos:prefLabel>
	<skos:prefLabel xml:lang="sv">vävning</skos:prefLabel>
	<skos:prefLabel xml:lang="hr">tkanje</skos:prefLabel>
	<skos:prefLabel xml:lang="fi">kudonta</skos:prefLabel>
	<skos:inScheme rdf:resource="http://partage.vocnet.org/Activities"/>
	<skos:broader rdf:resource="http://partage.vocnet.org/part00494"/>
	<skos:exactMatch rdf:resource="http://vocab.getty.edu/aat/300053642"/>
	<skos:scopeNote xml:lang="en">Generally, the process of interlacing strands or strips of various materials, such as cane, textile, or twigs, to make materials or objects such as wicker, cloth, baskets, or wreaths. Specifically used for the process of making textile on a loom or other weaving device by interlacing warp and weft in a particular order.</skos:scopeNote>
	<skos:editorialNote xml:lang="en">PPTechnique</skos:editorialNote>
</skos:Concept>
<skos:Concept rdf:about="http://partage.vocnet.org/part00479">
	<skos:prefLabel xml:lang="en">incising</skos:prefLabel>
	<skos:altLabel xml:lang="pt">gravar</skos:altLabel>
	<skos:prefLabel xml:lang="pt">talhar</skos:prefLabel>
	<skos:altLabel xml:lang="de">gestochen</skos:altLabel>
	<skos:prefLabel xml:lang="de">graviert</skos:prefLabel>
	<skos:altLabel xml:lang="sv">gravering</skos:altLabel>
	<skos:prefLabel xml:lang="sv">ristning</skos:prefLabel>
	<skos:prefLabel xml:lang="hr">urezivanje</skos:prefLabel>
	<skos:prefLabel xml:lang="fi">kaiverrus</skos:prefLabel>
	<skos:inScheme rdf:resource="http://partage.vocnet.org/Activities"/>
	<skos:exactMatch rdf:resource="http://vocab.getty.edu/aat/300053847"/>
	<skos:editorialNote xml:lang="en">PPTechnique</skos:editorialNote>
	<skos:scopeNote xml:lang="en">scope note nicht vorhanden</skos:scopeNote>
</skos:Concept>
<skos:Concept rdf:about="http://partage.vocnet.org/part00480">
	<skos:prefLabel xml:lang="en">coating (process)</skos:prefLabel>
	<skos:inScheme rdf:resource="http://partage.vocnet.org/Activities"/>
	<skos:narrower rdf:resource="http://partage.vocnet.org/part00454"/>
	<skos:narrower rdf:resource="http://partage.vocnet.org/part00456"/>
	<skos:exactMatch rdf:resource="http://vocab.getty.edu/aat/300053772"/>
	<skos:scopeNote xml:lang="en">Covering a surface with a layer of substance, especially a substance that is spread on.</skos:scopeNote>
</skos:Concept>
<skos:Concept rdf:about="http://partage.vocnet.org/part00483">
	<skos:prefLabel xml:lang="en">metallizing</skos:prefLabel>
	<skos:inScheme rdf:resource="http://partage.vocnet.org/Activities"/>
	<skos:narrower rdf:resource="http://partage.vocnet.org/part00455"/>
	<skos:narrower rdf:resource="http://partage.vocnet.org/part00669"/>
	<skos:exactMatch rdf:resource="http://vocab.getty.edu/aat/300053985"/>
	<skos:scopeNote xml:lang="en">The process of coating, treating, or combining with a metal.</skos:scopeNote>
</skos:Concept>
<skos:Concept rdf:about="http://partage.vocnet.org/part00492">
	<skos:prefLabel xml:lang="en">needleworking (process)</skos:prefLabel>
	<skos:inScheme rdf:resource="http://partage.vocnet.org/Activities"/>
	<skos:narrower rdf:resource="http://partage.vocnet.org/part00461"/>
	<skos:narrower rdf:resource="http://partage.vocnet.org/part00647"/>
	<skos:narrower rdf:resource="http://partage.vocnet.org/part01248"/>
	<skos:exactMatch rdf:resource="http://vocab.getty.edu/aat/300053652"/>
	<skos:scopeNote xml:lang="en">Refers to any process or technique done with a needle and thread, such as sewing, stitching, smocking, quilting, and embroidery. In common usage, the term is sometimes used to refer to decorative work rather than plain sewing; however, to distinguish more decorative work from plain sewing, it is less ambiguous to use "fancy needlework" or a specific needlework technique, such as "embroidery.</skos:scopeNote>
	<skos:scopeNote xml:lang="en">PPTechnique</skos:scopeNote>
</skos:Concept>
<skos:Concept rdf:about="http://partage.vocnet.org/part00494">
	<skos:prefLabel xml:lang="en">assembling (additive and joining process)</skos:prefLabel>
	<skos:inScheme rdf:resource="http://partage.vocnet.org/Activities"/>
	<skos:narrower rdf:resource="http://partage.vocnet.org/part00464"/>
	<skos:exactMatch rdf:resource="http://vocab.getty.edu/aat/300053007"/>
	<skos:scopeNote xml:lang="en">Fitting together various parts to make an operative whole.</skos:scopeNote>
</skos:Concept>
<skos:Concept rdf:about="http://partage.vocnet.org/part00497">
	<skos:altLabel xml:lang="en">coloring</skos:altLabel>
	<skos:prefLabel xml:lang="en">colouring</skos:prefLabel>
	<skos:inScheme rdf:resource="http://partage.vocnet.org/Activities"/>
	<skos:narrower rdf:resource="http://partage.vocnet.org/part00462"/>
	<skos:narrower rdf:resource="http://partage.vocnet.org/part00673"/>
	<skos:narrower rdf:resource="http://partage.vocnet.org/part00877"/>
	<skos:exactMatch rdf:resource="http://vocab.getty.edu/aat/300053043"/>
	<skos:scopeNote xml:lang="en">Changing or altering the color of something, whether by penetrating or coating it.</skos:scopeNote>
</skos:Concept>
<skos:Concept rdf:about="http://partage.vocnet.org/part00647">
	<skos:altLabel xml:lang="en">appliqué (technique)</skos:altLabel>
	<skos:prefLabel xml:lang="en">appliqué</skos:prefLabel>
	<skos:prefLabel xml:lang="pt">apliques</skos:prefLabel>
	<skos:prefLabel xml:lang="sv">applikation</skos:prefLabel>
	<skos:altLabel xml:lang="de">aufgenäht</skos:altLabel>
	<skos:prefLabel xml:lang="de">appliziert</skos:prefLabel>
	<skos:prefLabel xml:lang="hr">apliciranje</skos:prefLabel>
	<skos:prefLabel xml:lang="fi">applikointi</skos:prefLabel>
	<skos:inScheme rdf:resource="http://partage.vocnet.org/Activities"/>
	<skos:broader rdf:resource="http://partage.vocnet.org/part00492"/>
	<skos:exactMatch rdf:resource="http://vocab.getty.edu/aat/300053646"/>
	<skos:editorialNote xml:lang="en">PPTechnique</skos:editorialNote>
	<skos:scopeNote xml:lang="en">Technique of forming a design by applying cut out pieces of a material to a ground material; generally associated with needleworking, but also used in ceramics, leatherworking, woodworking, and metalworking.</skos:scopeNote>
</skos:Concept>
<skos:Concept rdf:about="http://partage.vocnet.org/part00648">
	<skos:prefLabel xml:lang="en">batik</skos:prefLabel>
	<skos:prefLabel xml:lang="pt">batik</skos:prefLabel>
	<skos:altLabel xml:lang="de">Batik</skos:altLabel>
	<skos:prefLabel xml:lang="de">gebatikt</skos:prefLabel>
	<skos:prefLabel xml:lang="sv">batik</skos:prefLabel>
	<skos:prefLabel xml:lang="fi">batiikki</skos:prefLabel>
	<skos:prefLabel xml:lang="hr">batik</skos:prefLabel>
	<skos:inScheme rdf:resource="http://partage.vocnet.org/Activities"/>
	<skos:broader rdf:resource="http://partage.vocnet.org/part00649"/>
	<skos:exactMatch rdf:resource="http://vocab.getty.edu/aat/300053050"/>
	<skos:editorialNote xml:lang="en">PPTechnique</skos:editorialNote>
	<skos:scopeNote xml:lang="en">Resist dyeing in which wax is used as the resist.</skos:scopeNote>
</skos:Concept>
<skos:Concept rdf:about="http://partage.vocnet.org/part00649">
	<skos:prefLabel xml:lang="en">resist dyeing</skos:prefLabel>
	<skos:inScheme rdf:resource="http://partage.vocnet.org/Activities"/>
	<skos:narrower rdf:resource="http://partage.vocnet.org/part00648"/>
	<skos:exactMatch rdf:resource="http://vocab.getty.edu/aat/300053053"/>
	<skos:scopeNote xml:lang="en">Dyeing cloth by repeatedly putting a resist on different parts of its pattern and placing it in successive dye baths.</skos:scopeNote>
</skos:Concept>
<skos:Concept rdf:about="http://partage.vocnet.org/part00652">
	<skos:altLabel xml:lang="en">forging (metal forming)</skos:altLabel>
	<skos:prefLabel xml:lang="en">forging</skos:prefLabel>
	<skos:prefLabel xml:lang="pt">forjar</skos:prefLabel>
	<skos:prefLabel xml:lang="de">geschmiedet</skos:prefLabel>
	<skos:prefLabel xml:lang="sv">smide</skos:prefLabel>
	<skos:prefLabel xml:lang="fi">taonta</skos:prefLabel>
	<skos:prefLabel xml:lang="hr">kovanje</skos:prefLabel>
	<skos:inScheme rdf:resource="http://partage.vocnet.org/Activities"/>
	<skos:exactMatch rdf:resource="http://vocab.getty.edu/aat/300054033"/>
	<skos:editorialNote xml:lang="en">PPTechnique</skos:editorialNote>
	<skos:scopeNote xml:lang="en">Forming the shape of a metal object by heating and hammering.</skos:scopeNote>
</skos:Concept>
<skos:Concept rdf:about="http://partage.vocnet.org/part00654">
	<skos:prefLabel xml:lang="en">letterpress printing</skos:prefLabel>
	<skos:prefLabel xml:lang="pt">impressão tipográfica</skos:prefLabel>
	<skos:altLabel xml:lang="de">Typendruck</skos:altLabel>
	<skos:prefLabel xml:lang="de">Buchdruck</skos:prefLabel>
	<skos:prefLabel xml:lang="sv">relieftryckning</skos:prefLabel>
	<skos:prefLabel xml:lang="hr">visoki tisak</skos:prefLabel>
	<skos:prefLabel xml:lang="fi">kohopaino</skos:prefLabel>
	<skos:inScheme rdf:resource="http://partage.vocnet.org/Activities"/>
	<skos:exactMatch rdf:resource="http://vocab.getty.edu/aat/300178926"/>
	<skos:editorialNote xml:lang="de">PPTechnique</skos:editorialNote>
	<skos:scopeNote xml:lang="en">Printing from raised and inked type, distinguished from lithographic or intaglio printing, particularly in the context of book and other text printing.</skos:scopeNote>
</skos:Concept>
<skos:Concept rdf:about="http://partage.vocnet.org/part00656">
	<skos:prefLabel xml:lang="en">matting (supporting)</skos:prefLabel>
	<skos:prefLabel xml:lang="pt">passe-partout</skos:prefLabel>
	<skos:prefLabel xml:lang="de">verstärkt</skos:prefLabel>
	<skos:prefLabel xml:lang="fi">tukeminen</skos:prefLabel>
	<skos:prefLabel xml:lang="hr">opremanje (slike)</skos:prefLabel>
	<skos:inScheme rdf:resource="http://partage.vocnet.org/Activities"/>
	<skos:broader rdf:resource="http://partage.vocnet.org/part00657"/>
	<skos:exactMatch rdf:resource="http://vocab.getty.edu/aat/300053766"/>
	<skos:editorialNote xml:lang="en">PPTechnique</skos:editorialNote>
	<skos:scopeNote xml:lang="en">Securing of a work of art, document, or other generally flat object within a mat for support, protection, or display.</skos:scopeNote>
</skos:Concept>
<skos:Concept rdf:about="http://partage.vocnet.org/part00657">
	<skos:prefLabel xml:lang="en">supporting</skos:prefLabel>
	<skos:inScheme rdf:resource="http://partage.vocnet.org/Activities"/>
	<skos:broader rdf:resource="http://partage.vocnet.org/part00658"/>
	<skos:narrower rdf:resource="http://partage.vocnet.org/part00656"/>
	<skos:narrower rdf:resource="http://partage.vocnet.org/part00661"/>
	<skos:exactMatch rdf:resource="http://vocab.getty.edu/aat/300053768"/>
</skos:Concept>
<skos:Concept rdf:about="http://partage.vocnet.org/part00658">
	<skos:prefLabel xml:lang="en">strengthening</skos:prefLabel>
	<skos:inScheme rdf:resource="http://partage.vocnet.org/Activities"/>
	<skos:broader rdf:resource="http://partage.vocnet.org/part00659"/>
	<skos:narrower rdf:resource="http://partage.vocnet.org/part00657"/>
	<skos:exactMatch rdf:resource="http://vocab.getty.edu/aat/300053762"/>
</skos:Concept>
<skos:Concept rdf:about="http://partage.vocnet.org/part00659">
	<skos:prefLabel xml:lang="en">stabilizing</skos:prefLabel>
	<skos:inScheme rdf:resource="http://partage.vocnet.org/Activities"/>
	<skos:narrower rdf:resource="http://partage.vocnet.org/part00658"/>
	<skos:exactMatch rdf:resource="http://vocab.getty.edu/aat/300163757"/>
	<skos:scopeNote xml:lang="en">The process of making stable, or maintaining stability of an object, such as a ship or airplane, often by means of a stabilizer.</skos:scopeNote>
</skos:Concept>
<skos:Concept rdf:about="http://partage.vocnet.org/part00660">
	<skos:altLabel xml:lang="en">molding (forming)</skos:altLabel>
	<skos:altLabel xml:lang="en">molding</skos:altLabel>
	<skos:prefLabel xml:lang="pt">moldar</skos:prefLabel>
	<skos:prefLabel xml:lang="de">modelliert</skos:prefLabel>
	<skos:altLabel xml:lang="sv">pressning</skos:altLabel>
	<skos:prefLabel xml:lang="sv">gjutning</skos:prefLabel>
	<skos:prefLabel xml:lang="en">moulding</skos:prefLabel>
	<skos:prefLabel xml:lang="hr">oblikovanje kalupom</skos:prefLabel>
	<skos:prefLabel xml:lang="fi">muovailu</skos:prefLabel>
	<skos:inScheme rdf:resource="http://partage.vocnet.org/Activities"/>
	<skos:broader rdf:resource="http://partage.vocnet.org/part01037"/>
	<skos:narrower rdf:resource="http://partage.vocnet.org/part01241"/>
	<skos:exactMatch rdf:resource="http://vocab.getty.edu/aat/300053134"/>
	<skos:editorialNote xml:lang="en">PPTechnique</skos:editorialNote>
	<skos:scopeNote xml:lang="en">Giving form to something by use of a mold; usually refers to pressing a material into the mold, as distinct from pouring liquid material into the mold, for which prefer "casting</skos:scopeNote>
</skos:Concept>
<skos:Concept rdf:about="http://partage.vocnet.org/part00661">
	<skos:prefLabel xml:lang="en">mounting</skos:prefLabel>
	<skos:prefLabel xml:lang="pt">montar</skos:prefLabel>
	<skos:altLabel xml:lang="de">aufgelegt</skos:altLabel>
	<skos:prefLabel xml:lang="de">montiert</skos:prefLabel>
	<skos:prefLabel xml:lang="sv">montering</skos:prefLabel>
	<skos:prefLabel xml:lang="fi">kiinnitys</skos:prefLabel>
	<skos:prefLabel xml:lang="hr">montiranje</skos:prefLabel>
	<skos:inScheme rdf:resource="http://partage.vocnet.org/Activities"/>
	<skos:broader rdf:resource="http://partage.vocnet.org/part00657"/>
	<skos:exactMatch rdf:resource="http://vocab.getty.edu/aat/300081370"/>
	<skos:editorialNote xml:lang="en">PPTechnique</skos:editorialNote>
	<skos:scopeNote xml:lang="en">Attaching to a secondary support; as in attaching a paper artifact to a stiff board, sometimes preparatory to matting.</skos:scopeNote>
</skos:Concept>
<skos:Concept rdf:about="http://partage.vocnet.org/part00662">
	<skos:prefLabel xml:lang="en">niello (technique)</skos:prefLabel>
	<skos:prefLabel xml:lang="pt">niello</skos:prefLabel>
	<skos:prefLabel xml:lang="de">Niello</skos:prefLabel>
	<skos:prefLabel xml:lang="sv">niello (teknik)</skos:prefLabel>
	<skos:prefLabel xml:lang="hr">niello</skos:prefLabel>
	<skos:prefLabel xml:lang="fi">niello</skos:prefLabel>
	<skos:inScheme rdf:resource="http://partage.vocnet.org/Activities"/>
	<skos:broader rdf:resource="http://partage.vocnet.org/part00457"/>
	<skos:exactMatch rdf:resource="http://vocab.getty.edu/aat/300054022"/>
	<skos:editorialNote xml:lang="en">PPTechnique</skos:editorialNote>
	<skos:scopeNote xml:lang="en">A technique of decorating metal, usually gold or silver, by engraving it with designs that are then filled with a black inlay. Prints are sometimes made from the engraved metal before inlaying.</skos:scopeNote>
</skos:Concept>
<skos:Concept rdf:about="http://partage.vocnet.org/part00663">
	<skos:prefLabel xml:lang="en">plating (metal coating)</skos:prefLabel>
	<skos:altLabel xml:lang="pt">banho de prata ou ouro</skos:altLabel>
	<skos:prefLabel xml:lang="pt">revestir</skos:prefLabel>
	<skos:prefLabel xml:lang="de">mit Metall überzogen</skos:prefLabel>
	<skos:prefLabel xml:lang="sv">plätering (metall överdrag)</skos:prefLabel>
	<skos:prefLabel xml:lang="fi">pinnoitus</skos:prefLabel>
	<skos:prefLabel xml:lang="hr">prevlačenje (metala)</skos:prefLabel>
	<skos:inScheme rdf:resource="http://partage.vocnet.org/Activities"/>
	<skos:exactMatch rdf:resource="http://vocab.getty.edu/aat/300053991"/>
	<skos:editorialNote xml:lang="en">PPTechnique</skos:editorialNote>
	<skos:scopeNote xml:lang="en">no scope note in AAT</skos:scopeNote>
</skos:Concept>
<skos:Concept rdf:about="http://partage.vocnet.org/part00664">
	<skos:prefLabel xml:lang="en">painting (image-making)</skos:prefLabel>
	<skos:prefLabel xml:lang="de">gemalt</skos:prefLabel>
	<skos:prefLabel xml:lang="pt">pintar</skos:prefLabel>
	<skos:prefLabel xml:lang="sv">måleri (bildskapande)</skos:prefLabel>
	<skos:prefLabel xml:lang="fi">maalaus</skos:prefLabel>
	<skos:prefLabel xml:lang="hr">slikanje</skos:prefLabel>
	<skos:inScheme rdf:resource="http://partage.vocnet.org/Activities"/>
	<skos:exactMatch rdf:resource="http://vocab.getty.edu/aat/300054216"/>
	<skos:editorialNote xml:lang="en">PPTechnique</skos:editorialNote>
	<skos:scopeNote xml:lang="en">The art and practice of applying pigments suspended in water, oil, egg yolk, molten wax, or other liquid to a surface to create an expressive or communicative image. For the application of paint primarily to protect a surface or add a general color, use "painting (coating)."</skos:scopeNote>
</skos:Concept>
<skos:Concept rdf:about="http://partage.vocnet.org/part00665">
	<skos:prefLabel xml:lang="en">polishing</skos:prefLabel>
	<skos:prefLabel xml:lang="pt">polir</skos:prefLabel>
	<skos:prefLabel xml:lang="de">poliert</skos:prefLabel>
	<skos:prefLabel xml:lang="sv">polering</skos:prefLabel>
	<skos:prefLabel xml:lang="hr">poliranje</skos:prefLabel>
	<skos:prefLabel xml:lang="fi">kiillotus</skos:prefLabel>
	<skos:inScheme rdf:resource="http://partage.vocnet.org/Activities"/>
	<skos:broader rdf:resource="http://partage.vocnet.org/part01026"/>
	<skos:exactMatch rdf:resource="http://vocab.getty.edu/aat/300053867"/>
	<skos:scopeNote xml:lang="en">PPTechnique</skos:scopeNote>
	<skos:scopeNote xml:lang="en">no scope note in AAT</skos:scopeNote>
</skos:Concept>
<skos:Concept rdf:about="http://partage.vocnet.org/part00666">
	<skos:prefLabel xml:lang="en">pressing</skos:prefLabel>
	<skos:prefLabel xml:lang="pt">prensar</skos:prefLabel>
	<skos:prefLabel xml:lang="de">gepresst</skos:prefLabel>
	<skos:prefLabel xml:lang="sv">pressning.</skos:prefLabel>
	<skos:prefLabel xml:lang="fi">prässäys</skos:prefLabel>
	<skos:prefLabel xml:lang="hr">tiještenje</skos:prefLabel>
	<skos:inScheme rdf:resource="http://partage.vocnet.org/Activities"/>
	<skos:broader rdf:resource="http://partage.vocnet.org/part01037"/>
	<skos:exactMatch rdf:resource="http://vocab.getty.edu/aat/300053136"/>
	<skos:editorialNote xml:lang="en">PPTechnique</skos:editorialNote>
	<skos:scopeNote xml:lang="en">Forming by means of pressure, especially a steady, overall pressure.</skos:scopeNote>
</skos:Concept>
<skos:Concept rdf:about="http://partage.vocnet.org/part00667">
	<skos:altLabel xml:lang="en">punching (surface marking technique)</skos:altLabel>
	<skos:prefLabel xml:lang="en">punching</skos:prefLabel>
	<skos:prefLabel xml:lang="pt">pontear</skos:prefLabel>
	<skos:prefLabel xml:lang="de">punziert</skos:prefLabel>
	<skos:prefLabel xml:lang="sv">stansning (ytskapande teknik)</skos:prefLabel>
	<skos:prefLabel xml:lang="fi">lyöminen</skos:prefLabel>
	<skos:prefLabel xml:lang="hr">punciranje</skos:prefLabel>
	<skos:inScheme rdf:resource="http://partage.vocnet.org/Activities"/>
	<skos:exactMatch rdf:resource="http://vocab.getty.edu/aat/300235631"/>
	<skos:editorialNote xml:lang="en">PPTechnique</skos:editorialNote>
	<skos:scopeNote xml:lang="en">Technique of decorating a surface with a pattern consisting of small depressions produced by use of punches.</skos:scopeNote>
</skos:Concept>
<skos:Concept rdf:about="http://partage.vocnet.org/part00668">
	<skos:prefLabel xml:lang="en">sgraffito (technique)</skos:prefLabel>
	<skos:prefLabel xml:lang="pt">sgraffito</skos:prefLabel>
	<skos:prefLabel xml:lang="de">Sgraffito</skos:prefLabel>
	<skos:prefLabel xml:lang="sv">sgraffito (teknik)</skos:prefLabel>
	<skos:prefLabel xml:lang="hr">sgraffito</skos:prefLabel>
	<skos:prefLabel xml:lang="fi">sgraffito</skos:prefLabel>
	<skos:inScheme rdf:resource="http://partage.vocnet.org/Activities"/>
	<skos:exactMatch rdf:resource="http://vocab.getty.edu/aat/300266416"/>
	<skos:editorialNote xml:lang="en">PPTechnique</skos:editorialNote>
	<skos:scopeNote xml:lang="en">The decorative technique of scratching through one surface layer, such as on a wall, slip on a pot, or the surface of glass, so as to reveal a layer beneath. For non-decorative, casual, or defacing marks on walls or other surfaces ancient or modern, use "graffiti."</skos:scopeNote>
</skos:Concept>
<skos:Concept rdf:about="http://partage.vocnet.org/part00669">
	<skos:prefLabel xml:lang="en">silvering</skos:prefLabel>
	<skos:prefLabel xml:lang="pt">prateado</skos:prefLabel>
	<skos:prefLabel xml:lang="de">versilbert</skos:prefLabel>
	<skos:prefLabel xml:lang="sv">försilvring</skos:prefLabel>
	<skos:prefLabel xml:lang="fi">hopeinti</skos:prefLabel>
	<skos:prefLabel xml:lang="hr">posrebrivanje</skos:prefLabel>
	<skos:inScheme rdf:resource="http://partage.vocnet.org/Activities"/>
	<skos:broader rdf:resource="http://partage.vocnet.org/part00483"/>
	<skos:exactMatch rdf:resource="http://vocab.getty.edu/aat/300053989"/>
	<skos:scopeNote xml:lang="en">The act or process of covering with silver.</skos:scopeNote>
	<skos:editorialNote xml:lang="en">PPTechnique</skos:editorialNote>
</skos:Concept>
<skos:Concept rdf:about="http://partage.vocnet.org/part00670">
	<skos:prefLabel xml:lang="en">slab method</skos:prefLabel>
	<skos:prefLabel xml:lang="pt">placa</skos:prefLabel>
	<skos:prefLabel xml:lang="de">Plattentechnik</skos:prefLabel>
	<skos:prefLabel xml:lang="hr">oblikovanje u pločama</skos:prefLabel>
	<skos:prefLabel xml:lang="fi">laattatekniikka</skos:prefLabel>
	<skos:inScheme rdf:resource="http://partage.vocnet.org/Activities"/>
	<skos:exactMatch rdf:resource="http://vocab.getty.edu/aat/300053905"/>
	<skos:editorialNote xml:lang="en">PPTechnique</skos:editorialNote>
	<skos:scopeNote xml:lang="en">A technique of forming pottery by hand, in which a mass of wet clay is flattened to a slab with a rolling pin. The slab may be beaten into various shapes, joined to other slabs with slip, or paddled over a wood form.</skos:scopeNote>
</skos:Concept>
<skos:Concept rdf:about="http://partage.vocnet.org/part00671">
	<skos:prefLabel xml:lang="en">stamping (marking)</skos:prefLabel>
	<skos:prefLabel xml:lang="pt">estampar</skos:prefLabel>
	<skos:prefLabel xml:lang="de">gestempelt</skos:prefLabel>
	<skos:prefLabel xml:lang="sv">stämpling</skos:prefLabel>
	<skos:prefLabel xml:lang="fi">leimaus</skos:prefLabel>
	<skos:prefLabel xml:lang="hr">otiskivanje</skos:prefLabel>
	<skos:inScheme rdf:resource="http://partage.vocnet.org/Activities"/>
	<skos:exactMatch rdf:resource="http://vocab.getty.edu/aat/300239001"/>
	<skos:editorialNote xml:lang="en">PPTechnique</skos:editorialNote>
	<skos:scopeNote xml:lang="en">Marking the surface of an object by applying pressure with a tool, for example, transferring an ink mark to paper or embossing soft clay; also, applying preprinted labels such as postage stamps that substitute for official stamped marks. In bookbinding, distinguished from "blocking", in which pressure is applied by a machine.</skos:scopeNote>
</skos:Concept>
<skos:Concept rdf:about="http://partage.vocnet.org/part00672">
	<skos:prefLabel xml:lang="en">throwing (pottery technique)</skos:prefLabel>
	<skos:prefLabel xml:lang="pt">tornear</skos:prefLabel>
	<skos:prefLabel xml:lang="de">gedreht (Töpferscheibe)</skos:prefLabel>
	<skos:prefLabel xml:lang="sv">drejning (keramisk teknik)</skos:prefLabel>
	<skos:prefLabel xml:lang="fi">dreijaus</skos:prefLabel>
	<skos:prefLabel xml:lang="hr">vrtenje na lončarskom kolu</skos:prefLabel>
	<skos:inScheme rdf:resource="http://partage.vocnet.org/Activities"/>
	<skos:exactMatch rdf:resource="http://vocab.getty.edu/aat/300053908"/>
	<skos:scopeNote xml:lang="en">The process of making a ceramic object on a potter's wheel.</skos:scopeNote>
	<skos:editorialNote xml:lang="en">PPTechnique</skos:editorialNote>
</skos:Concept>
<skos:Concept rdf:about="http://partage.vocnet.org/part00673">
	<skos:prefLabel xml:lang="en">tinting</skos:prefLabel>
	<skos:prefLabel xml:lang="pt">tingir.</skos:prefLabel>
	<skos:prefLabel xml:lang="de">getönt</skos:prefLabel>
	<skos:prefLabel xml:lang="sv">tintning</skos:prefLabel>
	<skos:altLabel xml:lang="hr">toniranje</skos:altLabel>
	<skos:prefLabel xml:lang="hr">nijansiranje</skos:prefLabel>
	<skos:prefLabel xml:lang="fi">sävytys</skos:prefLabel>
	<skos:inScheme rdf:resource="http://partage.vocnet.org/Activities"/>
	<skos:broader rdf:resource="http://partage.vocnet.org/part00497"/>
	<skos:exactMatch rdf:resource="http://vocab.getty.edu/aat/300053059"/>
	<skos:editorialNote xml:lang="en">PPTechnique</skos:editorialNote>
	<skos:scopeNote xml:lang="de">no scope note available</skos:scopeNote>
</skos:Concept>
<skos:Concept rdf:about="http://partage.vocnet.org/part00877">
	<skos:prefLabel xml:lang="en">dyeing</skos:prefLabel>
	<skos:prefLabel xml:lang="pt">tingir</skos:prefLabel>
	<skos:altLabel xml:lang="de">eingefärbt</skos:altLabel>
	<skos:prefLabel xml:lang="de">gefärbt (Textilien)</skos:prefLabel>
	<skos:prefLabel xml:lang="sv">färgning</skos:prefLabel>
	<skos:prefLabel xml:lang="fi">värjäys</skos:prefLabel>
	<skos:prefLabel xml:lang="hr">bojenje (tkanine)</skos:prefLabel>
	<skos:inScheme rdf:resource="http://partage.vocnet.org/Activities"/>
	<skos:broader rdf:resource="http://partage.vocnet.org/part00497"/>
	<skos:exactMatch rdf:resource="http://vocab.getty.edu/aat/300053049"/>
	<skos:editorialNote xml:lang="en">PPTechnique</skos:editorialNote>
	<skos:scopeNote xml:lang="en">Process of applying a coloring matter that is in a solution or fine dispersion so that at least some of the coloring matter is taken up by the substance.</skos:scopeNote>
</skos:Concept>
<skos:Concept rdf:about="http://partage.vocnet.org/part00878">
	<skos:prefLabel xml:lang="en">photography (image making)</skos:prefLabel>
	<skos:altLabel xml:lang="en">photography</skos:altLabel>
	<skos:prefLabel xml:lang="pt">fotografar</skos:prefLabel>
	<skos:prefLabel xml:lang="de">Fotografie (Technik)</skos:prefLabel>
	<skos:prefLabel xml:lang="sv">fotografering (bildskapande)</skos:prefLabel>
	<skos:prefLabel xml:lang="hr">fotografiranje</skos:prefLabel>
	<skos:prefLabel xml:lang="fi">valokuvaus</skos:prefLabel>
	<skos:inScheme rdf:resource="http://partage.vocnet.org/Activities"/>
	<skos:exactMatch rdf:resource="http://vocab.getty.edu/aat/300054225"/>
	<skos:editorialNote xml:lang="en">PPTechnique</skos:editorialNote>
	<skos:scopeNote xml:lang="en">The art or process of making photographs, which are pictures produced by means of the chemical action of light on a sensitive film, glass, paper, or metal.</skos:scopeNote>
</skos:Concept>
<skos:Concept rdf:about="http://partage.vocnet.org/part00879">
	<skos:prefLabel xml:lang="en">toning (photography)</skos:prefLabel>
	<skos:prefLabel xml:lang="pt">virador</skos:prefLabel>
	<skos:prefLabel xml:lang="de">getont (Fotografie)</skos:prefLabel>
	<skos:prefLabel xml:lang="sv">toning (fotografi)</skos:prefLabel>
	<skos:altLabel xml:lang="pt">viragem</skos:altLabel>
	<skos:prefLabel xml:lang="hr">toniranje (fotografije)</skos:prefLabel>
	<skos:prefLabel xml:lang="fi">toonaus</skos:prefLabel>
	<skos:inScheme rdf:resource="http://partage.vocnet.org/Activities"/>
	<skos:broader rdf:resource="http://partage.vocnet.org/part01020"/>
	<skos:exactMatch rdf:resource="http://vocab.getty.edu/aat/300053423"/>
	<skos:editorialNote xml:lang="en">PPTechnique</skos:editorialNote>
	<skos:scopeNote xml:lang="en">In photographic processing, converting some or all of the silver in a black-and-white image using inorganic salts or mordant dyes, and usually altering the overall tone of the image.</skos:scopeNote>
</skos:Concept>
<skos:Concept rdf:about="http://partage.vocnet.org/part00880">
	<skos:prefLabel xml:lang="en">sculpting</skos:prefLabel>
	<skos:prefLabel xml:lang="pt">esculpir</skos:prefLabel>
	<skos:prefLabel xml:lang="de">Skulptur (Technik)</skos:prefLabel>
	<skos:prefLabel xml:lang="sv">skulptering</skos:prefLabel>
	<skos:prefLabel xml:lang="hr">oblikovanje (skulpture)</skos:prefLabel>
	<skos:prefLabel xml:lang="fi">veistäminen</skos:prefLabel>
	<skos:inScheme rdf:resource="http://partage.vocnet.org/Activities"/>
	<skos:narrower rdf:resource="http://partage.vocnet.org/part01230"/>
	<skos:exactMatch rdf:resource="http://vocab.getty.edu/aat/300264383"/>
	<skos:editorialNote xml:lang="en">PPTechnique</skos:editorialNote>
	<skos:scopeNote xml:lang="en">Refers to the process or branch of fine art concerned with creating sculpture, which are three-dimensional works. It refers particularly to carving or engraving a hard material, or with molding or casting a malleable material, so as to produce designs or figures in relief, in intaglio, or in the round. It is typically used to refer to the production of large or medium-sized objects in stone, clay, or bronze. The production of small objects in bronze or stone is typically referred to by a specific term, such as "stone carving" or "die sinking." The production of sculpture in wood or ivory is typically referred to as "carving," even though the finished work in these materials may be called "sculpture (visual work)."</skos:scopeNote>
</skos:Concept>
<skos:Concept rdf:about="http://partage.vocnet.org/part00881">
	<skos:prefLabel xml:lang="en">drawing (image-making)</skos:prefLabel>
	<skos:prefLabel xml:lang="pt">desenhar</skos:prefLabel>
	<skos:prefLabel xml:lang="de">gezeichnet</skos:prefLabel>
	<skos:prefLabel xml:lang="sv">teckning (bildskapande)</skos:prefLabel>
	<skos:prefLabel xml:lang="hr">crtanje</skos:prefLabel>
	<skos:prefLabel xml:lang="fi">piirustus</skos:prefLabel>
	<skos:inScheme rdf:resource="http://partage.vocnet.org/Activities"/>
	<skos:exactMatch rdf:resource="http://vocab.getty.edu/aat/300054196"/>
	<skos:editorialNote xml:lang="en">PPTechnique</skos:editorialNote>
	<skos:scopeNote xml:lang="en">Producing visible forms primarily by delineation, usually by the direct application of material or instrument to the surface of the support.</skos:scopeNote>
</skos:Concept>
<skos:Concept rdf:about="http://partage.vocnet.org/part01020">
	<skos:prefLabel xml:lang="en">photographic techniques</skos:prefLabel>
	<skos:inScheme rdf:resource="http://partage.vocnet.org/Activities"/>
	<skos:narrower rdf:resource="http://partage.vocnet.org/part00879"/>
	<skos:narrower rdf:resource="http://partage.vocnet.org/part01231"/>
	<skos:exactMatch rdf:resource="http://vocab.getty.edu/aat/300134334"/>
	<skos:scopeNote xml:lang="en">Use with regard to specialized procedures related to how a photograph is taken or composed, or is manipulated during or after processing. Use "photographic processes" for the procedures by which light-sensitive materials are made to produce an image.</skos:scopeNote>
</skos:Concept>
<skos:Concept rdf:about="http://partage.vocnet.org/part01026">
	<skos:prefLabel xml:lang="en">finishing (process)</skos:prefLabel>
	<skos:inScheme rdf:resource="http://partage.vocnet.org/Activities"/>
	<skos:narrower rdf:resource="http://partage.vocnet.org/part00665"/>
	<skos:exactMatch rdf:resource="http://vocab.getty.edu/aat/300053844"/>
	<skos:scopeNote xml:lang="en">Refers generally to processes that complete an object, treatment, or work, including the chemical, electrolytic, and mechanical application of finishes. In the context of bookbinding, refers to that sequence of processes carried out on a book and its binding after forwarding, up to the point of attaching its cover. In case binding, where the cover is attached prior to the applicaiton of lettering or decoration, the attachment of the cover is part of the forwarding, not the finishing. In the context of leather manufacture, all the processes carried out on the leather after tanning. In the context of papermaking, all the processes carried out on the paper after it leaves the papermaking machine.</skos:scopeNote>
</skos:Concept>
<skos:Concept rdf:about="http://partage.vocnet.org/part01037">
	<skos:prefLabel xml:lang="en">forming</skos:prefLabel>
	<skos:inScheme rdf:resource="http://partage.vocnet.org/Activities"/>
	<skos:narrower rdf:resource="http://partage.vocnet.org/part00450"/>
	<skos:narrower rdf:resource="http://partage.vocnet.org/part00660"/>
	<skos:narrower rdf:resource="http://partage.vocnet.org/part00666"/>
	<skos:narrower rdf:resource="http://partage.vocnet.org/part01119"/>
	<skos:narrower rdf:resource="http://partage.vocnet.org/part01246"/>
	<skos:exactMatch rdf:resource="http://vocab.getty.edu/aat/300053098"/>
	<skos:scopeNote xml:lang="en">Shaping, molding, or fashioning into a certain state or condition.</skos:scopeNote>
	<skos:editorialNote xml:lang="en">PPTechnique</skos:editorialNote>
</skos:Concept>
<skos:Concept rdf:about="http://partage.vocnet.org/part01119">
	<skos:prefLabel xml:lang="en">bending</skos:prefLabel>
	<skos:inScheme rdf:resource="http://partage.vocnet.org/Activities"/>
	<skos:broader rdf:resource="http://partage.vocnet.org/part01037"/>
	<skos:exactMatch rdf:resource="http://vocab.getty.edu/aat/300053101"/>
	<skos:editorialNote xml:lang="en">PPTechnique</skos:editorialNote>
	<skos:scopeNote xml:lang="en">Turning, pressing, or forcing with stress concentrated at specific points in order to form angular or curved forms.</skos:scopeNote>
</skos:Concept>
<skos:Concept rdf:about="http://partage.vocnet.org/part01225">
	<skos:prefLabel xml:lang="en">metalworking</skos:prefLabel>
	<skos:inScheme rdf:resource="http://partage.vocnet.org/Activities"/>
	<skos:exactMatch rdf:resource="http://vocab.getty.edu/aat/300053946"/>
	<skos:editorialNote xml:lang="en">PPTechnique</skos:editorialNote>
	<skos:scopeNote xml:lang="en">The act or process of shaping things out of metal or of decorating with metal.</skos:scopeNote>
</skos:Concept>
<skos:Concept rdf:about="http://partage.vocnet.org/part01226">
	<skos:prefLabel xml:lang="en">granulation</skos:prefLabel>
	<skos:inScheme rdf:resource="http://partage.vocnet.org/Activities"/>
	<skos:exactMatch rdf:resource="http://vocab.getty.edu/aat/300054021"/>
	<skos:editorialNote xml:lang="en">PPTechnique</skos:editorialNote>
	<skos:scopeNote xml:lang="en">Technique of jewelry decoration in which minute grains of gold or silver are applied to an object of the same metal; in ancient times achieved without using solder, in modern times done with solder.</skos:scopeNote>
</skos:Concept>
<skos:Concept rdf:about="http://partage.vocnet.org/part01227">
	<skos:prefLabel xml:lang="en">pâte-sur-pâte</skos:prefLabel>
	<skos:inScheme rdf:resource="http://partage.vocnet.org/Activities"/>
	<skos:exactMatch rdf:resource="http://vocab.getty.edu/aat/300179400"/>
	<skos:editorialNote xml:lang="en">PPTechnique</skos:editorialNote>
	<skos:scopeNote xml:lang="en">An expensive and difficult method of decorating porcelain in which designs are painted in successive layers of white porcelain slip applied in slight relief on vessels or plaques of unfired clay and lightly carved with metal instruments before first firing to achieve a cameo-like effect. The pieces are then glazed and fired again. The technique developed at S\u00e8vres in the mid-19th century; it was most effectively practiced there and at the Minton factory by Marc-Louis-Emmanuel Solon.</skos:scopeNote>
</skos:Concept>
<skos:Concept rdf:about="http://partage.vocnet.org/part01229">
	<skos:prefLabel xml:lang="en">relief (sculpture techniques)</skos:prefLabel>
	<skos:inScheme rdf:resource="http://partage.vocnet.org/Activities"/>
	<skos:broader rdf:resource="http://partage.vocnet.org/part01230"/>
	<skos:exactMatch rdf:resource="http://vocab.getty.edu/aat/300053622"/>
	<skos:editorialNote xml:lang="en">PPTechnique</skos:editorialNote>
	<skos:scopeNote xml:lang="en">Use to describe a surface that has been carved, molded, or stamped so that an image or design projects from or is sunk into a continuous surface.</skos:scopeNote>
</skos:Concept>
<skos:Concept rdf:about="http://partage.vocnet.org/part01230">
	<skos:prefLabel xml:lang="en">sculpture techniques</skos:prefLabel>
	<skos:inScheme rdf:resource="http://partage.vocnet.org/Activities"/>
	<skos:broader rdf:resource="http://partage.vocnet.org/part00880"/>
	<skos:narrower rdf:resource="http://partage.vocnet.org/part01229"/>
	<skos:exactMatch rdf:resource="http://vocab.getty.edu/aat/300053618"/>
</skos:Concept>
<skos:Concept rdf:about="http://partage.vocnet.org/part01231">
	<skos:prefLabel xml:lang="de">Solarisation</skos:prefLabel>
	<skos:prefLabel xml:lang="en">solarisation</skos:prefLabel>
	<skos:altLabel xml:lang="en">solarization</skos:altLabel>
	<skos:prefLabel xml:lang="hr">solarizacija</skos:prefLabel>
	<skos:inScheme rdf:resource="http://partage.vocnet.org/Activities"/>
	<skos:broader rdf:resource="http://partage.vocnet.org/part01020"/>
	<skos:exactMatch rdf:resource="http://vocab.getty.edu/aat/300135005"/>
	<skos:editorialNote xml:lang="en">PPTechnique</skos:editorialNote>
	<skos:scopeNote xml:lang="en">Tone reversal in photographs caused by massive overexposure of the photographic emulsion to light. True solarization rarely occurs in modern emulsions, and is most commonly seen in early daguerreotypes. For the similar effect that occurs with exposure of negatives or emulsions to bright light during development, rather than at the moment of camera exposure, as was used by the Surrealists, use "Sabattier effect."</skos:scopeNote>
</skos:Concept>
<skos:Concept rdf:about="http://partage.vocnet.org/part01232">
	<skos:prefLabel xml:lang="hr">slijepi tisak</skos:prefLabel>
	<skos:prefLabel xml:lang="de">Blinddruck</skos:prefLabel>
	<skos:prefLabel xml:lang="en">blind embossing</skos:prefLabel>
	<skos:inScheme rdf:resource="http://partage.vocnet.org/Activities"/>
	<skos:broader rdf:resource="http://partage.vocnet.org/part00453"/>
	<skos:exactMatch rdf:resource="http://vocab.getty.edu/aat/300178639"/>
	<skos:editorialNote xml:lang="en">PPTechnique</skos:editorialNote>
	<skos:scopeNote xml:lang="en">Creating raised letters or designs without ink, foil, or other color.</skos:scopeNote>
</skos:Concept>
<skos:Concept rdf:about="http://partage.vocnet.org/part01233">
	<skos:prefLabel xml:lang="en">engraving (action)</skos:prefLabel>
	<skos:inScheme rdf:resource="http://partage.vocnet.org/Activities"/>
	<skos:exactMatch rdf:resource="http://vocab.getty.edu/aat/300053829"/>
	<skos:editorialNote xml:lang="en">PPTechnique</skos:editorialNote>
	<skos:scopeNote xml:lang="en">Creating marks on the surface of a hard material, such as metal or glass, by incising with a sharp tool, when the designs or images created are for their own sake and not to be printed from. For printing processes that involve this technique plus intaglio printing from the surface, use "engraving (printing process)."</skos:scopeNote>
</skos:Concept>
<skos:Concept rdf:about="http://partage.vocnet.org/part01234">
	<skos:prefLabel xml:lang="en">engraving (printing process)</skos:prefLabel>
	<skos:prefLabel xml:lang="hr">graviranje</skos:prefLabel>
	<skos:altLabel xml:lang="de">gestochen (Druckplatte)</skos:altLabel>
	<skos:prefLabel xml:lang="de">gestochen (Druckvorgang)</skos:prefLabel>
	<skos:inScheme rdf:resource="http://partage.vocnet.org/Activities"/>
	<skos:exactMatch rdf:resource="http://vocab.getty.edu/aat/300053225"/>
	<skos:editorialNote xml:lang="en">PPTechnique</skos:editorialNote>
	<skos:scopeNote xml:lang="en">The intaglio process in which the design is incised into a printing plate, usually a flat copper plate, with the aid of a graver or burin that is held in the palm of the hand and pushed against the copper to cut lines comprising V-shaped grooves. The plate is then inked up, wiped so that ink is retained in the grooves and then forced out under the pressure of the printing process to create lines on the paper. The technique was first developed in the early 15th century in Germany, probably by goldsmiths who wished to keep records of the designs they had engraved on their wares. The process is distinct from "wood engraving (process)," which is a process for relief printing; "wood cut (process)" refers to engraving wood blocks for printing. Historically, "engraving" has sometimes been used incorrectly to refer to all printmaking processes, particulalry any process employing printing plates. For the single step of incising an inscription or design into any surface, not only a printing plate, see "engraving (action)."</skos:scopeNote>
</skos:Concept>
<skos:Concept rdf:about="http://partage.vocnet.org/part01236">
	<skos:prefLabel xml:lang="de">radiert (Druckvorgang)</skos:prefLabel>
	<skos:altLabel xml:lang="de">radiert (Druckplatte)</skos:altLabel>
	<skos:prefLabel xml:lang="en">etching (printing process)</skos:prefLabel>
	<skos:inScheme rdf:resource="http://partage.vocnet.org/Activities"/>
	<skos:exactMatch rdf:resource="http://vocab.getty.edu/aat/300053241"/>
	<skos:editorialNote xml:lang="en">PPTechnique</skos:editorialNote>
	<skos:scopeNote xml:lang="en">ntaglio process in which the design is worked into an acid-resistant substance coating the metal printing plate; the plate is then exposed to acid, which etches the plate where the metal is exposed, to create lines and dark areas. For the single step of exposing the plate to acid, use "biting."</skos:scopeNote>
</skos:Concept>
<skos:Concept rdf:about="http://partage.vocnet.org/part01239">
	<skos:prefLabel xml:lang="de">Intarsie</skos:prefLabel>
	<skos:prefLabel xml:lang="en">intarsia</skos:prefLabel>
	<skos:prefLabel xml:lang="hr">intarzija</skos:prefLabel>
	<skos:inScheme rdf:resource="http://partage.vocnet.org/Activities"/>
	<skos:broader rdf:resource="http://partage.vocnet.org/part00459"/>
	<skos:exactMatch rdf:resource="http://vocab.getty.edu/aat/300053852"/>
	<skos:editorialNote xml:lang="en">PPTechnique</skos:editorialNote>
	<skos:scopeNote xml:lang="en">Italian type of stone or marble inlay characterized especially by representational motifs. Distinguished from mosaics, as pieces in intarsia work are precision-cut to tightly fit together.</skos:scopeNote>
</skos:Concept>
<skos:Concept rdf:about="http://partage.vocnet.org/part01240">
	<skos:prefLabel xml:lang="en">turning (shaping process)</skos:prefLabel>
	<skos:altLabel xml:lang="de">gedreht</skos:altLabel>
	<skos:prefLabel xml:lang="hr">tokarenje</skos:prefLabel>
	<skos:prefLabel xml:lang="de">gedrechselt</skos:prefLabel>
	<skos:inScheme rdf:resource="http://partage.vocnet.org/Activities"/>
	<skos:exactMatch rdf:resource="http://vocab.getty.edu/aat/300053158"/>
	<skos:editorialNote xml:lang="en">PPTechnique</skos:editorialNote>
	<skos:scopeNote xml:lang="en">The shaping of objects by means of cutting tools while the material from which the objects are made rotates rapidly on a lathe.</skos:scopeNote>
</skos:Concept>
<skos:Concept rdf:about="http://partage.vocnet.org/part01241">
	<skos:prefLabel xml:lang="de">geblasen</skos:prefLabel>
	<skos:prefLabel xml:lang="hr">puhanje u kalup</skos:prefLabel>
	<skos:prefLabel xml:lang="en">blow molding</skos:prefLabel>
	<skos:inScheme rdf:resource="http://partage.vocnet.org/Activities"/>
	<skos:broader rdf:resource="http://partage.vocnet.org/part00660"/>
	<skos:exactMatch rdf:resource="http://vocab.getty.edu/aat/300054067"/>
	<skos:editorialNote xml:lang="en">PPTechnique</skos:editorialNote>
	<skos:scopeNote xml:lang="en">Forming process whereby a hollow unit is formed and then forced, by internal pneumatic pressure, against a surrounding mold shaped to form a bottle or other container. Usually used with reference to glass and plastics.</skos:scopeNote>
</skos:Concept>
<skos:Concept rdf:about="http://partage.vocnet.org/part01242">
	<skos:prefLabel xml:lang="de">gebrannt</skos:prefLabel>
	<skos:prefLabel xml:lang="en">firing (technique)</skos:prefLabel>
	<skos:prefLabel xml:lang="hr">pečenje (keramike)</skos:prefLabel>
	<skos:inScheme rdf:resource="http://partage.vocnet.org/Activities"/>
	<skos:exactMatch rdf:resource="http://vocab.getty.edu/aat/300053887"/>
	<skos:editorialNote xml:lang="en">PPTechnique</skos:editorialNote>
	<skos:scopeNote xml:lang="en">Refers to the processes of preparing, curing, or purposely transforming materials, such as clay, silica, or glass, by means of heat.</skos:scopeNote>
</skos:Concept>
<skos:Concept rdf:about="http://partage.vocnet.org/part01246">
	<skos:prefLabel xml:lang="hr">modeliranje</skos:prefLabel>
	<skos:prefLabel xml:lang="de">modelliert.</skos:prefLabel>
	<skos:prefLabel xml:lang="en">modelling (forming)</skos:prefLabel>
	<skos:inScheme rdf:resource="http://partage.vocnet.org/Activities"/>
	<skos:broader rdf:resource="http://partage.vocnet.org/part01037"/>
	<skos:exactMatch rdf:resource="http://vocab.getty.edu/aat/300053130"/>
	<skos:editorialNote xml:lang="en">PPTechnique</skos:editorialNote>
	<skos:scopeNote xml:lang="en">Generally, use of malleable material such as wax or clay to create a form which is three-dimensional. Specifically, in ceramic art, the shaping of an original ceramic object or the model or maquette from which a mold is made.</skos:scopeNote>
</skos:Concept>
<skos:Concept rdf:about="http://partage.vocnet.org/part01247">
	<skos:prefLabel xml:lang="de">Lederbearbeitung</skos:prefLabel>
	<skos:prefLabel xml:lang="en">leatherworking</skos:prefLabel>
	<skos:inScheme rdf:resource="http://partage.vocnet.org/Activities"/>
	<skos:exactMatch rdf:resource="http://vocab.getty.edu/aat/300053941"/>
	<skos:editorialNote xml:lang="en">PPTechnique</skos:editorialNote>
	<skos:scopeNote xml:lang="en">The process of making things from or decorating leather. For the making of leather itself, use "leather" plus "manufacture."</skos:scopeNote>
</skos:Concept>
<skos:Concept rdf:about="http://partage.vocnet.org/part01248">
	<skos:prefLabel xml:lang="de">gestickt</skos:prefLabel>
	<skos:prefLabel xml:lang="en">embroidering</skos:prefLabel>
	<skos:inScheme rdf:resource="http://partage.vocnet.org/Activities"/>
	<skos:broader rdf:resource="http://partage.vocnet.org/part00492"/>
	<skos:exactMatch rdf:resource="http://vocab.getty.edu/aat/300053653"/>
	<skos:editorialNote xml:lang="en">PPTechnique</skos:editorialNote>
	<skos:scopeNote xml:lang="en">Refers to the process in which a needle and thread or fine wire are used to stitch decorative designs into cloth, leather, paper, or other material. It may also refer to the process used to create machine-made imitations of hand-made embroidery. For the weft patterning technique of weaving raised patterns on a woven textile, use "brocading."</skos:scopeNote>
</skos:Concept>
<skos:Concept rdf:about="http://partage.vocnet.org/part01249">
	<skos:prefLabel xml:lang="en">brocading</skos:prefLabel>
	<skos:inScheme rdf:resource="http://partage.vocnet.org/Activities"/>
	<skos:broader rdf:resource="http://partage.vocnet.org/part01253"/>
	<skos:exactMatch rdf:resource="http://vocab.getty.edu/aat/300053648"/>
	<skos:editorialNote xml:lang="en">PPTechnique</skos:editorialNote>
	<skos:scopeNote xml:lang="en">Weft patterning technique of weaving raised patterns on a woven textile. For the process of stitching decorative designs into cloth, leather, or paper by hand or machine, use "embroidering."</skos:scopeNote>
</skos:Concept>
<skos:Concept rdf:about="http://partage.vocnet.org/part01250">
	<skos:prefLabel xml:lang="en">mosaic (process)</skos:prefLabel>
	<skos:inScheme rdf:resource="http://partage.vocnet.org/Activities"/>
	<skos:broader rdf:resource="http://partage.vocnet.org/part00457"/>
	<skos:exactMatch rdf:resource="http://vocab.getty.edu/aat/300138684"/>
	<skos:editorialNote xml:lang="en">PPTechnique</skos:editorialNote>
	<skos:scopeNote xml:lang="en">A method of decorating surfaces with patterns or pictures composed of small, regularly-shaped pieces of colored durable material, such as stone or glass.</skos:scopeNote>
</skos:Concept>
<skos:Concept rdf:about="http://partage.vocnet.org/part01251">
	<skos:prefLabel xml:lang="en">leading (process)</skos:prefLabel>
	<skos:inScheme rdf:resource="http://partage.vocnet.org/Activities"/>
	<skos:exactMatch rdf:resource="http://vocab.getty.edu/aat/300241557"/>
	<skos:scopeNote xml:lang="en">Refers to the process of assembling pieces of glass together by inserting their edges into cames, for example to form windows or lampshades.</skos:scopeNote>
	<skos:editorialNote xml:lang="en">PPTechnique</skos:editorialNote>
</skos:Concept>
<skos:Concept rdf:about="http://partage.vocnet.org/part01252">
	<skos:prefLabel xml:lang="en">upholstering</skos:prefLabel>
	<skos:inScheme rdf:resource="http://partage.vocnet.org/Activities"/>
	<skos:exactMatch rdf:resource="http://vocab.getty.edu/aat/300231992"/>
	<skos:editorialNote xml:lang="en">PPTechnique</skos:editorialNote>
	<skos:scopeNote xml:lang="en">Provision of fixed soft coverings for furniture, especially seating and reclining furniture. Originally referred to the provision of all textile components of a room.</skos:scopeNote>
</skos:Concept>
<skos:Concept rdf:about="http://partage.vocnet.org/part01253">
	<skos:prefLabel xml:lang="en">weft patterning</skos:prefLabel>
	<skos:inScheme rdf:resource="http://partage.vocnet.org/Activities"/>
	<skos:narrower rdf:resource="http://partage.vocnet.org/part01249"/>
	<skos:exactMatch rdf:resource="http://vocab.getty.edu/aat/300228486"/>
	<skos:scopeNote xml:lang="en">Textile weaving technique in which a pattern is formed or the ground enriched by the use of more than one series of weft strands; the patterning is done using either a supplementary or complementary weft.</skos:scopeNote>
</skos:Concept>
<skos:Collection rdf:about="http://partage.vocnet.org/PPTechnique">
	<skos:prefLabel>PPTechnique</skos:prefLabel>
	<skos:member rdf:resource="http://partage.vocnet.org/part00211"/>
	<skos:member rdf:resource="http://partage.vocnet.org/part00340"/>
	<skos:member rdf:resource="http://partage.vocnet.org/part00417"/>
	<skos:member rdf:resource="http://partage.vocnet.org/part00449"/>
	<skos:member rdf:resource="http://partage.vocnet.org/part00450"/>
	<skos:member rdf:resource="http://partage.vocnet.org/part00451"/>
	<skos:member rdf:resource="http://partage.vocnet.org/part00452"/>
	<skos:member rdf:resource="http://partage.vocnet.org/part00453"/>
	<skos:member rdf:resource="http://partage.vocnet.org/part00454"/>
	<skos:member rdf:resource="http://partage.vocnet.org/part00455"/>
	<skos:member rdf:resource="http://partage.vocnet.org/part00456"/>
	<skos:member rdf:resource="http://partage.vocnet.org/part00457"/>
	<skos:member rdf:resource="http://partage.vocnet.org/part00458"/>
	<skos:member rdf:resource="http://partage.vocnet.org/part00459"/>
	<skos:member rdf:resource="http://partage.vocnet.org/part00460"/>
	<skos:member rdf:resource="http://partage.vocnet.org/part00461"/>
	<skos:member rdf:resource="http://partage.vocnet.org/part00462"/>
	<skos:member rdf:resource="http://partage.vocnet.org/part00463"/>
	<skos:member rdf:resource="http://partage.vocnet.org/part00464"/>
	<skos:member rdf:resource="http://partage.vocnet.org/part00479"/>
	<skos:member rdf:resource="http://partage.vocnet.org/part00647"/>
	<skos:member rdf:resource="http://partage.vocnet.org/part00648"/>
	<skos:member rdf:resource="http://partage.vocnet.org/part00652"/>
	<skos:member rdf:resource="http://partage.vocnet.org/part00654"/>
	<skos:member rdf:resource="http://partage.vocnet.org/part00656"/>
	<skos:member rdf:resource="http://partage.vocnet.org/part00660"/>
	<skos:member rdf:resource="http://partage.vocnet.org/part00661"/>
	<skos:member rdf:resource="http://partage.vocnet.org/part00662"/>
	<skos:member rdf:resource="http://partage.vocnet.org/part00663"/>
	<skos:member rdf:resource="http://partage.vocnet.org/part00664"/>
	<skos:member rdf:resource="http://partage.vocnet.org/part00666"/>
	<skos:member rdf:resource="http://partage.vocnet.org/part00667"/>
	<skos:member rdf:resource="http://partage.vocnet.org/part00668"/>
	<skos:member rdf:resource="http://partage.vocnet.org/part00669"/>
	<skos:member rdf:resource="http://partage.vocnet.org/part00670"/>
	<skos:member rdf:resource="http://partage.vocnet.org/part00671"/>
	<skos:member rdf:resource="http://partage.vocnet.org/part00672"/>
	<skos:member rdf:resource="http://partage.vocnet.org/part00673"/>
	<skos:member rdf:resource="http://partage.vocnet.org/part00877"/>
	<skos:member rdf:resource="http://partage.vocnet.org/part00878"/>
	<skos:member rdf:resource="http://partage.vocnet.org/part00879"/>
	<skos:member rdf:resource="http://partage.vocnet.org/part00880"/>
	<skos:member rdf:resource="http://partage.vocnet.org/part00881"/>
	<skos:member rdf:resource="http://partage.vocnet.org/part01037"/>
	<skos:member rdf:resource="http://partage.vocnet.org/part01119"/>
	<skos:member rdf:resource="http://partage.vocnet.org/part01225"/>
	<skos:member rdf:resource="http://partage.vocnet.org/part01226"/>
	<skos:member rdf:resource="http://partage.vocnet.org/part01227"/>
	<skos:member rdf:resource="http://partage.vocnet.org/part01229"/>
	<skos:member rdf:resource="http://partage.vocnet.org/part01231"/>
	<skos:member rdf:resource="http://partage.vocnet.org/part01232"/>
	<skos:member rdf:resource="http://partage.vocnet.org/part01233"/>
	<skos:member rdf:resource="http://partage.vocnet.org/part01234"/>
	<skos:member rdf:resource="http://partage.vocnet.org/part01236"/>
	<skos:member rdf:resource="http://partage.vocnet.org/part01239"/>
	<skos:member rdf:resource="http://partage.vocnet.org/part01240"/>
	<skos:member rdf:resource="http://partage.vocnet.org/part01241"/>
	<skos:member rdf:resource="http://partage.vocnet.org/part01242"/>
	<skos:member rdf:resource="http://partage.vocnet.org/part01246"/>
	<skos:member rdf:resource="http://partage.vocnet.org/part01247"/>
	<skos:member rdf:resource="http://partage.vocnet.org/part01248"/>
	<skos:member rdf:resource="http://partage.vocnet.org/part01249"/>
	<skos:member rdf:resource="http://partage.vocnet.org/part01250"/>
	<skos:member rdf:resource="http://partage.vocnet.org/part01251"/>
	<skos:member rdf:resource="http://partage.vocnet.org/part01252"/>
</skos:Collection>
<skos:Collection rdf:about="http://partage.vocnet.org/IndexingConcepts">
	<skos:prefLabel>IndexingConcepts</skos:prefLabel>
	<skos:member rdf:resource="http://partage.vocnet.org/part00211"/>
	<skos:member rdf:resource="http://partage.vocnet.org/part00340"/>
	<skos:member rdf:resource="http://partage.vocnet.org/part00417"/>
	<skos:member rdf:resource="http://partage.vocnet.org/part00449"/>
	<skos:member rdf:resource="http://partage.vocnet.org/part00450"/>
	<skos:member rdf:resource="http://partage.vocnet.org/part00451"/>
	<skos:member rdf:resource="http://partage.vocnet.org/part00452"/>
	<skos:member rdf:resource="http://partage.vocnet.org/part00453"/>
	<skos:member rdf:resource="http://partage.vocnet.org/part00454"/>
	<skos:member rdf:resource="http://partage.vocnet.org/part00455"/>
	<skos:member rdf:resource="http://partage.vocnet.org/part00456"/>
	<skos:member rdf:resource="http://partage.vocnet.org/part00457"/>
	<skos:member rdf:resource="http://partage.vocnet.org/part00458"/>
	<skos:member rdf:resource="http://partage.vocnet.org/part00459"/>
	<skos:member rdf:resource="http://partage.vocnet.org/part00460"/>
	<skos:member rdf:resource="http://partage.vocnet.org/part00461"/>
	<skos:member rdf:resource="http://partage.vocnet.org/part00462"/>
	<skos:member rdf:resource="http://partage.vocnet.org/part00463"/>
	<skos:member rdf:resource="http://partage.vocnet.org/part00464"/>
	<skos:member rdf:resource="http://partage.vocnet.org/part00479"/>
	<skos:member rdf:resource="http://partage.vocnet.org/part00647"/>
	<skos:member rdf:resource="http://partage.vocnet.org/part00648"/>
	<skos:member rdf:resource="http://partage.vocnet.org/part00652"/>
	<skos:member rdf:resource="http://partage.vocnet.org/part00654"/>
	<skos:member rdf:resource="http://partage.vocnet.org/part00656"/>
	<skos:member rdf:resource="http://partage.vocnet.org/part00660"/>
	<skos:member rdf:resource="http://partage.vocnet.org/part00661"/>
	<skos:member rdf:resource="http://partage.vocnet.org/part00662"/>
	<skos:member rdf:resource="http://partage.vocnet.org/part00663"/>
	<skos:member rdf:resource="http://partage.vocnet.org/part00664"/>
	<skos:member rdf:resource="http://partage.vocnet.org/part00666"/>
	<skos:member rdf:resource="http://partage.vocnet.org/part00667"/>
	<skos:member rdf:resource="http://partage.vocnet.org/part00668"/>
	<skos:member rdf:resource="http://partage.vocnet.org/part00669"/>
	<skos:member rdf:resource="http://partage.vocnet.org/part00670"/>
	<skos:member rdf:resource="http://partage.vocnet.org/part00671"/>
	<skos:member rdf:resource="http://partage.vocnet.org/part00672"/>
	<skos:member rdf:resource="http://partage.vocnet.org/part00673"/>
	<skos:member rdf:resource="http://partage.vocnet.org/part00877"/>
	<skos:member rdf:resource="http://partage.vocnet.org/part00878"/>
	<skos:member rdf:resource="http://partage.vocnet.org/part00879"/>
	<skos:member rdf:resource="http://partage.vocnet.org/part00880"/>
	<skos:member rdf:resource="http://partage.vocnet.org/part00881"/>
	<skos:member rdf:resource="http://partage.vocnet.org/part01037"/>
	<skos:member rdf:resource="http://partage.vocnet.org/part01119"/>
	<skos:member rdf:resource="http://partage.vocnet.org/part01225"/>
	<skos:member rdf:resource="http://partage.vocnet.org/part01226"/>
	<skos:member rdf:resource="http://partage.vocnet.org/part01227"/>
	<skos:member rdf:resource="http://partage.vocnet.org/part01229"/>
	<skos:member rdf:resource="http://partage.vocnet.org/part01231"/>
	<skos:member rdf:resource="http://partage.vocnet.org/part01232"/>
	<skos:member rdf:resource="http://partage.vocnet.org/part01233"/>
	<skos:member rdf:resource="http://partage.vocnet.org/part01234"/>
	<skos:member rdf:resource="http://partage.vocnet.org/part01236"/>
	<skos:member rdf:resource="http://partage.vocnet.org/part01239"/>
	<skos:member rdf:resource="http://partage.vocnet.org/part01240"/>
	<skos:member rdf:resource="http://partage.vocnet.org/part01241"/>
	<skos:member rdf:resource="http://partage.vocnet.org/part01242"/>
	<skos:member rdf:resource="http://partage.vocnet.org/part01246"/>
	<skos:member rdf:resource="http://partage.vocnet.org/part01247"/>
	<skos:member rdf:resource="http://partage.vocnet.org/part01248"/>
	<skos:member rdf:resource="http://partage.vocnet.org/part01249"/>
	<skos:member rdf:resource="http://partage.vocnet.org/part01250"/>
	<skos:member rdf:resource="http://partage.vocnet.org/part01251"/>
	<skos:member rdf:resource="http://partage.vocnet.org/part01252"/>
</skos:Collection>
<skos:Collection rdf:about="http://partage.vocnet.org/NonIndexingConcepts">
	<skos:prefLabel>NonIndexingConcepts</skos:prefLabel>
	<skos:member rdf:resource="http://partage.vocnet.org/part00480"/>
	<skos:member rdf:resource="http://partage.vocnet.org/part00483"/>
	<skos:member rdf:resource="http://partage.vocnet.org/part00492"/>
	<skos:member rdf:resource="http://partage.vocnet.org/part00494"/>
	<skos:member rdf:resource="http://partage.vocnet.org/part00497"/>
	<skos:member rdf:resource="http://partage.vocnet.org/part00649"/>
	<skos:member rdf:resource="http://partage.vocnet.org/part00657"/>
	<skos:member rdf:resource="http://partage.vocnet.org/part00658"/>
	<skos:member rdf:resource="http://partage.vocnet.org/part00659"/>
	<skos:member rdf:resource="http://partage.vocnet.org/part00665"/>
	<skos:member rdf:resource="http://partage.vocnet.org/part01020"/>
	<skos:member rdf:resource="http://partage.vocnet.org/part01026"/>
	<skos:member rdf:resource="http://partage.vocnet.org/part01230"/>
	<skos:member rdf:resource="http://partage.vocnet.org/part01253"/>
</skos:Collection>
</rdf:RDF>