<?xml version='1.0' encoding='UTF-8'?>
<rdf:RDF xmlns:rdf="http://www.w3.org/1999/02/22-rdf-syntax-ns#" xmlns:dcterms="http://purl.org/dc/terms/" xmlns:owl="http://www.w3.org/2002/07/owl#" xmlns:skos="http://www.w3.org/2004/02/skos/core#">
<skos:ConceptScheme rdf:about="http://partage.vocnet.org/Agents">
	<rdf:type rdf:resource="http://www.w3.org/2004/02/skos/core#ConceptScheme"/>
</skos:ConceptScheme>
<skos:Concept rdf:about="http://partage.vocnet.org/part00420">
	<skos:prefLabel xml:lang="en">authors</skos:prefLabel>
	<skos:altLabel xml:lang="en">author</skos:altLabel>
	<skos:altLabel xml:lang="de">Verfasser</skos:altLabel>
	<skos:altLabel xml:lang="de">Autoren</skos:altLabel>
	<skos:prefLabel xml:lang="de">Autor</skos:prefLabel>
	<skos:prefLabel xml:lang="hr">autor</skos:prefLabel>
	<skos:prefLabel xml:lang="sv">författare</skos:prefLabel>
	<skos:prefLabel xml:lang="pt">autor</skos:prefLabel>
	<skos:prefLabel xml:lang="fi">kirjoittaja</skos:prefLabel>
	<skos:inScheme rdf:resource="http://partage.vocnet.org/Agents"/>
	<skos:broader rdf:resource="http://partage.vocnet.org/part00425"/>
	<skos:exactMatch rdf:resource="http://vocab.getty.edu/aat/300025492"/>
	<skos:editorialNote xml:lang="en">PPRoleActor</skos:editorialNote>
	<skos:scopeNote xml:lang="en">Persons responsible for the intellectual content of books, namely those who write or otherwise compose books, articles, poems, plays, or other works which involve literary composition and are intended for publication.</skos:scopeNote>
</skos:Concept>
<skos:Concept rdf:about="http://partage.vocnet.org/part00425">
	<skos:prefLabel xml:lang="en">people (agents)</skos:prefLabel>
	<skos:inScheme rdf:resource="http://partage.vocnet.org/Agents"/>
	<skos:narrower rdf:resource="http://partage.vocnet.org/part00420"/>
	<skos:narrower rdf:resource="http://partage.vocnet.org/part00428"/>
	<skos:narrower rdf:resource="http://partage.vocnet.org/part00434"/>
	<skos:narrower rdf:resource="http://partage.vocnet.org/part00439"/>
	<skos:narrower rdf:resource="http://partage.vocnet.org/part00445"/>
	<skos:narrower rdf:resource="http://partage.vocnet.org/part00473"/>
	<skos:narrower rdf:resource="http://partage.vocnet.org/part00475"/>
	<skos:narrower rdf:resource="http://partage.vocnet.org/part00541"/>
	<skos:narrower rdf:resource="http://partage.vocnet.org/part00545"/>
	<skos:narrower rdf:resource="http://partage.vocnet.org/part00859"/>
	<skos:narrower rdf:resource="http://partage.vocnet.org/part00862"/>
	<skos:narrower rdf:resource="http://partage.vocnet.org/part00989"/>
	<skos:exactMatch rdf:resource="http://vocab.getty.edu/aat/300024979"/>
	<skos:editorialNote xml:lang="en">Partage Plus Specialist Terms</skos:editorialNote>
</skos:Concept>
<skos:Concept rdf:about="http://partage.vocnet.org/part00428">
	<skos:prefLabel xml:lang="en">craftsmen</skos:prefLabel>
	<skos:altLabel xml:lang="en">craftsman</skos:altLabel>
	<skos:prefLabel xml:lang="de">Kunsthandwerker</skos:prefLabel>
	<skos:prefLabel xml:lang="hr">obrtnik</skos:prefLabel>
	<skos:prefLabel xml:lang="sv">hantverkare</skos:prefLabel>
	<skos:prefLabel xml:lang="pt">artesão</skos:prefLabel>
	<skos:prefLabel xml:lang="fi">käsityöläinen</skos:prefLabel>
	<skos:inScheme rdf:resource="http://partage.vocnet.org/Agents"/>
	<skos:broader rdf:resource="http://partage.vocnet.org/part00425"/>
	<skos:exactMatch rdf:resource="http://vocab.getty.edu/aat/300025389"/>
	<skos:editorialNote xml:lang="en">PPRoleActor</skos:editorialNote>
	<skos:scopeNote xml:lang="en">Refers to those who practice an occupation, trade, or pursuit requiring manual dexterity or artistic skill, typically excluding those who produce painting, sculpture, drawing, or architecture. Generally distinguished from "artists" and "architects," based on the media of their creations. For a more general term for those who create or construct artifacts directly by their own labor, especially as their profession or primary occupation, use "makers."</skos:scopeNote>
</skos:Concept>
<skos:Concept rdf:about="http://partage.vocnet.org/part00432">
	<skos:altLabel xml:lang="en">draftsmen (artists)</skos:altLabel>
	<skos:prefLabel xml:lang="en">draftsmen</skos:prefLabel>
	<skos:altLabel xml:lang="en">draftsman</skos:altLabel>
	<skos:prefLabel xml:lang="de">Zeichner</skos:prefLabel>
	<skos:prefLabel xml:lang="hr">crtač (tehnički)</skos:prefLabel>
	<skos:prefLabel xml:lang="sv">tecknare</skos:prefLabel>
	<skos:prefLabel xml:lang="pt">desenhador</skos:prefLabel>
	<skos:prefLabel xml:lang="fi">piirtäjä</skos:prefLabel>
	<skos:inScheme rdf:resource="http://partage.vocnet.org/Agents"/>
	<skos:broader rdf:resource="http://partage.vocnet.org/part00434"/>
	<skos:exactMatch rdf:resource="http://vocab.getty.edu/aat/300112172"/>
	<skos:editorialNote xml:lang="en">PPRoleActor</skos:editorialNote>
	<skos:scopeNote xml:lang="en">Artists who specialize in making drawings, which are designs formed by lines on a surface, often paper, by using a pencil, pen, chalk, or some other tracing instrument to focus on the delineation of form rather than the application of color.</skos:scopeNote>
</skos:Concept>
<skos:Concept rdf:about="http://partage.vocnet.org/part00434">
	<skos:altLabel xml:lang="en">artists (visual artists)</skos:altLabel>
	<skos:altLabel xml:lang="en">artist</skos:altLabel>
	<skos:prefLabel xml:lang="en">artists</skos:prefLabel>
	<skos:prefLabel xml:lang="de">Künstler</skos:prefLabel>
	<skos:prefLabel xml:lang="hr">umjetnik</skos:prefLabel>
	<skos:prefLabel xml:lang="sv">konstnärer</skos:prefLabel>
	<skos:prefLabel xml:lang="pt">artista</skos:prefLabel>
	<skos:prefLabel xml:lang="fi">taiteilija</skos:prefLabel>
	<skos:inScheme rdf:resource="http://partage.vocnet.org/Agents"/>
	<skos:broader rdf:resource="http://partage.vocnet.org/part00425"/>
	<skos:narrower rdf:resource="http://partage.vocnet.org/part00432"/>
	<skos:narrower rdf:resource="http://partage.vocnet.org/part00438"/>
	<skos:narrower rdf:resource="http://partage.vocnet.org/part00444"/>
	<skos:narrower rdf:resource="http://partage.vocnet.org/part00471"/>
	<skos:narrower rdf:resource="http://partage.vocnet.org/part00540"/>
	<skos:narrower rdf:resource="http://partage.vocnet.org/part00860"/>
	<skos:exactMatch rdf:resource="http://vocab.getty.edu/aat/300025103"/>
	<skos:editorialNote xml:lang="en">PPRoleActor</skos:editorialNote>
	<skos:scopeNote xml:lang="en">People who produce work in the visual arts. For those in the performing arts, see "performing artists."</skos:scopeNote>
</skos:Concept>
<skos:Concept rdf:about="http://partage.vocnet.org/part00438">
	<skos:prefLabel xml:lang="en">illustrators</skos:prefLabel>
	<skos:altLabel xml:lang="en">illustrator</skos:altLabel>
	<skos:altLabel xml:lang="de">Illustratoren</skos:altLabel>
	<skos:prefLabel xml:lang="de">Illustrator</skos:prefLabel>
	<skos:prefLabel xml:lang="hr">ilustrator</skos:prefLabel>
	<skos:prefLabel xml:lang="sv">illustratörer</skos:prefLabel>
	<skos:prefLabel xml:lang="pt">ilustrador</skos:prefLabel>
	<skos:prefLabel xml:lang="fi">kuvittaja</skos:prefLabel>
	<skos:inScheme rdf:resource="http://partage.vocnet.org/Agents"/>
	<skos:broader rdf:resource="http://partage.vocnet.org/part00434"/>
	<skos:exactMatch rdf:resource="http://vocab.getty.edu/aat/300025123"/>
	<skos:editorialNote xml:lang="en">PPRoleActor</skos:editorialNote>
	<skos:scopeNote xml:lang="en">Artists who specialize in creating drawings, prints, or other pictures intended to elucidate a description, story, or other written material, usually in a book or periodical.</skos:scopeNote>
</skos:Concept>
<skos:Concept rdf:about="http://partage.vocnet.org/part00439">
	<skos:prefLabel xml:lang="en">makers</skos:prefLabel>
	<skos:altLabel xml:lang="en">maker</skos:altLabel>
	<skos:prefLabel xml:lang="de">Hersteller</skos:prefLabel>
	<skos:prefLabel xml:lang="hr">stvaratelj</skos:prefLabel>
	<skos:prefLabel xml:lang="sv">tillverkare</skos:prefLabel>
	<skos:prefLabel xml:lang="pt">fabricante</skos:prefLabel>
	<skos:prefLabel xml:lang="fi">tekijä</skos:prefLabel>
	<skos:inScheme rdf:resource="http://partage.vocnet.org/Agents"/>
	<skos:broader rdf:resource="http://partage.vocnet.org/part00425"/>
	<skos:exactMatch rdf:resource="http://vocab.getty.edu/aat/300251917"/>
	<skos:editorialNote xml:lang="en">PPRoleActor</skos:editorialNote>
	<skos:scopeNote xml:lang="en">Those who create or construct artifacts directly by their own labor, especially as their craft or profession. For industrialists who own or run a manufacturing plant, use "manufacturers." For those who practice an occupation, trade, or pursuit requiring manual dexterity or artistic skill, use "craftsmen."</skos:scopeNote>
</skos:Concept>
<skos:Concept rdf:about="http://partage.vocnet.org/part00444">
	<skos:altLabel xml:lang="en">painters (artists)</skos:altLabel>
	<skos:altLabel xml:lang="en">painter</skos:altLabel>
	<skos:prefLabel xml:lang="en">painters</skos:prefLabel>
	<skos:prefLabel xml:lang="de">Maler</skos:prefLabel>
	<skos:prefLabel xml:lang="sl">slikar</skos:prefLabel>
	<skos:prefLabel xml:lang="sv">konstnärer.</skos:prefLabel>
	<skos:prefLabel xml:lang="pt">pintor</skos:prefLabel>
	<skos:prefLabel xml:lang="fi">taidemaalari</skos:prefLabel>
	<skos:inScheme rdf:resource="http://partage.vocnet.org/Agents"/>
	<skos:broader rdf:resource="http://partage.vocnet.org/part00434"/>
	<skos:exactMatch rdf:resource="http://vocab.getty.edu/aat/300025136"/>
	<skos:editorialNote xml:lang="en">PPRoleActor</skos:editorialNote>
	<skos:scopeNote xml:lang="en">People who practice the art of painting, which is applying pigments suspended in liquid to a surface to create an expressive or communicative image. For people who apply paint primarily to protect or give simple color to a surface, use "painters (tradespeople)."</skos:scopeNote>
</skos:Concept>
<skos:Concept rdf:about="http://partage.vocnet.org/part00445">
	<skos:altLabel xml:lang="en">printers (people)</skos:altLabel>
	<skos:altLabel xml:lang="en">printer</skos:altLabel>
	<skos:prefLabel xml:lang="en">printers</skos:prefLabel>
	<skos:prefLabel xml:lang="de">Drucker</skos:prefLabel>
	<skos:prefLabel xml:lang="hr">tiskar</skos:prefLabel>
	<skos:altLabel xml:lang="pt">tipografia (corporation)</skos:altLabel>
	<skos:altLabel xml:lang="pt">tipógrafo (person)</skos:altLabel>
	<skos:prefLabel xml:lang="pt">impressor</skos:prefLabel>
	<skos:prefLabel xml:lang="sv">tryckare</skos:prefLabel>
	<skos:prefLabel xml:lang="fi">painaja</skos:prefLabel>
	<skos:inScheme rdf:resource="http://partage.vocnet.org/Agents"/>
	<skos:broader rdf:resource="http://partage.vocnet.org/part00425"/>
	<skos:exactMatch rdf:resource="http://vocab.getty.edu/aat/300025732"/>
	<skos:editorialNote xml:lang="en">PPRoleActor</skos:editorialNote>
	<skos:scopeNote xml:lang="en">Refers to people in the commercial printing trade. For artists who make prints, see "printmakers."</skos:scopeNote>
</skos:Concept>
<skos:Concept rdf:about="http://partage.vocnet.org/part00471">
	<skos:prefLabel xml:lang="en">printmakers</skos:prefLabel>
	<skos:altLabel xml:lang="en">printmaker</skos:altLabel>
	<skos:altLabel xml:lang="de">Lithographen</skos:altLabel>
	<skos:altLabel xml:lang="de">Lithograph</skos:altLabel>
	<skos:altLabel xml:lang="de">Radierer</skos:altLabel>
	<skos:altLabel xml:lang="de">Kupferstecher</skos:altLabel>
	<skos:prefLabel xml:lang="de">Stecher</skos:prefLabel>
	<skos:prefLabel xml:lang="hr">grafičar</skos:prefLabel>
	<skos:prefLabel xml:lang="sv">grafiker</skos:prefLabel>
	<skos:altLabel xml:lang="pt">tipógrafo</skos:altLabel>
	<skos:prefLabel xml:lang="pt">impressor.</skos:prefLabel>
	<skos:prefLabel xml:lang="fi">vedostaja</skos:prefLabel>
	<skos:inScheme rdf:resource="http://partage.vocnet.org/Agents"/>
	<skos:broader rdf:resource="http://partage.vocnet.org/part00434"/>
	<skos:exactMatch rdf:resource="http://vocab.getty.edu/aat/300025164"/>
	<skos:editorialNote xml:lang="en">PPRoleActor</skos:editorialNote>
	<skos:scopeNote xml:lang="en">Persons who prepare, conceive, and develop drawings and other art work and prepare printmaking media used to print fine arts graphics. For persons in the commercial printing trade, use "printers (people)."</skos:scopeNote>
</skos:Concept>
<skos:Concept rdf:about="http://partage.vocnet.org/part00473">
	<skos:prefLabel xml:lang="en">merchants</skos:prefLabel>
	<skos:altLabel xml:lang="en">merchant</skos:altLabel>
	<skos:prefLabel xml:lang="de">Händler</skos:prefLabel>
	<skos:prefLabel xml:lang="hr">trgovac</skos:prefLabel>
	<skos:prefLabel xml:lang="sv">köpmän</skos:prefLabel>
	<skos:prefLabel xml:lang="pt">mercador</skos:prefLabel>
	<skos:prefLabel xml:lang="fi">myyjä</skos:prefLabel>
	<skos:inScheme rdf:resource="http://partage.vocnet.org/Agents"/>
	<skos:broader rdf:resource="http://partage.vocnet.org/part00425"/>
	<skos:exactMatch rdf:resource="http://vocab.getty.edu/aat/300025245"/>
	<skos:editorialNote xml:lang="en">PPRoleActor</skos:editorialNote>
	<skos:scopeNote xml:lang="en">Buyers and sellers of commodities for profit.</skos:scopeNote>
</skos:Concept>
<skos:Concept rdf:about="http://partage.vocnet.org/part00475">
	<skos:prefLabel xml:lang="en">architects</skos:prefLabel>
	<skos:altLabel xml:lang="en">architect</skos:altLabel>
	<skos:altLabel xml:lang="de">Architekten</skos:altLabel>
	<skos:prefLabel xml:lang="de">Architekt</skos:prefLabel>
	<skos:prefLabel xml:lang="hr">arhitekt</skos:prefLabel>
	<skos:prefLabel xml:lang="sv">arkitekter</skos:prefLabel>
	<skos:prefLabel xml:lang="pt">arquitecto</skos:prefLabel>
	<skos:prefLabel xml:lang="fi">arkkitehti</skos:prefLabel>
	<skos:inScheme rdf:resource="http://partage.vocnet.org/Agents"/>
	<skos:broader rdf:resource="http://partage.vocnet.org/part00425"/>
	<skos:exactMatch rdf:resource="http://vocab.getty.edu/aat/300024987"/>
	<skos:editorialNote xml:lang="en">PPRoleActor</skos:editorialNote>
	<skos:scopeNote xml:lang="en">People trained in or practicing architecture, which is the art of designing and building habitable structures, especially those considered to have aesthetic value.</skos:scopeNote>
</skos:Concept>
<skos:Concept rdf:about="http://partage.vocnet.org/part00540">
	<skos:altLabel xml:lang="en">sculptor</skos:altLabel>
	<skos:prefLabel xml:lang="en">sculptors</skos:prefLabel>
	<skos:prefLabel xml:lang="de">Bildhauer</skos:prefLabel>
	<skos:prefLabel xml:lang="hr">kipar</skos:prefLabel>
	<skos:prefLabel xml:lang="sv">skulptörer</skos:prefLabel>
	<skos:prefLabel xml:lang="pt">escultor</skos:prefLabel>
	<skos:prefLabel xml:lang="fi">kuvanveistäjä</skos:prefLabel>
	<skos:inScheme rdf:resource="http://partage.vocnet.org/Agents"/>
	<skos:broader rdf:resource="http://partage.vocnet.org/part00434"/>
	<skos:exactMatch rdf:resource="http://vocab.getty.edu/aat/300025181"/>
	<skos:editorialNote xml:lang="en">PPRoleActor</skos:editorialNote>
	<skos:scopeNote xml:lang="en">Artists who specialize in creating images and forms that are carried out primarily in three dimensions, generally of large or medium size, and in the media of stone, wood, or metal. It may also refer to artists who create relief or intaglio works. For artists who create small works, or for craftsmen who carve three dimensional forms that are not considered art, use "carvers."</skos:scopeNote>
</skos:Concept>
<skos:Concept rdf:about="http://partage.vocnet.org/part00541">
	<skos:altLabel xml:lang="en">publisher</skos:altLabel>
	<skos:prefLabel xml:lang="en">publishers</skos:prefLabel>
	<skos:prefLabel xml:lang="de">Verleger</skos:prefLabel>
	<skos:prefLabel xml:lang="hr">izdavač</skos:prefLabel>
	<skos:prefLabel xml:lang="sv">förläggare</skos:prefLabel>
	<skos:prefLabel xml:lang="pt">editor</skos:prefLabel>
	<skos:prefLabel xml:lang="fi">julkaisija</skos:prefLabel>
	<skos:inScheme rdf:resource="http://partage.vocnet.org/Agents"/>
	<skos:broader rdf:resource="http://partage.vocnet.org/part00425"/>
	<skos:exactMatch rdf:resource="http://vocab.getty.edu/aat/300025574"/>
	<skos:editorialNote xml:lang="en">PPRoleActor</skos:editorialNote>
	<skos:scopeNote xml:lang="en">People, firms, or corporate bodies responsible for placing a book or other work on the market for sale or distribution to the public. For those active before about 1800, see "booksellers."</skos:scopeNote>
</skos:Concept>
<skos:Concept rdf:about="http://partage.vocnet.org/part00545">
	<skos:altLabel xml:lang="en">designer</skos:altLabel>
	<skos:prefLabel xml:lang="en">designers</skos:prefLabel>
	<skos:altLabel xml:lang="de">Entwerfer</skos:altLabel>
	<skos:prefLabel xml:lang="de">Designer</skos:prefLabel>
	<skos:altLabel xml:lang="de">Zeichner des Entwurfs</skos:altLabel>
	<skos:prefLabel xml:lang="hr">dizajner</skos:prefLabel>
	<skos:altLabel xml:lang="sv">designers</skos:altLabel>
	<skos:prefLabel xml:lang="sv">formgivare</skos:prefLabel>
	<skos:prefLabel xml:lang="pt">designer</skos:prefLabel>
	<skos:prefLabel xml:lang="fi">suunnittelija</skos:prefLabel>
	<skos:inScheme rdf:resource="http://partage.vocnet.org/Agents"/>
	<skos:broader rdf:resource="http://partage.vocnet.org/part00425"/>
	<skos:exactMatch rdf:resource="http://vocab.getty.edu/aat/300025190"/>
	<skos:editorialNote xml:lang="en">PPRoleActor</skos:editorialNote>
	<skos:scopeNote xml:lang="en">People who create conceptual schemes for the organization or appearance of graphic works, objects, structures, or systems.</skos:scopeNote>
</skos:Concept>
<skos:Concept rdf:about="http://partage.vocnet.org/part00549">
	<skos:altLabel xml:lang="en">artists' collective</skos:altLabel>
	<skos:prefLabel xml:lang="en">artists' collectives</skos:prefLabel>
	<skos:prefLabel xml:lang="de">Künstlergruppe</skos:prefLabel>
	<skos:altLabel xml:lang="de">Künstlerkollektiv</skos:altLabel>
	<skos:prefLabel xml:lang="hr">udruga umjetnika</skos:prefLabel>
	<skos:altLabel xml:lang="sv">konstnärskollektiv</skos:altLabel>
	<skos:prefLabel xml:lang="sv">konstnärsgrupper</skos:prefLabel>
	<skos:prefLabel xml:lang="pt">colectiva de artistas</skos:prefLabel>
	<skos:prefLabel xml:lang="fi">taiteilijaryhmä</skos:prefLabel>
	<skos:inScheme rdf:resource="http://partage.vocnet.org/Agents"/>
	<skos:broader rdf:resource="http://partage.vocnet.org/part00550"/>
	<skos:exactMatch rdf:resource="http://vocab.getty.edu/aat/300265433"/>
	<skos:editorialNote xml:lang="en">PPRoleActor</skos:editorialNote>
	<skos:scopeNote xml:lang="en">Associations of artists, wherein members of each group collaborate in a formal manner.</skos:scopeNote>
</skos:Concept>
<skos:Concept rdf:about="http://partage.vocnet.org/part00550">
	<skos:prefLabel xml:lang="en">associations</skos:prefLabel>
	<skos:inScheme rdf:resource="http://partage.vocnet.org/Agents"/>
	<skos:broader rdf:resource="http://partage.vocnet.org/part00551"/>
	<skos:narrower rdf:resource="http://partage.vocnet.org/part00549"/>
	<skos:exactMatch rdf:resource="http://vocab.getty.edu/aat/300025950"/>
</skos:Concept>
<skos:Concept rdf:about="http://partage.vocnet.org/part00551">
	<skos:altLabel xml:lang="en">organizations (groups)</skos:altLabel>
	<skos:prefLabel xml:lang="en">organisations</skos:prefLabel>
	<skos:inScheme rdf:resource="http://partage.vocnet.org/Agents"/>
	<skos:narrower rdf:resource="http://partage.vocnet.org/part00550"/>
	<skos:narrower rdf:resource="http://partage.vocnet.org/part01015"/>
	<skos:exactMatch rdf:resource="http://vocab.getty.edu/aat/300025948"/>
	<skos:scopeNote xml:lang="en">Groups of people organized for a purpose, typically characterized by a more or less constant membership, a body of officers or functionaries, and a set of regulations governing their activities and conduct.</skos:scopeNote>
</skos:Concept>
<skos:Concept rdf:about="http://partage.vocnet.org/part00859">
	<skos:prefLabel xml:lang="en">owners</skos:prefLabel>
	<skos:altLabel xml:lang="en">owner</skos:altLabel>
	<skos:prefLabel xml:lang="de">Eigentümer</skos:prefLabel>
	<skos:prefLabel xml:lang="hr">vlasnik</skos:prefLabel>
	<skos:prefLabel xml:lang="sv">ägare</skos:prefLabel>
	<skos:prefLabel xml:lang="pt">proprietário</skos:prefLabel>
	<skos:prefLabel xml:lang="fi">omistaja</skos:prefLabel>
	<skos:inScheme rdf:resource="http://partage.vocnet.org/Agents"/>
	<skos:broader rdf:resource="http://partage.vocnet.org/part00425"/>
	<skos:exactMatch rdf:resource="http://vocab.getty.edu/aat/300203630"/>
	<skos:editorialNote xml:lang="en">PPRoleActor</skos:editorialNote>
	<skos:scopeNote xml:lang="en">People who have legal title to something. For those who own specifically businesses or commercial establishments, use "proprietors."</skos:scopeNote>
</skos:Concept>
<skos:Concept rdf:about="http://partage.vocnet.org/part00860">
	<skos:prefLabel xml:lang="en">photographers</skos:prefLabel>
	<skos:altLabel xml:lang="en">photographer</skos:altLabel>
	<skos:altLabel xml:lang="de">Photograph</skos:altLabel>
	<skos:altLabel xml:lang="de">Photographen</skos:altLabel>
	<skos:altLabel xml:lang="de">Fotografen</skos:altLabel>
	<skos:prefLabel xml:lang="de">Fotograf</skos:prefLabel>
	<skos:prefLabel xml:lang="hr">fotograf</skos:prefLabel>
	<skos:prefLabel xml:lang="sv">fotografer</skos:prefLabel>
	<skos:prefLabel xml:lang="pt">fotógrafo</skos:prefLabel>
	<skos:prefLabel xml:lang="fi">valokuvaaja</skos:prefLabel>
	<skos:inScheme rdf:resource="http://partage.vocnet.org/Agents"/>
	<skos:broader rdf:resource="http://partage.vocnet.org/part00434"/>
	<skos:exactMatch rdf:resource="http://vocab.getty.edu/aat/300025687"/>
	<skos:editorialNote xml:lang="en">PPRoleActor</skos:editorialNote>
	<skos:scopeNote xml:lang="en">Individuals who specialize in creating photographs, which are still images produced from radiation-sensitive materials, typically by means of the chemical action of light on a sensitive film, paper, glass, or metal.</skos:scopeNote>
</skos:Concept>
<skos:Concept rdf:about="http://partage.vocnet.org/part00862">
	<skos:prefLabel xml:lang="en">clients</skos:prefLabel>
	<skos:altLabel xml:lang="en">client</skos:altLabel>
	<skos:prefLabel xml:lang="de">Auftraggeber</skos:prefLabel>
	<skos:prefLabel xml:lang="hr">klijent</skos:prefLabel>
	<skos:altLabel xml:lang="sv">kunder</skos:altLabel>
	<skos:prefLabel xml:lang="sv">klienter</skos:prefLabel>
	<skos:prefLabel xml:lang="pl">cliente</skos:prefLabel>
	<skos:prefLabel xml:lang="fi">toimeksiantaja</skos:prefLabel>
	<skos:inScheme rdf:resource="http://partage.vocnet.org/Agents"/>
	<skos:broader rdf:resource="http://partage.vocnet.org/part00425"/>
	<skos:exactMatch rdf:resource="http://vocab.getty.edu/aat/300025833"/>
	<skos:scopeNote xml:lang="en">Persons who engage the professional advice or services of others.</skos:scopeNote>
	<skos:editorialNote xml:lang="en">PPRoleActor</skos:editorialNote>
</skos:Concept>
<skos:Concept rdf:about="http://partage.vocnet.org/part00989">
	<skos:prefLabel xml:lang="en">donors</skos:prefLabel>
	<skos:altLabel xml:lang="en">donor</skos:altLabel>
	<skos:prefLabel xml:lang="de">Stifter</skos:prefLabel>
	<skos:prefLabel xml:lang="hr">donator</skos:prefLabel>
	<skos:prefLabel xml:lang="sv">donatorer</skos:prefLabel>
	<skos:prefLabel xml:lang="pt">doador</skos:prefLabel>
	<skos:prefLabel xml:lang="fi">lahjoittaja</skos:prefLabel>
	<skos:inScheme rdf:resource="http://partage.vocnet.org/Agents"/>
	<skos:broader rdf:resource="http://partage.vocnet.org/part00425"/>
	<skos:exactMatch rdf:resource="http://vocab.getty.edu/aat/300025240"/>
	<skos:editorialNote xml:lang="en">PPRoleActor</skos:editorialNote>
	<skos:scopeNote xml:lang="en">People who leave personal property to another person or institution.</skos:scopeNote>
	<skos:scopeNote xml:lang="de">no scope note available in AAT</skos:scopeNote>
</skos:Concept>
<skos:Concept rdf:about="http://partage.vocnet.org/part01015">
	<skos:altLabel xml:lang="en">manufactory</skos:altLabel>
	<skos:prefLabel xml:lang="en">manufactories</skos:prefLabel>
	<skos:altLabel xml:lang="de">Manufakturen</skos:altLabel>
	<skos:prefLabel xml:lang="de">Manufaktur</skos:prefLabel>
	<skos:prefLabel xml:lang="hr">manufaktura</skos:prefLabel>
	<skos:prefLabel xml:lang="sv">manufakturer</skos:prefLabel>
	<skos:prefLabel xml:lang="pt">manufactura</skos:prefLabel>
	<skos:prefLabel xml:lang="fi">valmistaja</skos:prefLabel>
	<skos:inScheme rdf:resource="http://partage.vocnet.org/Agents"/>
	<skos:broader rdf:resource="http://partage.vocnet.org/part00551"/>
	<skos:exactMatch rdf:resource="http://vocab.getty.edu/aat/300264603"/>
	<skos:editorialNote xml:lang="en">PPRoleActor</skos:editorialNote>
	<skos:scopeNote xml:lang="en">Refers to organized groups who make objects primarily by hand. In the context of Western art and decorative arts, the term "manufactory" is often used rather than "factory (organization)" to distinguish groups active in the 17th century or later that made fine art, furniture, tapestries, ceramics, and other decorative objects, as contrasted to workers active in modern industrial complexes, or "factories (structures)," where objects other than art are produced. Manufactories are typically characterized by the types of objects they produce, by the relatively large numbers of artists and craftsmen employed, and by the relatively complex administrative structure of director, or "directeur," and several masters, who may each supervise a separate workshop or studio of artisans and apprentices. Manufactories were often sponsored by a monarch or other powerful person. For smaller groups consisting of a master artist or architect and his or her assistants or pupils, especially those dating from the mid-17th century on, use "studios (organizations)." For smaller groups of artists or craftsmen collaborating to produce works, often under a master's name, especially when the groups existed prior to the 17th century, use "workshops (organizations)."</skos:scopeNote>
</skos:Concept>
<skos:Collection rdf:about="http://partage.vocnet.org/PPRoleActor">
	<skos:prefLabel>PPRoleActor</skos:prefLabel>
	<skos:member rdf:resource="http://partage.vocnet.org/part00420"/>
	<skos:member rdf:resource="http://partage.vocnet.org/part00428"/>
	<skos:member rdf:resource="http://partage.vocnet.org/part00432"/>
	<skos:member rdf:resource="http://partage.vocnet.org/part00434"/>
	<skos:member rdf:resource="http://partage.vocnet.org/part00438"/>
	<skos:member rdf:resource="http://partage.vocnet.org/part00439"/>
	<skos:member rdf:resource="http://partage.vocnet.org/part00444"/>
	<skos:member rdf:resource="http://partage.vocnet.org/part00445"/>
	<skos:member rdf:resource="http://partage.vocnet.org/part00471"/>
	<skos:member rdf:resource="http://partage.vocnet.org/part00473"/>
	<skos:member rdf:resource="http://partage.vocnet.org/part00475"/>
	<skos:member rdf:resource="http://partage.vocnet.org/part00540"/>
	<skos:member rdf:resource="http://partage.vocnet.org/part00541"/>
	<skos:member rdf:resource="http://partage.vocnet.org/part00545"/>
	<skos:member rdf:resource="http://partage.vocnet.org/part00549"/>
	<skos:member rdf:resource="http://partage.vocnet.org/part00859"/>
	<skos:member rdf:resource="http://partage.vocnet.org/part00860"/>
	<skos:member rdf:resource="http://partage.vocnet.org/part00862"/>
	<skos:member rdf:resource="http://partage.vocnet.org/part00989"/>
	<skos:member rdf:resource="http://partage.vocnet.org/part01015"/>
</skos:Collection>
<skos:Collection rdf:about="http://partage.vocnet.org/IndexingConcepts">
	<skos:prefLabel>IndexingConcepts</skos:prefLabel>
	<skos:member rdf:resource="http://partage.vocnet.org/part00420"/>
	<skos:member rdf:resource="http://partage.vocnet.org/part00428"/>
	<skos:member rdf:resource="http://partage.vocnet.org/part00432"/>
	<skos:member rdf:resource="http://partage.vocnet.org/part00434"/>
	<skos:member rdf:resource="http://partage.vocnet.org/part00438"/>
	<skos:member rdf:resource="http://partage.vocnet.org/part00439"/>
	<skos:member rdf:resource="http://partage.vocnet.org/part00444"/>
	<skos:member rdf:resource="http://partage.vocnet.org/part00445"/>
	<skos:member rdf:resource="http://partage.vocnet.org/part00471"/>
	<skos:member rdf:resource="http://partage.vocnet.org/part00473"/>
	<skos:member rdf:resource="http://partage.vocnet.org/part00475"/>
	<skos:member rdf:resource="http://partage.vocnet.org/part00540"/>
	<skos:member rdf:resource="http://partage.vocnet.org/part00541"/>
	<skos:member rdf:resource="http://partage.vocnet.org/part00545"/>
	<skos:member rdf:resource="http://partage.vocnet.org/part00549"/>
	<skos:member rdf:resource="http://partage.vocnet.org/part00859"/>
	<skos:member rdf:resource="http://partage.vocnet.org/part00860"/>
	<skos:member rdf:resource="http://partage.vocnet.org/part00862"/>
	<skos:member rdf:resource="http://partage.vocnet.org/part00989"/>
	<skos:member rdf:resource="http://partage.vocnet.org/part01015"/>
</skos:Collection>
<skos:Collection rdf:about="http://partage.vocnet.org/NonIndexingConcepts">
	<skos:prefLabel>NonIndexingConcepts</skos:prefLabel>
	<skos:member rdf:resource="http://partage.vocnet.org/part00425"/>
	<skos:member rdf:resource="http://partage.vocnet.org/part00550"/>
	<skos:member rdf:resource="http://partage.vocnet.org/part00551"/>
</skos:Collection>
</rdf:RDF>