<?xml version='1.0' encoding='UTF-8'?>
<rdf:RDF xmlns:rdf="http://www.w3.org/1999/02/22-rdf-syntax-ns#" xmlns:dcterms="http://purl.org/dc/terms/" xmlns:owl="http://www.w3.org/2002/07/owl#" xmlns:skos="http://www.w3.org/2004/02/skos/core#">
<skos:ConceptScheme rdf:about="http://partage.vocnet.org/Materials">
	<rdf:type rdf:resource="http://www.w3.org/2004/02/skos/core#ConceptScheme"/>
</skos:ConceptScheme>
<skos:Concept rdf:about="http://partage.vocnet.org/part00227">
	<skos:prefLabel xml:lang="en">clay</skos:prefLabel>
	<skos:prefLabel xml:lang="sv">lera</skos:prefLabel>
	<skos:prefLabel xml:lang="pt">argila</skos:prefLabel>
	<skos:prefLabel xml:lang="de">Ton</skos:prefLabel>
	<skos:prefLabel xml:lang="fi">savi</skos:prefLabel>
	<skos:prefLabel xml:lang="hr">glina</skos:prefLabel>
	<skos:inScheme rdf:resource="http://partage.vocnet.org/Materials"/>
	<skos:broader rdf:resource="http://partage.vocnet.org/part00229"/>
	<skos:narrower rdf:resource="http://partage.vocnet.org/part00233"/>
	<skos:narrower rdf:resource="http://partage.vocnet.org/part00239"/>
	<skos:narrower rdf:resource="http://partage.vocnet.org/part00567"/>
	<skos:narrower rdf:resource="http://partage.vocnet.org/part01212"/>
	<skos:narrower rdf:resource="http://partage.vocnet.org/part01214"/>
	<skos:exactMatch rdf:resource="http://vocab.getty.edu/aat/300010439"/>
	<skos:editorialNote xml:lang="en">PPMaterial</skos:editorialNote>
	<skos:scopeNote xml:lang="en">Naturally occurring sediments that are produced by chemical actions resulting during the weathering of rocks. It is often the term applied to all earths that form a paste with water and harden when heated.</skos:scopeNote>
</skos:Concept>
<skos:Concept rdf:about="http://partage.vocnet.org/part00229">
	<skos:prefLabel xml:lang="en">materials (matter)</skos:prefLabel>
	<skos:inScheme rdf:resource="http://partage.vocnet.org/Materials"/>
	<skos:narrower rdf:resource="http://partage.vocnet.org/part00227"/>
	<skos:narrower rdf:resource="http://partage.vocnet.org/part00246"/>
	<skos:narrower rdf:resource="http://partage.vocnet.org/part00257"/>
	<skos:narrower rdf:resource="http://partage.vocnet.org/part00259"/>
	<skos:narrower rdf:resource="http://partage.vocnet.org/part00281"/>
	<skos:narrower rdf:resource="http://partage.vocnet.org/part00288"/>
	<skos:narrower rdf:resource="http://partage.vocnet.org/part00289"/>
	<skos:narrower rdf:resource="http://partage.vocnet.org/part00290"/>
	<skos:narrower rdf:resource="http://partage.vocnet.org/part00292"/>
	<skos:narrower rdf:resource="http://partage.vocnet.org/part00297"/>
	<skos:narrower rdf:resource="http://partage.vocnet.org/part00394"/>
	<skos:narrower rdf:resource="http://partage.vocnet.org/part00489"/>
	<skos:narrower rdf:resource="http://partage.vocnet.org/part00518"/>
	<skos:narrower rdf:resource="http://partage.vocnet.org/part00519"/>
	<skos:narrower rdf:resource="http://partage.vocnet.org/part00538"/>
	<skos:narrower rdf:resource="http://partage.vocnet.org/part00539"/>
	<skos:narrower rdf:resource="http://partage.vocnet.org/part00565"/>
	<skos:narrower rdf:resource="http://partage.vocnet.org/part00568"/>
	<skos:narrower rdf:resource="http://partage.vocnet.org/part00571"/>
	<skos:narrower rdf:resource="http://partage.vocnet.org/part00575"/>
	<skos:narrower rdf:resource="http://partage.vocnet.org/part00576"/>
	<skos:narrower rdf:resource="http://partage.vocnet.org/part00582"/>
	<skos:narrower rdf:resource="http://partage.vocnet.org/part00587"/>
	<skos:narrower rdf:resource="http://partage.vocnet.org/part00588"/>
	<skos:narrower rdf:resource="http://partage.vocnet.org/part00590"/>
	<skos:narrower rdf:resource="http://partage.vocnet.org/part00591"/>
	<skos:narrower rdf:resource="http://partage.vocnet.org/part00592"/>
	<skos:narrower rdf:resource="http://partage.vocnet.org/part00601"/>
	<skos:narrower rdf:resource="http://partage.vocnet.org/part00602"/>
	<skos:narrower rdf:resource="http://partage.vocnet.org/part00610"/>
	<skos:narrower rdf:resource="http://partage.vocnet.org/part00613"/>
	<skos:narrower rdf:resource="http://partage.vocnet.org/part00615"/>
	<skos:narrower rdf:resource="http://partage.vocnet.org/part00618"/>
	<skos:narrower rdf:resource="http://partage.vocnet.org/part00621"/>
	<skos:narrower rdf:resource="http://partage.vocnet.org/part00625"/>
	<skos:narrower rdf:resource="http://partage.vocnet.org/part00626"/>
	<skos:narrower rdf:resource="http://partage.vocnet.org/part00632"/>
	<skos:narrower rdf:resource="http://partage.vocnet.org/part00832"/>
	<skos:narrower rdf:resource="http://partage.vocnet.org/part00900"/>
	<skos:narrower rdf:resource="http://partage.vocnet.org/part00913"/>
	<skos:narrower rdf:resource="http://partage.vocnet.org/part01035"/>
	<skos:narrower rdf:resource="http://partage.vocnet.org/part01208"/>
	<skos:exactMatch rdf:resource="http://vocab.getty.edu/aat/300010358"/>
	<skos:scopeNote xml:lang="en">The matter or substance from which a thing is or may be made; the tangible substance that goes into the makeup of a physical object. Physical substances, either naturally or synthetically derived, ranging from specific materials to types of material designated by their function.</skos:scopeNote>
</skos:Concept>
<skos:Concept rdf:about="http://partage.vocnet.org/part00233">
	<skos:altLabel xml:lang="en">ceramic (material)</skos:altLabel>
	<skos:prefLabel xml:lang="en">ceramic</skos:prefLabel>
	<skos:prefLabel xml:lang="de">Keramik (Material)</skos:prefLabel>
	<skos:prefLabel xml:lang="sv">keramik (material)</skos:prefLabel>
	<skos:prefLabel xml:lang="pt">cerâmica (material)</skos:prefLabel>
	<skos:prefLabel xml:lang="fi">keramiikka (mat.)</skos:prefLabel>
	<skos:prefLabel xml:lang="hr">keramika (mat.)</skos:prefLabel>
	<skos:inScheme rdf:resource="http://partage.vocnet.org/Materials"/>
	<skos:broader rdf:resource="http://partage.vocnet.org/part00227"/>
	<skos:narrower rdf:resource="http://partage.vocnet.org/part00236"/>
	<skos:narrower rdf:resource="http://partage.vocnet.org/part00237"/>
	<skos:exactMatch rdf:resource="http://vocab.getty.edu/aat/300235507"/>
	<skos:editorialNote xml:lang="en">PPMaterial</skos:editorialNote>
	<skos:scopeNote xml:lang="en">Refers to any of various hard, brittle, heat-resistant and corrosion-resistant materials made by shaping and then firing a nonmetallic mineral, such as clay, at a high temperature.</skos:scopeNote>
</skos:Concept>
<skos:Concept rdf:about="http://partage.vocnet.org/part00236">
	<skos:prefLabel xml:lang="en">biscuit</skos:prefLabel>
	<skos:prefLabel xml:lang="de">Bisquitporzellan</skos:prefLabel>
	<skos:prefLabel xml:lang="sv">biskviporslin</skos:prefLabel>
	<skos:prefLabel xml:lang="pt">biscuit</skos:prefLabel>
	<skos:prefLabel xml:lang="hr">biskvit</skos:prefLabel>
	<skos:prefLabel xml:lang="fi">biskviitti</skos:prefLabel>
	<skos:inScheme rdf:resource="http://partage.vocnet.org/Materials"/>
	<skos:broader rdf:resource="http://partage.vocnet.org/part00233"/>
	<skos:exactMatch rdf:resource="http://vocab.getty.edu/aat/300242297"/>
	<skos:editorialNote xml:lang="en">PPMaterial</skos:editorialNote>
	<skos:scopeNote xml:lang="en">Unglazed porcelain or earthenware that has been fired only once; generally producing a grainy texture; frequently used for modeling ornament or making small statues, dolls, or vessels. Distinct from "parian (porcelain)," which is silky in texture and marblelike in appearance.</skos:scopeNote>
</skos:Concept>
<skos:Concept rdf:about="http://partage.vocnet.org/part00237">
	<skos:prefLabel xml:lang="en">porcelain</skos:prefLabel>
	<skos:prefLabel xml:lang="sv">porslin</skos:prefLabel>
	<skos:prefLabel xml:lang="pt">porcelana</skos:prefLabel>
	<skos:prefLabel xml:lang="de">Porzellan</skos:prefLabel>
	<skos:prefLabel xml:lang="hr">porculan</skos:prefLabel>
	<skos:prefLabel xml:lang="fi">posliini</skos:prefLabel>
	<skos:inScheme rdf:resource="http://partage.vocnet.org/Materials"/>
	<skos:broader rdf:resource="http://partage.vocnet.org/part00233"/>
	<skos:exactMatch rdf:resource="http://vocab.getty.edu/aat/300010662"/>
	<skos:editorialNote xml:lang="en">PPMaterial</skos:editorialNote>
	<skos:scopeNote xml:lang="en">A type of ceramic ware made of a refractory white clay, or "kaolin," and a feldspathic rock, that react when fired so the clay serves to hold the shape of the object and the rock fuses into a natural glass. In China, it includes any such ware that is highly fired enough to produce a ringing sound when struck. In Europe, it is limited to hard-fired ceramic ware that is translucent.</skos:scopeNote>
</skos:Concept>
<skos:Concept rdf:about="http://partage.vocnet.org/part00239">
	<skos:prefLabel xml:lang="en">ceramic tile</skos:prefLabel>
	<skos:altLabel xml:lang="de">Kachel</skos:altLabel>
	<skos:prefLabel xml:lang="de">Keramikfliese</skos:prefLabel>
	<skos:prefLabel xml:lang="sv">kakel</skos:prefLabel>
	<skos:prefLabel xml:lang="pt">azulejo</skos:prefLabel>
	<skos:prefLabel xml:lang="hr">keramički crijep</skos:prefLabel>
	<skos:prefLabel xml:lang="fi">kaakeli</skos:prefLabel>
	<skos:inScheme rdf:resource="http://partage.vocnet.org/Materials"/>
	<skos:broader rdf:resource="http://partage.vocnet.org/part00227"/>
	<skos:exactMatch rdf:resource="http://vocab.getty.edu/aat/300010678"/>
	<skos:scopeNote xml:lang="en">Fired clay in various shapes and thicknesses and with a variety of uses, as for surface covering, drainage, or construction. For flat, solid, and relatively thin durable material used primarily for surface covering, use "tile."</skos:scopeNote>
	<skos:editorialNote xml:lang="en">PPMaterial</skos:editorialNote>
</skos:Concept>
<skos:Concept rdf:about="http://partage.vocnet.org/part00241">
	<skos:altLabel xml:lang="en">crystal (lead glass)</skos:altLabel>
	<skos:prefLabel xml:lang="en">crystal</skos:prefLabel>
	<skos:prefLabel xml:lang="de">Kristall</skos:prefLabel>
	<skos:prefLabel xml:lang="sv">kristall</skos:prefLabel>
	<skos:prefLabel xml:lang="pt">cristal</skos:prefLabel>
	<skos:prefLabel xml:lang="fi">kristalli</skos:prefLabel>
	<skos:prefLabel xml:lang="hr">kristal</skos:prefLabel>
	<skos:inScheme rdf:resource="http://partage.vocnet.org/Materials"/>
	<skos:broader rdf:resource="http://partage.vocnet.org/part00242"/>
	<skos:exactMatch rdf:resource="http://vocab.getty.edu/aat/300010814"/>
	<skos:editorialNote xml:lang="en">PPMaterial</skos:editorialNote>
	<skos:scopeNote xml:lang="en">Fine, high quality, heavy, decorative glass made with fine white sand, at least 24% lead oxide, and small amounts of potash and niter. It is clear, colorless, highly refractive glass that is heavy and has greater than twice the density of standard borate glass. It was developed in England in 1676; often used for high quality chandelier prisms and fine stemware.</skos:scopeNote>
</skos:Concept>
<skos:Concept rdf:about="http://partage.vocnet.org/part00242">
	<skos:prefLabel xml:lang="en">lead glass</skos:prefLabel>
	<skos:inScheme rdf:resource="http://partage.vocnet.org/Materials"/>
	<skos:broader rdf:resource="http://partage.vocnet.org/part00246"/>
	<skos:narrower rdf:resource="http://partage.vocnet.org/part00241"/>
	<skos:exactMatch rdf:resource="http://vocab.getty.edu/aat/300010811"/>
	<skos:scopeNote xml:lang="en">Glass containing a high proportion of lead oxide and having a relatively high refractive index, with poor acid resistance and low rigidity; used in many optical components, neon-sign tubing, and light bulbs.</skos:scopeNote>
</skos:Concept>
<skos:Concept rdf:about="http://partage.vocnet.org/part00244">
	<skos:altLabel xml:lang="en">pâte de verre (glass)</skos:altLabel>
	<skos:prefLabel xml:lang="en">pâte de verre</skos:prefLabel>
	<skos:prefLabel xml:lang="sv">pâte de verre</skos:prefLabel>
	<skos:prefLabel xml:lang="pt">pasta de vidro</skos:prefLabel>
	<skos:prefLabel xml:lang="de">Pâte de Verre</skos:prefLabel>
	<skos:prefLabel xml:lang="fi">lasitahna</skos:prefLabel>
	<skos:prefLabel xml:lang="hr">pâte de verre</skos:prefLabel>
	<skos:inScheme rdf:resource="http://partage.vocnet.org/Materials"/>
	<skos:broader rdf:resource="http://partage.vocnet.org/part00246"/>
	<skos:exactMatch rdf:resource="http://vocab.getty.edu/aat/300263723"/>
	<skos:editorialNote xml:lang="en">PPMaterial</skos:editorialNote>
	<skos:scopeNote xml:lang="en">Refers to glass created by a technique in which ground glass is made into a paste and molded into a vessel or figure, and then the design is refined by carving. Glass created by this method was known in ancient times and revived in France in the late 19th and early 20th centuries, notably in the studio of glass and jewelry designer, Ren\u00e9 Lalique.</skos:scopeNote>
</skos:Concept>
<skos:Concept rdf:about="http://partage.vocnet.org/part00246">
	<skos:altLabel xml:lang="en">glass (material)</skos:altLabel>
	<skos:prefLabel xml:lang="en">glass</skos:prefLabel>
	<skos:prefLabel xml:lang="de">Glas (Material)</skos:prefLabel>
	<skos:prefLabel xml:lang="sv">glas</skos:prefLabel>
	<skos:prefLabel xml:lang="pt">vidro</skos:prefLabel>
	<skos:prefLabel xml:lang="fi">lasi</skos:prefLabel>
	<skos:prefLabel xml:lang="hr">staklo</skos:prefLabel>
	<skos:inScheme rdf:resource="http://partage.vocnet.org/Materials"/>
	<skos:broader rdf:resource="http://partage.vocnet.org/part00229"/>
	<skos:narrower rdf:resource="http://partage.vocnet.org/part00242"/>
	<skos:narrower rdf:resource="http://partage.vocnet.org/part00244"/>
	<skos:narrower rdf:resource="http://partage.vocnet.org/part00247"/>
	<skos:narrower rdf:resource="http://partage.vocnet.org/part00248"/>
	<skos:narrower rdf:resource="http://partage.vocnet.org/part00250"/>
	<skos:narrower rdf:resource="http://partage.vocnet.org/part01077"/>
	<skos:exactMatch rdf:resource="http://vocab.getty.edu/aat/300010797"/>
	<skos:scopeNote xml:lang="en">An amorphous, inorganic substance made by fusing silica (silicon dioxide) with a basic oxide; generally transparent but often translucent or opaque. Its characteristic properties are its hardness and rigidity at ordinary temperatures, its capacity for plastic working at elevated temperatures, and its resistance to weathering and to most chemicals except hydrofluoric acid. Used for both utilitarian and decorative purposes, it can be formed into various shapes, colored or decorated. Glass originated as a glaze in Mesopotamia in about 3500 BCE and the first objects made wholly of glass date to about 2500 BCE.</skos:scopeNote>
	<skos:editorialNote xml:lang="en">PPMaterial</skos:editorialNote>
</skos:Concept>
<skos:Concept rdf:about="http://partage.vocnet.org/part00247">
	<skos:prefLabel xml:lang="en">cased glass</skos:prefLabel>
	<skos:prefLabel xml:lang="de">Überfangglas</skos:prefLabel>
	<skos:prefLabel xml:lang="sv">överfångsglas</skos:prefLabel>
	<skos:prefLabel xml:lang="pt">vidro cameo</skos:prefLabel>
	<skos:prefLabel xml:lang="hr">lijevano staklo</skos:prefLabel>
	<skos:inScheme rdf:resource="http://partage.vocnet.org/Materials"/>
	<skos:broader rdf:resource="http://partage.vocnet.org/part00246"/>
	<skos:narrower rdf:resource="http://partage.vocnet.org/part00514"/>
	<skos:exactMatch rdf:resource="http://vocab.getty.edu/aat/300010833"/>
	<skos:editorialNote xml:lang="en">PPMaterial</skos:editorialNote>
	<skos:scopeNote xml:lang="en">Glass formed of two or more fused layers of different colored glass.</skos:scopeNote>
</skos:Concept>
<skos:Concept rdf:about="http://partage.vocnet.org/part00248">
	<skos:prefLabel xml:lang="en">cut glass</skos:prefLabel>
	<skos:altLabel xml:lang="de">geschliffenes Glas</skos:altLabel>
	<skos:prefLabel xml:lang="de">Kristallglas</skos:prefLabel>
	<skos:prefLabel xml:lang="sv">slipat glas</skos:prefLabel>
	<skos:prefLabel xml:lang="pt">vidro talhado</skos:prefLabel>
	<skos:prefLabel xml:lang="hr">brušeno staklo</skos:prefLabel>
	<skos:prefLabel xml:lang="fi">hiottu kristalli</skos:prefLabel>
	<skos:inScheme rdf:resource="http://partage.vocnet.org/Materials"/>
	<skos:broader rdf:resource="http://partage.vocnet.org/part00246"/>
	<skos:exactMatch rdf:resource="http://vocab.getty.edu/aat/300206355"/>
	<skos:editorialNote xml:lang="en">PPMaterial</skos:editorialNote>
	<skos:scopeNote xml:lang="en">Generally used to describe glassware with facets, grooves, and depressions produced by cutting with a rotating wheel of metal or stone.</skos:scopeNote>
</skos:Concept>
<skos:Concept rdf:about="http://partage.vocnet.org/part00250">
	<skos:prefLabel xml:lang="en">Favrile glass (TM)</skos:prefLabel>
	<skos:inScheme rdf:resource="http://partage.vocnet.org/Materials"/>
	<skos:broader rdf:resource="http://partage.vocnet.org/part00246"/>
	<skos:exactMatch rdf:resource="http://vocab.getty.edu/aat/300206359"/>
	<skos:editorialNote xml:lang="en">PPSpecialistTerms</skos:editorialNote>
	<skos:scopeNote xml:lang="en">Trademark name for a type of glass developed by Tiffany and Company with an iridescent surface simulating that of excavated ancient Roman glass; this effect was produced by spraying the surface of the glass while hot with metallic salts.</skos:scopeNote>
	<skos:editorialNote xml:lang="de">PPMaterial</skos:editorialNote>
</skos:Concept>
<skos:Concept rdf:about="http://partage.vocnet.org/part00252">
	<skos:altLabel xml:lang="en">horn (animal material)</skos:altLabel>
	<skos:prefLabel xml:lang="en">horn</skos:prefLabel>
	<skos:prefLabel xml:lang="sv">horn</skos:prefLabel>
	<skos:prefLabel xml:lang="pt">chifre</skos:prefLabel>
	<skos:prefLabel xml:lang="de">Horn (Material)</skos:prefLabel>
	<skos:prefLabel xml:lang="hr">rog</skos:prefLabel>
	<skos:prefLabel xml:lang="fi">sarvi</skos:prefLabel>
	<skos:inScheme rdf:resource="http://partage.vocnet.org/Materials"/>
	<skos:broader rdf:resource="http://partage.vocnet.org/part00257"/>
	<skos:exactMatch rdf:resource="http://vocab.getty.edu/aat/300011826"/>
	<skos:editorialNote xml:lang="en">PPMaterial</skos:editorialNote>
	<skos:scopeNote xml:lang="en">Outgrowth of modified skin or compacted hair, often occuring in pairs, projecting from the frontal bones on either side of the skull, consisting of a nondeciduous cuticle composed of keratin. Distinguished from "antler," which is modified bone.</skos:scopeNote>
</skos:Concept>
<skos:Concept rdf:about="http://partage.vocnet.org/part00253">
	<skos:prefLabel xml:lang="en">leather</skos:prefLabel>
	<skos:prefLabel xml:lang="sv">läder</skos:prefLabel>
	<skos:prefLabel xml:lang="pt">pele</skos:prefLabel>
	<skos:prefLabel xml:lang="de">Leder</skos:prefLabel>
	<skos:prefLabel xml:lang="hr">koža</skos:prefLabel>
	<skos:prefLabel xml:lang="fi">nahka</skos:prefLabel>
	<skos:inScheme rdf:resource="http://partage.vocnet.org/Materials"/>
	<skos:broader rdf:resource="http://partage.vocnet.org/part00257"/>
	<skos:narrower rdf:resource="http://partage.vocnet.org/part00583"/>
	<skos:narrower rdf:resource="http://partage.vocnet.org/part00627"/>
	<skos:exactMatch rdf:resource="http://vocab.getty.edu/aat/300011845"/>
	<skos:editorialNote xml:lang="en">PPMaterial</skos:editorialNote>
	<skos:scopeNote xml:lang="en">The skin or hide of an animal that has been tanned to render it resistant to putrefication and relatively soft and flexible when dry. For composite material made from scrap leather pieces, use "maril."</skos:scopeNote>
</skos:Concept>
<skos:Concept rdf:about="http://partage.vocnet.org/part00257">
	<skos:prefLabel xml:lang="en">animal material</skos:prefLabel>
	<skos:inScheme rdf:resource="http://partage.vocnet.org/Materials"/>
	<skos:broader rdf:resource="http://partage.vocnet.org/part00229"/>
	<skos:narrower rdf:resource="http://partage.vocnet.org/part00252"/>
	<skos:narrower rdf:resource="http://partage.vocnet.org/part00253"/>
	<skos:narrower rdf:resource="http://partage.vocnet.org/part00521"/>
	<skos:narrower rdf:resource="http://partage.vocnet.org/part00580"/>
	<skos:narrower rdf:resource="http://partage.vocnet.org/part00599"/>
	<skos:exactMatch rdf:resource="http://vocab.getty.edu/aat/300011793"/>
	<skos:scopeNote xml:lang="en">Material of animal origin.</skos:scopeNote>
</skos:Concept>
<skos:Concept rdf:about="http://partage.vocnet.org/part00259">
	<skos:prefLabel xml:lang="en">metal</skos:prefLabel>
	<skos:prefLabel xml:lang="sv">metall</skos:prefLabel>
	<skos:prefLabel xml:lang="pt">metal</skos:prefLabel>
	<skos:prefLabel xml:lang="de">Metall</skos:prefLabel>
	<skos:prefLabel xml:lang="hr">metal</skos:prefLabel>
	<skos:prefLabel xml:lang="fi">metalli</skos:prefLabel>
	<skos:inScheme rdf:resource="http://partage.vocnet.org/Materials"/>
	<skos:broader rdf:resource="http://partage.vocnet.org/part00229"/>
	<skos:narrower rdf:resource="http://partage.vocnet.org/part00261"/>
	<skos:narrower rdf:resource="http://partage.vocnet.org/part00265"/>
	<skos:narrower rdf:resource="http://partage.vocnet.org/part00515"/>
	<skos:narrower rdf:resource="http://partage.vocnet.org/part01203"/>
	<skos:narrower rdf:resource="http://partage.vocnet.org/part01215"/>
	<skos:exactMatch rdf:resource="http://vocab.getty.edu/aat/300010900"/>
	<skos:editorialNote xml:lang="en">PPMaterial</skos:editorialNote>
	<skos:scopeNote xml:lang="en">Any of a large group of substances that typically show a characteristic luster, are good conductors of electricity and heat, are opaque, can be fused, and are usually malleable or ductile.</skos:scopeNote>
</skos:Concept>
<skos:Concept rdf:about="http://partage.vocnet.org/part00261">
	<skos:prefLabel xml:lang="en">iron alloy</skos:prefLabel>
	<skos:inScheme rdf:resource="http://partage.vocnet.org/Materials"/>
	<skos:broader rdf:resource="http://partage.vocnet.org/part00259"/>
	<skos:narrower rdf:resource="http://partage.vocnet.org/part00263"/>
	<skos:narrower rdf:resource="http://partage.vocnet.org/part00264"/>
	<skos:narrower rdf:resource="http://partage.vocnet.org/part00537"/>
	<skos:exactMatch rdf:resource="http://vocab.getty.edu/aat/300010904"/>
	<skos:scopeNote xml:lang="en">Alloy in which iron is the principle element.</skos:scopeNote>
</skos:Concept>
<skos:Concept rdf:about="http://partage.vocnet.org/part00263">
	<skos:prefLabel xml:lang="en">cast iron</skos:prefLabel>
	<skos:prefLabel xml:lang="de">Gusseisen</skos:prefLabel>
	<skos:prefLabel xml:lang="sv">gjutjärn</skos:prefLabel>
	<skos:prefLabel xml:lang="pt">ferro fundido</skos:prefLabel>
	<skos:prefLabel xml:lang="fi">valurauta</skos:prefLabel>
	<skos:prefLabel xml:lang="hr">lijevano željezo</skos:prefLabel>
	<skos:inScheme rdf:resource="http://partage.vocnet.org/Materials"/>
	<skos:broader rdf:resource="http://partage.vocnet.org/part00261"/>
	<skos:exactMatch rdf:resource="http://vocab.getty.edu/aat/300011004"/>
	<skos:editorialNote xml:lang="en">PPMaterial</skos:editorialNote>
	<skos:scopeNote xml:lang="en">An iron alloy containing about 2 to 4% carbon and 1 to 3% silicon, having a high compressive strength but low tensile strength. Cast iron is manufactured by melting scrap iron or pig iron in a cupola that is in contact with the coal fuel, then casting the molten iron into a mold. A large range of building and decorative items are made of cast iron by pouring the molten metal into sand molds and then machining. It is inexpensive and easy to make. It was made in China by at least the 3rd century BCE; the technique for its production did not reach Europe until medieval times.</skos:scopeNote>
</skos:Concept>
<skos:Concept rdf:about="http://partage.vocnet.org/part00264">
	<skos:altLabel xml:lang="en">wrought iron (iron alloy)</skos:altLabel>
	<skos:prefLabel xml:lang="en">wrought iron</skos:prefLabel>
	<skos:prefLabel xml:lang="sv">smidesjärn</skos:prefLabel>
	<skos:prefLabel xml:lang="pt">ferro forjado</skos:prefLabel>
	<skos:prefLabel xml:lang="de">Schmiedeeisen</skos:prefLabel>
	<skos:prefLabel xml:lang="fi">takorauta</skos:prefLabel>
	<skos:prefLabel xml:lang="hr">kovano željezo</skos:prefLabel>
	<skos:inScheme rdf:resource="http://partage.vocnet.org/Materials"/>
	<skos:broader rdf:resource="http://partage.vocnet.org/part00261"/>
	<skos:exactMatch rdf:resource="http://vocab.getty.edu/aat/300011012"/>
	<skos:editorialNote xml:lang="en">PPMaterial</skos:editorialNote>
	<skos:scopeNote xml:lang="en">Iron alloy of fibrous nature made by melting white cast iron, passing an oxidizing flame over it, and rolling it into a mass; valued for its corrosion resistance and ductility. When describing objects produced or shaped by beating with a hammer, use "wrought."</skos:scopeNote>
</skos:Concept>
<skos:Concept rdf:about="http://partage.vocnet.org/part00265">
	<skos:prefLabel xml:lang="en">nonferrous metal</skos:prefLabel>
	<skos:inScheme rdf:resource="http://partage.vocnet.org/Materials"/>
	<skos:broader rdf:resource="http://partage.vocnet.org/part00259"/>
	<skos:narrower rdf:resource="http://partage.vocnet.org/part00267"/>
	<skos:narrower rdf:resource="http://partage.vocnet.org/part00269"/>
	<skos:narrower rdf:resource="http://partage.vocnet.org/part00271"/>
	<skos:narrower rdf:resource="http://partage.vocnet.org/part00272"/>
	<skos:narrower rdf:resource="http://partage.vocnet.org/part00276"/>
	<skos:narrower rdf:resource="http://partage.vocnet.org/part00278"/>
	<skos:narrower rdf:resource="http://partage.vocnet.org/part00279"/>
	<skos:narrower rdf:resource="http://partage.vocnet.org/part00563"/>
	<skos:narrower rdf:resource="http://partage.vocnet.org/part00634"/>
	<skos:narrower rdf:resource="http://partage.vocnet.org/part01218"/>
	<skos:exactMatch rdf:resource="http://vocab.getty.edu/aat/300011014"/>
	<skos:scopeNote xml:lang="en">Metal that does not have iron as its major ingredient.</skos:scopeNote>
</skos:Concept>
<skos:Concept rdf:about="http://partage.vocnet.org/part00267">
	<skos:altLabel xml:lang="en">gold (metal)</skos:altLabel>
	<skos:prefLabel xml:lang="en">gold</skos:prefLabel>
	<skos:prefLabel xml:lang="de">Gold</skos:prefLabel>
	<skos:prefLabel xml:lang="sv">guld</skos:prefLabel>
	<skos:prefLabel xml:lang="pt">ouro</skos:prefLabel>
	<skos:prefLabel xml:lang="hr">zlato</skos:prefLabel>
	<skos:prefLabel xml:lang="fi">kulta</skos:prefLabel>
	<skos:inScheme rdf:resource="http://partage.vocnet.org/Materials"/>
	<skos:broader rdf:resource="http://partage.vocnet.org/part00265"/>
	<skos:exactMatch rdf:resource="http://vocab.getty.edu/aat/300011021"/>
	<skos:editorialNote xml:lang="en">PPMaterial</skos:editorialNote>
	<skos:scopeNote xml:lang="en">Pure metallic element having symbol Au and atomic number 79; a soft, inert, shiny reddish yellow metal that is very malleable and ductile. Gold has been highly valued and found in artifacts dating to before 5000 BCE. Native gold, found in quartz veins (vein gold) and alluvial deposits (placer gold), generally contains some silver and copper. Gold is purified by dissolution in mercury or cyanide solutions, by melting, or by electrodeposition. The purity of commercial gold is expressed in karats which is the number of parts of gold in 24 parts of the alloy. Today gold is primarily used for monetary systems and for jewelry.</skos:scopeNote>
</skos:Concept>
<skos:Concept rdf:about="http://partage.vocnet.org/part00269">
	<skos:altLabel xml:lang="en">silver (metal)</skos:altLabel>
	<skos:prefLabel xml:lang="en">silver</skos:prefLabel>
	<skos:prefLabel xml:lang="sv">silver</skos:prefLabel>
	<skos:prefLabel xml:lang="pt">prata</skos:prefLabel>
	<skos:prefLabel xml:lang="de">Silber</skos:prefLabel>
	<skos:prefLabel xml:lang="fi">hopea</skos:prefLabel>
	<skos:prefLabel xml:lang="hr">srebro</skos:prefLabel>
	<skos:inScheme rdf:resource="http://partage.vocnet.org/Materials"/>
	<skos:broader rdf:resource="http://partage.vocnet.org/part00265"/>
	<skos:exactMatch rdf:resource="http://vocab.getty.edu/aat/300011029"/>
	<skos:editorialNote xml:lang="en">PPMaterial</skos:editorialNote>
	<skos:scopeNote xml:lang="en">Pure metallic element having symbol Ag and atomic number 47; a malleable, ductile, white metal with characteristic sheen, considered a precious metal. Silver is widely distributed throughout the world, occurring rarely as metallic silver (in Peru, Norway) but more often as silver-gold alloys and silver ore. Today silver is obtained as a byproduct in the refinement of gold, lead, copper, or zinc ores. Silver was smelted from the ore galena as early as 3800 BCE. As a pure metal, silver is second to gold in malleability and ductility, can be polished to a highly reflective surface, and used -- typically in an alloy -- in jewelry, coinage, photography, mirrors, electrical contacts, and tableware.</skos:scopeNote>
</skos:Concept>
<skos:Concept rdf:about="http://partage.vocnet.org/part00271">
	<skos:altLabel xml:lang="en">copper (metal)</skos:altLabel>
	<skos:prefLabel xml:lang="en">copper</skos:prefLabel>
	<skos:prefLabel xml:lang="de">Kupfer</skos:prefLabel>
	<skos:prefLabel xml:lang="pt">cobre</skos:prefLabel>
	<skos:prefLabel xml:lang="sv">koppar (material)</skos:prefLabel>
	<skos:prefLabel xml:lang="hr">bakar</skos:prefLabel>
	<skos:prefLabel xml:lang="fi">kupari</skos:prefLabel>
	<skos:inScheme rdf:resource="http://partage.vocnet.org/Materials"/>
	<skos:broader rdf:resource="http://partage.vocnet.org/part00265"/>
	<skos:exactMatch rdf:resource="http://vocab.getty.edu/aat/300011020"/>
	<skos:editorialNote xml:lang="en">PPMaterial</skos:editorialNote>
	<skos:scopeNote xml:lang="en">Pure metallic element having the symbol Cu and atomic number 29; a reddish brown, ductile metal that is present in the earth's crust, occurring as a native metal and as ores of sulfide, sulfate and carbonate (azurite, malachite, etc.). It was the first metal used by humans, probably from about 8000 BCE, in the regions of Mesopotamia and India. By about 3800 BCE copper was made into bronze for weapons and knives. Today, copper is one of the most widely used metals because it has high electrical and thermal conductivity, can be easily fabricated, is ductile and polishes well. In moist air, copper forms a protective green film of basic carbonate. Metallic copper combines well with other metals to form alloys, most commonly brass and bronze. Copper and its alloys are used for wire, electrical devices, pipes, cooking vessels, ammunition, ornamental trim, roofing, grillwork, coins, musical instruments, jewelry, and sculptures.</skos:scopeNote>
</skos:Concept>
<skos:Concept rdf:about="http://partage.vocnet.org/part00272">
	<skos:prefLabel xml:lang="en">copper alloy</skos:prefLabel>
	<skos:inScheme rdf:resource="http://partage.vocnet.org/Materials"/>
	<skos:broader rdf:resource="http://partage.vocnet.org/part00265"/>
	<skos:narrower rdf:resource="http://partage.vocnet.org/part00273"/>
	<skos:narrower rdf:resource="http://partage.vocnet.org/part00274"/>
	<skos:exactMatch rdf:resource="http://vocab.getty.edu/aat/300010942"/>
	<skos:scopeNote xml:lang="en">Alloy in which copper is the principle element.</skos:scopeNote>
</skos:Concept>
<skos:Concept rdf:about="http://partage.vocnet.org/part00273">
	<skos:altLabel xml:lang="en">brass (alloy)</skos:altLabel>
	<skos:prefLabel xml:lang="en">brass</skos:prefLabel>
	<skos:prefLabel xml:lang="de">Messing</skos:prefLabel>
	<skos:prefLabel xml:lang="sv">mässing</skos:prefLabel>
	<skos:prefLabel xml:lang="pt">latão</skos:prefLabel>
	<skos:prefLabel xml:lang="hr">mjed</skos:prefLabel>
	<skos:prefLabel xml:lang="fi">messinki</skos:prefLabel>
	<skos:inScheme rdf:resource="http://partage.vocnet.org/Materials"/>
	<skos:broader rdf:resource="http://partage.vocnet.org/part00272"/>
	<skos:exactMatch rdf:resource="http://vocab.getty.edu/aat/300010946"/>
	<skos:editorialNote xml:lang="en">PPMaterial</skos:editorialNote>
	<skos:scopeNote xml:lang="en">Alloy of copper and zinc, usually with copper as the major alloying element and zinc up to 40% by weight.</skos:scopeNote>
</skos:Concept>
<skos:Concept rdf:about="http://partage.vocnet.org/part00274">
	<skos:altLabel xml:lang="en">bronze (metal)</skos:altLabel>
	<skos:prefLabel xml:lang="en">bronze</skos:prefLabel>
	<skos:prefLabel xml:lang="de">Bronze</skos:prefLabel>
	<skos:prefLabel xml:lang="sv">brons</skos:prefLabel>
	<skos:prefLabel xml:lang="pt">bronze</skos:prefLabel>
	<skos:prefLabel xml:lang="fi">pronssi</skos:prefLabel>
	<skos:prefLabel xml:lang="hr">bronca</skos:prefLabel>
	<skos:inScheme rdf:resource="http://partage.vocnet.org/Materials"/>
	<skos:broader rdf:resource="http://partage.vocnet.org/part00272"/>
	<skos:exactMatch rdf:resource="http://vocab.getty.edu/aat/300010957"/>
	<skos:editorialNote xml:lang="en">PPMaterial</skos:editorialNote>
	<skos:scopeNote xml:lang="en">Refers to a broad range of alloys of copper, specifically any non-ferrous alloy of copper, tin, and zinc or other trace metals. Bronze was made before 3,000 BCE -- possibly as early as 10,000 BCE, although its common use in tools and decorative items is dated only in later artifacts. The proportions of copper and tin vary widely, from 70 to 95 percent copper in surviving ancient artifacts. Because of the copper base, bronze may be very malleable and easy to work. By the Middle Ages in Europe, it was recognized that using the metals in certain proportions could yield specific properties. Some modern bronzes contain no tin at all, substituting other metals such as aluminum, manganese, and even zinc. Historically, the term was used interchangeably with "latten." U.S. standard bronze is composed of 90% copper, 7% tin and 3% zinc. Ancient bronze alloys sometimes contained up to 14% tin.</skos:scopeNote>
</skos:Concept>
<skos:Concept rdf:about="http://partage.vocnet.org/part00276">
	<skos:altLabel xml:lang="en">lead (metal)</skos:altLabel>
	<skos:prefLabel xml:lang="en">lead</skos:prefLabel>
	<skos:prefLabel xml:lang="sv">bly</skos:prefLabel>
	<skos:prefLabel xml:lang="pt">chumbo</skos:prefLabel>
	<skos:prefLabel xml:lang="de">Blei</skos:prefLabel>
	<skos:prefLabel xml:lang="fi">lyijy</skos:prefLabel>
	<skos:prefLabel xml:lang="hr">olovo</skos:prefLabel>
	<skos:inScheme rdf:resource="http://partage.vocnet.org/Materials"/>
	<skos:broader rdf:resource="http://partage.vocnet.org/part00265"/>
	<skos:exactMatch rdf:resource="http://vocab.getty.edu/aat/300011022"/>
	<skos:editorialNote xml:lang="en">PPMaterial</skos:editorialNote>
	<skos:scopeNote xml:lang="en">Pure metallic element having symbol Pb and atomic number 82; soft, dense ductile metal of a dull gray color, shiny when freshly cut, occuring naturally most often as a sulfide in the mineral galena. Other lead minerals include anglesite (lead sulfate) and cerussite (lead carbonate). Native metallic lead was found and used from about 3600-2600 BCE when the technique for obtaining lead from roasting the sulfide ore (galena) was discovered. Lead was used to make small cast items such as coins and statuettes, plumbing pipes, spires, statues, cisterns, gargoyles, pigments (lead white, litharge, orange mineral, etc.), as a component in pottery glazes, for roofing, flashing, stained glass windows, as a soft solder, and as radiation shielding.</skos:scopeNote>
</skos:Concept>
<skos:Concept rdf:about="http://partage.vocnet.org/part00278">
	<skos:altLabel xml:lang="en">tin (metal)</skos:altLabel>
	<skos:prefLabel xml:lang="en">tin</skos:prefLabel>
	<skos:prefLabel xml:lang="sv">tenn</skos:prefLabel>
	<skos:prefLabel xml:lang="pt">lata.</skos:prefLabel>
	<skos:prefLabel xml:lang="de">Zinn.</skos:prefLabel>
	<skos:altLabel xml:lang="de">Blech</skos:altLabel>
	<skos:prefLabel xml:lang="hr">lim</skos:prefLabel>
	<skos:prefLabel xml:lang="fi">tina.</skos:prefLabel>
	<skos:inScheme rdf:resource="http://partage.vocnet.org/Materials"/>
	<skos:broader rdf:resource="http://partage.vocnet.org/part00265"/>
	<skos:exactMatch rdf:resource="http://vocab.getty.edu/aat/300133748"/>
	<skos:editorialNote xml:lang="en">PPMaterial</skos:editorialNote>
	<skos:scopeNote xml:lang="en">Pure metallic element having symbol Sn and atomic number 50; a soft, pliable, silvery white metal. Use also for this metal as processed and formed, usually in combination with other substances, to make various objects and materials.</skos:scopeNote>
</skos:Concept>
<skos:Concept rdf:about="http://partage.vocnet.org/part00279">
	<skos:prefLabel xml:lang="en">tin alloy</skos:prefLabel>
	<skos:inScheme rdf:resource="http://partage.vocnet.org/Materials"/>
	<skos:broader rdf:resource="http://partage.vocnet.org/part00265"/>
	<skos:narrower rdf:resource="http://partage.vocnet.org/part00280"/>
	<skos:exactMatch rdf:resource="http://vocab.getty.edu/aat/300010978"/>
	<skos:scopeNote xml:lang="en">Alloy in which tin is the principle component.</skos:scopeNote>
</skos:Concept>
<skos:Concept rdf:about="http://partage.vocnet.org/part00280">
	<skos:altLabel xml:lang="en">pewter (tin alloy)</skos:altLabel>
	<skos:prefLabel xml:lang="en">pewter</skos:prefLabel>
	<skos:prefLabel xml:lang="sv">hårdtenn</skos:prefLabel>
	<skos:prefLabel xml:lang="pt">estanho</skos:prefLabel>
	<skos:prefLabel xml:lang="de">Zinn</skos:prefLabel>
	<skos:prefLabel xml:lang="fi">tina</skos:prefLabel>
	<skos:prefLabel xml:lang="hr">kositar</skos:prefLabel>
	<skos:inScheme rdf:resource="http://partage.vocnet.org/Materials"/>
	<skos:broader rdf:resource="http://partage.vocnet.org/part00279"/>
	<skos:exactMatch rdf:resource="http://vocab.getty.edu/aat/300010979"/>
	<skos:editorialNote xml:lang="en">PPMaterial</skos:editorialNote>
	<skos:scopeNote xml:lang="en">Alloy of tin and various proportions and combinations of lead and antimony, and sometimes also copper.</skos:scopeNote>
</skos:Concept>
<skos:Concept rdf:about="http://partage.vocnet.org/part00281">
	<skos:prefLabel xml:lang="en">mineral</skos:prefLabel>
	<skos:prefLabel xml:lang="sv">mineral</skos:prefLabel>
	<skos:prefLabel xml:lang="pt">mineral</skos:prefLabel>
	<skos:prefLabel xml:lang="de">Mineral</skos:prefLabel>
	<skos:prefLabel xml:lang="fi">mineraali</skos:prefLabel>
	<skos:prefLabel xml:lang="hr">mineral</skos:prefLabel>
	<skos:inScheme rdf:resource="http://partage.vocnet.org/Materials"/>
	<skos:broader rdf:resource="http://partage.vocnet.org/part00229"/>
	<skos:narrower rdf:resource="http://partage.vocnet.org/part00905"/>
	<skos:exactMatch rdf:resource="http://vocab.getty.edu/aat/300011068"/>
	<skos:editorialNote xml:lang="en">PPMaterial</skos:editorialNote>
	<skos:scopeNote xml:lang="en">Naturally occurring inorganic element or compound having an orderly internal structure and characteristic chemical composition, crystal form, and physical properties; use also for synthetically derived equivalents.</skos:scopeNote>
</skos:Concept>
<skos:Concept rdf:about="http://partage.vocnet.org/part00288">
	<skos:altLabel xml:lang="en">cotton (textile)</skos:altLabel>
	<skos:prefLabel xml:lang="en">cotton</skos:prefLabel>
	<skos:prefLabel xml:lang="de">Baumwolle</skos:prefLabel>
	<skos:prefLabel xml:lang="sv">bomull</skos:prefLabel>
	<skos:prefLabel xml:lang="pt">algodão</skos:prefLabel>
	<skos:prefLabel xml:lang="fi">puuvilla</skos:prefLabel>
	<skos:prefLabel xml:lang="hr">pamuk</skos:prefLabel>
	<skos:inScheme rdf:resource="http://partage.vocnet.org/Materials"/>
	<skos:broader rdf:resource="http://partage.vocnet.org/part00229"/>
	<skos:narrower rdf:resource="http://partage.vocnet.org/part00612"/>
	<skos:narrower rdf:resource="http://partage.vocnet.org/part01210"/>
	<skos:exactMatch rdf:resource="http://vocab.getty.edu/aat/300014067"/>
	<skos:scopeNote xml:lang="en">Textile made from cotton fiber.</skos:scopeNote>
	<skos:editorialNote xml:lang="en">PPMaterial</skos:editorialNote>
</skos:Concept>
<skos:Concept rdf:about="http://partage.vocnet.org/part00289">
	<skos:altLabel xml:lang="en">linen (material)</skos:altLabel>
	<skos:prefLabel xml:lang="en">linen</skos:prefLabel>
	<skos:prefLabel xml:lang="sv">linne</skos:prefLabel>
	<skos:prefLabel xml:lang="pt">linho</skos:prefLabel>
	<skos:prefLabel xml:lang="de">Leinen</skos:prefLabel>
	<skos:prefLabel xml:lang="fi">pellava</skos:prefLabel>
	<skos:prefLabel xml:lang="hr">lan</skos:prefLabel>
	<skos:inScheme rdf:resource="http://partage.vocnet.org/Materials"/>
	<skos:broader rdf:resource="http://partage.vocnet.org/part00229"/>
	<skos:exactMatch rdf:resource="http://vocab.getty.edu/aat/300014069"/>
	<skos:editorialNote xml:lang="en">PPMaterial</skos:editorialNote>
	<skos:scopeNote xml:lang="en">General name for textile woven from the spun fiber of the flax plant.</skos:scopeNote>
</skos:Concept>
<skos:Concept rdf:about="http://partage.vocnet.org/part00290">
	<skos:altLabel xml:lang="en">silk (textile)</skos:altLabel>
	<skos:prefLabel xml:lang="en">silk</skos:prefLabel>
	<skos:prefLabel xml:lang="sv">siden</skos:prefLabel>
	<skos:prefLabel xml:lang="pt">seda</skos:prefLabel>
	<skos:prefLabel xml:lang="de">Seide</skos:prefLabel>
	<skos:prefLabel xml:lang="hr">svila</skos:prefLabel>
	<skos:prefLabel xml:lang="fi">silkki</skos:prefLabel>
	<skos:inScheme rdf:resource="http://partage.vocnet.org/Materials"/>
	<skos:broader rdf:resource="http://partage.vocnet.org/part00229"/>
	<skos:narrower rdf:resource="http://partage.vocnet.org/part00291"/>
	<skos:exactMatch rdf:resource="http://vocab.getty.edu/aat/300243428"/>
	<skos:scopeNote xml:lang="en">Textile made from silk fiber, which is a fiber derived from the cocoon of the silkworm moth.</skos:scopeNote>
	<skos:editorialNote xml:lang="en">PPMaterial</skos:editorialNote>
</skos:Concept>
<skos:Concept rdf:about="http://partage.vocnet.org/part00291">
	<skos:prefLabel xml:lang="en">organza</skos:prefLabel>
	<skos:prefLabel xml:lang="sv">organza</skos:prefLabel>
	<skos:prefLabel xml:lang="pt">organza</skos:prefLabel>
	<skos:prefLabel xml:lang="de">Organza</skos:prefLabel>
	<skos:prefLabel xml:lang="fi">organza</skos:prefLabel>
	<skos:prefLabel xml:lang="hr">organza</skos:prefLabel>
	<skos:inScheme rdf:resource="http://partage.vocnet.org/Materials"/>
	<skos:broader rdf:resource="http://partage.vocnet.org/part00290"/>
	<skos:exactMatch rdf:resource="http://vocab.getty.edu/aat/300310123"/>
	<skos:editorialNote xml:lang="en">PPMaterial</skos:editorialNote>
	<skos:scopeNote xml:lang="en">Sheer, crisp fabric made with a loose plain weave; usually made from silk or synthetics such as rayon, nylon, acrylic or polyester. It is fine to leightweight, strong, stable, and durable. It is distinct from organdy, which is made from cotton.</skos:scopeNote>
</skos:Concept>
<skos:Concept rdf:about="http://partage.vocnet.org/part00292">
	<skos:altLabel xml:lang="en">luster (textile)</skos:altLabel>
	<skos:prefLabel xml:lang="en">lustre (textile)</skos:prefLabel>
	<skos:prefLabel xml:lang="sv">lyster</skos:prefLabel>
	<skos:prefLabel xml:lang="pt">pano de polir</skos:prefLabel>
	<skos:prefLabel xml:lang="de">Lüstergewebe</skos:prefLabel>
	<skos:prefLabel xml:lang="hr">lister</skos:prefLabel>
	<skos:inScheme rdf:resource="http://partage.vocnet.org/Materials"/>
	<skos:broader rdf:resource="http://partage.vocnet.org/part00229"/>
	<skos:exactMatch rdf:resource="http://vocab.getty.edu/aat/300231608"/>
	<skos:scopeNote xml:lang="en">Textile made with cotton, silk, or linen warp and wool, mohair, alpaca, or some other glossy hair fiber as weft in order to produce a lustrous surface.</skos:scopeNote>
	<skos:editorialNote xml:lang="en">PPMaterial</skos:editorialNote>
</skos:Concept>
<skos:Concept rdf:about="http://partage.vocnet.org/part00295">
	<skos:altLabel xml:lang="en">wood (plant material)</skos:altLabel>
	<skos:prefLabel xml:lang="en">wood</skos:prefLabel>
	<skos:prefLabel xml:lang="sv">trä</skos:prefLabel>
	<skos:prefLabel xml:lang="pt">madeira</skos:prefLabel>
	<skos:prefLabel xml:lang="de">Holz</skos:prefLabel>
	<skos:prefLabel xml:lang="fi">puu</skos:prefLabel>
	<skos:prefLabel xml:lang="hr">drvo</skos:prefLabel>
	<skos:inScheme rdf:resource="http://partage.vocnet.org/Materials"/>
	<skos:broader rdf:resource="http://partage.vocnet.org/part00297"/>
	<skos:narrower rdf:resource="http://partage.vocnet.org/part00606"/>
	<skos:narrower rdf:resource="http://partage.vocnet.org/part00617"/>
	<skos:narrower rdf:resource="http://partage.vocnet.org/part01221"/>
	<skos:exactMatch rdf:resource="http://vocab.getty.edu/aat/300011914"/>
	<skos:editorialNote xml:lang="en">PPMaterial</skos:editorialNote>
	<skos:scopeNote xml:lang="en">The principal tissue of trees and other plants that provides both strength and a means of conducting nutrients. Wood is one of the most versatile materials known</skos:scopeNote>
</skos:Concept>
<skos:Concept rdf:about="http://partage.vocnet.org/part00297">
	<skos:prefLabel xml:lang="en">plant material</skos:prefLabel>
	<skos:inScheme rdf:resource="http://partage.vocnet.org/Materials"/>
	<skos:broader rdf:resource="http://partage.vocnet.org/part00229"/>
	<skos:narrower rdf:resource="http://partage.vocnet.org/part00295"/>
	<skos:narrower rdf:resource="http://partage.vocnet.org/part00570"/>
	<skos:narrower rdf:resource="http://partage.vocnet.org/part00585"/>
	<skos:narrower rdf:resource="http://partage.vocnet.org/part00624"/>
	<skos:narrower rdf:resource="http://partage.vocnet.org/part01148"/>
	<skos:narrower rdf:resource="http://partage.vocnet.org/part01211"/>
	<skos:exactMatch rdf:resource="http://vocab.getty.edu/aat/00124117"/>
</skos:Concept>
<skos:Concept rdf:about="http://partage.vocnet.org/part00394">
	<skos:altLabel xml:lang="en">fabrics (textile materials)</skos:altLabel>
	<skos:prefLabel xml:lang="en">cloth</skos:prefLabel>
	<skos:altLabel xml:lang="de">Stoff (Gewebe)</skos:altLabel>
	<skos:altLabel xml:lang="de">Gewebe</skos:altLabel>
	<skos:prefLabel xml:lang="de">Tuch</skos:prefLabel>
	<skos:prefLabel xml:lang="sv">textil</skos:prefLabel>
	<skos:altLabel xml:lang="pt">pano</skos:altLabel>
	<skos:prefLabel xml:lang="pt">tecido</skos:prefLabel>
	<skos:altLabel xml:lang="hr">tkanina</skos:altLabel>
	<skos:prefLabel xml:lang="hr">sukno</skos:prefLabel>
	<skos:prefLabel xml:lang="fi">kangas</skos:prefLabel>
	<skos:inScheme rdf:resource="http://partage.vocnet.org/Materials"/>
	<skos:broader rdf:resource="http://partage.vocnet.org/part00229"/>
	<skos:exactMatch rdf:resource="http://vocab.getty.edu/aat/300162391"/>
	<skos:editorialNote xml:lang="en">PPMaterial</skos:editorialNote>
	<skos:scopeNote xml:lang="en">Generally, textile that is woven, felted, knit, pounded, or otherwise made into a flat piece. For textile in the form of continuous strands made from filaments of fiber by reeling, spinning, twisting, or throwing, see "yarn."</skos:scopeNote>
</skos:Concept>
<skos:Concept rdf:about="http://partage.vocnet.org/part00484">
	<skos:altLabel xml:lang="en">ivory (tooth component)</skos:altLabel>
	<skos:prefLabel xml:lang="en">ivory</skos:prefLabel>
	<skos:prefLabel xml:lang="de">Elfenbein</skos:prefLabel>
	<skos:prefLabel xml:lang="pt">marfim</skos:prefLabel>
	<skos:prefLabel xml:lang="sv">elfenben</skos:prefLabel>
	<skos:prefLabel xml:lang="hr">bjelokost</skos:prefLabel>
	<skos:prefLabel xml:lang="fi">norsunluu</skos:prefLabel>
	<skos:inScheme rdf:resource="http://partage.vocnet.org/Materials"/>
	<skos:broader rdf:resource="http://partage.vocnet.org/part00485"/>
	<skos:exactMatch rdf:resource="http://vocab.getty.edu/aat/300011857"/>
	<skos:editorialNote xml:lang="en">PPMaterial</skos:editorialNote>
	<skos:scopeNote xml:lang="en">The modified form of dentine found on the tusks of mature elephants, and for similar material from any tusked or large-toothed mammal such as a walrus or narwhal.</skos:scopeNote>
</skos:Concept>
<skos:Concept rdf:about="http://partage.vocnet.org/part00485">
	<skos:prefLabel xml:lang="en">dentin</skos:prefLabel>
	<skos:inScheme rdf:resource="http://partage.vocnet.org/Materials"/>
	<skos:broader rdf:resource="http://partage.vocnet.org/part00489"/>
	<skos:narrower rdf:resource="http://partage.vocnet.org/part00484"/>
	<skos:exactMatch rdf:resource="http://vocab.getty.edu/aat/300191881"/>
	<skos:scopeNote xml:lang="en">Calcareous materials similar to bones but harder and denser that compose the principal parts of teeth.</skos:scopeNote>
</skos:Concept>
<skos:Concept rdf:about="http://partage.vocnet.org/part00489">
	<skos:altLabel xml:lang="en">bone (material)</skos:altLabel>
	<skos:prefLabel xml:lang="en">bone</skos:prefLabel>
	<skos:prefLabel xml:lang="de">Knochen</skos:prefLabel>
	<skos:altLabel xml:lang="de">Gebein</skos:altLabel>
	<skos:prefLabel xml:lang="sv">ben</skos:prefLabel>
	<skos:prefLabel xml:lang="pt">osso</skos:prefLabel>
	<skos:prefLabel xml:lang="fi">luu</skos:prefLabel>
	<skos:prefLabel xml:lang="hr">kost</skos:prefLabel>
	<skos:inScheme rdf:resource="http://partage.vocnet.org/Materials"/>
	<skos:broader rdf:resource="http://partage.vocnet.org/part00229"/>
	<skos:narrower rdf:resource="http://partage.vocnet.org/part00485"/>
	<skos:exactMatch rdf:resource="http://vocab.getty.edu/aat/300011798"/>
	<skos:editorialNote xml:lang="en">PPMaterial</skos:editorialNote>
	<skos:scopeNote xml:lang="en">The rigid, calcareous material that is white in color and forms the skeleton of vertebrates; primarily composed of calcium hydroxyapatite with smaller amounts of calcium carbonate, calcium fluoride, magnesium phosphate, and ossein, a high molecular weight protein. Bones have a concentric structure with central lymphatic canals surrounded by a spongy lamellar region protected by a dense outer cortex. Bone has been carved and used since ancient times for many purposes, including fish-hooks, spear heads, needles, handles, and art objects. Bones were also burnt to produce bone black and boiled to produce bone glue. Bone can be distinguished from ivory by being generally whiter, more porous, and less dense.</skos:scopeNote>
</skos:Concept>
<skos:Concept rdf:about="http://partage.vocnet.org/part00514">
	<skos:prefLabel xml:lang="en">cameo glass</skos:prefLabel>
	<skos:prefLabel xml:lang="de">Kamee</skos:prefLabel>
	<skos:prefLabel xml:lang="pt">vidro dobrado</skos:prefLabel>
	<skos:prefLabel xml:lang="hr">kameo staklo</skos:prefLabel>
	<skos:prefLabel xml:lang="fi">verholasi</skos:prefLabel>
	<skos:inScheme rdf:resource="http://partage.vocnet.org/Materials"/>
	<skos:broader rdf:resource="http://partage.vocnet.org/part00247"/>
	<skos:exactMatch rdf:resource="http://vocab.getty.edu/aat/300181908"/>
	<skos:editorialNote xml:lang="en">PPMaterial</skos:editorialNote>
	<skos:scopeNote xml:lang="en">Cased glass of two or more layers in contrasting colors. The outer layers are carved, cut, or engraved to produce a design which stands out from the background.</skos:scopeNote>
</skos:Concept>
<skos:Concept rdf:about="http://partage.vocnet.org/part00515">
	<skos:altLabel xml:lang="en">iron (metal)</skos:altLabel>
	<skos:prefLabel xml:lang="en">iron</skos:prefLabel>
	<skos:prefLabel xml:lang="sv">järn</skos:prefLabel>
	<skos:prefLabel xml:lang="pt">ferro</skos:prefLabel>
	<skos:prefLabel xml:lang="de">Eisen</skos:prefLabel>
	<skos:prefLabel xml:lang="fi">rauta</skos:prefLabel>
	<skos:prefLabel xml:lang="hr">željezo</skos:prefLabel>
	<skos:inScheme rdf:resource="http://partage.vocnet.org/Materials"/>
	<skos:broader rdf:resource="http://partage.vocnet.org/part00259"/>
	<skos:exactMatch rdf:resource="http://vocab.getty.edu/aat/300011002"/>
	<skos:editorialNote xml:lang="en">PPMaterial</skos:editorialNote>
	<skos:scopeNote xml:lang="en">Pure metallic element having symbol Fe and atomic number 26; metallic iron is silvery in color, lustrous, soft, ductile, malleable, and slightly magnetic; it rusts when exposed to moist air. It is rarely found as a native metal (telluric iron) except in meteorites (meteoric iron). Iron is most often found throughout the world as iron oxides (hematite, magnetite, limonite, and siderite) mixed with other ores.</skos:scopeNote>
</skos:Concept>
<skos:Concept rdf:about="http://partage.vocnet.org/part00516">
	<skos:altLabel xml:lang="en">marble (rock)</skos:altLabel>
	<skos:prefLabel xml:lang="en">marble</skos:prefLabel>
	<skos:prefLabel xml:lang="sv">marmor</skos:prefLabel>
	<skos:prefLabel xml:lang="pt">mármore</skos:prefLabel>
	<skos:prefLabel xml:lang="de">Marmor</skos:prefLabel>
	<skos:prefLabel xml:lang="fi">marmori</skos:prefLabel>
	<skos:prefLabel xml:lang="hr">mramor</skos:prefLabel>
	<skos:inScheme rdf:resource="http://partage.vocnet.org/Materials"/>
	<skos:broader rdf:resource="http://partage.vocnet.org/part00517"/>
	<skos:exactMatch rdf:resource="http://vocab.getty.edu/aat/300011443"/>
	<skos:editorialNote xml:lang="en">PPMaterial</skos:editorialNote>
	<skos:scopeNote xml:lang="en">A metamorphic, hard, dense, crystalline stone primarily composed of calcium carbonate; it is limestone or dolomite that has been metamorphosed with heat and pressure. Pure calcite marble is white, but impurities produce a wide variety of coloring and patterns. It is finely grained and polishes to a smooth, high gloss. It is used primarily for statuary and buildings. Marble has been quarried from sites around the world since at least the 7th century BCE. The term can also refer more broadly to any crystallized carbonate rock, including true marble and certain types of limestone, that will take a polish and can be used for architectural and ornamental purposes.</skos:scopeNote>
</skos:Concept>
<skos:Concept rdf:about="http://partage.vocnet.org/part00517">
	<skos:prefLabel xml:lang="en">metamorphic rock</skos:prefLabel>
	<skos:inScheme rdf:resource="http://partage.vocnet.org/Materials"/>
	<skos:broader rdf:resource="http://partage.vocnet.org/part00518"/>
	<skos:narrower rdf:resource="http://partage.vocnet.org/part00516"/>
	<skos:exactMatch rdf:resource="http://vocab.getty.edu/aat/300011437"/>
	<skos:scopeNote xml:lang="en">Rocks that result from the alteration of pre-existing rocks in response to changing environmental conditions, such as variations in temperature, pressure, and mechanical stress, and the addition or subtraction of chemical components. The pre-existing rocks may be igneous, sedimentary, or other metamorphic rocks.</skos:scopeNote>
</skos:Concept>
<skos:Concept rdf:about="http://partage.vocnet.org/part00518">
	<skos:prefLabel xml:lang="en">rock</skos:prefLabel>
	<skos:inScheme rdf:resource="http://partage.vocnet.org/Materials"/>
	<skos:broader rdf:resource="http://partage.vocnet.org/part00229"/>
	<skos:narrower rdf:resource="http://partage.vocnet.org/part00517"/>
	<skos:narrower rdf:resource="http://partage.vocnet.org/part00536"/>
	<skos:narrower rdf:resource="http://partage.vocnet.org/part00597"/>
	<skos:exactMatch rdf:resource="http://vocab.getty.edu/aat/300011692"/>
	<skos:scopeNote xml:lang="en">Naturally formed aggregate of one or more minerals. For processed or dressed rock use "stone."</skos:scopeNote>
</skos:Concept>
<skos:Concept rdf:about="http://partage.vocnet.org/part00519">
	<skos:prefLabel xml:lang="en">mother of pearl</skos:prefLabel>
	<skos:prefLabel xml:lang="de">Perlmutt</skos:prefLabel>
	<skos:prefLabel xml:lang="hr">sedef</skos:prefLabel>
	<skos:inScheme rdf:resource="http://partage.vocnet.org/Materials"/>
	<skos:broader rdf:resource="http://partage.vocnet.org/part00229"/>
	<skos:exactMatch rdf:resource="http://vocab.getty.edu/aat/300011835"/>
	<skos:editorialNote xml:lang="en">PPSpecialistTerms</skos:editorialNote>
	<skos:scopeNote xml:lang="en">Hard, pearly, iridescent internal layer of various kinds of mollusk shell, extensively used for making small articles and inlays.</skos:scopeNote>
	<skos:editorialNote xml:lang="de">PPMaterial</skos:editorialNote>
</skos:Concept>
<skos:Concept rdf:about="http://partage.vocnet.org/part00521">
	<skos:prefLabel xml:lang="en">tortoise shell</skos:prefLabel>
	<skos:inScheme rdf:resource="http://partage.vocnet.org/Materials"/>
	<skos:broader rdf:resource="http://partage.vocnet.org/part00257"/>
	<skos:exactMatch rdf:resource="http://vocab.getty.edu/aat/300011837"/>
	<skos:editorialNote xml:lang="en">PPSpecialistTerms</skos:editorialNote>
	<skos:scopeNote xml:lang="en">Material made from the thinly sliced horny plates covering the shells of some turtles and tortoises. It was popular in the 19th-century for inlays, jewelry, hair combs, and other ornaments, but its use is banned today.</skos:scopeNote>
	<skos:editorialNote xml:lang="de">PPMaterial</skos:editorialNote>
</skos:Concept>
<skos:Concept rdf:about="http://partage.vocnet.org/part00534">
	<skos:prefLabel xml:lang="en">sandstone</skos:prefLabel>
	<skos:prefLabel xml:lang="sv">sandsten</skos:prefLabel>
	<skos:prefLabel xml:lang="pt">grés.</skos:prefLabel>
	<skos:prefLabel xml:lang="de">Sandstein</skos:prefLabel>
	<skos:prefLabel xml:lang="hr">pješčenjak</skos:prefLabel>
	<skos:prefLabel xml:lang="fi">hiekkakivi</skos:prefLabel>
	<skos:inScheme rdf:resource="http://partage.vocnet.org/Materials"/>
	<skos:broader rdf:resource="http://partage.vocnet.org/part00536"/>
	<skos:exactMatch rdf:resource="http://vocab.getty.edu/aat/300011376"/>
	<skos:editorialNote xml:lang="en">PPMaterial</skos:editorialNote>
	<skos:scopeNote xml:lang="en">A consolidated sedimentary rock, consisting of sand grains united with a natural cementing material; the most common sand in sandstone contains quartz, with considerable feldspar, lime, mica, and clayey matter.</skos:scopeNote>
</skos:Concept>
<skos:Concept rdf:about="http://partage.vocnet.org/part00536">
	<skos:prefLabel xml:lang="en">sedimentary rock</skos:prefLabel>
	<skos:inScheme rdf:resource="http://partage.vocnet.org/Materials"/>
	<skos:broader rdf:resource="http://partage.vocnet.org/part00518"/>
	<skos:narrower rdf:resource="http://partage.vocnet.org/part00534"/>
	<skos:exactMatch rdf:resource="http://vocab.getty.edu/aat/300011273"/>
	<skos:scopeNote xml:lang="en">Rock, such as sandstone or limestone, formed from materials deposited as sediments.</skos:scopeNote>
</skos:Concept>
<skos:Concept rdf:about="http://partage.vocnet.org/part00537">
	<skos:altLabel xml:lang="en">steel (alloy)</skos:altLabel>
	<skos:prefLabel xml:lang="en">steel</skos:prefLabel>
	<skos:prefLabel xml:lang="sv">stål</skos:prefLabel>
	<skos:prefLabel xml:lang="pt">aço</skos:prefLabel>
	<skos:prefLabel xml:lang="de">Stahl</skos:prefLabel>
	<skos:prefLabel xml:lang="fi">teräs</skos:prefLabel>
	<skos:prefLabel xml:lang="hr">čelik</skos:prefLabel>
	<skos:inScheme rdf:resource="http://partage.vocnet.org/Materials"/>
	<skos:broader rdf:resource="http://partage.vocnet.org/part00261"/>
	<skos:exactMatch rdf:resource="http://vocab.getty.edu/aat/300133751"/>
	<skos:editorialNote xml:lang="en">PPMaterial</skos:editorialNote>
	<skos:scopeNote xml:lang="en">Any of various hard, strong, durable, malleable alloys of iron and carbon, often with other elements such as manganese, chromium, nickel, molybdenum, copper, tungsten, cobalt, or silicon; widely used as a structural material.</skos:scopeNote>
</skos:Concept>
<skos:Concept rdf:about="http://partage.vocnet.org/part00538">
	<skos:prefLabel xml:lang="en">veneer</skos:prefLabel>
	<skos:prefLabel xml:lang="de">Furnier</skos:prefLabel>
	<skos:prefLabel xml:lang="pt">embutido</skos:prefLabel>
	<skos:prefLabel xml:lang="sv">faner</skos:prefLabel>
	<skos:prefLabel xml:lang="fi">viilu</skos:prefLabel>
	<skos:prefLabel xml:lang="hr">furnir</skos:prefLabel>
	<skos:inScheme rdf:resource="http://partage.vocnet.org/Materials"/>
	<skos:broader rdf:resource="http://partage.vocnet.org/part00229"/>
	<skos:exactMatch rdf:resource="http://vocab.getty.edu/aat/300012855"/>
	<skos:editorialNote xml:lang="en">PPMaterial</skos:editorialNote>
	<skos:scopeNote xml:lang="en">Thin sheets of decorative material, usually wood, but also occasionally ivory, tortoiseshell or brass, used to cover the surface of furniture or another object constructed of coarser and cheaper wood.</skos:scopeNote>
</skos:Concept>
<skos:Concept rdf:about="http://partage.vocnet.org/part00539">
	<skos:prefLabel xml:lang="en">wicker</skos:prefLabel>
	<skos:prefLabel xml:lang="sv">korg</skos:prefLabel>
	<skos:altLabel xml:lang="de">Rattan</skos:altLabel>
	<skos:prefLabel xml:lang="pt">verga</skos:prefLabel>
	<skos:prefLabel xml:lang="de">Geflecht</skos:prefLabel>
	<skos:prefLabel xml:lang="hr">šiblje</skos:prefLabel>
	<skos:prefLabel xml:lang="fi">korityö</skos:prefLabel>
	<skos:inScheme rdf:resource="http://partage.vocnet.org/Materials"/>
	<skos:broader rdf:resource="http://partage.vocnet.org/part00229"/>
	<skos:exactMatch rdf:resource="http://vocab.getty.edu/aat/300014690"/>
	<skos:editorialNote xml:lang="en">PPMaterial</skos:editorialNote>
	<skos:scopeNote xml:lang="en">Woven reed, rattan, twigs, or other material, especially used to construct furniture.</skos:scopeNote>
</skos:Concept>
<skos:Concept rdf:about="http://partage.vocnet.org/part00563">
	<skos:prefLabel xml:lang="en">aluminium</skos:prefLabel>
	<skos:prefLabel xml:lang="de">Aluminium</skos:prefLabel>
	<skos:prefLabel xml:lang="sv">aluminium</skos:prefLabel>
	<skos:prefLabel xml:lang="pt">alumínio</skos:prefLabel>
	<skos:prefLabel xml:lang="fi">alumiini</skos:prefLabel>
	<skos:prefLabel xml:lang="hr">aluminij</skos:prefLabel>
	<skos:inScheme rdf:resource="http://partage.vocnet.org/Materials"/>
	<skos:broader rdf:resource="http://partage.vocnet.org/part00265"/>
	<skos:exactMatch rdf:resource="http://vocab.getty.edu/aat/300011015"/>
	<skos:editorialNote xml:lang="en">PPMaterial</skos:editorialNote>
	<skos:scopeNote xml:lang="en">Pure metallic element having symbol Al and atomic number 13; a hard, strong, silver white metal. This metal is also processed and formed, usually in combination with other substances, to make objects and materials.</skos:scopeNote>
</skos:Concept>
<skos:Concept rdf:about="http://partage.vocnet.org/part00565">
	<skos:prefLabel xml:lang="en">batiste</skos:prefLabel>
	<skos:prefLabel xml:lang="de">Batist</skos:prefLabel>
	<skos:prefLabel xml:lang="sv">batist</skos:prefLabel>
	<skos:prefLabel xml:lang="pt">cambraia</skos:prefLabel>
	<skos:prefLabel xml:lang="hr">batist</skos:prefLabel>
	<skos:prefLabel xml:lang="fi">batisti</skos:prefLabel>
	<skos:inScheme rdf:resource="http://partage.vocnet.org/Materials"/>
	<skos:broader rdf:resource="http://partage.vocnet.org/part00229"/>
	<skos:exactMatch rdf:resource="http://vocab.getty.edu/aat/300183634"/>
	<skos:editorialNote xml:lang="en">PPMaterial</skos:editorialNote>
	<skos:scopeNote xml:lang="en">Fine, soft, sheer cloth of plain weave made of any of the principal types of fiber, such as cotton, linen, rayon, silk, or wool.</skos:scopeNote>
</skos:Concept>
<skos:Concept rdf:about="http://partage.vocnet.org/part00567">
	<skos:altLabel xml:lang="en">brick (clay product)</skos:altLabel>
	<skos:prefLabel xml:lang="en">brick</skos:prefLabel>
	<skos:altLabel xml:lang="de">Backstein</skos:altLabel>
	<skos:prefLabel xml:lang="de">Ziegel</skos:prefLabel>
	<skos:prefLabel xml:lang="sv">tegel</skos:prefLabel>
	<skos:prefLabel xml:lang="pt">tijolo</skos:prefLabel>
	<skos:prefLabel xml:lang="fi">tiili</skos:prefLabel>
	<skos:prefLabel xml:lang="hr">cigla</skos:prefLabel>
	<skos:inScheme rdf:resource="http://partage.vocnet.org/Materials"/>
	<skos:broader rdf:resource="http://partage.vocnet.org/part00227"/>
	<skos:exactMatch rdf:resource="http://vocab.getty.edu/aat/300010463"/>
	<skos:editorialNote xml:lang="en">PPMaterial</skos:editorialNote>
	<skos:scopeNote xml:lang="en">Clay or clay products formed into a rectangular block and hardened by drying in the sun or firing in a kiln.</skos:scopeNote>
</skos:Concept>
<skos:Concept rdf:about="http://partage.vocnet.org/part00568">
	<skos:altLabel xml:lang="en">brocade (textile)</skos:altLabel>
	<skos:prefLabel xml:lang="en">brocade</skos:prefLabel>
	<skos:prefLabel xml:lang="de">Brokat</skos:prefLabel>
	<skos:prefLabel xml:lang="sv">brokad</skos:prefLabel>
	<skos:prefLabel xml:lang="pt">brocado</skos:prefLabel>
	<skos:prefLabel xml:lang="hr">brokat</skos:prefLabel>
	<skos:prefLabel xml:lang="fi">brokadi</skos:prefLabel>
	<skos:inScheme rdf:resource="http://partage.vocnet.org/Materials"/>
	<skos:broader rdf:resource="http://partage.vocnet.org/part00229"/>
	<skos:exactMatch rdf:resource="http://vocab.getty.edu/aat/300227779"/>
	<skos:editorialNote xml:lang="en">PPMaterial</skos:editorialNote>
	<skos:scopeNote xml:lang="en">Textile produced by brocading, typically richly figured and incorporating metal thread.</skos:scopeNote>
</skos:Concept>
<skos:Concept rdf:about="http://partage.vocnet.org/part00570">
	<skos:altLabel xml:lang="en">cane (plant material)</skos:altLabel>
	<skos:prefLabel xml:lang="en">cane</skos:prefLabel>
	<skos:prefLabel xml:lang="de">Rohr (Botanik)</skos:prefLabel>
	<skos:prefLabel xml:lang="sv">rotting</skos:prefLabel>
	<skos:prefLabel xml:lang="pt">cana</skos:prefLabel>
	<skos:altLabel xml:lang="fi">rottinki</skos:altLabel>
	<skos:prefLabel xml:lang="fi">kasvimateriaali</skos:prefLabel>
	<skos:prefLabel xml:lang="hr">trska</skos:prefLabel>
	<skos:inScheme rdf:resource="http://partage.vocnet.org/Materials"/>
	<skos:broader rdf:resource="http://partage.vocnet.org/part00297"/>
	<skos:exactMatch rdf:resource="http://vocab.getty.edu/aat/300011864"/>
	<skos:editorialNote xml:lang="en">PPMaterial</skos:editorialNote>
	<skos:scopeNote xml:lang="en">The long, hollow, pithy, jointed stem of certain plants, such as bamboo, rattan, sugarcane or certain palms.</skos:scopeNote>
</skos:Concept>
<skos:Concept rdf:about="http://partage.vocnet.org/part00571">
	<skos:prefLabel xml:lang="en">canvas</skos:prefLabel>
	<skos:prefLabel xml:lang="de">Leinwand</skos:prefLabel>
	<skos:prefLabel xml:lang="sv">kanvas</skos:prefLabel>
	<skos:prefLabel xml:lang="pt">tela</skos:prefLabel>
	<skos:prefLabel xml:lang="hr">platno</skos:prefLabel>
	<skos:prefLabel xml:lang="fi">taustakangas</skos:prefLabel>
	<skos:inScheme rdf:resource="http://partage.vocnet.org/Materials"/>
	<skos:broader rdf:resource="http://partage.vocnet.org/part00229"/>
	<skos:exactMatch rdf:resource="http://vocab.getty.edu/aat/300014078"/>
	<skos:editorialNote xml:lang="en">PPMaterial</skos:editorialNote>
	<skos:scopeNote xml:lang="en">Closely woven textile made in various weights, usually of flax, hemp, jute, or cotton, used especially for sails, tarpaulins, awnings, upholstery, and as a support for oil painting. Also used for a loosely woven, latticelike mesh made of similar material, used as a needlepoint foundation.</skos:scopeNote>
</skos:Concept>
<skos:Concept rdf:about="http://partage.vocnet.org/part00572">
	<skos:prefLabel xml:lang="en">cardboard</skos:prefLabel>
	<skos:prefLabel xml:lang="de">Karton (Trägermaterial)</skos:prefLabel>
	<skos:prefLabel xml:lang="sv">kartong</skos:prefLabel>
	<skos:prefLabel xml:lang="pt">cartão</skos:prefLabel>
	<skos:prefLabel xml:lang="fi">kartonki</skos:prefLabel>
	<skos:prefLabel xml:lang="hr">karton.</skos:prefLabel>
	<skos:inScheme rdf:resource="http://partage.vocnet.org/Materials"/>
	<skos:broader rdf:resource="http://partage.vocnet.org/part00573"/>
	<skos:exactMatch rdf:resource="http://vocab.getty.edu/aat/300014224"/>
	<skos:editorialNote xml:lang="en">PPMaterial</skos:editorialNote>
	<skos:scopeNote xml:lang="en">A type of stiff pasteboard that is thicker than 0.006 inches, typically consisting of good-quality chemical pulp or rag pasteboard, and varying greatly in type and stability. High quality archival cardboard is made from rag pulp and has a low acid content, used for mounting prints, drawings and watercolors. Other grades of cardboard is used for cards, signs, printed materials, and high-quality boxes. Inferior grades of cardboard, such as corrugated board, are made from coarsely ground sulfite treated wood pulp; for this board, use "corrugated board." The first carboard box was produced in England in 1817. Corrugated cardboard was patented in 1871.</skos:scopeNote>
</skos:Concept>
<skos:Concept rdf:about="http://partage.vocnet.org/part00573">
	<skos:altLabel xml:lang="en">pasteboard (paper)</skos:altLabel>
	<skos:prefLabel xml:lang="en">pasteboard</skos:prefLabel>
	<skos:prefLabel xml:lang="sv">papp</skos:prefLabel>
	<skos:prefLabel xml:lang="pt">cartolina</skos:prefLabel>
	<skos:altLabel xml:lang="pt">cartão.</skos:altLabel>
	<skos:prefLabel xml:lang="de">Pappe</skos:prefLabel>
	<skos:prefLabel xml:lang="fi">pahvi</skos:prefLabel>
	<skos:prefLabel xml:lang="hr">ljepenka</skos:prefLabel>
	<skos:inScheme rdf:resource="http://partage.vocnet.org/Materials"/>
	<skos:broader rdf:resource="http://partage.vocnet.org/part00575"/>
	<skos:narrower rdf:resource="http://partage.vocnet.org/part00572"/>
	<skos:exactMatch rdf:resource="http://vocab.getty.edu/aat/300162474"/>
	<skos:editorialNote xml:lang="en">PPMaterial</skos:editorialNote>
	<skos:scopeNote xml:lang="en">Class of thick paper usually in the form of heavy sheets; characterized by being stiff and created by pasting together layers of paper.</skos:scopeNote>
</skos:Concept>
<skos:Concept rdf:about="http://partage.vocnet.org/part00575">
	<skos:altLabel xml:lang="en">paper (fiber product)</skos:altLabel>
	<skos:prefLabel xml:lang="en">paper</skos:prefLabel>
	<skos:prefLabel xml:lang="sv">papper</skos:prefLabel>
	<skos:prefLabel xml:lang="pt">papel</skos:prefLabel>
	<skos:prefLabel xml:lang="de">Papier</skos:prefLabel>
	<skos:prefLabel xml:lang="fi">paperi</skos:prefLabel>
	<skos:prefLabel xml:lang="hr">papir</skos:prefLabel>
	<skos:inScheme rdf:resource="http://partage.vocnet.org/Materials"/>
	<skos:broader rdf:resource="http://partage.vocnet.org/part00229"/>
	<skos:narrower rdf:resource="http://partage.vocnet.org/part00573"/>
	<skos:exactMatch rdf:resource="http://vocab.getty.edu/aat/300014109"/>
	<skos:editorialNote xml:lang="en">PPMaterial</skos:editorialNote>
	<skos:scopeNote xml:lang="en">Refers generally to all types of thin matted or felted sheets or webs of fiber formed and dried on a fine screen from a pulpy water suspension. The fibers may be animal, such as hair, silk or wool, or mineral, such as asbestos, or synthetic. However most paper is made from cellulosic plant fiber, such as from wood pulp, grass, cotton, linen, and straw.</skos:scopeNote>
</skos:Concept>
<skos:Concept rdf:about="http://partage.vocnet.org/part00576">
	<skos:prefLabel xml:lang="en">papier mâché</skos:prefLabel>
	<skos:prefLabel xml:lang="sv">papier-maché</skos:prefLabel>
	<skos:prefLabel xml:lang="pt">papier mâché</skos:prefLabel>
	<skos:altLabel xml:lang="de">Papiermaché</skos:altLabel>
	<skos:altLabel xml:lang="de">Pappmaschee</skos:altLabel>
	<skos:prefLabel xml:lang="de">Pappmaché</skos:prefLabel>
	<skos:altLabel xml:lang="hr">papirmaše</skos:altLabel>
	<skos:prefLabel xml:lang="hr">papier mâché</skos:prefLabel>
	<skos:altLabel xml:lang="fi">paperimassa</skos:altLabel>
	<skos:prefLabel xml:lang="fi">papier mache</skos:prefLabel>
	<skos:inScheme rdf:resource="http://partage.vocnet.org/Materials"/>
	<skos:broader rdf:resource="http://partage.vocnet.org/part00229"/>
	<skos:exactMatch rdf:resource="http://vocab.getty.edu/aat/300014245"/>
	<skos:editorialNote xml:lang="en">PPMaterial</skos:editorialNote>
	<skos:scopeNote xml:lang="en">Composite material used for molding objects; made of repulped or pulverized paper and a liquid adhesive binder. May also comprise strips of paper, sometimes reinforced with textiles, stuck together with a wet adhesive, and used to form an object. The object becomes solid when the paste dries; the object may then be sanded, lacquered, and painted. Such objects are very durable; they first developed in Asia and were common in Europe and elsewhere since the 17th century.</skos:scopeNote>
</skos:Concept>
<skos:Concept rdf:about="http://partage.vocnet.org/part00577">
	<skos:altLabel xml:lang="en">cashmere (wool)</skos:altLabel>
	<skos:prefLabel xml:lang="en">cashmere</skos:prefLabel>
	<skos:prefLabel xml:lang="de">Kaschmir</skos:prefLabel>
	<skos:prefLabel xml:lang="sv">kashmir</skos:prefLabel>
	<skos:prefLabel xml:lang="pt">cachemira</skos:prefLabel>
	<skos:prefLabel xml:lang="hr">kašmir</skos:prefLabel>
	<skos:prefLabel xml:lang="fi">kashmir</skos:prefLabel>
	<skos:inScheme rdf:resource="http://partage.vocnet.org/Materials"/>
	<skos:broader rdf:resource="http://partage.vocnet.org/part00578"/>
	<skos:exactMatch rdf:resource="http://vocab.getty.edu/aat/300192990"/>
	<skos:editorialNote xml:lang="en">PPMaterial</skos:editorialNote>
	<skos:scopeNote xml:lang="en">Fine, soft, light wool from the undercoat of the Kashmir goat; also yarn or fabric made from the wool.</skos:scopeNote>
</skos:Concept>
<skos:Concept rdf:about="http://partage.vocnet.org/part00578">
	<skos:altLabel xml:lang="en">wool (hair)</skos:altLabel>
	<skos:prefLabel xml:lang="en">wool</skos:prefLabel>
	<skos:prefLabel xml:lang="sv">ull</skos:prefLabel>
	<skos:prefLabel xml:lang="pt">lâ</skos:prefLabel>
	<skos:prefLabel xml:lang="de">Wolle</skos:prefLabel>
	<skos:prefLabel xml:lang="hr">vuna</skos:prefLabel>
	<skos:prefLabel xml:lang="fi">villa</skos:prefLabel>
	<skos:inScheme rdf:resource="http://partage.vocnet.org/Materials"/>
	<skos:broader rdf:resource="http://partage.vocnet.org/part00580"/>
	<skos:narrower rdf:resource="http://partage.vocnet.org/part00577"/>
	<skos:exactMatch rdf:resource="http://vocab.getty.edu/aat/300014074"/>
	<skos:editorialNote xml:lang="en">PPMaterial</skos:editorialNote>
	<skos:scopeNote xml:lang="en">Refers especially to the fine, soft, curly hair or fleece of the sheep, but also refers to hair of the alpaca, vicuna, certain goats, and a few other animals.</skos:scopeNote>
</skos:Concept>
<skos:Concept rdf:about="http://partage.vocnet.org/part00580">
	<skos:prefLabel xml:lang="en">hair</skos:prefLabel>
	<skos:prefLabel xml:lang="de">Haar</skos:prefLabel>
	<skos:prefLabel xml:lang="sv">hår</skos:prefLabel>
	<skos:prefLabel xml:lang="pt">cabelo</skos:prefLabel>
	<skos:prefLabel xml:lang="fi">hius</skos:prefLabel>
	<skos:prefLabel xml:lang="hr">kosa</skos:prefLabel>
	<skos:inScheme rdf:resource="http://partage.vocnet.org/Materials"/>
	<skos:broader rdf:resource="http://partage.vocnet.org/part00257"/>
	<skos:narrower rdf:resource="http://partage.vocnet.org/part00578"/>
	<skos:narrower rdf:resource="http://partage.vocnet.org/part00600"/>
	<skos:exactMatch rdf:resource="http://vocab.getty.edu/aat/300011814"/>
	<skos:editorialNote xml:lang="en">PPMaterial</skos:editorialNote>
	<skos:scopeNote xml:lang="en">The fibrous outgrowths of the skins of various animals, composed of the protein keratin, used with other fibers for making fabrics, as stuffing, and for making brushes.</skos:scopeNote>
</skos:Concept>
<skos:Concept rdf:about="http://partage.vocnet.org/part00582">
	<skos:altLabel xml:lang="en">cement (construction material)</skos:altLabel>
	<skos:prefLabel xml:lang="en">cement</skos:prefLabel>
	<skos:prefLabel xml:lang="pt">cimento</skos:prefLabel>
	<skos:prefLabel xml:lang="sv">cement</skos:prefLabel>
	<skos:prefLabel xml:lang="de">Zement</skos:prefLabel>
	<skos:prefLabel xml:lang="hr">cement</skos:prefLabel>
	<skos:prefLabel xml:lang="fi">sementti</skos:prefLabel>
	<skos:inScheme rdf:resource="http://partage.vocnet.org/Materials"/>
	<skos:broader rdf:resource="http://partage.vocnet.org/part00229"/>
	<skos:exactMatch rdf:resource="http://vocab.getty.edu/aat/300010362"/>
	<skos:scopeNote xml:lang="en">Any of several finely powdered inorganic materials that can be mixed with water then dried to form a solid, durable mass, such as plaster, lime, pozzolan cement, and portland cement. It is used in construction as an ingredient of mortar and concrete.</skos:scopeNote>
	<skos:editorialNote xml:lang="en">PPMaterial</skos:editorialNote>
</skos:Concept>
<skos:Concept rdf:about="http://partage.vocnet.org/part00583">
	<skos:prefLabel xml:lang="en">chamois (animal material)</skos:prefLabel>
	<skos:inScheme rdf:resource="http://partage.vocnet.org/Materials"/>
	<skos:broader rdf:resource="http://partage.vocnet.org/part00253"/>
	<skos:exactMatch rdf:resource="http://vocab.getty.edu/aat/300032341"/>
	<skos:editorialNote xml:lang="en">Partage Plus Additional Terms</skos:editorialNote>
	<skos:scopeNote xml:lang="en">Soft, pliable oil-tanned leather originally made from the skins of the chamois, Antilopa rupicapra, a small deer; now made from the skins of lamb, sheep, goat, or from the flesh split of skins or hides.</skos:scopeNote>
</skos:Concept>
<skos:Concept rdf:about="http://partage.vocnet.org/part00585">
	<skos:altLabel xml:lang="en">charcoal (plant material)</skos:altLabel>
	<skos:prefLabel xml:lang="en">charcoal</skos:prefLabel>
	<skos:prefLabel xml:lang="de">Kohle</skos:prefLabel>
	<skos:prefLabel xml:lang="sv">träkol</skos:prefLabel>
	<skos:prefLabel xml:lang="pt">carvão vegetal</skos:prefLabel>
	<skos:prefLabel xml:lang="fi">hiili</skos:prefLabel>
	<skos:prefLabel xml:lang="hr">ugljen</skos:prefLabel>
	<skos:inScheme rdf:resource="http://partage.vocnet.org/Materials"/>
	<skos:broader rdf:resource="http://partage.vocnet.org/part00297"/>
	<skos:exactMatch rdf:resource="http://vocab.getty.edu/aat/300012862"/>
	<skos:editorialNote xml:lang="en">PPMaterial</skos:editorialNote>
	<skos:scopeNote xml:lang="en">Refers to an impure form of graphitic carbon that is created as a residue when carbonaceous material is partially burned, or heated with limited access of air. It is used as a drawing material, for filtering liquids or air, and for other purposes.</skos:scopeNote>
</skos:Concept>
<skos:Concept rdf:about="http://partage.vocnet.org/part00587">
	<skos:prefLabel xml:lang="en">chiffon</skos:prefLabel>
	<skos:prefLabel xml:lang="de">Chiffon</skos:prefLabel>
	<skos:prefLabel xml:lang="sv">chiffong</skos:prefLabel>
	<skos:prefLabel xml:lang="pt">chiffon</skos:prefLabel>
	<skos:prefLabel xml:lang="hr">šifon</skos:prefLabel>
	<skos:prefLabel xml:lang="fi">sifonki</skos:prefLabel>
	<skos:inScheme rdf:resource="http://partage.vocnet.org/Materials"/>
	<skos:broader rdf:resource="http://partage.vocnet.org/part00229"/>
	<skos:editorialNote xml:lang="en">PPMaterial</skos:editorialNote>
	<skos:scopeNote xml:lang="en">Sheer, lightweight plain-woven textile of fine, tightly-twisted yarn, originally of silk now also of various synthetic fibers, used, for example, for scarves, dresses, blouses, underwear, and veils.</skos:scopeNote>
</skos:Concept>
<skos:Concept rdf:about="http://partage.vocnet.org/part00588">
	<skos:prefLabel xml:lang="en">clinker</skos:prefLabel>
	<skos:prefLabel xml:lang="pt">escória</skos:prefLabel>
	<skos:prefLabel xml:lang="sv">klinker</skos:prefLabel>
	<skos:prefLabel xml:lang="de">Klinker</skos:prefLabel>
	<skos:altLabel xml:lang="hr">tvrdo pečena cigla</skos:altLabel>
	<skos:prefLabel xml:lang="hr">klinker</skos:prefLabel>
	<skos:prefLabel xml:lang="fi">kuona</skos:prefLabel>
	<skos:inScheme rdf:resource="http://partage.vocnet.org/Materials"/>
	<skos:broader rdf:resource="http://partage.vocnet.org/part00229"/>
	<skos:exactMatch rdf:resource="http://vocab.getty.edu/aat/300011789"/>
	<skos:editorialNote xml:lang="en">PPMaterial</skos:editorialNote>
	<skos:scopeNote xml:lang="en">Partially fused product from a kiln, which is ground and used for cement.</skos:scopeNote>
</skos:Concept>
<skos:Concept rdf:about="http://partage.vocnet.org/part00590">
	<skos:prefLabel xml:lang="en">concrete</skos:prefLabel>
	<skos:prefLabel xml:lang="de">Beton</skos:prefLabel>
	<skos:prefLabel xml:lang="sv">betong</skos:prefLabel>
	<skos:prefLabel xml:lang="pt">betão</skos:prefLabel>
	<skos:prefLabel xml:lang="fi">betoni</skos:prefLabel>
	<skos:prefLabel xml:lang="hr">beton</skos:prefLabel>
	<skos:inScheme rdf:resource="http://partage.vocnet.org/Materials"/>
	<skos:broader rdf:resource="http://partage.vocnet.org/part00229"/>
	<skos:exactMatch rdf:resource="http://vocab.getty.edu/aat/300010737"/>
	<skos:editorialNote xml:lang="en">PPMaterial</skos:editorialNote>
	<skos:scopeNote xml:lang="en">A hard, strong construction material comprising a mixture of sand, gravel, crushed rock, or other aggregate, held together, typically by a hardened paste of cement and\/or lime. Several types of aggregate are used such as crushed stone, slag, cinders or gravel. Ancient Romans developed pozzolan cement about the 3rd century BCE. Modern concretes use various cements such as portland or hydraulic. Concrete is durable and relatively inexpensive, used for foundations, bridges, dams, walls, and highways. Concrete is strong in compression but weak in tension so it is often reinforced with steel bars or wire netting. Once a concrete mixture is stirred with water and poured into a mold, it is allowed to cure slowly over about a week. Stresses, such as vibration, freezing, and rapid drying, will diminish the strength and durability of the concrete. As it ages, concrete is subject to erosion, spalling, and pollution. Poor mixing can cause erosion. Spalling can be due to freeze-thaw cycles of moisture and ice, salt crystallization, or corrosion of steel reinforcements. Acid rain can deplete the natural alkaline reserve of fresh concrete.</skos:scopeNote>
</skos:Concept>
<skos:Concept rdf:about="http://partage.vocnet.org/part00591">
	<skos:altLabel xml:lang="en">crepe (textile)</skos:altLabel>
	<skos:prefLabel xml:lang="en">crepe</skos:prefLabel>
	<skos:prefLabel xml:lang="de">Krepp</skos:prefLabel>
	<skos:prefLabel xml:lang="sv">crêpe</skos:prefLabel>
	<skos:prefLabel xml:lang="pt">crepe</skos:prefLabel>
	<skos:prefLabel xml:lang="hr">krep</skos:prefLabel>
	<skos:prefLabel xml:lang="fi">kreppi</skos:prefLabel>
	<skos:inScheme rdf:resource="http://partage.vocnet.org/Materials"/>
	<skos:broader rdf:resource="http://partage.vocnet.org/part00229"/>
	<skos:exactMatch rdf:resource="http://vocab.getty.edu/aat/300183741"/>
	<skos:editorialNote xml:lang="en">PPMaterial</skos:editorialNote>
	<skos:scopeNote xml:lang="en">Lightweight textile made of various types of fiber, having a crinkled surface obtained by using hard twisted thread or yarn, by printing with caustic soda, by weaving with varied tensions, or by embossing.</skos:scopeNote>
</skos:Concept>
<skos:Concept rdf:about="http://partage.vocnet.org/part00592">
	<skos:prefLabel xml:lang="en">damask</skos:prefLabel>
	<skos:prefLabel xml:lang="de">Damast</skos:prefLabel>
	<skos:prefLabel xml:lang="sv">damast</skos:prefLabel>
	<skos:prefLabel xml:lang="pt">damasco</skos:prefLabel>
	<skos:prefLabel xml:lang="fi">damasti</skos:prefLabel>
	<skos:prefLabel xml:lang="hr">damast</skos:prefLabel>
	<skos:inScheme rdf:resource="http://partage.vocnet.org/Materials"/>
	<skos:broader rdf:resource="http://partage.vocnet.org/part00229"/>
	<skos:exactMatch rdf:resource="http://vocab.getty.edu/aat/300163295"/>
	<skos:editorialNote xml:lang="en">PPMaterial</skos:editorialNote>
	<skos:scopeNote xml:lang="en">Woven figured textile with one warp and one weft in which the pattern is formed by a contrast of binding systems, and appears on the face and the back in reverse positions.</skos:scopeNote>
</skos:Concept>
<skos:Concept rdf:about="http://partage.vocnet.org/part00593">
	<skos:altLabel xml:lang="en">diamond (mineral)</skos:altLabel>
	<skos:prefLabel xml:lang="en">diamond</skos:prefLabel>
	<skos:prefLabel xml:lang="de">Diamant</skos:prefLabel>
	<skos:prefLabel xml:lang="sv">diamant</skos:prefLabel>
	<skos:prefLabel xml:lang="pt">diamante</skos:prefLabel>
	<skos:prefLabel xml:lang="hr">dijamant</skos:prefLabel>
	<skos:prefLabel xml:lang="fi">timantti</skos:prefLabel>
	<skos:inScheme rdf:resource="http://partage.vocnet.org/Materials"/>
	<skos:broader rdf:resource="http://partage.vocnet.org/part00595"/>
	<skos:exactMatch rdf:resource="http://vocab.getty.edu/aat/300011084"/>
	<skos:editorialNote xml:lang="en">PPMaterial</skos:editorialNote>
	<skos:scopeNote xml:lang="en">A highly transparent and exceedingly hard mineral of carbon; it is the hardest known substance.</skos:scopeNote>
</skos:Concept>
<skos:Concept rdf:about="http://partage.vocnet.org/part00595">
	<skos:prefLabel xml:lang="en">gemstone</skos:prefLabel>
	<skos:prefLabel xml:lang="de">Schmuckstein</skos:prefLabel>
	<skos:prefLabel xml:lang="sv">ädelsten.</skos:prefLabel>
	<skos:prefLabel xml:lang="pt">pedra preciosa.</skos:prefLabel>
	<skos:altLabel xml:lang="hr">gema</skos:altLabel>
	<skos:prefLabel xml:lang="hr">dragi kamen</skos:prefLabel>
	<skos:altLabel xml:lang="fi">korukivi</skos:altLabel>
	<skos:prefLabel xml:lang="fi">jalokivi</skos:prefLabel>
	<skos:inScheme rdf:resource="http://partage.vocnet.org/Materials"/>
	<skos:broader rdf:resource="http://partage.vocnet.org/part00597"/>
	<skos:narrower rdf:resource="http://partage.vocnet.org/part00593"/>
	<skos:narrower rdf:resource="http://partage.vocnet.org/part00897"/>
	<skos:narrower rdf:resource="http://partage.vocnet.org/part00898"/>
	<skos:exactMatch rdf:resource="http://vocab.getty.edu/aat/300201964"/>
	<skos:editorialNote xml:lang="en">PPMaterial</skos:editorialNote>
	<skos:scopeNote xml:lang="en">Precious or semiprecious stone that can be cut, polished, or otherwise dressed for use as gems; distinguished from "gems," which are made of gemstone that has been worked or other material such as pearl.</skos:scopeNote>
</skos:Concept>
<skos:Concept rdf:about="http://partage.vocnet.org/part00597">
	<skos:altLabel xml:lang="en">stone (rock)</skos:altLabel>
	<skos:prefLabel xml:lang="en">stone</skos:prefLabel>
	<skos:prefLabel xml:lang="sv">sten</skos:prefLabel>
	<skos:prefLabel xml:lang="pt">pedra</skos:prefLabel>
	<skos:prefLabel xml:lang="de">Stein</skos:prefLabel>
	<skos:prefLabel xml:lang="hr">kamen</skos:prefLabel>
	<skos:prefLabel xml:lang="fi">kivi</skos:prefLabel>
	<skos:inScheme rdf:resource="http://partage.vocnet.org/Materials"/>
	<skos:broader rdf:resource="http://partage.vocnet.org/part00518"/>
	<skos:narrower rdf:resource="http://partage.vocnet.org/part00595"/>
	<skos:exactMatch rdf:resource="http://vocab.getty.edu/aat/300011176"/>
	<skos:editorialNote xml:lang="en">PPMaterial</skos:editorialNote>
	<skos:scopeNote xml:lang="en">General term for rock that has been cut, shaped, crushed, or otherwise formed for use in construction or other purposes. Includes the specific archaeological and anthropological sense of individual stones which may be decorated or ornamented and which may be used in ritual contexts. These are usually not carved or dressed, and so differ from sculptures made from stone.</skos:scopeNote>
</skos:Concept>
<skos:Concept rdf:about="http://partage.vocnet.org/part00599">
	<skos:prefLabel xml:lang="en">feather (material)</skos:prefLabel>
	<skos:prefLabel xml:lang="pt">pena</skos:prefLabel>
	<skos:prefLabel xml:lang="sv">fjäder</skos:prefLabel>
	<skos:altLabel xml:lang="pt">penas</skos:altLabel>
	<skos:prefLabel xml:lang="de">Feder (Gefieder)</skos:prefLabel>
	<skos:prefLabel xml:lang="fi">höyhen</skos:prefLabel>
	<skos:prefLabel xml:lang="hr">perje</skos:prefLabel>
	<skos:inScheme rdf:resource="http://partage.vocnet.org/Materials"/>
	<skos:broader rdf:resource="http://partage.vocnet.org/part00257"/>
	<skos:exactMatch rdf:resource="http://vocab.getty.edu/aat/300011809"/>
	<skos:editorialNote xml:lang="en">PPMaterial</skos:editorialNote>
	<skos:scopeNote xml:lang="en">One of the light, horny, epidermal outgrowths that form the external covering of the body of birds.</skos:scopeNote>
</skos:Concept>
<skos:Concept rdf:about="http://partage.vocnet.org/part00600">
	<skos:prefLabel xml:lang="en">fur</skos:prefLabel>
	<skos:prefLabel xml:lang="de">Pelz</skos:prefLabel>
	<skos:prefLabel xml:lang="sv">päls</skos:prefLabel>
	<skos:prefLabel xml:lang="pt">pelo</skos:prefLabel>
	<skos:prefLabel xml:lang="fi">turkis</skos:prefLabel>
	<skos:prefLabel xml:lang="hr">krzno</skos:prefLabel>
	<skos:inScheme rdf:resource="http://partage.vocnet.org/Materials"/>
	<skos:broader rdf:resource="http://partage.vocnet.org/part00580"/>
	<skos:exactMatch rdf:resource="http://vocab.getty.edu/aat/300011811"/>
	<skos:editorialNote xml:lang="en">PPMaterial</skos:editorialNote>
	<skos:scopeNote xml:lang="en">Fine, soft, thick, hairy coat of a mammal, usually consisting of a double coat of hair that includes a layer of comparatively short, soft, curly barbed hair next to the skin, protected by longer, smoother, stiffer hair growing up through it.</skos:scopeNote>
</skos:Concept>
<skos:Concept rdf:about="http://partage.vocnet.org/part00601">
	<skos:prefLabel xml:lang="en">gauze</skos:prefLabel>
	<skos:prefLabel xml:lang="de">Gaze</skos:prefLabel>
	<skos:prefLabel xml:lang="sv">gasbinda</skos:prefLabel>
	<skos:prefLabel xml:lang="pt">gaze</skos:prefLabel>
	<skos:prefLabel xml:lang="fi">harso</skos:prefLabel>
	<skos:prefLabel xml:lang="hr">gaza</skos:prefLabel>
	<skos:inScheme rdf:resource="http://partage.vocnet.org/Materials"/>
	<skos:broader rdf:resource="http://partage.vocnet.org/part00229"/>
	<skos:exactMatch rdf:resource="http://vocab.getty.edu/aat/300014083"/>
	<skos:editorialNote xml:lang="en">PPMaterial</skos:editorialNote>
	<skos:scopeNote xml:lang="en">Woven textile in which the binding is achieved by a displacement of warp ends secured by the weft, resulting usually, though not always, in a very open weave; used particularly for surgical dressings and as backing for paper, especially maps.</skos:scopeNote>
</skos:Concept>
<skos:Concept rdf:about="http://partage.vocnet.org/part00602">
	<skos:altLabel xml:lang="en">felt (textile)</skos:altLabel>
	<skos:prefLabel xml:lang="en">felt</skos:prefLabel>
	<skos:prefLabel xml:lang="sv">filt</skos:prefLabel>
	<skos:prefLabel xml:lang="pt">feltro</skos:prefLabel>
	<skos:prefLabel xml:lang="de">Filz</skos:prefLabel>
	<skos:altLabel xml:lang="hr">filc</skos:altLabel>
	<skos:prefLabel xml:lang="hr">pust</skos:prefLabel>
	<skos:prefLabel xml:lang="fi">huopa</skos:prefLabel>
	<skos:inScheme rdf:resource="http://partage.vocnet.org/Materials"/>
	<skos:broader rdf:resource="http://partage.vocnet.org/part00229"/>
	<skos:exactMatch rdf:resource="http://vocab.getty.edu/aat/300014107"/>
	<skos:editorialNote xml:lang="en">PPMaterial</skos:editorialNote>
	<skos:scopeNote xml:lang="en">Textile constructed usually of wool and fur fiber often mixed with natural or synthetic fiber by the interlocking of the loose fiber through the action of heat, moisture, chemicals, and pressure without spinning, weaving, or knitting.</skos:scopeNote>
</skos:Concept>
<skos:Concept rdf:about="http://partage.vocnet.org/part00603">
	<skos:altLabel xml:lang="en">gouache (paint)</skos:altLabel>
	<skos:prefLabel xml:lang="en">gouache</skos:prefLabel>
	<skos:prefLabel xml:lang="de">Gouache</skos:prefLabel>
	<skos:altLabel xml:lang="de">gouache</skos:altLabel>
	<skos:prefLabel xml:lang="pt">guache</skos:prefLabel>
	<skos:prefLabel xml:lang="fi">guassi</skos:prefLabel>
	<skos:prefLabel xml:lang="hr">gvaš</skos:prefLabel>
	<skos:inScheme rdf:resource="http://partage.vocnet.org/Materials"/>
	<skos:broader rdf:resource="http://partage.vocnet.org/part00604"/>
	<skos:exactMatch rdf:resource="http://vocab.getty.edu/aat/300070114"/>
	<skos:editorialNote xml:lang="en">PPMaterial</skos:editorialNote>
	<skos:scopeNote xml:lang="en">A matte, opaque watercolor paint typically using gum arabic, gum senegal, or dextrin as a binder. Gouache paints use opaque pigments rather than the transparent pigments used in watercolor paints. Chalk and other white fillers may be added to some colors. Gouache was used for miniature paintings in the 16th-18th centuries, for decorative paintings on interior walls, and for printing wall paper patterns. Poster paints are an inexpensive version of gouache. The term originally had a different meaning, referring to oil applied on top of tempera painting.</skos:scopeNote>
</skos:Concept>
<skos:Concept rdf:about="http://partage.vocnet.org/part00604">
	<skos:prefLabel xml:lang="en">watercolour (paint)</skos:prefLabel>
	<skos:altLabel xml:lang="en">watercolor (paint)</skos:altLabel>
	<skos:prefLabel xml:lang="sv">akvarell</skos:prefLabel>
	<skos:prefLabel xml:lang="pt">aguarela.</skos:prefLabel>
	<skos:prefLabel xml:lang="de">Aquarell (Farbe)</skos:prefLabel>
	<skos:prefLabel xml:lang="hr">akvarel</skos:prefLabel>
	<skos:prefLabel xml:lang="fi">vesiväri</skos:prefLabel>
	<skos:inScheme rdf:resource="http://partage.vocnet.org/Materials"/>
	<skos:broader rdf:resource="http://partage.vocnet.org/part00605"/>
	<skos:narrower rdf:resource="http://partage.vocnet.org/part00603"/>
	<skos:exactMatch rdf:resource="http://vocab.getty.edu/aat/300015045"/>
	<skos:editorialNote xml:lang="en">PPMaterial</skos:editorialNote>
	<skos:scopeNote xml:lang="en">A transparent aqueous based paint produced by mixing ground pigments with water and, generally, gum arabic. Aqueous based paints made with vegetable gum binders were used by Egyptian, Greek, and Roman artists for wall paintings. Japanese and Chinese painters extensively used watercolor paints on silk panels and delicate paper scrolls. In the 16th through18th century, watercolor paints were used for miniature illustrations on porcelain, ivory, cards, books and manuscripts. By the 18th and early 19th centuries, watercolors rapidly increased in popularity due to the availability of small cakes of watercolor paints in metal pans, usually applied to a paper support by using a brush.</skos:scopeNote>
</skos:Concept>
<skos:Concept rdf:about="http://partage.vocnet.org/part00605">
	<skos:prefLabel xml:lang="en">water-base paint</skos:prefLabel>
	<skos:altLabel xml:lang="de">Wasserfarben</skos:altLabel>
	<skos:prefLabel xml:lang="de">Wasserfarbe</skos:prefLabel>
	<skos:inScheme rdf:resource="http://partage.vocnet.org/Materials"/>
	<skos:broader rdf:resource="http://partage.vocnet.org/part00608"/>
	<skos:narrower rdf:resource="http://partage.vocnet.org/part00604"/>
	<skos:narrower rdf:resource="http://partage.vocnet.org/part00628"/>
	<skos:exactMatch rdf:resource="http://vocab.getty.edu/aat/300183946"/>
	<skos:scopeNote xml:lang="en">Paint consisting of gypsum or whiting with some zinc oxide, with water as the vehicle and glue as the adhesion.</skos:scopeNote>
</skos:Concept>
<skos:Concept rdf:about="http://partage.vocnet.org/part00606">
	<skos:prefLabel xml:lang="en">hardwood</skos:prefLabel>
	<skos:inScheme rdf:resource="http://partage.vocnet.org/Materials"/>
	<skos:broader rdf:resource="http://partage.vocnet.org/part00295"/>
	<skos:narrower rdf:resource="http://partage.vocnet.org/part00635"/>
	<skos:narrower rdf:resource="http://partage.vocnet.org/part00899"/>
	<skos:narrower rdf:resource="http://partage.vocnet.org/part00901"/>
	<skos:narrower rdf:resource="http://partage.vocnet.org/part00902"/>
	<skos:narrower rdf:resource="http://partage.vocnet.org/part00903"/>
	<skos:narrower rdf:resource="http://partage.vocnet.org/part00907"/>
	<skos:narrower rdf:resource="http://partage.vocnet.org/part00908"/>
	<skos:narrower rdf:resource="http://partage.vocnet.org/part00909"/>
	<skos:narrower rdf:resource="http://partage.vocnet.org/part00912"/>
	<skos:narrower rdf:resource="http://partage.vocnet.org/part01154"/>
	<skos:narrower rdf:resource="http://partage.vocnet.org/part01209"/>
	<skos:narrower rdf:resource="http://partage.vocnet.org/part01219"/>
	<skos:narrower rdf:resource="http://partage.vocnet.org/part01222"/>
	<skos:narrower rdf:resource="http://partage.vocnet.org/part01223"/>
	<skos:narrower rdf:resource="http://partage.vocnet.org/part01224"/>
	<skos:exactMatch rdf:resource="http://vocab.getty.edu/aat/300011916"/>
	<skos:scopeNote xml:lang="en">Wood produced from broad-leaved deciduous trees, varying widely in color and grain pattern; usually but not always harder than softwood. Examples of hardwood trees are ash, beech, birch, cherry, mahogany, maple, oak, poplar, and walnut. Hardwood trees are found in temperate and tropical climate zones. Most of the wood used for cabinetry, furniture and flooring is obtained from hardwood trees; only a small amount of hardwood is used for paper pulp. The term hardwood is somewhat confusing since some deciduous trees, such as basswood, have timber that is softer than some coniferous trees, such as yellow pine.</skos:scopeNote>
</skos:Concept>
<skos:Concept rdf:about="http://partage.vocnet.org/part00608">
	<skos:altLabel xml:lang="en">paint (coating)</skos:altLabel>
	<skos:prefLabel xml:lang="en">paint</skos:prefLabel>
	<skos:prefLabel xml:lang="sv">färg</skos:prefLabel>
	<skos:prefLabel xml:lang="pt">tinta.</skos:prefLabel>
	<skos:prefLabel xml:lang="de">Farbe</skos:prefLabel>
	<skos:prefLabel xml:lang="hr">boja</skos:prefLabel>
	<skos:prefLabel xml:lang="fi">maali</skos:prefLabel>
	<skos:inScheme rdf:resource="http://partage.vocnet.org/Materials"/>
	<skos:broader rdf:resource="http://partage.vocnet.org/part00610"/>
	<skos:narrower rdf:resource="http://partage.vocnet.org/part00605"/>
	<skos:narrower rdf:resource="http://partage.vocnet.org/part00616"/>
	<skos:exactMatch rdf:resource="http://vocab.getty.edu/aat/300015029"/>
	<skos:editorialNote xml:lang="en">PPMaterial</skos:editorialNote>
	<skos:scopeNote xml:lang="en">Any dispersion of pigment in a liquid binder. Paint is applied with a brush, roller, sprayer, or by dipping and dries to form a decorative or protective film.</skos:scopeNote>
</skos:Concept>
<skos:Concept rdf:about="http://partage.vocnet.org/part00610">
	<skos:prefLabel xml:lang="en">coating (material)</skos:prefLabel>
	<skos:inScheme rdf:resource="http://partage.vocnet.org/Materials"/>
	<skos:broader rdf:resource="http://partage.vocnet.org/part00229"/>
	<skos:narrower rdf:resource="http://partage.vocnet.org/part00608"/>
	<skos:narrower rdf:resource="http://partage.vocnet.org/part00622"/>
	<skos:narrower rdf:resource="http://partage.vocnet.org/part00906"/>
	<skos:narrower rdf:resource="http://partage.vocnet.org/part01153"/>
	<skos:exactMatch rdf:resource="http://vocab.getty.edu/aat/300014907"/>
	<skos:scopeNote xml:lang="en">Use generally for any substance spread over a surface, usually for protection or decoration.</skos:scopeNote>
</skos:Concept>
<skos:Concept rdf:about="http://partage.vocnet.org/part00612">
	<skos:prefLabel xml:lang="en">muslin</skos:prefLabel>
	<skos:prefLabel xml:lang="sv">muslin</skos:prefLabel>
	<skos:prefLabel xml:lang="pt">musselina</skos:prefLabel>
	<skos:prefLabel xml:lang="de">Musselin</skos:prefLabel>
	<skos:prefLabel xml:lang="hr">muslin</skos:prefLabel>
	<skos:prefLabel xml:lang="fi">musliini</skos:prefLabel>
	<skos:inScheme rdf:resource="http://partage.vocnet.org/Materials"/>
	<skos:broader rdf:resource="http://partage.vocnet.org/part00288"/>
	<skos:exactMatch rdf:resource="http://vocab.getty.edu/aat/300014087"/>
	<skos:editorialNote xml:lang="en">PPMaterial</skos:editorialNote>
	<skos:scopeNote xml:lang="en">Very fine plain weave white cotton made in a great variety of qualities; originally from India, it has been extensively produced and used in Europe and North America for costume, and sometimes as an artist's support.</skos:scopeNote>
</skos:Concept>
<skos:Concept rdf:about="http://partage.vocnet.org/part00613">
	<skos:prefLabel xml:lang="en">net (textile)</skos:prefLabel>
	<skos:prefLabel xml:lang="sv">nät</skos:prefLabel>
	<skos:prefLabel xml:lang="pt">rede</skos:prefLabel>
	<skos:prefLabel xml:lang="de">Netzgewebe</skos:prefLabel>
	<skos:prefLabel xml:lang="fi">verkko</skos:prefLabel>
	<skos:prefLabel xml:lang="hr">mreža</skos:prefLabel>
	<skos:inScheme rdf:resource="http://partage.vocnet.org/Materials"/>
	<skos:broader rdf:resource="http://partage.vocnet.org/part00229"/>
	<skos:narrower rdf:resource="http://partage.vocnet.org/part00629"/>
	<skos:exactMatch rdf:resource="http://vocab.getty.edu/aat/300249438"/>
	<skos:editorialNote xml:lang="en">PPMaterial</skos:editorialNote>
	<skos:scopeNote xml:lang="en">Refers to an open weave textile made of thread, twine, yarn, or cord, usually of silk, cotton, nylon, or rayon, with fine to coarse meshes of fixed dimension. It is characterized by being a simple mesh joined by knots; it may be made by hand or by machine. It may be used to make various items from veils and trimming on clothing to tennis nets and fishing nets. Fine net that is used in lace, headwear, and other apparel is often referred to as "netting" rather than as "net." For the objects consisting of meshed arrangements of threads, cords, or ropes that have been twisted, knotted, or woven together at regular intervals, use "nets (objects)."</skos:scopeNote>
</skos:Concept>
<skos:Concept rdf:about="http://partage.vocnet.org/part00614">
	<skos:prefLabel xml:lang="en">oil (organic material)</skos:prefLabel>
	<skos:prefLabel xml:lang="sv">olja</skos:prefLabel>
	<skos:prefLabel xml:lang="pt">óleo</skos:prefLabel>
	<skos:prefLabel xml:lang="de">Öl (organische Substanz)</skos:prefLabel>
	<skos:prefLabel xml:lang="fi">öljy</skos:prefLabel>
	<skos:prefLabel xml:lang="hr">ulje</skos:prefLabel>
	<skos:inScheme rdf:resource="http://partage.vocnet.org/Materials"/>
	<skos:broader rdf:resource="http://partage.vocnet.org/part00615"/>
	<skos:exactMatch rdf:resource="http://vocab.getty.edu/aat/300014254"/>
	<skos:editorialNote xml:lang="en">PPMaterial</skos:editorialNote>
	<skos:scopeNote xml:lang="en">Any greasy substance that is liquid at room temperature and insoluble in water. Fixed (nonvolatile) oils have the same chemical composition as fats: they consist chiefly of glycerides, resulting from a reaction between glycerol and fatty acids. Oils may be divided by function and type: mineral (e.g., paraffin), vegetable (e.g., linseed), animal (e.g., fish), essential (e.g., turpentine), or edible (e.g., olive).</skos:scopeNote>
</skos:Concept>
<skos:Concept rdf:about="http://partage.vocnet.org/part00615">
	<skos:prefLabel xml:lang="en">organic material</skos:prefLabel>
	<skos:inScheme rdf:resource="http://partage.vocnet.org/Materials"/>
	<skos:broader rdf:resource="http://partage.vocnet.org/part00229"/>
	<skos:narrower rdf:resource="http://partage.vocnet.org/part00614"/>
	<skos:narrower rdf:resource="http://partage.vocnet.org/part00941"/>
	<skos:exactMatch rdf:resource="http://vocab.getty.edu/aat/300011792"/>
	<skos:scopeNote xml:lang="en">Material containing carbon, including those derived from living organisms.</skos:scopeNote>
</skos:Concept>
<skos:Concept rdf:about="http://partage.vocnet.org/part00616">
	<skos:altLabel xml:lang="en">oil paint (paint)</skos:altLabel>
	<skos:prefLabel xml:lang="en">oil</skos:prefLabel>
	<skos:altLabel xml:lang="en">oil (oil paint)</skos:altLabel>
	<skos:prefLabel xml:lang="sv">oljefärg</skos:prefLabel>
	<skos:prefLabel xml:lang="pt">pintura a óleo</skos:prefLabel>
	<skos:altLabel xml:lang="de">Öl (Malerei)</skos:altLabel>
	<skos:prefLabel xml:lang="de">Öl</skos:prefLabel>
	<skos:prefLabel xml:lang="hr">uljana boja</skos:prefLabel>
	<skos:prefLabel xml:lang="fi">öljyväri</skos:prefLabel>
	<skos:inScheme rdf:resource="http://partage.vocnet.org/Materials"/>
	<skos:broader rdf:resource="http://partage.vocnet.org/part00608"/>
	<skos:exactMatch rdf:resource="http://vocab.getty.edu/aat/300015050"/>
	<skos:editorialNote xml:lang="en">PPMaterial</skos:editorialNote>
	<skos:scopeNote xml:lang="en">A paint made by grinding pigments with a drying oil such as linseed oil. After 1940 alkyd binders were often added to oil paint to provide faster drying times.</skos:scopeNote>
</skos:Concept>
<skos:Concept rdf:about="http://partage.vocnet.org/part00617">
	<skos:altLabel xml:lang="en">panels (wood)</skos:altLabel>
	<skos:prefLabel xml:lang="en">panel</skos:prefLabel>
	<skos:prefLabel xml:lang="sv">panel</skos:prefLabel>
	<skos:prefLabel xml:lang="pt">tábua</skos:prefLabel>
	<skos:prefLabel xml:lang="de">Tafel</skos:prefLabel>
	<skos:altLabel xml:lang="de">Paneel</skos:altLabel>
	<skos:prefLabel xml:lang="hr">daska</skos:prefLabel>
	<skos:prefLabel xml:lang="fi">paneeli</skos:prefLabel>
	<skos:inScheme rdf:resource="http://partage.vocnet.org/Materials"/>
	<skos:broader rdf:resource="http://partage.vocnet.org/part00295"/>
	<skos:exactMatch rdf:resource="http://vocab.getty.edu/aat/300014657"/>
	<skos:editorialNote xml:lang="en">PPMaterial</skos:editorialNote>
	<skos:scopeNote xml:lang="en">In art, the term refers to wood in the form of broad, thin, flat or sometimes curved pieces as, for example, with paintings on wood. In architecture and other constructive arts, use "panels (surface components" to refer to a panel, whether of wood or another material, that is typically a compartment of a surface either sunken below or raised above the general level, and set in a molding or other border, as in a frame, sometimes of different color or material.</skos:scopeNote>
</skos:Concept>
<skos:Concept rdf:about="http://partage.vocnet.org/part00618">
	<skos:altLabel xml:lang="en">pearl (animal material)</skos:altLabel>
	<skos:prefLabel xml:lang="en">pearl</skos:prefLabel>
	<skos:prefLabel xml:lang="sv">pärla</skos:prefLabel>
	<skos:prefLabel xml:lang="pt">pérola</skos:prefLabel>
	<skos:prefLabel xml:lang="de">Perle (Material)</skos:prefLabel>
	<skos:prefLabel xml:lang="hr">biser</skos:prefLabel>
	<skos:prefLabel xml:lang="fi">helmi</skos:prefLabel>
	<skos:inScheme rdf:resource="http://partage.vocnet.org/Materials"/>
	<skos:broader rdf:resource="http://partage.vocnet.org/part00229"/>
	<skos:exactMatch rdf:resource="http://vocab.getty.edu/aat/300011827"/>
	<skos:editorialNote xml:lang="en">PPMaterial</skos:editorialNote>
	<skos:scopeNote xml:lang="en">A smooth round bead formed primarily within the shells of two distantly related groups of molluscan bivalves or clams, including the ocean-dwelling pearl oysters and the freshwater river mussels. Pearls are used in jewelry and for other ornamental puposes; they are considered a gem.</skos:scopeNote>
</skos:Concept>
<skos:Concept rdf:about="http://partage.vocnet.org/part00620">
	<skos:prefLabel xml:lang="en">pigment</skos:prefLabel>
	<skos:prefLabel xml:lang="sv">pigment</skos:prefLabel>
	<skos:prefLabel xml:lang="pt">pigmento</skos:prefLabel>
	<skos:prefLabel xml:lang="de">Pigment</skos:prefLabel>
	<skos:prefLabel xml:lang="hr">pigment</skos:prefLabel>
	<skos:altLabel xml:lang="fi">väriaine</skos:altLabel>
	<skos:prefLabel xml:lang="fi">pigmentti</skos:prefLabel>
	<skos:inScheme rdf:resource="http://partage.vocnet.org/Materials"/>
	<skos:broader rdf:resource="http://partage.vocnet.org/part00621"/>
	<skos:exactMatch rdf:resource="http://vocab.getty.edu/aat/300013109"/>
	<skos:editorialNote xml:lang="en">PPMaterial</skos:editorialNote>
	<skos:scopeNote xml:lang="en">Any relatively insoluble organic, inorganic, natural or artificial substance that imparts a color to another substance or mixture and always appears as the same specific color when viewed in white light. It is the constituent of paint or ink that provides the color. Distinguished from a dye, which is soluble in the vehicle, a pigment is insoluble in the vehicle, but instead is held in a suspension.</skos:scopeNote>
</skos:Concept>
<skos:Concept rdf:about="http://partage.vocnet.org/part00621">
	<skos:prefLabel xml:lang="en">colorant (material)</skos:prefLabel>
	<skos:inScheme rdf:resource="http://partage.vocnet.org/Materials"/>
	<skos:broader rdf:resource="http://partage.vocnet.org/part00229"/>
	<skos:narrower rdf:resource="http://partage.vocnet.org/part00620"/>
	<skos:exactMatch rdf:resource="http://vocab.getty.edu/aat/300013026"/>
	<skos:scopeNote xml:lang="en">Any substance capable of or used for coloring another material. A colorant may be a dye or a pigment.</skos:scopeNote>
</skos:Concept>
<skos:Concept rdf:about="http://partage.vocnet.org/part00622">
	<skos:prefLabel xml:lang="en">plaster</skos:prefLabel>
	<skos:prefLabel xml:lang="sv">gips</skos:prefLabel>
	<skos:prefLabel xml:lang="pt">gesso</skos:prefLabel>
	<skos:prefLabel xml:lang="de">Gips</skos:prefLabel>
	<skos:prefLabel xml:lang="fi">kipsi</skos:prefLabel>
	<skos:prefLabel xml:lang="hr">gips</skos:prefLabel>
	<skos:inScheme rdf:resource="http://partage.vocnet.org/Materials"/>
	<skos:broader rdf:resource="http://partage.vocnet.org/part00610"/>
	<skos:exactMatch rdf:resource="http://vocab.getty.edu/aat/300014922"/>
	<skos:editorialNote xml:lang="en">PPMaterial</skos:editorialNote>
	<skos:scopeNote xml:lang="en">Refers to a soft, plastic material that can be spread or daubed on a wall, ceiling, or other surface, where it afterwards hardens. In the context of art and architecture, it generally refers specifically to a mixture of water, lime, and sand, often combined with other materials, such as animal hair, to give the resulting material strength, texture, and if the surface is to be painted, porosity.</skos:scopeNote>
</skos:Concept>
<skos:Concept rdf:about="http://partage.vocnet.org/part00624">
	<skos:prefLabel xml:lang="en">plywood</skos:prefLabel>
	<skos:prefLabel xml:lang="sv">plywood</skos:prefLabel>
	<skos:altLabel xml:lang="pt">contraplacado</skos:altLabel>
	<skos:prefLabel xml:lang="pt">madeira contraplacada</skos:prefLabel>
	<skos:prefLabel xml:lang="de">Sperrholz</skos:prefLabel>
	<skos:altLabel xml:lang="hr">ljepenka.</skos:altLabel>
	<skos:prefLabel xml:lang="hr">šperploča</skos:prefLabel>
	<skos:prefLabel xml:lang="fi">vaneri</skos:prefLabel>
	<skos:inScheme rdf:resource="http://partage.vocnet.org/Materials"/>
	<skos:broader rdf:resource="http://partage.vocnet.org/part00297"/>
	<skos:exactMatch rdf:resource="http://vocab.getty.edu/aat/300012849"/>
	<skos:editorialNote xml:lang="en">PPMaterial</skos:editorialNote>
	<skos:scopeNote xml:lang="en">Wood board consisting of a number of thin layers of rotary-cut veneers glued together so that the grain of each layer is at right angles to the grain of the adjacent layer.</skos:scopeNote>
</skos:Concept>
<skos:Concept rdf:about="http://partage.vocnet.org/part00625">
	<skos:prefLabel xml:lang="en">satin</skos:prefLabel>
	<skos:prefLabel xml:lang="sv">satin</skos:prefLabel>
	<skos:prefLabel xml:lang="pt">cetim</skos:prefLabel>
	<skos:prefLabel xml:lang="de">Satin</skos:prefLabel>
	<skos:prefLabel xml:lang="fi">satiini</skos:prefLabel>
	<skos:prefLabel xml:lang="hr">saten</skos:prefLabel>
	<skos:inScheme rdf:resource="http://partage.vocnet.org/Materials"/>
	<skos:broader rdf:resource="http://partage.vocnet.org/part00229"/>
	<skos:exactMatch rdf:resource="http://vocab.getty.edu/aat/300132902"/>
	<skos:editorialNote xml:lang="en">PPMaterial</skos:editorialNote>
	<skos:scopeNote xml:lang="en">Woven textile characterized by a basic binding system or weave with smooth, shiny surface formed by long warp floats. Generally, each warp end passes over four or more adjacent weft picks and under the next one.</skos:scopeNote>
</skos:Concept>
<skos:Concept rdf:about="http://partage.vocnet.org/part00626">
	<skos:altLabel xml:lang="en">shell (animal material)</skos:altLabel>
	<skos:prefLabel xml:lang="en">shell</skos:prefLabel>
	<skos:prefLabel xml:lang="sv">snäcka</skos:prefLabel>
	<skos:prefLabel xml:lang="pt">concha</skos:prefLabel>
	<skos:altLabel xml:lang="de">Panzer (Material)</skos:altLabel>
	<skos:prefLabel xml:lang="de">Schale (Material)</skos:prefLabel>
	<skos:prefLabel xml:lang="fi">simpukka</skos:prefLabel>
	<skos:prefLabel xml:lang="hr">školjka</skos:prefLabel>
	<skos:inScheme rdf:resource="http://partage.vocnet.org/Materials"/>
	<skos:broader rdf:resource="http://partage.vocnet.org/part00229"/>
	<skos:exactMatch rdf:resource="http://vocab.getty.edu/aat/300011829"/>
	<skos:editorialNote xml:lang="en">PPMaterial</skos:editorialNote>
	<skos:scopeNote xml:lang="en">Hard outer covering of invertebrate creatures, composed of calcareous or chitinous material.</skos:scopeNote>
</skos:Concept>
<skos:Concept rdf:about="http://partage.vocnet.org/part00627">
	<skos:prefLabel xml:lang="en">suede</skos:prefLabel>
	<skos:prefLabel xml:lang="sv">mocka</skos:prefLabel>
	<skos:prefLabel xml:lang="pt">camurça</skos:prefLabel>
	<skos:prefLabel xml:lang="de">Veloursleder</skos:prefLabel>
	<skos:altLabel xml:lang="de">Wildleder</skos:altLabel>
	<skos:prefLabel xml:lang="fi">mokkanahka</skos:prefLabel>
	<skos:prefLabel xml:lang="hr">antilop koža</skos:prefLabel>
	<skos:inScheme rdf:resource="http://partage.vocnet.org/Materials"/>
	<skos:broader rdf:resource="http://partage.vocnet.org/part00253"/>
	<skos:exactMatch rdf:resource="http://vocab.getty.edu/aat/300193368"/>
	<skos:editorialNote xml:lang="en">PPMaterial</skos:editorialNote>
	<skos:scopeNote xml:lang="en">Leather finished by buffing on an emery wheel, usually on the flesh side to produce a napped surface. Distinct from "rough calf" which is always finished on the flesh side and not polished with an emery wheel.</skos:scopeNote>
</skos:Concept>
<skos:Concept rdf:about="http://partage.vocnet.org/part00628">
	<skos:prefLabel xml:lang="en">tempera</skos:prefLabel>
	<skos:prefLabel xml:lang="sv">tempera</skos:prefLabel>
	<skos:prefLabel xml:lang="pt">têmpera</skos:prefLabel>
	<skos:prefLabel xml:lang="de">Tempera</skos:prefLabel>
	<skos:prefLabel xml:lang="hr">tempera</skos:prefLabel>
	<skos:prefLabel xml:lang="fi">tempera</skos:prefLabel>
	<skos:inScheme rdf:resource="http://partage.vocnet.org/Materials"/>
	<skos:broader rdf:resource="http://partage.vocnet.org/part00605"/>
	<skos:exactMatch rdf:resource="http://vocab.getty.edu/aat/300015062"/>
	<skos:editorialNote xml:lang="en">PPMaterial</skos:editorialNote>
	<skos:scopeNote xml:lang="en">Paint formed of an emulsion of fatty and watery constituents. The standard emulsion is usually created with egg yolk and water, with variants of man-made emulsions created with whole egg, linseed oil, casein glue, gum, or wax.</skos:scopeNote>
</skos:Concept>
<skos:Concept rdf:about="http://partage.vocnet.org/part00629">
	<skos:altLabel xml:lang="en">tulle (meshed textile)</skos:altLabel>
	<skos:prefLabel xml:lang="en">tulle</skos:prefLabel>
	<skos:prefLabel xml:lang="sv">tyll</skos:prefLabel>
	<skos:prefLabel xml:lang="pt">tule</skos:prefLabel>
	<skos:prefLabel xml:lang="de">Tüll</skos:prefLabel>
	<skos:prefLabel xml:lang="hr">til</skos:prefLabel>
	<skos:prefLabel xml:lang="fi">tylli</skos:prefLabel>
	<skos:inScheme rdf:resource="http://partage.vocnet.org/Materials"/>
	<skos:broader rdf:resource="http://partage.vocnet.org/part00613"/>
	<skos:exactMatch rdf:resource="http://vocab.getty.edu/aat/300256611"/>
	<skos:editorialNote xml:lang="en">PPMaterial</skos:editorialNote>
	<skos:scopeNote xml:lang="en">Meshed textile made of sheer silk, nylon, or rayon with a hexagonal mesh; used for hats, veils, ballet costumes, and women's dresses.</skos:scopeNote>
</skos:Concept>
<skos:Concept rdf:about="http://partage.vocnet.org/part00630">
	<skos:prefLabel xml:lang="en">velours</skos:prefLabel>
	<skos:prefLabel xml:lang="sv">velour</skos:prefLabel>
	<skos:prefLabel xml:lang="pt">fazenda</skos:prefLabel>
	<skos:prefLabel xml:lang="de">Velours</skos:prefLabel>
	<skos:prefLabel xml:lang="fi">veluuri</skos:prefLabel>
	<skos:prefLabel xml:lang="hr">velur</skos:prefLabel>
	<skos:inScheme rdf:resource="http://partage.vocnet.org/Materials"/>
	<skos:broader rdf:resource="http://partage.vocnet.org/part00631"/>
	<skos:exactMatch rdf:resource="http://vocab.getty.edu/aat/300311594"/>
	<skos:editorialNote xml:lang="en">PPMaterial</skos:editorialNote>
	<skos:scopeNote xml:lang="en">Woollen fabric with a velvet pile.</skos:scopeNote>
</skos:Concept>
<skos:Concept rdf:about="http://partage.vocnet.org/part00631">
	<skos:prefLabel xml:lang="en">warp pile weave</skos:prefLabel>
	<skos:inScheme rdf:resource="http://partage.vocnet.org/Materials"/>
	<skos:broader rdf:resource="http://partage.vocnet.org/part00632"/>
	<skos:narrower rdf:resource="http://partage.vocnet.org/part00630"/>
	<skos:narrower rdf:resource="http://partage.vocnet.org/part00633"/>
	<skos:exactMatch rdf:resource="http://vocab.getty.edu/aat/300227932"/>
	<skos:scopeNote xml:lang="en">Pile weave in which the pile is produced by a supplementary pile warp.</skos:scopeNote>
</skos:Concept>
<skos:Concept rdf:about="http://partage.vocnet.org/part00632">
	<skos:prefLabel xml:lang="en">pile weave</skos:prefLabel>
	<skos:inScheme rdf:resource="http://partage.vocnet.org/Materials"/>
	<skos:broader rdf:resource="http://partage.vocnet.org/part00229"/>
	<skos:narrower rdf:resource="http://partage.vocnet.org/part00631"/>
	<skos:exactMatch rdf:resource="http://vocab.getty.edu/aat/300227872"/>
	<skos:scopeNote xml:lang="en">Woven textile in which a pile is produced above the ground by the use of either a pile warp or a pile weft.</skos:scopeNote>
</skos:Concept>
<skos:Concept rdf:about="http://partage.vocnet.org/part00633">
	<skos:altLabel xml:lang="en">velvet (fabric weave)</skos:altLabel>
	<skos:prefLabel xml:lang="en">velvet</skos:prefLabel>
	<skos:prefLabel xml:lang="sv">sammet</skos:prefLabel>
	<skos:prefLabel xml:lang="pt">veludo</skos:prefLabel>
	<skos:prefLabel xml:lang="de">Samt</skos:prefLabel>
	<skos:prefLabel xml:lang="hr">baršun</skos:prefLabel>
	<skos:prefLabel xml:lang="fi">sametti</skos:prefLabel>
	<skos:inScheme rdf:resource="http://partage.vocnet.org/Materials"/>
	<skos:broader rdf:resource="http://partage.vocnet.org/part00631"/>
	<skos:exactMatch rdf:resource="http://vocab.getty.edu/aat/300133711"/>
	<skos:editorialNote xml:lang="en">PPMaterial</skos:editorialNote>
	<skos:scopeNote xml:lang="en">Warp pile weave, typically silk, with a short, soft dense pile produced by a supplementary warp that is raised in loops above the surface of the textile through the introduction of rods during the weaving; the loops may be cut or left uncut.</skos:scopeNote>
</skos:Concept>
<skos:Concept rdf:about="http://partage.vocnet.org/part00634">
	<skos:prefLabel xml:lang="en">zinc</skos:prefLabel>
	<skos:prefLabel xml:lang="sv">zink</skos:prefLabel>
	<skos:prefLabel xml:lang="pt">zinco</skos:prefLabel>
	<skos:prefLabel xml:lang="de">Zink</skos:prefLabel>
	<skos:prefLabel xml:lang="hr">cink</skos:prefLabel>
	<skos:prefLabel xml:lang="fi">sinkki</skos:prefLabel>
	<skos:inScheme rdf:resource="http://partage.vocnet.org/Materials"/>
	<skos:broader rdf:resource="http://partage.vocnet.org/part00265"/>
	<skos:exactMatch rdf:resource="http://vocab.getty.edu/aat/300011037"/>
	<skos:editorialNote xml:lang="en">PPMaterial</skos:editorialNote>
	<skos:scopeNote xml:lang="en">ure metallic element having symbol Zn and atomic number 30; a bluish white crystalline metal. Use also for this metal as processed and formed, usually in combination with other substances, to make various objects and materials.</skos:scopeNote>
</skos:Concept>
<skos:Concept rdf:about="http://partage.vocnet.org/part00635">
	<skos:altLabel xml:lang="en">ash (wood)</skos:altLabel>
	<skos:prefLabel xml:lang="en">ash</skos:prefLabel>
	<skos:prefLabel xml:lang="de">Esche</skos:prefLabel>
	<skos:prefLabel xml:lang="sv">ask</skos:prefLabel>
	<skos:prefLabel xml:lang="pt">cinza</skos:prefLabel>
	<skos:prefLabel xml:lang="hr">jasen</skos:prefLabel>
	<skos:prefLabel xml:lang="fi">saarni</skos:prefLabel>
	<skos:inScheme rdf:resource="http://partage.vocnet.org/Materials"/>
	<skos:broader rdf:resource="http://partage.vocnet.org/part00606"/>
	<skos:exactMatch rdf:resource="http://vocab.getty.edu/aat/300164025"/>
	<skos:scopeNote xml:lang="en">Wood of any of several trees belonging to the genus Fraxinus, having distinctive growth rings with very large open pores beside small, tight pores. The wood is light in color, dense, elastic, and having a straight grain that is moderately durable but susceptible to insect attack and moisture degradation. The tough, heavy timber is used for ladders, tool handles, oars, poles, gymnasium equipment, and hockey sticks because it produces a smooth surface that rarely splinters. Ash was also popular for furniture (especially Colonial pieces), wheels, and carriage frames, and is used for decorative veneers.</skos:scopeNote>
	<skos:editorialNote xml:lang="en">PPMaterial</skos:editorialNote>
</skos:Concept>
<skos:Concept rdf:about="http://partage.vocnet.org/part00832">
	<skos:prefLabel xml:lang="en">chalk</skos:prefLabel>
	<skos:prefLabel xml:lang="de">Kreide</skos:prefLabel>
	<skos:inScheme rdf:resource="http://partage.vocnet.org/Materials"/>
	<skos:broader rdf:resource="http://partage.vocnet.org/part00229"/>
	<skos:exactMatch rdf:resource="http://vocab.getty.edu/aat/300011727"/>
	<skos:scopeNote xml:lang="en">A fine-grained limestone, or soft, earthy form of calcium carbonate; used chiefly in putty, crayons, paint, rubber products, linoleum, and as a pigment and abrasive.</skos:scopeNote>
	<skos:editorialNote xml:lang="en">PPMaterial</skos:editorialNote>
</skos:Concept>
<skos:Concept rdf:about="http://partage.vocnet.org/part00889">
	<skos:prefLabel xml:lang="en">silver bromide</skos:prefLabel>
	<skos:prefLabel xml:lang="sv">silverbromid</skos:prefLabel>
	<skos:prefLabel xml:lang="pt">brometo de prata</skos:prefLabel>
	<skos:prefLabel xml:lang="de">Bromsilber</skos:prefLabel>
	<skos:prefLabel xml:lang="hr">srebrobromid</skos:prefLabel>
	<skos:prefLabel xml:lang="fi">hopeabromidi</skos:prefLabel>
	<skos:inScheme rdf:resource="http://partage.vocnet.org/Materials"/>
	<skos:broader rdf:resource="http://partage.vocnet.org/part01035"/>
	<skos:exactMatch rdf:resource="http://vocab.getty.edu/aat/300130944"/>
	<skos:editorialNote xml:lang="en">PPMaterial</skos:editorialNote>
	<skos:scopeNote xml:lang="en">A yellow, water-insoluble powder, AgBr, which darkens upon exposure to light, produced by the reaction of silver nitrate with a bromide. It was used chiefly in the manufacture of photographic emulsions from about 1875-1880.</skos:scopeNote>
</skos:Concept>
<skos:Concept rdf:about="http://partage.vocnet.org/part00897">
	<skos:prefLabel xml:lang="en">precious stone</skos:prefLabel>
	<skos:prefLabel xml:lang="sv">ädelsten</skos:prefLabel>
	<skos:prefLabel xml:lang="pt">pedra preciosa</skos:prefLabel>
	<skos:prefLabel xml:lang="de">Edelstein</skos:prefLabel>
	<skos:prefLabel xml:lang="hr">dragi kamen.</skos:prefLabel>
	<skos:altLabel xml:lang="fi">korukivi.</skos:altLabel>
	<skos:prefLabel xml:lang="fi">jalokivi.</skos:prefLabel>
	<skos:inScheme rdf:resource="http://partage.vocnet.org/Materials"/>
	<skos:broader rdf:resource="http://partage.vocnet.org/part00595"/>
	<skos:exactMatch rdf:resource="http://vocab.getty.edu/aat/300133732"/>
	<skos:editorialNote xml:lang="en">PPMaterial</skos:editorialNote>
	<skos:scopeNote xml:lang="en">Gemstone considered more valuable than other types, especially diamond, sapphire, emerald, ruby, and sometimes pearl.</skos:scopeNote>
</skos:Concept>
<skos:Concept rdf:about="http://partage.vocnet.org/part00898">
	<skos:prefLabel xml:lang="en">semiprecious stone</skos:prefLabel>
	<skos:prefLabel xml:lang="sv">halvädelsten</skos:prefLabel>
	<skos:prefLabel xml:lang="pt">pedra semipreciosa</skos:prefLabel>
	<skos:prefLabel xml:lang="de">Halbedelstein</skos:prefLabel>
	<skos:prefLabel xml:lang="hr">poludragi kamen</skos:prefLabel>
	<skos:prefLabel xml:lang="fi">puolijalokivi</skos:prefLabel>
	<skos:inScheme rdf:resource="http://partage.vocnet.org/Materials"/>
	<skos:broader rdf:resource="http://partage.vocnet.org/part00595"/>
	<skos:exactMatch rdf:resource="http://vocab.getty.edu/aat/300011175"/>
	<skos:editorialNote xml:lang="en">PPMaterial</skos:editorialNote>
	<skos:scopeNote xml:lang="en">Stone with less commercial value than those classified as precious.</skos:scopeNote>
</skos:Concept>
<skos:Concept rdf:about="http://partage.vocnet.org/part00899">
	<skos:prefLabel xml:lang="en">walnut</skos:prefLabel>
	<skos:prefLabel xml:lang="sv">valnöt</skos:prefLabel>
	<skos:prefLabel xml:lang="pt">nogueira</skos:prefLabel>
	<skos:prefLabel xml:lang="de">Nussbaum</skos:prefLabel>
	<skos:prefLabel xml:lang="hr">orahovina</skos:prefLabel>
	<skos:prefLabel xml:lang="fi">pähkinäpuu</skos:prefLabel>
	<skos:inScheme rdf:resource="http://partage.vocnet.org/Materials"/>
	<skos:broader rdf:resource="http://partage.vocnet.org/part00606"/>
	<skos:exactMatch rdf:resource="http://vocab.getty.edu/aat/300012476"/>
	<skos:editorialNote xml:lang="en">PPMaterial</skos:editorialNote>
	<skos:scopeNote xml:lang="en">Wood of several trees belonging to the genus Juglans, ranging in color from grey-brown to purple brown, used in making cabinetwork, veneer, butts and rifle stocks.</skos:scopeNote>
</skos:Concept>
<skos:Concept rdf:about="http://partage.vocnet.org/part00900">
	<skos:prefLabel xml:lang="en">taffeta</skos:prefLabel>
	<skos:prefLabel xml:lang="sv">taft</skos:prefLabel>
	<skos:prefLabel xml:lang="pt">tafetá</skos:prefLabel>
	<skos:prefLabel xml:lang="de">Taft</skos:prefLabel>
	<skos:prefLabel xml:lang="hr">taft</skos:prefLabel>
	<skos:prefLabel xml:lang="fi">tafti</skos:prefLabel>
	<skos:inScheme rdf:resource="http://partage.vocnet.org/Materials"/>
	<skos:broader rdf:resource="http://partage.vocnet.org/part00229"/>
	<skos:exactMatch rdf:resource="http://vocab.getty.edu/aat/300249434"/>
	<skos:editorialNote xml:lang="en">PPMaterial</skos:editorialNote>
	<skos:scopeNote xml:lang="en">Crisp textile, typically in plain weave, sometimes with a fine crosswise rib and a smooth lustrous surface on both sides, originally of silk, now of various fibers.</skos:scopeNote>
</skos:Concept>
<skos:Concept rdf:about="http://partage.vocnet.org/part00901">
	<skos:prefLabel xml:lang="en">palisander</skos:prefLabel>
	<skos:prefLabel xml:lang="sv">jakaranda</skos:prefLabel>
	<skos:prefLabel xml:lang="pt">jacarandá</skos:prefLabel>
	<skos:prefLabel xml:lang="de">Palisander</skos:prefLabel>
	<skos:prefLabel xml:lang="fi">palisanteri</skos:prefLabel>
	<skos:prefLabel xml:lang="hr">palisandrovina</skos:prefLabel>
	<skos:altLabel xml:lang="hr">ružino drvo</skos:altLabel>
	<skos:inScheme rdf:resource="http://partage.vocnet.org/Materials"/>
	<skos:broader rdf:resource="http://partage.vocnet.org/part00606"/>
	<skos:exactMatch rdf:resource="http://vocab.getty.edu/aat/300375333"/>
	<skos:editorialNote xml:lang="en">PPMaterial</skos:editorialNote>
	<skos:scopeNote xml:lang="en">General term for any dark ornamental wood derived from various tropical American trees, especially of the genus Jacaranda, the species Dalbergia nigra (Brazilian rosewood), or the genus Peltogyne.</skos:scopeNote>
</skos:Concept>
<skos:Concept rdf:about="http://partage.vocnet.org/part00902">
	<skos:prefLabel xml:lang="en">oak</skos:prefLabel>
	<skos:prefLabel xml:lang="sv">ek</skos:prefLabel>
	<skos:prefLabel xml:lang="pt">carvalho</skos:prefLabel>
	<skos:prefLabel xml:lang="de">Eiche</skos:prefLabel>
	<skos:prefLabel xml:lang="hr">hrastovina</skos:prefLabel>
	<skos:prefLabel xml:lang="fi">tammi</skos:prefLabel>
	<skos:inScheme rdf:resource="http://partage.vocnet.org/Materials"/>
	<skos:broader rdf:resource="http://partage.vocnet.org/part00606"/>
	<skos:exactMatch rdf:resource="http://vocab.getty.edu/aat/300012264"/>
	<skos:editorialNote xml:lang="en">PPMaterial</skos:editorialNote>
	<skos:scopeNote xml:lang="en">Wood of trees belonging to the genus Quercus, of the beech family. It is a durable wood that has a distinctive coarse grain, used in cabinetry, flooring, paneling, musical instruments, ship interiors and moldings, panel painting, and sculptures.</skos:scopeNote>
</skos:Concept>
<skos:Concept rdf:about="http://partage.vocnet.org/part00903">
	<skos:prefLabel xml:lang="en">maple</skos:prefLabel>
	<skos:prefLabel xml:lang="sv">lönn</skos:prefLabel>
	<skos:prefLabel xml:lang="pt">ácer</skos:prefLabel>
	<skos:prefLabel xml:lang="de">Ahorn</skos:prefLabel>
	<skos:prefLabel xml:lang="hr">javor</skos:prefLabel>
	<skos:prefLabel xml:lang="fi">vaahtera</skos:prefLabel>
	<skos:inScheme rdf:resource="http://partage.vocnet.org/Materials"/>
	<skos:broader rdf:resource="http://partage.vocnet.org/part00606"/>
	<skos:exactMatch rdf:resource="http://vocab.getty.edu/aat/300012236"/>
	<skos:editorialNote xml:lang="en">PPMaterial</skos:editorialNote>
	<skos:scopeNote xml:lang="en">Wood of trees belonging to the genus Acer, light reddish brown in color, with small pores, distinct rings, and rays that show as fine dashes in quarter sawed wood. Maple wood is used for fine furniture, cabinetry, flooring, shoe lasts, and musical instruments.</skos:scopeNote>
</skos:Concept>
<skos:Concept rdf:about="http://partage.vocnet.org/part00905">
	<skos:prefLabel xml:lang="en">graphite</skos:prefLabel>
	<skos:altLabel xml:lang="en">graphite (mineral)</skos:altLabel>
	<skos:prefLabel xml:lang="de">Graphit</skos:prefLabel>
	<skos:prefLabel xml:lang="sv">blyertspennor</skos:prefLabel>
	<skos:prefLabel xml:lang="pt">lápis de grafite</skos:prefLabel>
	<skos:prefLabel xml:lang="hr">grafitna olovka</skos:prefLabel>
	<skos:prefLabel xml:lang="fi">lyijykynä</skos:prefLabel>
	<skos:inScheme rdf:resource="http://partage.vocnet.org/Materials"/>
	<skos:broader rdf:resource="http://partage.vocnet.org/part00281"/>
	<skos:exactMatch rdf:resource="http://vocab.getty.edu/aat/300011098"/>
	<skos:editorialNote xml:lang="en">PPMaterial</skos:editorialNote>
	<skos:scopeNote xml:lang="en">Naturally occurring crystalline form of carbon dimorphous with diamond. Graphite has a layered structure that consists of rings of six carbon atoms arranged in widely spaced horizontal sheets, and thus crystallizes in the hexagonal system, in contrast to the same element crystallizing in the octahedral or tetrahedral system as diamond, resulting in very different characteristics in each. Graphite is opaque, soft, greasy to the touch, and iron black to steel gray in color; it occurs as crystals, flakes, scales, veins, bedded masses, or disseminations in metamorphic rocks.</skos:scopeNote>
</skos:Concept>
<skos:Concept rdf:about="http://partage.vocnet.org/part00906">
	<skos:prefLabel xml:lang="en">ink</skos:prefLabel>
	<skos:prefLabel xml:lang="de">Tusche</skos:prefLabel>
	<skos:altLabel xml:lang="sv">tusch</skos:altLabel>
	<skos:prefLabel xml:lang="sv">bläck</skos:prefLabel>
	<skos:prefLabel xml:lang="pt">tinta</skos:prefLabel>
	<skos:altLabel xml:lang="hr">tuš</skos:altLabel>
	<skos:altLabel xml:lang="de">Tinte</skos:altLabel>
	<skos:prefLabel xml:lang="fi">muste</skos:prefLabel>
	<skos:prefLabel xml:lang="hr">tinta</skos:prefLabel>
	<skos:inScheme rdf:resource="http://partage.vocnet.org/Materials"/>
	<skos:broader rdf:resource="http://partage.vocnet.org/part00610"/>
	<skos:exactMatch rdf:resource="http://vocab.getty.edu/aat/300015012"/>
	<skos:editorialNote xml:lang="en">PPMaterial</skos:editorialNote>
	<skos:scopeNote xml:lang="en">A fluid medium used for drawings or tracings. An opaque, usually black, pigment is mixed with a vehicle such as water to produce a fluid which can be applied with a pen or stylus. Through the end of the 19th century, ink was supplied dried in stick or block form which was ground and mixed with water as needed. At the beginning of this century prepared ink became popular.</skos:scopeNote>
</skos:Concept>
<skos:Concept rdf:about="http://partage.vocnet.org/part00907">
	<skos:prefLabel xml:lang="en">elm</skos:prefLabel>
	<skos:prefLabel xml:lang="de">Ulme</skos:prefLabel>
	<skos:prefLabel xml:lang="sv">alm</skos:prefLabel>
	<skos:prefLabel xml:lang="pt">olmo</skos:prefLabel>
	<skos:prefLabel xml:lang="hr">brijestovina</skos:prefLabel>
	<skos:prefLabel xml:lang="fi">jalava</skos:prefLabel>
	<skos:inScheme rdf:resource="http://partage.vocnet.org/Materials"/>
	<skos:broader rdf:resource="http://partage.vocnet.org/part00606"/>
	<skos:exactMatch rdf:resource="http://vocab.getty.edu/aat/300012070"/>
	<skos:editorialNote xml:lang="en">PPMaterial</skos:editorialNote>
	<skos:scopeNote xml:lang="en">Tough, durable, brown-color wood of the genus Ulmus that is used for ax handles, yokes, wheels, weapons, coffins, ships' structure, and gymnasium equipment.</skos:scopeNote>
</skos:Concept>
<skos:Concept rdf:about="http://partage.vocnet.org/part00908">
	<skos:prefLabel xml:lang="en">ebony</skos:prefLabel>
	<skos:prefLabel xml:lang="de">Ebenholz</skos:prefLabel>
	<skos:prefLabel xml:lang="sv">ebenholts</skos:prefLabel>
	<skos:prefLabel xml:lang="pt">ébano</skos:prefLabel>
	<skos:prefLabel xml:lang="fi">eebenpuu</skos:prefLabel>
	<skos:prefLabel xml:lang="hr">ebanovina</skos:prefLabel>
	<skos:inScheme rdf:resource="http://partage.vocnet.org/Materials"/>
	<skos:broader rdf:resource="http://partage.vocnet.org/part00606"/>
	<skos:exactMatch rdf:resource="http://vocab.getty.edu/aat/300012055"/>
	<skos:editorialNote xml:lang="en">PPMaterial</skos:editorialNote>
	<skos:scopeNote xml:lang="en">A hard, heavy, durable heartwood wood yielded by various trees of the genus Diospyros in tropical Asia and Africa, valued for its dense, smooth-grain from the earliest times; was imported to Egypt from Nubia and the Sudan. It is extremely durable, resistant to rotting, fungi and powder post beetles, but difficult to work and carve. It has been used for decorative items, inlay work, black piano keys, musical instruments, and tool handles. Several other dark, heavy woods from unrelated species are also called ebony because of their color, including cocuswood, coffeewood, blue ebony, and African blackwood.</skos:scopeNote>
</skos:Concept>
<skos:Concept rdf:about="http://partage.vocnet.org/part00909">
	<skos:prefLabel xml:lang="en">beech</skos:prefLabel>
	<skos:prefLabel xml:lang="de">Buche</skos:prefLabel>
	<skos:prefLabel xml:lang="sv">bok</skos:prefLabel>
	<skos:prefLabel xml:lang="pt">faia</skos:prefLabel>
	<skos:prefLabel xml:lang="fi">pyökki</skos:prefLabel>
	<skos:prefLabel xml:lang="hr">bukovina</skos:prefLabel>
	<skos:inScheme rdf:resource="http://partage.vocnet.org/Materials"/>
	<skos:broader rdf:resource="http://partage.vocnet.org/part00606"/>
	<skos:exactMatch rdf:resource="http://vocab.getty.edu/aat/300011948"/>
	<skos:editorialNote xml:lang="en">PPMaterial</skos:editorialNote>
	<skos:scopeNote xml:lang="en">Pale reddish-brown, close-grain wood from any of several trees of the genus Fagus; it is hard and heavy, bends well, is durable under water, and gives a smooth shiny finish. Beech wood is commonly used for flooring, cabinetry, furniture (especially bentwood chairs), veneer, plywood, tool handles, and turnery. It was used in panel paintings in western Europe.</skos:scopeNote>
</skos:Concept>
<skos:Concept rdf:about="http://partage.vocnet.org/part00910">
	<skos:prefLabel xml:lang="en">Bakelite (TM)</skos:prefLabel>
	<skos:prefLabel xml:lang="de">Bakelit (TM)</skos:prefLabel>
	<skos:prefLabel xml:lang="sv">bakelit</skos:prefLabel>
	<skos:prefLabel xml:lang="pt">bakelite</skos:prefLabel>
	<skos:prefLabel xml:lang="fi">bakeliitti</skos:prefLabel>
	<skos:prefLabel xml:lang="hr">bakelit</skos:prefLabel>
	<skos:inScheme rdf:resource="http://partage.vocnet.org/Materials"/>
	<skos:broader rdf:resource="http://partage.vocnet.org/part00911"/>
	<skos:exactMatch rdf:resource="http://vocab.getty.edu/aat/300014544"/>
	<skos:editorialNote xml:lang="en">PPMaterial</skos:editorialNote>
	<skos:scopeNote xml:lang="en">The original trademarked name for phenol-formaldehyde resin, but now used to refer to a range of different types of plastic. The method for manufacturing the original resin was devised in 1909 by L. H. Baekeland in the United States, and the name Bakelite is a registered trademark of the Union Carbide Corporation. It is a hard, infusible, and chemically resistant plastic, nonconductor of electricity, and used in electrical appliances, industrial applications, in molding and casting operations, as an adhesive, in paints, and in baked-enamel coatings.</skos:scopeNote>
</skos:Concept>
<skos:Concept rdf:about="http://partage.vocnet.org/part00911">
	<skos:prefLabel xml:lang="de">Phenol</skos:prefLabel>
	<skos:prefLabel xml:lang="en">phenolic</skos:prefLabel>
	<skos:inScheme rdf:resource="http://partage.vocnet.org/Materials"/>
	<skos:broader rdf:resource="http://partage.vocnet.org/part00940"/>
	<skos:narrower rdf:resource="http://partage.vocnet.org/part00910"/>
	<skos:exactMatch rdf:resource="http://vocab.getty.edu/aat/300014540"/>
	<skos:scopeNote xml:lang="en">Refers to any of a large class of synthetic resins made by reacting phenol with formaldehyde. Phenolic resins were the first totally synthetic polymers to be commercialized. Bakelite is a phenolic plastic. Current industrial applications include adhesives in plywood.</skos:scopeNote>
</skos:Concept>
<skos:Concept rdf:about="http://partage.vocnet.org/part00912">
	<skos:prefLabel xml:lang="en">mahogany</skos:prefLabel>
	<skos:prefLabel xml:lang="sv">mahogny</skos:prefLabel>
	<skos:prefLabel xml:lang="pt">mogno</skos:prefLabel>
	<skos:prefLabel xml:lang="de">Mahagoni</skos:prefLabel>
	<skos:prefLabel xml:lang="fi">mahonki</skos:prefLabel>
	<skos:prefLabel xml:lang="hr">mahagonij</skos:prefLabel>
	<skos:inScheme rdf:resource="http://partage.vocnet.org/Materials"/>
	<skos:broader rdf:resource="http://partage.vocnet.org/part00606"/>
	<skos:exactMatch rdf:resource="http://vocab.getty.edu/aat/300012221"/>
	<skos:editorialNote xml:lang="en">PPMaterial</skos:editorialNote>
	<skos:scopeNote xml:lang="en">Refers to the wood of trees of the genus Swietenia, found in tropical climates, primarily in Mexico, Cuba, Central America, and the West Indies. It varies in color from yellow to a rich red brown, and is valued in furniture-making and sculpture-carving because it is hard, fine-grained, and takes a high polish. Mahogany has a fine, straight grain that takes a high polish. It is dimensionally stable and does not shrink, warp, or swell. The durable, dark reddish-brown wood was imported to Europe in the 18th century where it became popular for furniture, paneling and veneer. Ammonia brings out a rich, red color in mahogany wood. Mahogany is frequently attacked by pinhole borer beetles. Many woods of similar colors have also been called mahoganies, but usually do not have rich color or fine cutting characteristics of the true mahogany wood. However, the related African genus Khaya produces a similar wood. Mahogany was used by Chippendale, Hepplewhite, and the Adam brothers for high quality furniture.</skos:scopeNote>
</skos:Concept>
<skos:Concept rdf:about="http://partage.vocnet.org/part00913">
	<skos:prefLabel xml:lang="en">gabardine</skos:prefLabel>
	<skos:altLabel xml:lang="de">Gabardine</skos:altLabel>
	<skos:prefLabel xml:lang="sv">gabardin</skos:prefLabel>
	<skos:prefLabel xml:lang="de">gabardin</skos:prefLabel>
	<skos:prefLabel xml:lang="pt">gabardin</skos:prefLabel>
	<skos:prefLabel xml:lang="hr">gabarden</skos:prefLabel>
	<skos:prefLabel xml:lang="fi">gabardiini</skos:prefLabel>
	<skos:inScheme rdf:resource="http://partage.vocnet.org/Materials"/>
	<skos:broader rdf:resource="http://partage.vocnet.org/part00229"/>
	<skos:editorialNote xml:lang="en">PPMaterial</skos:editorialNote>
	<skos:scopeNote xml:lang="de">Festes Kammgarngewebe, h\u00e4ufig f\u00fcr M\u00e4ntel und Jacken verwendet.</skos:scopeNote>
	<skos:scopeNote xml:lang="de">Textile material made of worsted yarn mainly used for coats and jackets.</skos:scopeNote>
</skos:Concept>
<skos:Concept rdf:about="http://partage.vocnet.org/part00940">
	<skos:prefLabel xml:lang="en">thermoset</skos:prefLabel>
	<skos:inScheme rdf:resource="http://partage.vocnet.org/Materials"/>
	<skos:broader rdf:resource="http://partage.vocnet.org/part00941"/>
	<skos:narrower rdf:resource="http://partage.vocnet.org/part00911"/>
	<skos:exactMatch rdf:resource="http://vocab.getty.edu/aat/300014515"/>
	<skos:scopeNote xml:lang="en">A polymer with strong intermolecular bonding that becomes rigid by chemical reaction and that is not remeltable. Thermoset polymers are usually insoluble in most solvents. Examples of thermoset polymers are epoxies, silicones, and phenolics along with some polyesters and polyurethanes.</skos:scopeNote>
</skos:Concept>
<skos:Concept rdf:about="http://partage.vocnet.org/part00941">
	<skos:prefLabel xml:lang="en">plastic (organic material)</skos:prefLabel>
	<skos:inScheme rdf:resource="http://partage.vocnet.org/Materials"/>
	<skos:broader rdf:resource="http://partage.vocnet.org/part00615"/>
	<skos:narrower rdf:resource="http://partage.vocnet.org/part00940"/>
	<skos:narrower rdf:resource="http://partage.vocnet.org/part01151"/>
	<skos:exactMatch rdf:resource="http://vocab.getty.edu/aat/300014570"/>
	<skos:scopeNote xml:lang="en">A general term for any of a large and varied class of natural or synthetic organic materials that can be molded, extruded, or cast when soft or liquid, and then set into a rigid or slightly elastic form. Natural plastics include tree resins, beeswax, gutta-percha, horn, and clay. Synthetic plastics were first made in the 19th century. Plastics are used widely in manufacturing.</skos:scopeNote>
</skos:Concept>
<skos:Concept rdf:about="http://partage.vocnet.org/part01035">
	<skos:prefLabel xml:lang="en">silver halide</skos:prefLabel>
	<skos:inScheme rdf:resource="http://partage.vocnet.org/Materials"/>
	<skos:broader rdf:resource="http://partage.vocnet.org/part00229"/>
	<skos:narrower rdf:resource="http://partage.vocnet.org/part00889"/>
	<skos:exactMatch rdf:resource="http://vocab.getty.edu/aat/300130942"/>
	<skos:editorialNote xml:lang="en">PPMaterial</skos:editorialNote>
	<skos:scopeNote xml:lang="en">A compound in which silver is combined with a halogen, typically silver chloride, bromide or iodide.</skos:scopeNote>
</skos:Concept>
<skos:Concept rdf:about="http://partage.vocnet.org/part01077">
	<skos:prefLabel xml:lang="en">Clutha glass</skos:prefLabel>
	<skos:inScheme rdf:resource="http://partage.vocnet.org/Materials"/>
	<skos:broader rdf:resource="http://partage.vocnet.org/part00246"/>
	<skos:exactMatch rdf:resource="http://vocab.getty.edu/aat/300206370"/>
	<skos:scopeNote xml:lang="en">A type of glass characterized by its mainly greenish, turquoise, yellow, brown-green, or smoky black color accented by air bubbles, streaks of pink and white, and speckles of aventurine; made by James Couper + Sons, Glasgow.</skos:scopeNote>
	<skos:editorialNote xml:lang="en">PPMaterial</skos:editorialNote>
</skos:Concept>
<skos:Concept rdf:about="http://partage.vocnet.org/part01147">
	<skos:prefLabel xml:lang="de">Bambus (Material)</skos:prefLabel>
	<skos:prefLabel xml:lang="en">bamboo (material)</skos:prefLabel>
	<skos:prefLabel xml:lang="hr">bambus</skos:prefLabel>
	<skos:inScheme rdf:resource="http://partage.vocnet.org/Materials"/>
	<skos:broader rdf:resource="http://partage.vocnet.org/part01148"/>
	<skos:exactMatch rdf:resource="http://vocab.getty.edu/aat/300011873"/>
	<skos:scopeNote xml:lang="en">Material derived from the stem or stalk of the bamboo plant, which is any of 480 species of woody or treelike tropical and semitropical grass.</skos:scopeNote>
	<skos:editorialNote xml:lang="en">PPMaterial</skos:editorialNote>
</skos:Concept>
<skos:Concept rdf:about="http://partage.vocnet.org/part01148">
	<skos:prefLabel xml:lang="de">Gras (Material)</skos:prefLabel>
	<skos:prefLabel xml:lang="en">grass (plant material)</skos:prefLabel>
	<skos:inScheme rdf:resource="http://partage.vocnet.org/Materials"/>
	<skos:broader rdf:resource="http://partage.vocnet.org/part00297"/>
	<skos:narrower rdf:resource="http://partage.vocnet.org/part01147"/>
	<skos:exactMatch rdf:resource="http://vocab.getty.edu/aat/300011872"/>
	<skos:editorialNote xml:lang="en">PPMaterial</skos:editorialNote>
	<skos:scopeNote xml:lang="en">Plants of the family Gramine\u00e6, and plants resembling these in general appearance.</skos:scopeNote>
</skos:Concept>
<skos:Concept rdf:about="http://partage.vocnet.org/part01149">
	<skos:prefLabel xml:lang="hr">celuloid</skos:prefLabel>
	<skos:prefLabel xml:lang="de">Zelluloid</skos:prefLabel>
	<skos:prefLabel xml:lang="en">celluloid (cellulosic)</skos:prefLabel>
	<skos:inScheme rdf:resource="http://partage.vocnet.org/Materials"/>
	<skos:broader rdf:resource="http://partage.vocnet.org/part01150"/>
	<skos:editorialNote xml:lang="en">PPMaterial</skos:editorialNote>
	<skos:scopeNote xml:lang="en">A tough, highly flammable but not usually explosive, synthetic thermoplastic composed essentially of cellulose nitrate and camphor or another plasticizer. It was originally a trademark of Hoechst Celanese. It was marketed as a substitute for ivory, horn, amber, tortoiseshell for use in piano keys, dolls, buttons, combs, brushes, mirrors, collars, dental plates, and other small items. Tough, transparent sheets and strips of celluloid were also used for photographic and motion picture films as well as animation cels. Celluloid film was cast from a solution of cellulose nitrate with wood alcohol (methanol), amyl nitrate, camphor and fusel oil (amyl alcohol).</skos:scopeNote>
</skos:Concept>
<skos:Concept rdf:about="http://partage.vocnet.org/part01150">
	<skos:prefLabel xml:lang="en">cellulosic</skos:prefLabel>
	<skos:inScheme rdf:resource="http://partage.vocnet.org/Materials"/>
	<skos:broader rdf:resource="http://partage.vocnet.org/part01151"/>
	<skos:narrower rdf:resource="http://partage.vocnet.org/part01149"/>
	<skos:exactMatch rdf:resource="http://vocab.getty.edu/aat/300014437"/>
	<skos:scopeNote xml:lang="en">Thermoplastic made from cellulose or a cellulose compound.</skos:scopeNote>
</skos:Concept>
<skos:Concept rdf:about="http://partage.vocnet.org/part01151">
	<skos:prefLabel xml:lang="en">thermoplastic</skos:prefLabel>
	<skos:inScheme rdf:resource="http://partage.vocnet.org/Materials"/>
	<skos:broader rdf:resource="http://partage.vocnet.org/part00941"/>
	<skos:narrower rdf:resource="http://partage.vocnet.org/part01150"/>
	<skos:exactMatch rdf:resource="http://vocab.getty.edu/aat/300014415"/>
	<skos:scopeNote xml:lang="en">Plastic that becomes soft when heated and hard when cooled, no matter how often these processes are repeated, because of little or no cross-bonding between molecules.</skos:scopeNote>
</skos:Concept>
<skos:Concept rdf:about="http://partage.vocnet.org/part01153">
	<skos:prefLabel xml:lang="hr">emajl</skos:prefLabel>
	<skos:altLabel xml:lang="de">Emaille</skos:altLabel>
	<skos:prefLabel xml:lang="en">enamel (fused coating)</skos:prefLabel>
	<skos:prefLabel xml:lang="de">Email (Beschichtung)</skos:prefLabel>
	<skos:inScheme rdf:resource="http://partage.vocnet.org/Materials"/>
	<skos:broader rdf:resource="http://partage.vocnet.org/part00610"/>
	<skos:exactMatch rdf:resource="http://vocab.getty.edu/aat/300014910"/>
	<skos:editorialNote xml:lang="en">PPMaterial</skos:editorialNote>
	<skos:scopeNote xml:lang="en">A semi-transparent or opaque vitreous, porcelain-like coating applied by fusion to metal, glass, or ceramic, having a glossy appearance after hardening. Enamel is typically made from powdered fusible glasses (e.g., quartz, feldspar, clay, soda, and borax) and opaque colorants (e.g., cobalt blue, tin oxide) mixed with oil or water, then painted or sprayed on the object and fired up to 800 C. Enamel is used to protect a surface, to decorate objects in various colors and patterns, to form a surface for encaustic painting, and for other purposes.</skos:scopeNote>
</skos:Concept>
<skos:Concept rdf:about="http://partage.vocnet.org/part01154">
	<skos:prefLabel xml:lang="hr">kruška</skos:prefLabel>
	<skos:prefLabel xml:lang="de">Birnenholz</skos:prefLabel>
	<skos:prefLabel xml:lang="en">pear (wood)</skos:prefLabel>
	<skos:inScheme rdf:resource="http://partage.vocnet.org/Materials"/>
	<skos:broader rdf:resource="http://partage.vocnet.org/part00606"/>
	<skos:exactMatch rdf:resource="http://vocab.getty.edu/aat/300012338"/>
	<skos:editorialNote xml:lang="en">PPMaterial</skos:editorialNote>
	<skos:scopeNote xml:lang="en">Wood trees belonging to the genus Pyrus, pale pinkish-brown in color with a very fine texture. It is used for making bowls, brush handles, drawing instruments, and cabinetry.</skos:scopeNote>
</skos:Concept>
<skos:Concept rdf:about="http://partage.vocnet.org/part01203">
	<skos:prefLabel xml:lang="de">Legierung</skos:prefLabel>
	<skos:prefLabel xml:lang="hr">legura</skos:prefLabel>
	<skos:prefLabel xml:lang="en">alloy</skos:prefLabel>
	<skos:inScheme rdf:resource="http://partage.vocnet.org/Materials"/>
	<skos:broader rdf:resource="http://partage.vocnet.org/part00259"/>
	<skos:exactMatch rdf:resource="http://vocab.getty.edu/aat/300010902"/>
	<skos:editorialNote xml:lang="en">PPMaterial</skos:editorialNote>
	<skos:scopeNote xml:lang="en">Substance having metallic properties, consisting of two or more metallic elements or of metallic and nonmetallic elements, which are miscible with each other when molten, and do not separate into distinct layers when solid.</skos:scopeNote>
</skos:Concept>
<skos:Concept rdf:about="http://partage.vocnet.org/part01205">
	<skos:prefLabel xml:lang="hr">liko</skos:prefLabel>
	<skos:prefLabel xml:lang="de">Bast</skos:prefLabel>
	<skos:prefLabel xml:lang="en">bast</skos:prefLabel>
	<skos:inScheme rdf:resource="http://partage.vocnet.org/Materials"/>
	<skos:broader rdf:resource="http://partage.vocnet.org/part01206"/>
	<skos:exactMatch rdf:resource="http://vocab.getty.edu/aat/300048153"/>
	<skos:editorialNote xml:lang="en">PPMaterial</skos:editorialNote>
	<skos:scopeNote xml:lang="en">Strong, woody fibers obtained from the phloem tissues (from the bark, stems, and leaves) of many plants, used for textiles, rope, and paper. Such fibers are characterized by fineness and flexibility. They are derived from flax, hemp, ramie, jute, abaca, cantala, henequen, sisal, pineapple, mitsumata, gampi, kozo, and other plants.</skos:scopeNote>
</skos:Concept>
<skos:Concept rdf:about="http://partage.vocnet.org/part01206">
	<skos:altLabel xml:lang="de">Pflanzliche Fasern</skos:altLabel>
	<skos:altLabel xml:lang="de">Pflanzenfasern</skos:altLabel>
	<skos:altLabel xml:lang="de">Pflanzliche Faser</skos:altLabel>
	<skos:prefLabel xml:lang="de">Pflanzenfaser</skos:prefLabel>
	<skos:prefLabel xml:lang="en">plant fibre</skos:prefLabel>
	<skos:altLabel xml:lang="en">plant fiber</skos:altLabel>
	<skos:inScheme rdf:resource="http://partage.vocnet.org/Materials"/>
	<skos:broader rdf:resource="http://partage.vocnet.org/part01207"/>
	<skos:narrower rdf:resource="http://partage.vocnet.org/part01205"/>
	<skos:exactMatch rdf:resource="http://vocab.getty.edu/aat/300014031"/>
	<skos:scopeNote xml:lang="en">Natural fiber made from plant material, often used in papermaking.</skos:scopeNote>
</skos:Concept>
<skos:Concept rdf:about="http://partage.vocnet.org/part01207">
	<skos:altLabel xml:lang="de">Naturfasern</skos:altLabel>
	<skos:prefLabel xml:lang="de">Naturfaser</skos:prefLabel>
	<skos:altLabel xml:lang="en">natural fiber</skos:altLabel>
	<skos:prefLabel xml:lang="en">natural fibre</skos:prefLabel>
	<skos:inScheme rdf:resource="http://partage.vocnet.org/Materials"/>
	<skos:broader rdf:resource="http://partage.vocnet.org/part01208"/>
	<skos:narrower rdf:resource="http://partage.vocnet.org/part01206"/>
	<skos:exactMatch rdf:resource="http://vocab.getty.edu/aat/300014027"/>
	<skos:scopeNote xml:lang="en">Fiber obtained from an animal, vegetable, or mineral source used for conversion into non-woven fabrics (felt, paper) or woven cloth.</skos:scopeNote>
</skos:Concept>
<skos:Concept rdf:about="http://partage.vocnet.org/part01208">
	<skos:prefLabel xml:lang="en">fibre</skos:prefLabel>
	<skos:altLabel xml:lang="en">fiber</skos:altLabel>
	<skos:inScheme rdf:resource="http://partage.vocnet.org/Materials"/>
	<skos:broader rdf:resource="http://partage.vocnet.org/part00229"/>
	<skos:narrower rdf:resource="http://partage.vocnet.org/part01207"/>
	<skos:narrower rdf:resource="http://partage.vocnet.org/part01217"/>
	<skos:exactMatch rdf:resource="http://vocab.getty.edu/aat/300014024"/>
	<skos:scopeNote xml:lang="en">Material comprising long, thin filaments with a length at least 100 times their diameter; characterized by flexibility. Fiber is used to make thread, cordage, textiles, paper, mats, and as fillers and strengtheners in composite materials.</skos:scopeNote>
</skos:Concept>
<skos:Concept rdf:about="http://partage.vocnet.org/part01209">
	<skos:prefLabel xml:lang="hr">lipa</skos:prefLabel>
	<skos:prefLabel xml:lang="de">Linde</skos:prefLabel>
	<skos:altLabel xml:lang="en">limewood (wood)</skos:altLabel>
	<skos:prefLabel xml:lang="en">linden (wood)</skos:prefLabel>
	<skos:inScheme rdf:resource="http://partage.vocnet.org/Materials"/>
	<skos:broader rdf:resource="http://partage.vocnet.org/part00606"/>
	<skos:exactMatch rdf:resource="http://vocab.getty.edu/aat/300012456"/>
	<skos:editorialNote xml:lang="en">PPMaterial</skos:editorialNote>
	<skos:scopeNote xml:lang="en">Light-brown wood from of any of several trees of the genus Tilia, having a straight grain and easily worked. Linden wood is used for furniture and cabinets. Its particular structural character lends itself well to carving, allowing tools to be used both along the grain and to some extent axially. Because linden wood is soft and workable, it has been used since the 1500s for decorative items with intricate carvings, such as picture frames and sculptures. Despite its relative cost, it was the most common wood used for sculpture in Germany. During the late 15th and early 16th centuries limewood was the preferred material for the genre of the winged altarpiece.</skos:scopeNote>
</skos:Concept>
<skos:Concept rdf:about="http://partage.vocnet.org/part01210">
	<skos:prefLabel xml:lang="hr">organdi</skos:prefLabel>
	<skos:prefLabel xml:lang="de">Organdy</skos:prefLabel>
	<skos:altLabel xml:lang="en">organdie</skos:altLabel>
	<skos:prefLabel xml:lang="en">organdy</skos:prefLabel>
	<skos:inScheme rdf:resource="http://partage.vocnet.org/Materials"/>
	<skos:broader rdf:resource="http://partage.vocnet.org/part00288"/>
	<skos:exactMatch rdf:resource="http://vocab.getty.edu/aat/300310128"/>
	<skos:editorialNote xml:lang="en">PPMaterial</skos:editorialNote>
	<skos:scopeNote xml:lang="en">Sheer, lightweight, crisp, semitransparent cotton fabric. It is a plain woven cloth of fine combed yarns.</skos:scopeNote>
</skos:Concept>
<skos:Concept rdf:about="http://partage.vocnet.org/part01211">
	<skos:prefLabel xml:lang="hr">slama</skos:prefLabel>
	<skos:prefLabel xml:lang="de">Stroh</skos:prefLabel>
	<skos:prefLabel xml:lang="en">straw (plant material)</skos:prefLabel>
	<skos:inScheme rdf:resource="http://partage.vocnet.org/Materials"/>
	<skos:broader rdf:resource="http://partage.vocnet.org/part00297"/>
	<skos:exactMatch rdf:resource="http://vocab.getty.edu/aat/300011908"/>
	<skos:editorialNote xml:lang="en">PPMaterials</skos:editorialNote>
	<skos:scopeNote xml:lang="en">Dried stalks of cereals or other grasses, used for many purposes, including weaving, plaiting, and braiding.</skos:scopeNote>
</skos:Concept>
<skos:Concept rdf:about="http://partage.vocnet.org/part01212">
	<skos:altLabel xml:lang="de">Schamott</skos:altLabel>
	<skos:prefLabel xml:lang="hr">šamot</skos:prefLabel>
	<skos:prefLabel xml:lang="en">fireclay (clay)</skos:prefLabel>
	<skos:prefLabel xml:lang="de">Schamotte</skos:prefLabel>
	<skos:inScheme rdf:resource="http://partage.vocnet.org/Materials"/>
	<skos:broader rdf:resource="http://partage.vocnet.org/part00227"/>
	<skos:exactMatch rdf:resource="http://vocab.getty.edu/aat/300010457"/>
	<skos:editorialNote xml:lang="en">PPMaterial</skos:editorialNote>
	<skos:scopeNote xml:lang="en">Clay capable of withstanding very high termperatures without fusing or softening; used especially for firebrick and crucibles.</skos:scopeNote>
</skos:Concept>
<skos:Concept rdf:about="http://partage.vocnet.org/part01214">
	<skos:prefLabel xml:lang="hr">terakota</skos:prefLabel>
	<skos:prefLabel xml:lang="de">Terracotta</skos:prefLabel>
	<skos:prefLabel xml:lang="en">terracotta (clay material)</skos:prefLabel>
	<skos:inScheme rdf:resource="http://partage.vocnet.org/Materials"/>
	<skos:broader rdf:resource="http://partage.vocnet.org/part00227"/>
	<skos:exactMatch rdf:resource="http://vocab.getty.edu/aat/300010669"/>
	<skos:editorialNote xml:lang="en">PPMaterial</skos:editorialNote>
	<skos:scopeNote xml:lang="en">A baked or semi-fired material that is usually a mixture of clay, grog, and water; it has been used for pottery, statuettes, lamps, roof tiles, and cornices since ancient times. It may be glazed prior to firing. To produce an item, terracotta is molded or shaped, dried for several days then fired to at least 600 C. It is fireproof, lighter in weight than stone, and usually brownish red in color.</skos:scopeNote>
</skos:Concept>
<skos:Concept rdf:about="http://partage.vocnet.org/part01215">
	<skos:prefLabel xml:lang="hr">žica</skos:prefLabel>
	<skos:prefLabel xml:lang="de">Draht</skos:prefLabel>
	<skos:prefLabel xml:lang="en">wire</skos:prefLabel>
	<skos:inScheme rdf:resource="http://partage.vocnet.org/Materials"/>
	<skos:broader rdf:resource="http://partage.vocnet.org/part00259"/>
	<skos:exactMatch rdf:resource="http://vocab.getty.edu/aat/300011063"/>
	<skos:editorialNote xml:lang="en">PPMaterial</skos:editorialNote>
	<skos:scopeNote xml:lang="en">Filament or slender rod of drawn metal.</skos:scopeNote>
</skos:Concept>
<skos:Concept rdf:about="http://partage.vocnet.org/part01217">
	<skos:altLabel xml:lang="de">Synthetische Faser</skos:altLabel>
	<skos:prefLabel xml:lang="de">Synthetikfaser</skos:prefLabel>
	<skos:prefLabel xml:lang="en">synthetic fibre</skos:prefLabel>
	<skos:altLabel xml:lang="en">synthetic fiber</skos:altLabel>
	<skos:inScheme rdf:resource="http://partage.vocnet.org/Materials"/>
	<skos:broader rdf:resource="http://partage.vocnet.org/part01208"/>
	<skos:exactMatch rdf:resource="http://vocab.getty.edu/aat/300014058"/>
	<skos:editorialNote xml:lang="en">PPMaterial</skos:editorialNote>
	<skos:scopeNote xml:lang="en">Fiber made from chemical substances, used for textile production.</skos:scopeNote>
</skos:Concept>
<skos:Concept rdf:about="http://partage.vocnet.org/part01218">
	<skos:prefLabel xml:lang="de">Platin</skos:prefLabel>
	<skos:prefLabel xml:lang="en">platinum (metal)</skos:prefLabel>
	<skos:inScheme rdf:resource="http://partage.vocnet.org/Materials"/>
	<skos:broader rdf:resource="http://partage.vocnet.org/part00265"/>
	<skos:exactMatch rdf:resource="http://vocab.getty.edu/aat/300011031"/>
	<skos:editorialNote xml:lang="en">PPMaterial</skos:editorialNote>
	<skos:scopeNote xml:lang="en">Pure metallic element having symbol Pt and atomic number 78; a lustrous, malleable, ductile, silvery white metal, considered a precious metal. Use also for this metal as processed and formed, usually in combination with other substances, to make objects and materials.</skos:scopeNote>
</skos:Concept>
<skos:Concept rdf:about="http://partage.vocnet.org/part01219">
	<skos:prefLabel xml:lang="en">alder (wood)</skos:prefLabel>
	<skos:prefLabel xml:lang="de">Erle</skos:prefLabel>
	<skos:inScheme rdf:resource="http://partage.vocnet.org/Materials"/>
	<skos:broader rdf:resource="http://partage.vocnet.org/part00606"/>
	<skos:exactMatch rdf:resource="http://vocab.getty.edu/aat/300011918"/>
	<skos:editorialNote xml:lang="en">PPMaterial</skos:editorialNote>
	<skos:scopeNote xml:lang="en">Wood of the shrub or tree belonging to the genus Alnus, of the birch family, ranging in color from pale yellow to reddish brown, and used for making furniture, cabinetry, turnery, and in charcoal manufacture and millwork.</skos:scopeNote>
</skos:Concept>
<skos:Concept rdf:about="http://partage.vocnet.org/part01220">
	<skos:prefLabel xml:lang="en">pine (wood)</skos:prefLabel>
	<skos:prefLabel xml:lang="de">Kiefer</skos:prefLabel>
	<skos:prefLabel xml:lang="fi">mänty</skos:prefLabel>
	<skos:inScheme rdf:resource="http://partage.vocnet.org/Materials"/>
	<skos:broader rdf:resource="http://partage.vocnet.org/part01221"/>
	<skos:exactMatch rdf:resource="http://vocab.getty.edu/aat/300012620"/>
	<skos:editorialNote xml:lang="en">PPMaterial</skos:editorialNote>
	<skos:scopeNote xml:lang="en">Wood from numerous trees of the genus Pinus. Pine is used largely in the construction and paper industries, although it is also a source of turpentine, resins, and oils, among other products.</skos:scopeNote>
</skos:Concept>
<skos:Concept rdf:about="http://partage.vocnet.org/part01221">
	<skos:prefLabel xml:lang="en">softwood</skos:prefLabel>
	<skos:inScheme rdf:resource="http://partage.vocnet.org/Materials"/>
	<skos:broader rdf:resource="http://partage.vocnet.org/part00295"/>
	<skos:narrower rdf:resource="http://partage.vocnet.org/part01220"/>
	<skos:exactMatch rdf:resource="http://vocab.getty.edu/aat/300012510"/>
	<skos:scopeNote xml:lang="en">Wood that is soft or easily cut, generally restricted to the timber of coniferous trees. Contrasted to "hardwood," which is usually, but not always, harder than softwood.</skos:scopeNote>
</skos:Concept>
<skos:Concept rdf:about="http://partage.vocnet.org/part01222">
	<skos:prefLabel xml:lang="en">purpleheart (wood)</skos:prefLabel>
	<skos:prefLabel xml:lang="de">Amarant (Holz)</skos:prefLabel>
	<skos:inScheme rdf:resource="http://partage.vocnet.org/Materials"/>
	<skos:broader rdf:resource="http://partage.vocnet.org/part00606"/>
	<skos:exactMatch rdf:resource="http://vocab.getty.edu/aat/300012419"/>
	<skos:editorialNote xml:lang="en">PPMaterial</skos:editorialNote>
	<skos:scopeNote xml:lang="en">Strong, elastic purplish wood derived from several species of the genus Peltogyne. The heartwood is brown when freshly cut becoming deep purple upon exposure to air, eventually turning to a dark brown with sharply demarcated off-white sapwood. Has a fine, uniform texture and grain that is straight or slightly roey. The durable, shock-resistant wood is sometimes used for carving and for vehicle construction. Also used widely in furniture-making, marquetry, veneers, flooring, etc.</skos:scopeNote>
</skos:Concept>
<skos:Concept rdf:about="http://partage.vocnet.org/part01223">
	<skos:prefLabel xml:lang="de">Rosenholz</skos:prefLabel>
	<skos:prefLabel xml:lang="en">rosewood (wood)</skos:prefLabel>
	<skos:inScheme rdf:resource="http://partage.vocnet.org/Materials"/>
	<skos:broader rdf:resource="http://partage.vocnet.org/part00606"/>
	<skos:exactMatch rdf:resource="http://vocab.getty.edu/aat/300012424"/>
	<skos:editorialNote xml:lang="en">PPMaterial</skos:editorialNote>
	<skos:scopeNote xml:lang="en">Wood from several tropical trees of the genus Dalbergia, all having a dark red or purplish color streaked and variegated with black. Rosewood timber produces a rose-like smell when cut. The wood has a fine grain, smooth texture, and polishes to a high gloss, but because of its resinous nature is difficult to work. It is used for cabinets, musical instruments, piano cases, and veneer. It was popular during the late 18th and early 19th centuries. It is still used to fashion xylophone bars, but waning supplies restrict its use. Only around 15 of the species in the large genus Dalbergia yield rosewood.</skos:scopeNote>
</skos:Concept>
<skos:Concept rdf:about="http://partage.vocnet.org/part01224">
	<skos:prefLabel xml:lang="en">satinwood (wood)</skos:prefLabel>
	<skos:inScheme rdf:resource="http://partage.vocnet.org/Materials"/>
	<skos:broader rdf:resource="http://partage.vocnet.org/part00606"/>
	<skos:exactMatch rdf:resource="http://vocab.getty.edu/aat/300012451"/>
	<skos:editorialNote xml:lang="en">PPMaterial</skos:editorialNote>
	<skos:scopeNote xml:lang="en">General term for wood from several species of trees, characterized by being very hard, yellowish brown in color, and having a satiny luster; used especially for fine woodworking and tools.</skos:scopeNote>
</skos:Concept>
<skos:Collection rdf:about="http://partage.vocnet.org/PPMaterial">
	<skos:prefLabel>PPMaterial</skos:prefLabel>
	<skos:member rdf:resource="http://partage.vocnet.org/part00227"/>
	<skos:member rdf:resource="http://partage.vocnet.org/part00233"/>
	<skos:member rdf:resource="http://partage.vocnet.org/part00236"/>
	<skos:member rdf:resource="http://partage.vocnet.org/part00237"/>
	<skos:member rdf:resource="http://partage.vocnet.org/part00239"/>
	<skos:member rdf:resource="http://partage.vocnet.org/part00241"/>
	<skos:member rdf:resource="http://partage.vocnet.org/part00244"/>
	<skos:member rdf:resource="http://partage.vocnet.org/part00246"/>
	<skos:member rdf:resource="http://partage.vocnet.org/part00247"/>
	<skos:member rdf:resource="http://partage.vocnet.org/part00248"/>
	<skos:member rdf:resource="http://partage.vocnet.org/part00250"/>
	<skos:member rdf:resource="http://partage.vocnet.org/part00252"/>
	<skos:member rdf:resource="http://partage.vocnet.org/part00253"/>
	<skos:member rdf:resource="http://partage.vocnet.org/part00259"/>
	<skos:member rdf:resource="http://partage.vocnet.org/part00263"/>
	<skos:member rdf:resource="http://partage.vocnet.org/part00264"/>
	<skos:member rdf:resource="http://partage.vocnet.org/part00267"/>
	<skos:member rdf:resource="http://partage.vocnet.org/part00269"/>
	<skos:member rdf:resource="http://partage.vocnet.org/part00271"/>
	<skos:member rdf:resource="http://partage.vocnet.org/part00273"/>
	<skos:member rdf:resource="http://partage.vocnet.org/part00274"/>
	<skos:member rdf:resource="http://partage.vocnet.org/part00276"/>
	<skos:member rdf:resource="http://partage.vocnet.org/part00278"/>
	<skos:member rdf:resource="http://partage.vocnet.org/part00280"/>
	<skos:member rdf:resource="http://partage.vocnet.org/part00281"/>
	<skos:member rdf:resource="http://partage.vocnet.org/part00288"/>
	<skos:member rdf:resource="http://partage.vocnet.org/part00289"/>
	<skos:member rdf:resource="http://partage.vocnet.org/part00290"/>
	<skos:member rdf:resource="http://partage.vocnet.org/part00291"/>
	<skos:member rdf:resource="http://partage.vocnet.org/part00292"/>
	<skos:member rdf:resource="http://partage.vocnet.org/part00295"/>
	<skos:member rdf:resource="http://partage.vocnet.org/part00394"/>
	<skos:member rdf:resource="http://partage.vocnet.org/part00484"/>
	<skos:member rdf:resource="http://partage.vocnet.org/part00489"/>
	<skos:member rdf:resource="http://partage.vocnet.org/part00514"/>
	<skos:member rdf:resource="http://partage.vocnet.org/part00515"/>
	<skos:member rdf:resource="http://partage.vocnet.org/part00516"/>
	<skos:member rdf:resource="http://partage.vocnet.org/part00519"/>
	<skos:member rdf:resource="http://partage.vocnet.org/part00521"/>
	<skos:member rdf:resource="http://partage.vocnet.org/part00534"/>
	<skos:member rdf:resource="http://partage.vocnet.org/part00537"/>
	<skos:member rdf:resource="http://partage.vocnet.org/part00538"/>
	<skos:member rdf:resource="http://partage.vocnet.org/part00539"/>
	<skos:member rdf:resource="http://partage.vocnet.org/part00563"/>
	<skos:member rdf:resource="http://partage.vocnet.org/part00565"/>
	<skos:member rdf:resource="http://partage.vocnet.org/part00567"/>
	<skos:member rdf:resource="http://partage.vocnet.org/part00568"/>
	<skos:member rdf:resource="http://partage.vocnet.org/part00570"/>
	<skos:member rdf:resource="http://partage.vocnet.org/part00571"/>
	<skos:member rdf:resource="http://partage.vocnet.org/part00572"/>
	<skos:member rdf:resource="http://partage.vocnet.org/part00573"/>
	<skos:member rdf:resource="http://partage.vocnet.org/part00575"/>
	<skos:member rdf:resource="http://partage.vocnet.org/part00576"/>
	<skos:member rdf:resource="http://partage.vocnet.org/part00577"/>
	<skos:member rdf:resource="http://partage.vocnet.org/part00578"/>
	<skos:member rdf:resource="http://partage.vocnet.org/part00580"/>
	<skos:member rdf:resource="http://partage.vocnet.org/part00582"/>
	<skos:member rdf:resource="http://partage.vocnet.org/part00585"/>
	<skos:member rdf:resource="http://partage.vocnet.org/part00587"/>
	<skos:member rdf:resource="http://partage.vocnet.org/part00588"/>
	<skos:member rdf:resource="http://partage.vocnet.org/part00590"/>
	<skos:member rdf:resource="http://partage.vocnet.org/part00591"/>
	<skos:member rdf:resource="http://partage.vocnet.org/part00592"/>
	<skos:member rdf:resource="http://partage.vocnet.org/part00593"/>
	<skos:member rdf:resource="http://partage.vocnet.org/part00595"/>
	<skos:member rdf:resource="http://partage.vocnet.org/part00597"/>
	<skos:member rdf:resource="http://partage.vocnet.org/part00599"/>
	<skos:member rdf:resource="http://partage.vocnet.org/part00600"/>
	<skos:member rdf:resource="http://partage.vocnet.org/part00601"/>
	<skos:member rdf:resource="http://partage.vocnet.org/part00602"/>
	<skos:member rdf:resource="http://partage.vocnet.org/part00603"/>
	<skos:member rdf:resource="http://partage.vocnet.org/part00604"/>
	<skos:member rdf:resource="http://partage.vocnet.org/part00608"/>
	<skos:member rdf:resource="http://partage.vocnet.org/part00612"/>
	<skos:member rdf:resource="http://partage.vocnet.org/part00613"/>
	<skos:member rdf:resource="http://partage.vocnet.org/part00614"/>
	<skos:member rdf:resource="http://partage.vocnet.org/part00616"/>
	<skos:member rdf:resource="http://partage.vocnet.org/part00617"/>
	<skos:member rdf:resource="http://partage.vocnet.org/part00618"/>
	<skos:member rdf:resource="http://partage.vocnet.org/part00620"/>
	<skos:member rdf:resource="http://partage.vocnet.org/part00622"/>
	<skos:member rdf:resource="http://partage.vocnet.org/part00624"/>
	<skos:member rdf:resource="http://partage.vocnet.org/part00625"/>
	<skos:member rdf:resource="http://partage.vocnet.org/part00626"/>
	<skos:member rdf:resource="http://partage.vocnet.org/part00627"/>
	<skos:member rdf:resource="http://partage.vocnet.org/part00628"/>
	<skos:member rdf:resource="http://partage.vocnet.org/part00629"/>
	<skos:member rdf:resource="http://partage.vocnet.org/part00630"/>
	<skos:member rdf:resource="http://partage.vocnet.org/part00633"/>
	<skos:member rdf:resource="http://partage.vocnet.org/part00634"/>
	<skos:member rdf:resource="http://partage.vocnet.org/part00635"/>
	<skos:member rdf:resource="http://partage.vocnet.org/part00832"/>
	<skos:member rdf:resource="http://partage.vocnet.org/part00889"/>
	<skos:member rdf:resource="http://partage.vocnet.org/part00897"/>
	<skos:member rdf:resource="http://partage.vocnet.org/part00898"/>
	<skos:member rdf:resource="http://partage.vocnet.org/part00899"/>
	<skos:member rdf:resource="http://partage.vocnet.org/part00900"/>
	<skos:member rdf:resource="http://partage.vocnet.org/part00901"/>
	<skos:member rdf:resource="http://partage.vocnet.org/part00902"/>
	<skos:member rdf:resource="http://partage.vocnet.org/part00903"/>
	<skos:member rdf:resource="http://partage.vocnet.org/part00905"/>
	<skos:member rdf:resource="http://partage.vocnet.org/part00906"/>
	<skos:member rdf:resource="http://partage.vocnet.org/part00907"/>
	<skos:member rdf:resource="http://partage.vocnet.org/part00908"/>
	<skos:member rdf:resource="http://partage.vocnet.org/part00909"/>
	<skos:member rdf:resource="http://partage.vocnet.org/part00910"/>
	<skos:member rdf:resource="http://partage.vocnet.org/part00912"/>
	<skos:member rdf:resource="http://partage.vocnet.org/part00913"/>
	<skos:member rdf:resource="http://partage.vocnet.org/part01035"/>
	<skos:member rdf:resource="http://partage.vocnet.org/part01077"/>
	<skos:member rdf:resource="http://partage.vocnet.org/part01147"/>
	<skos:member rdf:resource="http://partage.vocnet.org/part01148"/>
	<skos:member rdf:resource="http://partage.vocnet.org/part01149"/>
	<skos:member rdf:resource="http://partage.vocnet.org/part01153"/>
	<skos:member rdf:resource="http://partage.vocnet.org/part01154"/>
	<skos:member rdf:resource="http://partage.vocnet.org/part01203"/>
	<skos:member rdf:resource="http://partage.vocnet.org/part01205"/>
	<skos:member rdf:resource="http://partage.vocnet.org/part01209"/>
	<skos:member rdf:resource="http://partage.vocnet.org/part01210"/>
	<skos:member rdf:resource="http://partage.vocnet.org/part01212"/>
	<skos:member rdf:resource="http://partage.vocnet.org/part01214"/>
	<skos:member rdf:resource="http://partage.vocnet.org/part01215"/>
	<skos:member rdf:resource="http://partage.vocnet.org/part01217"/>
	<skos:member rdf:resource="http://partage.vocnet.org/part01218"/>
	<skos:member rdf:resource="http://partage.vocnet.org/part01219"/>
	<skos:member rdf:resource="http://partage.vocnet.org/part01220"/>
	<skos:member rdf:resource="http://partage.vocnet.org/part01222"/>
	<skos:member rdf:resource="http://partage.vocnet.org/part01223"/>
	<skos:member rdf:resource="http://partage.vocnet.org/part01224"/>
</skos:Collection>
<skos:Collection rdf:about="http://partage.vocnet.org/IndexingConcepts">
	<skos:prefLabel>IndexingConcepts</skos:prefLabel>
	<skos:member rdf:resource="http://partage.vocnet.org/part00227"/>
	<skos:member rdf:resource="http://partage.vocnet.org/part00233"/>
	<skos:member rdf:resource="http://partage.vocnet.org/part00236"/>
	<skos:member rdf:resource="http://partage.vocnet.org/part00237"/>
	<skos:member rdf:resource="http://partage.vocnet.org/part00239"/>
	<skos:member rdf:resource="http://partage.vocnet.org/part00241"/>
	<skos:member rdf:resource="http://partage.vocnet.org/part00244"/>
	<skos:member rdf:resource="http://partage.vocnet.org/part00246"/>
	<skos:member rdf:resource="http://partage.vocnet.org/part00247"/>
	<skos:member rdf:resource="http://partage.vocnet.org/part00248"/>
	<skos:member rdf:resource="http://partage.vocnet.org/part00250"/>
	<skos:member rdf:resource="http://partage.vocnet.org/part00250"/>
	<skos:member rdf:resource="http://partage.vocnet.org/part00252"/>
	<skos:member rdf:resource="http://partage.vocnet.org/part00253"/>
	<skos:member rdf:resource="http://partage.vocnet.org/part00259"/>
	<skos:member rdf:resource="http://partage.vocnet.org/part00263"/>
	<skos:member rdf:resource="http://partage.vocnet.org/part00264"/>
	<skos:member rdf:resource="http://partage.vocnet.org/part00267"/>
	<skos:member rdf:resource="http://partage.vocnet.org/part00269"/>
	<skos:member rdf:resource="http://partage.vocnet.org/part00271"/>
	<skos:member rdf:resource="http://partage.vocnet.org/part00273"/>
	<skos:member rdf:resource="http://partage.vocnet.org/part00274"/>
	<skos:member rdf:resource="http://partage.vocnet.org/part00276"/>
	<skos:member rdf:resource="http://partage.vocnet.org/part00278"/>
	<skos:member rdf:resource="http://partage.vocnet.org/part00280"/>
	<skos:member rdf:resource="http://partage.vocnet.org/part00281"/>
	<skos:member rdf:resource="http://partage.vocnet.org/part00288"/>
	<skos:member rdf:resource="http://partage.vocnet.org/part00289"/>
	<skos:member rdf:resource="http://partage.vocnet.org/part00290"/>
	<skos:member rdf:resource="http://partage.vocnet.org/part00291"/>
	<skos:member rdf:resource="http://partage.vocnet.org/part00292"/>
	<skos:member rdf:resource="http://partage.vocnet.org/part00295"/>
	<skos:member rdf:resource="http://partage.vocnet.org/part00394"/>
	<skos:member rdf:resource="http://partage.vocnet.org/part00484"/>
	<skos:member rdf:resource="http://partage.vocnet.org/part00489"/>
	<skos:member rdf:resource="http://partage.vocnet.org/part00514"/>
	<skos:member rdf:resource="http://partage.vocnet.org/part00515"/>
	<skos:member rdf:resource="http://partage.vocnet.org/part00516"/>
	<skos:member rdf:resource="http://partage.vocnet.org/part00519"/>
	<skos:member rdf:resource="http://partage.vocnet.org/part00519"/>
	<skos:member rdf:resource="http://partage.vocnet.org/part00521"/>
	<skos:member rdf:resource="http://partage.vocnet.org/part00521"/>
	<skos:member rdf:resource="http://partage.vocnet.org/part00534"/>
	<skos:member rdf:resource="http://partage.vocnet.org/part00537"/>
	<skos:member rdf:resource="http://partage.vocnet.org/part00538"/>
	<skos:member rdf:resource="http://partage.vocnet.org/part00539"/>
	<skos:member rdf:resource="http://partage.vocnet.org/part00563"/>
	<skos:member rdf:resource="http://partage.vocnet.org/part00565"/>
	<skos:member rdf:resource="http://partage.vocnet.org/part00567"/>
	<skos:member rdf:resource="http://partage.vocnet.org/part00568"/>
	<skos:member rdf:resource="http://partage.vocnet.org/part00570"/>
	<skos:member rdf:resource="http://partage.vocnet.org/part00571"/>
	<skos:member rdf:resource="http://partage.vocnet.org/part00572"/>
	<skos:member rdf:resource="http://partage.vocnet.org/part00573"/>
	<skos:member rdf:resource="http://partage.vocnet.org/part00575"/>
	<skos:member rdf:resource="http://partage.vocnet.org/part00576"/>
	<skos:member rdf:resource="http://partage.vocnet.org/part00577"/>
	<skos:member rdf:resource="http://partage.vocnet.org/part00578"/>
	<skos:member rdf:resource="http://partage.vocnet.org/part00580"/>
	<skos:member rdf:resource="http://partage.vocnet.org/part00582"/>
	<skos:member rdf:resource="http://partage.vocnet.org/part00585"/>
	<skos:member rdf:resource="http://partage.vocnet.org/part00587"/>
	<skos:member rdf:resource="http://partage.vocnet.org/part00588"/>
	<skos:member rdf:resource="http://partage.vocnet.org/part00590"/>
	<skos:member rdf:resource="http://partage.vocnet.org/part00591"/>
	<skos:member rdf:resource="http://partage.vocnet.org/part00592"/>
	<skos:member rdf:resource="http://partage.vocnet.org/part00593"/>
	<skos:member rdf:resource="http://partage.vocnet.org/part00595"/>
	<skos:member rdf:resource="http://partage.vocnet.org/part00597"/>
	<skos:member rdf:resource="http://partage.vocnet.org/part00599"/>
	<skos:member rdf:resource="http://partage.vocnet.org/part00600"/>
	<skos:member rdf:resource="http://partage.vocnet.org/part00601"/>
	<skos:member rdf:resource="http://partage.vocnet.org/part00602"/>
	<skos:member rdf:resource="http://partage.vocnet.org/part00603"/>
	<skos:member rdf:resource="http://partage.vocnet.org/part00604"/>
	<skos:member rdf:resource="http://partage.vocnet.org/part00608"/>
	<skos:member rdf:resource="http://partage.vocnet.org/part00612"/>
	<skos:member rdf:resource="http://partage.vocnet.org/part00613"/>
	<skos:member rdf:resource="http://partage.vocnet.org/part00614"/>
	<skos:member rdf:resource="http://partage.vocnet.org/part00616"/>
	<skos:member rdf:resource="http://partage.vocnet.org/part00617"/>
	<skos:member rdf:resource="http://partage.vocnet.org/part00618"/>
	<skos:member rdf:resource="http://partage.vocnet.org/part00620"/>
	<skos:member rdf:resource="http://partage.vocnet.org/part00622"/>
	<skos:member rdf:resource="http://partage.vocnet.org/part00624"/>
	<skos:member rdf:resource="http://partage.vocnet.org/part00625"/>
	<skos:member rdf:resource="http://partage.vocnet.org/part00626"/>
	<skos:member rdf:resource="http://partage.vocnet.org/part00627"/>
	<skos:member rdf:resource="http://partage.vocnet.org/part00628"/>
	<skos:member rdf:resource="http://partage.vocnet.org/part00629"/>
	<skos:member rdf:resource="http://partage.vocnet.org/part00630"/>
	<skos:member rdf:resource="http://partage.vocnet.org/part00633"/>
	<skos:member rdf:resource="http://partage.vocnet.org/part00634"/>
	<skos:member rdf:resource="http://partage.vocnet.org/part00635"/>
	<skos:member rdf:resource="http://partage.vocnet.org/part00832"/>
	<skos:member rdf:resource="http://partage.vocnet.org/part00889"/>
	<skos:member rdf:resource="http://partage.vocnet.org/part00897"/>
	<skos:member rdf:resource="http://partage.vocnet.org/part00898"/>
	<skos:member rdf:resource="http://partage.vocnet.org/part00899"/>
	<skos:member rdf:resource="http://partage.vocnet.org/part00900"/>
	<skos:member rdf:resource="http://partage.vocnet.org/part00901"/>
	<skos:member rdf:resource="http://partage.vocnet.org/part00902"/>
	<skos:member rdf:resource="http://partage.vocnet.org/part00903"/>
	<skos:member rdf:resource="http://partage.vocnet.org/part00905"/>
	<skos:member rdf:resource="http://partage.vocnet.org/part00906"/>
	<skos:member rdf:resource="http://partage.vocnet.org/part00907"/>
	<skos:member rdf:resource="http://partage.vocnet.org/part00908"/>
	<skos:member rdf:resource="http://partage.vocnet.org/part00909"/>
	<skos:member rdf:resource="http://partage.vocnet.org/part00910"/>
	<skos:member rdf:resource="http://partage.vocnet.org/part00912"/>
	<skos:member rdf:resource="http://partage.vocnet.org/part00913"/>
	<skos:member rdf:resource="http://partage.vocnet.org/part01035"/>
	<skos:member rdf:resource="http://partage.vocnet.org/part01077"/>
	<skos:member rdf:resource="http://partage.vocnet.org/part01147"/>
	<skos:member rdf:resource="http://partage.vocnet.org/part01148"/>
	<skos:member rdf:resource="http://partage.vocnet.org/part01149"/>
	<skos:member rdf:resource="http://partage.vocnet.org/part01153"/>
	<skos:member rdf:resource="http://partage.vocnet.org/part01154"/>
	<skos:member rdf:resource="http://partage.vocnet.org/part01203"/>
	<skos:member rdf:resource="http://partage.vocnet.org/part01205"/>
	<skos:member rdf:resource="http://partage.vocnet.org/part01209"/>
	<skos:member rdf:resource="http://partage.vocnet.org/part01210"/>
	<skos:member rdf:resource="http://partage.vocnet.org/part01211"/>
	<skos:member rdf:resource="http://partage.vocnet.org/part01212"/>
	<skos:member rdf:resource="http://partage.vocnet.org/part01214"/>
	<skos:member rdf:resource="http://partage.vocnet.org/part01215"/>
	<skos:member rdf:resource="http://partage.vocnet.org/part01217"/>
	<skos:member rdf:resource="http://partage.vocnet.org/part01218"/>
	<skos:member rdf:resource="http://partage.vocnet.org/part01219"/>
	<skos:member rdf:resource="http://partage.vocnet.org/part01220"/>
	<skos:member rdf:resource="http://partage.vocnet.org/part01222"/>
	<skos:member rdf:resource="http://partage.vocnet.org/part01223"/>
	<skos:member rdf:resource="http://partage.vocnet.org/part01224"/>
</skos:Collection>
<skos:Collection rdf:about="http://partage.vocnet.org/NonIndexingConcepts">
	<skos:prefLabel>NonIndexingConcepts</skos:prefLabel>
	<skos:member rdf:resource="http://partage.vocnet.org/part00229"/>
	<skos:member rdf:resource="http://partage.vocnet.org/part00242"/>
	<skos:member rdf:resource="http://partage.vocnet.org/part00257"/>
	<skos:member rdf:resource="http://partage.vocnet.org/part00261"/>
	<skos:member rdf:resource="http://partage.vocnet.org/part00265"/>
	<skos:member rdf:resource="http://partage.vocnet.org/part00272"/>
	<skos:member rdf:resource="http://partage.vocnet.org/part00279"/>
	<skos:member rdf:resource="http://partage.vocnet.org/part00297"/>
	<skos:member rdf:resource="http://partage.vocnet.org/part00485"/>
	<skos:member rdf:resource="http://partage.vocnet.org/part00517"/>
	<skos:member rdf:resource="http://partage.vocnet.org/part00518"/>
	<skos:member rdf:resource="http://partage.vocnet.org/part00536"/>
	<skos:member rdf:resource="http://partage.vocnet.org/part00583"/>
	<skos:member rdf:resource="http://partage.vocnet.org/part00605"/>
	<skos:member rdf:resource="http://partage.vocnet.org/part00606"/>
	<skos:member rdf:resource="http://partage.vocnet.org/part00610"/>
	<skos:member rdf:resource="http://partage.vocnet.org/part00615"/>
	<skos:member rdf:resource="http://partage.vocnet.org/part00621"/>
	<skos:member rdf:resource="http://partage.vocnet.org/part00631"/>
	<skos:member rdf:resource="http://partage.vocnet.org/part00632"/>
	<skos:member rdf:resource="http://partage.vocnet.org/part00911"/>
	<skos:member rdf:resource="http://partage.vocnet.org/part00940"/>
	<skos:member rdf:resource="http://partage.vocnet.org/part00941"/>
	<skos:member rdf:resource="http://partage.vocnet.org/part01150"/>
	<skos:member rdf:resource="http://partage.vocnet.org/part01151"/>
	<skos:member rdf:resource="http://partage.vocnet.org/part01206"/>
	<skos:member rdf:resource="http://partage.vocnet.org/part01207"/>
	<skos:member rdf:resource="http://partage.vocnet.org/part01208"/>
	<skos:member rdf:resource="http://partage.vocnet.org/part01221"/>
</skos:Collection>
</rdf:RDF>