<?xml version='1.0' encoding='UTF-8'?>
<rdf:RDF xmlns:rdf="http://www.w3.org/1999/02/22-rdf-syntax-ns#" xmlns:dcterms="http://purl.org/dc/terms/" xmlns:owl="http://www.w3.org/2002/07/owl#" xmlns:skos="http://www.w3.org/2004/02/skos/core#">
<skos:ConceptScheme rdf:about="http://partage.vocnet.org/Objects">
	<rdf:type rdf:resource="http://www.w3.org/2004/02/skos/core#ConceptScheme"/>
</skos:ConceptScheme>
<skos:Concept rdf:about="http://partage.vocnet.org/part00036">
	<skos:prefLabel xml:lang="en">works on paper</skos:prefLabel>
	<skos:altLabel xml:lang="de">Kunst auf Papier</skos:altLabel>
	<skos:prefLabel xml:lang="sv">konst på papper</skos:prefLabel>
	<skos:prefLabel xml:lang="fi">paperityöt</skos:prefLabel>
	<skos:altLabel xml:lang="es">obras en papel</skos:altLabel>
	<skos:prefLabel xml:lang="es">obras sobre papel</skos:prefLabel>
	<skos:prefLabel xml:lang="sl">dela na papirju</skos:prefLabel>
	<skos:prefLabel xml:lang="pt">trabalho sobre papel</skos:prefLabel>
	<skos:prefLabel xml:lang="pl">prace na papierze</skos:prefLabel>
	<skos:prefLabel xml:lang="nl">werken op papier</skos:prefLabel>
	<skos:prefLabel xml:lang="it">oggetti di carta</skos:prefLabel>
	<skos:prefLabel xml:lang="cs">práce na papíře</skos:prefLabel>
	<skos:prefLabel xml:lang="ca">obra sobre paper</skos:prefLabel>
	<skos:prefLabel xml:lang="fr">œuvre sur papier</skos:prefLabel>
	<skos:prefLabel xml:lang="hu">papír alapú tárgy</skos:prefLabel>
	<skos:prefLabel xml:lang="no">arbeid på papir</skos:prefLabel>
	<skos:prefLabel xml:lang="hr">radovi na papiru</skos:prefLabel>
	<skos:prefLabel xml:lang="de">Graphik</skos:prefLabel>
	<skos:altLabel xml:lang="de">Arbeiten auf Papier</skos:altLabel>
	<skos:inScheme rdf:resource="http://partage.vocnet.org/Objects"/>
	<skos:exactMatch rdf:resource="http://vocab.getty.edu/aat/300189621"/>
	<skos:editorialNote xml:lang="en">PPObjectType</skos:editorialNote>
	<skos:scopeNote xml:lang="en">Use collectively to bring together works of art in which paper is the support, only when terms such as "drawings" or "prints" are not appropriate.</skos:scopeNote>
</skos:Concept>
<skos:Concept rdf:about="http://partage.vocnet.org/part00040">
	<skos:prefLabel xml:lang="en">sketches</skos:prefLabel>
	<skos:altLabel xml:lang="de">Skizze</skos:altLabel>
	<skos:prefLabel xml:lang="sv">skisser</skos:prefLabel>
	<skos:prefLabel xml:lang="fi">luonnokset</skos:prefLabel>
	<skos:prefLabel xml:lang="es">bocetos</skos:prefLabel>
	<skos:prefLabel xml:lang="sl">skice</skos:prefLabel>
	<skos:prefLabel xml:lang="pt">esboço</skos:prefLabel>
	<skos:prefLabel xml:lang="pl">szkice</skos:prefLabel>
	<skos:prefLabel xml:lang="nl">schetsen</skos:prefLabel>
	<skos:altLabel xml:lang="it">schizzi</skos:altLabel>
	<skos:prefLabel xml:lang="it">bozzetti</skos:prefLabel>
	<skos:prefLabel xml:lang="cs">skica</skos:prefLabel>
	<skos:prefLabel xml:lang="ca">esbossos</skos:prefLabel>
	<skos:prefLabel xml:lang="de">Skizzen</skos:prefLabel>
	<skos:prefLabel xml:lang="fr">esquisse</skos:prefLabel>
	<skos:prefLabel xml:lang="hu">vázlat</skos:prefLabel>
	<skos:prefLabel xml:lang="no">skisser</skos:prefLabel>
	<skos:prefLabel xml:lang="hr">skice</skos:prefLabel>
	<skos:inScheme rdf:resource="http://partage.vocnet.org/Objects"/>
	<skos:exactMatch rdf:resource="http://vocab.getty.edu/aat/300015617"/>
	<skos:editorialNote xml:lang="en">PPObjectType</skos:editorialNote>
	<skos:scopeNote xml:lang="en">Rough or summary art works; less finished than studies. Though sketches are often in the drawing medium, the term "drawings" in general implies more finished works than does "sketches."</skos:scopeNote>
</skos:Concept>
<skos:Concept rdf:about="http://partage.vocnet.org/part00041">
	<skos:altLabel xml:lang="en">sculpture (visual work)</skos:altLabel>
	<skos:prefLabel xml:lang="en">sculpture</skos:prefLabel>
	<skos:prefLabel xml:lang="de">Skulptur</skos:prefLabel>
	<skos:prefLabel xml:lang="sv">skulpturer</skos:prefLabel>
	<skos:prefLabel xml:lang="fi">veistokset</skos:prefLabel>
	<skos:prefLabel xml:lang="es">escultura</skos:prefLabel>
	<skos:altLabel xml:lang="sl">kipi</skos:altLabel>
	<skos:prefLabel xml:lang="sl">skulpture</skos:prefLabel>
	<skos:prefLabel xml:lang="pt">escultura</skos:prefLabel>
	<skos:prefLabel xml:lang="pl">rzeźba</skos:prefLabel>
	<skos:prefLabel xml:lang="nl">beeldhouwwerken</skos:prefLabel>
	<skos:prefLabel xml:lang="it">scultura</skos:prefLabel>
	<skos:prefLabel xml:lang="cs">sochařství</skos:prefLabel>
	<skos:prefLabel xml:lang="ca">escultura</skos:prefLabel>
	<skos:altLabel xml:lang="de">Plastik</skos:altLabel>
	<skos:prefLabel xml:lang="hr">skulpture</skos:prefLabel>
	<skos:prefLabel xml:lang="hu">szobrászat</skos:prefLabel>
	<skos:prefLabel xml:lang="no">skulptur</skos:prefLabel>
	<skos:prefLabel xml:lang="fr">sculpture</skos:prefLabel>
	<skos:inScheme rdf:resource="http://partage.vocnet.org/Objects"/>
	<skos:narrower rdf:resource="http://partage.vocnet.org/part00410"/>
	<skos:narrower rdf:resource="http://partage.vocnet.org/part00813"/>
	<skos:exactMatch rdf:resource="http://vocab.getty.edu/aat/300047090"/>
	<skos:editorialNote xml:lang="en">PPObjectType</skos:editorialNote>
	<skos:scopeNote xml:lang="en">Three-dimensional works of art in which images and forms are produced in relief, in intaglio, or in the round. The term refers particularly to art works created by carving or engraving a hard material, by molding or casting a malleable material (which usually then hardens), or by assembling parts to create a three-dimensional object. It is typically used to refer to large or medium-sized objects made of stone, wood, bronze, or another metal. Small objects are typically referred to as "carvings" or another appropriate term. "Sculpture" refers to works that represent tangible beings, objects, or groups of objects, or are abstract works that have defined edges and boundaries and can be measured. As three-dimensional works become more diffused in space or time, or less tangible, use appropriate specific terms, such as "mail art" or "environmental art."</skos:scopeNote>
</skos:Concept>
<skos:Concept rdf:about="http://partage.vocnet.org/part00042">
	<skos:altLabel xml:lang="en">prints (visual works)</skos:altLabel>
	<skos:prefLabel xml:lang="en">prints</skos:prefLabel>
	<skos:prefLabel xml:lang="sv">tryck</skos:prefLabel>
	<skos:prefLabel xml:lang="fi">painokuvat</skos:prefLabel>
	<skos:prefLabel xml:lang="es">estampas</skos:prefLabel>
	<skos:prefLabel xml:lang="sl">tiski</skos:prefLabel>
	<skos:prefLabel xml:lang="pt">impressões</skos:prefLabel>
	<skos:prefLabel xml:lang="pl">odbitki graficzne</skos:prefLabel>
	<skos:prefLabel xml:lang="nl">prenten</skos:prefLabel>
	<skos:prefLabel xml:lang="it">stampe</skos:prefLabel>
	<skos:prefLabel xml:lang="cs">tisk</skos:prefLabel>
	<skos:prefLabel xml:lang="ca">estampes</skos:prefLabel>
	<skos:prefLabel xml:lang="de">Druckgraphik</skos:prefLabel>
	<skos:prefLabel xml:lang="fr">imprimé</skos:prefLabel>
	<skos:prefLabel xml:lang="hu">metszet</skos:prefLabel>
	<skos:prefLabel xml:lang="no">trykk</skos:prefLabel>
	<skos:prefLabel xml:lang="hr">grafike</skos:prefLabel>
	<skos:inScheme rdf:resource="http://partage.vocnet.org/Objects"/>
	<skos:narrower rdf:resource="http://partage.vocnet.org/part00525"/>
	<skos:narrower rdf:resource="http://partage.vocnet.org/part00836"/>
	<skos:narrower rdf:resource="http://partage.vocnet.org/part00837"/>
	<skos:exactMatch rdf:resource="http://vocab.getty.edu/aat/300041273"/>
	<skos:editorialNote xml:lang="en">PPObjectType</skos:editorialNote>
	<skos:scopeNote xml:lang="en">Pictorial works produced by transferring images by means of a matrix such as a plate, block, or screen, using any of various printing processes. When emphasizing the individual printed image, use "impressions." Avoid the controversial expression "original prints," except in reference to discussions of the expression's use. If prints are neither "reproductive prints" nor "popular prints," use just "prints." With regard to photographs, see "photographic prints"; for types of reproductions of technical drawings and documents, see terms found under "reprographic copies."</skos:scopeNote>
</skos:Concept>
<skos:Concept rdf:about="http://partage.vocnet.org/part00043">
	<skos:altLabel xml:lang="en">pastels (visual works)</skos:altLabel>
	<skos:prefLabel xml:lang="en">pastels</skos:prefLabel>
	<skos:altLabel xml:lang="de">Pastelle</skos:altLabel>
	<skos:prefLabel xml:lang="sv">pasteller</skos:prefLabel>
	<skos:prefLabel xml:lang="fi">pastelli</skos:prefLabel>
	<skos:altLabel xml:lang="es">pinturas al pastel</skos:altLabel>
	<skos:prefLabel xml:lang="es">pasteles</skos:prefLabel>
	<skos:prefLabel xml:lang="sl">pasteli</skos:prefLabel>
	<skos:prefLabel xml:lang="pt">pastel</skos:prefLabel>
	<skos:prefLabel xml:lang="pl">pastele</skos:prefLabel>
	<skos:prefLabel xml:lang="nl">pastels</skos:prefLabel>
	<skos:prefLabel xml:lang="it">disegni a pastello</skos:prefLabel>
	<skos:prefLabel xml:lang="cs">pastel</skos:prefLabel>
	<skos:prefLabel xml:lang="ca">pastels</skos:prefLabel>
	<skos:prefLabel xml:lang="hr">pasteli</skos:prefLabel>
	<skos:prefLabel xml:lang="no">pastell</skos:prefLabel>
	<skos:prefLabel xml:lang="hu">pasztell</skos:prefLabel>
	<skos:prefLabel xml:lang="fr">pastel</skos:prefLabel>
	<skos:prefLabel xml:lang="de">Pastell</skos:prefLabel>
	<skos:inScheme rdf:resource="http://partage.vocnet.org/Objects"/>
	<skos:exactMatch rdf:resource="http://vocab.getty.edu/aat/300076922"/>
	<skos:editorialNote xml:lang="en">PPObjectType</skos:editorialNote>
	<skos:scopeNote xml:lang="en">Works of art, typically on a paper or vellum support, to which designs are applied using crayons made of ground pigment held together with a binder, typically oil or water and gum. Works in this medium are sometimes classified as drawings, and sometimes as paintings, typically based on the local curatorial department responsible for the work or on the material of the support (pastels on paper may be classified as drawings, while pastels on vellum may be classified as paintings).</skos:scopeNote>
</skos:Concept>
<skos:Concept rdf:about="http://partage.vocnet.org/part00044">
	<skos:altLabel xml:lang="en">paintings (visual works)</skos:altLabel>
	<skos:prefLabel xml:lang="en">paintings</skos:prefLabel>
	<skos:prefLabel xml:lang="sv">målningar</skos:prefLabel>
	<skos:prefLabel xml:lang="fi">maalaukset</skos:prefLabel>
	<skos:altLabel xml:lang="es">pinturas</skos:altLabel>
	<skos:prefLabel xml:lang="es">pintura</skos:prefLabel>
	<skos:prefLabel xml:lang="sl">slike</skos:prefLabel>
	<skos:altLabel xml:lang="pt">pinturas</skos:altLabel>
	<skos:prefLabel xml:lang="pt">pintura</skos:prefLabel>
	<skos:prefLabel xml:lang="pl">obrazy</skos:prefLabel>
	<skos:prefLabel xml:lang="nl">schilderingen</skos:prefLabel>
	<skos:prefLabel xml:lang="it">dipinti</skos:prefLabel>
	<skos:prefLabel xml:lang="cs">malba</skos:prefLabel>
	<skos:prefLabel xml:lang="ca">pintura</skos:prefLabel>
	<skos:altLabel xml:lang="de">Malerei</skos:altLabel>
	<skos:prefLabel xml:lang="de">Gemälde</skos:prefLabel>
	<skos:prefLabel xml:lang="fr">peinture</skos:prefLabel>
	<skos:prefLabel xml:lang="hu">festmény</skos:prefLabel>
	<skos:prefLabel xml:lang="no">maleri</skos:prefLabel>
	<skos:prefLabel xml:lang="hr">slikarstvo</skos:prefLabel>
	<skos:inScheme rdf:resource="http://partage.vocnet.org/Objects"/>
	<skos:narrower rdf:resource="http://partage.vocnet.org/part00249"/>
	<skos:narrower rdf:resource="http://partage.vocnet.org/part00470"/>
	<skos:narrower rdf:resource="http://partage.vocnet.org/part00501"/>
	<skos:narrower rdf:resource="http://partage.vocnet.org/part00510"/>
	<skos:narrower rdf:resource="http://partage.vocnet.org/part00814"/>
	<skos:exactMatch rdf:resource="http://vocab.getty.edu/aat/300033618"/>
	<skos:editorialNote xml:lang="en">PPObjectType</skos:editorialNote>
	<skos:scopeNote xml:lang="en">Unique works in which images are formed primarily by the direct application of pigments suspended in oil, water, egg yolk, molten wax, or other liquid, arranged in masses of color, onto a generally two-dimensional surface.</skos:scopeNote>
</skos:Concept>
<skos:Concept rdf:about="http://partage.vocnet.org/part00045">
	<skos:prefLabel xml:lang="en">needlework (visual works)</skos:prefLabel>
	<skos:inScheme rdf:resource="http://partage.vocnet.org/Objects"/>
	<skos:narrower rdf:resource="http://partage.vocnet.org/part00221"/>
	<skos:narrower rdf:resource="http://partage.vocnet.org/part00222"/>
	<skos:exactMatch rdf:resource="http://vocab.getty.edu/aat/300264072"/>
	<skos:scopeNote xml:lang="en">Refers to works done with one or more needles and thread, yarn or cord. The term generally refers to work done by hand. Needlework includes sewing, embroidery, knitting, and other works. Until the 20th century "plain sewing" was the most widely practiced form of needlework in Western cultures. Most females learned basic sewing and knitting, which was used in the construction of clothing and the finishing of household textiles. With the introduction of machine sewing, needlework done by hand was often limited to decorative work.</skos:scopeNote>
</skos:Concept>
<skos:Concept rdf:about="http://partage.vocnet.org/part00046">
	<skos:altLabel xml:lang="en">mosaics (visual works)</skos:altLabel>
	<skos:prefLabel xml:lang="en">mosaics</skos:prefLabel>
	<skos:prefLabel xml:lang="sv">mosaiker</skos:prefLabel>
	<skos:prefLabel xml:lang="fi">mosaiikit</skos:prefLabel>
	<skos:prefLabel xml:lang="es">mosaicos</skos:prefLabel>
	<skos:prefLabel xml:lang="sl">mozaiki</skos:prefLabel>
	<skos:prefLabel xml:lang="pt">mosaico</skos:prefLabel>
	<skos:prefLabel xml:lang="pl">mozaiki</skos:prefLabel>
	<skos:prefLabel xml:lang="nl">mozaïeken</skos:prefLabel>
	<skos:prefLabel xml:lang="it">mosaici</skos:prefLabel>
	<skos:prefLabel xml:lang="cs">mozaika</skos:prefLabel>
	<skos:prefLabel xml:lang="ca">mosaics</skos:prefLabel>
	<skos:prefLabel xml:lang="de">Mosaik</skos:prefLabel>
	<skos:prefLabel xml:lang="hr">mozaici</skos:prefLabel>
	<skos:prefLabel xml:lang="no">mosaikk</skos:prefLabel>
	<skos:prefLabel xml:lang="hu">mozaik</skos:prefLabel>
	<skos:prefLabel xml:lang="fr">mosaïque</skos:prefLabel>
	<skos:inScheme rdf:resource="http://partage.vocnet.org/Objects"/>
	<skos:exactMatch rdf:resource="http://vocab.getty.edu/aat/300015342"/>
	<skos:editorialNote xml:lang="en">PPObjectType</skos:editorialNote>
	<skos:scopeNote xml:lang="en">Images or patterns composed of small, regularly shaped pieces of durable material, usually stone or colored glass. Distinguished from "opus sectile" which is composed of individually shaped pieces of durable material, usually stone or glass, which conform to the design or pattern.</skos:scopeNote>
</skos:Concept>
<skos:Concept rdf:about="http://partage.vocnet.org/part00047">
	<skos:altLabel xml:lang="en">drawings (visual works)</skos:altLabel>
	<skos:prefLabel xml:lang="en">drawings</skos:prefLabel>
	<skos:altLabel xml:lang="de">Zeichnungen</skos:altLabel>
	<skos:prefLabel xml:lang="de">Zeichnung</skos:prefLabel>
	<skos:prefLabel xml:lang="sv">teckningar</skos:prefLabel>
	<skos:prefLabel xml:lang="fi">piirustukset</skos:prefLabel>
	<skos:prefLabel xml:lang="es">dibujo</skos:prefLabel>
	<skos:prefLabel xml:lang="sl">risbe</skos:prefLabel>
	<skos:altLabel xml:lang="pt">desenhos</skos:altLabel>
	<skos:prefLabel xml:lang="pt">desenho</skos:prefLabel>
	<skos:prefLabel xml:lang="pl">rysunki</skos:prefLabel>
	<skos:prefLabel xml:lang="nl">tekeningen</skos:prefLabel>
	<skos:prefLabel xml:lang="it">disegni</skos:prefLabel>
	<skos:prefLabel xml:lang="cs">kresba</skos:prefLabel>
	<skos:prefLabel xml:lang="ca">dibuix</skos:prefLabel>
	<skos:altLabel xml:lang="de">Handzeichnungen</skos:altLabel>
	<skos:prefLabel xml:lang="fr">dessin</skos:prefLabel>
	<skos:prefLabel xml:lang="hu">rajz</skos:prefLabel>
	<skos:prefLabel xml:lang="no">tegninger</skos:prefLabel>
	<skos:prefLabel xml:lang="hr">crteži</skos:prefLabel>
	<skos:inScheme rdf:resource="http://partage.vocnet.org/Objects"/>
	<skos:narrower rdf:resource="http://partage.vocnet.org/part00415"/>
	<skos:narrower rdf:resource="http://partage.vocnet.org/part00560"/>
	<skos:narrower rdf:resource="http://partage.vocnet.org/part00948"/>
	<skos:exactMatch rdf:resource="http://vocab.getty.edu/aat/300033973"/>
	<skos:editorialNote xml:lang="en">PPObjectType</skos:editorialNote>
	<skos:scopeNote xml:lang="en">Visual works produced by drawing, which is the application of lines on a surface, often paper, by using a pencil, pen, chalk, or some other tracing instrument to focus on the delineation of form rather than the application of color. This term is often defined broadly to refer to computer-generated images as well.</skos:scopeNote>
</skos:Concept>
<skos:Concept rdf:about="http://partage.vocnet.org/part00048">
	<skos:altLabel xml:lang="en">calligraphy (visual works)</skos:altLabel>
	<skos:prefLabel xml:lang="en">calligraphy</skos:prefLabel>
	<skos:prefLabel xml:lang="sv">kalligrafi</skos:prefLabel>
	<skos:prefLabel xml:lang="fi">kalligrafia</skos:prefLabel>
	<skos:prefLabel xml:lang="es">caligrafía</skos:prefLabel>
	<skos:prefLabel xml:lang="sl">kaligrafija</skos:prefLabel>
	<skos:prefLabel xml:lang="pt">caligrafia</skos:prefLabel>
	<skos:prefLabel xml:lang="pl">kaligrafia</skos:prefLabel>
	<skos:prefLabel xml:lang="nl">kalligrafie</skos:prefLabel>
	<skos:altLabel xml:lang="it">carattere</skos:altLabel>
	<skos:prefLabel xml:lang="it">calligrafia</skos:prefLabel>
	<skos:prefLabel xml:lang="cs">kaligrafie</skos:prefLabel>
	<skos:prefLabel xml:lang="ca">cal·ligrafia</skos:prefLabel>
	<skos:prefLabel xml:lang="de">Kalligraphie</skos:prefLabel>
	<skos:altLabel xml:lang="de">Kalligrafie</skos:altLabel>
	<skos:prefLabel xml:lang="hr">kaligrafija</skos:prefLabel>
	<skos:prefLabel xml:lang="no">kalligrafi</skos:prefLabel>
	<skos:prefLabel xml:lang="hu">kalligráfia</skos:prefLabel>
	<skos:prefLabel xml:lang="fr">calligraphie</skos:prefLabel>
	<skos:inScheme rdf:resource="http://partage.vocnet.org/Objects"/>
	<skos:exactMatch rdf:resource="http://vocab.getty.edu/aat/300266660"/>
	<skos:editorialNote xml:lang="en">PPObjectType</skos:editorialNote>
	<skos:scopeNote xml:lang="en">Works composed primarily of beautiful, elegant letters or flourishes that are typically created by hand with a pen, either in unjoined characters or in cursive writing. May also refer to similar works created by computer or another means.</skos:scopeNote>
</skos:Concept>
<skos:Concept rdf:about="http://partage.vocnet.org/part00052">
	<skos:altLabel xml:lang="en">studies (visual works)</skos:altLabel>
	<skos:prefLabel xml:lang="en">studies</skos:prefLabel>
	<skos:prefLabel xml:lang="sv">studier</skos:prefLabel>
	<skos:prefLabel xml:lang="fi">harjoitelmat</skos:prefLabel>
	<skos:prefLabel xml:lang="es">estudios</skos:prefLabel>
	<skos:prefLabel xml:lang="sl">študije</skos:prefLabel>
	<skos:prefLabel xml:lang="pt">estudos</skos:prefLabel>
	<skos:prefLabel xml:lang="pl">studia</skos:prefLabel>
	<skos:prefLabel xml:lang="nl">studies</skos:prefLabel>
	<skos:prefLabel xml:lang="it">studi</skos:prefLabel>
	<skos:prefLabel xml:lang="cs">studie</skos:prefLabel>
	<skos:prefLabel xml:lang="ca">estudis</skos:prefLabel>
	<skos:prefLabel xml:lang="de">Studien</skos:prefLabel>
	<skos:prefLabel xml:lang="hr">studije</skos:prefLabel>
	<skos:prefLabel xml:lang="fr">étude</skos:prefLabel>
	<skos:prefLabel xml:lang="hu">tanulmányrajz</skos:prefLabel>
	<skos:prefLabel xml:lang="no">studie</skos:prefLabel>
	<skos:inScheme rdf:resource="http://partage.vocnet.org/Objects"/>
	<skos:exactMatch rdf:resource="http://vocab.getty.edu/aat/300081053"/>
	<skos:editorialNote xml:lang="en">PPObjectType</skos:editorialNote>
	<skos:scopeNote xml:lang="en">Works in any medium of the visual arts that explore a subject or are preliminary to a separate, more finalized work; more finished than sketches. For representations or diagrams that clarify, usually accompanying a text, use "illustrations."</skos:scopeNote>
</skos:Concept>
<skos:Concept rdf:about="http://partage.vocnet.org/part00053">
	<skos:prefLabel xml:lang="en">pendants (companion pieces)</skos:prefLabel>
	<skos:prefLabel xml:lang="hr">pandan</skos:prefLabel>
	<skos:altLabel xml:lang="de">Pendant</skos:altLabel>
	<skos:prefLabel xml:lang="de">Pendants</skos:prefLabel>
	<skos:prefLabel xml:lang="sv">pendanger (tillhörande delar)</skos:prefLabel>
	<skos:prefLabel xml:lang="pt">pendentes</skos:prefLabel>
	<skos:prefLabel xml:lang="fi">pari (taideteos)</skos:prefLabel>
	<skos:inScheme rdf:resource="http://partage.vocnet.org/Objects"/>
	<skos:exactMatch rdf:resource="http://vocab.getty.edu/aat/300179422"/>
	<skos:editorialNote xml:lang="en">PPRefiningObjectType</skos:editorialNote>
	<skos:scopeNote xml:lang="en">Pairs of works of art that were designed, or purposefully chosen, to be displayed together</skos:scopeNote>
</skos:Concept>
<skos:Concept rdf:about="http://partage.vocnet.org/part00055">
	<skos:prefLabel xml:lang="en">tapestries</skos:prefLabel>
	<skos:prefLabel xml:lang="sv">vävar</skos:prefLabel>
	<skos:prefLabel xml:lang="fi">seinätekstiilit</skos:prefLabel>
	<skos:altLabel xml:lang="es">tapiz de Arras</skos:altLabel>
	<skos:prefLabel xml:lang="es">tapices</skos:prefLabel>
	<skos:prefLabel xml:lang="sl">tapiserije</skos:prefLabel>
	<skos:prefLabel xml:lang="pt">tapeçaria</skos:prefLabel>
	<skos:prefLabel xml:lang="pl">tkaniny dekoracyjne</skos:prefLabel>
	<skos:prefLabel xml:lang="nl">tapisserieën</skos:prefLabel>
	<skos:prefLabel xml:lang="it">tappezzerie</skos:prefLabel>
	<skos:prefLabel xml:lang="cs">tapiserie</skos:prefLabel>
	<skos:prefLabel xml:lang="ca">tapissos</skos:prefLabel>
	<skos:prefLabel xml:lang="de">Tapisserie</skos:prefLabel>
	<skos:prefLabel xml:lang="hr">tapiserije</skos:prefLabel>
	<skos:prefLabel xml:lang="no">veggtepper</skos:prefLabel>
	<skos:prefLabel xml:lang="hu">szőnyeg</skos:prefLabel>
	<skos:prefLabel xml:lang="fr">tapisserie</skos:prefLabel>
	<skos:inScheme rdf:resource="http://partage.vocnet.org/Objects"/>
	<skos:broader rdf:resource="http://partage.vocnet.org/part00104"/>
	<skos:exactMatch rdf:resource="http://vocab.getty.edu/aat/300205002"/>
	<skos:editorialNote xml:lang="en">PPObjectType</skos:editorialNote>
	<skos:scopeNote xml:lang="en">Heavy, woven textiles used as wall hangings, curtains, upholstery, or to hang from windows or balconies. Tapestries are characterized by decoration that may include ornamental or pictorial subjects; they often have details that are painted or embroidered. They are usually of wool and hand-woven on a tapestry loom by a process that differs from cloth-weaving in that the weft travels only to the warp at the edge of a particular color or pattern in the design, rather traveling from edge to edge of the entire piece of fabric. Various techniques are used in mixing and overlaying colors to create shading and patterns. The term also refers to machine-woven imitations of hand-made hangings.</skos:scopeNote>
</skos:Concept>
<skos:Concept rdf:about="http://partage.vocnet.org/part00056">
	<skos:prefLabel xml:lang="en">medals</skos:prefLabel>
	<skos:prefLabel xml:lang="de">Medaillen</skos:prefLabel>
	<skos:altLabel xml:lang="de">Medaille</skos:altLabel>
	<skos:prefLabel xml:lang="sv">medaljer</skos:prefLabel>
	<skos:prefLabel xml:lang="fi">mitalit</skos:prefLabel>
	<skos:prefLabel xml:lang="es">medallas</skos:prefLabel>
	<skos:prefLabel xml:lang="sl">medalje</skos:prefLabel>
	<skos:altLabel xml:lang="pt">medalhas</skos:altLabel>
	<skos:prefLabel xml:lang="pt">medalha</skos:prefLabel>
	<skos:prefLabel xml:lang="pl">medale</skos:prefLabel>
	<skos:prefLabel xml:lang="nl">medailles</skos:prefLabel>
	<skos:prefLabel xml:lang="it">medaglie</skos:prefLabel>
	<skos:prefLabel xml:lang="cs">medaile</skos:prefLabel>
	<skos:prefLabel xml:lang="ca">medalles</skos:prefLabel>
	<skos:prefLabel xml:lang="hr">medalje</skos:prefLabel>
	<skos:prefLabel xml:lang="no">medaljer</skos:prefLabel>
	<skos:prefLabel xml:lang="hu">medál</skos:prefLabel>
	<skos:prefLabel xml:lang="fr">médaille</skos:prefLabel>
	<skos:inScheme rdf:resource="http://partage.vocnet.org/Objects"/>
	<skos:exactMatch rdf:resource="http://vocab.getty.edu/aat/300046025"/>
	<skos:editorialNote xml:lang="en">PPObjectType</skos:editorialNote>
	<skos:scopeNote xml:lang="en">Small pieces of metal, usually gold, silver, or bronze, bearing a relief design on one or both sides and having a commemorative purpose; not used as a medium of exchange.</skos:scopeNote>
</skos:Concept>
<skos:Concept rdf:about="http://partage.vocnet.org/part00059">
	<skos:prefLabel xml:lang="en">lacquerware</skos:prefLabel>
	<skos:prefLabel xml:lang="sv">lackarbete</skos:prefLabel>
	<skos:prefLabel xml:lang="fi">lakkatyöt</skos:prefLabel>
	<skos:altLabel xml:lang="es">obra de laca</skos:altLabel>
	<skos:prefLabel xml:lang="es">lacados</skos:prefLabel>
	<skos:altLabel xml:lang="sl">lak</skos:altLabel>
	<skos:prefLabel xml:lang="sl">lakirani izdelki</skos:prefLabel>
	<skos:prefLabel xml:lang="pt">objetos de laca</skos:prefLabel>
	<skos:prefLabel xml:lang="pl">wyroby z laki</skos:prefLabel>
	<skos:prefLabel xml:lang="nl">lakwerk</skos:prefLabel>
	<skos:prefLabel xml:lang="it">lacche</skos:prefLabel>
	<skos:prefLabel xml:lang="cs">lakované předměty</skos:prefLabel>
	<skos:prefLabel xml:lang="ca">lacats</skos:prefLabel>
	<skos:altLabel xml:lang="de">Lackkunst</skos:altLabel>
	<skos:prefLabel xml:lang="de">Lacke</skos:prefLabel>
	<skos:prefLabel xml:lang="hr">lakirani predmeti</skos:prefLabel>
	<skos:prefLabel xml:lang="no">lakkarbeid</skos:prefLabel>
	<skos:prefLabel xml:lang="hu">lakkbútor</skos:prefLabel>
	<skos:prefLabel xml:lang="fr">laque</skos:prefLabel>
	<skos:inScheme rdf:resource="http://partage.vocnet.org/Objects"/>
	<skos:exactMatch rdf:resource="http://vocab.getty.edu/aat/300264021"/>
	<skos:editorialNote xml:lang="en">PPObjectType</skos:editorialNote>
	<skos:scopeNote xml:lang="en">Objects, usually made of thin wood, that are coated and decorated with layers of lacquer, often accompanied by inlays of other substances such as mother-of-pearl and metal.</skos:scopeNote>
</skos:Concept>
<skos:Concept rdf:about="http://partage.vocnet.org/part00060">
	<skos:prefLabel xml:lang="en">woodwork</skos:prefLabel>
	<skos:prefLabel xml:lang="nl">houtwerk</skos:prefLabel>
	<skos:prefLabel xml:lang="it">oggetti di legno lavorato</skos:prefLabel>
	<skos:prefLabel xml:lang="cs">práce ze dřeva</skos:prefLabel>
	<skos:prefLabel xml:lang="ca">obra en fusta</skos:prefLabel>
	<skos:altLabel xml:lang="de">Tischlerarbeit</skos:altLabel>
	<skos:prefLabel xml:lang="de">Holzarbeiten</skos:prefLabel>
	<skos:prefLabel xml:lang="sv">snickerier</skos:prefLabel>
	<skos:prefLabel xml:lang="fi">puutyöt</skos:prefLabel>
	<skos:altLabel xml:lang="es">objeto de madera</skos:altLabel>
	<skos:prefLabel xml:lang="es">obra en madera</skos:prefLabel>
	<skos:prefLabel xml:lang="sl">leseni izdelki</skos:prefLabel>
	<skos:prefLabel xml:lang="pt">carpintaria</skos:prefLabel>
	<skos:prefLabel xml:lang="pl">wyroby z drewna</skos:prefLabel>
	<skos:prefLabel xml:lang="fr">ébénisterie</skos:prefLabel>
	<skos:prefLabel xml:lang="hu">faberendezés</skos:prefLabel>
	<skos:prefLabel xml:lang="no">trearbeid</skos:prefLabel>
	<skos:prefLabel xml:lang="hr">drveni predmeti</skos:prefLabel>
	<skos:altLabel xml:lang="de">Kunsttischlerei</skos:altLabel>
	<skos:inScheme rdf:resource="http://partage.vocnet.org/Objects"/>
	<skos:exactMatch rdf:resource="http://vocab.getty.edu/aat/300015348"/>
	<skos:editorialNote xml:lang="en">PPObjectType</skos:editorialNote>
	<skos:scopeNote xml:lang="en">Interior fittings of wood, such as moldings and staircases; also any visual work done in wood, or with wooden objects or parts made of wood.</skos:scopeNote>
</skos:Concept>
<skos:Concept rdf:about="http://partage.vocnet.org/part00061">
	<skos:prefLabel xml:lang="en">textiles</skos:prefLabel>
	<skos:altLabel xml:lang="de">Textilwaren</skos:altLabel>
	<skos:altLabel xml:lang="de">Textilien</skos:altLabel>
	<skos:prefLabel xml:lang="sv">textilier</skos:prefLabel>
	<skos:prefLabel xml:lang="fi">tekstiilit</skos:prefLabel>
	<skos:prefLabel xml:lang="es">textiles</skos:prefLabel>
	<skos:prefLabel xml:lang="sl">tkanine</skos:prefLabel>
	<skos:altLabel xml:lang="pt">produto têxtil</skos:altLabel>
	<skos:prefLabel xml:lang="pt">têxtil</skos:prefLabel>
	<skos:prefLabel xml:lang="pl">tkaniny</skos:prefLabel>
	<skos:prefLabel xml:lang="nl">textilia</skos:prefLabel>
	<skos:prefLabel xml:lang="it">tessuti</skos:prefLabel>
	<skos:prefLabel xml:lang="cs">textil</skos:prefLabel>
	<skos:prefLabel xml:lang="ca">tèxtils</skos:prefLabel>
	<skos:prefLabel xml:lang="fr">textile</skos:prefLabel>
	<skos:prefLabel xml:lang="hu">textil</skos:prefLabel>
	<skos:prefLabel xml:lang="no">tekstil</skos:prefLabel>
	<skos:prefLabel xml:lang="hr">tekstilni predmeti</skos:prefLabel>
	<skos:prefLabel xml:lang="de">Textilkunst</skos:prefLabel>
	<skos:inScheme rdf:resource="http://partage.vocnet.org/Objects"/>
	<skos:exactMatch rdf:resource="http://vocab.getty.edu/aat/300014063"/>
	<skos:editorialNote xml:lang="en">PPObjectType</skos:editorialNote>
	<skos:scopeNote xml:lang="en">Refers collectively to items made of textile materials. For the general category of these materials, see "textile materials."</skos:scopeNote>
</skos:Concept>
<skos:Concept rdf:about="http://partage.vocnet.org/part00062">
	<skos:prefLabel xml:lang="en">metalwork</skos:prefLabel>
	<skos:prefLabel xml:lang="nl">metaalwerk</skos:prefLabel>
	<skos:prefLabel xml:lang="it">metalli lavorati</skos:prefLabel>
	<skos:prefLabel xml:lang="cs">práce v kovu</skos:prefLabel>
	<skos:prefLabel xml:lang="ca">obra de metal·listeria</skos:prefLabel>
	<skos:altLabel xml:lang="de">Metallwaren</skos:altLabel>
	<skos:prefLabel xml:lang="de">Metallarbeiten</skos:prefLabel>
	<skos:prefLabel xml:lang="sv">metallarbeten</skos:prefLabel>
	<skos:prefLabel xml:lang="fi">metallityöt</skos:prefLabel>
	<skos:altLabel xml:lang="es">obra de metal</skos:altLabel>
	<skos:prefLabel xml:lang="es">obra de metalistería</skos:prefLabel>
	<skos:prefLabel xml:lang="sl">kovinski izdelki</skos:prefLabel>
	<skos:prefLabel xml:lang="pt">objeto em metal</skos:prefLabel>
	<skos:prefLabel xml:lang="pl">wyroby z metalu</skos:prefLabel>
	<skos:prefLabel xml:lang="fr">œuvre d'art en métal</skos:prefLabel>
	<skos:prefLabel xml:lang="hu">ötvösség</skos:prefLabel>
	<skos:prefLabel xml:lang="no">metallarbeid</skos:prefLabel>
	<skos:prefLabel xml:lang="hr">metalni predmeti</skos:prefLabel>
	<skos:inScheme rdf:resource="http://partage.vocnet.org/Objects"/>
	<skos:exactMatch rdf:resource="http://vocab.getty.edu/aat/300015336"/>
	<skos:editorialNote xml:lang="en">PPObjectType</skos:editorialNote>
	<skos:scopeNote xml:lang="en">Refers to the products of metalworking, particularly metal objects of artistic merit.</skos:scopeNote>
</skos:Concept>
<skos:Concept rdf:about="http://partage.vocnet.org/part00063">
	<skos:prefLabel xml:lang="en">glassware</skos:prefLabel>
	<skos:prefLabel xml:lang="de">Glas</skos:prefLabel>
	<skos:prefLabel xml:lang="sv">glasservis</skos:prefLabel>
	<skos:prefLabel xml:lang="fi">lasiesineet</skos:prefLabel>
	<skos:prefLabel xml:lang="es">cristalería</skos:prefLabel>
	<skos:prefLabel xml:lang="sl">stekleno posodje</skos:prefLabel>
	<skos:prefLabel xml:lang="pt">objetos de vidro</skos:prefLabel>
	<skos:prefLabel xml:lang="pl">szkło</skos:prefLabel>
	<skos:prefLabel xml:lang="nl">glaswerk</skos:prefLabel>
	<skos:prefLabel xml:lang="it">oggetti di vetro</skos:prefLabel>
	<skos:prefLabel xml:lang="cs">sklo</skos:prefLabel>
	<skos:prefLabel xml:lang="ca">cristalleria</skos:prefLabel>
	<skos:prefLabel xml:lang="fr">verrerie</skos:prefLabel>
	<skos:prefLabel xml:lang="hu">üveg</skos:prefLabel>
	<skos:prefLabel xml:lang="no">glasstøy</skos:prefLabel>
	<skos:prefLabel xml:lang="hr">stakleni predmeti</skos:prefLabel>
	<skos:inScheme rdf:resource="http://partage.vocnet.org/Objects"/>
	<skos:exactMatch rdf:resource="http://vocab.getty.edu/aat/300010898"/>
	<skos:editorialNote xml:lang="en">PPObjectType</skos:editorialNote>
	<skos:scopeNote xml:lang="de">Articles made of glass; especially tableware of glass used in serving food and drink.</skos:scopeNote>
</skos:Concept>
<skos:Concept rdf:about="http://partage.vocnet.org/part00064">
	<skos:altLabel xml:lang="en">ceramics (objects)</skos:altLabel>
	<skos:prefLabel xml:lang="en">ceramics</skos:prefLabel>
	<skos:prefLabel xml:lang="de">Keramik</skos:prefLabel>
	<skos:prefLabel xml:lang="sv">keramik</skos:prefLabel>
	<skos:prefLabel xml:lang="fi">keramiikka</skos:prefLabel>
	<skos:prefLabel xml:lang="es">cerámica</skos:prefLabel>
	<skos:prefLabel xml:lang="sl">keramika</skos:prefLabel>
	<skos:prefLabel xml:lang="pt">cerâmica</skos:prefLabel>
	<skos:prefLabel xml:lang="pl">ceramika</skos:prefLabel>
	<skos:prefLabel xml:lang="nl">keramiek</skos:prefLabel>
	<skos:prefLabel xml:lang="it">ceramica</skos:prefLabel>
	<skos:prefLabel xml:lang="cs">keramika</skos:prefLabel>
	<skos:prefLabel xml:lang="ca">ceràmica</skos:prefLabel>
	<skos:prefLabel xml:lang="fr">céramique</skos:prefLabel>
	<skos:prefLabel xml:lang="hu">kerámia</skos:prefLabel>
	<skos:prefLabel xml:lang="no">keramikk</skos:prefLabel>
	<skos:prefLabel xml:lang="hr">keramika</skos:prefLabel>
	<skos:inScheme rdf:resource="http://partage.vocnet.org/Objects"/>
	<skos:narrower rdf:resource="http://partage.vocnet.org/part00224"/>
	<skos:exactMatch rdf:resource="http://vocab.getty.edu/aat/300151343"/>
	<skos:editorialNote xml:lang="en">PPObjectType</skos:editorialNote>
	<skos:scopeNote xml:lang="en">Refers in general to articles made of ceramic, which is any of various hard, brittle, heat-resistant and corrosion-resistant materials made by shaping and then firing a nonmetallic mineral, such as clay, at a high temperature. Earthenware, porcelain, and brick products are examples of ceramics.</skos:scopeNote>
</skos:Concept>
<skos:Concept rdf:about="http://partage.vocnet.org/part00066">
	<skos:prefLabel xml:lang="en">posters</skos:prefLabel>
	<skos:prefLabel xml:lang="sv">affischer</skos:prefLabel>
	<skos:prefLabel xml:lang="fi">julisteet</skos:prefLabel>
	<skos:prefLabel xml:lang="es">carteles</skos:prefLabel>
	<skos:prefLabel xml:lang="sl">plakati</skos:prefLabel>
	<skos:altLabel xml:lang="pt">posters</skos:altLabel>
	<skos:prefLabel xml:lang="pt">poster</skos:prefLabel>
	<skos:prefLabel xml:lang="pl">plakaty</skos:prefLabel>
	<skos:prefLabel xml:lang="nl">posters</skos:prefLabel>
	<skos:prefLabel xml:lang="it">manifesti</skos:prefLabel>
	<skos:prefLabel xml:lang="cs">plakát</skos:prefLabel>
	<skos:prefLabel xml:lang="ca">cartells</skos:prefLabel>
	<skos:altLabel xml:lang="de">Plakat</skos:altLabel>
	<skos:prefLabel xml:lang="de">Plakate</skos:prefLabel>
	<skos:prefLabel xml:lang="fr">affiche</skos:prefLabel>
	<skos:prefLabel xml:lang="hu">plakát</skos:prefLabel>
	<skos:prefLabel xml:lang="no">plakat</skos:prefLabel>
	<skos:prefLabel xml:lang="hr">plakati</skos:prefLabel>
	<skos:inScheme rdf:resource="http://partage.vocnet.org/Objects"/>
	<skos:exactMatch rdf:resource="http://vocab.getty.edu/aat/300027221"/>
	<skos:editorialNote xml:lang="en">PPObjectType</skos:editorialNote>
	<skos:scopeNote xml:lang="en">Notices, usually decorative or pictorial, intended to be posted to advertise, promote, or publicize an activity, cause, product, or service; also, decorative, mass-produced prints intended for hanging. For small printed notices or advertisements intended for distribution by hand, use "handbills."</skos:scopeNote>
</skos:Concept>
<skos:Concept rdf:about="http://partage.vocnet.org/part00072">
	<skos:prefLabel xml:lang="en">religious buildings</skos:prefLabel>
	<skos:prefLabel xml:lang="hr">vjerski objekt</skos:prefLabel>
	<skos:prefLabel xml:lang="pt">edifícios religiosos</skos:prefLabel>
	<skos:altLabel xml:lang="de">Sakralbau</skos:altLabel>
	<skos:prefLabel xml:lang="de">Sakralbauten</skos:prefLabel>
	<skos:prefLabel xml:lang="sv">religiösa byggnader</skos:prefLabel>
	<skos:prefLabel xml:lang="fi">uskonnolliset rakennukset</skos:prefLabel>
	<skos:inScheme rdf:resource="http://partage.vocnet.org/Objects"/>
	<skos:broader rdf:resource="http://partage.vocnet.org/part00074"/>
	<skos:narrower rdf:resource="http://partage.vocnet.org/part00725"/>
	<skos:narrower rdf:resource="http://partage.vocnet.org/part00756"/>
	<skos:exactMatch rdf:resource="http://vocab.getty.edu/aat/300007391"/>
	<skos:scopeNote xml:lang="en">Buildings built or used for religious ceremonies or other functions having to do with a particular religion.</skos:scopeNote>
	<skos:editorialNote xml:lang="en">PPRefiningObjectType</skos:editorialNote>
</skos:Concept>
<skos:Concept rdf:about="http://partage.vocnet.org/part00074">
	<skos:prefLabel xml:lang="en">ceremonial structures</skos:prefLabel>
	<skos:inScheme rdf:resource="http://partage.vocnet.org/Objects"/>
	<skos:narrower rdf:resource="http://partage.vocnet.org/part00072"/>
	<skos:narrower rdf:resource="http://partage.vocnet.org/part00153"/>
	<skos:narrower rdf:resource="http://partage.vocnet.org/part00166"/>
	<skos:exactMatch rdf:resource="http://vocab.getty.edu/aat/300263489"/>
	<skos:scopeNote xml:lang="en">Structures built or used primarily or exculsively for ceremonies or related activities.</skos:scopeNote>
</skos:Concept>
<skos:Concept rdf:about="http://partage.vocnet.org/part00075">
	<skos:prefLabel xml:lang="en">dwellings</skos:prefLabel>
	<skos:altLabel xml:lang="pt">residência</skos:altLabel>
	<skos:prefLabel xml:lang="pt">habitação</skos:prefLabel>
	<skos:altLabel xml:lang="de">Wohnhaus</skos:altLabel>
	<skos:prefLabel xml:lang="de">Wohngebäude</skos:prefLabel>
	<skos:prefLabel xml:lang="sv">bostäder</skos:prefLabel>
	<skos:prefLabel xml:lang="hr">prebivalište</skos:prefLabel>
	<skos:prefLabel xml:lang="fi">asunnot</skos:prefLabel>
	<skos:inScheme rdf:resource="http://partage.vocnet.org/Objects"/>
	<skos:narrower rdf:resource="http://partage.vocnet.org/part00200"/>
	<skos:exactMatch rdf:resource="http://vocab.getty.edu/aat/300005425"/>
	<skos:editorialNote xml:lang="en">PPRefiningObjectType</skos:editorialNote>
	<skos:scopeNote xml:lang="en">Buildings or portions of a building designed exclusively for human residential occupancy, but not including hotels or other buildings intended for use by transients. For the locale which constitutes the center of an individual's domestic life, affectional relationships, and interests, together with the feeling of comfort and satisfaction that it conveys, use "home." For the collective concept referring to types of living arrangements of a particular group, use "housing."</skos:scopeNote>
</skos:Concept>
<skos:Concept rdf:about="http://partage.vocnet.org/part00078">
	<skos:prefLabel xml:lang="en">jewellery</skos:prefLabel>
	<skos:altLabel xml:lang="en">jewelry</skos:altLabel>
	<skos:prefLabel xml:lang="pt">joalharia</skos:prefLabel>
	<skos:prefLabel xml:lang="pl">biżuteria</skos:prefLabel>
	<skos:prefLabel xml:lang="nl">sieraden</skos:prefLabel>
	<skos:prefLabel xml:lang="it">gioielli</skos:prefLabel>
	<skos:prefLabel xml:lang="cs">šperk</skos:prefLabel>
	<skos:prefLabel xml:lang="ca">joies</skos:prefLabel>
	<skos:prefLabel xml:lang="de">Schmuck</skos:prefLabel>
	<skos:prefLabel xml:lang="sv">smycken</skos:prefLabel>
	<skos:prefLabel xml:lang="fi">korut</skos:prefLabel>
	<skos:altLabel xml:lang="es">joya</skos:altLabel>
	<skos:prefLabel xml:lang="es">joyas</skos:prefLabel>
	<skos:prefLabel xml:lang="sl">nakit</skos:prefLabel>
	<skos:altLabel xml:lang="pt">jóias</skos:altLabel>
	<skos:prefLabel xml:lang="hr">nakit</skos:prefLabel>
	<skos:prefLabel xml:lang="no">smykker</skos:prefLabel>
	<skos:prefLabel xml:lang="hu">ékszer</skos:prefLabel>
	<skos:prefLabel xml:lang="fr">bijou</skos:prefLabel>
	<skos:inScheme rdf:resource="http://partage.vocnet.org/Objects"/>
	<skos:broader rdf:resource="http://partage.vocnet.org/part00080"/>
	<skos:narrower rdf:resource="http://partage.vocnet.org/part00771"/>
	<skos:narrower rdf:resource="http://partage.vocnet.org/part00772"/>
	<skos:narrower rdf:resource="http://partage.vocnet.org/part00773"/>
	<skos:narrower rdf:resource="http://partage.vocnet.org/part00774"/>
	<skos:narrower rdf:resource="http://partage.vocnet.org/part00775"/>
	<skos:narrower rdf:resource="http://partage.vocnet.org/part00776"/>
	<skos:narrower rdf:resource="http://partage.vocnet.org/part00779"/>
	<skos:narrower rdf:resource="http://partage.vocnet.org/part00783"/>
	<skos:narrower rdf:resource="http://partage.vocnet.org/part00958"/>
	<skos:exactMatch rdf:resource="http://vocab.getty.edu/aat/300209286"/>
	<skos:editorialNote xml:lang="en">PPObjectType</skos:editorialNote>
	<skos:scopeNote xml:lang="en">Ornaments such as bracelets, necklaces, and rings, of precious or semiprecious materials worn or carried on the person for adornment; also includes similar articles worn or carried for devotional or mourning purposes.</skos:scopeNote>
</skos:Concept>
<skos:Concept rdf:about="http://partage.vocnet.org/part00080">
	<skos:prefLabel xml:lang="en">costume accessories</skos:prefLabel>
	<skos:prefLabel xml:lang="pt">acessórios</skos:prefLabel>
	<skos:prefLabel xml:lang="de">Accessoires</skos:prefLabel>
	<skos:altLabel xml:lang="de">Mode-Accessoires</skos:altLabel>
	<skos:altLabel xml:lang="de">Bekleidungszubehör</skos:altLabel>
	<skos:altLabel xml:lang="de">Mode-Accessoir</skos:altLabel>
	<skos:prefLabel xml:lang="sv">accessoarer</skos:prefLabel>
	<skos:prefLabel xml:lang="hr">modni dodaci</skos:prefLabel>
	<skos:prefLabel xml:lang="fi">asusteet</skos:prefLabel>
	<skos:inScheme rdf:resource="http://partage.vocnet.org/Objects"/>
	<skos:broader rdf:resource="http://partage.vocnet.org/part00081"/>
	<skos:narrower rdf:resource="http://partage.vocnet.org/part00078"/>
	<skos:narrower rdf:resource="http://partage.vocnet.org/part00704"/>
	<skos:narrower rdf:resource="http://partage.vocnet.org/part00705"/>
	<skos:narrower rdf:resource="http://partage.vocnet.org/part00706"/>
	<skos:narrower rdf:resource="http://partage.vocnet.org/part00708"/>
	<skos:narrower rdf:resource="http://partage.vocnet.org/part00713"/>
	<skos:narrower rdf:resource="http://partage.vocnet.org/part00714"/>
	<skos:narrower rdf:resource="http://partage.vocnet.org/part00716"/>
	<skos:narrower rdf:resource="http://partage.vocnet.org/part00719"/>
	<skos:narrower rdf:resource="http://partage.vocnet.org/part00722"/>
	<skos:narrower rdf:resource="http://partage.vocnet.org/part00955"/>
	<skos:narrower rdf:resource="http://partage.vocnet.org/part00965"/>
	<skos:narrower rdf:resource="http://partage.vocnet.org/part00974"/>
	<skos:narrower rdf:resource="http://partage.vocnet.org/part01180"/>
	<skos:exactMatch rdf:resource="http://vocab.getty.edu/aat/300209273"/>
	<skos:editorialNote xml:lang="en">PPRefiningObjectType</skos:editorialNote>
	<skos:scopeNote xml:lang="en">Items that do not form the primary articles of clothing, but are instead the smaller articles of dress, such as shoes, gloves, hats, jewelry, etc.</skos:scopeNote>
</skos:Concept>
<skos:Concept rdf:about="http://partage.vocnet.org/part00081">
	<skos:altLabel xml:lang="en">costume (mode of fashion)</skos:altLabel>
	<skos:prefLabel xml:lang="en">costume</skos:prefLabel>
	<skos:altLabel xml:lang="de">Kleidung</skos:altLabel>
	<skos:prefLabel xml:lang="de">Mode</skos:prefLabel>
	<skos:prefLabel xml:lang="sv">dräkt</skos:prefLabel>
	<skos:prefLabel xml:lang="fi">asut</skos:prefLabel>
	<skos:prefLabel xml:lang="es">indumentaria</skos:prefLabel>
	<skos:prefLabel xml:lang="sl">noše</skos:prefLabel>
	<skos:prefLabel xml:lang="pt">traje</skos:prefLabel>
	<skos:prefLabel xml:lang="pl">akcesoria mody</skos:prefLabel>
	<skos:prefLabel xml:lang="nl">kleding</skos:prefLabel>
	<skos:prefLabel xml:lang="it">moda</skos:prefLabel>
	<skos:prefLabel xml:lang="cs">móda</skos:prefLabel>
	<skos:prefLabel xml:lang="ca">indumentària</skos:prefLabel>
	<skos:prefLabel xml:lang="hr">odjeća</skos:prefLabel>
	<skos:prefLabel xml:lang="no">drakt</skos:prefLabel>
	<skos:prefLabel xml:lang="hu">viselet</skos:prefLabel>
	<skos:prefLabel xml:lang="fr">costume</skos:prefLabel>
	<skos:inScheme rdf:resource="http://partage.vocnet.org/Objects"/>
	<skos:narrower rdf:resource="http://partage.vocnet.org/part00080"/>
	<skos:narrower rdf:resource="http://partage.vocnet.org/part00213"/>
	<skos:narrower rdf:resource="http://partage.vocnet.org/part00699"/>
	<skos:narrower rdf:resource="http://partage.vocnet.org/part00700"/>
	<skos:narrower rdf:resource="http://partage.vocnet.org/part00701"/>
	<skos:narrower rdf:resource="http://partage.vocnet.org/part00851"/>
	<skos:narrower rdf:resource="http://partage.vocnet.org/part01135"/>
	<skos:exactMatch rdf:resource="http://vocab.getty.edu/aat/300178802"/>
	<skos:editorialNote xml:lang="en">PPObjectType</skos:editorialNote>
	<skos:scopeNote xml:lang="en">The mode or fashion of personal attire and dress, including the way of wearing the hair, style of clothing, jewelry, crowns, scepters, and other accessories of personal adornment, belonging to a particular nation, class, period, or special occasion, including all items worn or carried by people for warmth, protection, embellishment, or symbolic purposes. In English, generally expressed in the singular.</skos:scopeNote>
</skos:Concept>
<skos:Concept rdf:about="http://partage.vocnet.org/part00083">
	<skos:prefLabel xml:lang="en">vessels (containers)</skos:prefLabel>
	<skos:prefLabel xml:lang="sv">behållare.</skos:prefLabel>
	<skos:prefLabel xml:lang="hr">posuđe</skos:prefLabel>
	<skos:altLabel xml:lang="pt">vasilha</skos:altLabel>
	<skos:prefLabel xml:lang="pt">recipiente</skos:prefLabel>
	<skos:altLabel xml:lang="de">Gefäß</skos:altLabel>
	<skos:prefLabel xml:lang="de">Gefäße</skos:prefLabel>
	<skos:prefLabel xml:lang="fi">astiat.</skos:prefLabel>
	<skos:inScheme rdf:resource="http://partage.vocnet.org/Objects"/>
	<skos:broader rdf:resource="http://partage.vocnet.org/part00085"/>
	<skos:narrower rdf:resource="http://partage.vocnet.org/part00321"/>
	<skos:narrower rdf:resource="http://partage.vocnet.org/part00322"/>
	<skos:narrower rdf:resource="http://partage.vocnet.org/part00323"/>
	<skos:narrower rdf:resource="http://partage.vocnet.org/part00325"/>
	<skos:narrower rdf:resource="http://partage.vocnet.org/part00326"/>
	<skos:narrower rdf:resource="http://partage.vocnet.org/part00327"/>
	<skos:narrower rdf:resource="http://partage.vocnet.org/part00401"/>
	<skos:narrower rdf:resource="http://partage.vocnet.org/part00413"/>
	<skos:narrower rdf:resource="http://partage.vocnet.org/part00682"/>
	<skos:narrower rdf:resource="http://partage.vocnet.org/part00684"/>
	<skos:narrower rdf:resource="http://partage.vocnet.org/part00686"/>
	<skos:narrower rdf:resource="http://partage.vocnet.org/part01136"/>
	<skos:narrower rdf:resource="http://partage.vocnet.org/part01162"/>
	<skos:exactMatch rdf:resource="http://vocab.getty.edu/aat/300193015"/>
	<skos:editorialNote xml:lang="en">PPRefiningObjectType</skos:editorialNote>
	<skos:scopeNote xml:lang="en">Containers designed to serve as receptacles for a liquid or other substance, usually those of circular section and made of some durable material; especially containers of this nature in domestic use, employed in connection with the preparation or serving of food or drink, and usually of a size suitable for carrying by hand.</skos:scopeNote>
</skos:Concept>
<skos:Concept rdf:about="http://partage.vocnet.org/part00085">
	<skos:prefLabel xml:lang="en">containers (receptacles)</skos:prefLabel>
	<skos:prefLabel xml:lang="pt">recepientes</skos:prefLabel>
	<skos:prefLabel xml:lang="de">Behälter</skos:prefLabel>
	<skos:prefLabel xml:lang="sv">behållare</skos:prefLabel>
	<skos:prefLabel xml:lang="hr">spremnik.</skos:prefLabel>
	<skos:prefLabel xml:lang="fi">säilytysastiat</skos:prefLabel>
	<skos:inScheme rdf:resource="http://partage.vocnet.org/Objects"/>
	<skos:narrower rdf:resource="http://partage.vocnet.org/part00083"/>
	<skos:narrower rdf:resource="http://partage.vocnet.org/part00193"/>
	<skos:narrower rdf:resource="http://partage.vocnet.org/part00318"/>
	<skos:narrower rdf:resource="http://partage.vocnet.org/part00319"/>
	<skos:narrower rdf:resource="http://partage.vocnet.org/part00320"/>
	<skos:narrower rdf:resource="http://partage.vocnet.org/part00396"/>
	<skos:narrower rdf:resource="http://partage.vocnet.org/part00403"/>
	<skos:narrower rdf:resource="http://partage.vocnet.org/part00676"/>
	<skos:narrower rdf:resource="http://partage.vocnet.org/part00677"/>
	<skos:narrower rdf:resource="http://partage.vocnet.org/part00678"/>
	<skos:narrower rdf:resource="http://partage.vocnet.org/part00679"/>
	<skos:narrower rdf:resource="http://partage.vocnet.org/part00680"/>
	<skos:narrower rdf:resource="http://partage.vocnet.org/part00683"/>
	<skos:narrower rdf:resource="http://partage.vocnet.org/part00685"/>
	<skos:narrower rdf:resource="http://partage.vocnet.org/part00689"/>
	<skos:narrower rdf:resource="http://partage.vocnet.org/part00712"/>
	<skos:narrower rdf:resource="http://partage.vocnet.org/part00721"/>
	<skos:narrower rdf:resource="http://partage.vocnet.org/part00939"/>
	<skos:narrower rdf:resource="http://partage.vocnet.org/part01125"/>
	<skos:narrower rdf:resource="http://partage.vocnet.org/part01160"/>
	<skos:narrower rdf:resource="http://partage.vocnet.org/part01161"/>
	<skos:narrower rdf:resource="http://partage.vocnet.org/part01168"/>
	<skos:narrower rdf:resource="http://partage.vocnet.org/part01169"/>
	<skos:narrower rdf:resource="http://partage.vocnet.org/part01190"/>
	<skos:narrower rdf:resource="http://partage.vocnet.org/part01193"/>
	<skos:exactMatch rdf:resource="http://vocab.getty.edu/aat/300197197"/>
	<skos:scopeNote xml:lang="en">Receptacles or formed or flexible coverings designed to hold, store, or ship objects or substances.</skos:scopeNote>
	<skos:editorialNote xml:lang="en">PPRefiningObjectType</skos:editorialNote>
</skos:Concept>
<skos:Concept rdf:about="http://partage.vocnet.org/part00087">
	<skos:prefLabel xml:lang="en">timepieces</skos:prefLabel>
	<skos:prefLabel xml:lang="it">orologi</skos:prefLabel>
	<skos:prefLabel xml:lang="cs">hodiny a hodinky</skos:prefLabel>
	<skos:prefLabel xml:lang="ca">rellotges</skos:prefLabel>
	<skos:prefLabel xml:lang="de">Uhren</skos:prefLabel>
	<skos:prefLabel xml:lang="sv">ur</skos:prefLabel>
	<skos:prefLabel xml:lang="fi">kellot</skos:prefLabel>
	<skos:altLabel xml:lang="es">indicadores de tiempo</skos:altLabel>
	<skos:prefLabel xml:lang="es">relojes</skos:prefLabel>
	<skos:prefLabel xml:lang="sl">ure</skos:prefLabel>
	<skos:altLabel xml:lang="pt">relógios</skos:altLabel>
	<skos:prefLabel xml:lang="pt">relógio</skos:prefLabel>
	<skos:prefLabel xml:lang="pl">czasomierze</skos:prefLabel>
	<skos:prefLabel xml:lang="nl">uurwerken</skos:prefLabel>
	<skos:prefLabel xml:lang="hr">satovi</skos:prefLabel>
	<skos:prefLabel xml:lang="no">ur</skos:prefLabel>
	<skos:prefLabel xml:lang="hu">óra</skos:prefLabel>
	<skos:prefLabel xml:lang="fr">horlogerie</skos:prefLabel>
	<skos:altLabel xml:lang="de">Uhr</skos:altLabel>
	<skos:altLabel xml:lang="de">Zeitmesser</skos:altLabel>
	<skos:inScheme rdf:resource="http://partage.vocnet.org/Objects"/>
	<skos:broader rdf:resource="http://partage.vocnet.org/part00089"/>
	<skos:narrower rdf:resource="http://partage.vocnet.org/part00789"/>
	<skos:narrower rdf:resource="http://partage.vocnet.org/part00790"/>
	<skos:exactMatch rdf:resource="http://vocab.getty.edu/aat/300041573"/>
	<skos:editorialNote xml:lang="en">PPObjectType</skos:editorialNote>
	<skos:scopeNote xml:lang="de">Devices for measuring and recording the passage of time.</skos:scopeNote>
</skos:Concept>
<skos:Concept rdf:about="http://partage.vocnet.org/part00089">
	<skos:prefLabel xml:lang="en">measuring devices (instruments)</skos:prefLabel>
	<skos:inScheme rdf:resource="http://partage.vocnet.org/Objects"/>
	<skos:narrower rdf:resource="http://partage.vocnet.org/part00087"/>
	<skos:exactMatch rdf:resource="http://vocab.getty.edu/aat/300207870"/>
	<skos:scopeNote xml:lang="en">Instruments or containers that measure, for example, extent, quantity, capacity, mass, or position in terms of a standard unit or fixed amount.</skos:scopeNote>
</skos:Concept>
<skos:Concept rdf:about="http://partage.vocnet.org/part00091">
	<skos:prefLabel xml:lang="en">bookworks</skos:prefLabel>
	<skos:prefLabel xml:lang="sv">bokverk</skos:prefLabel>
	<skos:prefLabel xml:lang="pt">livros de artista</skos:prefLabel>
	<skos:altLabel xml:lang="de">Künstlerbuch</skos:altLabel>
	<skos:prefLabel xml:lang="hr">knjiga (umjetnička)</skos:prefLabel>
	<skos:prefLabel xml:lang="de">Künstlerbücher</skos:prefLabel>
	<skos:prefLabel xml:lang="fi">kirjataide</skos:prefLabel>
	<skos:inScheme rdf:resource="http://partage.vocnet.org/Objects"/>
	<skos:broader rdf:resource="http://partage.vocnet.org/part00092"/>
	<skos:exactMatch rdf:resource="http://vocab.getty.edu/aat/300178842"/>
	<skos:editorialNote xml:lang="en">PPRefiningObjectType</skos:editorialNote>
	<skos:scopeNote xml:lang="en">Artists' books that exploit the book form or alter its physical structure as part of the content of the work. Also includes works where emphasis is on the fine crafting of the book. For sculptures that look like or incorporate books but do not communicate in the ways characteristic of books, use "book objects."</skos:scopeNote>
</skos:Concept>
<skos:Concept rdf:about="http://partage.vocnet.org/part00092">
	<skos:prefLabel xml:lang="en">artists' books</skos:prefLabel>
	<skos:inScheme rdf:resource="http://partage.vocnet.org/Objects"/>
	<skos:broader rdf:resource="http://partage.vocnet.org/part00094"/>
	<skos:narrower rdf:resource="http://partage.vocnet.org/part00091"/>
	<skos:exactMatch rdf:resource="http://vocab.getty.edu/aat/300123016"/>
	<skos:scopeNote xml:lang="en">Books, whether unique items or multiples, made or conceived by artists, including commercial publications (usually in limited editions), as well as unique items formed or arranged by the artist. For texts written by artists for the sake of their informational content, use "writings." For artists' books that emphasize the physical book as a work of art rather than the content, use "bookworks." For works that look like or incorporate books but do not communicate in the ways characteristic of books, see "book objects."</skos:scopeNote>
</skos:Concept>
<skos:Concept rdf:about="http://partage.vocnet.org/part00094">
	<skos:prefLabel xml:lang="en">books</skos:prefLabel>
	<skos:prefLabel xml:lang="de">Bücher</skos:prefLabel>
	<skos:altLabel xml:lang="de">Buch</skos:altLabel>
	<skos:prefLabel xml:lang="sv">böcker</skos:prefLabel>
	<skos:prefLabel xml:lang="fi">kirjat</skos:prefLabel>
	<skos:prefLabel xml:lang="es">libros</skos:prefLabel>
	<skos:prefLabel xml:lang="sl">knjige</skos:prefLabel>
	<skos:altLabel xml:lang="pt">livros</skos:altLabel>
	<skos:prefLabel xml:lang="pt">livro</skos:prefLabel>
	<skos:prefLabel xml:lang="pl">książki</skos:prefLabel>
	<skos:prefLabel xml:lang="nl">boeken</skos:prefLabel>
	<skos:prefLabel xml:lang="it">libri</skos:prefLabel>
	<skos:prefLabel xml:lang="cs">kniha</skos:prefLabel>
	<skos:prefLabel xml:lang="ca">llibres</skos:prefLabel>
	<skos:prefLabel xml:lang="fr">livre</skos:prefLabel>
	<skos:prefLabel xml:lang="hu">könyv</skos:prefLabel>
	<skos:prefLabel xml:lang="no">bøker</skos:prefLabel>
	<skos:prefLabel xml:lang="hr">knjige</skos:prefLabel>
	<skos:inScheme rdf:resource="http://partage.vocnet.org/Objects"/>
	<skos:narrower rdf:resource="http://partage.vocnet.org/part00092"/>
	<skos:exactMatch rdf:resource="http://vocab.getty.edu/aat/300028051"/>
	<skos:editorialNote xml:lang="en">PPObjectType</skos:editorialNote>
	<skos:scopeNote xml:lang="en">Items comprising a collection of leaves of paper, parchment, wood, stiffened textile, ivory, metal tablets, or other flat material, that are blank, written on, or printed, and are strung or bound together in a volume.</skos:scopeNote>
</skos:Concept>
<skos:Concept rdf:about="http://partage.vocnet.org/part00099">
	<skos:prefLabel xml:lang="en">furniture</skos:prefLabel>
	<skos:altLabel xml:lang="de">Mobiliar</skos:altLabel>
	<skos:prefLabel xml:lang="de">Möbel</skos:prefLabel>
	<skos:prefLabel xml:lang="sv">möbler</skos:prefLabel>
	<skos:prefLabel xml:lang="fi">huonekalut</skos:prefLabel>
	<skos:prefLabel xml:lang="es">muebles</skos:prefLabel>
	<skos:prefLabel xml:lang="sl">pohištvo</skos:prefLabel>
	<skos:altLabel xml:lang="pt">mobília</skos:altLabel>
	<skos:prefLabel xml:lang="pt">mobiliário</skos:prefLabel>
	<skos:prefLabel xml:lang="pl">meble</skos:prefLabel>
	<skos:prefLabel xml:lang="nl">meubilair</skos:prefLabel>
	<skos:prefLabel xml:lang="it">mobilia</skos:prefLabel>
	<skos:prefLabel xml:lang="cs">nábytek</skos:prefLabel>
	<skos:prefLabel xml:lang="ca">mobles</skos:prefLabel>
	<skos:prefLabel xml:lang="hr">namještaj</skos:prefLabel>
	<skos:prefLabel xml:lang="no">møbler</skos:prefLabel>
	<skos:prefLabel xml:lang="hu">bútor</skos:prefLabel>
	<skos:prefLabel xml:lang="fr">mobilier</skos:prefLabel>
	<skos:inScheme rdf:resource="http://partage.vocnet.org/Objects"/>
	<skos:broader rdf:resource="http://partage.vocnet.org/part00100"/>
	<skos:narrower rdf:resource="http://partage.vocnet.org/part00102"/>
	<skos:narrower rdf:resource="http://partage.vocnet.org/part00299"/>
	<skos:narrower rdf:resource="http://partage.vocnet.org/part00306"/>
	<skos:narrower rdf:resource="http://partage.vocnet.org/part00314"/>
	<skos:narrower rdf:resource="http://partage.vocnet.org/part00316"/>
	<skos:narrower rdf:resource="http://partage.vocnet.org/part00802"/>
	<skos:narrower rdf:resource="http://partage.vocnet.org/part00810"/>
	<skos:narrower rdf:resource="http://partage.vocnet.org/part00928"/>
	<skos:exactMatch rdf:resource="http://vocab.getty.edu/aat/300037680"/>
	<skos:editorialNote xml:lang="en">PPObjectType</skos:editorialNote>
	<skos:scopeNote xml:lang="en">Movable or fixed objects or equipment, which may be either functional or ornamental, for use in a dwelling, business, or public space.</skos:scopeNote>
</skos:Concept>
<skos:Concept rdf:about="http://partage.vocnet.org/part00100">
	<skos:altLabel xml:lang="en">furnishings (artifacts)</skos:altLabel>
	<skos:prefLabel xml:lang="en">furnishings</skos:prefLabel>
	<skos:altLabel xml:lang="de">Raumausstattung</skos:altLabel>
	<skos:prefLabel xml:lang="de">Inneneinrichtung</skos:prefLabel>
	<skos:prefLabel xml:lang="sv">möblemang</skos:prefLabel>
	<skos:prefLabel xml:lang="fi">sisustus</skos:prefLabel>
	<skos:prefLabel xml:lang="es">mobiliario</skos:prefLabel>
	<skos:prefLabel xml:lang="sl">oprema</skos:prefLabel>
	<skos:prefLabel xml:lang="pt">recheio</skos:prefLabel>
	<skos:prefLabel xml:lang="pl">wyroby użytkowe</skos:prefLabel>
	<skos:prefLabel xml:lang="nl">interieurinrichting</skos:prefLabel>
	<skos:prefLabel xml:lang="it">oggetti di uso domestico</skos:prefLabel>
	<skos:prefLabel xml:lang="cs">bytové vybavení</skos:prefLabel>
	<skos:prefLabel xml:lang="ca">mobiliari</skos:prefLabel>
	<skos:prefLabel xml:lang="hu">berendezés</skos:prefLabel>
	<skos:prefLabel xml:lang="no">inventar</skos:prefLabel>
	<skos:prefLabel xml:lang="hr">oprema</skos:prefLabel>
	<skos:inScheme rdf:resource="http://partage.vocnet.org/Objects"/>
	<skos:narrower rdf:resource="http://partage.vocnet.org/part00099"/>
	<skos:narrower rdf:resource="http://partage.vocnet.org/part00104"/>
	<skos:narrower rdf:resource="http://partage.vocnet.org/part00109"/>
	<skos:narrower rdf:resource="http://partage.vocnet.org/part00110"/>
	<skos:narrower rdf:resource="http://partage.vocnet.org/part00179"/>
	<skos:narrower rdf:resource="http://partage.vocnet.org/part00180"/>
	<skos:narrower rdf:resource="http://partage.vocnet.org/part00504"/>
	<skos:narrower rdf:resource="http://partage.vocnet.org/part00794"/>
	<skos:narrower rdf:resource="http://partage.vocnet.org/part00795"/>
	<skos:narrower rdf:resource="http://partage.vocnet.org/part00809"/>
	<skos:narrower rdf:resource="http://partage.vocnet.org/part01157"/>
	<skos:narrower rdf:resource="http://partage.vocnet.org/part01164"/>
	<skos:narrower rdf:resource="http://partage.vocnet.org/part01175"/>
	<skos:narrower rdf:resource="http://partage.vocnet.org/part01185"/>
	<skos:narrower rdf:resource="http://partage.vocnet.org/part01192"/>
	<skos:exactMatch rdf:resource="http://vocab.getty.edu/aat/300037336"/>
	<skos:editorialNote xml:lang="en">PPObjectType</skos:editorialNote>
	<skos:scopeNote xml:lang="en">Artifacts originally created to facilitate human activity and to provide for physical needs of people in or around a building generally by offering comfort, convenience, or protection</skos:scopeNote>
</skos:Concept>
<skos:Concept rdf:about="http://partage.vocnet.org/part00102">
	<skos:prefLabel xml:lang="en">screens (furniture)</skos:prefLabel>
	<skos:prefLabel xml:lang="hr">zaslon.</skos:prefLabel>
	<skos:prefLabel xml:lang="pt">divisória</skos:prefLabel>
	<skos:altLabel xml:lang="pt">biombo</skos:altLabel>
	<skos:prefLabel xml:lang="de">Schirm (Raumteiler)</skos:prefLabel>
	<skos:prefLabel xml:lang="sv">skärmar (möbler)</skos:prefLabel>
	<skos:prefLabel xml:lang="fi">sermit</skos:prefLabel>
	<skos:inScheme rdf:resource="http://partage.vocnet.org/Objects"/>
	<skos:broader rdf:resource="http://partage.vocnet.org/part00099"/>
	<skos:narrower rdf:resource="http://partage.vocnet.org/part00303"/>
	<skos:narrower rdf:resource="http://partage.vocnet.org/part00304"/>
	<skos:exactMatch rdf:resource="http://vocab.getty.edu/aat/300037737"/>
	<skos:editorialNote xml:lang="en">PPRefiningObjectType</skos:editorialNote>
	<skos:scopeNote xml:lang="en">Refers to furniture in the form of an upright partition that can be used to embellish, partition, shelter, and provide privacy. Screens are often highly decorated.</skos:scopeNote>
</skos:Concept>
<skos:Concept rdf:about="http://partage.vocnet.org/part00104">
	<skos:prefLabel xml:lang="en">wall hangings</skos:prefLabel>
	<skos:inScheme rdf:resource="http://partage.vocnet.org/Objects"/>
	<skos:broader rdf:resource="http://partage.vocnet.org/part00100"/>
	<skos:narrower rdf:resource="http://partage.vocnet.org/part00055"/>
	<skos:exactMatch rdf:resource="http://vocab.getty.edu/aat/300204886"/>
	<skos:scopeNote xml:lang="en">Artifacts, often textiles, that are hung on walls, especially for protection, warmth or embellishment.</skos:scopeNote>
</skos:Concept>
<skos:Concept rdf:about="http://partage.vocnet.org/part00109">
	<skos:prefLabel xml:lang="en">lighting devices</skos:prefLabel>
	<skos:prefLabel xml:lang="de">Beleuchtung</skos:prefLabel>
	<skos:altLabel xml:lang="es">artefactos de iluminación</skos:altLabel>
	<skos:prefLabel xml:lang="es">luces</skos:prefLabel>
	<skos:prefLabel xml:lang="sl">svetila</skos:prefLabel>
	<skos:altLabel xml:lang="pt">candeeiro</skos:altLabel>
	<skos:prefLabel xml:lang="pt">iluminação</skos:prefLabel>
	<skos:prefLabel xml:lang="pl">oświetlenie</skos:prefLabel>
	<skos:prefLabel xml:lang="nl">verlichtingsmiddelen</skos:prefLabel>
	<skos:prefLabel xml:lang="it">illuminazione</skos:prefLabel>
	<skos:prefLabel xml:lang="cs">osvětlovací tělesa</skos:prefLabel>
	<skos:prefLabel xml:lang="ca">llums</skos:prefLabel>
	<skos:prefLabel xml:lang="fi">valaisimet</skos:prefLabel>
	<skos:prefLabel xml:lang="sv">armaturer</skos:prefLabel>
	<skos:altLabel xml:lang="de">Leuchten</skos:altLabel>
	<skos:prefLabel xml:lang="fr">lumière</skos:prefLabel>
	<skos:prefLabel xml:lang="hu">lámpa</skos:prefLabel>
	<skos:prefLabel xml:lang="no">belysning</skos:prefLabel>
	<skos:prefLabel xml:lang="hr">rasvjetna tijela</skos:prefLabel>
	<skos:inScheme rdf:resource="http://partage.vocnet.org/Objects"/>
	<skos:broader rdf:resource="http://partage.vocnet.org/part00100"/>
	<skos:narrower rdf:resource="http://partage.vocnet.org/part00330"/>
	<skos:narrower rdf:resource="http://partage.vocnet.org/part00331"/>
	<skos:narrower rdf:resource="http://partage.vocnet.org/part00332"/>
	<skos:narrower rdf:resource="http://partage.vocnet.org/part00335"/>
	<skos:narrower rdf:resource="http://partage.vocnet.org/part00791"/>
	<skos:exactMatch rdf:resource="http://vocab.getty.edu/aat/300037581"/>
	<skos:scopeNote xml:lang="en">Apparatus, fixed or portable, whose primary purpose is to produce artificial light.</skos:scopeNote>
	<skos:editorialNote xml:lang="en">PPObjectType</skos:editorialNote>
</skos:Concept>
<skos:Concept rdf:about="http://partage.vocnet.org/part00110">
	<skos:prefLabel xml:lang="en">mirrors</skos:prefLabel>
	<skos:prefLabel xml:lang="ca">zrcalo</skos:prefLabel>
	<skos:prefLabel xml:lang="de">Spiegel</skos:prefLabel>
	<skos:prefLabel xml:lang="sv">speglar</skos:prefLabel>
	<skos:prefLabel xml:lang="pt">espelho</skos:prefLabel>
	<skos:prefLabel xml:lang="fi">peilit</skos:prefLabel>
	<skos:inScheme rdf:resource="http://partage.vocnet.org/Objects"/>
	<skos:broader rdf:resource="http://partage.vocnet.org/part00100"/>
	<skos:exactMatch rdf:resource="http://vocab.getty.edu/aat/300037682"/>
	<skos:editorialNote xml:lang="en">PPRefiningObjectType</skos:editorialNote>
	<skos:scopeNote xml:lang="en">Objects with a highly polished surface, often framed, which are designed to reflect images</skos:scopeNote>
</skos:Concept>
<skos:Concept rdf:about="http://partage.vocnet.org/part00116">
	<skos:prefLabel xml:lang="en">components (objects)</skos:prefLabel>
	<skos:inScheme rdf:resource="http://partage.vocnet.org/Objects"/>
	<skos:narrower rdf:resource="http://partage.vocnet.org/part00127"/>
	<skos:narrower rdf:resource="http://partage.vocnet.org/part00498"/>
	<skos:narrower rdf:resource="http://partage.vocnet.org/part00513"/>
	<skos:narrower rdf:resource="http://partage.vocnet.org/part00644"/>
	<skos:narrower rdf:resource="http://partage.vocnet.org/part00701"/>
	<skos:narrower rdf:resource="http://partage.vocnet.org/part00711"/>
	<skos:narrower rdf:resource="http://partage.vocnet.org/part00724"/>
	<skos:narrower rdf:resource="http://partage.vocnet.org/part00753"/>
	<skos:narrower rdf:resource="http://partage.vocnet.org/part00784"/>
	<skos:narrower rdf:resource="http://partage.vocnet.org/part00786"/>
	<skos:narrower rdf:resource="http://partage.vocnet.org/part00828"/>
	<skos:narrower rdf:resource="http://partage.vocnet.org/part00994"/>
	<skos:narrower rdf:resource="http://partage.vocnet.org/part01200"/>
	<skos:exactMatch rdf:resource="http://vocab.getty.edu/aat/300241583"/>
	<skos:scopeNote xml:lang="en">Constituent parts of objects or structures.</skos:scopeNote>
</skos:Concept>
<skos:Concept rdf:about="http://partage.vocnet.org/part00118">
	<skos:prefLabel xml:lang="en">façades</skos:prefLabel>
	<skos:prefLabel xml:lang="pt">fachada</skos:prefLabel>
	<skos:altLabel xml:lang="de">Fassaden</skos:altLabel>
	<skos:prefLabel xml:lang="de">Fassade</skos:prefLabel>
	<skos:prefLabel xml:lang="sv">fasader</skos:prefLabel>
	<skos:prefLabel xml:lang="hr">fasada</skos:prefLabel>
	<skos:prefLabel xml:lang="fi">fasadit</skos:prefLabel>
	<skos:inScheme rdf:resource="http://partage.vocnet.org/Objects"/>
	<skos:broader rdf:resource="http://partage.vocnet.org/part00120"/>
	<skos:exactMatch rdf:resource="http://vocab.getty.edu/aat/300002526"/>
	<skos:editorialNote xml:lang="en">PPRefiningObjectType</skos:editorialNote>
	<skos:scopeNote xml:lang="en">Refers to exterior faces of a building which are substantially in one plane and seem to have been designed with special regard to their conspicuousness or association with entrance. Distinct from "elevations (building divisions)," which may constitute any side or face of a building or large interior space.</skos:scopeNote>
</skos:Concept>
<skos:Concept rdf:about="http://partage.vocnet.org/part00120">
	<skos:prefLabel xml:lang="en">exterior walls</skos:prefLabel>
	<skos:inScheme rdf:resource="http://partage.vocnet.org/Objects"/>
	<skos:broader rdf:resource="http://partage.vocnet.org/part00122"/>
	<skos:narrower rdf:resource="http://partage.vocnet.org/part00118"/>
	<skos:exactMatch rdf:resource="http://vocab.getty.edu/aat/300002523"/>
	<skos:scopeNote xml:lang="en">Walls which are part of the building envelope, thereby having one face exposed to the weather or to earth.</skos:scopeNote>
</skos:Concept>
<skos:Concept rdf:about="http://partage.vocnet.org/part00122">
	<skos:prefLabel xml:lang="en">walls</skos:prefLabel>
	<skos:inScheme rdf:resource="http://partage.vocnet.org/Objects"/>
	<skos:broader rdf:resource="http://partage.vocnet.org/part00127"/>
	<skos:narrower rdf:resource="http://partage.vocnet.org/part00120"/>
	<skos:exactMatch rdf:resource="http://vocab.getty.edu/aat/300002469"/>
	<skos:scopeNote xml:lang="en">Vertical architectural members used to define and divide spaces.</skos:scopeNote>
</skos:Concept>
<skos:Concept rdf:about="http://partage.vocnet.org/part00127">
	<skos:prefLabel xml:lang="en">architectural elements</skos:prefLabel>
	<skos:prefLabel xml:lang="sv">arkitektoniska element</skos:prefLabel>
	<skos:prefLabel xml:lang="pt">elementos arquitecturais</skos:prefLabel>
	<skos:altLabel xml:lang="de">Architekturelemente</skos:altLabel>
	<skos:prefLabel xml:lang="de">Architekturelement</skos:prefLabel>
	<skos:prefLabel xml:lang="hr">arhitektonski elementi</skos:prefLabel>
	<skos:prefLabel xml:lang="fi">rakennuselementit</skos:prefLabel>
	<skos:inScheme rdf:resource="http://partage.vocnet.org/Objects"/>
	<skos:broader rdf:resource="http://partage.vocnet.org/part00116"/>
	<skos:narrower rdf:resource="http://partage.vocnet.org/part00122"/>
	<skos:narrower rdf:resource="http://partage.vocnet.org/part00745"/>
	<skos:narrower rdf:resource="http://partage.vocnet.org/part00746"/>
	<skos:narrower rdf:resource="http://partage.vocnet.org/part00747"/>
	<skos:narrower rdf:resource="http://partage.vocnet.org/part00752"/>
	<skos:narrower rdf:resource="http://partage.vocnet.org/part00785"/>
	<skos:narrower rdf:resource="http://partage.vocnet.org/part00823"/>
	<skos:narrower rdf:resource="http://partage.vocnet.org/part00825"/>
	<skos:narrower rdf:resource="http://partage.vocnet.org/part00826"/>
	<skos:narrower rdf:resource="http://partage.vocnet.org/part00827"/>
	<skos:narrower rdf:resource="http://partage.vocnet.org/part00923"/>
	<skos:narrower rdf:resource="http://partage.vocnet.org/part01129"/>
	<skos:narrower rdf:resource="http://partage.vocnet.org/part01188"/>
	<skos:exactMatch rdf:resource="http://vocab.getty.edu/aat/300000885"/>
	<skos:editorialNote xml:lang="en">PPRefiningObjectType</skos:editorialNote>
	<skos:scopeNote xml:lang="en">Forms, structural or decorative, developed originally or primarily as components of architecture, often adapted to other habitable spaces, such as in large vehicles, and often borrowed or imitated for structural or decorative use on other objects.</skos:scopeNote>
</skos:Concept>
<skos:Concept rdf:about="http://partage.vocnet.org/part00128">
	<skos:prefLabel xml:lang="en">tableware</skos:prefLabel>
	<skos:prefLabel xml:lang="de">Tafelgeschirr</skos:prefLabel>
	<skos:prefLabel xml:lang="sv">serviser</skos:prefLabel>
	<skos:altLabel xml:lang="fi">kattaus</skos:altLabel>
	<skos:prefLabel xml:lang="fi">ruokailuvälineet</skos:prefLabel>
	<skos:altLabel xml:lang="es">servicios de mesa</skos:altLabel>
	<skos:prefLabel xml:lang="es">servicio de mesa</skos:prefLabel>
	<skos:prefLabel xml:lang="sl">namizno posodje</skos:prefLabel>
	<skos:prefLabel xml:lang="pt">artigos para cozinha e sala de jantar</skos:prefLabel>
	<skos:prefLabel xml:lang="pl">zastawa stołowa</skos:prefLabel>
	<skos:prefLabel xml:lang="nl">tafelgerei</skos:prefLabel>
	<skos:prefLabel xml:lang="it">stoviglie da tavola</skos:prefLabel>
	<skos:prefLabel xml:lang="cs">stolní náčiní</skos:prefLabel>
	<skos:prefLabel xml:lang="ca">parament de taula</skos:prefLabel>
	<skos:prefLabel xml:lang="hr">stolno posuđe</skos:prefLabel>
	<skos:prefLabel xml:lang="fr">vaisselle</skos:prefLabel>
	<skos:prefLabel xml:lang="hu">asztali készlet</skos:prefLabel>
	<skos:prefLabel xml:lang="no">dekketøy</skos:prefLabel>
	<skos:inScheme rdf:resource="http://partage.vocnet.org/Objects"/>
	<skos:exactMatch rdf:resource="http://vocab.getty.edu/aat/300043196"/>
	<skos:editorialNote xml:lang="en">PPObjectType</skos:editorialNote>
	<skos:scopeNote xml:lang="en">Articles, collectively, that are generally used for serving food at the table, including various types of flatware, cutlery, hollowware, plates, and accessories, such as coasters and napkin rings, but not necessarily constituting a service.</skos:scopeNote>
</skos:Concept>
<skos:Concept rdf:about="http://partage.vocnet.org/part00133">
	<skos:prefLabel xml:lang="en">editions</skos:prefLabel>
	<skos:altLabel xml:lang="de">edição</skos:altLabel>
	<skos:altLabel xml:lang="de">Auflage</skos:altLabel>
	<skos:prefLabel xml:lang="de">Ausgabe (Druckwerk)</skos:prefLabel>
	<skos:altLabel xml:lang="de">Edition</skos:altLabel>
	<skos:altLabel xml:lang="sv">utgåvor</skos:altLabel>
	<skos:prefLabel xml:lang="sv">upplagor</skos:prefLabel>
	<skos:altLabel xml:lang="hr">edicija</skos:altLabel>
	<skos:prefLabel xml:lang="hr">izdanje</skos:prefLabel>
	<skos:prefLabel xml:lang="fi">painokset</skos:prefLabel>
	<skos:inScheme rdf:resource="http://partage.vocnet.org/Objects"/>
	<skos:exactMatch rdf:resource="http://vocab.getty.edu/aat/300121294"/>
	<skos:editorialNote xml:lang="en">PPRefiningObjectType</skos:editorialNote>
	<skos:scopeNote xml:lang="en">Groups of multiples of one work issued together, such as of a book, print, photograph, or cast sculpture. All copies of a book, print, etc., produced from substantially the same master, and issued at one time are part of the same edition.</skos:scopeNote>
</skos:Concept>
<skos:Concept rdf:about="http://partage.vocnet.org/part00134">
	<skos:prefLabel xml:lang="en">series (groups)</skos:prefLabel>
	<skos:prefLabel xml:lang="hr">serija</skos:prefLabel>
	<skos:prefLabel xml:lang="pt">série</skos:prefLabel>
	<skos:altLabel xml:lang="de">Serien</skos:altLabel>
	<skos:altLabel xml:lang="de">Reihen</skos:altLabel>
	<skos:altLabel xml:lang="de">Reihe</skos:altLabel>
	<skos:prefLabel xml:lang="de">Serie</skos:prefLabel>
	<skos:altLabel xml:lang="de">serier (grupper)</skos:altLabel>
	<skos:prefLabel xml:lang="fi">sarjat</skos:prefLabel>
	<skos:inScheme rdf:resource="http://partage.vocnet.org/Objects"/>
	<skos:exactMatch rdf:resource="http://vocab.getty.edu/aat/300027349"/>
	<skos:editorialNote xml:lang="en">PPRefiningObjectType</skos:editorialNote>
	<skos:scopeNote xml:lang="en">Groups of separate bibliographic items related to one another by the fact that each bears, in addition to its own title proper, a collective title applying to the group as a whole and issued successively; in the visual arts, for groups of works by a single artist having a specific and purposeful relation among the works.</skos:scopeNote>
</skos:Concept>
<skos:Concept rdf:about="http://partage.vocnet.org/part00135">
	<skos:altLabel xml:lang="en">portfolios (groups of works)</skos:altLabel>
	<skos:prefLabel xml:lang="en">portfolios</skos:prefLabel>
	<skos:prefLabel xml:lang="hr">portfolio</skos:prefLabel>
	<skos:prefLabel xml:lang="de">Mappenwerke</skos:prefLabel>
	<skos:altLabel xml:lang="de">Portfolios</skos:altLabel>
	<skos:altLabel xml:lang="de">Mappenwerk</skos:altLabel>
	<skos:altLabel xml:lang="de">Portfolio</skos:altLabel>
	<skos:prefLabel xml:lang="sv">arbetsprover</skos:prefLabel>
	<skos:prefLabel xml:lang="pt">portfólio</skos:prefLabel>
	<skos:prefLabel xml:lang="fi">portfoliot</skos:prefLabel>
	<skos:inScheme rdf:resource="http://partage.vocnet.org/Objects"/>
	<skos:exactMatch rdf:resource="http://vocab.getty.edu/aat/300179434"/>
	<skos:editorialNote xml:lang="en">PPRefiningObjectType</skos:editorialNote>
	<skos:scopeNote xml:lang="en">Groups of works brought together such as to exemplify the work of an artist or student. Also, groups of art works or other visual materials (often by one artist) such as photographs or prints, issued or housed together in a portfolio; they often include a loose title page or text introduction.</skos:scopeNote>
</skos:Concept>
<skos:Concept rdf:about="http://partage.vocnet.org/part00136">
	<skos:prefLabel xml:lang="en">marks (symbols)</skos:prefLabel>
	<skos:prefLabel xml:lang="hr">oznaka</skos:prefLabel>
	<skos:altLabel xml:lang="de">Marken (Zeichen)</skos:altLabel>
	<skos:prefLabel xml:lang="de">Marke (Zeichen)</skos:prefLabel>
	<skos:prefLabel xml:lang="sv">märken (symboler)</skos:prefLabel>
	<skos:prefLabel xml:lang="pt">marca</skos:prefLabel>
	<skos:prefLabel xml:lang="fi">merkit</skos:prefLabel>
	<skos:inScheme rdf:resource="http://partage.vocnet.org/Objects"/>
	<skos:narrower rdf:resource="http://partage.vocnet.org/part00140"/>
	<skos:exactMatch rdf:resource="http://vocab.getty.edu/aat/300028744"/>
	<skos:editorialNote xml:lang="en">PPRefiningObjectType</skos:editorialNote>
	<skos:scopeNote xml:lang="en">Standardized symbols, notations, or other markings on objects that convey official information, such as the object's origin or maker, its authenticity, or a change in its official status. For lettering marked on something for documentation or commemoration, use "inscriptions."</skos:scopeNote>
</skos:Concept>
<skos:Concept rdf:about="http://partage.vocnet.org/part00139">
	<skos:prefLabel xml:lang="en">promotional materials</skos:prefLabel>
	<skos:altLabel xml:lang="de">Werbegrafik</skos:altLabel>
	<skos:altLabel xml:lang="de">Gebrauchsgraphik</skos:altLabel>
	<skos:prefLabel xml:lang="de">Gebrauchsgrafik</skos:prefLabel>
	<skos:prefLabel xml:lang="sv">reklam</skos:prefLabel>
	<skos:prefLabel xml:lang="fi">mainokset</skos:prefLabel>
	<skos:prefLabel xml:lang="es">materiales promocionales</skos:prefLabel>
	<skos:prefLabel xml:lang="sl">promocijska gradiva</skos:prefLabel>
	<skos:prefLabel xml:lang="pt">materiais promocionais</skos:prefLabel>
	<skos:prefLabel xml:lang="pl">materiały reklamowe</skos:prefLabel>
	<skos:prefLabel xml:lang="nl">reclamematerialen</skos:prefLabel>
	<skos:prefLabel xml:lang="it">materiale promozionale</skos:prefLabel>
	<skos:prefLabel xml:lang="cs">propagační materiál</skos:prefLabel>
	<skos:prefLabel xml:lang="ca">materials promocionals</skos:prefLabel>
	<skos:prefLabel xml:lang="hr">promotivni materijali</skos:prefLabel>
	<skos:prefLabel xml:lang="no">markedsføringsmateriale</skos:prefLabel>
	<skos:prefLabel xml:lang="hu">reklámanyag</skos:prefLabel>
	<skos:prefLabel xml:lang="fr">matériel promotionnel</skos:prefLabel>
	<skos:inScheme rdf:resource="http://partage.vocnet.org/Objects"/>
	<skos:exactMatch rdf:resource="http://vocab.getty.edu/aat/300249572"/>
	<skos:editorialNote xml:lang="en">PPObjectType</skos:editorialNote>
	<skos:scopeNote xml:lang="en">Printed matter or objects devised to advertise or promote products, causes, or other concerns, especially those items given away to prospective consumers, clients, or contributors. Not used with reference to items produced before the late 19th century.</skos:scopeNote>
</skos:Concept>
<skos:Concept rdf:about="http://partage.vocnet.org/part00140">
	<skos:prefLabel xml:lang="en">factory marks</skos:prefLabel>
	<skos:altLabel xml:lang="de">marca de fabricante</skos:altLabel>
	<skos:altLabel xml:lang="de">Herstellermarken</skos:altLabel>
	<skos:altLabel xml:lang="de">Herstellermarke</skos:altLabel>
	<skos:altLabel xml:lang="de">Markenzeichen</skos:altLabel>
	<skos:prefLabel xml:lang="de">Signet</skos:prefLabel>
	<skos:prefLabel xml:lang="sv">fabriksmärkningar</skos:prefLabel>
	<skos:prefLabel xml:lang="hr">tvornička oznaka</skos:prefLabel>
	<skos:prefLabel xml:lang="fi">valmistusleimat</skos:prefLabel>
	<skos:inScheme rdf:resource="http://partage.vocnet.org/Objects"/>
	<skos:broader rdf:resource="http://partage.vocnet.org/part00136"/>
	<skos:exactMatch rdf:resource="http://vocab.getty.edu/aat/300028765"/>
	<skos:editorialNote xml:lang="en">PPRefiningObjectType</skos:editorialNote>
	<skos:scopeNote xml:lang="en">Devices applied to pottery, often to the bottom of a vessel or plate, for the purpose of identifying the origin of commercial pottery wares. Some ancient Greek wares include such marks; more are evident in Renaissance European wares; and the application of factory marks became nearly universally common in the 20th century.</skos:scopeNote>
</skos:Concept>
<skos:Concept rdf:about="http://partage.vocnet.org/part00141">
	<skos:prefLabel xml:lang="en">bookplates</skos:prefLabel>
	<skos:prefLabel xml:lang="sv">exlibris</skos:prefLabel>
	<skos:prefLabel xml:lang="pt">ex-libris</skos:prefLabel>
	<skos:altLabel xml:lang="de">Bücherzeichen</skos:altLabel>
	<skos:altLabel xml:lang="de">Ex-Libris</skos:altLabel>
	<skos:prefLabel xml:lang="de">Exlibris</skos:prefLabel>
	<skos:prefLabel xml:lang="hr">ex libris</skos:prefLabel>
	<skos:prefLabel xml:lang="fi">exlibrikset</skos:prefLabel>
	<skos:inScheme rdf:resource="http://partage.vocnet.org/Objects"/>
	<skos:broader rdf:resource="http://partage.vocnet.org/part00142"/>
	<skos:exactMatch rdf:resource="http://vocab.getty.edu/aat/300028731"/>
	<skos:editorialNote xml:lang="en">PPRefiningObjectType</skos:editorialNote>
	<skos:scopeNote xml:lang="en">Labels affixed to a book to indicate ownership and often its location in a collection. They may be printed or engraved, frequently with a distinctive design, pasted or tipped into books on the inside of the upper cover.</skos:scopeNote>
</skos:Concept>
<skos:Concept rdf:about="http://partage.vocnet.org/part00142">
	<skos:prefLabel xml:lang="en">labels (identifying artifacts)</skos:prefLabel>
	<skos:altLabel xml:lang="de">Etiketten</skos:altLabel>
	<skos:prefLabel xml:lang="de">Etikett</skos:prefLabel>
	<skos:prefLabel xml:lang="hr">etiketa</skos:prefLabel>
	<skos:inScheme rdf:resource="http://partage.vocnet.org/Objects"/>
	<skos:narrower rdf:resource="http://partage.vocnet.org/part00141"/>
	<skos:exactMatch rdf:resource="http://vocab.getty.edu/aat/300028730"/>
	<skos:scopeNote xml:lang="en">Pieces of paper, leather, fabric, or small tablets inscribed and affixed to something for identification or description. In the context of bookbinding, refers specifically to paper or other material separate from that used to cover a book, on which the author's name and the title are printed or engraved and glued to the spine or front board. For larger, more public identifying notices, use "identification signs."</skos:scopeNote>
	<skos:editorialNote xml:lang="en">PPRefiningObjectType</skos:editorialNote>
</skos:Concept>
<skos:Concept rdf:about="http://partage.vocnet.org/part00151">
	<skos:altLabel xml:lang="en">architecture (object genre)</skos:altLabel>
	<skos:prefLabel xml:lang="en">architecture</skos:prefLabel>
	<skos:prefLabel xml:lang="sv">arkitektur</skos:prefLabel>
	<skos:prefLabel xml:lang="fi">arkkitehtuuri</skos:prefLabel>
	<skos:prefLabel xml:lang="es">arquitectura</skos:prefLabel>
	<skos:prefLabel xml:lang="sl">arhitekturna dela</skos:prefLabel>
	<skos:prefLabel xml:lang="pt">arquitetura</skos:prefLabel>
	<skos:prefLabel xml:lang="pl">architektura</skos:prefLabel>
	<skos:prefLabel xml:lang="nl">architectuur</skos:prefLabel>
	<skos:prefLabel xml:lang="it">architettura</skos:prefLabel>
	<skos:prefLabel xml:lang="cs">architektura</skos:prefLabel>
	<skos:prefLabel xml:lang="de">Architektur</skos:prefLabel>
	<skos:prefLabel xml:lang="ca">arquitectura</skos:prefLabel>
	<skos:altLabel xml:lang="de">Baukunst</skos:altLabel>
	<skos:prefLabel xml:lang="hr">arhitektura</skos:prefLabel>
	<skos:prefLabel xml:lang="fr">architecture</skos:prefLabel>
	<skos:prefLabel xml:lang="hu">építészet</skos:prefLabel>
	<skos:prefLabel xml:lang="no">arkitektur</skos:prefLabel>
	<skos:inScheme rdf:resource="http://partage.vocnet.org/Objects"/>
	<skos:exactMatch rdf:resource="http://vocab.getty.edu/aat/300263552"/>
	<skos:editorialNote xml:lang="en">PPObjectType</skos:editorialNote>
	<skos:scopeNote xml:lang="en">Structures or parts of structures that are the result of conscious construction, are of practical use, are relatively stable and permanent, and are of a size and scale appropriate for--but not limited to--habitable buildings. Works of architecture are manifestations of the built environment that is typically classified as fine art, meaning it is generally considered to have aesthetic value, was designed by an architect (whether or not his or her name is known), and constructed with skilled labor. For the art or science of designing and building structures, use "architecture (discipline)."</skos:scopeNote>
</skos:Concept>
<skos:Concept rdf:about="http://partage.vocnet.org/part00152">
	<skos:prefLabel xml:lang="en">exhibition buildings</skos:prefLabel>
	<skos:prefLabel xml:lang="pt">galeria</skos:prefLabel>
	<skos:prefLabel xml:lang="de">Ausstellungsgebäude</skos:prefLabel>
	<skos:prefLabel xml:lang="sv">utställningsbyggnader</skos:prefLabel>
	<skos:prefLabel xml:lang="hr">izložbeni objekt</skos:prefLabel>
	<skos:prefLabel xml:lang="fi">näyttelypaviljongit</skos:prefLabel>
	<skos:inScheme rdf:resource="http://partage.vocnet.org/Objects"/>
	<skos:narrower rdf:resource="http://partage.vocnet.org/part00731"/>
	<skos:exactMatch rdf:resource="http://vocab.getty.edu/aat/300005748"/>
	<skos:editorialNote xml:lang="en">PPRefiningObjectType</skos:editorialNote>
	<skos:scopeNote xml:lang="en">Buildings built or used exculsively or primarily for exhibitions, which are organized displays of works of art or other objects of human making. Exhibition buildings may be permanent facilities or temporary structures, as at a world's fair.</skos:scopeNote>
</skos:Concept>
<skos:Concept rdf:about="http://partage.vocnet.org/part00153">
	<skos:prefLabel xml:lang="en">sepulchral monuments</skos:prefLabel>
	<skos:prefLabel xml:lang="de">Grabmal</skos:prefLabel>
	<skos:prefLabel xml:lang="sv">gravmonument</skos:prefLabel>
	<skos:prefLabel xml:lang="hr">nadgrobni spomenik</skos:prefLabel>
	<skos:prefLabel xml:lang="pt">monumentos funerários</skos:prefLabel>
	<skos:altLabel xml:lang="de">Sepulkralbauten</skos:altLabel>
	<skos:altLabel xml:lang="de">Grabmäler</skos:altLabel>
	<skos:altLabel xml:lang="de">Sepulkralbau</skos:altLabel>
	<skos:prefLabel xml:lang="fi">hautamuistomerkit</skos:prefLabel>
	<skos:inScheme rdf:resource="http://partage.vocnet.org/Objects"/>
	<skos:broader rdf:resource="http://partage.vocnet.org/part00074"/>
	<skos:exactMatch rdf:resource="http://vocab.getty.edu/aat/300005909"/>
	<skos:editorialNote xml:lang="en">PPRefiningObjectType</skos:editorialNote>
	<skos:scopeNote xml:lang="en">Structures marking or denoting burial sites.</skos:scopeNote>
</skos:Concept>
<skos:Concept rdf:about="http://partage.vocnet.org/part00155">
	<skos:prefLabel xml:lang="en">complexes (buildings)</skos:prefLabel>
	<skos:prefLabel xml:lang="pt">complexo edificado</skos:prefLabel>
	<skos:altLabel xml:lang="de">Gebäudeensembles</skos:altLabel>
	<skos:altLabel xml:lang="de">Gebäudekomplexe</skos:altLabel>
	<skos:altLabel xml:lang="de">Gebäudeensemble</skos:altLabel>
	<skos:prefLabel xml:lang="de">Gebäudekomplex</skos:prefLabel>
	<skos:prefLabel xml:lang="sv">komplex</skos:prefLabel>
	<skos:prefLabel xml:lang="hr">kompleks</skos:prefLabel>
	<skos:prefLabel xml:lang="fi">rakennuskompleksit</skos:prefLabel>
	<skos:inScheme rdf:resource="http://partage.vocnet.org/Objects"/>
	<skos:narrower rdf:resource="http://partage.vocnet.org/part00156"/>
	<skos:exactMatch rdf:resource="http://vocab.getty.edu/aat/300000202"/>
	<skos:editorialNote xml:lang="en">PPRefiningObjectType</skos:editorialNote>
	<skos:scopeNote xml:lang="en">Aggregations of buildings, other structures, and\/or open spaces, often multifunctional, and more extensive than single built works, usually shaped over a longer period of time by more participants.</skos:scopeNote>
</skos:Concept>
<skos:Concept rdf:about="http://partage.vocnet.org/part00156">
	<skos:prefLabel xml:lang="en">recreation areas</skos:prefLabel>
	<skos:prefLabel xml:lang="hr">područje za rekreaciju</skos:prefLabel>
	<skos:prefLabel xml:lang="pt">áreas recreacionais</skos:prefLabel>
	<skos:prefLabel xml:lang="de">Erholungsgebiet</skos:prefLabel>
	<skos:prefLabel xml:lang="sv">rekreationsområden</skos:prefLabel>
	<skos:altLabel xml:lang="de">Freizeitgebiet</skos:altLabel>
	<skos:prefLabel xml:lang="fi">vapaa-aikatilat</skos:prefLabel>
	<skos:inScheme rdf:resource="http://partage.vocnet.org/Objects"/>
	<skos:broader rdf:resource="http://partage.vocnet.org/part00155"/>
	<skos:exactMatch rdf:resource="http://vocab.getty.edu/aat/300000510"/>
	<skos:editorialNote xml:lang="en">PPRefiningObjectType</skos:editorialNote>
	<skos:scopeNote xml:lang="en">Land and water spaces and associated structures set aside for recreation.</skos:scopeNote>
</skos:Concept>
<skos:Concept rdf:about="http://partage.vocnet.org/part00158">
	<skos:prefLabel xml:lang="en">recreation buildings</skos:prefLabel>
	<skos:inScheme rdf:resource="http://partage.vocnet.org/Objects"/>
	<skos:narrower rdf:resource="http://partage.vocnet.org/part00853"/>
	<skos:exactMatch rdf:resource="http://vocab.getty.edu/aat/300007193"/>
	<skos:scopeNote xml:lang="en">Distinguished from "entertainment buildings" by more broadly designating buildings designed for or containing equipment for amusement, exercise, sports, or some pastime.</skos:scopeNote>
</skos:Concept>
<skos:Concept rdf:about="http://partage.vocnet.org/part00160">
	<skos:prefLabel xml:lang="en">health facilities</skos:prefLabel>
	<skos:prefLabel xml:lang="sv">sjukvårdsinrättningar</skos:prefLabel>
	<skos:prefLabel xml:lang="pt">centros sanitários</skos:prefLabel>
	<skos:altLabel xml:lang="de">Gesundheitseinrichtung</skos:altLabel>
	<skos:altLabel xml:lang="de">Medizinische Einrichtungen</skos:altLabel>
	<skos:prefLabel xml:lang="de">Gesundheitseinrichtungen</skos:prefLabel>
	<skos:altLabel xml:lang="de">Medizinische Einrichtung</skos:altLabel>
	<skos:prefLabel xml:lang="hr">zdravstvena ustanova</skos:prefLabel>
	<skos:prefLabel xml:lang="fi">terveydenhuoltolaitokset</skos:prefLabel>
	<skos:inScheme rdf:resource="http://partage.vocnet.org/Objects"/>
	<skos:narrower rdf:resource="http://partage.vocnet.org/part00742"/>
	<skos:narrower rdf:resource="http://partage.vocnet.org/part01057"/>
	<skos:exactMatch rdf:resource="http://vocab.getty.edu/aat/300006653"/>
	<skos:editorialNote xml:lang="en">PPRefiningObjectType</skos:editorialNote>
	<skos:scopeNote xml:lang="en">Buildings, other structures, and complexes of structures whose primary function is health care.</skos:scopeNote>
</skos:Concept>
<skos:Concept rdf:about="http://partage.vocnet.org/part00163">
	<skos:prefLabel xml:lang="en">schools (buildings)</skos:prefLabel>
	<skos:prefLabel xml:lang="hr">škola</skos:prefLabel>
	<skos:prefLabel xml:lang="pt">escola</skos:prefLabel>
	<skos:altLabel xml:lang="de">Schulen (Gebäude)</skos:altLabel>
	<skos:prefLabel xml:lang="de">Schule (Gebäude)</skos:prefLabel>
	<skos:prefLabel xml:lang="sv">skolor (byggnader)</skos:prefLabel>
	<skos:prefLabel xml:lang="fi">koulurakennukset</skos:prefLabel>
	<skos:inScheme rdf:resource="http://partage.vocnet.org/Objects"/>
	<skos:exactMatch rdf:resource="http://vocab.getty.edu/aat/300006495"/>
	<skos:editorialNote xml:lang="en">PPRefiningObjectType</skos:editorialNote>
	<skos:scopeNote xml:lang="en">Individual buildings or groups of buildings designed or used as places of instruction, typically having one or more classrooms where students may sit at desks and listen to an instructor, often including a library and other areas having books, computers, or other items necessary for the lessons.</skos:scopeNote>
</skos:Concept>
<skos:Concept rdf:about="http://partage.vocnet.org/part00164">
	<skos:prefLabel xml:lang="en">public buildings</skos:prefLabel>
	<skos:prefLabel xml:lang="hr">javna zgrada</skos:prefLabel>
	<skos:prefLabel xml:lang="pt">edifícios públicos</skos:prefLabel>
	<skos:prefLabel xml:lang="de">Öffentliche Gebäude</skos:prefLabel>
	<skos:altLabel xml:lang="de">Öffentliches Gebäude</skos:altLabel>
	<skos:prefLabel xml:lang="sv">offentliga byggnader</skos:prefLabel>
	<skos:prefLabel xml:lang="fi">julkiset rakennukset</skos:prefLabel>
	<skos:inScheme rdf:resource="http://partage.vocnet.org/Objects"/>
	<skos:narrower rdf:resource="http://partage.vocnet.org/part00735"/>
	<skos:exactMatch rdf:resource="http://vocab.getty.edu/aat/300008059"/>
	<skos:editorialNote xml:lang="en">PPRefiningObjectType</skos:editorialNote>
	<skos:scopeNote xml:lang="en">Buildings or groups of buildings owned and operated by a governing body and often occupied by a governmental agency.</skos:scopeNote>
</skos:Concept>
<skos:Concept rdf:about="http://partage.vocnet.org/part00165">
	<skos:prefLabel xml:lang="en">commercial buildings</skos:prefLabel>
	<skos:prefLabel xml:lang="pt">edifícios comerciais</skos:prefLabel>
	<skos:prefLabel xml:lang="de">Gewerbegebäude</skos:prefLabel>
	<skos:prefLabel xml:lang="sv">affärsfastigheter</skos:prefLabel>
	<skos:prefLabel xml:lang="hr">trgovačka građevina.</skos:prefLabel>
	<skos:prefLabel xml:lang="fi">liikerakennukset</skos:prefLabel>
	<skos:inScheme rdf:resource="http://partage.vocnet.org/Objects"/>
	<skos:narrower rdf:resource="http://partage.vocnet.org/part00739"/>
	<skos:narrower rdf:resource="http://partage.vocnet.org/part00847"/>
	<skos:exactMatch rdf:resource="http://vocab.getty.edu/aat/300005147"/>
	<skos:editorialNote xml:lang="en">PPRefiningObjectType</skos:editorialNote>
	<skos:scopeNote xml:lang="en">Use broadly to refer to buildings associated with any aspect of the various activities and business relationships of industry and trade; when referring to structures associated with the purchase, sale, or exchange of goods in business, use "mercantile buildings."</skos:scopeNote>
</skos:Concept>
<skos:Concept rdf:about="http://partage.vocnet.org/part00166">
	<skos:altLabel xml:lang="en">memorials (structures)</skos:altLabel>
	<skos:prefLabel xml:lang="en">memorials</skos:prefLabel>
	<skos:prefLabel xml:lang="de">Denkmal</skos:prefLabel>
	<skos:prefLabel xml:lang="sv">minnesmärken</skos:prefLabel>
	<skos:prefLabel xml:lang="pt">monumento de homenagem</skos:prefLabel>
	<skos:prefLabel xml:lang="hr">spomenik</skos:prefLabel>
	<skos:altLabel xml:lang="de">Gedenkstätten</skos:altLabel>
	<skos:altLabel xml:lang="de">Gedenkstätte</skos:altLabel>
	<skos:altLabel xml:lang="de">Monumente</skos:altLabel>
	<skos:altLabel xml:lang="de">Mahnmale</skos:altLabel>
	<skos:altLabel xml:lang="de">Denkmäler</skos:altLabel>
	<skos:altLabel xml:lang="de">Mahnmal</skos:altLabel>
	<skos:altLabel xml:lang="de">Monument</skos:altLabel>
	<skos:prefLabel xml:lang="fi">muistomerkit</skos:prefLabel>
	<skos:inScheme rdf:resource="http://partage.vocnet.org/Objects"/>
	<skos:broader rdf:resource="http://partage.vocnet.org/part00074"/>
	<skos:exactMatch rdf:resource="http://vocab.getty.edu/aat/300006956"/>
	<skos:editorialNote xml:lang="en">PPRefiningObjectType</skos:editorialNote>
	<skos:scopeNote xml:lang="en">Structures built to preserve the memory of beings or events. For other objects created, issued, or worn to commemorate persons or events, use "commemoratives."</skos:scopeNote>
</skos:Concept>
<skos:Concept rdf:about="http://partage.vocnet.org/part00167">
	<skos:prefLabel xml:lang="en">railway buildings</skos:prefLabel>
	<skos:prefLabel xml:lang="hr">zgrada željeznice</skos:prefLabel>
	<skos:prefLabel xml:lang="pt">estação de comboio</skos:prefLabel>
	<skos:prefLabel xml:lang="de">Bahnhofsgebäude</skos:prefLabel>
	<skos:prefLabel xml:lang="sv">järnvägsstationer</skos:prefLabel>
	<skos:prefLabel xml:lang="fi">rautatieasemat</skos:prefLabel>
	<skos:inScheme rdf:resource="http://partage.vocnet.org/Objects"/>
	<skos:broader rdf:resource="http://partage.vocnet.org/part00169"/>
	<skos:exactMatch rdf:resource="http://vocab.getty.edu/aat/300120696"/>
	<skos:editorialNote xml:lang="en">PPRefiningObjectType</skos:editorialNote>
	<skos:scopeNote xml:lang="en">Structures specifically designed for the business of a railroad or railway</skos:scopeNote>
</skos:Concept>
<skos:Concept rdf:about="http://partage.vocnet.org/part00169">
	<skos:prefLabel xml:lang="en">transportation buildings</skos:prefLabel>
	<skos:prefLabel xml:lang="sv">kommunikationsbyggnader</skos:prefLabel>
	<skos:altLabel xml:lang="hr">zračna luka</skos:altLabel>
	<skos:prefLabel xml:lang="hr">kolodvo</skos:prefLabel>
	<skos:prefLabel xml:lang="pt">instalação para transporte</skos:prefLabel>
	<skos:altLabel xml:lang="de">Verkehrsgebäude</skos:altLabel>
	<skos:prefLabel xml:lang="de">Verkehrsbauwerke</skos:prefLabel>
	<skos:altLabel xml:lang="de">Verkehrsbauwerk</skos:altLabel>
	<skos:prefLabel xml:lang="fi">liikennerakennukset</skos:prefLabel>
	<skos:inScheme rdf:resource="http://partage.vocnet.org/Objects"/>
	<skos:narrower rdf:resource="http://partage.vocnet.org/part00167"/>
	<skos:narrower rdf:resource="http://partage.vocnet.org/part00171"/>
	<skos:exactMatch rdf:resource="http://vocab.getty.edu/aat/300007736"/>
	<skos:scopeNote xml:lang="en">Buildings designed or utilized for the needs of boarding and unloading passengers and the transportaion vehicles transporting them, such as a train station, bus station, or airport.</skos:scopeNote>
</skos:Concept>
<skos:Concept rdf:about="http://partage.vocnet.org/part00171">
	<skos:prefLabel xml:lang="en">subway stations</skos:prefLabel>
	<skos:altLabel xml:lang="de">U-Bahnstationen</skos:altLabel>
	<skos:prefLabel xml:lang="sv">tunnelbanestationer</skos:prefLabel>
	<skos:prefLabel xml:lang="hr">postaja podzemne željeznice</skos:prefLabel>
	<skos:prefLabel xml:lang="pt">estação de metro</skos:prefLabel>
	<skos:altLabel xml:lang="de">U-Bahn \/ Haltestelle</skos:altLabel>
	<skos:altLabel xml:lang="de">Untergrundbahnstation</skos:altLabel>
	<skos:altLabel xml:lang="de">U-Bahnhof</skos:altLabel>
	<skos:prefLabel xml:lang="de">U-Bahnstation</skos:prefLabel>
	<skos:prefLabel xml:lang="fi">maanalaisen asemat</skos:prefLabel>
	<skos:inScheme rdf:resource="http://partage.vocnet.org/Objects"/>
	<skos:broader rdf:resource="http://partage.vocnet.org/part00169"/>
	<skos:exactMatch rdf:resource="http://vocab.getty.edu/aat/300007780"/>
	<skos:editorialNote xml:lang="en">PPRefiningObjectType</skos:editorialNote>
	<skos:scopeNote xml:lang="en">Intermediate stopping places along subway lines.</skos:scopeNote>
</skos:Concept>
<skos:Concept rdf:about="http://partage.vocnet.org/part00172">
	<skos:prefLabel xml:lang="en">industrial buildings</skos:prefLabel>
	<skos:prefLabel xml:lang="hr">industrijske građevine</skos:prefLabel>
	<skos:prefLabel xml:lang="sv">industribyggnader</skos:prefLabel>
	<skos:prefLabel xml:lang="pt">edifícios industriais</skos:prefLabel>
	<skos:prefLabel xml:lang="de">Industriegebäude</skos:prefLabel>
	<skos:prefLabel xml:lang="fi">teollisuusrakennukset</skos:prefLabel>
	<skos:inScheme rdf:resource="http://partage.vocnet.org/Objects"/>
	<skos:narrower rdf:resource="http://partage.vocnet.org/part00741"/>
	<skos:exactMatch rdf:resource="http://vocab.getty.edu/aat/300006231"/>
	<skos:editorialNote xml:lang="en">PPRefiningObjectType</skos:editorialNote>
	<skos:scopeNote xml:lang="en">Refers to buildings or groups of buildings intended to house the machinery and activities associated with modern industry and machine manufacture that arose after the Industrial Revolution, beginning in the mid-19th century.</skos:scopeNote>
</skos:Concept>
<skos:Concept rdf:about="http://partage.vocnet.org/part00177">
	<skos:prefLabel xml:lang="en">wallpapers</skos:prefLabel>
	<skos:prefLabel xml:lang="de">Tapeten</skos:prefLabel>
	<skos:prefLabel xml:lang="sv">tapeter</skos:prefLabel>
	<skos:prefLabel xml:lang="fi">tapetit</skos:prefLabel>
	<skos:altLabel xml:lang="es">papel pintado para paredes</skos:altLabel>
	<skos:prefLabel xml:lang="es">papel pintado</skos:prefLabel>
	<skos:prefLabel xml:lang="sl">tapete</skos:prefLabel>
	<skos:prefLabel xml:lang="pt">papel de parede</skos:prefLabel>
	<skos:prefLabel xml:lang="pl">tapety</skos:prefLabel>
	<skos:prefLabel xml:lang="nl">behang</skos:prefLabel>
	<skos:prefLabel xml:lang="it">carte da parati</skos:prefLabel>
	<skos:prefLabel xml:lang="cs">tapety</skos:prefLabel>
	<skos:prefLabel xml:lang="ca">paper pintat</skos:prefLabel>
	<skos:prefLabel xml:lang="fr">papier peint</skos:prefLabel>
	<skos:prefLabel xml:lang="hu">tapéta</skos:prefLabel>
	<skos:prefLabel xml:lang="no">tapet</skos:prefLabel>
	<skos:prefLabel xml:lang="hr">tapete</skos:prefLabel>
	<skos:altLabel xml:lang="de">Tapete</skos:altLabel>
	<skos:inScheme rdf:resource="http://partage.vocnet.org/Objects"/>
	<skos:broader rdf:resource="http://partage.vocnet.org/part00179"/>
	<skos:exactMatch rdf:resource="http://vocab.getty.edu/aat/300037366"/>
	<skos:editorialNote xml:lang="en">PPObjectType</skos:editorialNote>
	<skos:scopeNote xml:lang="en">Papers or paperlike materials, often decorative in nature, made primarily for attachment to walls and ceilings but sometimes applied to other surfaces.</skos:scopeNote>
</skos:Concept>
<skos:Concept rdf:about="http://partage.vocnet.org/part00179">
	<skos:prefLabel xml:lang="en">wall coverings</skos:prefLabel>
	<skos:inScheme rdf:resource="http://partage.vocnet.org/Objects"/>
	<skos:broader rdf:resource="http://partage.vocnet.org/part00100"/>
	<skos:narrower rdf:resource="http://partage.vocnet.org/part00177"/>
	<skos:narrower rdf:resource="http://partage.vocnet.org/part01121"/>
	<skos:exactMatch rdf:resource="http://vocab.getty.edu/aat/300037353"/>
	<skos:scopeNote xml:lang="en">Various materials used to decorate and protect walls and other surfaces, often in the form of flexible sheets.</skos:scopeNote>
</skos:Concept>
<skos:Concept rdf:about="http://partage.vocnet.org/part00180">
	<skos:prefLabel xml:lang="en">floor coverings</skos:prefLabel>
	<skos:prefLabel xml:lang="sv">golvbeläggningar</skos:prefLabel>
	<skos:prefLabel xml:lang="de">Bodenbelag</skos:prefLabel>
	<skos:prefLabel xml:lang="pt">tapetes</skos:prefLabel>
	<skos:prefLabel xml:lang="hr">podni pokrov</skos:prefLabel>
	<skos:prefLabel xml:lang="fi">lattianpäällysteet</skos:prefLabel>
	<skos:inScheme rdf:resource="http://partage.vocnet.org/Objects"/>
	<skos:broader rdf:resource="http://partage.vocnet.org/part00100"/>
	<skos:narrower rdf:resource="http://partage.vocnet.org/part00904"/>
	<skos:exactMatch rdf:resource="http://vocab.getty.edu/aat/300186091"/>
	<skos:editorialNote xml:lang="en">PPRefiningObjectType</skos:editorialNote>
	<skos:scopeNote xml:lang="en">Covers for floors, intended to protect the floor from soiling or wear, to provide warmth or a more comfortable walking surface, or for decoration.</skos:scopeNote>
</skos:Concept>
<skos:Concept rdf:about="http://partage.vocnet.org/part00181">
	<skos:prefLabel xml:lang="en">recreational artifacts</skos:prefLabel>
	<skos:prefLabel xml:lang="de">Freizeitgegenstände</skos:prefLabel>
	<skos:prefLabel xml:lang="sv">rekreationsföremål</skos:prefLabel>
	<skos:prefLabel xml:lang="fi">vapaa-ajan välineet</skos:prefLabel>
	<skos:prefLabel xml:lang="es">artefactos recreativos</skos:prefLabel>
	<skos:prefLabel xml:lang="sl">pribor za rekreacijo</skos:prefLabel>
	<skos:prefLabel xml:lang="pt">objetos recreativos or objetos lúdicos</skos:prefLabel>
	<skos:prefLabel xml:lang="pl">przedmioty rekreacyjne</skos:prefLabel>
	<skos:prefLabel xml:lang="nl">ontspanningsmiddelen</skos:prefLabel>
	<skos:prefLabel xml:lang="it">oggetti per il tempo libero</skos:prefLabel>
	<skos:prefLabel xml:lang="cs">vybavení pro volnočasové aktivity</skos:prefLabel>
	<skos:prefLabel xml:lang="ca">objectes recreatius</skos:prefLabel>
	<skos:prefLabel xml:lang="fr">équipement de loisir</skos:prefLabel>
	<skos:prefLabel xml:lang="hu">szabadidős termékek</skos:prefLabel>
	<skos:prefLabel xml:lang="no">fritidsutstyr</skos:prefLabel>
	<skos:prefLabel xml:lang="hr">oprema za rekreaciju</skos:prefLabel>
	<skos:inScheme rdf:resource="http://partage.vocnet.org/Objects"/>
	<skos:narrower rdf:resource="http://partage.vocnet.org/part00184"/>
	<skos:narrower rdf:resource="http://partage.vocnet.org/part01170"/>
	<skos:exactMatch rdf:resource="http://vocab.getty.edu/aat/300218781"/>
	<skos:editorialNote xml:lang="en">PPObjectType</skos:editorialNote>
	<skos:scopeNote xml:lang="en">Equipment and accessories used in any of a large array of activities that are engaged in for personal satisfaction or amusement during leisure time.</skos:scopeNote>
</skos:Concept>
<skos:Concept rdf:about="http://partage.vocnet.org/part00184">
	<skos:prefLabel xml:lang="en">playing cards</skos:prefLabel>
	<skos:prefLabel xml:lang="hr">igraće karte</skos:prefLabel>
	<skos:altLabel xml:lang="de">Spielkarte</skos:altLabel>
	<skos:prefLabel xml:lang="de">Spielkarten</skos:prefLabel>
	<skos:prefLabel xml:lang="sv">spelkort</skos:prefLabel>
	<skos:altLabel xml:lang="pt">baralho de cartas</skos:altLabel>
	<skos:prefLabel xml:lang="pt">cartas de jogo</skos:prefLabel>
	<skos:prefLabel xml:lang="fi">pelikortit</skos:prefLabel>
	<skos:inScheme rdf:resource="http://partage.vocnet.org/Objects"/>
	<skos:broader rdf:resource="http://partage.vocnet.org/part00181"/>
	<skos:exactMatch rdf:resource="http://vocab.getty.edu/aat/300211294"/>
	<skos:editorialNote xml:lang="en">PPRefiningObjectType</skos:editorialNote>
	<skos:scopeNote xml:lang="en">Cards made in sets of a designated number and marked for use as game accessories during play. The markings or designs may follow a standard suit or rank system or may be special and individualized.</skos:scopeNote>
</skos:Concept>
<skos:Concept rdf:about="http://partage.vocnet.org/part00185">
	<skos:prefLabel xml:lang="en">musical instruments</skos:prefLabel>
	<skos:prefLabel xml:lang="sv">musikinstrument</skos:prefLabel>
	<skos:prefLabel xml:lang="fi">soittimet</skos:prefLabel>
	<skos:prefLabel xml:lang="es">instrumentos musicales</skos:prefLabel>
	<skos:prefLabel xml:lang="sl">glasbila</skos:prefLabel>
	<skos:altLabel xml:lang="pt">instrumentos musicais</skos:altLabel>
	<skos:prefLabel xml:lang="pt">instrumento musical</skos:prefLabel>
	<skos:prefLabel xml:lang="pl">instrumenty muzyczne</skos:prefLabel>
	<skos:prefLabel xml:lang="nl">muziekinstrumenten</skos:prefLabel>
	<skos:prefLabel xml:lang="it">strumenti musicali</skos:prefLabel>
	<skos:prefLabel xml:lang="cs">hudební nástroje</skos:prefLabel>
	<skos:prefLabel xml:lang="ca">instruments musicals</skos:prefLabel>
	<skos:altLabel xml:lang="de">Musikinstrument</skos:altLabel>
	<skos:prefLabel xml:lang="de">Musikinstrumente</skos:prefLabel>
	<skos:prefLabel xml:lang="hr">glazbeni instrumenti</skos:prefLabel>
	<skos:prefLabel xml:lang="no">musikkinstrument</skos:prefLabel>
	<skos:prefLabel xml:lang="hu">hangszer</skos:prefLabel>
	<skos:prefLabel xml:lang="fr">instrument de musique</skos:prefLabel>
	<skos:inScheme rdf:resource="http://partage.vocnet.org/Objects"/>
	<skos:exactMatch rdf:resource="http://vocab.getty.edu/aat/300041620"/>
	<skos:editorialNote xml:lang="en">PPObjectType</skos:editorialNote>
	<skos:scopeNote xml:lang="en">Sound-producing apparatuses whose primary function is to play music.</skos:scopeNote>
</skos:Concept>
<skos:Concept rdf:about="http://partage.vocnet.org/part00188">
	<skos:prefLabel xml:lang="en">models (representations)</skos:prefLabel>
	<skos:prefLabel xml:lang="hr">model</skos:prefLabel>
	<skos:prefLabel xml:lang="de">Modelle</skos:prefLabel>
	<skos:altLabel xml:lang="de">Modell</skos:altLabel>
	<skos:prefLabel xml:lang="sv">modeller (representationer)</skos:prefLabel>
	<skos:prefLabel xml:lang="pt">modelos</skos:prefLabel>
	<skos:prefLabel xml:lang="fi">mallit</skos:prefLabel>
	<skos:inScheme rdf:resource="http://partage.vocnet.org/Objects"/>
	<skos:exactMatch rdf:resource="http://vocab.getty.edu/aat/300047753"/>
	<skos:editorialNote xml:lang="en">PPRefiningObjectType</skos:editorialNote>
	<skos:scopeNote xml:lang="en">Refers to scaled representations of objects or structures, usually three-dimensional.</skos:scopeNote>
</skos:Concept>
<skos:Concept rdf:about="http://partage.vocnet.org/part00190">
	<skos:altLabel xml:lang="en">prototypes (object genre)</skos:altLabel>
	<skos:prefLabel xml:lang="en">prototypes</skos:prefLabel>
	<skos:prefLabel xml:lang="hr">prototip</skos:prefLabel>
	<skos:prefLabel xml:lang="pt">protótipo</skos:prefLabel>
	<skos:altLabel xml:lang="de">Prototypen</skos:altLabel>
	<skos:prefLabel xml:lang="de">Prototyp</skos:prefLabel>
	<skos:prefLabel xml:lang="sv">prototyper</skos:prefLabel>
	<skos:prefLabel xml:lang="fi">prototyypit</skos:prefLabel>
	<skos:inScheme rdf:resource="http://partage.vocnet.org/Objects"/>
	<skos:exactMatch rdf:resource="http://vocab.getty.edu/aat/300166391"/>
	<skos:editorialNote xml:lang="en">PPRefiningObjectType</skos:editorialNote>
	<skos:scopeNote xml:lang="en">A manufactured object that serves as the working model for the production of subsequent copies. The term is most often associated with three-dimensional objects that are functional: furniture, buildings, and machines, and less often with painting, drawing, or sculpture. Usage is extended to paintings and drawings to describe conceptual affinities, rather than discrete objects. Use "prototypes" to describe sculpture only if the works conform to other completed works in size, shape, and detail. For small-scale three dimensional renderings for sculpture, use "maquettes," and for more finely detailed sketches for sculpture or painting, use "bozzetti."</skos:scopeNote>
</skos:Concept>
<skos:Concept rdf:about="http://partage.vocnet.org/part00191">
	<skos:prefLabel xml:lang="en">monstrances</skos:prefLabel>
	<skos:altLabel xml:lang="hr">monstanca</skos:altLabel>
	<skos:prefLabel xml:lang="hr">pokaznica</skos:prefLabel>
	<skos:altLabel xml:lang="de">Monstranzen</skos:altLabel>
	<skos:prefLabel xml:lang="de">Monstranz</skos:prefLabel>
	<skos:prefLabel xml:lang="ru">monstranser</skos:prefLabel>
	<skos:prefLabel xml:lang="pt">custódia</skos:prefLabel>
	<skos:prefLabel xml:lang="fi">monstranssit</skos:prefLabel>
	<skos:inScheme rdf:resource="http://partage.vocnet.org/Objects"/>
	<skos:broader rdf:resource="http://partage.vocnet.org/part00193"/>
	<skos:exactMatch rdf:resource="http://vocab.getty.edu/aat/300083005"/>
	<skos:editorialNote xml:lang="en">PPRefiningObjectType</skos:editorialNote>
	<skos:scopeNote xml:lang="en">Christian liturgical vessels in which the Host (the bread consecrated in the Eucharist) may be displayed through an opening or through a transparent material; used either on an altar or in processions. It is usually made of gold or silver and is often decorated with precious stones. From the Baroque period onwards the Host is typically surrounded by a sunburst design. Modern usage has limited the meaning to vessels intended for the exposition of the Host; however the term was originally applied to all kinds of vessels of goldsmith's or silversmith's work in which glass or crystal were used to allow the contents to be readily visible, whether the contents were the Host, a relic of a saint, or another object. Distinguished from "pyxes," which are vessels used to hold the reserved Host on the altar or to carry the Eucharist to the sick.</skos:scopeNote>
</skos:Concept>
<skos:Concept rdf:about="http://partage.vocnet.org/part00193">
	<skos:prefLabel xml:lang="en">ceremonial containers</skos:prefLabel>
	<skos:prefLabel xml:lang="sv">ceremoniella behållare</skos:prefLabel>
	<skos:prefLabel xml:lang="pt">recipientes cerimoniais</skos:prefLabel>
	<skos:altLabel xml:lang="de">Liturgisches Gerät</skos:altLabel>
	<skos:prefLabel xml:lang="de">Zeremonialgefäß</skos:prefLabel>
	<skos:altLabel xml:lang="de">Kultgerät</skos:altLabel>
	<skos:altLabel xml:lang="de">Ritualgerät</skos:altLabel>
	<skos:prefLabel xml:lang="hr">spremnica (ceremonijalna)</skos:prefLabel>
	<skos:prefLabel xml:lang="fi">rituaaliastiat</skos:prefLabel>
	<skos:inScheme rdf:resource="http://partage.vocnet.org/Objects"/>
	<skos:broader rdf:resource="http://partage.vocnet.org/part00085"/>
	<skos:narrower rdf:resource="http://partage.vocnet.org/part00191"/>
	<skos:exactMatch rdf:resource="http://vocab.getty.edu/aat/300197576"/>
	<skos:editorialNote xml:lang="en">PPRefiningObjectType</skos:editorialNote>
	<skos:scopeNote xml:lang="en">Containers having a primarily ceremonial or ritual purpose.</skos:scopeNote>
</skos:Concept>
<skos:Concept rdf:about="http://partage.vocnet.org/part00195">
	<skos:prefLabel xml:lang="en">sequences</skos:prefLabel>
	<skos:prefLabel xml:lang="hr">niz</skos:prefLabel>
	<skos:prefLabel xml:lang="pt">sequência</skos:prefLabel>
	<skos:altLabel xml:lang="de">Sequenzen</skos:altLabel>
	<skos:prefLabel xml:lang="de">Sequenz</skos:prefLabel>
	<skos:prefLabel xml:lang="ru">sekvenser</skos:prefLabel>
	<skos:prefLabel xml:lang="fi">jaksot</skos:prefLabel>
	<skos:inScheme rdf:resource="http://partage.vocnet.org/Objects"/>
	<skos:exactMatch rdf:resource="http://vocab.getty.edu/aat/300192339"/>
	<skos:editorialNote xml:lang="en">PPRefiningObjectType</skos:editorialNote>
	<skos:scopeNote xml:lang="en">Groups of objects, images, or data elements arranged in a specified order. For photographs taken in chronological order to record motion or change, use "chronophotographs" or "motion photographs</skos:scopeNote>
</skos:Concept>
<skos:Concept rdf:about="http://partage.vocnet.org/part00196">
	<skos:prefLabel xml:lang="en">sets (groups)</skos:prefLabel>
	<skos:prefLabel xml:lang="hr">garnitura</skos:prefLabel>
	<skos:prefLabel xml:lang="pt">conjunto</skos:prefLabel>
	<skos:altLabel xml:lang="de">Ensembles</skos:altLabel>
	<skos:altLabel xml:lang="de">Sets</skos:altLabel>
	<skos:altLabel xml:lang="de">Ensemble</skos:altLabel>
	<skos:prefLabel xml:lang="de">Set</skos:prefLabel>
	<skos:prefLabel xml:lang="sv">set</skos:prefLabel>
	<skos:prefLabel xml:lang="fi">kokonaisuudet</skos:prefLabel>
	<skos:inScheme rdf:resource="http://partage.vocnet.org/Objects"/>
	<skos:narrower rdf:resource="http://partage.vocnet.org/part00197"/>
	<skos:narrower rdf:resource="http://partage.vocnet.org/part00759"/>
	<skos:exactMatch rdf:resource="http://vocab.getty.edu/aat/300133146"/>
	<skos:editorialNote xml:lang="en">PPRefiningObjectType</skos:editorialNote>
	<skos:scopeNote xml:lang="en">Use with reference to a group of things designed to be used or viewed together.</skos:scopeNote>
</skos:Concept>
<skos:Concept rdf:about="http://partage.vocnet.org/part00197">
	<skos:prefLabel xml:lang="en">services (sets)</skos:prefLabel>
	<skos:prefLabel xml:lang="hr">servis</skos:prefLabel>
	<skos:prefLabel xml:lang="pt">serviço</skos:prefLabel>
	<skos:prefLabel xml:lang="de">Service (Hausrat)</skos:prefLabel>
	<skos:prefLabel xml:lang="sv">serviser (set)</skos:prefLabel>
	<skos:altLabel xml:lang="de">Services (Hausrat)</skos:altLabel>
	<skos:prefLabel xml:lang="fi">astiastot</skos:prefLabel>
	<skos:inScheme rdf:resource="http://partage.vocnet.org/Objects"/>
	<skos:broader rdf:resource="http://partage.vocnet.org/part00196"/>
	<skos:narrower rdf:resource="http://partage.vocnet.org/part00761"/>
	<skos:narrower rdf:resource="http://partage.vocnet.org/part00762"/>
	<skos:narrower rdf:resource="http://partage.vocnet.org/part00763"/>
	<skos:narrower rdf:resource="http://partage.vocnet.org/part00764"/>
	<skos:exactMatch rdf:resource="http://vocab.getty.edu/aat/300236054"/>
	<skos:editorialNote xml:lang="en">PPRefiningObjectType</skos:editorialNote>
	<skos:scopeNote xml:lang="en">Matching sets of containers, such as cups and dishes, or utensils, such as flatware or cutlery, needed to serve a meal for a specified number of persons for general table use or for a particular use, such as for breakfast or tea.</skos:scopeNote>
</skos:Concept>
<skos:Concept rdf:about="http://partage.vocnet.org/part00198">
	<skos:prefLabel xml:lang="en">mansions</skos:prefLabel>
	<skos:prefLabel xml:lang="hr">vila</skos:prefLabel>
	<skos:altLabel xml:lang="de">Villen</skos:altLabel>
	<skos:prefLabel xml:lang="de">Villa</skos:prefLabel>
	<skos:prefLabel xml:lang="sv">herrgårdar</skos:prefLabel>
	<skos:prefLabel xml:lang="pl">mansão</skos:prefLabel>
	<skos:prefLabel xml:lang="fi">kartanot</skos:prefLabel>
	<skos:inScheme rdf:resource="http://partage.vocnet.org/Objects"/>
	<skos:broader rdf:resource="http://partage.vocnet.org/part00200"/>
	<skos:exactMatch rdf:resource="http://vocab.getty.edu/aat/300071272"/>
	<skos:editorialNote xml:lang="en">PPRefiningObjectType</skos:editorialNote>
	<skos:scopeNote xml:lang="en">Large imposing, and usually elegant and costly, dwellings.</skos:scopeNote>
</skos:Concept>
<skos:Concept rdf:about="http://partage.vocnet.org/part00200">
	<skos:prefLabel xml:lang="en">houses</skos:prefLabel>
	<skos:prefLabel xml:lang="hr">kuća</skos:prefLabel>
	<skos:altLabel xml:lang="de">Häuser</skos:altLabel>
	<skos:prefLabel xml:lang="de">Haus</skos:prefLabel>
	<skos:prefLabel xml:lang="sv">hus</skos:prefLabel>
	<skos:prefLabel xml:lang="pt">casa</skos:prefLabel>
	<skos:prefLabel xml:lang="fi">asuinrakennukset</skos:prefLabel>
	<skos:inScheme rdf:resource="http://partage.vocnet.org/Objects"/>
	<skos:broader rdf:resource="http://partage.vocnet.org/part00075"/>
	<skos:narrower rdf:resource="http://partage.vocnet.org/part00198"/>
	<skos:narrower rdf:resource="http://partage.vocnet.org/part00755"/>
	<skos:exactMatch rdf:resource="http://vocab.getty.edu/aat/300005433"/>
	<skos:editorialNote xml:lang="en">PPRefiningObjectType</skos:editorialNote>
	<skos:scopeNote xml:lang="en">Individual dwellings designed to be occupied by a single tenant or family. May also refer to a building for human occupation, for some purpose other than that of an ordinary dwelling; with this usage, "house" is generally prefaced (e.g., "cowhouse," "almshouse").</skos:scopeNote>
</skos:Concept>
<skos:Concept rdf:about="http://partage.vocnet.org/part00202">
	<skos:prefLabel xml:lang="en">publications</skos:prefLabel>
	<skos:inScheme rdf:resource="http://partage.vocnet.org/Objects"/>
	<skos:narrower rdf:resource="http://partage.vocnet.org/part00203"/>
	<skos:exactMatch rdf:resource="http://vocab.getty.edu/aat/300111999"/>
	<skos:scopeNote xml:lang="en">Documents distributed to the public by sale or other transfer of ownership, or by rental, lease, or lending.</skos:scopeNote>
</skos:Concept>
<skos:Concept rdf:about="http://partage.vocnet.org/part00203">
	<skos:prefLabel xml:lang="en">serials (publications)</skos:prefLabel>
	<skos:inScheme rdf:resource="http://partage.vocnet.org/Objects"/>
	<skos:broader rdf:resource="http://partage.vocnet.org/part00202"/>
	<skos:narrower rdf:resource="http://partage.vocnet.org/part00204"/>
	<skos:exactMatch rdf:resource="http://vocab.getty.edu/aat/300026642"/>
	<skos:scopeNote xml:lang="en">Publications in any medium issued in successive parts bearing numerical or chronological designations and intended to be continued indefinitely, such as periodicals, newspapers, annuals (reports, yearbooks, etc.), journals, memoires, proceedings, transactions, etc., of societies and numbered monographic series.</skos:scopeNote>
</skos:Concept>
<skos:Concept rdf:about="http://partage.vocnet.org/part00204">
	<skos:prefLabel xml:lang="en">periodicals (serials (publications)</skos:prefLabel>
	<skos:inScheme rdf:resource="http://partage.vocnet.org/Objects"/>
	<skos:broader rdf:resource="http://partage.vocnet.org/part00203"/>
	<skos:narrower rdf:resource="http://partage.vocnet.org/part00502"/>
	<skos:exactMatch rdf:resource="http://vocab.getty.edu/aat/300026657"/>
	<skos:scopeNote xml:lang="en">Publications issued at regular intervals, but not daily, containing articles on various subjects by different authors for the general reader.</skos:scopeNote>
</skos:Concept>
<skos:Concept rdf:about="http://partage.vocnet.org/part00213">
	<skos:prefLabel xml:lang="en">clothing</skos:prefLabel>
	<skos:prefLabel xml:lang="sv">kläder</skos:prefLabel>
	<skos:prefLabel xml:lang="pt">vestuário</skos:prefLabel>
	<skos:prefLabel xml:lang="de">Bekleidung</skos:prefLabel>
	<skos:prefLabel xml:lang="hr">odjeća.</skos:prefLabel>
	<skos:prefLabel xml:lang="fi">vaatteet</skos:prefLabel>
	<skos:inScheme rdf:resource="http://partage.vocnet.org/Objects"/>
	<skos:broader rdf:resource="http://partage.vocnet.org/part00081"/>
	<skos:exactMatch rdf:resource="http://vocab.getty.edu/aat/300266639"/>
	<skos:editorialNote xml:lang="en">PPRefiningObjectType</skos:editorialNote>
	<skos:scopeNote xml:lang="en">Coverings for the torso, limbs, hands, feet, and head for warmth, fashion, or to cover nudity. It generally excludes other items of costume such as jewelry, crowns, and other accessories that are purely decorative or symbolic and have no practical function.</skos:scopeNote>
</skos:Concept>
<skos:Concept rdf:about="http://partage.vocnet.org/part00215">
	<skos:prefLabel xml:lang="en">cutlery</skos:prefLabel>
	<skos:prefLabel xml:lang="pt">cutelaria</skos:prefLabel>
	<skos:prefLabel xml:lang="de">Schneidwerkzeug</skos:prefLabel>
	<skos:altLabel xml:lang="de">Schneidware</skos:altLabel>
	<skos:prefLabel xml:lang="sv">bestick</skos:prefLabel>
	<skos:prefLabel xml:lang="hr">pribor za posluživanje</skos:prefLabel>
	<skos:prefLabel xml:lang="fi">aterimet</skos:prefLabel>
	<skos:inScheme rdf:resource="http://partage.vocnet.org/Objects"/>
	<skos:broader rdf:resource="http://partage.vocnet.org/part00218"/>
	<skos:exactMatch rdf:resource="http://vocab.getty.edu/aat/300199794"/>
	<skos:editorialNote xml:lang="en">PPRefiningObjectType</skos:editorialNote>
	<skos:scopeNote xml:lang="en">Culinary utensils that have a cutting edge, especially various forms of knives used for cutting, carving, dividing, or serving food. Sometimes used to embrace all types of flat culinary utensils; however, prefer "flatware" when referring to forks, spoons, and similar culinary tools without a cutting edge.</skos:scopeNote>
</skos:Concept>
<skos:Concept rdf:about="http://partage.vocnet.org/part00218">
	<skos:prefLabel xml:lang="en">equipment</skos:prefLabel>
	<skos:prefLabel xml:lang="es">equipo</skos:prefLabel>
	<skos:prefLabel xml:lang="sl">pribor</skos:prefLabel>
	<skos:prefLabel xml:lang="pt">apetrechos</skos:prefLabel>
	<skos:altLabel xml:lang="pt">equipamento</skos:altLabel>
	<skos:prefLabel xml:lang="pl">wyposażenie</skos:prefLabel>
	<skos:prefLabel xml:lang="nl">uitrusting</skos:prefLabel>
	<skos:prefLabel xml:lang="it">strumenti</skos:prefLabel>
	<skos:prefLabel xml:lang="cs">vybavení</skos:prefLabel>
	<skos:prefLabel xml:lang="ca">equip</skos:prefLabel>
	<skos:altLabel xml:lang="fi">välineet</skos:altLabel>
	<skos:prefLabel xml:lang="fi">varusteet</skos:prefLabel>
	<skos:prefLabel xml:lang="de">Gerät</skos:prefLabel>
	<skos:altLabel xml:lang="de">Ausstattung</skos:altLabel>
	<skos:altLabel xml:lang="de">Gerätschaften</skos:altLabel>
	<skos:prefLabel xml:lang="hr">pribor</skos:prefLabel>
	<skos:prefLabel xml:lang="no">utstyr</skos:prefLabel>
	<skos:prefLabel xml:lang="hu">felszerelés</skos:prefLabel>
	<skos:prefLabel xml:lang="fr">équipement</skos:prefLabel>
	<skos:prefLabel xml:lang="sv">utrustning</skos:prefLabel>
	<skos:inScheme rdf:resource="http://partage.vocnet.org/Objects"/>
	<skos:narrower rdf:resource="http://partage.vocnet.org/part00215"/>
	<skos:narrower rdf:resource="http://partage.vocnet.org/part00219"/>
	<skos:narrower rdf:resource="http://partage.vocnet.org/part00505"/>
	<skos:narrower rdf:resource="http://partage.vocnet.org/part00829"/>
	<skos:narrower rdf:resource="http://partage.vocnet.org/part00830"/>
	<skos:narrower rdf:resource="http://partage.vocnet.org/part00831"/>
	<skos:narrower rdf:resource="http://partage.vocnet.org/part00833"/>
	<skos:narrower rdf:resource="http://partage.vocnet.org/part00834"/>
	<skos:narrower rdf:resource="http://partage.vocnet.org/part00983"/>
	<skos:narrower rdf:resource="http://partage.vocnet.org/part01028"/>
	<skos:narrower rdf:resource="http://partage.vocnet.org/part01172"/>
	<skos:narrower rdf:resource="http://partage.vocnet.org/part01181"/>
	<skos:exactMatch rdf:resource="http://vocab.getty.edu/aat/300122241"/>
	<skos:editorialNote xml:lang="en">PPObjectType</skos:editorialNote>
	<skos:scopeNote xml:lang="en">Articles or physical resources used to equip a person or thing, such as the instruments used in an activity or operation.</skos:scopeNote>
</skos:Concept>
<skos:Concept rdf:about="http://partage.vocnet.org/part00219">
	<skos:prefLabel xml:lang="en">flatware</skos:prefLabel>
	<skos:altLabel xml:lang="de">Flachware</skos:altLabel>
	<skos:prefLabel xml:lang="de">Besteck</skos:prefLabel>
	<skos:prefLabel xml:lang="pt">faqueiro</skos:prefLabel>
	<skos:prefLabel xml:lang="hr">pribor za jelo</skos:prefLabel>
	<skos:prefLabel xml:lang="fi">ruokailuvälineet.</skos:prefLabel>
	<skos:inScheme rdf:resource="http://partage.vocnet.org/Objects"/>
	<skos:broader rdf:resource="http://partage.vocnet.org/part00218"/>
	<skos:narrower rdf:resource="http://partage.vocnet.org/part00835"/>
	<skos:narrower rdf:resource="http://partage.vocnet.org/part01144"/>
	<skos:exactMatch rdf:resource="http://vocab.getty.edu/aat/300199800"/>
	<skos:editorialNote xml:lang="en">PPRefiningObjectType</skos:editorialNote>
	<skos:scopeNote xml:lang="en">Culinary utensils that are basically flat, such as forks and spoons, and have no cutting edge. Distinguished from "hollowware" such as drinking vessels and bowls. In modern usage the term embraces all types of flat culinary utensils with or without a cutting edge; however, prefer "cutlery" when referring to culinary utensils with a cutting edge, especially various forms of knives used for food. Flatware is now usually made in sets having on the handles similar or related decorative patterns. The term can also refer to relatively flat or shallow items of crockery such as plates and saucers.</skos:scopeNote>
</skos:Concept>
<skos:Concept rdf:about="http://partage.vocnet.org/part00221">
	<skos:altLabel xml:lang="en">embroidery (visual works)</skos:altLabel>
	<skos:prefLabel xml:lang="en">embroidery</skos:prefLabel>
	<skos:prefLabel xml:lang="sv">broderi</skos:prefLabel>
	<skos:prefLabel xml:lang="es">bordado</skos:prefLabel>
	<skos:prefLabel xml:lang="sl">vezenine</skos:prefLabel>
	<skos:prefLabel xml:lang="pt">bordado</skos:prefLabel>
	<skos:prefLabel xml:lang="pl">haft</skos:prefLabel>
	<skos:prefLabel xml:lang="nl">borduurwerk</skos:prefLabel>
	<skos:prefLabel xml:lang="it">ricamo</skos:prefLabel>
	<skos:prefLabel xml:lang="cs">výšivka</skos:prefLabel>
	<skos:prefLabel xml:lang="ca">brodat</skos:prefLabel>
	<skos:prefLabel xml:lang="de">Stickerei</skos:prefLabel>
	<skos:prefLabel xml:lang="hr">vezivo</skos:prefLabel>
	<skos:prefLabel xml:lang="no">broderi</skos:prefLabel>
	<skos:prefLabel xml:lang="fr">broderie</skos:prefLabel>
	<skos:prefLabel xml:lang="fi">kirjonta</skos:prefLabel>
	<skos:inScheme rdf:resource="http://partage.vocnet.org/Objects"/>
	<skos:broader rdf:resource="http://partage.vocnet.org/part00045"/>
	<skos:exactMatch rdf:resource="http://vocab.getty.edu/aat/300264024"/>
	<skos:editorialNote xml:lang="en">PPObjectType</skos:editorialNote>
	<skos:scopeNote xml:lang="en">Refers to works characterized by a pattern or design executed in stitches using thread or fine wire. The designs are typically executed on textiles, but leather, paper, or another media may also be used; the designs may be intended to be framed, or to decorate apparel, bed linens, furniture coverings, pillows, altar cloths, ceremonial hangings, or other items.</skos:scopeNote>
</skos:Concept>
<skos:Concept rdf:about="http://partage.vocnet.org/part00222">
	<skos:altLabel xml:lang="en">lace (needlework)</skos:altLabel>
	<skos:prefLabel xml:lang="en">lace</skos:prefLabel>
	<skos:altLabel xml:lang="de">Spitze</skos:altLabel>
	<skos:prefLabel xml:lang="de">Spitzen</skos:prefLabel>
	<skos:prefLabel xml:lang="sv">spets</skos:prefLabel>
	<skos:prefLabel xml:lang="fi">pitsit</skos:prefLabel>
	<skos:prefLabel xml:lang="es">encaje</skos:prefLabel>
	<skos:prefLabel xml:lang="sl">čipke</skos:prefLabel>
	<skos:prefLabel xml:lang="pt">renda</skos:prefLabel>
	<skos:prefLabel xml:lang="pl">koronka</skos:prefLabel>
	<skos:prefLabel xml:lang="nl">kant</skos:prefLabel>
	<skos:prefLabel xml:lang="it">merletti</skos:prefLabel>
	<skos:prefLabel xml:lang="cs">krajka</skos:prefLabel>
	<skos:prefLabel xml:lang="ca">puntes</skos:prefLabel>
	<skos:prefLabel xml:lang="fr">dentelle</skos:prefLabel>
	<skos:prefLabel xml:lang="hu">csipke</skos:prefLabel>
	<skos:prefLabel xml:lang="no">lasur</skos:prefLabel>
	<skos:prefLabel xml:lang="hr">čipka</skos:prefLabel>
	<skos:inScheme rdf:resource="http://partage.vocnet.org/Objects"/>
	<skos:broader rdf:resource="http://partage.vocnet.org/part00045"/>
	<skos:exactMatch rdf:resource="http://vocab.getty.edu/aat/300132861"/>
	<skos:editorialNote xml:lang="en">PPObjectType</skos:editorialNote>
	<skos:scopeNote xml:lang="en">Refers to a fine, openwork ornamental textile work formed by looping, interlacing, twisting, plaiting, or braiding threads of linen, cotton, silk, hair, metal, or another fiber to form designs or patterns. Lace may be made with a needle or with bobbins. Embroidery may be added. Modern lace may be made by machine. Openwork fabrics made on a loom and ornamental openwork knitting are generally not classified as lace. Lace is often white or monochromatic. True lace developed in the fourteenth century in Europe and the Middle East, although ornamented openwork fabrics were known in ancient cultures, including the Egyptian culture. Lace may be used as a border, edging, or insert on linens or apparel; it is also formed into large pieces of cloth used for hangings, draperies, apparel, or other items.</skos:scopeNote>
</skos:Concept>
<skos:Concept rdf:about="http://partage.vocnet.org/part00223">
	<skos:prefLabel xml:lang="en">earthenware</skos:prefLabel>
	<skos:prefLabel xml:lang="nl">aardewerk</skos:prefLabel>
	<skos:prefLabel xml:lang="it">terracotta</skos:prefLabel>
	<skos:prefLabel xml:lang="cs">pórovina</skos:prefLabel>
	<skos:prefLabel xml:lang="ca">pisa</skos:prefLabel>
	<skos:altLabel xml:lang="de">Töpferware</skos:altLabel>
	<skos:prefLabel xml:lang="de">Irdenware</skos:prefLabel>
	<skos:prefLabel xml:lang="sv">lergods</skos:prefLabel>
	<skos:prefLabel xml:lang="fi">savitavara</skos:prefLabel>
	<skos:prefLabel xml:lang="es">loza</skos:prefLabel>
	<skos:prefLabel xml:lang="sl">lončenina</skos:prefLabel>
	<skos:prefLabel xml:lang="pt">louça de barro</skos:prefLabel>
	<skos:prefLabel xml:lang="pl">wyroby garncarskie</skos:prefLabel>
	<skos:prefLabel xml:lang="fr">faïence</skos:prefLabel>
	<skos:prefLabel xml:lang="hu">agyagkerámia</skos:prefLabel>
	<skos:prefLabel xml:lang="no">leirgods</skos:prefLabel>
	<skos:prefLabel xml:lang="hr">glineno posuđe</skos:prefLabel>
	<skos:inScheme rdf:resource="http://partage.vocnet.org/Objects"/>
	<skos:broader rdf:resource="http://partage.vocnet.org/part00224"/>
	<skos:narrower rdf:resource="http://partage.vocnet.org/part00226"/>
	<skos:narrower rdf:resource="http://partage.vocnet.org/part00811"/>
	<skos:exactMatch rdf:resource="http://vocab.getty.edu/aat/300140803"/>
	<skos:editorialNote xml:lang="en">PPObjectType</skos:editorialNote>
	<skos:scopeNote xml:lang="en">Pottery with a porous body, fired below 1200 degrees Centigrade. It is not vitrified, and must be glazed to render it nonporous.</skos:scopeNote>
</skos:Concept>
<skos:Concept rdf:about="http://partage.vocnet.org/part00224">
	<skos:prefLabel xml:lang="en">pottery (object genre)</skos:prefLabel>
	<skos:inScheme rdf:resource="http://partage.vocnet.org/Objects"/>
	<skos:broader rdf:resource="http://partage.vocnet.org/part00064"/>
	<skos:narrower rdf:resource="http://partage.vocnet.org/part00223"/>
	<skos:narrower rdf:resource="http://partage.vocnet.org/part00225"/>
	<skos:narrower rdf:resource="http://partage.vocnet.org/part01228"/>
	<skos:exactMatch rdf:resource="http://vocab.getty.edu/aat/300010666"/>
	<skos:scopeNote xml:lang="en">Generally, all ware made of ceramic, which is any of various hard, brittle, heat-resistant and corrosion-resistant materials made by shaping and then firing a nonmetallic mineral, such as clay, at a high temperature. In specialized usage, it typically does not include porcelain, which is a type of ceramic ware made of a refractory white clay, or "kaolin," and a feldspathic rock, that react when fired so the clay serves to hold the shape of the object and the rock fuses into a natural glass.</skos:scopeNote>
</skos:Concept>
<skos:Concept rdf:about="http://partage.vocnet.org/part00225">
	<skos:altLabel xml:lang="en">stoneware (pottery)</skos:altLabel>
	<skos:prefLabel xml:lang="en">stoneware</skos:prefLabel>
	<skos:prefLabel xml:lang="de">Steingut</skos:prefLabel>
	<skos:prefLabel xml:lang="sv">stengods</skos:prefLabel>
	<skos:prefLabel xml:lang="fi">kivitavara</skos:prefLabel>
	<skos:altLabel xml:lang="es">gres vidriado</skos:altLabel>
	<skos:prefLabel xml:lang="es">gres</skos:prefLabel>
	<skos:altLabel xml:lang="sl">posodje iz kamenine</skos:altLabel>
	<skos:prefLabel xml:lang="sl">kamenina</skos:prefLabel>
	<skos:prefLabel xml:lang="pt">grés</skos:prefLabel>
	<skos:prefLabel xml:lang="pl">kamionka</skos:prefLabel>
	<skos:prefLabel xml:lang="nl">steengoed</skos:prefLabel>
	<skos:prefLabel xml:lang="it">vasellame</skos:prefLabel>
	<skos:prefLabel xml:lang="cs">kamenina</skos:prefLabel>
	<skos:prefLabel xml:lang="ca">gres</skos:prefLabel>
	<skos:prefLabel xml:lang="fr">grès</skos:prefLabel>
	<skos:prefLabel xml:lang="hu">kőedény</skos:prefLabel>
	<skos:prefLabel xml:lang="no">steingods</skos:prefLabel>
	<skos:prefLabel xml:lang="hr">kamenjača</skos:prefLabel>
	<skos:inScheme rdf:resource="http://partage.vocnet.org/Objects"/>
	<skos:broader rdf:resource="http://partage.vocnet.org/part00224"/>
	<skos:exactMatch rdf:resource="http://vocab.getty.edu/aat/300010672"/>
	<skos:editorialNote xml:lang="en">PPObjectType</skos:editorialNote>
	<skos:scopeNote xml:lang="en">A type of pottery midway between earthenware and porcelain being made of clay and a fusible stone. It is fired to a point where partial vitrification renders it impervious to liquids, but, unlike porcelain, it is very seldom more than faintly translucent. The vitrification makes it unnecessary to add a glaze, but for reasons of utility and appearance decorative glazes are sometimes used, such as salt glaze and lead glaze.</skos:scopeNote>
</skos:Concept>
<skos:Concept rdf:about="http://partage.vocnet.org/part00226">
	<skos:prefLabel xml:lang="en">maiolica</skos:prefLabel>
	<skos:prefLabel xml:lang="sv">majolika</skos:prefLabel>
	<skos:prefLabel xml:lang="es">mayólica</skos:prefLabel>
	<skos:altLabel xml:lang="sl">posodje iz majolike</skos:altLabel>
	<skos:prefLabel xml:lang="sl">majolika</skos:prefLabel>
	<skos:prefLabel xml:lang="pt">majólica</skos:prefLabel>
	<skos:prefLabel xml:lang="pl">majolika</skos:prefLabel>
	<skos:prefLabel xml:lang="nl">majolica</skos:prefLabel>
	<skos:prefLabel xml:lang="it">maioliche</skos:prefLabel>
	<skos:prefLabel xml:lang="cs">majolika</skos:prefLabel>
	<skos:prefLabel xml:lang="ca">majòlica</skos:prefLabel>
	<skos:prefLabel xml:lang="de">Majolika</skos:prefLabel>
	<skos:prefLabel xml:lang="fi">majolika</skos:prefLabel>
	<skos:prefLabel xml:lang="fr">majolique</skos:prefLabel>
	<skos:prefLabel xml:lang="hu">majolika</skos:prefLabel>
	<skos:prefLabel xml:lang="no">majolika</skos:prefLabel>
	<skos:prefLabel xml:lang="hr">majolika</skos:prefLabel>
	<skos:inScheme rdf:resource="http://partage.vocnet.org/Objects"/>
	<skos:broader rdf:resource="http://partage.vocnet.org/part00223"/>
	<skos:exactMatch rdf:resource="http://vocab.getty.edu/aat/300021170"/>
	<skos:editorialNote xml:lang="en">PPObjectType</skos:editorialNote>
	<skos:scopeNote xml:lang="en">Refers to tin-glazed earthenware, particularly such ware produced in Italy. The term originally referred to the island of Majorca (or an alternate theory has it referring to Malaga), and designated only Hispano-Moresque lusterware; but since the 16th century it has been used to refer to Italian tin-glazed ware and imitations of the Italian ware. It is characterized by painted decoration of high quality executed in several colors on the dry but unfired tin glaze, generally with a final coating of clear lead glaze. The range of colors is typically limited to cobalt blue, copper green, manganese purple, antimony yellow, and iron red, with white provided by the tin-glaze material. When white is used for painting, it is applied onto a bluish-white glaze or blue ground. The luster is typically a golden color derived from silver or a mother-of-pearl effect.</skos:scopeNote>
</skos:Concept>
<skos:Concept rdf:about="http://partage.vocnet.org/part00249">
	<skos:altLabel xml:lang="en">stained glass (visual works)</skos:altLabel>
	<skos:prefLabel xml:lang="en">stained glass</skos:prefLabel>
	<skos:prefLabel xml:lang="hr">vitraji</skos:prefLabel>
	<skos:prefLabel xml:lang="no">blyglass</skos:prefLabel>
	<skos:prefLabel xml:lang="hu">ólomüveg</skos:prefLabel>
	<skos:prefLabel xml:lang="fr">vitrail</skos:prefLabel>
	<skos:prefLabel xml:lang="pl">witraże</skos:prefLabel>
	<skos:prefLabel xml:lang="pt">vitral</skos:prefLabel>
	<skos:prefLabel xml:lang="sl">vitraži</skos:prefLabel>
	<skos:prefLabel xml:lang="es">vidriera de colores</skos:prefLabel>
	<skos:prefLabel xml:lang="sv">blyglas</skos:prefLabel>
	<skos:altLabel xml:lang="de">Buntglas</skos:altLabel>
	<skos:altLabel xml:lang="de">Farbglas</skos:altLabel>
	<skos:prefLabel xml:lang="de">Glasmalerei (Glasfenster)</skos:prefLabel>
	<skos:prefLabel xml:lang="ca">vitrall</skos:prefLabel>
	<skos:prefLabel xml:lang="cs">vitráž</skos:prefLabel>
	<skos:prefLabel xml:lang="it">vetri colorati</skos:prefLabel>
	<skos:prefLabel xml:lang="nl">gebrandschilderd glas</skos:prefLabel>
	<skos:prefLabel xml:lang="fi">lasimaalaus</skos:prefLabel>
	<skos:inScheme rdf:resource="http://partage.vocnet.org/Objects"/>
	<skos:broader rdf:resource="http://partage.vocnet.org/part00044"/>
	<skos:exactMatch rdf:resource="http://vocab.getty.edu/aat/300263722"/>
	<skos:editorialNote xml:lang="en">PPObjectType</skos:editorialNote>
	<skos:scopeNote xml:lang="en">Refers to works made of colored glass, generally in the form of a window, autonomous panel, or lampshade, in which the design is meant to be observed through refracted light and its effect is greatly dependent on the quality of the light. The stages of manufacture were described in a manual written in the early twelfth century by the monk Theophilus and the process has hardly changed since then. The window or other item is made by cutting pieces of colored glass based on a full-scale cartoon and holding the pieces together by strips of lead. Details may be painted on the surface of the pieces of glass and fired in a kiln before piecing the glass together. The method of weatherproofing and fixing the glass in a window is often highly decorative and forms an important element of the design. The highest achievements in stained glass are thought to be those of the Gothic era in Europe and those of the Gothic Revival of the nineteenth century.</skos:scopeNote>
</skos:Concept>
<skos:Concept rdf:about="http://partage.vocnet.org/part00298">
	<skos:prefLabel xml:lang="en">cabinets</skos:prefLabel>
	<skos:prefLabel xml:lang="sv">kabinett</skos:prefLabel>
	<skos:prefLabel xml:lang="pt">armário</skos:prefLabel>
	<skos:altLabel xml:lang="de">Kabinettschränke</skos:altLabel>
	<skos:prefLabel xml:lang="de">Kabinettschrank</skos:prefLabel>
	<skos:prefLabel xml:lang="hr">kabinetski ormarić</skos:prefLabel>
	<skos:prefLabel xml:lang="fi">kabinettikaapit</skos:prefLabel>
	<skos:inScheme rdf:resource="http://partage.vocnet.org/Objects"/>
	<skos:broader rdf:resource="http://partage.vocnet.org/part00299"/>
	<skos:narrower rdf:resource="http://partage.vocnet.org/part00800"/>
	<skos:exactMatch rdf:resource="http://vocab.getty.edu/aat/300038888"/>
	<skos:scopeNote xml:lang="en">Case furniture consisting of a set of shelves, small drawers, or pigeonholes, fronted by one or more doors, and intended for the storage and sometimes the display of small objects. Also, similar built-in or fitted cases often designed for specific purposes, as in a kitchen or bathroom.</skos:scopeNote>
</skos:Concept>
<skos:Concept rdf:about="http://partage.vocnet.org/part00299">
	<skos:prefLabel xml:lang="en">case furniture</skos:prefLabel>
	<skos:prefLabel xml:lang="sv">förvaringsmöbler</skos:prefLabel>
	<skos:altLabel xml:lang="pt">prateleira.</skos:altLabel>
	<skos:prefLabel xml:lang="pt">estante.</skos:prefLabel>
	<skos:prefLabel xml:lang="de">Kastenmöbel</skos:prefLabel>
	<skos:prefLabel xml:lang="hr">kasetni namještaj</skos:prefLabel>
	<skos:prefLabel xml:lang="fi">laatikostot.</skos:prefLabel>
	<skos:inScheme rdf:resource="http://partage.vocnet.org/Objects"/>
	<skos:broader rdf:resource="http://partage.vocnet.org/part00099"/>
	<skos:narrower rdf:resource="http://partage.vocnet.org/part00298"/>
	<skos:narrower rdf:resource="http://partage.vocnet.org/part00301"/>
	<skos:narrower rdf:resource="http://partage.vocnet.org/part00302"/>
	<skos:narrower rdf:resource="http://partage.vocnet.org/part00305"/>
	<skos:narrower rdf:resource="http://partage.vocnet.org/part00315"/>
	<skos:narrower rdf:resource="http://partage.vocnet.org/part00799"/>
	<skos:narrower rdf:resource="http://partage.vocnet.org/part00801"/>
	<skos:narrower rdf:resource="http://partage.vocnet.org/part00803"/>
	<skos:narrower rdf:resource="http://partage.vocnet.org/part00804"/>
	<skos:narrower rdf:resource="http://partage.vocnet.org/part00805"/>
	<skos:exactMatch rdf:resource="http://vocab.getty.edu/aat/300038860"/>
	<skos:editorialNote xml:lang="en">PPRefiningObjectType</skos:editorialNote>
	<skos:scopeNote xml:lang="en">Furniture that encloses a space and is generally boxlike in structure; intended for storage or display.</skos:scopeNote>
</skos:Concept>
<skos:Concept rdf:about="http://partage.vocnet.org/part00301">
	<skos:prefLabel xml:lang="en">cupboards</skos:prefLabel>
	<skos:prefLabel xml:lang="pt">louceiro.</skos:prefLabel>
	<skos:altLabel xml:lang="de">Kästen (Schränke)</skos:altLabel>
	<skos:altLabel xml:lang="de">Kasten (Schrank)</skos:altLabel>
	<skos:altLabel xml:lang="de">Schränke</skos:altLabel>
	<skos:prefLabel xml:lang="de">Schrank</skos:prefLabel>
	<skos:altLabel xml:lang="hr">ormarić</skos:altLabel>
	<skos:prefLabel xml:lang="hr">kredenc</skos:prefLabel>
	<skos:prefLabel xml:lang="fi">astiakaapit</skos:prefLabel>
	<skos:inScheme rdf:resource="http://partage.vocnet.org/Objects"/>
	<skos:broader rdf:resource="http://partage.vocnet.org/part00299"/>
	<skos:exactMatch rdf:resource="http://vocab.getty.edu/aat/300039183"/>
	<skos:editorialNote xml:lang="en">PPRefiningObjectType</skos:editorialNote>
	<skos:scopeNote xml:lang="en">Originally boards or open structures of shelves on which cups, especially silver, might be placed for storage or display. Beginning in the 15th century, doors were added. Today a generic term for a closet or a cabinet enclosed by doors, often placed in a corner of a room or a recess in the wall, with shelves for keeping cups, dishes, provisions, books, or valuables.</skos:scopeNote>
</skos:Concept>
<skos:Concept rdf:about="http://partage.vocnet.org/part00302">
	<skos:prefLabel xml:lang="en">chests (case furniture)</skos:prefLabel>
	<skos:prefLabel xml:lang="sv">kistor</skos:prefLabel>
	<skos:prefLabel xml:lang="pt">arca</skos:prefLabel>
	<skos:altLabel xml:lang="de">Truhen</skos:altLabel>
	<skos:prefLabel xml:lang="de">Truhe</skos:prefLabel>
	<skos:prefLabel xml:lang="hr">škrinja</skos:prefLabel>
	<skos:prefLabel xml:lang="fi">arkut</skos:prefLabel>
	<skos:inScheme rdf:resource="http://partage.vocnet.org/Objects"/>
	<skos:broader rdf:resource="http://partage.vocnet.org/part00299"/>
	<skos:narrower rdf:resource="http://partage.vocnet.org/part01184"/>
	<skos:scopeNote xml:lang="en">Large boxes with hinged lids intended for the storage of textiles, clothing, and other articles.</skos:scopeNote>
	<skos:editorialNote xml:lang="en">PPRefiningObjectType</skos:editorialNote>
</skos:Concept>
<skos:Concept rdf:about="http://partage.vocnet.org/part00303">
	<skos:prefLabel xml:lang="en">fire screens (furniture)</skos:prefLabel>
	<skos:prefLabel xml:lang="sv">eldskärmar (möbler)</skos:prefLabel>
	<skos:prefLabel xml:lang="pt">guarda fogo (madeira)</skos:prefLabel>
	<skos:altLabel xml:lang="de">Ofenschirme</skos:altLabel>
	<skos:altLabel xml:lang="de">Ofenschirm</skos:altLabel>
	<skos:prefLabel xml:lang="de">Kaminschirm (Möbel)</skos:prefLabel>
	<skos:altLabel xml:lang="de">Kaminschirme (Möbel)</skos:altLabel>
	<skos:prefLabel xml:lang="hr">zaslon za peć</skos:prefLabel>
	<skos:prefLabel xml:lang="fi">tulenvarjostimet</skos:prefLabel>
	<skos:inScheme rdf:resource="http://partage.vocnet.org/Objects"/>
	<skos:broader rdf:resource="http://partage.vocnet.org/part00102"/>
	<skos:narrower rdf:resource="http://partage.vocnet.org/part00562"/>
	<skos:editorialNote xml:lang="en">PPRefiningObjectType</skos:editorialNote>
	<skos:scopeNote xml:lang="en">Screens used to shelter the face or legs from the heat of a fire. Often includes a decorated panel or panels.</skos:scopeNote>
</skos:Concept>
<skos:Concept rdf:about="http://partage.vocnet.org/part00304">
	<skos:prefLabel xml:lang="en">folding screens</skos:prefLabel>
	<skos:prefLabel xml:lang="sv">vikskärmar</skos:prefLabel>
	<skos:prefLabel xml:lang="pt">biombos</skos:prefLabel>
	<skos:prefLabel xml:lang="de">Stellschirm</skos:prefLabel>
	<skos:altLabel xml:lang="de">Raumteiler</skos:altLabel>
	<skos:altLabel xml:lang="de">Faltwand</skos:altLabel>
	<skos:prefLabel xml:lang="hr">sklopivi zasloni</skos:prefLabel>
	<skos:prefLabel xml:lang="fi">väliseinät</skos:prefLabel>
	<skos:inScheme rdf:resource="http://partage.vocnet.org/Objects"/>
	<skos:broader rdf:resource="http://partage.vocnet.org/part00102"/>
	<skos:exactMatch rdf:resource="http://vocab.getty.edu/aat/300265156"/>
	<skos:editorialNote xml:lang="en">PPRefiningObjectType</skos:editorialNote>
	<skos:scopeNote xml:lang="en">Refers to screens comprised of two or more panels, typically decorated and often lacquered. Invented by the Chinese, the form was mentioned as early as the 2nd century BCE. The earliest surviving examples date to the MIng dynasty. Folding screens were introduced to Japan from China in the 8th century; such screens were often designed in pairs in Japan. From the early 17th century eastern folding screens were imported to Europe and the form was soon adopted by European craftsmen. European folding screens, like those of Japan, were usually composed of six panels but were often taller and more substantial.</skos:scopeNote>
</skos:Concept>
<skos:Concept rdf:about="http://partage.vocnet.org/part00305">
	<skos:altLabel xml:lang="en">buffets (sideboards)</skos:altLabel>
	<skos:prefLabel xml:lang="en">buffets</skos:prefLabel>
	<skos:prefLabel xml:lang="sv">bufféer</skos:prefLabel>
	<skos:prefLabel xml:lang="pt">consola</skos:prefLabel>
	<skos:altLabel xml:lang="de">Speiseschrank</skos:altLabel>
	<skos:altLabel xml:lang="de">Anrichte</skos:altLabel>
	<skos:altLabel xml:lang="de">Buffet</skos:altLabel>
	<skos:prefLabel xml:lang="de">Büffet</skos:prefLabel>
	<skos:prefLabel xml:lang="hr">buffet</skos:prefLabel>
	<skos:prefLabel xml:lang="fi">tarjoilupöydät</skos:prefLabel>
	<skos:inScheme rdf:resource="http://partage.vocnet.org/Objects"/>
	<skos:broader rdf:resource="http://partage.vocnet.org/part00299"/>
	<skos:exactMatch rdf:resource="http://vocab.getty.edu/aat/300172119"/>
	<skos:editorialNote xml:lang="en">PPRefiningObjectType</skos:editorialNote>
	<skos:scopeNote xml:lang="en">Refers to any piece of dining room furniture having compartments or shelves for holding articles of table service below a surface for serving or preparing food. The term has been in use since the 16th century. Its usage often overlaps with "sideboards," although buffets tend to be large enough to hold platters and serving dishes, and may have relatively tall legs, very short legs, or a solid base.</skos:scopeNote>
</skos:Concept>
<skos:Concept rdf:about="http://partage.vocnet.org/part00306">
	<skos:prefLabel xml:lang="en">seating furniture</skos:prefLabel>
	<skos:prefLabel xml:lang="hr">namještaj za sjedenje</skos:prefLabel>
	<skos:prefLabel xml:lang="pt">móveis de assento</skos:prefLabel>
	<skos:prefLabel xml:lang="de">Sitzmöbel</skos:prefLabel>
	<skos:prefLabel xml:lang="sv">sittmöbler</skos:prefLabel>
	<skos:prefLabel xml:lang="fi">istuinhuonekalut</skos:prefLabel>
	<skos:inScheme rdf:resource="http://partage.vocnet.org/Objects"/>
	<skos:broader rdf:resource="http://partage.vocnet.org/part00099"/>
	<skos:narrower rdf:resource="http://partage.vocnet.org/part00308"/>
	<skos:narrower rdf:resource="http://partage.vocnet.org/part00309"/>
	<skos:narrower rdf:resource="http://partage.vocnet.org/part00311"/>
	<skos:narrower rdf:resource="http://partage.vocnet.org/part00312"/>
	<skos:exactMatch rdf:resource="http://vocab.getty.edu/aat/300037769"/>
	<skos:editorialNote xml:lang="en">PPRefiningObjectType</skos:editorialNote>
	<skos:scopeNote xml:lang="en">no scope note in AAT</skos:scopeNote>
</skos:Concept>
<skos:Concept rdf:about="http://partage.vocnet.org/part00308">
	<skos:altLabel xml:lang="en">chairs (furniture forms)</skos:altLabel>
	<skos:prefLabel xml:lang="en">chairs</skos:prefLabel>
	<skos:prefLabel xml:lang="sv">stolar</skos:prefLabel>
	<skos:prefLabel xml:lang="pt">cadeiras</skos:prefLabel>
	<skos:altLabel xml:lang="de">Sessel</skos:altLabel>
	<skos:altLabel xml:lang="de">Stühle</skos:altLabel>
	<skos:prefLabel xml:lang="de">Stuhl</skos:prefLabel>
	<skos:prefLabel xml:lang="hr">stolac</skos:prefLabel>
	<skos:prefLabel xml:lang="fi">tuolit</skos:prefLabel>
	<skos:inScheme rdf:resource="http://partage.vocnet.org/Objects"/>
	<skos:broader rdf:resource="http://partage.vocnet.org/part00306"/>
	<skos:narrower rdf:resource="http://partage.vocnet.org/part00807"/>
	<skos:exactMatch rdf:resource="http://vocab.getty.edu/aat/300037772"/>
	<skos:editorialNote xml:lang="en">PPRefiningObjectType</skos:editorialNote>
	<skos:scopeNote xml:lang="en">Seats for one person with a back or a back and arms. Distinct from "stools" which have no back.</skos:scopeNote>
</skos:Concept>
<skos:Concept rdf:about="http://partage.vocnet.org/part00309">
	<skos:altLabel xml:lang="en">stools (seating furniture)</skos:altLabel>
	<skos:prefLabel xml:lang="en">stools</skos:prefLabel>
	<skos:prefLabel xml:lang="sv">pallar</skos:prefLabel>
	<skos:prefLabel xml:lang="hr">stolac bez naslona</skos:prefLabel>
	<skos:altLabel xml:lang="pt">bancos</skos:altLabel>
	<skos:prefLabel xml:lang="pt">banco.</skos:prefLabel>
	<skos:prefLabel xml:lang="de">Hocker</skos:prefLabel>
	<skos:prefLabel xml:lang="fi">jakkarat</skos:prefLabel>
	<skos:inScheme rdf:resource="http://partage.vocnet.org/Objects"/>
	<skos:broader rdf:resource="http://partage.vocnet.org/part00306"/>
	<skos:narrower rdf:resource="http://partage.vocnet.org/part00806"/>
	<skos:exactMatch rdf:resource="http://vocab.getty.edu/aat/300038418"/>
	<skos:editorialNote xml:lang="en">PPRefiningObjectType</skos:editorialNote>
	<skos:scopeNote xml:lang="en">A seat for one person, often without a back. They were the most common type of seat furniture until the 19th century. Distinct from "benches" in that they seat only one person; usually distinguished from "chairs" in that they have no back; however, tall seating pieces at a bar or counter are called stools though they sometimes have backs. Generally made in two types; one supported on four straight legs and the other with legs arranged crosswise.</skos:scopeNote>
</skos:Concept>
<skos:Concept rdf:about="http://partage.vocnet.org/part00311">
	<skos:altLabel xml:lang="en">benches (furniture)</skos:altLabel>
	<skos:prefLabel xml:lang="en">benches</skos:prefLabel>
	<skos:prefLabel xml:lang="hr">klupa</skos:prefLabel>
	<skos:prefLabel xml:lang="pt">banco..</skos:prefLabel>
	<skos:altLabel xml:lang="de">Bänke</skos:altLabel>
	<skos:prefLabel xml:lang="de">Bank (Sitzmöbel)</skos:prefLabel>
	<skos:prefLabel xml:lang="sv">bänkar</skos:prefLabel>
	<skos:prefLabel xml:lang="fi">penkit</skos:prefLabel>
	<skos:inScheme rdf:resource="http://partage.vocnet.org/Objects"/>
	<skos:broader rdf:resource="http://partage.vocnet.org/part00306"/>
	<skos:exactMatch rdf:resource="http://vocab.getty.edu/aat/300038494"/>
	<skos:editorialNote xml:lang="en">PPRefiningObjectType</skos:editorialNote>
	<skos:scopeNote xml:lang="en">Long seats for two or more people, with or without a back, usually of wood, but also of stone, metal, or another material. A bench is distinguished from a stool by its greater length.</skos:scopeNote>
</skos:Concept>
<skos:Concept rdf:about="http://partage.vocnet.org/part00312">
	<skos:prefLabel xml:lang="en">sofas</skos:prefLabel>
	<skos:prefLabel xml:lang="sv">soffor</skos:prefLabel>
	<skos:prefLabel xml:lang="hr">sofa</skos:prefLabel>
	<skos:altLabel xml:lang="pt">sofás</skos:altLabel>
	<skos:prefLabel xml:lang="pt">sofá</skos:prefLabel>
	<skos:altLabel xml:lang="de">Sofas</skos:altLabel>
	<skos:altLabel xml:lang="de">Couch</skos:altLabel>
	<skos:prefLabel xml:lang="de">Sofa</skos:prefLabel>
	<skos:prefLabel xml:lang="fi">sohvat</skos:prefLabel>
	<skos:inScheme rdf:resource="http://partage.vocnet.org/Objects"/>
	<skos:broader rdf:resource="http://partage.vocnet.org/part00306"/>
	<skos:exactMatch rdf:resource="http://vocab.getty.edu/aat/300038634"/>
	<skos:editorialNote xml:lang="en">PPRefiningObjectType</skos:editorialNote>
	<skos:scopeNote xml:lang="en">Long, upholstered seating objects with a back and two ends, and primarily used for sitting rather than reclining. Distinct from "couches (reclining furniture)" which have a back support and one end and are primarily used for reclining rather than sitting. The term "sofa" was first used in France at the end of the 17th century as an alternative for canap\u00e9. The terms sofa and settee are virtually interchangeable in 20th-century usage but there is a distinction between the two; a sofa is generally completely upholstered</skos:scopeNote>
</skos:Concept>
<skos:Concept rdf:about="http://partage.vocnet.org/part00314">
	<skos:altLabel xml:lang="en">beds (furniture)</skos:altLabel>
	<skos:prefLabel xml:lang="en">beds</skos:prefLabel>
	<skos:prefLabel xml:lang="sv">sängar</skos:prefLabel>
	<skos:prefLabel xml:lang="pt">cama</skos:prefLabel>
	<skos:altLabel xml:lang="de">Betten</skos:altLabel>
	<skos:prefLabel xml:lang="de">Bett</skos:prefLabel>
	<skos:prefLabel xml:lang="hr">krevet</skos:prefLabel>
	<skos:prefLabel xml:lang="fi">sängyt</skos:prefLabel>
	<skos:inScheme rdf:resource="http://partage.vocnet.org/Objects"/>
	<skos:broader rdf:resource="http://partage.vocnet.org/part00099"/>
	<skos:narrower rdf:resource="http://partage.vocnet.org/part00884"/>
	<skos:exactMatch rdf:resource="http://vocab.getty.edu/aat/300038697"/>
	<skos:editorialNote xml:lang="en">PPRefiningObjectType</skos:editorialNote>
	<skos:scopeNote xml:lang="en">Generally, the sleeping places of humans and animals. Specifically, permanent pieces of furniture comprised of a bedstead, which is the wooden or metal support, and the bedding, including the mattress and cover.</skos:scopeNote>
</skos:Concept>
<skos:Concept rdf:about="http://partage.vocnet.org/part00315">
	<skos:prefLabel xml:lang="en">desks</skos:prefLabel>
	<skos:prefLabel xml:lang="pt">secretária</skos:prefLabel>
	<skos:altLabel xml:lang="de">Schreibtische</skos:altLabel>
	<skos:prefLabel xml:lang="de">Schreibtisch</skos:prefLabel>
	<skos:prefLabel xml:lang="sv">skrivbord</skos:prefLabel>
	<skos:prefLabel xml:lang="hr">radni stol</skos:prefLabel>
	<skos:prefLabel xml:lang="fi">kirjoituspöydät</skos:prefLabel>
	<skos:inScheme rdf:resource="http://partage.vocnet.org/Objects"/>
	<skos:broader rdf:resource="http://partage.vocnet.org/part00299"/>
	<skos:exactMatch rdf:resource="http://vocab.getty.edu/aat/300039338"/>
	<skos:editorialNote xml:lang="en">PPRefiningObjectType</skos:editorialNote>
	<skos:scopeNote xml:lang="en">Various forms of furniture for readers or writers, generally having a flat writing surface and often drawers and other compartments.</skos:scopeNote>
</skos:Concept>
<skos:Concept rdf:about="http://partage.vocnet.org/part00316">
	<skos:altLabel xml:lang="en">tables (support furniture)</skos:altLabel>
	<skos:prefLabel xml:lang="en">tables</skos:prefLabel>
	<skos:prefLabel xml:lang="sv">bord</skos:prefLabel>
	<skos:prefLabel xml:lang="hr">stol</skos:prefLabel>
	<skos:prefLabel xml:lang="pt">mesa</skos:prefLabel>
	<skos:prefLabel xml:lang="de">Tisch</skos:prefLabel>
	<skos:altLabel xml:lang="de">Tische</skos:altLabel>
	<skos:prefLabel xml:lang="fi">pöydät</skos:prefLabel>
	<skos:inScheme rdf:resource="http://partage.vocnet.org/Objects"/>
	<skos:broader rdf:resource="http://partage.vocnet.org/part00099"/>
	<skos:narrower rdf:resource="http://partage.vocnet.org/part00798"/>
	<skos:narrower rdf:resource="http://partage.vocnet.org/part01143"/>
	<skos:exactMatch rdf:resource="http://vocab.getty.edu/aat/300039548"/>
	<skos:editorialNote xml:lang="en">PPRefiningObjectType</skos:editorialNote>
	<skos:scopeNote xml:lang="en">Articles of furniture consisting of a flat, slablike top supported on one or more legs or supports.</skos:scopeNote>
</skos:Concept>
<skos:Concept rdf:about="http://partage.vocnet.org/part00318">
	<skos:altLabel xml:lang="en">boxes (containers)</skos:altLabel>
	<skos:prefLabel xml:lang="en">boxes</skos:prefLabel>
	<skos:prefLabel xml:lang="sv">lådor</skos:prefLabel>
	<skos:prefLabel xml:lang="pt">caixa</skos:prefLabel>
	<skos:altLabel xml:lang="de">Kästen</skos:altLabel>
	<skos:altLabel xml:lang="de">Kasten</skos:altLabel>
	<skos:altLabel xml:lang="de">Schachteln</skos:altLabel>
	<skos:prefLabel xml:lang="de">Schachtel</skos:prefLabel>
	<skos:prefLabel xml:lang="hr">kutija</skos:prefLabel>
	<skos:prefLabel xml:lang="fi">laatikot</skos:prefLabel>
	<skos:inScheme rdf:resource="http://partage.vocnet.org/Objects"/>
	<skos:broader rdf:resource="http://partage.vocnet.org/part00085"/>
	<skos:narrower rdf:resource="http://partage.vocnet.org/part01184"/>
	<skos:exactMatch rdf:resource="http://vocab.getty.edu/aat/300045643"/>
	<skos:editorialNote xml:lang="en">PPRefiningObjectType</skos:editorialNote>
	<skos:scopeNote xml:lang="en">Rigid, often rectangular containers usually with a lid or cover in which something nonliquid is kept or carried.</skos:scopeNote>
</skos:Concept>
<skos:Concept rdf:about="http://partage.vocnet.org/part00319">
	<skos:altLabel xml:lang="en">cans (containers)</skos:altLabel>
	<skos:prefLabel xml:lang="en">cans</skos:prefLabel>
	<skos:prefLabel xml:lang="sv">burkar</skos:prefLabel>
	<skos:prefLabel xml:lang="pt">lata</skos:prefLabel>
	<skos:altLabel xml:lang="de">Dosen</skos:altLabel>
	<skos:prefLabel xml:lang="de">Dose</skos:prefLabel>
	<skos:prefLabel xml:lang="hr">limenka</skos:prefLabel>
	<skos:prefLabel xml:lang="fi">tölkit</skos:prefLabel>
	<skos:inScheme rdf:resource="http://partage.vocnet.org/Objects"/>
	<skos:broader rdf:resource="http://partage.vocnet.org/part00085"/>
	<skos:exactMatch rdf:resource="http://vocab.getty.edu/aat/300045657"/>
	<skos:editorialNote xml:lang="en">PPRefiningObjectType</skos:editorialNote>
	<skos:scopeNote xml:lang="en">Sealed metal containers for food or beverages. Also, other containers for holding or carrying liquids, such as oilcans, and metal or plastic containers for holding film on cores or reels.</skos:scopeNote>
</skos:Concept>
<skos:Concept rdf:about="http://partage.vocnet.org/part00320">
	<skos:prefLabel xml:lang="en">cases (containers)</skos:prefLabel>
	<skos:prefLabel xml:lang="sv">lådor.</skos:prefLabel>
	<skos:prefLabel xml:lang="pt">estojo</skos:prefLabel>
	<skos:prefLabel xml:lang="de">Behälter.</skos:prefLabel>
	<skos:prefLabel xml:lang="hr">spremnik</skos:prefLabel>
	<skos:prefLabel xml:lang="fi">laatikot.</skos:prefLabel>
	<skos:inScheme rdf:resource="http://partage.vocnet.org/Objects"/>
	<skos:broader rdf:resource="http://partage.vocnet.org/part00085"/>
	<skos:exactMatch rdf:resource="http://vocab.getty.edu/aat/300045659"/>
	<skos:editorialNote xml:lang="en">PPRefiningObjectType</skos:editorialNote>
	<skos:scopeNote xml:lang="en">A receptacle, holder, box, chest, bag, sheath, or covering fitted to contain or enclose something else; typically used for transporting or protecting the enclosed item or items.</skos:scopeNote>
</skos:Concept>
<skos:Concept rdf:about="http://partage.vocnet.org/part00321">
	<skos:altLabel xml:lang="en">bowls (vessels)</skos:altLabel>
	<skos:prefLabel xml:lang="en">bowls</skos:prefLabel>
	<skos:prefLabel xml:lang="sv">skålar</skos:prefLabel>
	<skos:prefLabel xml:lang="pt">taça</skos:prefLabel>
	<skos:altLabel xml:lang="de">Schüsseln</skos:altLabel>
	<skos:prefLabel xml:lang="de">Schüssel</skos:prefLabel>
	<skos:prefLabel xml:lang="hr">zdjela</skos:prefLabel>
	<skos:prefLabel xml:lang="fi">maljat</skos:prefLabel>
	<skos:inScheme rdf:resource="http://partage.vocnet.org/Objects"/>
	<skos:broader rdf:resource="http://partage.vocnet.org/part00083"/>
	<skos:narrower rdf:resource="http://partage.vocnet.org/part01136"/>
	<skos:exactMatch rdf:resource="http://vocab.getty.edu/aat/300203596"/>
	<skos:editorialNote xml:lang="en">PPRefiningObjectType</skos:editorialNote>
	<skos:scopeNote xml:lang="en">Rounded vessels that are generally wider than they are high, usually hemispherical or nearly so. A bowl may have a spreading base or foot ring and sometimes two handles or a cover. Distinguished from a cup, which is rather deep than wide.</skos:scopeNote>
</skos:Concept>
<skos:Concept rdf:about="http://partage.vocnet.org/part00322">
	<skos:prefLabel xml:lang="en">jars</skos:prefLabel>
	<skos:prefLabel xml:lang="hr">staklenka</skos:prefLabel>
	<skos:altLabel xml:lang="de">Dosen.</skos:altLabel>
	<skos:altLabel xml:lang="de">Vorratsgefäße</skos:altLabel>
	<skos:altLabel xml:lang="de">Vorratsgefäß</skos:altLabel>
	<skos:prefLabel xml:lang="de">Dose.</skos:prefLabel>
	<skos:prefLabel xml:lang="sv">burkar.</skos:prefLabel>
	<skos:prefLabel xml:lang="pt">frasco</skos:prefLabel>
	<skos:prefLabel xml:lang="fi">ruukut</skos:prefLabel>
	<skos:inScheme rdf:resource="http://partage.vocnet.org/Objects"/>
	<skos:broader rdf:resource="http://partage.vocnet.org/part00083"/>
	<skos:exactMatch rdf:resource="http://vocab.getty.edu/aat/300195347"/>
	<skos:editorialNote xml:lang="en">PPRefiningObjectType</skos:editorialNote>
	<skos:scopeNote xml:lang="en">Deep, wide-mouthed vessels used for holding a variety of substances, usually without handles and generally cylindrical, although sometimes made in other shapes. For narrower-necked vessles, use "bottles."</skos:scopeNote>
</skos:Concept>
<skos:Concept rdf:about="http://partage.vocnet.org/part00323">
	<skos:altLabel xml:lang="en">jugs (vessels)</skos:altLabel>
	<skos:prefLabel xml:lang="en">jugs</skos:prefLabel>
	<skos:prefLabel xml:lang="hr">vrč</skos:prefLabel>
	<skos:altLabel xml:lang="de">Krüge</skos:altLabel>
	<skos:altLabel xml:lang="de">Kannen</skos:altLabel>
	<skos:altLabel xml:lang="de">Krug</skos:altLabel>
	<skos:prefLabel xml:lang="de">Kanne</skos:prefLabel>
	<skos:prefLabel xml:lang="sv">tillbringare</skos:prefLabel>
	<skos:altLabel xml:lang="pt">caneca</skos:altLabel>
	<skos:prefLabel xml:lang="pt">jarro.</skos:prefLabel>
	<skos:prefLabel xml:lang="fi">kannut.</skos:prefLabel>
	<skos:inScheme rdf:resource="http://partage.vocnet.org/Objects"/>
	<skos:broader rdf:resource="http://partage.vocnet.org/part00083"/>
	<skos:exactMatch rdf:resource="http://vocab.getty.edu/aat/300045685"/>
	<skos:editorialNote xml:lang="en">PPRefiningObjectType</skos:editorialNote>
	<skos:scopeNote xml:lang="en">Vessels, generally made of earthenware, stoneware or porcelain and often of large capacity, which have a narrow neck and a handle (usually a vertical loop or scroll handle); may sometimes have a pouring lip.</skos:scopeNote>
</skos:Concept>
<skos:Concept rdf:about="http://partage.vocnet.org/part00325">
	<skos:prefLabel xml:lang="en">urns</skos:prefLabel>
	<skos:prefLabel xml:lang="sv">urnor</skos:prefLabel>
	<skos:prefLabel xml:lang="hr">urna</skos:prefLabel>
	<skos:altLabel xml:lang="pt">urnas</skos:altLabel>
	<skos:prefLabel xml:lang="pt">urna</skos:prefLabel>
	<skos:altLabel xml:lang="de">Urnen</skos:altLabel>
	<skos:prefLabel xml:lang="de">Urne</skos:prefLabel>
	<skos:prefLabel xml:lang="fi">uurnat</skos:prefLabel>
	<skos:inScheme rdf:resource="http://partage.vocnet.org/Objects"/>
	<skos:broader rdf:resource="http://partage.vocnet.org/part00083"/>
	<skos:exactMatch rdf:resource="http://vocab.getty.edu/aat/300129425"/>
	<skos:editorialNote xml:lang="en">PPRefiningObjectType</skos:editorialNote>
	<skos:scopeNote xml:lang="en">Large or decorative vessels, especially ones with an ornamental foot or pedestal, that usually have a mouth that is smaller than the body, and which often have two side handles.</skos:scopeNote>
</skos:Concept>
<skos:Concept rdf:about="http://partage.vocnet.org/part00326">
	<skos:prefLabel xml:lang="en">vases</skos:prefLabel>
	<skos:prefLabel xml:lang="sv">vaser</skos:prefLabel>
	<skos:prefLabel xml:lang="hr">vaza</skos:prefLabel>
	<skos:altLabel xml:lang="pt">vasos</skos:altLabel>
	<skos:prefLabel xml:lang="pt">vaso</skos:prefLabel>
	<skos:altLabel xml:lang="de">Vasen</skos:altLabel>
	<skos:prefLabel xml:lang="de">Vase</skos:prefLabel>
	<skos:prefLabel xml:lang="fi">maljakot</skos:prefLabel>
	<skos:inScheme rdf:resource="http://partage.vocnet.org/Objects"/>
	<skos:broader rdf:resource="http://partage.vocnet.org/part00083"/>
	<skos:exactMatch rdf:resource="http://vocab.getty.edu/aat/300132254"/>
	<skos:editorialNote xml:lang="en">PPRefiningObjectType</skos:editorialNote>
	<skos:scopeNote xml:lang="en">Vessels of varying shape and size but which are usually taller than they are wide, varying greatly in actual form and use. In modern usage, typically refers to vessels for displaying flowers. When referring to ancient art, often refers to any ceramic or metal vessel in a range of shapes and used to hold liquids, grain, or another substance.</skos:scopeNote>
</skos:Concept>
<skos:Concept rdf:about="http://partage.vocnet.org/part00327">
	<skos:prefLabel xml:lang="en">vials</skos:prefLabel>
	<skos:prefLabel xml:lang="sv">medicinflaskor</skos:prefLabel>
	<skos:prefLabel xml:lang="hr">fijala</skos:prefLabel>
	<skos:prefLabel xml:lang="pt">frasco.</skos:prefLabel>
	<skos:altLabel xml:lang="de">Ampullen</skos:altLabel>
	<skos:altLabel xml:lang="de">Phiolen</skos:altLabel>
	<skos:prefLabel xml:lang="de">Ampulle</skos:prefLabel>
	<skos:prefLabel xml:lang="fi">lääkepullot</skos:prefLabel>
	<skos:inScheme rdf:resource="http://partage.vocnet.org/Objects"/>
	<skos:broader rdf:resource="http://partage.vocnet.org/part00083"/>
	<skos:exactMatch rdf:resource="http://vocab.getty.edu/aat/300198822"/>
	<skos:editorialNote xml:lang="en">PPRefiningObjectType</skos:editorialNote>
	<skos:scopeNote xml:lang="en">Small or moderate-sized vessels mainly for medicinal and toilet preparations.</skos:scopeNote>
</skos:Concept>
<skos:Concept rdf:about="http://partage.vocnet.org/part00330">
	<skos:prefLabel xml:lang="en">candleholders</skos:prefLabel>
	<skos:prefLabel xml:lang="sv">ljushållare</skos:prefLabel>
	<skos:prefLabel xml:lang="pt">castiçal</skos:prefLabel>
	<skos:altLabel xml:lang="de">Kerzenhalter</skos:altLabel>
	<skos:altLabel xml:lang="de">Kerzenleuchter</skos:altLabel>
	<skos:prefLabel xml:lang="de">Leuchter</skos:prefLabel>
	<skos:prefLabel xml:lang="hr">svijećnjak</skos:prefLabel>
	<skos:prefLabel xml:lang="fi">kyntteliköt</skos:prefLabel>
	<skos:inScheme rdf:resource="http://partage.vocnet.org/Objects"/>
	<skos:broader rdf:resource="http://partage.vocnet.org/part00109"/>
	<skos:narrower rdf:resource="http://partage.vocnet.org/part00792"/>
	<skos:narrower rdf:resource="http://partage.vocnet.org/part00793"/>
	<skos:exactMatch rdf:resource="http://vocab.getty.edu/aat/300037583"/>
	<skos:scopeNote xml:lang="en">Term generally applied to a variety of devices having either a single spike or one or more candle sockets to hold candles; sometimes having drips to catch wax, push-ups and other devices for removing the stub, or adjustable features for controlling the position of the flame. For lamps using candles as the source of illumination and containing the candle within a vessel, use "candle lamps."</skos:scopeNote>
	<skos:editorialNote xml:lang="en">PPRefiningObjectType</skos:editorialNote>
</skos:Concept>
<skos:Concept rdf:about="http://partage.vocnet.org/part00331">
	<skos:altLabel xml:lang="en">chandeliers (hanging lights)</skos:altLabel>
	<skos:prefLabel xml:lang="en">chandeliers</skos:prefLabel>
	<skos:prefLabel xml:lang="sv">ljuskronor</skos:prefLabel>
	<skos:prefLabel xml:lang="pt">lustre</skos:prefLabel>
	<skos:altLabel xml:lang="de">Lüster.</skos:altLabel>
	<skos:prefLabel xml:lang="de">Kronleuchter</skos:prefLabel>
	<skos:prefLabel xml:lang="hr">luster.</skos:prefLabel>
	<skos:prefLabel xml:lang="fi">kattokruunut</skos:prefLabel>
	<skos:inScheme rdf:resource="http://partage.vocnet.org/Objects"/>
	<skos:broader rdf:resource="http://partage.vocnet.org/part00109"/>
	<skos:exactMatch rdf:resource="http://vocab.getty.edu/aat/300037622"/>
	<skos:scopeNote xml:lang="en">Lighting devices designed to hang from the roof or ceiling having two or more branches, holding candles, burners, or lamps; often ornamental.</skos:scopeNote>
	<skos:editorialNote xml:lang="en">PPRefiningObjectType</skos:editorialNote>
</skos:Concept>
<skos:Concept rdf:about="http://partage.vocnet.org/part00332">
	<skos:altLabel xml:lang="en">lamps (lighting devices)</skos:altLabel>
	<skos:prefLabel xml:lang="en">lamps</skos:prefLabel>
	<skos:prefLabel xml:lang="hr">svjetiljka</skos:prefLabel>
	<skos:altLabel xml:lang="de">Lampen (Leuchten)</skos:altLabel>
	<skos:altLabel xml:lang="de">Leuchten.</skos:altLabel>
	<skos:altLabel xml:lang="de">Lampe (Leuchte)</skos:altLabel>
	<skos:prefLabel xml:lang="de">Leuchte</skos:prefLabel>
	<skos:prefLabel xml:lang="sv">lampor</skos:prefLabel>
	<skos:prefLabel xml:lang="pt">candeeiro.</skos:prefLabel>
	<skos:prefLabel xml:lang="fi">lamput</skos:prefLabel>
	<skos:inScheme rdf:resource="http://partage.vocnet.org/Objects"/>
	<skos:broader rdf:resource="http://partage.vocnet.org/part00109"/>
	<skos:narrower rdf:resource="http://partage.vocnet.org/part00334"/>
	<skos:narrower rdf:resource="http://partage.vocnet.org/part00338"/>
	<skos:narrower rdf:resource="http://partage.vocnet.org/part00339"/>
	<skos:exactMatch rdf:resource="http://vocab.getty.edu/aat/300037592"/>
	<skos:editorialNote xml:lang="en">PPRefiningObjectType</skos:editorialNote>
	<skos:scopeNote xml:lang="en">Lighting devices having a vessel to contain fuel used as a source of illumination, such as grease or oil. The term also refers to relatively small -- of a size to be placed on or beside a desk or table -- household or office lighting devices that incorporate a vessel of glass or some similar material that encloses the source of illumination, whether a candle, oil, gas-jet, or incandescent wire inside a light bulb. The lamp was invented at least as early as 70,000 BCE, originally consisting of a hollowed-out rock filled with moss or some other absorbent material that was soaked with animal fat and ignited. To refer to the glass bulbs used as a component of electric lamps, use "light bulbs."</skos:scopeNote>
</skos:Concept>
<skos:Concept rdf:about="http://partage.vocnet.org/part00334">
	<skos:prefLabel xml:lang="en">Tiffany lamps</skos:prefLabel>
	<skos:prefLabel xml:lang="sv">tiffanylampor</skos:prefLabel>
	<skos:prefLabel xml:lang="hr">Tiffany svjetiljka</skos:prefLabel>
	<skos:prefLabel xml:lang="pt">candeeiro Tiffany</skos:prefLabel>
	<skos:altLabel xml:lang="de">Tiffany-Lampen</skos:altLabel>
	<skos:prefLabel xml:lang="de">Tiffany-Lampe</skos:prefLabel>
	<skos:prefLabel xml:lang="fi">tiffany-valaisimet</skos:prefLabel>
	<skos:inScheme rdf:resource="http://partage.vocnet.org/Objects"/>
	<skos:broader rdf:resource="http://partage.vocnet.org/part00332"/>
	<skos:exactMatch rdf:resource="http://vocab.getty.edu/aat/300183168"/>
	<skos:editorialNote xml:lang="en">PPRefiningObjectType</skos:editorialNote>
	<skos:scopeNote xml:lang="en">Lamps produced by Tiffany Studios beginning in 1895 having shades made of various types of stained glass, sometimes set in intricate leaded patterns. Other lamps have shades resembling flowers made of iridescent glass.</skos:scopeNote>
</skos:Concept>
<skos:Concept rdf:about="http://partage.vocnet.org/part00335">
	<skos:altLabel xml:lang="en">lusters (lighting devices)</skos:altLabel>
	<skos:prefLabel xml:lang="en">lusters</skos:prefLabel>
	<skos:prefLabel xml:lang="hr">luster</skos:prefLabel>
	<skos:prefLabel xml:lang="de">Lüster</skos:prefLabel>
	<skos:altLabel xml:lang="de">Kristallkronleuchter</skos:altLabel>
	<skos:prefLabel xml:lang="sv">lystrar</skos:prefLabel>
	<skos:altLabel xml:lang="pt">candelabro</skos:altLabel>
	<skos:prefLabel xml:lang="pt">lustre.</skos:prefLabel>
	<skos:prefLabel xml:lang="fi">seinäkyntteliköt</skos:prefLabel>
	<skos:altLabel xml:lang="fi">kristallikoristeinen</skos:altLabel>
	<skos:inScheme rdf:resource="http://partage.vocnet.org/Objects"/>
	<skos:broader rdf:resource="http://partage.vocnet.org/part00109"/>
	<skos:exactMatch rdf:resource="http://vocab.getty.edu/aat/300196169"/>
	<skos:editorialNote xml:lang="en">PPRefiningObjectType</skos:editorialNote>
	<skos:scopeNote xml:lang="en">Period term for lighting devices, such as chandeliers and candelabras, made of glass or ornamented with glass pendants.</skos:scopeNote>
</skos:Concept>
<skos:Concept rdf:about="http://partage.vocnet.org/part00338">
	<skos:prefLabel xml:lang="en">wall lamps</skos:prefLabel>
	<skos:prefLabel xml:lang="sv">vägglampor</skos:prefLabel>
	<skos:prefLabel xml:lang="hr">zidne svjetiljke</skos:prefLabel>
	<skos:prefLabel xml:lang="pt">candeeiro de parede</skos:prefLabel>
	<skos:altLabel xml:lang="de">Wandlampen</skos:altLabel>
	<skos:altLabel xml:lang="de">Wandlampe</skos:altLabel>
	<skos:altLabel xml:lang="de">Wandleuchten</skos:altLabel>
	<skos:prefLabel xml:lang="de">Wandleuchte</skos:prefLabel>
	<skos:prefLabel xml:lang="fi">seinävalaisimet</skos:prefLabel>
	<skos:inScheme rdf:resource="http://partage.vocnet.org/Objects"/>
	<skos:broader rdf:resource="http://partage.vocnet.org/part00332"/>
	<skos:exactMatch rdf:resource="http://vocab.getty.edu/aat/300037646"/>
	<skos:editorialNote xml:lang="en">PPRefiningObjectType</skos:editorialNote>
	<skos:scopeNote xml:lang="en">Any lamp (lighting device) intended to be hung on the wall. Use "brackets (lighting devices)" for wall lamps attached to or suspended from some form of bracket, by means of which it can be hung on the wall</skos:scopeNote>
</skos:Concept>
<skos:Concept rdf:about="http://partage.vocnet.org/part00339">
	<skos:prefLabel xml:lang="en">table lamps</skos:prefLabel>
	<skos:prefLabel xml:lang="sv">bordslampor</skos:prefLabel>
	<skos:prefLabel xml:lang="hr">stolna svjetiljka</skos:prefLabel>
	<skos:prefLabel xml:lang="pl">candeeiro de mesa</skos:prefLabel>
	<skos:altLabel xml:lang="de">Tischlampen</skos:altLabel>
	<skos:prefLabel xml:lang="de">Tischlampe</skos:prefLabel>
	<skos:prefLabel xml:lang="fi">pöytävalaisimet</skos:prefLabel>
	<skos:inScheme rdf:resource="http://partage.vocnet.org/Objects"/>
	<skos:broader rdf:resource="http://partage.vocnet.org/part00332"/>
	<skos:exactMatch rdf:resource="http://vocab.getty.edu/aat/300037644"/>
	<skos:editorialNote xml:lang="en">PPRefiningObjectType</skos:editorialNote>
	<skos:scopeNote xml:lang="en">Lamps with a relatively short stem making them suitable for standing on tables and other furniture. The term is especially used in reference to late 18th-century lamps designed to burn whale oil and burning fluid compounds, which generally maintain the traditional stemware divisions of top, stem, and foot and often resemble stemmed drinking glasses of the same period.</skos:scopeNote>
</skos:Concept>
<skos:Concept rdf:about="http://partage.vocnet.org/part00396">
	<skos:altLabel xml:lang="en">dishes (vessels)</skos:altLabel>
	<skos:prefLabel xml:lang="en">dishes</skos:prefLabel>
	<skos:prefLabel xml:lang="pt">pratos</skos:prefLabel>
	<skos:altLabel xml:lang="de">Platten (Geschirr)</skos:altLabel>
	<skos:altLabel xml:lang="de">Platte (Eßgeschirr)</skos:altLabel>
	<skos:prefLabel xml:lang="sv">tallrikar</skos:prefLabel>
	<skos:prefLabel xml:lang="hr">posuđe.</skos:prefLabel>
	<skos:altLabel xml:lang="de">Schalen (Gefäße)</skos:altLabel>
	<skos:prefLabel xml:lang="de">Schale (Gefäß)</skos:prefLabel>
	<skos:prefLabel xml:lang="fi">astiat</skos:prefLabel>
	<skos:inScheme rdf:resource="http://partage.vocnet.org/Objects"/>
	<skos:broader rdf:resource="http://partage.vocnet.org/part00085"/>
	<skos:narrower rdf:resource="http://partage.vocnet.org/part00400"/>
	<skos:exactMatch rdf:resource="http://vocab.getty.edu/aat/300042973"/>
	<skos:editorialNote xml:lang="en">PPRefiningObjectType</skos:editorialNote>
	<skos:scopeNote xml:lang="en">Any of various broad, relatively shallow, open vessels with a flat bottom, concave sides, and nearly level rim, sometimes having a cover; made of pottery, glass, metal, wood or another material and used for many purposes, especially for holding or serving food. In modern usage it is typically reserved for vessels at a dining table used for serving or holding food other than the round, flat or very shallow object used by the person dining, which is called a "plate"; however, formerly the plate was also called a "dish."</skos:scopeNote>
</skos:Concept>
<skos:Concept rdf:about="http://partage.vocnet.org/part00400">
	<skos:prefLabel xml:lang="en">plates (dishes)</skos:prefLabel>
	<skos:prefLabel xml:lang="hr">tanjur</skos:prefLabel>
	<skos:prefLabel xml:lang="de">Teller</skos:prefLabel>
	<skos:prefLabel xml:lang="sv">tallrikar.</skos:prefLabel>
	<skos:prefLabel xml:lang="pt">pratos.</skos:prefLabel>
	<skos:prefLabel xml:lang="fi">lautaset</skos:prefLabel>
	<skos:inScheme rdf:resource="http://partage.vocnet.org/Objects"/>
	<skos:broader rdf:resource="http://partage.vocnet.org/part00396"/>
	<skos:narrower rdf:resource="http://partage.vocnet.org/part00681"/>
	<skos:exactMatch rdf:resource="http://vocab.getty.edu/aat/300042991"/>
	<skos:editorialNote xml:lang="en">PPRefiningObjectType</skos:editorialNote>
	<skos:scopeNote xml:lang="en">Shallow, usually circular dishes from which food is eaten.</skos:scopeNote>
</skos:Concept>
<skos:Concept rdf:about="http://partage.vocnet.org/part00401">
	<skos:altLabel xml:lang="en">ewers (vessels)</skos:altLabel>
	<skos:prefLabel xml:lang="en">ewers</skos:prefLabel>
	<skos:prefLabel xml:lang="pt">jarro</skos:prefLabel>
	<skos:altLabel xml:lang="de">Wasserkrüge</skos:altLabel>
	<skos:prefLabel xml:lang="de">Wasserkrug</skos:prefLabel>
	<skos:prefLabel xml:lang="sv">vattenkannor</skos:prefLabel>
	<skos:prefLabel xml:lang="hr">bokal</skos:prefLabel>
	<skos:altLabel xml:lang="fi">kaatimet</skos:altLabel>
	<skos:prefLabel xml:lang="fi">kannut</skos:prefLabel>
	<skos:inScheme rdf:resource="http://partage.vocnet.org/Objects"/>
	<skos:broader rdf:resource="http://partage.vocnet.org/part00083"/>
	<skos:exactMatch rdf:resource="http://vocab.getty.edu/aat/300045666"/>
	<skos:editorialNote xml:lang="en">PPRefiningObjectType</skos:editorialNote>
	<skos:scopeNote xml:lang="en">Tall, wide-mouthed vessels, generally having a pouring lip, and that have a deep bowl on a stemmed base and a single vertical handle. The bowl is usually cylindrical, baluster-shaped, or helmet-shaped.</skos:scopeNote>
</skos:Concept>
<skos:Concept rdf:about="http://partage.vocnet.org/part00402">
	<skos:altLabel xml:lang="en">beakers (drinking vessels)</skos:altLabel>
	<skos:prefLabel xml:lang="en">beakers</skos:prefLabel>
	<skos:prefLabel xml:lang="pt">proveta</skos:prefLabel>
	<skos:prefLabel xml:lang="sv">bägare</skos:prefLabel>
	<skos:prefLabel xml:lang="de">Becher</skos:prefLabel>
	<skos:prefLabel xml:lang="hr">čaša</skos:prefLabel>
	<skos:prefLabel xml:lang="fi">pikarit</skos:prefLabel>
	<skos:inScheme rdf:resource="http://partage.vocnet.org/Objects"/>
	<skos:broader rdf:resource="http://partage.vocnet.org/part00403"/>
	<skos:exactMatch rdf:resource="http://vocab.getty.edu/aat/300043198"/>
	<skos:editorialNote xml:lang="en">PPRefiningObjectType</skos:editorialNote>
	<skos:scopeNote xml:lang="en">Generally, refers to many varieties of relatively large drinking vessels without handles, cylindrical or conical in shape, generally with a flat base in the form of an open cup or goblet. Specifically, in archaeology refers to the tall wide-mouthed vessels produced by the Bell Beaker culture and found in certain early Bronze Age graves.</skos:scopeNote>
</skos:Concept>
<skos:Concept rdf:about="http://partage.vocnet.org/part00403">
	<skos:prefLabel xml:lang="en">drinking vessels</skos:prefLabel>
	<skos:prefLabel xml:lang="pt">vasilhas</skos:prefLabel>
	<skos:altLabel xml:lang="de">Trinkgefäß</skos:altLabel>
	<skos:prefLabel xml:lang="de">Trinkgefäße</skos:prefLabel>
	<skos:prefLabel xml:lang="sv">dryckeskärl</skos:prefLabel>
	<skos:prefLabel xml:lang="hr">posude za piće</skos:prefLabel>
	<skos:prefLabel xml:lang="fi">juoma-astiat</skos:prefLabel>
	<skos:inScheme rdf:resource="http://partage.vocnet.org/Objects"/>
	<skos:broader rdf:resource="http://partage.vocnet.org/part00085"/>
	<skos:narrower rdf:resource="http://partage.vocnet.org/part00402"/>
	<skos:narrower rdf:resource="http://partage.vocnet.org/part00688"/>
	<skos:narrower rdf:resource="http://partage.vocnet.org/part00690"/>
	<skos:narrower rdf:resource="http://partage.vocnet.org/part00693"/>
	<skos:exactMatch rdf:resource="http://vocab.getty.edu/aat/300194567"/>
	<skos:editorialNote xml:lang="en">PPRefiningObjectType</skos:editorialNote>
	<skos:scopeNote xml:lang="en">Vessels used for drinking liquids.</skos:scopeNote>
</skos:Concept>
<skos:Concept rdf:about="http://partage.vocnet.org/part00404">
	<skos:prefLabel xml:lang="en">interior views</skos:prefLabel>
	<skos:prefLabel xml:lang="hr">interijer</skos:prefLabel>
	<skos:altLabel xml:lang="de">Innenansichten</skos:altLabel>
	<skos:prefLabel xml:lang="de">Innenansicht</skos:prefLabel>
	<skos:prefLabel xml:lang="sv">interiörer</skos:prefLabel>
	<skos:prefLabel xml:lang="pt">vista interior</skos:prefLabel>
	<skos:prefLabel xml:lang="fi">interiöörit</skos:prefLabel>
	<skos:inScheme rdf:resource="http://partage.vocnet.org/Objects"/>
	<skos:broader rdf:resource="http://partage.vocnet.org/part00406"/>
	<skos:exactMatch rdf:resource="http://vocab.getty.edu/aat/300124520"/>
	<skos:editorialNote xml:lang="en">PPRefiningObjectType</skos:editorialNote>
	<skos:scopeNote xml:lang="en">Refers to photographs or other representations of the inside of a building or other structure or object that has interior and exterior space.</skos:scopeNote>
</skos:Concept>
<skos:Concept rdf:about="http://partage.vocnet.org/part00406">
	<skos:prefLabel xml:lang="en">views (visual works)</skos:prefLabel>
	<skos:inScheme rdf:resource="http://partage.vocnet.org/Objects"/>
	<skos:narrower rdf:resource="http://partage.vocnet.org/part00404"/>
	<skos:narrower rdf:resource="http://partage.vocnet.org/part00812"/>
	<skos:exactMatch rdf:resource="http://vocab.getty.edu/aat/300015424"/>
</skos:Concept>
<skos:Concept rdf:about="http://partage.vocnet.org/part00410">
	<skos:prefLabel xml:lang="en">statues</skos:prefLabel>
	<skos:prefLabel xml:lang="sv">statyer</skos:prefLabel>
	<skos:altLabel xml:lang="hr">kip</skos:altLabel>
	<skos:prefLabel xml:lang="hr">skulptura</skos:prefLabel>
	<skos:altLabel xml:lang="pt">estátuas</skos:altLabel>
	<skos:prefLabel xml:lang="pt">estátua</skos:prefLabel>
	<skos:altLabel xml:lang="de">Statuen</skos:altLabel>
	<skos:altLabel xml:lang="de">Standbild</skos:altLabel>
	<skos:prefLabel xml:lang="de">Statue</skos:prefLabel>
	<skos:altLabel xml:lang="de">Standbilder</skos:altLabel>
	<skos:prefLabel xml:lang="fi">patsaat</skos:prefLabel>
	<skos:inScheme rdf:resource="http://partage.vocnet.org/Objects"/>
	<skos:broader rdf:resource="http://partage.vocnet.org/part00041"/>
	<skos:narrower rdf:resource="http://partage.vocnet.org/part00412"/>
	<skos:narrower rdf:resource="http://partage.vocnet.org/part01191"/>
	<skos:exactMatch rdf:resource="http://vocab.getty.edu/aat/300047600"/>
	<skos:editorialNote xml:lang="en">PPRefiningObjectType</skos:editorialNote>
	<skos:scopeNote xml:lang="en">Sculpture in the round, usually but not always depicting humans, animals, mythical beings, or small figure groups. Statues are relatively large in scale, being life-size, larger than life-size, or only slightly smaller than life-size. For small-scale representations of humans, animals, or mythical beings, use "figurines," "statuettes," or another appropriate term. For depictions of humans, animals, or mythcial beings in media other than sculpture, use "figures (representations)."</skos:scopeNote>
</skos:Concept>
<skos:Concept rdf:about="http://partage.vocnet.org/part00412">
	<skos:prefLabel xml:lang="en">figurines</skos:prefLabel>
	<skos:prefLabel xml:lang="pt">figurino</skos:prefLabel>
	<skos:altLabel xml:lang="de">Figurinen</skos:altLabel>
	<skos:prefLabel xml:lang="de">Figurine</skos:prefLabel>
	<skos:prefLabel xml:lang="sv">figuriner</skos:prefLabel>
	<skos:prefLabel xml:lang="hr">figurica</skos:prefLabel>
	<skos:prefLabel xml:lang="fi">pienoisveistokset</skos:prefLabel>
	<skos:inScheme rdf:resource="http://partage.vocnet.org/Objects"/>
	<skos:broader rdf:resource="http://partage.vocnet.org/part00410"/>
	<skos:narrower rdf:resource="http://partage.vocnet.org/part01137"/>
	<skos:exactMatch rdf:resource="http://vocab.getty.edu/aat/300047455"/>
	<skos:editorialNote xml:lang="en">PPRefiningObjectType</skos:editorialNote>
	<skos:scopeNote xml:lang="en">Three-dimensional works that represent humans, animals, or mythical beasts at less than half life-size. While the term may be used interchangeably with "statuette" in certain situations, it differs in that a statuette is always free-standing while a figurine may be part of a larger work, such as a decorative detail on a candelabra or mirror.</skos:scopeNote>
</skos:Concept>
<skos:Concept rdf:about="http://partage.vocnet.org/part00413">
	<skos:prefLabel xml:lang="en">bottles</skos:prefLabel>
	<skos:prefLabel xml:lang="sv">flaskor</skos:prefLabel>
	<skos:prefLabel xml:lang="pt">garrafa</skos:prefLabel>
	<skos:altLabel xml:lang="de">Flaschen</skos:altLabel>
	<skos:prefLabel xml:lang="de">Flasche</skos:prefLabel>
	<skos:prefLabel xml:lang="hr">boca</skos:prefLabel>
	<skos:prefLabel xml:lang="fi">pullot</skos:prefLabel>
	<skos:inScheme rdf:resource="http://partage.vocnet.org/Objects"/>
	<skos:broader rdf:resource="http://partage.vocnet.org/part00083"/>
	<skos:exactMatch rdf:resource="http://vocab.getty.edu/aat/300045627"/>
	<skos:editorialNote xml:lang="en">PPRefiningObjectType</skos:editorialNote>
	<skos:scopeNote xml:lang="en">Vessels having a neck and mouth considerably narrower than the body, used for packaging and containing liquid and dry preparations. For vessles having wider necks and mouths, use "jars.</skos:scopeNote>
</skos:Concept>
<skos:Concept rdf:about="http://partage.vocnet.org/part00415">
	<skos:altLabel xml:lang="en">design drawings</skos:altLabel>
	<skos:prefLabel xml:lang="en">designs (drawings)</skos:prefLabel>
	<skos:prefLabel xml:lang="pt">desenhos.</skos:prefLabel>
	<skos:altLabel xml:lang="de">Entwürfe</skos:altLabel>
	<skos:altLabel xml:lang="de">Entwurfszeichnung</skos:altLabel>
	<skos:prefLabel xml:lang="de">Entwurf</skos:prefLabel>
	<skos:prefLabel xml:lang="sv">designskisser</skos:prefLabel>
	<skos:prefLabel xml:lang="hr">dizajn (crtež)</skos:prefLabel>
	<skos:prefLabel xml:lang="fi">suunnitelmat</skos:prefLabel>
	<skos:inScheme rdf:resource="http://partage.vocnet.org/Objects"/>
	<skos:broader rdf:resource="http://partage.vocnet.org/part00047"/>
	<skos:exactMatch rdf:resource="http://vocab.getty.edu/aat/300069413"/>
	<skos:editorialNote xml:lang="en">PPRefiningObjectType</skos:editorialNote>
	<skos:scopeNote xml:lang="en">Drawings intended to work out the scheme of a project, whether the project is expected to be executed or not; more finished than sketches.</skos:scopeNote>
</skos:Concept>
<skos:Concept rdf:about="http://partage.vocnet.org/part00419">
	<skos:prefLabel xml:lang="en">photographs</skos:prefLabel>
	<skos:prefLabel xml:lang="de">Fotografie</skos:prefLabel>
	<skos:altLabel xml:lang="de">Photographie</skos:altLabel>
	<skos:prefLabel xml:lang="sv">fotografier</skos:prefLabel>
	<skos:prefLabel xml:lang="fi">valokuvat</skos:prefLabel>
	<skos:prefLabel xml:lang="es">fotografías</skos:prefLabel>
	<skos:prefLabel xml:lang="sl">fotografije</skos:prefLabel>
	<skos:altLabel xml:lang="pt">fotografias</skos:altLabel>
	<skos:prefLabel xml:lang="pt">fotografia</skos:prefLabel>
	<skos:prefLabel xml:lang="pl">fotografie</skos:prefLabel>
	<skos:prefLabel xml:lang="nl">foto's</skos:prefLabel>
	<skos:prefLabel xml:lang="it">fotografie</skos:prefLabel>
	<skos:prefLabel xml:lang="cs">fotografie</skos:prefLabel>
	<skos:prefLabel xml:lang="ca">fotografies</skos:prefLabel>
	<skos:prefLabel xml:lang="hr">fotografije</skos:prefLabel>
	<skos:prefLabel xml:lang="no">fotografi</skos:prefLabel>
	<skos:prefLabel xml:lang="hu">fénykép</skos:prefLabel>
	<skos:prefLabel xml:lang="fr">photographie</skos:prefLabel>
	<skos:altLabel xml:lang="de">Photographien</skos:altLabel>
	<skos:altLabel xml:lang="de">Fotografien</skos:altLabel>
	<skos:altLabel xml:lang="de">Fotos</skos:altLabel>
	<skos:inScheme rdf:resource="http://partage.vocnet.org/Objects"/>
	<skos:narrower rdf:resource="http://partage.vocnet.org/part00890"/>
	<skos:narrower rdf:resource="http://partage.vocnet.org/part00914"/>
	<skos:narrower rdf:resource="http://partage.vocnet.org/part00918"/>
	<skos:exactMatch rdf:resource="http://vocab.getty.edu/aat/300046300"/>
	<skos:editorialNote xml:lang="en">PPObjectType</skos:editorialNote>
	<skos:scopeNote xml:lang="en">Refers to still images produced from radiation-sensitive materials (sensitive to light, electron beams, or nuclear radiation), generally by means of the chemical action of light on a sensitive film, paper, glass, or metal. It does not include reproductive prints of documents and technical drawings, for which descriptors found under "reprographic copies" are more appropriate. Photographs may be positive or negative, opaque or transparent.</skos:scopeNote>
</skos:Concept>
<skos:Concept rdf:about="http://partage.vocnet.org/part00465">
	<skos:prefLabel xml:lang="en">colour lithographs</skos:prefLabel>
	<skos:altLabel xml:lang="en">color lithographs</skos:altLabel>
	<skos:altLabel xml:lang="de">Farblithographien</skos:altLabel>
	<skos:altLabel xml:lang="de">Farblithografien</skos:altLabel>
	<skos:prefLabel xml:lang="de">Farblithographie</skos:prefLabel>
	<skos:altLabel xml:lang="de">Farblithografie</skos:altLabel>
	<skos:prefLabel xml:lang="pt">litografia a cores</skos:prefLabel>
	<skos:prefLabel xml:lang="sv">färglitografier</skos:prefLabel>
	<skos:prefLabel xml:lang="hr">litografija u boji</skos:prefLabel>
	<skos:prefLabel xml:lang="fi">värilitografiat</skos:prefLabel>
	<skos:inScheme rdf:resource="http://partage.vocnet.org/Objects"/>
	<skos:broader rdf:resource="http://partage.vocnet.org/part00524"/>
	<skos:narrower rdf:resource="http://partage.vocnet.org/part00528"/>
	<skos:exactMatch rdf:resource="http://vocab.getty.edu/aat/300041383"/>
	<skos:editorialNote xml:lang="en">PPRefiningObjectType</skos:editorialNote>
	<skos:scopeNote xml:lang="en">Lithographs printed in several colors.</skos:scopeNote>
</skos:Concept>
<skos:Concept rdf:about="http://partage.vocnet.org/part00470">
	<skos:altLabel xml:lang="en">mural paintings (visual works)</skos:altLabel>
	<skos:prefLabel xml:lang="en">mural paintings</skos:prefLabel>
	<skos:prefLabel xml:lang="nl">muurschilderingen</skos:prefLabel>
	<skos:prefLabel xml:lang="it">murali</skos:prefLabel>
	<skos:prefLabel xml:lang="cs">nástěnné malířství</skos:prefLabel>
	<skos:prefLabel xml:lang="ca">pintura mural</skos:prefLabel>
	<skos:prefLabel xml:lang="de">Wandmalerei</skos:prefLabel>
	<skos:prefLabel xml:lang="sv">muralmålningar</skos:prefLabel>
	<skos:altLabel xml:lang="fi">kattomaalaukset</skos:altLabel>
	<skos:prefLabel xml:lang="fi">seinämaalaukset</skos:prefLabel>
	<skos:prefLabel xml:lang="es">pinturas murales</skos:prefLabel>
	<skos:altLabel xml:lang="sl">freske</skos:altLabel>
	<skos:prefLabel xml:lang="sl">stensko slikarstvo</skos:prefLabel>
	<skos:prefLabel xml:lang="pt">pintura mural</skos:prefLabel>
	<skos:prefLabel xml:lang="pl">malarstwo ścienne</skos:prefLabel>
	<skos:prefLabel xml:lang="fr">peinture murale</skos:prefLabel>
	<skos:prefLabel xml:lang="hu">falkép</skos:prefLabel>
	<skos:prefLabel xml:lang="no">muralmaleri</skos:prefLabel>
	<skos:prefLabel xml:lang="hr">zidno slikarstvo</skos:prefLabel>
	<skos:inScheme rdf:resource="http://partage.vocnet.org/Objects"/>
	<skos:broader rdf:resource="http://partage.vocnet.org/part00044"/>
	<skos:exactMatch rdf:resource="http://vocab.getty.edu/aat/300033644"/>
	<skos:editorialNote xml:lang="en">PPObjectType</skos:editorialNote>
	<skos:scopeNote xml:lang="en">Painted decorations or scenes that dominate a wall (or ceiling) surface. For works in other media that dominate a wall (or ceiling), use the more general term "murals (any medium)".</skos:scopeNote>
</skos:Concept>
<skos:Concept rdf:about="http://partage.vocnet.org/part00498">
	<skos:altLabel xml:lang="en">hardware (components)</skos:altLabel>
	<skos:prefLabel xml:lang="en">hardware</skos:prefLabel>
	<skos:prefLabel xml:lang="sv">verktyg</skos:prefLabel>
	<skos:prefLabel xml:lang="fi">rakennustarvikkeet</skos:prefLabel>
	<skos:prefLabel xml:lang="es">herraje</skos:prefLabel>
	<skos:altLabel xml:lang="sl">spojke</skos:altLabel>
	<skos:prefLabel xml:lang="sl">okovje</skos:prefLabel>
	<skos:prefLabel xml:lang="pt">ferragens</skos:prefLabel>
	<skos:prefLabel xml:lang="pl">okucia</skos:prefLabel>
	<skos:prefLabel xml:lang="nl">ijzerwaren</skos:prefLabel>
	<skos:prefLabel xml:lang="it">utensili</skos:prefLabel>
	<skos:prefLabel xml:lang="cs">komponenty</skos:prefLabel>
	<skos:prefLabel xml:lang="ca">ferramenta</skos:prefLabel>
	<skos:prefLabel xml:lang="de">Eisenwaren</skos:prefLabel>
	<skos:prefLabel xml:lang="hr">okovi</skos:prefLabel>
	<skos:prefLabel xml:lang="no">jernvare</skos:prefLabel>
	<skos:prefLabel xml:lang="hu">veret</skos:prefLabel>
	<skos:prefLabel xml:lang="fr">quincaillerie</skos:prefLabel>
	<skos:inScheme rdf:resource="http://partage.vocnet.org/Objects"/>
	<skos:broader rdf:resource="http://partage.vocnet.org/part00116"/>
	<skos:narrower rdf:resource="http://partage.vocnet.org/part01194"/>
	<skos:exactMatch rdf:resource="http://vocab.getty.edu/aat/300033260"/>
	<skos:editorialNote xml:lang="en">PPObjectType</skos:editorialNote>
	<skos:scopeNote xml:lang="en">Large and small items that are necessary to attach, anchor, hold, or join materials and components of structures, furniture, and other objects. Also, items used in the finishing of buildings and objects, such as hinges and knobs.</skos:scopeNote>
</skos:Concept>
<skos:Concept rdf:about="http://partage.vocnet.org/part00501">
	<skos:altLabel xml:lang="en">watercolors (paintings)</skos:altLabel>
	<skos:prefLabel xml:lang="en">watercolours</skos:prefLabel>
	<skos:altLabel xml:lang="de">Aquarelle</skos:altLabel>
	<skos:prefLabel xml:lang="sv">akvareller</skos:prefLabel>
	<skos:prefLabel xml:lang="fi">akvarellimaalaus</skos:prefLabel>
	<skos:prefLabel xml:lang="es">acuarelas</skos:prefLabel>
	<skos:prefLabel xml:lang="sl">akvareli</skos:prefLabel>
	<skos:prefLabel xml:lang="pt">aguarela</skos:prefLabel>
	<skos:prefLabel xml:lang="pl">akwarele</skos:prefLabel>
	<skos:prefLabel xml:lang="nl">aquarellen</skos:prefLabel>
	<skos:prefLabel xml:lang="it">acquarelli</skos:prefLabel>
	<skos:prefLabel xml:lang="cs">akvarel</skos:prefLabel>
	<skos:prefLabel xml:lang="ca">aquarel·les</skos:prefLabel>
	<skos:prefLabel xml:lang="fr">aquarelle</skos:prefLabel>
	<skos:prefLabel xml:lang="hu">akvarell</skos:prefLabel>
	<skos:prefLabel xml:lang="no">akvarell</skos:prefLabel>
	<skos:prefLabel xml:lang="hr">akvareli</skos:prefLabel>
	<skos:prefLabel xml:lang="de">Aquarell</skos:prefLabel>
	<skos:altLabel xml:lang="en">watercolors</skos:altLabel>
	<skos:inScheme rdf:resource="http://partage.vocnet.org/Objects"/>
	<skos:broader rdf:resource="http://partage.vocnet.org/part00044"/>
	<skos:exactMatch rdf:resource="http://vocab.getty.edu/aat/300078925"/>
	<skos:editorialNote xml:lang="en">PPObjectType</skos:editorialNote>
	<skos:scopeNote xml:lang="en">Refers to two-dimensional works of art, usually on a paper support, to which pigment suspended in water is applied with a brush to create an image or design.</skos:scopeNote>
</skos:Concept>
<skos:Concept rdf:about="http://partage.vocnet.org/part00502">
	<skos:altLabel xml:lang="en">magazines (periodicals)</skos:altLabel>
	<skos:prefLabel xml:lang="en">magazines</skos:prefLabel>
	<skos:prefLabel xml:lang="sv">tidskrifter</skos:prefLabel>
	<skos:prefLabel xml:lang="fi">aikakauslehdet</skos:prefLabel>
	<skos:prefLabel xml:lang="es">revistas</skos:prefLabel>
	<skos:prefLabel xml:lang="sl">revije</skos:prefLabel>
	<skos:altLabel xml:lang="pt">revistas</skos:altLabel>
	<skos:prefLabel xml:lang="pt">revista</skos:prefLabel>
	<skos:prefLabel xml:lang="pl">czasopisma</skos:prefLabel>
	<skos:prefLabel xml:lang="nl">magazines</skos:prefLabel>
	<skos:prefLabel xml:lang="it">riviste</skos:prefLabel>
	<skos:prefLabel xml:lang="cs">časopisy</skos:prefLabel>
	<skos:prefLabel xml:lang="ca">revistes</skos:prefLabel>
	<skos:altLabel xml:lang="de">Magazin</skos:altLabel>
	<skos:prefLabel xml:lang="de">Zeitschriften</skos:prefLabel>
	<skos:altLabel xml:lang="de">Zeitschrift</skos:altLabel>
	<skos:prefLabel xml:lang="hr">časopisi</skos:prefLabel>
	<skos:prefLabel xml:lang="no">tidsskrift</skos:prefLabel>
	<skos:prefLabel xml:lang="hu">folyóirat</skos:prefLabel>
	<skos:prefLabel xml:lang="fr">revue</skos:prefLabel>
	<skos:altLabel xml:lang="de">Magazine</skos:altLabel>
	<skos:inScheme rdf:resource="http://partage.vocnet.org/Objects"/>
	<skos:broader rdf:resource="http://partage.vocnet.org/part00204"/>
	<skos:exactMatch rdf:resource="http://vocab.getty.edu/aat/300215389"/>
	<skos:editorialNote xml:lang="en">PPObjectType</skos:editorialNote>
	<skos:scopeNote xml:lang="en">Periodicals containing articles, essays, poems, or other writings by different authors, usually on a variety of topics and intended for a general reading public or treating a particular area of interest for a popular audience.</skos:scopeNote>
</skos:Concept>
<skos:Concept rdf:about="http://partage.vocnet.org/part00504">
	<skos:prefLabel xml:lang="en">rugs</skos:prefLabel>
	<skos:altLabel xml:lang="de">Teppiche.</skos:altLabel>
	<skos:prefLabel xml:lang="de">Teppich.</skos:prefLabel>
	<skos:inScheme rdf:resource="http://partage.vocnet.org/Objects"/>
	<skos:broader rdf:resource="http://partage.vocnet.org/part00100"/>
	<skos:narrower rdf:resource="http://partage.vocnet.org/part00808"/>
	<skos:exactMatch rdf:resource="http://vocab.getty.edu/aat/300185749"/>
	<skos:scopeNote xml:lang="en">Heavy woven textiles used for a variety of utilitarian purposes essentially in the form in which they left the loom. In Western societies they are used primarily as floor coverings.</skos:scopeNote>
</skos:Concept>
<skos:Concept rdf:about="http://partage.vocnet.org/part00505">
	<skos:prefLabel xml:lang="en">printing plates</skos:prefLabel>
	<skos:prefLabel xml:lang="de">Druckplatten</skos:prefLabel>
	<skos:prefLabel xml:lang="sv">tryckplåtar</skos:prefLabel>
	<skos:prefLabel xml:lang="fi">painolaatat</skos:prefLabel>
	<skos:prefLabel xml:lang="es">planchas de impresión</skos:prefLabel>
	<skos:prefLabel xml:lang="sl">tiskarske plošče</skos:prefLabel>
	<skos:prefLabel xml:lang="pt">chapa de impressão</skos:prefLabel>
	<skos:prefLabel xml:lang="pl">płyty graficzne</skos:prefLabel>
	<skos:prefLabel xml:lang="nl">drukplaten</skos:prefLabel>
	<skos:prefLabel xml:lang="it">matrici di incisione</skos:prefLabel>
	<skos:prefLabel xml:lang="cs">tisková matrice</skos:prefLabel>
	<skos:prefLabel xml:lang="ca">planxes d'impressió</skos:prefLabel>
	<skos:altLabel xml:lang="de">Matritze</skos:altLabel>
	<skos:altLabel xml:lang="de">Druckstock</skos:altLabel>
	<skos:altLabel xml:lang="de">Druckform</skos:altLabel>
	<skos:prefLabel xml:lang="hr">grafičke ploče</skos:prefLabel>
	<skos:prefLabel xml:lang="hu">nyomódúc</skos:prefLabel>
	<skos:prefLabel xml:lang="no">trykkeplater</skos:prefLabel>
	<skos:prefLabel xml:lang="fr">plaque d'imprimerie</skos:prefLabel>
	<skos:altLabel xml:lang="de">Matritzen</skos:altLabel>
	<skos:altLabel xml:lang="de">Druckstöcke</skos:altLabel>
	<skos:altLabel xml:lang="de">Druckformen</skos:altLabel>
	<skos:inScheme rdf:resource="http://partage.vocnet.org/Objects"/>
	<skos:broader rdf:resource="http://partage.vocnet.org/part00218"/>
	<skos:exactMatch rdf:resource="http://vocab.getty.edu/aat/300022755"/>
	<skos:editorialNote xml:lang="en">PPObjectType</skos:editorialNote>
	<skos:scopeNote xml:lang="en">Flat pieces of metal from which textual or pictorial images are printed. For blocks of other material, usually wood, cut to print an image or used to support other materials that form the printing surface, use "printing blocks" or a more specific term.</skos:scopeNote>
</skos:Concept>
<skos:Concept rdf:about="http://partage.vocnet.org/part00510">
	<skos:altLabel xml:lang="en">painted glass (visual works)</skos:altLabel>
	<skos:prefLabel xml:lang="en">painted glass</skos:prefLabel>
	<skos:prefLabel xml:lang="de">Glasmalerei</skos:prefLabel>
	<skos:prefLabel xml:lang="sv">målat glas</skos:prefLabel>
	<skos:prefLabel xml:lang="fi">maalattu lasi</skos:prefLabel>
	<skos:altLabel xml:lang="fi">lasimaalaus.</skos:altLabel>
	<skos:altLabel xml:lang="es">pintura en vidrio</skos:altLabel>
	<skos:prefLabel xml:lang="es">vidrio pintado</skos:prefLabel>
	<skos:prefLabel xml:lang="sl">slikano steklo</skos:prefLabel>
	<skos:prefLabel xml:lang="pt">vidro pintado</skos:prefLabel>
	<skos:prefLabel xml:lang="pl">szkło malowane</skos:prefLabel>
	<skos:prefLabel xml:lang="nl">geschilderd glas</skos:prefLabel>
	<skos:prefLabel xml:lang="it">vetri dipinti</skos:prefLabel>
	<skos:prefLabel xml:lang="cs">malované sklo</skos:prefLabel>
	<skos:prefLabel xml:lang="ca">vidre pintat</skos:prefLabel>
	<skos:altLabel xml:lang="de">gefasstes Glas</skos:altLabel>
	<skos:prefLabel xml:lang="fr">peinture sur verre</skos:prefLabel>
	<skos:prefLabel xml:lang="hu">festett üveg</skos:prefLabel>
	<skos:prefLabel xml:lang="no">glassmaleri</skos:prefLabel>
	<skos:prefLabel xml:lang="hr">oslikano staklo</skos:prefLabel>
	<skos:inScheme rdf:resource="http://partage.vocnet.org/Objects"/>
	<skos:broader rdf:resource="http://partage.vocnet.org/part00044"/>
	<skos:exactMatch rdf:resource="http://vocab.getty.edu/aat/300343822"/>
	<skos:editorialNote xml:lang="en">PPObjectType</skos:editorialNote>
	<skos:scopeNote xml:lang="en">Works done by painting on the front or the reverse of glass, whether or not the paint is then fired onto the glass. Painted glass mirrors and other glass decoration, and painted works in the manner of painting on canvas or wooden panels were known since ancient times. In the context of stained glass windows and panels, refers to parts of the image that are painted on glass (often stained glass), especially the smaller details.</skos:scopeNote>
</skos:Concept>
<skos:Concept rdf:about="http://partage.vocnet.org/part00511">
	<skos:prefLabel xml:lang="en">fine bindings</skos:prefLabel>
	<skos:altLabel xml:lang="de">Bucheinband</skos:altLabel>
	<skos:prefLabel xml:lang="sv">bokband</skos:prefLabel>
	<skos:prefLabel xml:lang="fi">taidesidokset</skos:prefLabel>
	<skos:prefLabel xml:lang="es">encuadernación de lujo</skos:prefLabel>
	<skos:prefLabel xml:lang="sl">bibliofilske vezave</skos:prefLabel>
	<skos:prefLabel xml:lang="pt">encadernação</skos:prefLabel>
	<skos:prefLabel xml:lang="pl">oprawy artystyczne</skos:prefLabel>
	<skos:prefLabel xml:lang="nl">kunstboekbanden</skos:prefLabel>
	<skos:prefLabel xml:lang="it">legature</skos:prefLabel>
	<skos:prefLabel xml:lang="cs">knižní vazba</skos:prefLabel>
	<skos:prefLabel xml:lang="ca">enquadernació de luxe</skos:prefLabel>
	<skos:altLabel xml:lang="de">Buchkunst</skos:altLabel>
	<skos:prefLabel xml:lang="de">Bucheinbände</skos:prefLabel>
	<skos:prefLabel xml:lang="hr">umjetničko knjigoveštvo</skos:prefLabel>
	<skos:prefLabel xml:lang="no">kunstbokbind</skos:prefLabel>
	<skos:prefLabel xml:lang="hu">művészi könyvkötés</skos:prefLabel>
	<skos:prefLabel xml:lang="fr">reliure d'art</skos:prefLabel>
	<skos:inScheme rdf:resource="http://partage.vocnet.org/Objects"/>
	<skos:broader rdf:resource="http://partage.vocnet.org/part00644"/>
	<skos:exactMatch rdf:resource="http://vocab.getty.edu/aat/300311788"/>
	<skos:editorialNote xml:lang="en">PPObjectType</skos:editorialNote>
	<skos:scopeNote xml:lang="en">Bindings produced as unique or limited editions and intended to be works of art in themselves.</skos:scopeNote>
</skos:Concept>
<skos:Concept rdf:about="http://partage.vocnet.org/part00512">
	<skos:prefLabel xml:lang="en">wickerwork</skos:prefLabel>
	<skos:prefLabel xml:lang="de">Flechtwerk</skos:prefLabel>
	<skos:prefLabel xml:lang="sv">korgarbete</skos:prefLabel>
	<skos:prefLabel xml:lang="fi">punontatyöt</skos:prefLabel>
	<skos:prefLabel xml:lang="es">obra de mimbre</skos:prefLabel>
	<skos:prefLabel xml:lang="sl">pletarski izdelki</skos:prefLabel>
	<skos:prefLabel xml:lang="pt">trabalho de verga</skos:prefLabel>
	<skos:prefLabel xml:lang="pl">wyroby wyplatane</skos:prefLabel>
	<skos:prefLabel xml:lang="nl">vlechtwerk</skos:prefLabel>
	<skos:prefLabel xml:lang="it">oggetti di vimini</skos:prefLabel>
	<skos:prefLabel xml:lang="cs">práce z proutí</skos:prefLabel>
	<skos:prefLabel xml:lang="ca">obra de vímet</skos:prefLabel>
	<skos:prefLabel xml:lang="hr">predmeti od šiblja</skos:prefLabel>
	<skos:prefLabel xml:lang="no">kurvfletting</skos:prefLabel>
	<skos:prefLabel xml:lang="hu">fonás</skos:prefLabel>
	<skos:prefLabel xml:lang="fr">vannerie</skos:prefLabel>
	<skos:inScheme rdf:resource="http://partage.vocnet.org/Objects"/>
	<skos:exactMatch rdf:resource="http://vocab.getty.edu/aat/300044074"/>
	<skos:editorialNote xml:lang="en">PPObjectType</skos:editorialNote>
	<skos:scopeNote xml:lang="en">Objects created with real or simulated flexible twigs, plaited together.</skos:scopeNote>
</skos:Concept>
<skos:Concept rdf:about="http://partage.vocnet.org/part00513">
	<skos:altLabel xml:lang="en">illustrations (layout features)</skos:altLabel>
	<skos:prefLabel xml:lang="en">illustrations</skos:prefLabel>
	<skos:prefLabel xml:lang="de">Illustration</skos:prefLabel>
	<skos:altLabel xml:lang="pt">ilustraçãos</skos:altLabel>
	<skos:prefLabel xml:lang="pt">ilustração</skos:prefLabel>
	<skos:prefLabel xml:lang="pl">ilustracje</skos:prefLabel>
	<skos:prefLabel xml:lang="nl">illustraties</skos:prefLabel>
	<skos:prefLabel xml:lang="it">illustrazioni</skos:prefLabel>
	<skos:prefLabel xml:lang="cs">ilustrace</skos:prefLabel>
	<skos:prefLabel xml:lang="ca">il·lustracions</skos:prefLabel>
	<skos:prefLabel xml:lang="sv">illustrationer</skos:prefLabel>
	<skos:prefLabel xml:lang="fi">kuvitus</skos:prefLabel>
	<skos:prefLabel xml:lang="fr">illustrations</skos:prefLabel>
	<skos:prefLabel xml:lang="hu">illusztráció</skos:prefLabel>
	<skos:prefLabel xml:lang="no">illustrasjoner</skos:prefLabel>
	<skos:prefLabel xml:lang="hr">ilustracije</skos:prefLabel>
	<skos:prefLabel xml:lang="es">ilustraciones</skos:prefLabel>
	<skos:prefLabel xml:lang="sl">ilustracije</skos:prefLabel>
	<skos:inScheme rdf:resource="http://partage.vocnet.org/Objects"/>
	<skos:broader rdf:resource="http://partage.vocnet.org/part00116"/>
	<skos:exactMatch rdf:resource="http://vocab.getty.edu/aat/300015578"/>
	<skos:editorialNote xml:lang="en">PPObjectType</skos:editorialNote>
	<skos:scopeNote xml:lang="en">Pictures or diagrams that clarify or provide an example or visualization. They usually accompany a text; the term is most often used to refer to pictures in books or published journal. For works that explore a subject or are preliminary to a separate, more finalized work, use "studies (visual works)." For paintings in manuscripts, use "illuminations" or "miniatures (paintings)."</skos:scopeNote>
</skos:Concept>
<skos:Concept rdf:about="http://partage.vocnet.org/part00524">
	<skos:prefLabel xml:lang="en">lithographs</skos:prefLabel>
	<skos:inScheme rdf:resource="http://partage.vocnet.org/Objects"/>
	<skos:broader rdf:resource="http://partage.vocnet.org/part00525"/>
	<skos:narrower rdf:resource="http://partage.vocnet.org/part00465"/>
	<skos:exactMatch rdf:resource="http://vocab.getty.edu/aat/300041379"/>
	<skos:scopeNote xml:lang="en">Prints made using the process of lithography, which is a planographic printing process in which a design is deposited on the stone or plate with a greasy substance which will accept ink.</skos:scopeNote>
</skos:Concept>
<skos:Concept rdf:about="http://partage.vocnet.org/part00525">
	<skos:prefLabel xml:lang="en">planographic prints</skos:prefLabel>
	<skos:inScheme rdf:resource="http://partage.vocnet.org/Objects"/>
	<skos:broader rdf:resource="http://partage.vocnet.org/part00042"/>
	<skos:narrower rdf:resource="http://partage.vocnet.org/part00524"/>
	<skos:narrower rdf:resource="http://partage.vocnet.org/part00892"/>
	<skos:exactMatch rdf:resource="http://vocab.getty.edu/aat/300178376"/>
	<skos:scopeNote xml:lang="en">Prints made using a process of planographic printing.</skos:scopeNote>
</skos:Concept>
<skos:Concept rdf:about="http://partage.vocnet.org/part00528">
	<skos:prefLabel xml:lang="en">chromolithographs</skos:prefLabel>
	<skos:prefLabel xml:lang="sv">litografier</skos:prefLabel>
	<skos:prefLabel xml:lang="pt">cromolitografia</skos:prefLabel>
	<skos:altLabel xml:lang="de">Chromolithographien</skos:altLabel>
	<skos:altLabel xml:lang="de">Chromolithografien</skos:altLabel>
	<skos:prefLabel xml:lang="de">Chromolithographie</skos:prefLabel>
	<skos:altLabel xml:lang="de">Chromolithografie</skos:altLabel>
	<skos:prefLabel xml:lang="hr">kromolitografija</skos:prefLabel>
	<skos:prefLabel xml:lang="fi">kromolitografiat</skos:prefLabel>
	<skos:inScheme rdf:resource="http://partage.vocnet.org/Objects"/>
	<skos:broader rdf:resource="http://partage.vocnet.org/part00465"/>
	<skos:exactMatch rdf:resource="http://vocab.getty.edu/aat/300041384"/>
	<skos:editorialNote xml:lang="en">PPRefiningObjectType</skos:editorialNote>
	<skos:scopeNote xml:lang="en">Color lithographs produced commercially in the latter half of the 19th century and later.</skos:scopeNote>
</skos:Concept>
<skos:Concept rdf:about="http://partage.vocnet.org/part00560">
	<skos:prefLabel xml:lang="en">architectural drawings</skos:prefLabel>
	<skos:altLabel xml:lang="de">Architekturzeichnungen</skos:altLabel>
	<skos:prefLabel xml:lang="de">Architekturzeichnung</skos:prefLabel>
	<skos:prefLabel xml:lang="pt">desenhos de arquitectura</skos:prefLabel>
	<skos:prefLabel xml:lang="sv">ritningar</skos:prefLabel>
	<skos:prefLabel xml:lang="hr">arhitektonski crtež</skos:prefLabel>
	<skos:prefLabel xml:lang="fi">arkkitehtuuripiirustukset</skos:prefLabel>
	<skos:inScheme rdf:resource="http://partage.vocnet.org/Objects"/>
	<skos:broader rdf:resource="http://partage.vocnet.org/part00047"/>
	<skos:exactMatch rdf:resource="http://vocab.getty.edu/aat/300034787"/>
	<skos:editorialNote xml:lang="en">PPRefiningObjectType</skos:editorialNote>
	<skos:scopeNote xml:lang="en">Drawings of architecture and drawings for architectural projects, whether the project was executed or not. The term may also refer to any image in a two-dimensional medium that serves this same purpose, including prints and computer images.</skos:scopeNote>
</skos:Concept>
<skos:Concept rdf:about="http://partage.vocnet.org/part00562">
	<skos:prefLabel xml:lang="en">paravents</skos:prefLabel>
	<skos:prefLabel xml:lang="hr">paravan</skos:prefLabel>
	<skos:altLabel xml:lang="hr">zaslon</skos:altLabel>
	<skos:prefLabel xml:lang="sv">rumsavskiljare</skos:prefLabel>
	<skos:prefLabel xml:lang="pt">paravento</skos:prefLabel>
	<skos:altLabel xml:lang="de">Spanische Wand</skos:altLabel>
	<skos:prefLabel xml:lang="de">Paravent</skos:prefLabel>
	<skos:altLabel xml:lang="de">Wandschirm</skos:altLabel>
	<skos:altLabel xml:lang="de">Paravents</skos:altLabel>
	<skos:prefLabel xml:lang="fi">väliseinät.</skos:prefLabel>
	<skos:inScheme rdf:resource="http://partage.vocnet.org/Objects"/>
	<skos:broader rdf:resource="http://partage.vocnet.org/part00303"/>
	<skos:exactMatch rdf:resource="http://vocab.getty.edu/aat/300134802"/>
	<skos:editorialNote xml:lang="en">PPRefiningObjectType</skos:editorialNote>
	<skos:scopeNote xml:lang="en">Large folding screens to provide protection against drafts.</skos:scopeNote>
</skos:Concept>
<skos:Concept rdf:about="http://partage.vocnet.org/part00644">
	<skos:prefLabel xml:lang="en">bindings (gathered matter components)</skos:prefLabel>
	<skos:inScheme rdf:resource="http://partage.vocnet.org/Objects"/>
	<skos:broader rdf:resource="http://partage.vocnet.org/part00116"/>
	<skos:narrower rdf:resource="http://partage.vocnet.org/part00511"/>
	<skos:exactMatch rdf:resource="http://vocab.getty.edu/aat/300055023"/>
	<skos:scopeNote xml:lang="en">Coverings of a book which hold the sheets together to provide protection, and collectively all the parts of books applied in the process of attaching the leaves and covering them.</skos:scopeNote>
</skos:Concept>
<skos:Concept rdf:about="http://partage.vocnet.org/part00676">
	<skos:prefLabel xml:lang="en">ashtrays</skos:prefLabel>
	<skos:prefLabel xml:lang="sv">askfat</skos:prefLabel>
	<skos:prefLabel xml:lang="pt">cinzeiro</skos:prefLabel>
	<skos:prefLabel xml:lang="de">Aschenbecher</skos:prefLabel>
	<skos:prefLabel xml:lang="hr">pepeljara</skos:prefLabel>
	<skos:prefLabel xml:lang="fi">tuhkakupit</skos:prefLabel>
	<skos:inScheme rdf:resource="http://partage.vocnet.org/Objects"/>
	<skos:broader rdf:resource="http://partage.vocnet.org/part00085"/>
	<skos:exactMatch rdf:resource="http://vocab.getty.edu/aat/300198897"/>
	<skos:editorialNote xml:lang="en">PPRefiningObjectType</skos:editorialNote>
	<skos:scopeNote xml:lang="en">Receptacles for smokers' tobacco ashes, made in a great range of sizes and designs.</skos:scopeNote>
</skos:Concept>
<skos:Concept rdf:about="http://partage.vocnet.org/part00677">
	<skos:altLabel xml:lang="en">baskets (containers)</skos:altLabel>
	<skos:prefLabel xml:lang="en">baskets</skos:prefLabel>
	<skos:prefLabel xml:lang="sv">korgar</skos:prefLabel>
	<skos:prefLabel xml:lang="pt">cesto</skos:prefLabel>
	<skos:altLabel xml:lang="de">Körbe</skos:altLabel>
	<skos:prefLabel xml:lang="de">Korb</skos:prefLabel>
	<skos:prefLabel xml:lang="hr">košara</skos:prefLabel>
	<skos:prefLabel xml:lang="fi">korit</skos:prefLabel>
	<skos:inScheme rdf:resource="http://partage.vocnet.org/Objects"/>
	<skos:broader rdf:resource="http://partage.vocnet.org/part00085"/>
	<skos:exactMatch rdf:resource="http://vocab.getty.edu/aat/300194498"/>
	<skos:editorialNote xml:lang="en">PPRefiningObjectType</skos:editorialNote>
	<skos:scopeNote xml:lang="en">Containers made of twigs, rushes, thin strips of wood, or other flexible material woven together.</skos:scopeNote>
</skos:Concept>
<skos:Concept rdf:about="http://partage.vocnet.org/part00678">
	<skos:prefLabel xml:lang="en">cachepots</skos:prefLabel>
	<skos:prefLabel xml:lang="sv">blomkrukor</skos:prefLabel>
	<skos:prefLabel xml:lang="pt">cachepot</skos:prefLabel>
	<skos:altLabel xml:lang="de">Übertöpfe</skos:altLabel>
	<skos:prefLabel xml:lang="de">Übertopf</skos:prefLabel>
	<skos:prefLabel xml:lang="hr">posuda za cvijeće</skos:prefLabel>
	<skos:prefLabel xml:lang="fi">suojaruukut</skos:prefLabel>
	<skos:inScheme rdf:resource="http://partage.vocnet.org/Objects"/>
	<skos:broader rdf:resource="http://partage.vocnet.org/part00085"/>
	<skos:exactMatch rdf:resource="http://vocab.getty.edu/aat/300197605"/>
	<skos:editorialNote xml:lang="en">PPRefiningObjectType</skos:editorialNote>
	<skos:scopeNote xml:lang="en">Ornamental containers for holding and concealing a flowerpot.</skos:scopeNote>
</skos:Concept>
<skos:Concept rdf:about="http://partage.vocnet.org/part00679">
	<skos:prefLabel xml:lang="en">cruet stands</skos:prefLabel>
	<skos:prefLabel xml:lang="de">Menage</skos:prefLabel>
	<skos:altLabel xml:lang="de">Gewürzständer</skos:altLabel>
	<skos:prefLabel xml:lang="pt">gaiteiro</skos:prefLabel>
	<skos:prefLabel xml:lang="sv">bordssyrtuter</skos:prefLabel>
	<skos:prefLabel xml:lang="hr">karafindl</skos:prefLabel>
	<skos:prefLabel xml:lang="fi">mausteikot</skos:prefLabel>
	<skos:inScheme rdf:resource="http://partage.vocnet.org/Objects"/>
	<skos:broader rdf:resource="http://partage.vocnet.org/part00085"/>
	<skos:exactMatch rdf:resource="http://vocab.getty.edu/aat/300043034"/>
	<skos:editorialNote xml:lang="en">PPRefiningObjectType</skos:editorialNote>
	<skos:scopeNote xml:lang="en">Trays or small receptacles for holding two or more small bottles or other vessels for ceremonial liquids or for oil, vinegar, spices, mustard, other condiments at meals.</skos:scopeNote>
</skos:Concept>
<skos:Concept rdf:about="http://partage.vocnet.org/part00680">
	<skos:prefLabel xml:lang="en">inkwells</skos:prefLabel>
	<skos:prefLabel xml:lang="hr">tintarnica</skos:prefLabel>
	<skos:altLabel xml:lang="de">Tintenfässer</skos:altLabel>
	<skos:prefLabel xml:lang="de">Tintenfass</skos:prefLabel>
	<skos:prefLabel xml:lang="sv">bläckhorn</skos:prefLabel>
	<skos:prefLabel xml:lang="pt">tinteiro</skos:prefLabel>
	<skos:prefLabel xml:lang="fi">mustepullot</skos:prefLabel>
	<skos:inScheme rdf:resource="http://partage.vocnet.org/Objects"/>
	<skos:broader rdf:resource="http://partage.vocnet.org/part00085"/>
	<skos:exactMatch rdf:resource="http://vocab.getty.edu/aat/300196797"/>
	<skos:scopeNote xml:lang="en">Small vessels for holding ink into which a pen can be dipped. For bottles in which ink is sold, see "ink bottles."</skos:scopeNote>
	<skos:editorialNote xml:lang="en">PPRefiningObjectType</skos:editorialNote>
</skos:Concept>
<skos:Concept rdf:about="http://partage.vocnet.org/part00681">
	<skos:altLabel xml:lang="en">saucers (plates)</skos:altLabel>
	<skos:prefLabel xml:lang="en">saucers</skos:prefLabel>
	<skos:prefLabel xml:lang="hr">tanjurić</skos:prefLabel>
	<skos:prefLabel xml:lang="pt">pires</skos:prefLabel>
	<skos:altLabel xml:lang="de">Untertassen</skos:altLabel>
	<skos:altLabel xml:lang="de">Dessertteller</skos:altLabel>
	<skos:prefLabel xml:lang="de">Untertasse</skos:prefLabel>
	<skos:prefLabel xml:lang="sv">tefat</skos:prefLabel>
	<skos:prefLabel xml:lang="fi">aluslautaset</skos:prefLabel>
	<skos:inScheme rdf:resource="http://partage.vocnet.org/Objects"/>
	<skos:broader rdf:resource="http://partage.vocnet.org/part00400"/>
	<skos:exactMatch rdf:resource="http://vocab.getty.edu/aat/300195535"/>
	<skos:editorialNote xml:lang="en">PPRefiningObjectType</skos:editorialNote>
	<skos:scopeNote xml:lang="en">Small plates of concave form, usually circular, either for eating food or as a stand for a cup. Generally, those for use with a cup have a slight depression in the center in which to place the cup.</skos:scopeNote>
</skos:Concept>
<skos:Concept rdf:about="http://partage.vocnet.org/part00682">
	<skos:altLabel xml:lang="en">pots (containers)</skos:altLabel>
	<skos:prefLabel xml:lang="en">pots</skos:prefLabel>
	<skos:prefLabel xml:lang="hr">posuda</skos:prefLabel>
	<skos:altLabel xml:lang="de">Töpfe</skos:altLabel>
	<skos:prefLabel xml:lang="de">Topf</skos:prefLabel>
	<skos:prefLabel xml:lang="sv">burkar (förvaringskärl)</skos:prefLabel>
	<skos:altLabel xml:lang="pt">panela</skos:altLabel>
	<skos:altLabel xml:lang="pt">bule</skos:altLabel>
	<skos:altLabel xml:lang="pt">marmita</skos:altLabel>
	<skos:prefLabel xml:lang="pt">pote</skos:prefLabel>
	<skos:prefLabel xml:lang="fi">padat</skos:prefLabel>
	<skos:inScheme rdf:resource="http://partage.vocnet.org/Objects"/>
	<skos:broader rdf:resource="http://partage.vocnet.org/part00083"/>
	<skos:narrower rdf:resource="http://partage.vocnet.org/part01141"/>
	<skos:narrower rdf:resource="http://partage.vocnet.org/part01162"/>
	<skos:exactMatch rdf:resource="http://vocab.getty.edu/aat/300045697"/>
	<skos:editorialNote xml:lang="en">PPRefiningObjectType</skos:editorialNote>
	<skos:scopeNote xml:lang="en">Cylindrical or rounded containers, often of metal or earthenware and varying in size; used chiefly for domestic purposes.</skos:scopeNote>
</skos:Concept>
<skos:Concept rdf:about="http://partage.vocnet.org/part00683">
	<skos:prefLabel xml:lang="en">trays</skos:prefLabel>
	<skos:prefLabel xml:lang="sv">brickor</skos:prefLabel>
	<skos:prefLabel xml:lang="hr">pladanj</skos:prefLabel>
	<skos:prefLabel xml:lang="pt">tabuleiro</skos:prefLabel>
	<skos:prefLabel xml:lang="de">Tablett</skos:prefLabel>
	<skos:altLabel xml:lang="de">Tabletts</skos:altLabel>
	<skos:prefLabel xml:lang="fi">tarjottimet</skos:prefLabel>
	<skos:inScheme rdf:resource="http://partage.vocnet.org/Objects"/>
	<skos:broader rdf:resource="http://partage.vocnet.org/part00085"/>
	<skos:exactMatch rdf:resource="http://vocab.getty.edu/aat/300043071"/>
	<skos:editorialNote xml:lang="en">PPRefiningObjectType</skos:editorialNote>
	<skos:scopeNote xml:lang="en">Open, variously shaped containers of wood, metal or other rigid material with a flat bottom and a low rim for holding, carrying, or exhibiting articles.</skos:scopeNote>
</skos:Concept>
<skos:Concept rdf:about="http://partage.vocnet.org/part00684">
	<skos:altLabel xml:lang="en">buckets (vessels)</skos:altLabel>
	<skos:prefLabel xml:lang="en">buckets</skos:prefLabel>
	<skos:prefLabel xml:lang="sv">spannar</skos:prefLabel>
	<skos:prefLabel xml:lang="pt">balde</skos:prefLabel>
	<skos:prefLabel xml:lang="de">Eimer</skos:prefLabel>
	<skos:altLabel xml:lang="de">Kübel</skos:altLabel>
	<skos:prefLabel xml:lang="hr">kanta</skos:prefLabel>
	<skos:prefLabel xml:lang="fi">sangot</skos:prefLabel>
	<skos:inScheme rdf:resource="http://partage.vocnet.org/Objects"/>
	<skos:broader rdf:resource="http://partage.vocnet.org/part00083"/>
	<skos:exactMatch rdf:resource="http://vocab.getty.edu/aat/300045651"/>
	<skos:editorialNote xml:lang="en">PPRefiningObjectType</skos:editorialNote>
	<skos:scopeNote xml:lang="en">Typically, round wooden vessels for drawing water from a well; also, any comparable vessel for catching, holding, or carrying liquids or solids.</skos:scopeNote>
</skos:Concept>
<skos:Concept rdf:about="http://partage.vocnet.org/part00685">
	<skos:prefLabel xml:lang="en">creamers</skos:prefLabel>
	<skos:prefLabel xml:lang="pt">leiteira</skos:prefLabel>
	<skos:altLabel xml:lang="de">Oberskännchen</skos:altLabel>
	<skos:prefLabel xml:lang="de">Sahnekännchen</skos:prefLabel>
	<skos:prefLabel xml:lang="sv">gräddkannor</skos:prefLabel>
	<skos:prefLabel xml:lang="hr">vrčić za mlijeko</skos:prefLabel>
	<skos:prefLabel xml:lang="fi">kemakot</skos:prefLabel>
	<skos:inScheme rdf:resource="http://partage.vocnet.org/Objects"/>
	<skos:broader rdf:resource="http://partage.vocnet.org/part00085"/>
	<skos:exactMatch rdf:resource="http://vocab.getty.edu/aat/300220996"/>
	<skos:editorialNote xml:lang="en">PPRefiningObjectType</skos:editorialNote>
	<skos:scopeNote xml:lang="en">Containers for holding and serving cream, especially a small pitcher that may be accompanied by a sugar bowl. Sometimes made as part of a tea or coffee service. For containers designed for holding and serving milk, especially medium-sized pitchers, use "milk jugs."</skos:scopeNote>
</skos:Concept>
<skos:Concept rdf:about="http://partage.vocnet.org/part00686">
	<skos:altLabel xml:lang="en">pitchers (vessels)</skos:altLabel>
	<skos:prefLabel xml:lang="en">pitchers</skos:prefLabel>
	<skos:prefLabel xml:lang="hr">krigla</skos:prefLabel>
	<skos:altLabel xml:lang="de">Henkelkrüge</skos:altLabel>
	<skos:prefLabel xml:lang="de">Henkelkrug</skos:prefLabel>
	<skos:prefLabel xml:lang="sv">tillbringare.</skos:prefLabel>
	<skos:prefLabel xml:lang="pt">jarros</skos:prefLabel>
	<skos:altLabel xml:lang="hr">vrč.</skos:altLabel>
	<skos:prefLabel xml:lang="fi">ruukut.</skos:prefLabel>
	<skos:inScheme rdf:resource="http://partage.vocnet.org/Objects"/>
	<skos:broader rdf:resource="http://partage.vocnet.org/part00083"/>
	<skos:exactMatch rdf:resource="http://vocab.getty.edu/aat/300194765"/>
	<skos:editorialNote xml:lang="en">PPRefiningObjectType</skos:editorialNote>
	<skos:scopeNote xml:lang="en">Vessels, generally of ceramic, glass, metal, or plastic, that have a wide mouth with a broad lip and usually a handle at one side, but sometimes having two ears; includes those accompanied by a washbowl and used for personal hygiene.</skos:scopeNote>
</skos:Concept>
<skos:Concept rdf:about="http://partage.vocnet.org/part00688">
	<skos:prefLabel xml:lang="en">cups</skos:prefLabel>
	<skos:altLabel xml:lang="pt">chávenas</skos:altLabel>
	<skos:prefLabel xml:lang="pt">canecas</skos:prefLabel>
	<skos:altLabel xml:lang="de">Tassen</skos:altLabel>
	<skos:prefLabel xml:lang="de">Tasse</skos:prefLabel>
	<skos:prefLabel xml:lang="sv">koppar</skos:prefLabel>
	<skos:prefLabel xml:lang="hr">šalica</skos:prefLabel>
	<skos:prefLabel xml:lang="fi">kupit</skos:prefLabel>
	<skos:inScheme rdf:resource="http://partage.vocnet.org/Objects"/>
	<skos:broader rdf:resource="http://partage.vocnet.org/part00403"/>
	<skos:exactMatch rdf:resource="http://vocab.getty.edu/aat/300043202"/>
	<skos:editorialNote xml:lang="en">PPRefiningObjectType</skos:editorialNote>
	<skos:scopeNote xml:lang="en">Open bowl-shaped vessels, used chiefly for drinking, often having one handle, but sometimes two handles or none, generally on a low foot-ring; also includes similar bowl-shaped vessels, generally without handles, resting on a stem and supported by a spreading foot. Occasionally made with a lid.</skos:scopeNote>
</skos:Concept>
<skos:Concept rdf:about="http://partage.vocnet.org/part00689">
	<skos:prefLabel xml:lang="en">decanters</skos:prefLabel>
	<skos:prefLabel xml:lang="pt">decantador</skos:prefLabel>
	<skos:altLabel xml:lang="de">Dekantierkraraffen</skos:altLabel>
	<skos:altLabel xml:lang="de">Dekantierkraraffe</skos:altLabel>
	<skos:prefLabel xml:lang="de">Dekanter</skos:prefLabel>
	<skos:prefLabel xml:lang="sv">karaffer</skos:prefLabel>
	<skos:prefLabel xml:lang="hr">boca.</skos:prefLabel>
	<skos:prefLabel xml:lang="fi">viinikarahvit</skos:prefLabel>
	<skos:inScheme rdf:resource="http://partage.vocnet.org/Objects"/>
	<skos:broader rdf:resource="http://partage.vocnet.org/part00085"/>
	<skos:exactMatch rdf:resource="http://vocab.getty.edu/aat/300045664"/>
	<skos:editorialNote xml:lang="en">PPRefiningObjectType</skos:editorialNote>
	<skos:scopeNote xml:lang="en">Decorative bottles, often with a stopper, used to store or serve beverages, especially wine or liquor.</skos:scopeNote>
</skos:Concept>
<skos:Concept rdf:about="http://partage.vocnet.org/part00690">
	<skos:prefLabel xml:lang="en">drinking glasses</skos:prefLabel>
	<skos:prefLabel xml:lang="pt">copos</skos:prefLabel>
	<skos:altLabel xml:lang="de">Trinkglas</skos:altLabel>
	<skos:prefLabel xml:lang="de">Trinkgläser</skos:prefLabel>
	<skos:prefLabel xml:lang="sv">dricksglas</skos:prefLabel>
	<skos:prefLabel xml:lang="hr">čaša za piće</skos:prefLabel>
	<skos:prefLabel xml:lang="fi">juomalasit</skos:prefLabel>
	<skos:inScheme rdf:resource="http://partage.vocnet.org/Objects"/>
	<skos:broader rdf:resource="http://partage.vocnet.org/part00403"/>
	<skos:narrower rdf:resource="http://partage.vocnet.org/part00691"/>
	<skos:narrower rdf:resource="http://partage.vocnet.org/part00692"/>
	<skos:exactMatch rdf:resource="http://vocab.getty.edu/aat/300043230"/>
	<skos:editorialNote xml:lang="en">PPRefiningObjectType</skos:editorialNote>
	<skos:scopeNote xml:lang="en">Vessels intended for an individual to use for drinking wine, water, or other beverage.</skos:scopeNote>
</skos:Concept>
<skos:Concept rdf:about="http://partage.vocnet.org/part00691">
	<skos:altLabel xml:lang="en">tumblers (drinking glasses)</skos:altLabel>
	<skos:prefLabel xml:lang="en">tumblers</skos:prefLabel>
	<skos:prefLabel xml:lang="de">Tumbler</skos:prefLabel>
	<skos:prefLabel xml:lang="sv">dricksglas.</skos:prefLabel>
	<skos:prefLabel xml:lang="hr">čaša za vodu</skos:prefLabel>
	<skos:prefLabel xml:lang="pt">copos.</skos:prefLabel>
	<skos:prefLabel xml:lang="fi">juomalasit.</skos:prefLabel>
	<skos:inScheme rdf:resource="http://partage.vocnet.org/Objects"/>
	<skos:broader rdf:resource="http://partage.vocnet.org/part00690"/>
	<skos:exactMatch rdf:resource="http://vocab.getty.edu/aat/300043257"/>
	<skos:editorialNote xml:lang="en">PPRefiningObjectType</skos:editorialNote>
	<skos:scopeNote xml:lang="en">Drinking vessels without a stem, foot, or handle and traditionally having a rounded bottom; also includes similar forms with heavy, flattened bottoms.</skos:scopeNote>
</skos:Concept>
<skos:Concept rdf:about="http://partage.vocnet.org/part00692">
	<skos:prefLabel xml:lang="en">goblets</skos:prefLabel>
	<skos:prefLabel xml:lang="sv">pokaler</skos:prefLabel>
	<skos:prefLabel xml:lang="pt">cálice</skos:prefLabel>
	<skos:altLabel xml:lang="de">Kelche</skos:altLabel>
	<skos:altLabel xml:lang="de">Pokale</skos:altLabel>
	<skos:prefLabel xml:lang="de">Kelch</skos:prefLabel>
	<skos:altLabel xml:lang="de">Pokal</skos:altLabel>
	<skos:altLabel xml:lang="hr">pokal</skos:altLabel>
	<skos:prefLabel xml:lang="hr">pehar</skos:prefLabel>
	<skos:prefLabel xml:lang="fi">pikarit.</skos:prefLabel>
	<skos:inScheme rdf:resource="http://partage.vocnet.org/Objects"/>
	<skos:broader rdf:resource="http://partage.vocnet.org/part00690"/>
	<skos:exactMatch rdf:resource="http://vocab.getty.edu/aat/300043236"/>
	<skos:editorialNote xml:lang="en">PPRefiningObjectType</skos:editorialNote>
	<skos:scopeNote xml:lang="en">Drinking glasses with a large bowl, of various shapes, resting on a stemmed foot.</skos:scopeNote>
</skos:Concept>
<skos:Concept rdf:about="http://partage.vocnet.org/part00693">
	<skos:prefLabel xml:lang="en">tankards</skos:prefLabel>
	<skos:prefLabel xml:lang="sv">sejdlar</skos:prefLabel>
	<skos:prefLabel xml:lang="hr">vrč..</skos:prefLabel>
	<skos:prefLabel xml:lang="pt">caneca de cerveja</skos:prefLabel>
	<skos:prefLabel xml:lang="de">Humpen</skos:prefLabel>
	<skos:altLabel xml:lang="de">Trinkkrüge</skos:altLabel>
	<skos:altLabel xml:lang="de">Trinkkrug</skos:altLabel>
	<skos:altLabel xml:lang="fi">tuopit</skos:altLabel>
	<skos:prefLabel xml:lang="fi">kolpakot</skos:prefLabel>
	<skos:inScheme rdf:resource="http://partage.vocnet.org/Objects"/>
	<skos:broader rdf:resource="http://partage.vocnet.org/part00403"/>
	<skos:exactMatch rdf:resource="http://vocab.getty.edu/aat/300043256"/>
	<skos:editorialNote xml:lang="en">PPRefiningObjectType</skos:editorialNote>
	<skos:scopeNote xml:lang="en">Tall, one-handled drinking vessels, usually with a hinged lid and often a thumbpiece; generally made of silver or pewter, but sometimes made of glass.</skos:scopeNote>
</skos:Concept>
<skos:Concept rdf:about="http://partage.vocnet.org/part00694">
	<skos:prefLabel xml:lang="en">lids</skos:prefLabel>
	<skos:prefLabel xml:lang="hr">poklopac</skos:prefLabel>
	<skos:prefLabel xml:lang="de">Deckel</skos:prefLabel>
	<skos:prefLabel xml:lang="sv">lock</skos:prefLabel>
	<skos:prefLabel xml:lang="pt">tampa</skos:prefLabel>
	<skos:prefLabel xml:lang="fi">kannet</skos:prefLabel>
	<skos:inScheme rdf:resource="http://partage.vocnet.org/Objects"/>
	<skos:broader rdf:resource="http://partage.vocnet.org/part01012"/>
	<skos:exactMatch rdf:resource="http://vocab.getty.edu/aat/300045712"/>
	<skos:editorialNote xml:lang="en">PPRefiningObjectType</skos:editorialNote>
	<skos:scopeNote xml:lang="en">Covers which are usually hinged or otherwise attached.</skos:scopeNote>
</skos:Concept>
<skos:Concept rdf:about="http://partage.vocnet.org/part00695">
	<skos:altLabel xml:lang="en">blouses (main garments)</skos:altLabel>
	<skos:prefLabel xml:lang="en">blouses</skos:prefLabel>
	<skos:prefLabel xml:lang="sv">blusar</skos:prefLabel>
	<skos:prefLabel xml:lang="pt">blusa</skos:prefLabel>
	<skos:altLabel xml:lang="de">Blusen</skos:altLabel>
	<skos:prefLabel xml:lang="de">Bluse</skos:prefLabel>
	<skos:prefLabel xml:lang="hr">bluza</skos:prefLabel>
	<skos:prefLabel xml:lang="fi">puserot</skos:prefLabel>
	<skos:inScheme rdf:resource="http://partage.vocnet.org/Objects"/>
	<skos:broader rdf:resource="http://partage.vocnet.org/part00851"/>
	<skos:exactMatch rdf:resource="http://vocab.getty.edu/aat/300046133"/>
	<skos:editorialNote xml:lang="en">PPRefiningObjectType</skos:editorialNote>
	<skos:scopeNote xml:lang="en">Main garments for the upper body, usually lightweight and loose-fitting, made with or without sleeves and worn over or tucked in the waistband of a skirt or trousers, especially by workmen, peasants and artists. Also, women's garments cut in the style of a man's classic, tailored-cut shirt, having a notch collar, collar band, front placket opening, and usually long sleeves with cuffs.</skos:scopeNote>
</skos:Concept>
<skos:Concept rdf:about="http://partage.vocnet.org/part00696">
	<skos:altLabel xml:lang="en">bodices (main garments)</skos:altLabel>
	<skos:prefLabel xml:lang="en">bodices</skos:prefLabel>
	<skos:prefLabel xml:lang="sv">liv</skos:prefLabel>
	<skos:prefLabel xml:lang="pt">corpete</skos:prefLabel>
	<skos:prefLabel xml:lang="de">Mieder</skos:prefLabel>
	<skos:prefLabel xml:lang="hr">steznik</skos:prefLabel>
	<skos:prefLabel xml:lang="fi">irtomiehustat</skos:prefLabel>
	<skos:inScheme rdf:resource="http://partage.vocnet.org/Objects"/>
	<skos:broader rdf:resource="http://partage.vocnet.org/part00851"/>
	<skos:exactMatch rdf:resource="http://vocab.getty.edu/aat/300209874"/>
	<skos:editorialNote xml:lang="en">PPRefiningObjectType</skos:editorialNote>
	<skos:scopeNote xml:lang="en">Originally, tight fitting, sleeveless garments for the torso and bust, quilted and strengthened with whalebone, worn chiefly by women, but also by men. Bodices were typically cross-laced at the side or back, and worn over a blouse or chemise. The term comes from "a pair of bodies," the use of the plural referring to the fact that the garment was made in two pieces laced together. The term also now refers to the generally tight-fitting upper part of a woman's dress or to any tight-fitting outer vest or waistcoat.</skos:scopeNote>
</skos:Concept>
<skos:Concept rdf:about="http://partage.vocnet.org/part00697">
	<skos:prefLabel xml:lang="en">coats (garments)</skos:prefLabel>
	<skos:altLabel xml:lang="sv">rockar</skos:altLabel>
	<skos:prefLabel xml:lang="sv">kappor</skos:prefLabel>
	<skos:prefLabel xml:lang="pt">casaco</skos:prefLabel>
	<skos:altLabel xml:lang="de">Jacken</skos:altLabel>
	<skos:altLabel xml:lang="de">Mäntel</skos:altLabel>
	<skos:altLabel xml:lang="de">Jacke</skos:altLabel>
	<skos:prefLabel xml:lang="de">Mantel</skos:prefLabel>
	<skos:prefLabel xml:lang="hr">kaput</skos:prefLabel>
	<skos:prefLabel xml:lang="fi">takit</skos:prefLabel>
	<skos:inScheme rdf:resource="http://partage.vocnet.org/Objects"/>
	<skos:broader rdf:resource="http://partage.vocnet.org/part00851"/>
	<skos:exactMatch rdf:resource="http://vocab.getty.edu/aat/300046143"/>
	<skos:editorialNote xml:lang="en">PPRefiningObjectType</skos:editorialNote>
	<skos:scopeNote xml:lang="en">Main garments usually fitted to the upper body, extending below the hip line, open at the front or side and generally having sleeves. Also, similar outer garments worn for warmth or protection from the weather.</skos:scopeNote>
</skos:Concept>
<skos:Concept rdf:about="http://partage.vocnet.org/part00698">
	<skos:altLabel xml:lang="en">dresses (garments)</skos:altLabel>
	<skos:prefLabel xml:lang="en">dresses</skos:prefLabel>
	<skos:prefLabel xml:lang="pt">vestido</skos:prefLabel>
	<skos:altLabel xml:lang="de">Kleider</skos:altLabel>
	<skos:prefLabel xml:lang="de">Kleid</skos:prefLabel>
	<skos:prefLabel xml:lang="sv">klänningar</skos:prefLabel>
	<skos:prefLabel xml:lang="hr">haljina</skos:prefLabel>
	<skos:prefLabel xml:lang="fi">puvut</skos:prefLabel>
	<skos:inScheme rdf:resource="http://partage.vocnet.org/Objects"/>
	<skos:broader rdf:resource="http://partage.vocnet.org/part00851"/>
	<skos:exactMatch rdf:resource="http://vocab.getty.edu/aat/300046159"/>
	<skos:editorialNote xml:lang="en">PPRefiningObjectType</skos:editorialNote>
	<skos:scopeNote xml:lang="en">Main garments for women, children, or infants consisting of a bodice and skirt made in one or more pieces.</skos:scopeNote>
</skos:Concept>
<skos:Concept rdf:about="http://partage.vocnet.org/part00699">
	<skos:prefLabel xml:lang="en">night and dressing wear</skos:prefLabel>
	<skos:prefLabel xml:lang="hr">večernja odjeća</skos:prefLabel>
	<skos:prefLabel xml:lang="de">Nachtwäsche</skos:prefLabel>
	<skos:prefLabel xml:lang="sv">nattdräkter</skos:prefLabel>
	<skos:prefLabel xml:lang="pt">roupa de noite</skos:prefLabel>
	<skos:altLabel xml:lang="de">Nachtkleidung</skos:altLabel>
	<skos:prefLabel xml:lang="fi">yöpuvut</skos:prefLabel>
	<skos:inScheme rdf:resource="http://partage.vocnet.org/Objects"/>
	<skos:broader rdf:resource="http://partage.vocnet.org/part00081"/>
	<skos:relatedMatch rdf:resource="http://vocab.getty.edu/aat/300211604"/>
	<skos:scopeNote xml:lang="en">Garments worn informally around the house, like nightshirts, pyjamas, dressing gowns, house coats.</skos:scopeNote>
	<skos:editorialNote xml:lang="en">PPRefiningObjectType</skos:editorialNote>
</skos:Concept>
<skos:Concept rdf:about="http://partage.vocnet.org/part00700">
	<skos:prefLabel xml:lang="en">underwear</skos:prefLabel>
	<skos:prefLabel xml:lang="sv">underkläder</skos:prefLabel>
	<skos:prefLabel xml:lang="hr">donje rublje</skos:prefLabel>
	<skos:prefLabel xml:lang="pt">roupa interior</skos:prefLabel>
	<skos:prefLabel xml:lang="de">Unterwäsche</skos:prefLabel>
	<skos:prefLabel xml:lang="fi">alusvaatteet</skos:prefLabel>
	<skos:inScheme rdf:resource="http://partage.vocnet.org/Objects"/>
	<skos:broader rdf:resource="http://partage.vocnet.org/part00081"/>
	<skos:exactMatch rdf:resource="http://vocab.getty.edu/aat/300209267"/>
	<skos:editorialNote xml:lang="en">PPRefiningObjectType</skos:editorialNote>
	<skos:scopeNote xml:lang="en">Garments worn beneath main garments, usually next to the skin.</skos:scopeNote>
</skos:Concept>
<skos:Concept rdf:about="http://partage.vocnet.org/part00701">
	<skos:altLabel xml:lang="en">corsages (costume components)</skos:altLabel>
	<skos:prefLabel xml:lang="en">corsages</skos:prefLabel>
	<skos:prefLabel xml:lang="pt">corsage</skos:prefLabel>
	<skos:altLabel xml:lang="de">Korsagen</skos:altLabel>
	<skos:prefLabel xml:lang="de">Korsage</skos:prefLabel>
	<skos:prefLabel xml:lang="sv">bröstbuketter</skos:prefLabel>
	<skos:prefLabel xml:lang="hr">haljetak</skos:prefLabel>
	<skos:prefLabel xml:lang="fi">miehustat</skos:prefLabel>
	<skos:inScheme rdf:resource="http://partage.vocnet.org/Objects"/>
	<skos:broader rdf:resource="http://partage.vocnet.org/part00081"/>
	<skos:broader rdf:resource="http://partage.vocnet.org/part00116"/>
	<skos:exactMatch rdf:resource="http://vocab.getty.edu/aat/300220745"/>
	<skos:editorialNote xml:lang="en">PPRefiningObjectType</skos:editorialNote>
	<skos:scopeNote xml:lang="en">Term used in the 18th and 19th centuries for a woman's bodice or upper portion of a dress or garment.</skos:scopeNote>
</skos:Concept>
<skos:Concept rdf:about="http://partage.vocnet.org/part00702">
	<skos:altLabel xml:lang="en">skirts (garments)</skos:altLabel>
	<skos:prefLabel xml:lang="en">skirts</skos:prefLabel>
	<skos:prefLabel xml:lang="hr">suknja</skos:prefLabel>
	<skos:altLabel xml:lang="pt">saias</skos:altLabel>
	<skos:prefLabel xml:lang="pt">saia</skos:prefLabel>
	<skos:altLabel xml:lang="de">Röcke</skos:altLabel>
	<skos:prefLabel xml:lang="de">Rock</skos:prefLabel>
	<skos:prefLabel xml:lang="sv">kjolar</skos:prefLabel>
	<skos:prefLabel xml:lang="fi">hameet</skos:prefLabel>
	<skos:inScheme rdf:resource="http://partage.vocnet.org/Objects"/>
	<skos:broader rdf:resource="http://partage.vocnet.org/part00851"/>
	<skos:exactMatch rdf:resource="http://vocab.getty.edu/aat/300209932"/>
	<skos:editorialNote xml:lang="en">PPRefiningObjectType</skos:editorialNote>
	<skos:scopeNote xml:lang="en">Main garments of varying length extending from the waist or hip and covering a part of the lower body. Also, the lower part of a dress, coat, or other garment.</skos:scopeNote>
</skos:Concept>
<skos:Concept rdf:about="http://partage.vocnet.org/part00703">
	<skos:altLabel xml:lang="en">suits (main garments)</skos:altLabel>
	<skos:prefLabel xml:lang="en">suits</skos:prefLabel>
	<skos:prefLabel xml:lang="ru">kostymer</skos:prefLabel>
	<skos:prefLabel xml:lang="hr">kostim</skos:prefLabel>
	<skos:prefLabel xml:lang="pt">fato</skos:prefLabel>
	<skos:altLabel xml:lang="de">Anzüge</skos:altLabel>
	<skos:prefLabel xml:lang="de">Anzug</skos:prefLabel>
	<skos:prefLabel xml:lang="fi">puvut.</skos:prefLabel>
	<skos:inScheme rdf:resource="http://partage.vocnet.org/Objects"/>
	<skos:broader rdf:resource="http://partage.vocnet.org/part00851"/>
	<skos:exactMatch rdf:resource="http://vocab.getty.edu/aat/300209863"/>
	<skos:editorialNote xml:lang="en">PPRefiningObjectType</skos:editorialNote>
	<skos:scopeNote xml:lang="en">Sets of two or more garments made to harmonize or match in color. Also, any costume designed to be worn for a special purpose or under particular conditions, such as a space suit or a snowsuit.</skos:scopeNote>
</skos:Concept>
<skos:Concept rdf:about="http://partage.vocnet.org/part00704">
	<skos:altLabel xml:lang="en">bags (costume accessories)</skos:altLabel>
	<skos:prefLabel xml:lang="en">bags</skos:prefLabel>
	<skos:prefLabel xml:lang="sv">väskor</skos:prefLabel>
	<skos:altLabel xml:lang="pt">mala</skos:altLabel>
	<skos:prefLabel xml:lang="pt">bolsa</skos:prefLabel>
	<skos:altLabel xml:lang="de">Taschen</skos:altLabel>
	<skos:prefLabel xml:lang="de">Tasche</skos:prefLabel>
	<skos:prefLabel xml:lang="hr">torba</skos:prefLabel>
	<skos:prefLabel xml:lang="fi">laukut</skos:prefLabel>
	<skos:inScheme rdf:resource="http://partage.vocnet.org/Objects"/>
	<skos:broader rdf:resource="http://partage.vocnet.org/part00080"/>
	<skos:narrower rdf:resource="http://partage.vocnet.org/part00715"/>
	<skos:exactMatch rdf:resource="http://vocab.getty.edu/aat/300198926"/>
	<skos:editorialNote xml:lang="en">PPRefiningObjectType</skos:editorialNote>
	<skos:scopeNote xml:lang="en">Small, medium, or large-sized soft or rigid receptacles, intended for carrying personal articles and usually used as ladies' costume accessories. A bag is closed in on all sides except at the top, where also it generally can be closed, and usually having handles or straps for carrying on the shoulder or in the hand.</skos:scopeNote>
</skos:Concept>
<skos:Concept rdf:about="http://partage.vocnet.org/part00705">
	<skos:altLabel xml:lang="en">belts (costume accessories)</skos:altLabel>
	<skos:prefLabel xml:lang="en">belts</skos:prefLabel>
	<skos:prefLabel xml:lang="de">Gürtel</skos:prefLabel>
	<skos:prefLabel xml:lang="pt">cinto</skos:prefLabel>
	<skos:altLabel xml:lang="sv">skärp</skos:altLabel>
	<skos:prefLabel xml:lang="sv">bälten</skos:prefLabel>
	<skos:prefLabel xml:lang="hr">remen</skos:prefLabel>
	<skos:prefLabel xml:lang="fi">vyöt</skos:prefLabel>
	<skos:inScheme rdf:resource="http://partage.vocnet.org/Objects"/>
	<skos:broader rdf:resource="http://partage.vocnet.org/part00080"/>
	<skos:exactMatch rdf:resource="http://vocab.getty.edu/aat/300210002"/>
	<skos:editorialNote xml:lang="en">PPRefiningObjectType</skos:editorialNote>
	<skos:scopeNote xml:lang="en">Flexible straps or bands generally encircling the waist or hips or passing over the shoulder and usually having some type of fastener, such as a buckle; worn for decoration, support, or to carry such items as weapons, tools, or money.</skos:scopeNote>
</skos:Concept>
<skos:Concept rdf:about="http://partage.vocnet.org/part00706">
	<skos:prefLabel xml:lang="en">footwear</skos:prefLabel>
	<skos:prefLabel xml:lang="sv">skodon</skos:prefLabel>
	<skos:prefLabel xml:lang="pt">calçado</skos:prefLabel>
	<skos:prefLabel xml:lang="de">Schuhwerk</skos:prefLabel>
	<skos:prefLabel xml:lang="hr">obuća</skos:prefLabel>
	<skos:prefLabel xml:lang="fi">jalkineet</skos:prefLabel>
	<skos:inScheme rdf:resource="http://partage.vocnet.org/Objects"/>
	<skos:broader rdf:resource="http://partage.vocnet.org/part00080"/>
	<skos:exactMatch rdf:resource="http://vocab.getty.edu/aat/300209280"/>
	<skos:editorialNote xml:lang="en">PPRefiningObjectType</skos:editorialNote>
	<skos:scopeNote xml:lang="en">Coverings for the feet that sometimes extend above the ankle; generally made of durable materials. Distinguished from "hosiery," which is primarily leg coverings.</skos:scopeNote>
</skos:Concept>
<skos:Concept rdf:about="http://partage.vocnet.org/part00707">
	<skos:altLabel xml:lang="en">buttons (fasteners)</skos:altLabel>
	<skos:prefLabel xml:lang="en">buttons</skos:prefLabel>
	<skos:prefLabel xml:lang="sv">knappar</skos:prefLabel>
	<skos:prefLabel xml:lang="pt">botões</skos:prefLabel>
	<skos:altLabel xml:lang="de">Knöpfe</skos:altLabel>
	<skos:prefLabel xml:lang="de">Knopf</skos:prefLabel>
	<skos:prefLabel xml:lang="hr">dugme</skos:prefLabel>
	<skos:prefLabel xml:lang="fi">napit</skos:prefLabel>
	<skos:inScheme rdf:resource="http://partage.vocnet.org/Objects"/>
	<skos:broader rdf:resource="http://partage.vocnet.org/part00711"/>
	<skos:exactMatch rdf:resource="http://vocab.getty.edu/aat/300239261"/>
	<skos:scopeNote xml:lang="en">Disks, balls, or devices of other shape having holes or a shank by which they are sewn or secured to an article and that are used as fasteners by passing through a buttonhole or loop or a trimming.</skos:scopeNote>
	<skos:editorialNote xml:lang="en">PPRefiningObjectType</skos:editorialNote>
</skos:Concept>
<skos:Concept rdf:about="http://partage.vocnet.org/part00708">
	<skos:prefLabel xml:lang="en">chatelaines</skos:prefLabel>
	<skos:prefLabel xml:lang="sv">chatelainer</skos:prefLabel>
	<skos:prefLabel xml:lang="pt">chateleine</skos:prefLabel>
	<skos:altLabel xml:lang="de">Chatelaines</skos:altLabel>
	<skos:prefLabel xml:lang="de">Chatelaine</skos:prefLabel>
	<skos:prefLabel xml:lang="hr">chatelaines</skos:prefLabel>
	<skos:prefLabel xml:lang="fi">vyökorut</skos:prefLabel>
	<skos:inScheme rdf:resource="http://partage.vocnet.org/Objects"/>
	<skos:broader rdf:resource="http://partage.vocnet.org/part00080"/>
	<skos:exactMatch rdf:resource="http://vocab.getty.edu/aat/300209297"/>
	<skos:editorialNote xml:lang="en">PPRefiningObjectType</skos:editorialNote>
	<skos:scopeNote xml:lang="en">Ornamental chains, pins, or clasps usually worn at a woman's waist, to which trinkets, keys, purses, or other articles are attached.</skos:scopeNote>
</skos:Concept>
<skos:Concept rdf:about="http://partage.vocnet.org/part00709">
	<skos:prefLabel xml:lang="en">combs (hair ornaments)</skos:prefLabel>
	<skos:prefLabel xml:lang="pt">pente</skos:prefLabel>
	<skos:altLabel xml:lang="de">Kämme (Haarschmuck)</skos:altLabel>
	<skos:prefLabel xml:lang="de">Kamm (Haarschmuck)</skos:prefLabel>
	<skos:prefLabel xml:lang="sv">prydnadskammar</skos:prefLabel>
	<skos:prefLabel xml:lang="hr">češalj</skos:prefLabel>
	<skos:prefLabel xml:lang="fi">koristekammat</skos:prefLabel>
	<skos:inScheme rdf:resource="http://partage.vocnet.org/Objects"/>
	<skos:broader rdf:resource="http://partage.vocnet.org/part00714"/>
	<skos:exactMatch rdf:resource="http://vocab.getty.edu/aat/300046265"/>
	<skos:editorialNote xml:lang="en">PPRefiningObjectType</skos:editorialNote>
	<skos:scopeNote xml:lang="en">Implements having two or more teeth and an ornamental portion intended to be seen when the teeth are inserted in the hair. For similar implements that are intended primarily for grooming rather than display, use "combs (grooming tools)."</skos:scopeNote>
</skos:Concept>
<skos:Concept rdf:about="http://partage.vocnet.org/part00710">
	<skos:altLabel xml:lang="en">clasps (fasteners)</skos:altLabel>
	<skos:prefLabel xml:lang="en">clasps</skos:prefLabel>
	<skos:altLabel xml:lang="sv">spännen.</skos:altLabel>
	<skos:prefLabel xml:lang="sv">lås</skos:prefLabel>
	<skos:altLabel xml:lang="pt">fecho</skos:altLabel>
	<skos:prefLabel xml:lang="pt">fivela.</skos:prefLabel>
	<skos:altLabel xml:lang="de">Schließen</skos:altLabel>
	<skos:prefLabel xml:lang="de">Schließe</skos:prefLabel>
	<skos:prefLabel xml:lang="hr">kopča.</skos:prefLabel>
	<skos:prefLabel xml:lang="fi">säpit (lukot)</skos:prefLabel>
	<skos:inScheme rdf:resource="http://partage.vocnet.org/Objects"/>
	<skos:broader rdf:resource="http://partage.vocnet.org/part00711"/>
	<skos:exactMatch rdf:resource="http://vocab.getty.edu/aat/300239507"/>
	<skos:editorialNote xml:lang="en">PPRefiningObjectType</skos:editorialNote>
	<skos:scopeNote xml:lang="en">steners made of two or more parts, often of metal, and consisting of separate interlocking hooking and catching elements that hold together two or more objects or complimentary parts of the same object.</skos:scopeNote>
</skos:Concept>
<skos:Concept rdf:about="http://partage.vocnet.org/part00711">
	<skos:prefLabel xml:lang="en">fasteners</skos:prefLabel>
	<skos:altLabel xml:lang="de">Verschlüsse</skos:altLabel>
	<skos:prefLabel xml:lang="de">Verschluss</skos:prefLabel>
	<skos:altLabel xml:lang="de">knäppen</skos:altLabel>
	<skos:prefLabel xml:lang="sv">fästanordningar</skos:prefLabel>
	<skos:prefLabel xml:lang="pt">colchete</skos:prefLabel>
	<skos:altLabel xml:lang="hr">spojnica</skos:altLabel>
	<skos:prefLabel xml:lang="hr">vijak</skos:prefLabel>
	<skos:prefLabel xml:lang="fi">kiinnittimet</skos:prefLabel>
	<skos:inScheme rdf:resource="http://partage.vocnet.org/Objects"/>
	<skos:broader rdf:resource="http://partage.vocnet.org/part00116"/>
	<skos:narrower rdf:resource="http://partage.vocnet.org/part00707"/>
	<skos:narrower rdf:resource="http://partage.vocnet.org/part00710"/>
	<skos:narrower rdf:resource="http://partage.vocnet.org/part00781"/>
	<skos:exactMatch rdf:resource="http://vocab.getty.edu/aat/300036363"/>
	<skos:editorialNote xml:lang="en">PPRefiningObjectType</skos:editorialNote>
	<skos:scopeNote xml:lang="en">Devices that fasten or hold together separate parts.</skos:scopeNote>
</skos:Concept>
<skos:Concept rdf:about="http://partage.vocnet.org/part00712">
	<skos:prefLabel xml:lang="en">glove boxes</skos:prefLabel>
	<skos:prefLabel xml:lang="sv">handskaskar</skos:prefLabel>
	<skos:prefLabel xml:lang="pt">luvas de boxe</skos:prefLabel>
	<skos:altLabel xml:lang="de">Handschuhschachteln</skos:altLabel>
	<skos:prefLabel xml:lang="de">Handschuhschachtel</skos:prefLabel>
	<skos:prefLabel xml:lang="hr">kutija za rukavice</skos:prefLabel>
	<skos:prefLabel xml:lang="fi">hansikaskotelot</skos:prefLabel>
	<skos:inScheme rdf:resource="http://partage.vocnet.org/Objects"/>
	<skos:broader rdf:resource="http://partage.vocnet.org/part00085"/>
	<skos:exactMatch rdf:resource="http://vocab.getty.edu/aat/300225931"/>
	<skos:editorialNote xml:lang="en">PPRefiningObjectType</skos:editorialNote>
	<skos:scopeNote xml:lang="en">Boxes, usually long and narrow, for the storage of gloves when not in use. Sometimes contains a fitting on the interior of the lid for the storage of glove stretchers.</skos:scopeNote>
</skos:Concept>
<skos:Concept rdf:about="http://partage.vocnet.org/part00713">
	<skos:prefLabel xml:lang="en">gloves</skos:prefLabel>
	<skos:prefLabel xml:lang="sv">handskar</skos:prefLabel>
	<skos:prefLabel xml:lang="pt">luvas</skos:prefLabel>
	<skos:altLabel xml:lang="de">Handschuhe</skos:altLabel>
	<skos:prefLabel xml:lang="de">Handschuh</skos:prefLabel>
	<skos:prefLabel xml:lang="hr">rukavice</skos:prefLabel>
	<skos:prefLabel xml:lang="fi">hansikkaat</skos:prefLabel>
	<skos:inScheme rdf:resource="http://partage.vocnet.org/Objects"/>
	<skos:broader rdf:resource="http://partage.vocnet.org/part00080"/>
	<skos:exactMatch rdf:resource="http://vocab.getty.edu/aat/300148821"/>
	<skos:editorialNote xml:lang="en">PPRefiningObjectType</skos:editorialNote>
	<skos:scopeNote xml:lang="en">Coverings for the hand enclosing each finger separately, sometimes extending over the wrist and arm.</skos:scopeNote>
</skos:Concept>
<skos:Concept rdf:about="http://partage.vocnet.org/part00714">
	<skos:prefLabel xml:lang="en">hair ornaments</skos:prefLabel>
	<skos:altLabel xml:lang="sv">hårornament</skos:altLabel>
	<skos:prefLabel xml:lang="sv">hårprydnader</skos:prefLabel>
	<skos:prefLabel xml:lang="pt">ornamentos para cabelo</skos:prefLabel>
	<skos:prefLabel xml:lang="de">Haarschmuck</skos:prefLabel>
	<skos:prefLabel xml:lang="hr">ukrasi za kosu</skos:prefLabel>
	<skos:prefLabel xml:lang="fi">hiuskoristeet</skos:prefLabel>
	<skos:inScheme rdf:resource="http://partage.vocnet.org/Objects"/>
	<skos:broader rdf:resource="http://partage.vocnet.org/part00080"/>
	<skos:narrower rdf:resource="http://partage.vocnet.org/part00709"/>
	<skos:exactMatch rdf:resource="http://vocab.getty.edu/aat/300209287"/>
	<skos:editorialNote xml:lang="en">PPRefiningObjectType</skos:editorialNote>
	<skos:scopeNote xml:lang="en">Term generally applied to various types of ornaments, such as hairpins and combs, worn by men or women.</skos:scopeNote>
</skos:Concept>
<skos:Concept rdf:about="http://partage.vocnet.org/part00715">
	<skos:prefLabel xml:lang="en">handbags</skos:prefLabel>
	<skos:prefLabel xml:lang="sv">handväskor</skos:prefLabel>
	<skos:altLabel xml:lang="pt">carteira</skos:altLabel>
	<skos:prefLabel xml:lang="pt">mala de senhora</skos:prefLabel>
	<skos:altLabel xml:lang="de">Handtaschen</skos:altLabel>
	<skos:prefLabel xml:lang="de">Handtasche</skos:prefLabel>
	<skos:prefLabel xml:lang="hr">torbica</skos:prefLabel>
	<skos:prefLabel xml:lang="fi">käsilaukut</skos:prefLabel>
	<skos:inScheme rdf:resource="http://partage.vocnet.org/Objects"/>
	<skos:broader rdf:resource="http://partage.vocnet.org/part00704"/>
	<skos:exactMatch rdf:resource="http://vocab.getty.edu/aat/300312361"/>
	<skos:editorialNote xml:lang="en">PPRefiningObjectType</skos:editorialNote>
	<skos:scopeNote xml:lang="en">Purses, usually with handles or straps, that are designed to be carried in the hand or on the arm and intended as ladies' accessories. Handbags are large enough to carry banknotes, coins, and everyday personal items.</skos:scopeNote>
</skos:Concept>
<skos:Concept rdf:about="http://partage.vocnet.org/part00716">
	<skos:prefLabel xml:lang="en">handkerchiefs</skos:prefLabel>
	<skos:prefLabel xml:lang="sv">näsdukar</skos:prefLabel>
	<skos:prefLabel xml:lang="pt">lenço</skos:prefLabel>
	<skos:altLabel xml:lang="de">Taschentücher</skos:altLabel>
	<skos:prefLabel xml:lang="de">Taschentuch</skos:prefLabel>
	<skos:prefLabel xml:lang="hr">rupčić</skos:prefLabel>
	<skos:prefLabel xml:lang="fi">nenäliinat</skos:prefLabel>
	<skos:inScheme rdf:resource="http://partage.vocnet.org/Objects"/>
	<skos:broader rdf:resource="http://partage.vocnet.org/part00080"/>
	<skos:exactMatch rdf:resource="http://vocab.getty.edu/aat/300216195"/>
	<skos:editorialNote xml:lang="en">PPRefiningObjectType</skos:editorialNote>
	<skos:scopeNote xml:lang="en">Pieces of cloth, usually square, varying in size and material, carried for usefulness or as a costume accessory.</skos:scopeNote>
</skos:Concept>
<skos:Concept rdf:about="http://partage.vocnet.org/part00717">
	<skos:prefLabel xml:lang="en">hats</skos:prefLabel>
	<skos:altLabel xml:lang="sv">mössor</skos:altLabel>
	<skos:prefLabel xml:lang="sv">hattar</skos:prefLabel>
	<skos:prefLabel xml:lang="pt">chapéu</skos:prefLabel>
	<skos:altLabel xml:lang="de">Hüte</skos:altLabel>
	<skos:prefLabel xml:lang="de">Hut</skos:prefLabel>
	<skos:prefLabel xml:lang="hr">šešir</skos:prefLabel>
	<skos:prefLabel xml:lang="fi">hatut</skos:prefLabel>
	<skos:inScheme rdf:resource="http://partage.vocnet.org/Objects"/>
	<skos:broader rdf:resource="http://partage.vocnet.org/part00965"/>
	<skos:exactMatch rdf:resource="http://vocab.getty.edu/aat/300046106"/>
	<skos:editorialNote xml:lang="en">PPRefiningObjectType</skos:editorialNote>
	<skos:scopeNote xml:lang="en">Shaped coverings for the head having a brim and crown, or one of the two.</skos:scopeNote>
</skos:Concept>
<skos:Concept rdf:about="http://partage.vocnet.org/part00718">
	<skos:prefLabel xml:lang="en">headdresses</skos:prefLabel>
	<skos:prefLabel xml:lang="sv">huvudbonader</skos:prefLabel>
	<skos:prefLabel xml:lang="pt">toucado</skos:prefLabel>
	<skos:prefLabel xml:lang="de">Kopfschmuck</skos:prefLabel>
	<skos:prefLabel xml:lang="hr">pokrivalo za glavu (svečano)</skos:prefLabel>
	<skos:altLabel xml:lang="fi">päänkoristeet</skos:altLabel>
	<skos:prefLabel xml:lang="fi">päähineet</skos:prefLabel>
	<skos:inScheme rdf:resource="http://partage.vocnet.org/Objects"/>
	<skos:broader rdf:resource="http://partage.vocnet.org/part00965"/>
	<skos:exactMatch rdf:resource="http://vocab.getty.edu/aat/300046023"/>
	<skos:editorialNote xml:lang="en">PPRefiningObjectType</skos:editorialNote>
	<skos:scopeNote xml:lang="en">Elaborate coverings or objects for the head, especially those worn for ceremonial or ornamental purposes.</skos:scopeNote>
</skos:Concept>
<skos:Concept rdf:about="http://partage.vocnet.org/part00719">
	<skos:prefLabel xml:lang="en">fans (costume accessories)</skos:prefLabel>
	<skos:altLabel xml:lang="en">fans</skos:altLabel>
	<skos:prefLabel xml:lang="pt">leque</skos:prefLabel>
	<skos:prefLabel xml:lang="de">Fächer (Accessoirs)</skos:prefLabel>
	<skos:prefLabel xml:lang="sv">solfjädrar</skos:prefLabel>
	<skos:prefLabel xml:lang="hr">lepeza</skos:prefLabel>
	<skos:prefLabel xml:lang="fi">viuhkat (leyhyttelyväline)</skos:prefLabel>
	<skos:inScheme rdf:resource="http://partage.vocnet.org/Objects"/>
	<skos:broader rdf:resource="http://partage.vocnet.org/part00080"/>
	<skos:exactMatch rdf:resource="http://vocab.getty.edu/aat/300258857"/>
	<skos:editorialNote xml:lang="en">PPRefiningObjectType</skos:editorialNote>
	<skos:scopeNote xml:lang="en">Hand-held implements used to produce a current of air or that serve as purely decorative accessories; may be rigid or collapsible.</skos:scopeNote>
</skos:Concept>
<skos:Concept rdf:about="http://partage.vocnet.org/part00720">
	<skos:prefLabel xml:lang="en">parures</skos:prefLabel>
	<skos:prefLabel xml:lang="hr">komplet nakita</skos:prefLabel>
	<skos:altLabel xml:lang="de">Parüren</skos:altLabel>
	<skos:prefLabel xml:lang="de">Parüre</skos:prefLabel>
	<skos:altLabel xml:lang="sv">garnityr</skos:altLabel>
	<skos:prefLabel xml:lang="sv">paryr</skos:prefLabel>
	<skos:prefLabel xml:lang="pt">jogo de jóias</skos:prefLabel>
	<skos:prefLabel xml:lang="fi">korusetit</skos:prefLabel>
	<skos:inScheme rdf:resource="http://partage.vocnet.org/Objects"/>
	<skos:exactMatch rdf:resource="http://vocab.getty.edu/aat/300261068"/>
	<skos:editorialNote xml:lang="en">PPRefiningObjectType</skos:editorialNote>
	<skos:scopeNote xml:lang="en">Matched sets of ornaments intended to be worn together, either jewels or trimmings for costume, usually a collar and cuffs.</skos:scopeNote>
</skos:Concept>
<skos:Concept rdf:about="http://partage.vocnet.org/part00721">
	<skos:prefLabel xml:lang="en">wallets</skos:prefLabel>
	<skos:prefLabel xml:lang="hr">novčanik</skos:prefLabel>
	<skos:prefLabel xml:lang="pt">porta-moedas</skos:prefLabel>
	<skos:altLabel xml:lang="pt">carteira.</skos:altLabel>
	<skos:altLabel xml:lang="de">Geldbörsen</skos:altLabel>
	<skos:altLabel xml:lang="de">Geldbörse</skos:altLabel>
	<skos:altLabel xml:lang="de">Portefeuilles</skos:altLabel>
	<skos:altLabel xml:lang="de">Portefeuille</skos:altLabel>
	<skos:altLabel xml:lang="de">Brieftaschen</skos:altLabel>
	<skos:prefLabel xml:lang="de">Brieftasche</skos:prefLabel>
	<skos:prefLabel xml:lang="sv">plånböcker</skos:prefLabel>
	<skos:prefLabel xml:lang="fi">lompakot</skos:prefLabel>
	<skos:inScheme rdf:resource="http://partage.vocnet.org/Objects"/>
	<skos:broader rdf:resource="http://partage.vocnet.org/part00085"/>
	<skos:exactMatch rdf:resource="http://vocab.getty.edu/aat/300046230"/>
	<skos:editorialNote xml:lang="en">PPRefiningObjectType</skos:editorialNote>
	<skos:scopeNote xml:lang="en">Relatively small, flat, often folding containers, typically of leather, designed with slits, pockets, and compartments for carrying paper money, credit cards, driver's license, and coins, and designed to be carried in a pocket or a ladies' purse.</skos:scopeNote>
</skos:Concept>
<skos:Concept rdf:about="http://partage.vocnet.org/part00722">
	<skos:prefLabel xml:lang="en">scarves (costume accessories)</skos:prefLabel>
	<skos:altLabel xml:lang="hr">marama</skos:altLabel>
	<skos:prefLabel xml:lang="hr">šal</skos:prefLabel>
	<skos:prefLabel xml:lang="pt">écharpe</skos:prefLabel>
	<skos:altLabel xml:lang="de">Halstücher</skos:altLabel>
	<skos:altLabel xml:lang="de">Schals</skos:altLabel>
	<skos:altLabel xml:lang="de">Halstuch</skos:altLabel>
	<skos:prefLabel xml:lang="de">Schal</skos:prefLabel>
	<skos:prefLabel xml:lang="sv">sjalar (dräkt accessoarer)</skos:prefLabel>
	<skos:prefLabel xml:lang="fi">huivit</skos:prefLabel>
	<skos:inScheme rdf:resource="http://partage.vocnet.org/Objects"/>
	<skos:broader rdf:resource="http://partage.vocnet.org/part00080"/>
	<skos:exactMatch rdf:resource="http://vocab.getty.edu/aat/300046123"/>
	<skos:editorialNote xml:lang="en">PPRefiningObjectType</skos:editorialNote>
	<skos:scopeNote xml:lang="en">Pieces of cloth made in varying widths and lengths and worn for decoration or warmth across the shoulders, around the neck, over the head, or about the waist.</skos:scopeNote>
</skos:Concept>
<skos:Concept rdf:about="http://partage.vocnet.org/part00723">
	<skos:prefLabel xml:lang="en">stockings</skos:prefLabel>
	<skos:prefLabel xml:lang="sv">strumpor</skos:prefLabel>
	<skos:prefLabel xml:lang="hr">samostojeće čarape</skos:prefLabel>
	<skos:altLabel xml:lang="pt">meias</skos:altLabel>
	<skos:prefLabel xml:lang="pt">meia</skos:prefLabel>
	<skos:altLabel xml:lang="de">Strümpfe</skos:altLabel>
	<skos:prefLabel xml:lang="de">Strumpf</skos:prefLabel>
	<skos:prefLabel xml:lang="fi">sukat</skos:prefLabel>
	<skos:inScheme rdf:resource="http://partage.vocnet.org/Objects"/>
	<skos:broader rdf:resource="http://partage.vocnet.org/part00974"/>
	<skos:exactMatch rdf:resource="http://vocab.getty.edu/aat/300046088"/>
	<skos:editorialNote xml:lang="en">PPRefiningObjectType</skos:editorialNote>
	<skos:scopeNote xml:lang="en">Hosiery that covers the foot and extends to the knee or above; can be heavy or lightweight.</skos:scopeNote>
</skos:Concept>
<skos:Concept rdf:about="http://partage.vocnet.org/part00724">
	<skos:prefLabel xml:lang="en">studios (work spaces)</skos:prefLabel>
	<skos:prefLabel xml:lang="sv">ateljéer</skos:prefLabel>
	<skos:prefLabel xml:lang="hr">atelier (radna soba)</skos:prefLabel>
	<skos:prefLabel xml:lang="pt">estúdio</skos:prefLabel>
	<skos:altLabel xml:lang="de">Ateliers</skos:altLabel>
	<skos:altLabel xml:lang="de">Künstlerwerkstatt</skos:altLabel>
	<skos:altLabel xml:lang="de">Studio</skos:altLabel>
	<skos:prefLabel xml:lang="de">Atelier</skos:prefLabel>
	<skos:prefLabel xml:lang="fi">ateljeet</skos:prefLabel>
	<skos:inScheme rdf:resource="http://partage.vocnet.org/Objects"/>
	<skos:broader rdf:resource="http://partage.vocnet.org/part00116"/>
	<skos:exactMatch rdf:resource="http://vocab.getty.edu/aat/300007725"/>
	<skos:editorialNote xml:lang="en">PPRefiningObjectType</skos:editorialNote>
	<skos:scopeNote xml:lang="en">Working places set aside for artists to work. The term is generally applied to workspaces used by artists creating fine art, particularly art dating from the 16th century to the present. The characteristics of a studio may be dictated by the practical requirements of adequate light, ample space in which to create the work of art, and storage of materials. Display of the finished art works and training may also be accommodated in a studio. Creation of an art work may require a range of artistic processes; therefore, separate areas of work may be delegated in the studio. The term may also refer to spaces used by dancers, singers, musicians, and other performing artists to create or practice. The term "workshops" is generally refers to spaces used by craftspeople, artists working prior to the 16th century, and industrial workers. For studios that are larger spaces or complexes, and are used to create films, television or radio programs, or other large scale productions, use "motion picture studios," "broadcasting studios," "sound studios," "recording studios," "radio studios," or "television studios."</skos:scopeNote>
</skos:Concept>
<skos:Concept rdf:about="http://partage.vocnet.org/part00725">
	<skos:altLabel xml:lang="en">chapels (rooms or structures)</skos:altLabel>
	<skos:prefLabel xml:lang="en">chapels</skos:prefLabel>
	<skos:prefLabel xml:lang="sv">kapell</skos:prefLabel>
	<skos:prefLabel xml:lang="pt">capela</skos:prefLabel>
	<skos:altLabel xml:lang="de">Kapellen</skos:altLabel>
	<skos:prefLabel xml:lang="de">Kapelle</skos:prefLabel>
	<skos:prefLabel xml:lang="hr">kapela</skos:prefLabel>
	<skos:prefLabel xml:lang="fi">kappelit</skos:prefLabel>
	<skos:inScheme rdf:resource="http://partage.vocnet.org/Objects"/>
	<skos:broader rdf:resource="http://partage.vocnet.org/part00072"/>
	<skos:exactMatch rdf:resource="http://vocab.getty.edu/aat/300004590"/>
	<skos:editorialNote xml:lang="en">PPRefiningObjectType</skos:editorialNote>
	<skos:scopeNote xml:lang="en">Rooms or small buildings that serve as sanctuaries or places of Christian worship. A chapel may be used for private worship in or attached to a church, palace, house, prison, monastery, or school. It may alternatively be used for public worship of the established Church, subordinate to or dependent upon the parish church, the accommodation supplied by which it in some way supplements. The concept includes both freestanding chapels and rooms or recesses serving as chapels in churches or other buildings. The Latin "cappella" or the French-derived "chappelle" or "chapelle" are occasionally used for "chapel" in English texts. The term may also be used in its original meaning, which was to refer specifically to the shrine in which the kings of France preserved the cape (cloak) of St. Martin.</skos:scopeNote>
</skos:Concept>
<skos:Concept rdf:about="http://partage.vocnet.org/part00726">
	<skos:altLabel xml:lang="en">bridges (built works)</skos:altLabel>
	<skos:prefLabel xml:lang="en">bridges</skos:prefLabel>
	<skos:prefLabel xml:lang="sv">broar</skos:prefLabel>
	<skos:prefLabel xml:lang="pt">ponte</skos:prefLabel>
	<skos:altLabel xml:lang="de">Brücken</skos:altLabel>
	<skos:prefLabel xml:lang="de">Brücke</skos:prefLabel>
	<skos:prefLabel xml:lang="hr">most</skos:prefLabel>
	<skos:prefLabel xml:lang="fi">sillat</skos:prefLabel>
	<skos:inScheme rdf:resource="http://partage.vocnet.org/Objects"/>
	<skos:exactMatch rdf:resource="http://vocab.getty.edu/aat/300007836"/>
	<skos:editorialNote xml:lang="en">PPRefiningObjectType</skos:editorialNote>
	<skos:scopeNote xml:lang="en">Structures spanning and providing passage over waterways, topographic depressions, transportation routes, or similar circulation barriers.</skos:scopeNote>
</skos:Concept>
<skos:Concept rdf:about="http://partage.vocnet.org/part00727">
	<skos:altLabel xml:lang="en">promenades (walkways)</skos:altLabel>
	<skos:prefLabel xml:lang="en">promenades</skos:prefLabel>
	<skos:prefLabel xml:lang="hr">šetnica</skos:prefLabel>
	<skos:altLabel xml:lang="de">Promenaden</skos:altLabel>
	<skos:prefLabel xml:lang="de">Promenade</skos:prefLabel>
	<skos:prefLabel xml:lang="sv">esplanader</skos:prefLabel>
	<skos:prefLabel xml:lang="pt">passeio marítimo</skos:prefLabel>
	<skos:prefLabel xml:lang="fi">kävelykadut</skos:prefLabel>
	<skos:inScheme rdf:resource="http://partage.vocnet.org/Objects"/>
	<skos:broader rdf:resource="http://partage.vocnet.org/part01052"/>
	<skos:exactMatch rdf:resource="http://vocab.getty.edu/aat/300008329"/>
	<skos:editorialNote xml:lang="en">PPRefiningObjectType</skos:editorialNote>
	<skos:scopeNote xml:lang="en">Places for strolling; public walks.</skos:scopeNote>
</skos:Concept>
<skos:Concept rdf:about="http://partage.vocnet.org/part00728">
	<skos:prefLabel xml:lang="en">open spaces</skos:prefLabel>
	<skos:prefLabel xml:lang="hr">otvoreni prostor</skos:prefLabel>
	<skos:prefLabel xml:lang="de">Freifläche</skos:prefLabel>
	<skos:altLabel xml:lang="de">Freiflächen</skos:altLabel>
	<skos:prefLabel xml:lang="sv">öppna ytor</skos:prefLabel>
	<skos:prefLabel xml:lang="pl">espaço aberto</skos:prefLabel>
	<skos:prefLabel xml:lang="fi">aukiot</skos:prefLabel>
	<skos:inScheme rdf:resource="http://partage.vocnet.org/Objects"/>
	<skos:narrower rdf:resource="http://partage.vocnet.org/part01052"/>
	<skos:exactMatch rdf:resource="http://vocab.getty.edu/aat/300008072"/>
	<skos:editorialNote xml:lang="en">PPRefiningObjectType</skos:editorialNote>
	<skos:scopeNote xml:lang="en">Spaces in urban environments designed as passages for pedestrians, and as social spaces, not as clearly delimited as parks, but sharing some of the same characteristics. Often these function as utilitarian connecting spaces between buildings, or simply as an open area designated by a municipal authority, but without the amenities or formality of a park.</skos:scopeNote>
</skos:Concept>
<skos:Concept rdf:about="http://partage.vocnet.org/part00729">
	<skos:altLabel xml:lang="en">theaters (buildings)</skos:altLabel>
	<skos:prefLabel xml:lang="en">theatres (buildings)</skos:prefLabel>
	<skos:prefLabel xml:lang="sv">teatrar</skos:prefLabel>
	<skos:prefLabel xml:lang="hr">kazalište</skos:prefLabel>
	<skos:prefLabel xml:lang="pt">teatro</skos:prefLabel>
	<skos:prefLabel xml:lang="de">Theater (Gebäude)</skos:prefLabel>
	<skos:prefLabel xml:lang="fi">teatterirakennukset</skos:prefLabel>
	<skos:inScheme rdf:resource="http://partage.vocnet.org/Objects"/>
	<skos:narrower rdf:resource="http://partage.vocnet.org/part00733"/>
	<skos:exactMatch rdf:resource="http://vocab.getty.edu/aat/300007117"/>
	<skos:editorialNote xml:lang="en">PPRefiningObjectType</skos:editorialNote>
	<skos:scopeNote xml:lang="en">Buildings having a stage or projection screen for the presentation of dramatic performances and providing seating areas for spectators.</skos:scopeNote>
</skos:Concept>
<skos:Concept rdf:about="http://partage.vocnet.org/part00730">
	<skos:prefLabel xml:lang="en">orphanages (buildings)</skos:prefLabel>
	<skos:prefLabel xml:lang="hr">sirotište</skos:prefLabel>
	<skos:altLabel xml:lang="de">Waisenhäuser</skos:altLabel>
	<skos:prefLabel xml:lang="de">Waisenhaus</skos:prefLabel>
	<skos:prefLabel xml:lang="sv">barnhem</skos:prefLabel>
	<skos:prefLabel xml:lang="pt">orfanato</skos:prefLabel>
	<skos:prefLabel xml:lang="fi">orpokodit</skos:prefLabel>
	<skos:inScheme rdf:resource="http://partage.vocnet.org/Objects"/>
	<skos:broader rdf:resource="http://partage.vocnet.org/part01034"/>
	<skos:exactMatch rdf:resource="http://vocab.getty.edu/aat/300006769"/>
	<skos:editorialNote xml:lang="en">PPRefiningObjectType</skos:editorialNote>
	<skos:scopeNote xml:lang="en">Buildings that house facilities for the housing and care of orphans, who are children whose parents are either dead or otherwise unable to care for their child.</skos:scopeNote>
</skos:Concept>
<skos:Concept rdf:about="http://partage.vocnet.org/part00731">
	<skos:prefLabel xml:lang="en">museums (buildings)</skos:prefLabel>
	<skos:prefLabel xml:lang="hr">muzej</skos:prefLabel>
	<skos:altLabel xml:lang="de">Museen (Gebäude)</skos:altLabel>
	<skos:prefLabel xml:lang="de">Museum (Gebäude)</skos:prefLabel>
	<skos:prefLabel xml:lang="sv">museer (byggnader)</skos:prefLabel>
	<skos:prefLabel xml:lang="pt">museu</skos:prefLabel>
	<skos:prefLabel xml:lang="fi">museorakennukset</skos:prefLabel>
	<skos:inScheme rdf:resource="http://partage.vocnet.org/Objects"/>
	<skos:broader rdf:resource="http://partage.vocnet.org/part00152"/>
	<skos:exactMatch rdf:resource="http://vocab.getty.edu/aat/300005768"/>
	<skos:editorialNote xml:lang="en">PPRefiningObjectType</skos:editorialNote>
	<skos:scopeNote xml:lang="en">Refers to buildings, groups of buildings, or spaces within buildings where objects of value such as works of art, antiquities, scientific specimens, or other artifacts are housed and displayed for public benefit.</skos:scopeNote>
</skos:Concept>
<skos:Concept rdf:about="http://partage.vocnet.org/part00732">
	<skos:altLabel xml:lang="en">hotels (public accomodations)</skos:altLabel>
	<skos:prefLabel xml:lang="en">hotels</skos:prefLabel>
	<skos:prefLabel xml:lang="hr">hotel</skos:prefLabel>
	<skos:altLabel xml:lang="de">Hotels</skos:altLabel>
	<skos:prefLabel xml:lang="de">Hotel</skos:prefLabel>
	<skos:prefLabel xml:lang="sv">hotell</skos:prefLabel>
	<skos:altLabel xml:lang="de">hóteis</skos:altLabel>
	<skos:prefLabel xml:lang="pt">hotel</skos:prefLabel>
	<skos:prefLabel xml:lang="fi">hotellit</skos:prefLabel>
	<skos:inScheme rdf:resource="http://partage.vocnet.org/Objects"/>
	<skos:exactMatch rdf:resource="http://vocab.getty.edu/aat/300007166"/>
	<skos:editorialNote xml:lang="en">PPRefiningObjectType</skos:editorialNote>
	<skos:scopeNote xml:lang="en">Buildings where travellers or tourists are provided with overnight accommodation, meals, and other services; often distinguished from inns and other forms of temporary lodging for travellers by their larger size and range of facilities, in modern times often equipped with a restaurant, bar, conference rooms, and leisure facilities.</skos:scopeNote>
</skos:Concept>
<skos:Concept rdf:about="http://partage.vocnet.org/part00733">
	<skos:altLabel xml:lang="en">movie theatres</skos:altLabel>
	<skos:altLabel xml:lang="en">motion picture theaters</skos:altLabel>
	<skos:prefLabel xml:lang="en">cinemas</skos:prefLabel>
	<skos:prefLabel xml:lang="sv">biografer</skos:prefLabel>
	<skos:prefLabel xml:lang="pt">cinema</skos:prefLabel>
	<skos:altLabel xml:lang="de">Lichtspielhäuser</skos:altLabel>
	<skos:altLabel xml:lang="de">Kinos</skos:altLabel>
	<skos:altLabel xml:lang="de">Filmtheater</skos:altLabel>
	<skos:altLabel xml:lang="de">Lichtspielhaus</skos:altLabel>
	<skos:prefLabel xml:lang="de">Kino</skos:prefLabel>
	<skos:prefLabel xml:lang="hr">kino</skos:prefLabel>
	<skos:prefLabel xml:lang="fi">elokuvateatterit</skos:prefLabel>
	<skos:inScheme rdf:resource="http://partage.vocnet.org/Objects"/>
	<skos:broader rdf:resource="http://partage.vocnet.org/part00729"/>
	<skos:exactMatch rdf:resource="http://vocab.getty.edu/aat/300007135"/>
	<skos:editorialNote xml:lang="en">PPRefiningObjectType</skos:editorialNote>
	<skos:scopeNote xml:lang="en">Theaters designed and equipped for the presentation of motion pictures to the public, or any buildings in which films are shown.</skos:scopeNote>
</skos:Concept>
<skos:Concept rdf:about="http://partage.vocnet.org/part00734">
	<skos:prefLabel xml:lang="en">casinos</skos:prefLabel>
	<skos:prefLabel xml:lang="sv">kasinon</skos:prefLabel>
	<skos:prefLabel xml:lang="pt">casino</skos:prefLabel>
	<skos:altLabel xml:lang="de">Spielkasinos</skos:altLabel>
	<skos:altLabel xml:lang="de">Spielcasinos</skos:altLabel>
	<skos:altLabel xml:lang="de">Spielbanken</skos:altLabel>
	<skos:altLabel xml:lang="de">Spielbank</skos:altLabel>
	<skos:altLabel xml:lang="de">Spielcasino</skos:altLabel>
	<skos:prefLabel xml:lang="de">Spielkasino</skos:prefLabel>
	<skos:prefLabel xml:lang="hr">kockarnica</skos:prefLabel>
	<skos:prefLabel xml:lang="fi">kasinot</skos:prefLabel>
	<skos:inScheme rdf:resource="http://partage.vocnet.org/Objects"/>
	<skos:broader rdf:resource="http://partage.vocnet.org/part00853"/>
	<skos:exactMatch rdf:resource="http://vocab.getty.edu/aat/300007227"/>
	<skos:scopeNote xml:lang="en">Public entertainment buildings for meeting, dancing, and general recreation, often with eating and drinking facilities, music, and game rooms; for similar buildings equipped with gambling devices, use "gambling casinos."</skos:scopeNote>
	<skos:editorialNote xml:lang="en">PPRefiningObjectType</skos:editorialNote>
</skos:Concept>
<skos:Concept rdf:about="http://partage.vocnet.org/part00735">
	<skos:prefLabel xml:lang="en">post offices</skos:prefLabel>
	<skos:prefLabel xml:lang="hr">pošta</skos:prefLabel>
	<skos:altLabel xml:lang="de">Postämter</skos:altLabel>
	<skos:prefLabel xml:lang="de">Postamt</skos:prefLabel>
	<skos:prefLabel xml:lang="sv">postkontor</skos:prefLabel>
	<skos:prefLabel xml:lang="pt">edíficio dos correios</skos:prefLabel>
	<skos:prefLabel xml:lang="fi">postitoimipaikat</skos:prefLabel>
	<skos:inScheme rdf:resource="http://partage.vocnet.org/Objects"/>
	<skos:broader rdf:resource="http://partage.vocnet.org/part00164"/>
	<skos:exactMatch rdf:resource="http://vocab.getty.edu/aat/300006036"/>
	<skos:editorialNote xml:lang="en">PPRefiningObjectType</skos:editorialNote>
	<skos:scopeNote xml:lang="en">Public buildings within a government postal system at which mail is received and sorted, from which it is distributed, and at which stamps are sold and other services rendered.</skos:scopeNote>
</skos:Concept>
<skos:Concept rdf:about="http://partage.vocnet.org/part00736">
	<skos:prefLabel xml:lang="en">drugstores</skos:prefLabel>
	<skos:prefLabel xml:lang="pt">drogaria</skos:prefLabel>
	<skos:prefLabel xml:lang="de">Drogerie</skos:prefLabel>
	<skos:altLabel xml:lang="de">Apotheke</skos:altLabel>
	<skos:prefLabel xml:lang="sv">apotek</skos:prefLabel>
	<skos:prefLabel xml:lang="hr">ljekarna</skos:prefLabel>
	<skos:prefLabel xml:lang="fi">apteekit</skos:prefLabel>
	<skos:inScheme rdf:resource="http://partage.vocnet.org/Objects"/>
	<skos:broader rdf:resource="http://partage.vocnet.org/part00737"/>
	<skos:exactMatch rdf:resource="http://vocab.getty.edu/aat/300005307"/>
	<skos:editorialNote xml:lang="en">PPRefiningObjectType</skos:editorialNote>
	<skos:scopeNote xml:lang="en">Retail stores that include a pharmacy and often sell other articles, such as toilet requisites, stationery, magazines, newspapers, and light refreshments.</skos:scopeNote>
</skos:Concept>
<skos:Concept rdf:about="http://partage.vocnet.org/part00737">
	<skos:altLabel xml:lang="en">stores</skos:altLabel>
	<skos:prefLabel xml:lang="en">shops (stores)</skos:prefLabel>
	<skos:prefLabel xml:lang="ru">butiker</skos:prefLabel>
	<skos:prefLabel xml:lang="hr">dućan</skos:prefLabel>
	<skos:altLabel xml:lang="de">lojas</skos:altLabel>
	<skos:prefLabel xml:lang="pt">loja</skos:prefLabel>
	<skos:altLabel xml:lang="de">Läden</skos:altLabel>
	<skos:altLabel xml:lang="de">Verkaufsraum</skos:altLabel>
	<skos:altLabel xml:lang="de">Ladenlokal</skos:altLabel>
	<skos:prefLabel xml:lang="de">Laden</skos:prefLabel>
	<skos:altLabel xml:lang="de">Geschäft</skos:altLabel>
	<skos:prefLabel xml:lang="fi">myymälät</skos:prefLabel>
	<skos:inScheme rdf:resource="http://partage.vocnet.org/Objects"/>
	<skos:broader rdf:resource="http://partage.vocnet.org/part00739"/>
	<skos:narrower rdf:resource="http://partage.vocnet.org/part00736"/>
	<skos:narrower rdf:resource="http://partage.vocnet.org/part00738"/>
	<skos:exactMatch rdf:resource="http://vocab.getty.edu/aat/300005283"/>
	<skos:editorialNote xml:lang="en">PPRefiningObjectType</skos:editorialNote>
	<skos:scopeNote xml:lang="en">Buildings offering merchandise for sale, usually on a retail basis.</skos:scopeNote>
</skos:Concept>
<skos:Concept rdf:about="http://partage.vocnet.org/part00738">
	<skos:prefLabel xml:lang="en">department stores</skos:prefLabel>
	<skos:prefLabel xml:lang="pt">armazém comercial</skos:prefLabel>
	<skos:altLabel xml:lang="de">Kaufhäuser</skos:altLabel>
	<skos:altLabel xml:lang="de">Warenhäuser</skos:altLabel>
	<skos:altLabel xml:lang="de">Kaufhaus</skos:altLabel>
	<skos:prefLabel xml:lang="de">Warenhaus</skos:prefLabel>
	<skos:prefLabel xml:lang="sv">varuhus</skos:prefLabel>
	<skos:prefLabel xml:lang="hr">trgovina</skos:prefLabel>
	<skos:prefLabel xml:lang="fi">tavaratalot</skos:prefLabel>
	<skos:inScheme rdf:resource="http://partage.vocnet.org/Objects"/>
	<skos:broader rdf:resource="http://partage.vocnet.org/part00737"/>
	<skos:exactMatch rdf:resource="http://vocab.getty.edu/aat/300005344"/>
	<skos:editorialNote xml:lang="en">PPRefiningObjectType</skos:editorialNote>
	<skos:scopeNote xml:lang="en">Large stores selling many different kinds of articles arranged in different departments or areas of the store.</skos:scopeNote>
</skos:Concept>
<skos:Concept rdf:about="http://partage.vocnet.org/part00739">
	<skos:prefLabel xml:lang="en">mercantile buildings</skos:prefLabel>
	<skos:prefLabel xml:lang="hr">trgovačka građevina</skos:prefLabel>
	<skos:altLabel xml:lang="de">Geschäftshäuser</skos:altLabel>
	<skos:altLabel xml:lang="de">Geschäftshaus</skos:altLabel>
	<skos:prefLabel xml:lang="de">Handelsgebäude</skos:prefLabel>
	<skos:prefLabel xml:lang="sv">handelshus</skos:prefLabel>
	<skos:prefLabel xml:lang="pt">edifícios comerciais.</skos:prefLabel>
	<skos:prefLabel xml:lang="fi">liikerakennukset.</skos:prefLabel>
	<skos:inScheme rdf:resource="http://partage.vocnet.org/Objects"/>
	<skos:broader rdf:resource="http://partage.vocnet.org/part00165"/>
	<skos:narrower rdf:resource="http://partage.vocnet.org/part00737"/>
	<skos:exactMatch rdf:resource="http://vocab.getty.edu/aat/300005230"/>
	<skos:editorialNote xml:lang="en">PPRefiningObjectType</skos:editorialNote>
</skos:Concept>
<skos:Concept rdf:about="http://partage.vocnet.org/part00740">
	<skos:altLabel xml:lang="en">banks (financial institutions)</skos:altLabel>
	<skos:prefLabel xml:lang="en">banks (financial institution buildings)</skos:prefLabel>
	<skos:prefLabel xml:lang="de">Bank (Gebäude)</skos:prefLabel>
	<skos:prefLabel xml:lang="sv">banker</skos:prefLabel>
	<skos:prefLabel xml:lang="pt">banco</skos:prefLabel>
	<skos:altLabel xml:lang="de">Banken</skos:altLabel>
	<skos:prefLabel xml:lang="hr">banka</skos:prefLabel>
	<skos:prefLabel xml:lang="fi">pankit</skos:prefLabel>
	<skos:inScheme rdf:resource="http://partage.vocnet.org/Objects"/>
	<skos:broader rdf:resource="http://partage.vocnet.org/part00847"/>
	<skos:exactMatch rdf:resource="http://vocab.getty.edu/aat/300005214"/>
	<skos:editorialNote xml:lang="en">PPRefiningObjectType</skos:editorialNote>
	<skos:scopeNote xml:lang="en">Buildings that house establishments for the custody of money received from, or on behalf of, customers, with the essential duty of payment of the orders given on it by the customers. Banks' profits arise mainly from the investment of the money left unused by the customers. Bank buildings typically have indoor counters and windows where customers may make transactions, often with bars or other security devices securing the window, offices where bank officials may meet with customers, vaults for the secure storage of money and other valuables, and other security devices and measures. Exterior bank architecture traditionally imitates a Greek temple, although many other styles are employed as well.</skos:scopeNote>
</skos:Concept>
<skos:Concept rdf:about="http://partage.vocnet.org/part00741">
	<skos:altLabel xml:lang="en">factories (structures)</skos:altLabel>
	<skos:prefLabel xml:lang="en">factories</skos:prefLabel>
	<skos:prefLabel xml:lang="pt">fábrica</skos:prefLabel>
	<skos:altLabel xml:lang="de">Fabriken</skos:altLabel>
	<skos:prefLabel xml:lang="de">Fabrik</skos:prefLabel>
	<skos:prefLabel xml:lang="sv">fabriker</skos:prefLabel>
	<skos:prefLabel xml:lang="hr">tvornica</skos:prefLabel>
	<skos:prefLabel xml:lang="fi">tehtaat</skos:prefLabel>
	<skos:inScheme rdf:resource="http://partage.vocnet.org/Objects"/>
	<skos:broader rdf:resource="http://partage.vocnet.org/part00172"/>
	<skos:exactMatch rdf:resource="http://vocab.getty.edu/aat/300006232"/>
	<skos:editorialNote xml:lang="en">PPRefiningObjectType</skos:editorialNote>
	<skos:scopeNote xml:lang="en">Refers to a building or group of buildings with the function of housing the action or process of making goods or producing anything, whether before or after the Industrial Revolution of the mid-19th century.</skos:scopeNote>
</skos:Concept>
<skos:Concept rdf:about="http://partage.vocnet.org/part00742">
	<skos:prefLabel xml:lang="en">public baths</skos:prefLabel>
	<skos:prefLabel xml:lang="de">Badeanstalt</skos:prefLabel>
	<skos:altLabel xml:lang="de">Badehaus</skos:altLabel>
	<skos:prefLabel xml:lang="sv">badhus</skos:prefLabel>
	<skos:prefLabel xml:lang="hr">javna kupelj</skos:prefLabel>
	<skos:prefLabel xml:lang="pt">banhos públicos</skos:prefLabel>
	<skos:prefLabel xml:lang="fi">kylpylät</skos:prefLabel>
	<skos:inScheme rdf:resource="http://partage.vocnet.org/Objects"/>
	<skos:broader rdf:resource="http://partage.vocnet.org/part00160"/>
	<skos:exactMatch rdf:resource="http://vocab.getty.edu/aat/300007353"/>
	<skos:editorialNote xml:lang="en">PPRefiningObjectType</skos:editorialNote>
	<skos:scopeNote xml:lang="en">Buildings equipped with swimming pools and other facilities for bathing and swimming, traditionally the primary hygienic facility in a city or town.</skos:scopeNote>
</skos:Concept>
<skos:Concept rdf:about="http://partage.vocnet.org/part00743">
	<skos:prefLabel xml:lang="en">sanatoriums</skos:prefLabel>
	<skos:prefLabel xml:lang="hr">sanatorij</skos:prefLabel>
	<skos:prefLabel xml:lang="pt">sanatório</skos:prefLabel>
	<skos:altLabel xml:lang="de">Sanatorien</skos:altLabel>
	<skos:altLabel xml:lang="de">Kuranstalt</skos:altLabel>
	<skos:altLabel xml:lang="de">Heilanstalt</skos:altLabel>
	<skos:prefLabel xml:lang="de">Sanatorium</skos:prefLabel>
	<skos:prefLabel xml:lang="sv">sanatorier</skos:prefLabel>
	<skos:prefLabel xml:lang="fi">parantolat</skos:prefLabel>
	<skos:inScheme rdf:resource="http://partage.vocnet.org/Objects"/>
	<skos:broader rdf:resource="http://partage.vocnet.org/part01057"/>
	<skos:exactMatch rdf:resource="http://vocab.getty.edu/aat/300006720"/>
	<skos:editorialNote xml:lang="en">PPRefiningObjectType</skos:editorialNote>
	<skos:scopeNote xml:lang="en">Health care facilities for the chronically ill.</skos:scopeNote>
</skos:Concept>
<skos:Concept rdf:about="http://partage.vocnet.org/part00744">
	<skos:altLabel xml:lang="en">pavilions (garden structures)</skos:altLabel>
	<skos:prefLabel xml:lang="en">pavilions</skos:prefLabel>
	<skos:prefLabel xml:lang="hr">paviljon</skos:prefLabel>
	<skos:altLabel xml:lang="de">Pavillons</skos:altLabel>
	<skos:prefLabel xml:lang="de">Pavillon</skos:prefLabel>
	<skos:prefLabel xml:lang="sv">paviljonger</skos:prefLabel>
	<skos:prefLabel xml:lang="pt">pavilhão</skos:prefLabel>
	<skos:prefLabel xml:lang="fi">paviljongit</skos:prefLabel>
	<skos:inScheme rdf:resource="http://partage.vocnet.org/Objects"/>
	<skos:broader rdf:resource="http://partage.vocnet.org/part00986"/>
	<skos:exactMatch rdf:resource="http://vocab.getty.edu/aat/300006819"/>
	<skos:editorialNote xml:lang="en">PPRefiningObjectType</skos:editorialNote>
	<skos:scopeNote xml:lang="en">Light, sometimes ornamental, structures in gardens, parks, or places of recreation that are used for entertainment or shelter.</skos:scopeNote>
</skos:Concept>
<skos:Concept rdf:about="http://partage.vocnet.org/part00745">
	<skos:prefLabel xml:lang="en">steps</skos:prefLabel>
	<skos:prefLabel xml:lang="sv">trappsteg</skos:prefLabel>
	<skos:prefLabel xml:lang="hr">stube</skos:prefLabel>
	<skos:altLabel xml:lang="pt">degraus</skos:altLabel>
	<skos:prefLabel xml:lang="pt">degrau</skos:prefLabel>
	<skos:altLabel xml:lang="de">Stufe</skos:altLabel>
	<skos:prefLabel xml:lang="de">Stufen</skos:prefLabel>
	<skos:prefLabel xml:lang="fi">portaikot</skos:prefLabel>
	<skos:inScheme rdf:resource="http://partage.vocnet.org/Objects"/>
	<skos:broader rdf:resource="http://partage.vocnet.org/part00127"/>
	<skos:exactMatch rdf:resource="http://vocab.getty.edu/aat/300003312"/>
	<skos:scopeNote xml:lang="en">Stair units that consist of one tread and one riser, or any similar element providing a horizontal surface on which to support the foot of a person descending or ascending.</skos:scopeNote>
	<skos:editorialNote xml:lang="en">PPRefiningObjectType</skos:editorialNote>
</skos:Concept>
<skos:Concept rdf:about="http://partage.vocnet.org/part00746">
	<skos:prefLabel xml:lang="en">pilasters</skos:prefLabel>
	<skos:prefLabel xml:lang="hr">pilastar</skos:prefLabel>
	<skos:prefLabel xml:lang="de">Pilaster</skos:prefLabel>
	<skos:prefLabel xml:lang="sv">pilastrar</skos:prefLabel>
	<skos:prefLabel xml:lang="pt">pilastras</skos:prefLabel>
	<skos:prefLabel xml:lang="fi">pilasterit</skos:prefLabel>
	<skos:inScheme rdf:resource="http://partage.vocnet.org/Objects"/>
	<skos:broader rdf:resource="http://partage.vocnet.org/part00127"/>
	<skos:exactMatch rdf:resource="http://vocab.getty.edu/aat/300002737"/>
	<skos:editorialNote xml:lang="en">PPRefiningObjectType</skos:editorialNote>
	<skos:scopeNote xml:lang="en">Shallow piers or rectangular columns projecting only slightly from a wall and, in classical architecture, conforming with one of the orders.(PDARC) Common also on furniture.</skos:scopeNote>
</skos:Concept>
<skos:Concept rdf:about="http://partage.vocnet.org/part00747">
	<skos:prefLabel xml:lang="en">pavements</skos:prefLabel>
	<skos:altLabel xml:lang="en">pavements (surface elements)</skos:altLabel>
	<skos:prefLabel xml:lang="hr">pločnik</skos:prefLabel>
	<skos:prefLabel xml:lang="de">Pflaster (Bodenbelag)</skos:prefLabel>
	<skos:prefLabel xml:lang="sv">stenläggningar</skos:prefLabel>
	<skos:prefLabel xml:lang="pl">pavimento</skos:prefLabel>
	<skos:prefLabel xml:lang="fi">jalkakäytävät</skos:prefLabel>
	<skos:inScheme rdf:resource="http://partage.vocnet.org/Objects"/>
	<skos:broader rdf:resource="http://partage.vocnet.org/part00127"/>
	<skos:exactMatch rdf:resource="http://vocab.getty.edu/aat/300002088"/>
	<skos:editorialNote xml:lang="en">PPRefiningObjectType</skos:editorialNote>
	<skos:scopeNote xml:lang="en">Durable coverings laid down to form the surface of a road or other outdoor area; by extension, hard floor coverings in large interiors, such as public halls or churches.</skos:scopeNote>
</skos:Concept>
<skos:Concept rdf:about="http://partage.vocnet.org/part00748">
	<skos:prefLabel xml:lang="en">windows</skos:prefLabel>
	<skos:prefLabel xml:lang="hr">prozor</skos:prefLabel>
	<skos:prefLabel xml:lang="sv">fönster</skos:prefLabel>
	<skos:altLabel xml:lang="pt">janelas</skos:altLabel>
	<skos:prefLabel xml:lang="pt">janela</skos:prefLabel>
	<skos:prefLabel xml:lang="de">Fenster</skos:prefLabel>
	<skos:prefLabel xml:lang="fi">ikkunat</skos:prefLabel>
	<skos:inScheme rdf:resource="http://partage.vocnet.org/Objects"/>
	<skos:broader rdf:resource="http://partage.vocnet.org/part00923"/>
	<skos:exactMatch rdf:resource="http://vocab.getty.edu/aat/300002944"/>
	<skos:editorialNote xml:lang="en">PPRefiningObjectType</skos:editorialNote>
	<skos:scopeNote xml:lang="en">Openings in the wall of a building, serving to admit light, usually to permit vision, and often to admit air.</skos:scopeNote>
</skos:Concept>
<skos:Concept rdf:about="http://partage.vocnet.org/part00749">
	<skos:prefLabel xml:lang="en">gates</skos:prefLabel>
	<skos:prefLabel xml:lang="sv">grindar</skos:prefLabel>
	<skos:prefLabel xml:lang="pt">portão</skos:prefLabel>
	<skos:altLabel xml:lang="de">Pforten</skos:altLabel>
	<skos:altLabel xml:lang="de">Pforte</skos:altLabel>
	<skos:altLabel xml:lang="de">Tore</skos:altLabel>
	<skos:prefLabel xml:lang="de">Tor</skos:prefLabel>
	<skos:prefLabel xml:lang="hr">vrata.</skos:prefLabel>
	<skos:prefLabel xml:lang="fi">portit</skos:prefLabel>
	<skos:inScheme rdf:resource="http://partage.vocnet.org/Objects"/>
	<skos:broader rdf:resource="http://partage.vocnet.org/part00923"/>
	<skos:exactMatch rdf:resource="http://vocab.getty.edu/aat/300002916"/>
	<skos:editorialNote xml:lang="en">PPRefiningObjectType</skos:editorialNote>
	<skos:scopeNote xml:lang="en">Swinging or sliding barriers used to fill or close a gateway between two exterior spaces, often made of a grating or open framework or forming a heavy or rough structure.(W) Also, interior barriers resembling these. For barriers of more solid and finished construction and usually leading to interior spaces, use "doors."</skos:scopeNote>
</skos:Concept>
<skos:Concept rdf:about="http://partage.vocnet.org/part00750">
	<skos:prefLabel xml:lang="en">fountains</skos:prefLabel>
	<skos:prefLabel xml:lang="sv">fontäner</skos:prefLabel>
	<skos:prefLabel xml:lang="pt">fonte</skos:prefLabel>
	<skos:altLabel xml:lang="de">Springbrunnen</skos:altLabel>
	<skos:prefLabel xml:lang="de">Brunnen</skos:prefLabel>
	<skos:prefLabel xml:lang="hr">fontana</skos:prefLabel>
	<skos:prefLabel xml:lang="fi">suihkukaivot</skos:prefLabel>
	<skos:inScheme rdf:resource="http://partage.vocnet.org/Objects"/>
	<skos:broader rdf:resource="http://partage.vocnet.org/part01006"/>
	<skos:exactMatch rdf:resource="http://vocab.getty.edu/aat/300006179"/>
	<skos:editorialNote xml:lang="en">PPRefiningObjectType</skos:editorialNote>
	<skos:scopeNote xml:lang="en">Structures with apertures designed to allow water to spout or flow periodically or continuously, as for amenity or public access.</skos:scopeNote>
</skos:Concept>
<skos:Concept rdf:about="http://partage.vocnet.org/part00751">
	<skos:prefLabel xml:lang="en">doors</skos:prefLabel>
	<skos:prefLabel xml:lang="pt">porta</skos:prefLabel>
	<skos:altLabel xml:lang="de">Türen</skos:altLabel>
	<skos:prefLabel xml:lang="de">Tür</skos:prefLabel>
	<skos:prefLabel xml:lang="sv">dörrar</skos:prefLabel>
	<skos:prefLabel xml:lang="hr">vrata</skos:prefLabel>
	<skos:prefLabel xml:lang="fi">ovet</skos:prefLabel>
	<skos:inScheme rdf:resource="http://partage.vocnet.org/Objects"/>
	<skos:broader rdf:resource="http://partage.vocnet.org/part00923"/>
	<skos:exactMatch rdf:resource="http://vocab.getty.edu/aat/300002803"/>
	<skos:editorialNote xml:lang="en">PPRefiningObjectType</skos:editorialNote>
	<skos:scopeNote xml:lang="en">Barriers that swing, slide, tilt, or fold to close a doorway, usually of solid and finished construction and usually leading to or separating interior spaces. Use also for similar features that close a container or a piece of case furniture. For barriers of less solid or finished construction, and usually separating two exterior spaces, use "gates."</skos:scopeNote>
</skos:Concept>
<skos:Concept rdf:about="http://partage.vocnet.org/part00752">
	<skos:prefLabel xml:lang="en">capitals (column components)</skos:prefLabel>
	<skos:prefLabel xml:lang="sv">kapitäl</skos:prefLabel>
	<skos:prefLabel xml:lang="pt">capitel</skos:prefLabel>
	<skos:altLabel xml:lang="de">Kapitelle</skos:altLabel>
	<skos:prefLabel xml:lang="de">Kapitell</skos:prefLabel>
	<skos:prefLabel xml:lang="hr">kapitel</skos:prefLabel>
	<skos:prefLabel xml:lang="fi">kapiteelit</skos:prefLabel>
	<skos:inScheme rdf:resource="http://partage.vocnet.org/Objects"/>
	<skos:broader rdf:resource="http://partage.vocnet.org/part00127"/>
	<skos:exactMatch rdf:resource="http://vocab.getty.edu/aat/300001662"/>
	<skos:editorialNote xml:lang="en">PPRefiningObjectType</skos:editorialNote>
	<skos:scopeNote xml:lang="en">The uppermost members of columns, piers, or pilasters.</skos:scopeNote>
</skos:Concept>
<skos:Concept rdf:about="http://partage.vocnet.org/part00753">
	<skos:prefLabel xml:lang="en">bases (object components)</skos:prefLabel>
	<skos:altLabel xml:lang="sv">grunder</skos:altLabel>
	<skos:prefLabel xml:lang="sv">baser</skos:prefLabel>
	<skos:prefLabel xml:lang="pt">base</skos:prefLabel>
	<skos:altLabel xml:lang="de">Basen</skos:altLabel>
	<skos:altLabel xml:lang="de">Basis</skos:altLabel>
	<skos:prefLabel xml:lang="de">Sockel</skos:prefLabel>
	<skos:prefLabel xml:lang="hr">baza</skos:prefLabel>
	<skos:prefLabel xml:lang="fi">jalustat</skos:prefLabel>
	<skos:inScheme rdf:resource="http://partage.vocnet.org/Objects"/>
	<skos:broader rdf:resource="http://partage.vocnet.org/part00116"/>
	<skos:exactMatch rdf:resource="http://vocab.getty.edu/aat/300001656"/>
	<skos:editorialNote xml:lang="en">PPRefiningObjectType</skos:editorialNote>
	<skos:scopeNote xml:lang="en">Relatively massive elements at the bottoms of structures or objects upon which the upper parts rest or are supported. For terminal elements upon which objects rest and that are small in relation to the body of the object, use "feet."</skos:scopeNote>
</skos:Concept>
<skos:Concept rdf:about="http://partage.vocnet.org/part00754">
	<skos:prefLabel xml:lang="en">water towers</skos:prefLabel>
	<skos:prefLabel xml:lang="sv">vattentorn</skos:prefLabel>
	<skos:prefLabel xml:lang="hr">vodeni toranj</skos:prefLabel>
	<skos:prefLabel xml:lang="pt">reservatório de água</skos:prefLabel>
	<skos:altLabel xml:lang="de">Wassertürme</skos:altLabel>
	<skos:prefLabel xml:lang="de">Wasserturm</skos:prefLabel>
	<skos:prefLabel xml:lang="fi">vesitornit</skos:prefLabel>
	<skos:inScheme rdf:resource="http://partage.vocnet.org/Objects"/>
	<skos:broader rdf:resource="http://partage.vocnet.org/part01064"/>
	<skos:exactMatch rdf:resource="http://vocab.getty.edu/aat/\u00a0300006204"/>
	<skos:scopeNote xml:lang="en">Elevated reservoirs, usually in the shape of towers, into which water is pumped to maintain desired pressure throughout a distribution system.</skos:scopeNote>
	<skos:editorialNote xml:lang="en">PPRefiningObjectType</skos:editorialNote>
</skos:Concept>
<skos:Concept rdf:about="http://partage.vocnet.org/part00755">
	<skos:prefLabel xml:lang="en">country houses</skos:prefLabel>
	<skos:prefLabel xml:lang="pt">casa de campo</skos:prefLabel>
	<skos:altLabel xml:lang="de">Landsitze</skos:altLabel>
	<skos:altLabel xml:lang="de">Landsitz</skos:altLabel>
	<skos:altLabel xml:lang="de">Landhäuser</skos:altLabel>
	<skos:prefLabel xml:lang="de">Landhaus</skos:prefLabel>
	<skos:prefLabel xml:lang="sv">lantställen</skos:prefLabel>
	<skos:prefLabel xml:lang="hr">ladanjska kuća</skos:prefLabel>
	<skos:prefLabel xml:lang="fi">maaseutuasunnot</skos:prefLabel>
	<skos:inScheme rdf:resource="http://partage.vocnet.org/Objects"/>
	<skos:broader rdf:resource="http://partage.vocnet.org/part00200"/>
	<skos:exactMatch rdf:resource="http://vocab.getty.edu/aat/300005567"/>
	<skos:editorialNote xml:lang="en">PPRefiningObjectType</skos:editorialNote>
	<skos:scopeNote xml:lang="en">Houses in the country, especially those that are large, have substantial property, and are used seasonally.</skos:scopeNote>
</skos:Concept>
<skos:Concept rdf:about="http://partage.vocnet.org/part00756">
	<skos:prefLabel xml:lang="en">churches (buildings)</skos:prefLabel>
	<skos:prefLabel xml:lang="sv">kyrkor</skos:prefLabel>
	<skos:prefLabel xml:lang="pt">igreja</skos:prefLabel>
	<skos:altLabel xml:lang="de">Kirchen (Gebäude)</skos:altLabel>
	<skos:prefLabel xml:lang="de">Kirche (Gebäude)</skos:prefLabel>
	<skos:prefLabel xml:lang="hr">crkva</skos:prefLabel>
	<skos:prefLabel xml:lang="fi">kirkkorakennukset</skos:prefLabel>
	<skos:inScheme rdf:resource="http://partage.vocnet.org/Objects"/>
	<skos:broader rdf:resource="http://partage.vocnet.org/part00072"/>
	<skos:exactMatch rdf:resource="http://vocab.getty.edu/aat/300007466"/>
	<skos:editorialNote xml:lang="en">PPRefiningObjectType</skos:editorialNote>
	<skos:scopeNote xml:lang="en">Buildings for public Christian worship that are distinguished historically from chapels and oratories, which are buildings that are in some respect private, or not public in the widest sense. Church architecture generally somewhat follows standard models, which vary depending upon the date, location, and characteristics of the congregation.</skos:scopeNote>
</skos:Concept>
<skos:Concept rdf:about="http://partage.vocnet.org/part00757">
	<skos:prefLabel xml:lang="en">ornaments</skos:prefLabel>
	<skos:prefLabel xml:lang="hr">ornament</skos:prefLabel>
	<skos:prefLabel xml:lang="de">Ornament</skos:prefLabel>
	<skos:prefLabel xml:lang="sv">ornament</skos:prefLabel>
	<skos:prefLabel xml:lang="pl">ornamento</skos:prefLabel>
	<skos:altLabel xml:lang="de">Zierrat</skos:altLabel>
	<skos:altLabel xml:lang="de">Zierde</skos:altLabel>
	<skos:altLabel xml:lang="de">Verzierung</skos:altLabel>
	<skos:prefLabel xml:lang="fi">ornamentit</skos:prefLabel>
	<skos:inScheme rdf:resource="http://partage.vocnet.org/Objects"/>
	<skos:exactMatch rdf:resource="http://vocab.getty.edu/aat/300266794"/>
	<skos:editorialNote xml:lang="en">PPRefiningObjectType</skos:editorialNote>
	<skos:scopeNote xml:lang="en">Decorative forms or embellishments that are an integral part of a building or object but are not essential to its structure. Refers also to decorative objects attached to or worn by humans and animals. For objects signifying an honor bestowed upon an individual, usually worn on the person, see "decorations." Regarding techniques of embellishment in general, see "decoration (process)."</skos:scopeNote>
</skos:Concept>
<skos:Concept rdf:about="http://partage.vocnet.org/part00758">
	<skos:prefLabel xml:lang="en">toilet sets (washing sets)</skos:prefLabel>
	<skos:prefLabel xml:lang="sv">tvättserviser</skos:prefLabel>
	<skos:prefLabel xml:lang="hr">toaletna garnitura</skos:prefLabel>
	<skos:altLabel xml:lang="pt">conjunto de lavatóri</skos:altLabel>
	<skos:prefLabel xml:lang="pt">lavatórioo</skos:prefLabel>
	<skos:altLabel xml:lang="de">Waschgarnituren</skos:altLabel>
	<skos:prefLabel xml:lang="de">Waschgarnitur</skos:prefLabel>
	<skos:prefLabel xml:lang="fi">pesukalustot</skos:prefLabel>
	<skos:inScheme rdf:resource="http://partage.vocnet.org/Objects"/>
	<skos:exactMatch rdf:resource="http://vocab.getty.edu/aat/300236098"/>
	<skos:editorialNote xml:lang="en">PPRefiningObjectType</skos:editorialNote>
	<skos:scopeNote xml:lang="en">Sets of vessels intended for use on a washstand generally including a basin and ewer, but may also include a soap dish and chamber pot.</skos:scopeNote>
</skos:Concept>
<skos:Concept rdf:about="http://partage.vocnet.org/part00759">
	<skos:prefLabel xml:lang="en">toilet sets (dresser sets)</skos:prefLabel>
	<skos:prefLabel xml:lang="sv">toalettuppsatser</skos:prefLabel>
	<skos:prefLabel xml:lang="pt">jogo de toucador</skos:prefLabel>
	<skos:prefLabel xml:lang="hr">toaletna garnitura.</skos:prefLabel>
	<skos:altLabel xml:lang="de">Toilettegarnituren</skos:altLabel>
	<skos:altLabel xml:lang="de">Toilettegarnitur</skos:altLabel>
	<skos:altLabel xml:lang="de">Toilettenartikel</skos:altLabel>
	<skos:prefLabel xml:lang="de">Toilettengarnitur</skos:prefLabel>
	<skos:altLabel xml:lang="de">Toilettengarnituren</skos:altLabel>
	<skos:prefLabel xml:lang="fi">toilettilaukut</skos:prefLabel>
	<skos:inScheme rdf:resource="http://partage.vocnet.org/Objects"/>
	<skos:broader rdf:resource="http://partage.vocnet.org/part00196"/>
	<skos:exactMatch rdf:resource="http://vocab.getty.edu/aat/300236191"/>
	<skos:editorialNote xml:lang="en">PPRefiningObjectType</skos:editorialNote>
	<skos:scopeNote xml:lang="en">Sets of vessels and other articles intended for use on a woman's toilet or dressing table generally including a variety of small boxes and bottles, and sometimes also a brush, comb, mirror, or tray.</skos:scopeNote>
</skos:Concept>
<skos:Concept rdf:about="http://partage.vocnet.org/part00760">
	<skos:prefLabel xml:lang="en">suites (furniture)</skos:prefLabel>
	<skos:prefLabel xml:lang="hr">garnitura.</skos:prefLabel>
	<skos:prefLabel xml:lang="pt">conjunto de mobília</skos:prefLabel>
	<skos:altLabel xml:lang="de">Ensembles (Möbel)</skos:altLabel>
	<skos:prefLabel xml:lang="de">Ensemble (Möbel)</skos:prefLabel>
	<skos:altLabel xml:lang="de">Garnitur (Möbel)</skos:altLabel>
	<skos:prefLabel xml:lang="fi">kalusteet</skos:prefLabel>
	<skos:inScheme rdf:resource="http://partage.vocnet.org/Objects"/>
	<skos:exactMatch rdf:resource="http://vocab.getty.edu/aat/300165808"/>
	<skos:editorialNote xml:lang="en">PPRefiningObjectType</skos:editorialNote>
	<skos:scopeNote xml:lang="en">Matched sets of furniture, especially those comprising the basic furniture necessary for one room.</skos:scopeNote>
</skos:Concept>
<skos:Concept rdf:about="http://partage.vocnet.org/part00761">
	<skos:prefLabel xml:lang="en">tea-services</skos:prefLabel>
	<skos:altLabel xml:lang="en">tea services</skos:altLabel>
	<skos:prefLabel xml:lang="sv">teserviser</skos:prefLabel>
	<skos:prefLabel xml:lang="hr">servis za čaj</skos:prefLabel>
	<skos:prefLabel xml:lang="pt">serviço de chá</skos:prefLabel>
	<skos:prefLabel xml:lang="de">Teeservice</skos:prefLabel>
	<skos:prefLabel xml:lang="fi">teeastiastot</skos:prefLabel>
	<skos:inScheme rdf:resource="http://partage.vocnet.org/Objects"/>
	<skos:broader rdf:resource="http://partage.vocnet.org/part00197"/>
	<skos:exactMatch rdf:resource="http://vocab.getty.edu/aat/300227686"/>
	<skos:editorialNote xml:lang="en">PPRefiningObjectType</skos:editorialNote>
	<skos:scopeNote xml:lang="en">Services intended for use in preparing and serving tea, generally consisting of a teapot, creamer, sugar bowl, and often a matching tray. May also include a coffeepot, cups, saucers, or dessert plates.</skos:scopeNote>
</skos:Concept>
<skos:Concept rdf:about="http://partage.vocnet.org/part00762">
	<skos:prefLabel xml:lang="en">dinner-services</skos:prefLabel>
	<skos:altLabel xml:lang="en">dinner services</skos:altLabel>
	<skos:prefLabel xml:lang="pt">serviço de jantar</skos:prefLabel>
	<skos:prefLabel xml:lang="de">Tafelservice</skos:prefLabel>
	<skos:altLabel xml:lang="sv">matserviser</skos:altLabel>
	<skos:prefLabel xml:lang="sv">bordsserviser</skos:prefLabel>
	<skos:prefLabel xml:lang="hr">servis za večeru</skos:prefLabel>
	<skos:prefLabel xml:lang="fi">ruoka-astiastot</skos:prefLabel>
	<skos:inScheme rdf:resource="http://partage.vocnet.org/Objects"/>
	<skos:broader rdf:resource="http://partage.vocnet.org/part00197"/>
	<skos:exactMatch rdf:resource="http://vocab.getty.edu/aat/300227296"/>
	<skos:editorialNote xml:lang="en">PPRefiningObjectType</skos:editorialNote>
	<skos:scopeNote xml:lang="en">Services intended for use at a dinner table by a number of diners, generally consisting of dishes, plates, and cups of different size, and sometimes other vessels such as tureens, platters, casters, or decorative articles such as vases and \u00e9pergnes.</skos:scopeNote>
</skos:Concept>
<skos:Concept rdf:about="http://partage.vocnet.org/part00763">
	<skos:prefLabel xml:lang="en">dessert-services</skos:prefLabel>
	<skos:altLabel xml:lang="en">dessert services</skos:altLabel>
	<skos:prefLabel xml:lang="pt">serviço de sobremesa</skos:prefLabel>
	<skos:altLabel xml:lang="de">Dessert-Service</skos:altLabel>
	<skos:prefLabel xml:lang="de">Dessertservice</skos:prefLabel>
	<skos:prefLabel xml:lang="sv">dessertserviser</skos:prefLabel>
	<skos:prefLabel xml:lang="hr">servis za desert</skos:prefLabel>
	<skos:prefLabel xml:lang="fi">jälkiruoka-astiat</skos:prefLabel>
	<skos:inScheme rdf:resource="http://partage.vocnet.org/Objects"/>
	<skos:broader rdf:resource="http://partage.vocnet.org/part00197"/>
	<skos:exactMatch rdf:resource="http://vocab.getty.edu/aat/300227295"/>
	<skos:editorialNote xml:lang="en">PPRefiningObjectType</skos:editorialNote>
	<skos:scopeNote xml:lang="en">Services intended for a dessert, usually consisting of dessert plates, dessert dishes, dessert forks, dessert knives, dessert spoons, and sometimes a serving spoon and finger bowls.</skos:scopeNote>
</skos:Concept>
<skos:Concept rdf:about="http://partage.vocnet.org/part00764">
	<skos:prefLabel xml:lang="en">coffee-services</skos:prefLabel>
	<skos:altLabel xml:lang="en">coffee services</skos:altLabel>
	<skos:altLabel xml:lang="de">Kaffee-Service</skos:altLabel>
	<skos:prefLabel xml:lang="de">Kaffeeservice</skos:prefLabel>
	<skos:prefLabel xml:lang="pt">serviço de café</skos:prefLabel>
	<skos:prefLabel xml:lang="sv">kaffeserviser</skos:prefLabel>
	<skos:prefLabel xml:lang="hr">servis za kavu</skos:prefLabel>
	<skos:prefLabel xml:lang="fi">kahviastiastot</skos:prefLabel>
	<skos:inScheme rdf:resource="http://partage.vocnet.org/Objects"/>
	<skos:broader rdf:resource="http://partage.vocnet.org/part00197"/>
	<skos:exactMatch rdf:resource="http://vocab.getty.edu/aat/300227293"/>
	<skos:editorialNote xml:lang="en">PPRefiningObjectType</skos:editorialNote>
	<skos:scopeNote xml:lang="en">Services intended for use in serving coffee generally consisting of a coffeepot, creamer, sugar bowl, and often a matching tray. May also include matching cups and urn, saucers, or dessert plates.</skos:scopeNote>
</skos:Concept>
<skos:Concept rdf:about="http://partage.vocnet.org/part00765">
	<skos:prefLabel xml:lang="en">suites (print groupings)</skos:prefLabel>
	<skos:prefLabel xml:lang="hr">mapa</skos:prefLabel>
	<skos:prefLabel xml:lang="pt">série (impressões)</skos:prefLabel>
	<skos:altLabel xml:lang="de">Serie (Druckgrafik)</skos:altLabel>
	<skos:altLabel xml:lang="de">Graphikkfolge</skos:altLabel>
	<skos:altLabel xml:lang="de">Graphischer Zyklus</skos:altLabel>
	<skos:prefLabel xml:lang="de">Serie (Druckgraphik)</skos:prefLabel>
	<skos:prefLabel xml:lang="sv">sviter</skos:prefLabel>
	<skos:altLabel xml:lang="de">Serien (Druckgraphik)</skos:altLabel>
	<skos:prefLabel xml:lang="fi">sarjat (grafiikka)</skos:prefLabel>
	<skos:inScheme rdf:resource="http://partage.vocnet.org/Objects"/>
	<skos:exactMatch rdf:resource="http://vocab.getty.edu/aat/300189634"/>
	<skos:editorialNote xml:lang="en">PPRefiningObjectType</skos:editorialNote>
	<skos:scopeNote xml:lang="en">Groups of prints related in theme or technique and usually issued together.</skos:scopeNote>
</skos:Concept>
<skos:Concept rdf:about="http://partage.vocnet.org/part00766">
	<skos:altLabel xml:lang="en">seals (artifacts)</skos:altLabel>
	<skos:prefLabel xml:lang="en">seals</skos:prefLabel>
	<skos:prefLabel xml:lang="hr">pečat</skos:prefLabel>
	<skos:prefLabel xml:lang="pt">selo</skos:prefLabel>
	<skos:prefLabel xml:lang="de">Siegel</skos:prefLabel>
	<skos:prefLabel xml:lang="sv">sigill</skos:prefLabel>
	<skos:prefLabel xml:lang="fi">sinettileimasimet</skos:prefLabel>
	<skos:inScheme rdf:resource="http://partage.vocnet.org/Objects"/>
	<skos:exactMatch rdf:resource="http://vocab.getty.edu/aat/300028877"/>
	<skos:editorialNote xml:lang="en">PPRefiningObjectType</skos:editorialNote>
	<skos:scopeNote xml:lang="en">Refers to artifacts bearing monograms, writing, numbers, symbols, or designs in intaglio that are used for making an impression in relief on some soft, tenacious substance such as clay or wax. They may be flat or cylindrical, the impression made by rolling the seal over the surface. The term also refers to the impressions that have been made in wax, clay, or another soft material by the impact of a seal or other hard engraved surface. Seals are generally used to authenticate documents or for decoration.</skos:scopeNote>
</skos:Concept>
<skos:Concept rdf:about="http://partage.vocnet.org/part00767">
	<skos:prefLabel xml:lang="en">cards (information artifacts)</skos:prefLabel>
	<skos:altLabel xml:lang="en">cards</skos:altLabel>
	<skos:prefLabel xml:lang="sv">kort</skos:prefLabel>
	<skos:prefLabel xml:lang="pt">cartas</skos:prefLabel>
	<skos:altLabel xml:lang="de">Karten</skos:altLabel>
	<skos:prefLabel xml:lang="de">Karte</skos:prefLabel>
	<skos:prefLabel xml:lang="hr">kartica</skos:prefLabel>
	<skos:prefLabel xml:lang="fi">kortit</skos:prefLabel>
	<skos:inScheme rdf:resource="http://partage.vocnet.org/Objects"/>
	<skos:exactMatch rdf:resource="http://vocab.getty.edu/aat/300026756"/>
	<skos:editorialNote xml:lang="en">PPRefiningObjectType</skos:editorialNote>
	<skos:scopeNote xml:lang="en">Rectangular pieces of stiff paper or plastic, usually of standard dimensions, used as a support on which information is typed, written, or transcribed.</skos:scopeNote>
</skos:Concept>
<skos:Concept rdf:about="http://partage.vocnet.org/part00768">
	<skos:prefLabel xml:lang="en">postcards</skos:prefLabel>
	<skos:prefLabel xml:lang="hr">razglednica</skos:prefLabel>
	<skos:prefLabel xml:lang="de">Postakarten</skos:prefLabel>
	<skos:altLabel xml:lang="de">Postkarte</skos:altLabel>
	<skos:prefLabel xml:lang="sv">vykort</skos:prefLabel>
	<skos:altLabel xml:lang="pt">postais</skos:altLabel>
	<skos:prefLabel xml:lang="pt">postal</skos:prefLabel>
	<skos:prefLabel xml:lang="fi">postikortit</skos:prefLabel>
	<skos:inScheme rdf:resource="http://partage.vocnet.org/Objects"/>
	<skos:exactMatch rdf:resource="http://vocab.getty.edu/aat/300026816"/>
	<skos:editorialNote xml:lang="en">PPRefiningObjectType</skos:editorialNote>
	<skos:scopeNote xml:lang="en">Cards on which a message may be written or printed for mailing without an envelope, usually at a lower rate than that for letters in envelopes.</skos:scopeNote>
</skos:Concept>
<skos:Concept rdf:about="http://partage.vocnet.org/part00769">
	<skos:prefLabel xml:lang="en">badges</skos:prefLabel>
	<skos:altLabel xml:lang="sv">emblem</skos:altLabel>
	<skos:prefLabel xml:lang="sv">märken</skos:prefLabel>
	<skos:altLabel xml:lang="pt">emblema</skos:altLabel>
	<skos:prefLabel xml:lang="pt">insígnia</skos:prefLabel>
	<skos:altLabel xml:lang="de">Embleme</skos:altLabel>
	<skos:altLabel xml:lang="de">Emblem</skos:altLabel>
	<skos:prefLabel xml:lang="de">Abzeichen</skos:prefLabel>
	<skos:prefLabel xml:lang="hr">značka</skos:prefLabel>
	<skos:altLabel xml:lang="fi">rintamerkit</skos:altLabel>
	<skos:prefLabel xml:lang="fi">tunnukset</skos:prefLabel>
	<skos:inScheme rdf:resource="http://partage.vocnet.org/Objects"/>
	<skos:exactMatch rdf:resource="http://vocab.getty.edu/aat/300193994"/>
	<skos:editorialNote xml:lang="en">PPRefiningObjectType</skos:editorialNote>
	<skos:scopeNote xml:lang="en">Objects bearing special or distinctive marks and worn for decoration or to signify affiliation. Originally, badges were heraldic symbols worn as identifying marks by a knight and his retainers, e.g., a badge of arms. In later use, the term refers to any distinctive device, emblem, or mark worn to indicate a person's affiliation, rank, office, name, or membership in an organization or support for a cause, particularly objects that comprise small pieces of metal, card, plastic, etc., that bear a distinguishing design or words.</skos:scopeNote>
</skos:Concept>
<skos:Concept rdf:about="http://partage.vocnet.org/part00770">
	<skos:prefLabel xml:lang="en">beads</skos:prefLabel>
	<skos:altLabel xml:lang="en">beads (pierced objects)</skos:altLabel>
	<skos:prefLabel xml:lang="sv">pärlor</skos:prefLabel>
	<skos:prefLabel xml:lang="pt">contas</skos:prefLabel>
	<skos:altLabel xml:lang="de">Perlen</skos:altLabel>
	<skos:prefLabel xml:lang="de">Perle</skos:prefLabel>
	<skos:prefLabel xml:lang="hr">perlice</skos:prefLabel>
	<skos:prefLabel xml:lang="fi">koristehelmet</skos:prefLabel>
	<skos:inScheme rdf:resource="http://partage.vocnet.org/Objects"/>
	<skos:exactMatch rdf:resource="http://vocab.getty.edu/aat/300234006"/>
	<skos:editorialNote xml:lang="en">PPRefiningObjectType</skos:editorialNote>
	<skos:scopeNote xml:lang="en">Refers to small objects, of any shape or material, pierced so that they may be strung or hung or attached, as by sewing.</skos:scopeNote>
</skos:Concept>
<skos:Concept rdf:about="http://partage.vocnet.org/part00771">
	<skos:prefLabel xml:lang="en">sautoirs</skos:prefLabel>
	<skos:prefLabel xml:lang="hr">ogrlica.</skos:prefLabel>
	<skos:prefLabel xml:lang="pt">sautoirs</skos:prefLabel>
	<skos:altLabel xml:lang="de">Sautoirs</skos:altLabel>
	<skos:prefLabel xml:lang="de">Sautoir</skos:prefLabel>
	<skos:prefLabel xml:lang="sv">sautoirs</skos:prefLabel>
	<skos:prefLabel xml:lang="fi">käädyt</skos:prefLabel>
	<skos:inScheme rdf:resource="http://partage.vocnet.org/Objects"/>
	<skos:broader rdf:resource="http://partage.vocnet.org/part00078"/>
	<skos:exactMatch rdf:resource="http://vocab.getty.edu/aat/300212115"/>
	<skos:editorialNote xml:lang="en">PPRefiningObjectType</skos:editorialNote>
	<skos:scopeNote xml:lang="en">Long neck chains worn loosely from the shoulders and usually extending below the waist. May have a pendant or tassel suspended at the bottom.</skos:scopeNote>
</skos:Concept>
<skos:Concept rdf:about="http://partage.vocnet.org/part00772">
	<skos:prefLabel xml:lang="en">pins (jewellery)</skos:prefLabel>
	<skos:altLabel xml:lang="en">pins</skos:altLabel>
	<skos:prefLabel xml:lang="hr">igla</skos:prefLabel>
	<skos:altLabel xml:lang="de">Schmucknadeln</skos:altLabel>
	<skos:altLabel xml:lang="de">Anstecknadeln</skos:altLabel>
	<skos:prefLabel xml:lang="de">Schmucknadel</skos:prefLabel>
	<skos:altLabel xml:lang="de">Anstecknadel</skos:altLabel>
	<skos:prefLabel xml:lang="sv">broschnålar</skos:prefLabel>
	<skos:prefLabel xml:lang="pt">alfinete</skos:prefLabel>
	<skos:prefLabel xml:lang="fi">rintaneulat.</skos:prefLabel>
	<skos:inScheme rdf:resource="http://partage.vocnet.org/Objects"/>
	<skos:broader rdf:resource="http://partage.vocnet.org/part00078"/>
	<skos:narrower rdf:resource="http://partage.vocnet.org/part00782"/>
	<skos:exactMatch rdf:resource="http://vocab.getty.edu/aat/300046006"/>
	<skos:editorialNote xml:lang="en">PPRefiningObjectType</skos:editorialNote>
	<skos:scopeNote xml:lang="en">Ornaments consisting essentially or partly of a pointed penetrating wire or shaft.</skos:scopeNote>
</skos:Concept>
<skos:Concept rdf:about="http://partage.vocnet.org/part00773">
	<skos:prefLabel xml:lang="en">rings (jewellery)</skos:prefLabel>
	<skos:altLabel xml:lang="en">rings (jewelry)</skos:altLabel>
	<skos:prefLabel xml:lang="hr">prsten</skos:prefLabel>
	<skos:altLabel xml:lang="pt">anéis</skos:altLabel>
	<skos:prefLabel xml:lang="pt">anel</skos:prefLabel>
	<skos:altLabel xml:lang="de">Fingerringe</skos:altLabel>
	<skos:altLabel xml:lang="de">Ringe (Schmuck)</skos:altLabel>
	<skos:altLabel xml:lang="de">Fingerring</skos:altLabel>
	<skos:prefLabel xml:lang="de">Ring (Schmuck)</skos:prefLabel>
	<skos:prefLabel xml:lang="sv">ringar (smycken)</skos:prefLabel>
	<skos:prefLabel xml:lang="fi">sormukset</skos:prefLabel>
	<skos:inScheme rdf:resource="http://partage.vocnet.org/Objects"/>
	<skos:broader rdf:resource="http://partage.vocnet.org/part00078"/>
	<skos:exactMatch rdf:resource="http://vocab.getty.edu/aat/300046012"/>
	<skos:editorialNote xml:lang="en">PPRefiningObjectType</skos:editorialNote>
	<skos:scopeNote xml:lang="en">Small circular bands worn on the finger; typically circlets of real or simulated precious metal, and frequently set with precious stones or imitations of these, intended for wearing upon the finger either as an ornament or as a token.</skos:scopeNote>
</skos:Concept>
<skos:Concept rdf:about="http://partage.vocnet.org/part00774">
	<skos:prefLabel xml:lang="en">pendants (jewellery)</skos:prefLabel>
	<skos:altLabel xml:lang="en">pendants (jewelry)</skos:altLabel>
	<skos:prefLabel xml:lang="hr">privjesak</skos:prefLabel>
	<skos:prefLabel xml:lang="de">Anhänger (Schmuck)</skos:prefLabel>
	<skos:prefLabel xml:lang="sv">berlocker</skos:prefLabel>
	<skos:prefLabel xml:lang="pt">pendente</skos:prefLabel>
	<skos:prefLabel xml:lang="fi">riipukset</skos:prefLabel>
	<skos:inScheme rdf:resource="http://partage.vocnet.org/Objects"/>
	<skos:broader rdf:resource="http://partage.vocnet.org/part00078"/>
	<skos:exactMatch rdf:resource="http://vocab.getty.edu/aat/300046002"/>
	<skos:editorialNote xml:lang="en">PPRefiningObjectType</skos:editorialNote>
	<skos:scopeNote xml:lang="en">Hanging articles of jewelry, usually suspended from a necklace, brooch, or earrings, but also includes Renaissance examples fastened to the sleeve often worn as decorative ornaments; can also be an article of devotional, magical, or mourning jewelry which then may sometimes be concealed under clothing.</skos:scopeNote>
</skos:Concept>
<skos:Concept rdf:about="http://partage.vocnet.org/part00775">
	<skos:prefLabel xml:lang="en">necklaces</skos:prefLabel>
	<skos:prefLabel xml:lang="hr">ogrlica</skos:prefLabel>
	<skos:altLabel xml:lang="de">Halsketten</skos:altLabel>
	<skos:prefLabel xml:lang="de">Halskette</skos:prefLabel>
	<skos:prefLabel xml:lang="sv">halsband</skos:prefLabel>
	<skos:prefLabel xml:lang="pt">colar</skos:prefLabel>
	<skos:prefLabel xml:lang="fi">kaulakorut</skos:prefLabel>
	<skos:inScheme rdf:resource="http://partage.vocnet.org/Objects"/>
	<skos:broader rdf:resource="http://partage.vocnet.org/part00078"/>
	<skos:narrower rdf:resource="http://partage.vocnet.org/part00778"/>
	<skos:exactMatch rdf:resource="http://vocab.getty.edu/aat/300046001"/>
	<skos:editorialNote xml:lang="en">PPRefiningObjectType</skos:editorialNote>
	<skos:scopeNote xml:lang="en">Ornaments worn around the neck, usually in the form of chains or strands of beads, pearls, stones, or decorative or precious materials, and often including a suspended ornamental pendant. Use "chokers" for short, narrow necklaces worn close to the throat. Use "dog collars (necklaces)" for wide ornamental bands worn tightly around the neck.</skos:scopeNote>
</skos:Concept>
<skos:Concept rdf:about="http://partage.vocnet.org/part00776">
	<skos:altLabel xml:lang="de">Medaillons</skos:altLabel>
	<skos:prefLabel xml:lang="en">lockets</skos:prefLabel>
	<skos:prefLabel xml:lang="hr">medaljon</skos:prefLabel>
	<skos:prefLabel xml:lang="de">Medaillon</skos:prefLabel>
	<skos:prefLabel xml:lang="sv">medaljonger</skos:prefLabel>
	<skos:prefLabel xml:lang="pt">medalhão</skos:prefLabel>
	<skos:prefLabel xml:lang="fi">medaljongit</skos:prefLabel>
	<skos:inScheme rdf:resource="http://partage.vocnet.org/Objects"/>
	<skos:broader rdf:resource="http://partage.vocnet.org/part00078"/>
	<skos:exactMatch rdf:resource="http://vocab.getty.edu/aat/300046004"/>
	<skos:editorialNote xml:lang="en">PPRefiningObjectType</skos:editorialNote>
	<skos:scopeNote xml:lang="en">Small decorative cases, opening to reveal a portrait or memento, generally worn suspended from a chain around the neck.</skos:scopeNote>
</skos:Concept>
<skos:Concept rdf:about="http://partage.vocnet.org/part00777">
	<skos:prefLabel xml:lang="en">earrings</skos:prefLabel>
	<skos:prefLabel xml:lang="pt">brincos</skos:prefLabel>
	<skos:prefLabel xml:lang="de">Ohrringe</skos:prefLabel>
	<skos:altLabel xml:lang="de">Ohrring</skos:altLabel>
	<skos:prefLabel xml:lang="sv">örhängen</skos:prefLabel>
	<skos:prefLabel xml:lang="hr">naušnice</skos:prefLabel>
	<skos:prefLabel xml:lang="fi">korvakorut</skos:prefLabel>
	<skos:inScheme rdf:resource="http://partage.vocnet.org/Objects"/>
	<skos:broader rdf:resource="http://partage.vocnet.org/part00958"/>
	<skos:exactMatch rdf:resource="http://vocab.getty.edu/aat/300045998"/>
	<skos:editorialNote xml:lang="en">PPRefiningObjectType</skos:editorialNote>
	<skos:scopeNote xml:lang="en">Ear ornaments worn suspended from a bent wire or a thin loop passed through a hole pierced in the lobe of the ear or clipped or screwed to the lobe.</skos:scopeNote>
</skos:Concept>
<skos:Concept rdf:about="http://partage.vocnet.org/part00778">
	<skos:prefLabel xml:lang="en">dogs collars (necklaces)</skos:prefLabel>
	<skos:prefLabel xml:lang="pt">gargantilha</skos:prefLabel>
	<skos:altLabel xml:lang="de">Halsbänder</skos:altLabel>
	<skos:altLabel xml:lang="de">Colliers de Chien</skos:altLabel>
	<skos:prefLabel xml:lang="de">Collier de Chien</skos:prefLabel>
	<skos:altLabel xml:lang="de">Halsband (Schmuck)</skos:altLabel>
	<skos:prefLabel xml:lang="sv">kraghalsband</skos:prefLabel>
	<skos:prefLabel xml:lang="hr">ogrlica uz vrat</skos:prefLabel>
	<skos:prefLabel xml:lang="fi">kaulapannat</skos:prefLabel>
	<skos:inScheme rdf:resource="http://partage.vocnet.org/Objects"/>
	<skos:broader rdf:resource="http://partage.vocnet.org/part00775"/>
	<skos:exactMatch rdf:resource="http://vocab.getty.edu/aat/300212029"/>
	<skos:editorialNote xml:lang="en">PPRefiningObjectType</skos:editorialNote>
	<skos:scopeNote xml:lang="en">Wide, close-fitting necklaces worn tightly around the neck, often ornamented with precious or semiprecious stones. For short, narrow necklaces worn close to the throat use "chokers."</skos:scopeNote>
</skos:Concept>
<skos:Concept rdf:about="http://partage.vocnet.org/part00779">
	<skos:prefLabel xml:lang="en">cuff links</skos:prefLabel>
	<skos:prefLabel xml:lang="de">Manschettenknöpfe</skos:prefLabel>
	<skos:prefLabel xml:lang="pt">botões de punho</skos:prefLabel>
	<skos:altLabel xml:lang="de">Manschettenknopf</skos:altLabel>
	<skos:prefLabel xml:lang="sv">manschettknappar</skos:prefLabel>
	<skos:prefLabel xml:lang="hr">manžete</skos:prefLabel>
	<skos:prefLabel xml:lang="fi">kalvosinnapit</skos:prefLabel>
	<skos:inScheme rdf:resource="http://partage.vocnet.org/Objects"/>
	<skos:broader rdf:resource="http://partage.vocnet.org/part00078"/>
	<skos:exactMatch rdf:resource="http://vocab.getty.edu/aat/300209299"/>
	<skos:scopeNote xml:lang="en">Linked ornamental buttons or buttonlike devices for fastening a shirt cuff.</skos:scopeNote>
	<skos:editorialNote xml:lang="en">PPRefiningObjectType</skos:editorialNote>
</skos:Concept>
<skos:Concept rdf:about="http://partage.vocnet.org/part00780">
	<skos:altLabel xml:lang="en">collars (neckwear)</skos:altLabel>
	<skos:prefLabel xml:lang="sv">kragar</skos:prefLabel>
	<skos:prefLabel xml:lang="en">collars</skos:prefLabel>
	<skos:altLabel xml:lang="pt">gola</skos:altLabel>
	<skos:prefLabel xml:lang="pt">colarinho</skos:prefLabel>
	<skos:altLabel xml:lang="de">Krägen</skos:altLabel>
	<skos:prefLabel xml:lang="de">Kragen</skos:prefLabel>
	<skos:prefLabel xml:lang="hr">ovratnik</skos:prefLabel>
	<skos:prefLabel xml:lang="fi">kaulukset</skos:prefLabel>
	<skos:inScheme rdf:resource="http://partage.vocnet.org/Objects"/>
	<skos:broader rdf:resource="http://partage.vocnet.org/part00955"/>
	<skos:exactMatch rdf:resource="http://vocab.getty.edu/aat/300210058"/>
	<skos:scopeNote xml:lang="en">Shaped articles worn at the neckline of a garment, either separate or attached.</skos:scopeNote>
	<skos:editorialNote xml:lang="en">PPRefiningObjectType</skos:editorialNote>
</skos:Concept>
<skos:Concept rdf:about="http://partage.vocnet.org/part00781">
	<skos:prefLabel xml:lang="en">buckles</skos:prefLabel>
	<skos:altLabel xml:lang="en">buckles (strap accessories)</skos:altLabel>
	<skos:prefLabel xml:lang="sv">spännen</skos:prefLabel>
	<skos:prefLabel xml:lang="pt">fivela</skos:prefLabel>
	<skos:altLabel xml:lang="de">Schnallen</skos:altLabel>
	<skos:prefLabel xml:lang="de">Schnalle</skos:prefLabel>
	<skos:prefLabel xml:lang="hr">kopča</skos:prefLabel>
	<skos:prefLabel xml:lang="fi">soljet</skos:prefLabel>
	<skos:inScheme rdf:resource="http://partage.vocnet.org/Objects"/>
	<skos:broader rdf:resource="http://partage.vocnet.org/part00711"/>
	<skos:exactMatch rdf:resource="http://vocab.getty.edu/aat/300239260"/>
	<skos:editorialNote xml:lang="en">PPRefiningObjectType</skos:editorialNote>
	<skos:scopeNote xml:lang="en">Devices used for fastening consisting of a usually open rectangular or rounded frame and a tongue or catch attached to one side or a vertical bar attached across the center. Sometimes used alone as an ornament.</skos:scopeNote>
</skos:Concept>
<skos:Concept rdf:about="http://partage.vocnet.org/part00782">
	<skos:prefLabel xml:lang="en">brooches</skos:prefLabel>
	<skos:prefLabel xml:lang="sv">broscher</skos:prefLabel>
	<skos:prefLabel xml:lang="pt">broche</skos:prefLabel>
	<skos:altLabel xml:lang="pt">alfinete de peito</skos:altLabel>
	<skos:altLabel xml:lang="de">Broschen</skos:altLabel>
	<skos:prefLabel xml:lang="de">Brosche</skos:prefLabel>
	<skos:prefLabel xml:lang="hr">broš</skos:prefLabel>
	<skos:prefLabel xml:lang="fi">rintaneulat</skos:prefLabel>
	<skos:inScheme rdf:resource="http://partage.vocnet.org/Objects"/>
	<skos:broader rdf:resource="http://partage.vocnet.org/part00772"/>
	<skos:exactMatch rdf:resource="http://vocab.getty.edu/aat/300045995"/>
	<skos:editorialNote xml:lang="en">PPRefiningObjectType</skos:editorialNote>
	<skos:scopeNote xml:lang="en">Ornamental jewelry made in a variety of forms fastened by a pin. For decorative items, similar in appearance to a brooch, but attached to a garment with a spring fastening, use "clips (jewelry)."</skos:scopeNote>
</skos:Concept>
<skos:Concept rdf:about="http://partage.vocnet.org/part00783">
	<skos:prefLabel xml:lang="en">bracelets</skos:prefLabel>
	<skos:prefLabel xml:lang="sv">armband</skos:prefLabel>
	<skos:prefLabel xml:lang="pt">pulseira</skos:prefLabel>
	<skos:altLabel xml:lang="de">Armbänder</skos:altLabel>
	<skos:prefLabel xml:lang="de">Armband</skos:prefLabel>
	<skos:prefLabel xml:lang="hr">narukvica</skos:prefLabel>
	<skos:prefLabel xml:lang="fi">rannerenkaat</skos:prefLabel>
	<skos:inScheme rdf:resource="http://partage.vocnet.org/Objects"/>
	<skos:broader rdf:resource="http://partage.vocnet.org/part00078"/>
	<skos:exactMatch rdf:resource="http://vocab.getty.edu/aat/300045991"/>
	<skos:editorialNote xml:lang="en">PPRefiningObjectType</skos:editorialNote>
	<skos:scopeNote xml:lang="en">Ornamental bands or circlets worn on the lower arm. Use "armlets" for similar articles worn on the upper arm.</skos:scopeNote>
</skos:Concept>
<skos:Concept rdf:about="http://partage.vocnet.org/part00784">
	<skos:prefLabel xml:lang="en">overlays</skos:prefLabel>
	<skos:prefLabel xml:lang="hr">nadsloj</skos:prefLabel>
	<skos:altLabel xml:lang="de">Schichtung</skos:altLabel>
	<skos:prefLabel xml:lang="de">Überlagerung</skos:prefLabel>
	<skos:prefLabel xml:lang="pt">guardas</skos:prefLabel>
	<skos:prefLabel xml:lang="fi">päällysteet</skos:prefLabel>
	<skos:inScheme rdf:resource="http://partage.vocnet.org/Objects"/>
	<skos:broader rdf:resource="http://partage.vocnet.org/part00116"/>
	<skos:exactMatch rdf:resource="http://vocab.getty.edu/aat/300015611"/>
	<skos:editorialNote xml:lang="en">PPRefiningObjectType</skos:editorialNote>
	<skos:scopeNote xml:lang="en">Generally, any thing laid over something else, more specifically a transparent sheet placed over an image, text, map, diagram, or artwork, to form a composite.</skos:scopeNote>
</skos:Concept>
<skos:Concept rdf:about="http://partage.vocnet.org/part00785">
	<skos:prefLabel xml:lang="en">fireplaces</skos:prefLabel>
	<skos:prefLabel xml:lang="sv">öppna spisar</skos:prefLabel>
	<skos:prefLabel xml:lang="pt">lareira</skos:prefLabel>
	<skos:altLabel xml:lang="de">Cheminées</skos:altLabel>
	<skos:altLabel xml:lang="de">Cheminée</skos:altLabel>
	<skos:altLabel xml:lang="de">Kamine</skos:altLabel>
	<skos:prefLabel xml:lang="de">Kamin</skos:prefLabel>
	<skos:prefLabel xml:lang="hr">kamin</skos:prefLabel>
	<skos:altLabel xml:lang="fi">tulisijat</skos:altLabel>
	<skos:prefLabel xml:lang="fi">takat</skos:prefLabel>
	<skos:inScheme rdf:resource="http://partage.vocnet.org/Objects"/>
	<skos:broader rdf:resource="http://partage.vocnet.org/part00127"/>
	<skos:exactMatch rdf:resource="http://vocab.getty.edu/aat/300052267"/>
	<skos:editorialNote xml:lang="en">PPRefiningObjectType</skos:editorialNote>
	<skos:scopeNote xml:lang="en">Openings or recesses in chimneys or walls in which fires may be built, as for heating or cooking; may also refer to low fireproof structures erected outdoors for cooking over open flames.</skos:scopeNote>
</skos:Concept>
<skos:Concept rdf:about="http://partage.vocnet.org/part00786">
	<skos:prefLabel xml:lang="en">handles</skos:prefLabel>
	<skos:prefLabel xml:lang="sv">handtag</skos:prefLabel>
	<skos:prefLabel xml:lang="pt">maçaneta</skos:prefLabel>
	<skos:altLabel xml:lang="de">Griff</skos:altLabel>
	<skos:prefLabel xml:lang="de">Handgriff</skos:prefLabel>
	<skos:altLabel xml:lang="de">Griffe</skos:altLabel>
	<skos:altLabel xml:lang="de">Handgriffe</skos:altLabel>
	<skos:prefLabel xml:lang="hr">ručka</skos:prefLabel>
	<skos:prefLabel xml:lang="fi">kädensijat</skos:prefLabel>
	<skos:inScheme rdf:resource="http://partage.vocnet.org/Objects"/>
	<skos:broader rdf:resource="http://partage.vocnet.org/part00116"/>
	<skos:exactMatch rdf:resource="http://vocab.getty.edu/aat/300024927"/>
	<skos:editorialNote xml:lang="en">PPRefiningObjectType</skos:editorialNote>
	<skos:scopeNote xml:lang="en">Those portions of, or attachments to, objects that are designed to be grasped by the hand.</skos:scopeNote>
</skos:Concept>
<skos:Concept rdf:about="http://partage.vocnet.org/part00787">
	<skos:prefLabel xml:lang="en">monocles</skos:prefLabel>
	<skos:prefLabel xml:lang="hr">monokl</skos:prefLabel>
	<skos:prefLabel xml:lang="de">Monokel</skos:prefLabel>
	<skos:prefLabel xml:lang="sv">monoklar</skos:prefLabel>
	<skos:prefLabel xml:lang="pl">monóclo</skos:prefLabel>
	<skos:prefLabel xml:lang="fi">monokkelit</skos:prefLabel>
	<skos:inScheme rdf:resource="http://partage.vocnet.org/Objects"/>
	<skos:broader rdf:resource="http://partage.vocnet.org/part00983"/>
	<skos:exactMatch rdf:resource="http://vocab.getty.edu/aat/300263207"/>
	<skos:editorialNote xml:lang="en">PPRefiningObjectType</skos:editorialNote>
	<skos:scopeNote xml:lang="en">Eyeglasses consisting of a single lens, without a nosepiece or frame, used to compensate for defective vision in one eye.</skos:scopeNote>
</skos:Concept>
<skos:Concept rdf:about="http://partage.vocnet.org/part00788">
	<skos:prefLabel xml:lang="en">perambulators</skos:prefLabel>
	<skos:altLabel xml:lang="en">baby carriages</skos:altLabel>
	<skos:prefLabel xml:lang="hr">dječja kolica</skos:prefLabel>
	<skos:altLabel xml:lang="de">Kinderwägen</skos:altLabel>
	<skos:prefLabel xml:lang="de">Kinderwagen</skos:prefLabel>
	<skos:prefLabel xml:lang="sv">barnvagnar</skos:prefLabel>
	<skos:prefLabel xml:lang="pt">carrinho de bebé</skos:prefLabel>
	<skos:prefLabel xml:lang="fi">lastenvaunut</skos:prefLabel>
	<skos:inScheme rdf:resource="http://partage.vocnet.org/Objects"/>
	<skos:broader rdf:resource="http://partage.vocnet.org/part01041"/>
	<skos:exactMatch rdf:resource="http://vocab.getty.edu/aat/300212630"/>
	<skos:editorialNote xml:lang="en">PPRefiningObjectType</skos:editorialNote>
	<skos:scopeNote xml:lang="en">Any of various wheeled vehicles designed primarily for carrying infants; may be pushed or pulled and are often wagonlike or carriagelike in appearance. For vehicles designed primarily for pushing small children sitting upright, prefer "strollers."</skos:scopeNote>
</skos:Concept>
<skos:Concept rdf:about="http://partage.vocnet.org/part00789">
	<skos:prefLabel xml:lang="en">watches</skos:prefLabel>
	<skos:prefLabel xml:lang="sv">klockor</skos:prefLabel>
	<skos:prefLabel xml:lang="hr">osobni sat</skos:prefLabel>
	<skos:prefLabel xml:lang="pt">relógio.</skos:prefLabel>
	<skos:altLabel xml:lang="de">Kleinuhren</skos:altLabel>
	<skos:prefLabel xml:lang="de">Kleinuhr</skos:prefLabel>
	<skos:altLabel xml:lang="de">Uhren (tragbar)</skos:altLabel>
	<skos:altLabel xml:lang="de">Uhr (tragbar)</skos:altLabel>
	<skos:prefLabel xml:lang="fi">kellot..</skos:prefLabel>
	<skos:inScheme rdf:resource="http://partage.vocnet.org/Objects"/>
	<skos:broader rdf:resource="http://partage.vocnet.org/part00087"/>
	<skos:narrower rdf:resource="http://partage.vocnet.org/part01198"/>
	<skos:exactMatch rdf:resource="http://vocab.getty.edu/aat/300041615"/>
	<skos:editorialNote xml:lang="en">PPRefiningObjectType</skos:editorialNote>
	<skos:scopeNote xml:lang="en">Timepieces small and convenient enough to be carried about on a person.</skos:scopeNote>
</skos:Concept>
<skos:Concept rdf:about="http://partage.vocnet.org/part00790">
	<skos:prefLabel xml:lang="en">clocks</skos:prefLabel>
	<skos:prefLabel xml:lang="sv">klockor.</skos:prefLabel>
	<skos:prefLabel xml:lang="hr">sat</skos:prefLabel>
	<skos:prefLabel xml:lang="pt">relógio..</skos:prefLabel>
	<skos:altLabel xml:lang="de">Uhren (stationär)</skos:altLabel>
	<skos:altLabel xml:lang="de">Uhr (stationär)</skos:altLabel>
	<skos:altLabel xml:lang="de">Großuhren</skos:altLabel>
	<skos:prefLabel xml:lang="de">Großuhr</skos:prefLabel>
	<skos:prefLabel xml:lang="fi">kellot.</skos:prefLabel>
	<skos:inScheme rdf:resource="http://partage.vocnet.org/Objects"/>
	<skos:broader rdf:resource="http://partage.vocnet.org/part00087"/>
	<skos:exactMatch rdf:resource="http://vocab.getty.edu/aat/300041575"/>
	<skos:editorialNote xml:lang="en">PPRefiningObjectType</skos:editorialNote>
	<skos:scopeNote xml:lang="en">Refers to instruments that measure and indicate the passage of time, especially by mechanical means producing a regularly recurring action and indicating, usually by hands or changing numbers, the hours and minutes; not designed to be worn or otherwise carried about on a person. For wearable timepieces, see "watches."</skos:scopeNote>
</skos:Concept>
<skos:Concept rdf:about="http://partage.vocnet.org/part00791">
	<skos:altLabel xml:lang="en">lanterns (lighting devices)</skos:altLabel>
	<skos:prefLabel xml:lang="en">lanterns</skos:prefLabel>
	<skos:prefLabel xml:lang="hr">lanterna</skos:prefLabel>
	<skos:altLabel xml:lang="de">Laternen</skos:altLabel>
	<skos:prefLabel xml:lang="de">Laterne</skos:prefLabel>
	<skos:prefLabel xml:lang="sv">lanterniner</skos:prefLabel>
	<skos:prefLabel xml:lang="pt">lanterna</skos:prefLabel>
	<skos:prefLabel xml:lang="fi">lyhdyt</skos:prefLabel>
	<skos:inScheme rdf:resource="http://partage.vocnet.org/Objects"/>
	<skos:broader rdf:resource="http://partage.vocnet.org/part00109"/>
	<skos:exactMatch rdf:resource="http://vocab.getty.edu/aat/300037647"/>
	<skos:editorialNote xml:lang="en">PPRefiningObjectType</skos:editorialNote>
	<skos:scopeNote xml:lang="en">Lighting devices, fixed or portable, designed to protect and enclose the light source, usually with sides of glass, horn or pierced metal, allowing light to emerge and often having a supporting frame or carrying handle.</skos:scopeNote>
</skos:Concept>
<skos:Concept rdf:about="http://partage.vocnet.org/part00792">
	<skos:prefLabel xml:lang="en">chambersticks</skos:prefLabel>
	<skos:prefLabel xml:lang="sv">kammarljusstakar</skos:prefLabel>
	<skos:prefLabel xml:lang="de">Kerzenhalter (flacher Fuß)</skos:prefLabel>
	<skos:prefLabel xml:lang="hr">noćni svijećnjak</skos:prefLabel>
	<skos:prefLabel xml:lang="pt">castiçal..</skos:prefLabel>
	<skos:prefLabel xml:lang="fi">yökynttilänjalat</skos:prefLabel>
	<skos:inScheme rdf:resource="http://partage.vocnet.org/Objects"/>
	<skos:broader rdf:resource="http://partage.vocnet.org/part00330"/>
	<skos:exactMatch rdf:resource="http://vocab.getty.edu/aat/300180070"/>
	<skos:editorialNote xml:lang="en">PPRefiningObjectType</skos:editorialNote>
	<skos:scopeNote xml:lang="en">Candleholders with a single candle socket set on a flat saucer or traylike base. For candleholders with a single candle socket mounted on a support with a widened base or foot, use "candlesticks."</skos:scopeNote>
</skos:Concept>
<skos:Concept rdf:about="http://partage.vocnet.org/part00793">
	<skos:prefLabel xml:lang="en">candlesticks</skos:prefLabel>
	<skos:prefLabel xml:lang="sv">ljusstakar</skos:prefLabel>
	<skos:prefLabel xml:lang="pt">castiçal.</skos:prefLabel>
	<skos:prefLabel xml:lang="de">Kerzenständer</skos:prefLabel>
	<skos:prefLabel xml:lang="hr">svijećnjak.</skos:prefLabel>
	<skos:prefLabel xml:lang="fi">kynttilänjalat</skos:prefLabel>
	<skos:inScheme rdf:resource="http://partage.vocnet.org/Objects"/>
	<skos:broader rdf:resource="http://partage.vocnet.org/part00330"/>
	<skos:exactMatch rdf:resource="http://vocab.getty.edu/aat/300037588"/>
	<skos:editorialNote xml:lang="en">PPRefiningObjectType</skos:editorialNote>
	<skos:scopeNote xml:lang="en">Candleholders with a single candle socket mounted on a support with a widened base or foot for balance; often the support is columnar in form. For candleholders with a single candle socket set on a flat saucer or traylike base, use "chambersticks."</skos:scopeNote>
</skos:Concept>
<skos:Concept rdf:about="http://partage.vocnet.org/part00794">
	<skos:prefLabel xml:lang="en">upholstery</skos:prefLabel>
	<skos:prefLabel xml:lang="sv">stoppade möbler</skos:prefLabel>
	<skos:prefLabel xml:lang="hr">presvlaka</skos:prefLabel>
	<skos:prefLabel xml:lang="pt">estofos</skos:prefLabel>
	<skos:altLabel xml:lang="de">Dekorstoffe</skos:altLabel>
	<skos:altLabel xml:lang="de">Dekorstoff</skos:altLabel>
	<skos:altLabel xml:lang="de">Dekorationsstoffe</skos:altLabel>
	<skos:prefLabel xml:lang="de">Dekostoffe</skos:prefLabel>
	<skos:altLabel xml:lang="de">Dekostoff</skos:altLabel>
	<skos:altLabel xml:lang="de">Dekorationsstoff</skos:altLabel>
	<skos:altLabel xml:lang="de">Polsterstoff</skos:altLabel>
	<skos:prefLabel xml:lang="fi">verhoilu</skos:prefLabel>
	<skos:inScheme rdf:resource="http://partage.vocnet.org/Objects"/>
	<skos:broader rdf:resource="http://partage.vocnet.org/part00100"/>
	<skos:exactMatch rdf:resource="http://vocab.getty.edu/aat/300204905"/>
	<skos:editorialNote xml:lang="en">PPRefiningObjectType</skos:editorialNote>
	<skos:scopeNote xml:lang="en">Refers to the fixed soft coverings for furniture, especially seating and reclining furniture. Originally referred to all the textile components of a room supplied by upholsterers, including wall hangings, bed hangings, window curtains, and table coverings.</skos:scopeNote>
</skos:Concept>
<skos:Concept rdf:about="http://partage.vocnet.org/part00795">
	<skos:prefLabel xml:lang="en">shelves</skos:prefLabel>
	<skos:prefLabel xml:lang="hr">polica</skos:prefLabel>
	<skos:altLabel xml:lang="pt">prateleiras</skos:altLabel>
	<skos:prefLabel xml:lang="pt">prateleira</skos:prefLabel>
	<skos:altLabel xml:lang="de">Regale</skos:altLabel>
	<skos:prefLabel xml:lang="de">Regal</skos:prefLabel>
	<skos:prefLabel xml:lang="sv">hyllor</skos:prefLabel>
	<skos:prefLabel xml:lang="fi">hyllyt</skos:prefLabel>
	<skos:inScheme rdf:resource="http://partage.vocnet.org/Objects"/>
	<skos:broader rdf:resource="http://partage.vocnet.org/part00100"/>
	<skos:exactMatch rdf:resource="http://vocab.getty.edu/aat/300165847"/>
	<skos:scopeNote xml:lang="en">Boards, planks, or slabs of wood or any other rigid material fixed in a horizontal position to a wall or in a case, to hold books or other objects as in a bookcase or cabinet.</skos:scopeNote>
	<skos:editorialNote xml:lang="en">PPRefiningObjectType</skos:editorialNote>
</skos:Concept>
<skos:Concept rdf:about="http://partage.vocnet.org/part00796">
	<skos:prefLabel xml:lang="en">washstands</skos:prefLabel>
	<skos:prefLabel xml:lang="sv">tvättställ</skos:prefLabel>
	<skos:prefLabel xml:lang="hr">umivaonik</skos:prefLabel>
	<skos:prefLabel xml:lang="pt">lavatório</skos:prefLabel>
	<skos:altLabel xml:lang="de">Waschtische</skos:altLabel>
	<skos:prefLabel xml:lang="de">Waschtisch</skos:prefLabel>
	<skos:prefLabel xml:lang="fi">pesupöydät</skos:prefLabel>
	<skos:inScheme rdf:resource="http://partage.vocnet.org/Objects"/>
	<skos:broader rdf:resource="http://partage.vocnet.org/part00928"/>
	<skos:exactMatch rdf:resource="http://vocab.getty.edu/aat/300039857"/>
	<skos:editorialNote xml:lang="en">PPRefiningObjectType</skos:editorialNote>
	<skos:scopeNote xml:lang="en">Furniture combining features of a table and cupboard and used to hold articles (as a pitcher, basin, and towel) for washing the hands and face.</skos:scopeNote>
</skos:Concept>
<skos:Concept rdf:about="http://partage.vocnet.org/part00797">
	<skos:altLabel xml:lang="en">jardinières (containers)</skos:altLabel>
	<skos:prefLabel xml:lang="en">jardinières</skos:prefLabel>
	<skos:prefLabel xml:lang="hr">žardinjera</skos:prefLabel>
	<skos:altLabel xml:lang="de">Blumentöpfe</skos:altLabel>
	<skos:altLabel xml:lang="de">Blumengefäße</skos:altLabel>
	<skos:altLabel xml:lang="de">Blumentopf</skos:altLabel>
	<skos:prefLabel xml:lang="de">Blumengefäß</skos:prefLabel>
	<skos:prefLabel xml:lang="sv">jardinjärer</skos:prefLabel>
	<skos:prefLabel xml:lang="pt">floreira</skos:prefLabel>
	<skos:prefLabel xml:lang="fi">kukkaruukut</skos:prefLabel>
	<skos:inScheme rdf:resource="http://partage.vocnet.org/Objects"/>
	<skos:broader rdf:resource="http://partage.vocnet.org/part00939"/>
	<skos:exactMatch rdf:resource="http://vocab.getty.edu/aat/300200350"/>
	<skos:editorialNote xml:lang="en">PPRefiningObjectType</skos:editorialNote>
	<skos:scopeNote xml:lang="en">Ornamental containers for holding or growing plants or flowers. Use "cachepots" for ornamental containers for holding or concealing a flowerpot.</skos:scopeNote>
</skos:Concept>
<skos:Concept rdf:about="http://partage.vocnet.org/part00798">
	<skos:prefLabel xml:lang="en">dressing tables</skos:prefLabel>
	<skos:altLabel xml:lang="de">Frisiertische</skos:altLabel>
	<skos:prefLabel xml:lang="pt">toucador</skos:prefLabel>
	<skos:altLabel xml:lang="de">Schminktisch</skos:altLabel>
	<skos:altLabel xml:lang="de">Toilettentisch</skos:altLabel>
	<skos:altLabel xml:lang="de">Frisiertisch</skos:altLabel>
	<skos:prefLabel xml:lang="de">Frisiertoilette</skos:prefLabel>
	<skos:prefLabel xml:lang="sv">sminkbord</skos:prefLabel>
	<skos:prefLabel xml:lang="hr">toaletni stolić</skos:prefLabel>
	<skos:prefLabel xml:lang="fi">pukeutumispöydät</skos:prefLabel>
	<skos:inScheme rdf:resource="http://partage.vocnet.org/Objects"/>
	<skos:broader rdf:resource="http://partage.vocnet.org/part00316"/>
	<skos:exactMatch rdf:resource="http://vocab.getty.edu/aat/300039668"/>
	<skos:editorialNote xml:lang="en">PPRefiningObjectType</skos:editorialNote>
	<skos:scopeNote xml:lang="en">Generally applied to a variety of tables used for dressing, usually fitted with a mirror and having drawers to hold toilet articles such as brushes and combs.</skos:scopeNote>
</skos:Concept>
<skos:Concept rdf:about="http://partage.vocnet.org/part00799">
	<skos:altLabel xml:lang="en">wardrobes (case furniture)</skos:altLabel>
	<skos:prefLabel xml:lang="en">wardrobes</skos:prefLabel>
	<skos:prefLabel xml:lang="sv">garderober</skos:prefLabel>
	<skos:prefLabel xml:lang="hr">ormar</skos:prefLabel>
	<skos:altLabel xml:lang="pt">roupeiro</skos:altLabel>
	<skos:prefLabel xml:lang="pt">guardafatos</skos:prefLabel>
	<skos:altLabel xml:lang="de">Kleiderschränke</skos:altLabel>
	<skos:prefLabel xml:lang="de">Kleiderschrank</skos:prefLabel>
	<skos:prefLabel xml:lang="fi">vaatekaapit</skos:prefLabel>
	<skos:inScheme rdf:resource="http://partage.vocnet.org/Objects"/>
	<skos:broader rdf:resource="http://partage.vocnet.org/part00299"/>
	<skos:exactMatch rdf:resource="http://vocab.getty.edu/aat/300039237"/>
	<skos:editorialNote xml:lang="en">PPRefiningObjectType</skos:editorialNote>
	<skos:scopeNote xml:lang="en">Large upright pieces of furniture fitted with hooks, pegs, or rods, used for hanging clothes, generally with two large doors and perhaps a drawer or drawers below. Although there may be a shelf in a wardrobe, the term is typically distinct from "clothes presses," in which clothes are stored exclusively on shelves rather than hanging.</skos:scopeNote>
</skos:Concept>
<skos:Concept rdf:about="http://partage.vocnet.org/part00800">
	<skos:prefLabel xml:lang="en">vitrines (cabinets)</skos:prefLabel>
	<skos:prefLabel xml:lang="sv">vitrinskåp</skos:prefLabel>
	<skos:prefLabel xml:lang="hr">vitrina</skos:prefLabel>
	<skos:prefLabel xml:lang="pt">vitrina</skos:prefLabel>
	<skos:altLabel xml:lang="de">Vitrinen</skos:altLabel>
	<skos:prefLabel xml:lang="de">Vitrine</skos:prefLabel>
	<skos:prefLabel xml:lang="fi">vitriinit</skos:prefLabel>
	<skos:inScheme rdf:resource="http://partage.vocnet.org/Objects"/>
	<skos:broader rdf:resource="http://partage.vocnet.org/part00298"/>
	<skos:exactMatch rdf:resource="http://vocab.getty.edu/aat/300079633"/>
	<skos:editorialNote xml:lang="en">PPRefiningObjectType</skos:editorialNote>
	<skos:scopeNote xml:lang="en">Small cabinets with glass doors and generally glass shelves for the display of miniatures or art objects; developed in France and adopted elsewhere. Also, small tables with glass tops used for the same purpose.</skos:scopeNote>
</skos:Concept>
<skos:Concept rdf:about="http://partage.vocnet.org/part00801">
	<skos:altLabel xml:lang="en">sideboards (furniture)</skos:altLabel>
	<skos:prefLabel xml:lang="en">sideboards</skos:prefLabel>
	<skos:prefLabel xml:lang="sv">skänker</skos:prefLabel>
	<skos:prefLabel xml:lang="hr">ormar za posuđe</skos:prefLabel>
	<skos:altLabel xml:lang="pt">louceiro</skos:altLabel>
	<skos:prefLabel xml:lang="pt">aparador</skos:prefLabel>
	<skos:altLabel xml:lang="de">Kredenzen</skos:altLabel>
	<skos:altLabel xml:lang="de">Sideboards</skos:altLabel>
	<skos:altLabel xml:lang="de">Kredenz</skos:altLabel>
	<skos:prefLabel xml:lang="de">Sideboard</skos:prefLabel>
	<skos:prefLabel xml:lang="fi">astiakaapit.</skos:prefLabel>
	<skos:inScheme rdf:resource="http://partage.vocnet.org/Objects"/>
	<skos:broader rdf:resource="http://partage.vocnet.org/part00299"/>
	<skos:exactMatch rdf:resource="http://vocab.getty.edu/aat/300039306"/>
	<skos:editorialNote xml:lang="en">PPRefiningObjectType</skos:editorialNote>
	<skos:scopeNote xml:lang="en">Rather low, wide case pieces on legs with cupboard space beneath. They are placed along the wall of a dining room and used for storage, serving, and displaying plate and other precious tableware. Early pieces were often simply a board on legs placed near the dining table. By the 17th century sideboards were being designed with a cupboard or drawers beneath a flat table surface. The top was higher than a standard table, allowing the plate on display to be seen easily, as well as making the food more conveniently accessible to a standing person. Victorian sideboards often had levels or shelves above the primary surface, in order to create more space for displaying tableware. "Dressers (cupboards)" may be similar in design and function, but were typically found in kitchens rather than dining rooms. For side tables used along the walls of dining rooms, use "sideboard tables."</skos:scopeNote>
</skos:Concept>
<skos:Concept rdf:about="http://partage.vocnet.org/part00802">
	<skos:prefLabel xml:lang="en">étagères</skos:prefLabel>
	<skos:altLabel xml:lang="de">Etageren</skos:altLabel>
	<skos:prefLabel xml:lang="pt">étagéres</skos:prefLabel>
	<skos:prefLabel xml:lang="de">Etagere</skos:prefLabel>
	<skos:prefLabel xml:lang="sv">étagèrer</skos:prefLabel>
	<skos:prefLabel xml:lang="hr">polica.</skos:prefLabel>
	<skos:prefLabel xml:lang="fi">hyllyköt</skos:prefLabel>
	<skos:inScheme rdf:resource="http://partage.vocnet.org/Objects"/>
	<skos:broader rdf:resource="http://partage.vocnet.org/part00099"/>
	<skos:exactMatch rdf:resource="http://vocab.getty.edu/aat/300039300"/>
	<skos:editorialNote xml:lang="en">PPRefiningObjectType</skos:editorialNote>
	<skos:scopeNote xml:lang="en">Open-tiered shelves for displaying small objects; often with a mirrored back and sometimes having drawers or a cabinet below</skos:scopeNote>
</skos:Concept>
<skos:Concept rdf:about="http://partage.vocnet.org/part00803">
	<skos:prefLabel xml:lang="en">counters</skos:prefLabel>
	<skos:altLabel xml:lang="en">counters (furniture)</skos:altLabel>
	<skos:prefLabel xml:lang="pt">balcão</skos:prefLabel>
	<skos:altLabel xml:lang="de">Theken</skos:altLabel>
	<skos:prefLabel xml:lang="de">Theke</skos:prefLabel>
	<skos:altLabel xml:lang="de">Ladentheke</skos:altLabel>
	<skos:prefLabel xml:lang="sv">diskar</skos:prefLabel>
	<skos:altLabel xml:lang="hr">šank</skos:altLabel>
	<skos:prefLabel xml:lang="hr">pult</skos:prefLabel>
	<skos:prefLabel xml:lang="fi">tiskit</skos:prefLabel>
	<skos:inScheme rdf:resource="http://partage.vocnet.org/Objects"/>
	<skos:broader rdf:resource="http://partage.vocnet.org/part00299"/>
	<skos:exactMatch rdf:resource="http://vocab.getty.edu/aat/300121378"/>
	<skos:editorialNote xml:lang="en">PPRefiningObjectType</skos:editorialNote>
	<skos:scopeNote xml:lang="en">Cases or shelflike surfaces, usually of a height convenient for a person standing before them, as in a kitchen or store, or sitting on stools in front of them, as in a restaurant or bar. For small tables or chests with the top marked for counting money, sometimes with a cupboard below, use the more specific "counter tables."</skos:scopeNote>
</skos:Concept>
<skos:Concept rdf:about="http://partage.vocnet.org/part00804">
	<skos:prefLabel xml:lang="en">chests of drawers</skos:prefLabel>
	<skos:altLabel xml:lang="de">Kommoden</skos:altLabel>
	<skos:prefLabel xml:lang="de">Kommode</skos:prefLabel>
	<skos:prefLabel xml:lang="pt">cómoda</skos:prefLabel>
	<skos:prefLabel xml:lang="sv">byråer</skos:prefLabel>
	<skos:prefLabel xml:lang="hr">komoda</skos:prefLabel>
	<skos:prefLabel xml:lang="fi">laatikostot</skos:prefLabel>
	<skos:inScheme rdf:resource="http://partage.vocnet.org/Objects"/>
	<skos:broader rdf:resource="http://partage.vocnet.org/part00299"/>
	<skos:exactMatch rdf:resource="http://vocab.getty.edu/aat/300039009"/>
	<skos:editorialNote xml:lang="en">PPRefiningObjectType</skos:editorialNote>
	<skos:scopeNote xml:lang="en">Refers to case furniture characterized by having drawers, typically three to five in number. A chest of drawers is generally supported on feet, but sometimes rests directly on the floor. Use "commodes (chests of drawers)" for similar case pieces generally supported on short legs. Use "chests with drawers" for chests with one or more tiers of drawers below a deep storage space.</skos:scopeNote>
</skos:Concept>
<skos:Concept rdf:about="http://partage.vocnet.org/part00805">
	<skos:prefLabel xml:lang="en">bookcases</skos:prefLabel>
	<skos:prefLabel xml:lang="sv">bokhyllor</skos:prefLabel>
	<skos:prefLabel xml:lang="pt">estante</skos:prefLabel>
	<skos:altLabel xml:lang="de">Bücherschränke</skos:altLabel>
	<skos:prefLabel xml:lang="de">Bücherschrank</skos:prefLabel>
	<skos:prefLabel xml:lang="hr">ormar za knjige</skos:prefLabel>
	<skos:prefLabel xml:lang="fi">kirjakaapit</skos:prefLabel>
	<skos:inScheme rdf:resource="http://partage.vocnet.org/Objects"/>
	<skos:broader rdf:resource="http://partage.vocnet.org/part00299"/>
	<skos:exactMatch rdf:resource="http://vocab.getty.edu/aat/300143716"/>
	<skos:editorialNote xml:lang="en">PPRefiningObjectType</skos:editorialNote>
	<skos:scopeNote xml:lang="en">Cases for holding books generally having several shelves enclosed by doors; distinct from "bookshelves" which are open shelves for holding books.</skos:scopeNote>
</skos:Concept>
<skos:Concept rdf:about="http://partage.vocnet.org/part00806">
	<skos:prefLabel xml:lang="en">tabourets (low stools)</skos:prefLabel>
	<skos:prefLabel xml:lang="sv">taburetter</skos:prefLabel>
	<skos:prefLabel xml:lang="hr">tabouret</skos:prefLabel>
	<skos:prefLabel xml:lang="pt">banquinho</skos:prefLabel>
	<skos:prefLabel xml:lang="de">Schemel</skos:prefLabel>
	<skos:prefLabel xml:lang="fi">taburetit</skos:prefLabel>
	<skos:inScheme rdf:resource="http://partage.vocnet.org/Objects"/>
	<skos:broader rdf:resource="http://partage.vocnet.org/part00309"/>
	<skos:exactMatch rdf:resource="http://vocab.getty.edu/aat/300038459"/>
	<skos:editorialNote xml:lang="en">PPRefiningObjectType</skos:editorialNote>
	<skos:scopeNote xml:lang="en">Refers to low seats or stools, without back or arms, often used for a child or as a footstool. It was originally in the shape of a drum, thus the name (from the diminutive of the French "tambour," for drum). In the 18th century the term was applied to any low stool with fixed upright legs, as distinct from "pliants," which had folding crossed legs. 18th-century tabourets were rectangular, not drum-shaped, with upholstered seats. For similar seats supported on six or more legs, use "banquettes (benches)."</skos:scopeNote>
</skos:Concept>
<skos:Concept rdf:about="http://partage.vocnet.org/part00807">
	<skos:prefLabel xml:lang="en">armchairs</skos:prefLabel>
	<skos:prefLabel xml:lang="sv">fåtöljer</skos:prefLabel>
	<skos:altLabel xml:lang="de">Fauteuils</skos:altLabel>
	<skos:altLabel xml:lang="de">Fauteuil</skos:altLabel>
	<skos:altLabel xml:lang="de">Lehnstühle</skos:altLabel>
	<skos:altLabel xml:lang="de">Polstersessel</skos:altLabel>
	<skos:prefLabel xml:lang="de">Lehnstuhl</skos:prefLabel>
	<skos:prefLabel xml:lang="pt">poltrona</skos:prefLabel>
	<skos:prefLabel xml:lang="hr">naslonjač</skos:prefLabel>
	<skos:prefLabel xml:lang="fi">nojatuolit</skos:prefLabel>
	<skos:inScheme rdf:resource="http://partage.vocnet.org/Objects"/>
	<skos:broader rdf:resource="http://partage.vocnet.org/part00308"/>
	<skos:exactMatch rdf:resource="http://vocab.getty.edu/aat/300037776"/>
	<skos:editorialNote xml:lang="en">PPRefiningObjectType</skos:editorialNote>
	<skos:scopeNote xml:lang="en">Term applied to a wide variety of chairs with arms, to distinguish them from side chairs which have no arms.</skos:scopeNote>
</skos:Concept>
<skos:Concept rdf:about="http://partage.vocnet.org/part00808">
	<skos:prefLabel xml:lang="en">carpets</skos:prefLabel>
	<skos:prefLabel xml:lang="sv">mattor</skos:prefLabel>
	<skos:prefLabel xml:lang="pt">carpetes</skos:prefLabel>
	<skos:altLabel xml:lang="de">Bodenteppiche</skos:altLabel>
	<skos:altLabel xml:lang="de">Bodenteppich</skos:altLabel>
	<skos:altLabel xml:lang="de">Teppiche</skos:altLabel>
	<skos:prefLabel xml:lang="de">Teppich</skos:prefLabel>
	<skos:prefLabel xml:lang="hr">tepih</skos:prefLabel>
	<skos:prefLabel xml:lang="fi">matot (sisustus)</skos:prefLabel>
	<skos:inScheme rdf:resource="http://partage.vocnet.org/Objects"/>
	<skos:broader rdf:resource="http://partage.vocnet.org/part00504"/>
	<skos:exactMatch rdf:resource="http://vocab.getty.edu/aat/300185756"/>
	<skos:editorialNote xml:lang="en">PPRefiningObjectType</skos:editorialNote>
	<skos:scopeNote xml:lang="en">Rugs of some size whose primary use is to cover a flat surface; carpets constitute the largest and most familiar group of rugs.</skos:scopeNote>
</skos:Concept>
<skos:Concept rdf:about="http://partage.vocnet.org/part00809">
	<skos:prefLabel xml:lang="en">centerpieces</skos:prefLabel>
	<skos:altLabel xml:lang="en">centerpieces (furnishings)</skos:altLabel>
	<skos:prefLabel xml:lang="sv">bordsuppsatser</skos:prefLabel>
	<skos:prefLabel xml:lang="pt">centro de mesa</skos:prefLabel>
	<skos:altLabel xml:lang="de">Tafelaufsätze</skos:altLabel>
	<skos:prefLabel xml:lang="de">Tafelaufsatz</skos:prefLabel>
	<skos:prefLabel xml:lang="hr">podnos</skos:prefLabel>
	<skos:prefLabel xml:lang="fi">pöytäkoristeet</skos:prefLabel>
	<skos:inScheme rdf:resource="http://partage.vocnet.org/Objects"/>
	<skos:broader rdf:resource="http://partage.vocnet.org/part00100"/>
	<skos:exactMatch rdf:resource="http://vocab.getty.edu/aat/300043082"/>
	<skos:editorialNote xml:lang="en">PPRefiningObjectType</skos:editorialNote>
	<skos:scopeNote xml:lang="en">Ornamental and often also functional pieces of silverplate, glass, flower arrangements, or other items intended for display and use in the center of a dining table.</skos:scopeNote>
</skos:Concept>
<skos:Concept rdf:about="http://partage.vocnet.org/part00810">
	<skos:altLabel xml:lang="en">frames (furnishings)</skos:altLabel>
	<skos:prefLabel xml:lang="en">frames</skos:prefLabel>
	<skos:prefLabel xml:lang="sv">ramar</skos:prefLabel>
	<skos:prefLabel xml:lang="pt">moldura</skos:prefLabel>
	<skos:prefLabel xml:lang="de">Bilderrahmen</skos:prefLabel>
	<skos:prefLabel xml:lang="hr">okvir</skos:prefLabel>
	<skos:prefLabel xml:lang="fi">kehykset</skos:prefLabel>
	<skos:inScheme rdf:resource="http://partage.vocnet.org/Objects"/>
	<skos:broader rdf:resource="http://partage.vocnet.org/part00099"/>
	<skos:exactMatch rdf:resource="http://vocab.getty.edu/aat/300189814"/>
	<skos:editorialNote xml:lang="en">PPRefiningObjectType</skos:editorialNote>
	<skos:scopeNote xml:lang="en">Cases or structures that surround or enclose such items as works of art, mirrors, or documents, serving as support or protection or to call attention, while leaving the items visible.</skos:scopeNote>
</skos:Concept>
<skos:Concept rdf:about="http://partage.vocnet.org/part00811">
	<skos:prefLabel xml:lang="en">creamware</skos:prefLabel>
	<skos:prefLabel xml:lang="pt">faiança</skos:prefLabel>
	<skos:prefLabel xml:lang="de">Cremefarbenes Irdengut</skos:prefLabel>
	<skos:prefLabel xml:lang="sv">flintgods</skos:prefLabel>
	<skos:prefLabel xml:lang="hr">kamenina</skos:prefLabel>
	<skos:prefLabel xml:lang="fi">piiposliini</skos:prefLabel>
	<skos:inScheme rdf:resource="http://partage.vocnet.org/Objects"/>
	<skos:broader rdf:resource="http://partage.vocnet.org/part00223"/>
	<skos:exactMatch rdf:resource="http://vocab.getty.edu/aat/300163214"/>
	<skos:editorialNote xml:lang="en">PPRefiningObjectType</skos:editorialNote>
	<skos:scopeNote xml:lang="en">Refers to English earthenware that is cream-colored with a transparent lead glaze dating from the second half of the 18th century; it also refers to imitations of this English ware. It was originally developed by Staffordshire potters, who were experimenting to find a substitute for Chinese porcelain. Around 1750 they created a a fine white earthenware with a rich yellowish glaze; the ware had a light body and clean glaze, making it desirable for domestic ware. At the time, the cream color was considered a fault; as an improvement, Wedgwood introduced a white to bluish white product called "pearlware" in 1779. It was produced for nearly a century. Creamware, however, continued to be made throughout the 19th century and later.</skos:scopeNote>
</skos:Concept>
<skos:Concept rdf:about="http://partage.vocnet.org/part00812">
	<skos:prefLabel xml:lang="en">exterior views</skos:prefLabel>
	<skos:altLabel xml:lang="de">Außenansichten</skos:altLabel>
	<skos:prefLabel xml:lang="pt">vista exterior</skos:prefLabel>
	<skos:prefLabel xml:lang="de">Außenansicht</skos:prefLabel>
	<skos:prefLabel xml:lang="sv">exteriörer</skos:prefLabel>
	<skos:prefLabel xml:lang="hr">eksterijer</skos:prefLabel>
	<skos:prefLabel xml:lang="fi">ulkokuva</skos:prefLabel>
	<skos:inScheme rdf:resource="http://partage.vocnet.org/Objects"/>
	<skos:broader rdf:resource="http://partage.vocnet.org/part00406"/>
	<skos:exactMatch rdf:resource="http://vocab.getty.edu/aat/300124515"/>
	<skos:editorialNote xml:lang="en">PPRefiningObjectType</skos:editorialNote>
	<skos:scopeNote xml:lang="en">Refers to photographs or other representations of the exterior of a building or other structure or object that has interior and exterior spaces.</skos:scopeNote>
</skos:Concept>
<skos:Concept rdf:about="http://partage.vocnet.org/part00813">
	<skos:altLabel xml:lang="en">reliefs (sculptures)</skos:altLabel>
	<skos:prefLabel xml:lang="en">reliefs</skos:prefLabel>
	<skos:prefLabel xml:lang="hr">reljef</skos:prefLabel>
	<skos:prefLabel xml:lang="pt">relevo</skos:prefLabel>
	<skos:altLabel xml:lang="de">Reliefs</skos:altLabel>
	<skos:prefLabel xml:lang="de">Relief</skos:prefLabel>
	<skos:prefLabel xml:lang="sv">reliefer (skulpturer)</skos:prefLabel>
	<skos:prefLabel xml:lang="fi">reliefit</skos:prefLabel>
	<skos:inScheme rdf:resource="http://partage.vocnet.org/Objects"/>
	<skos:broader rdf:resource="http://partage.vocnet.org/part00041"/>
	<skos:exactMatch rdf:resource="http://vocab.getty.edu/aat/300047230"/>
	<skos:editorialNote xml:lang="en">PPRefiningObjectType</skos:editorialNote>
	<skos:scopeNote xml:lang="en">Sculptures in which the ornaments or figures are attached to a background from which they stand out to a greater or lesser degree. Reliefs are often used as architectural decoration and because of their capacity for narration they are often used for pictorial narrative purposes.</skos:scopeNote>
</skos:Concept>
<skos:Concept rdf:about="http://partage.vocnet.org/part00814">
	<skos:prefLabel xml:lang="en">miniatures (paintings)</skos:prefLabel>
	<skos:prefLabel xml:lang="hr">minijatura</skos:prefLabel>
	<skos:prefLabel xml:lang="de">Miniaturen</skos:prefLabel>
	<skos:altLabel xml:lang="de">Miniatur</skos:altLabel>
	<skos:prefLabel xml:lang="sv">miniatyrer (målningar)</skos:prefLabel>
	<skos:prefLabel xml:lang="pt">miniaturas</skos:prefLabel>
	<skos:prefLabel xml:lang="fi">miniatyyrit</skos:prefLabel>
	<skos:inScheme rdf:resource="http://partage.vocnet.org/Objects"/>
	<skos:broader rdf:resource="http://partage.vocnet.org/part00044"/>
	<skos:exactMatch rdf:resource="http://vocab.getty.edu/aat/300033936"/>
	<skos:editorialNote xml:lang="en">PPRefiningObjectType</skos:editorialNote>
	<skos:scopeNote xml:lang="en">Paintings on a very small scale. The term is often applied specifically to small scenes in illuminated manuscripts or to portraits on vellum or ivory that were popular in Europe and America from the Renaissance into the 19th century. For paintings in manuscripts, the term "illuminations" may also be appropriate.</skos:scopeNote>
</skos:Concept>
<skos:Concept rdf:about="http://partage.vocnet.org/part00815">
	<skos:prefLabel xml:lang="en">altarpieces</skos:prefLabel>
	<skos:prefLabel xml:lang="sv">altaruppsatser</skos:prefLabel>
	<skos:prefLabel xml:lang="pt">altar</skos:prefLabel>
	<skos:altLabel xml:lang="de">Altarbilder</skos:altLabel>
	<skos:prefLabel xml:lang="de">Altarbild</skos:prefLabel>
	<skos:prefLabel xml:lang="hr">oltarna pala</skos:prefLabel>
	<skos:prefLabel xml:lang="fi">alttaritaulut</skos:prefLabel>
	<skos:inScheme rdf:resource="http://partage.vocnet.org/Objects"/>
	<skos:exactMatch rdf:resource="http://vocab.getty.edu/aat/300075940"/>
	<skos:editorialNote xml:lang="en">PPRefiningObjectType</skos:editorialNote>
	<skos:scopeNote xml:lang="en">Refers to painted or carved image-bearing objects in a Christian church. Altarpieces are characterized by usually being framed and either set on the rear part of the altar abutting the back of the altarblock or hung on the wall behind the altar. Altarpieces may be set on both the central high altar and side altars. The subject of the image is typically a religious figure or figures, often included in a narrative or didactic scene; it may also include a patron of the church.</skos:scopeNote>
</skos:Concept>
<skos:Concept rdf:about="http://partage.vocnet.org/part00816">
	<skos:prefLabel xml:lang="en">woodcuts</skos:prefLabel>
	<skos:altLabel xml:lang="en">woodcuts (prints)</skos:altLabel>
	<skos:prefLabel xml:lang="sv">träsnitt</skos:prefLabel>
	<skos:prefLabel xml:lang="hr">drvorez</skos:prefLabel>
	<skos:prefLabel xml:lang="pt">xilogravura</skos:prefLabel>
	<skos:altLabel xml:lang="de">Holzschnitte</skos:altLabel>
	<skos:prefLabel xml:lang="de">Holzschnitt</skos:prefLabel>
	<skos:prefLabel xml:lang="fi">puupiirros</skos:prefLabel>
	<skos:inScheme rdf:resource="http://partage.vocnet.org/Objects"/>
	<skos:broader rdf:resource="http://partage.vocnet.org/part00837"/>
	<skos:exactMatch rdf:resource="http://vocab.getty.edu/aat/300041405"/>
	<skos:editorialNote xml:lang="en">PPRefiningObjectType</skos:editorialNote>
	<skos:scopeNote xml:lang="en">Prints made using the process of woodcut, which is a relief process in which the design is cut into and printed from the plank side of a wood block; distinct from "wood engraving (process)," which is a relief process using the grain end of a wood block.</skos:scopeNote>
</skos:Concept>
<skos:Concept rdf:about="http://partage.vocnet.org/part00817">
	<skos:altLabel xml:lang="en">linocuts (prints)</skos:altLabel>
	<skos:prefLabel xml:lang="en">linocuts</skos:prefLabel>
	<skos:prefLabel xml:lang="hr">linorez</skos:prefLabel>
	<skos:altLabel xml:lang="de">Linolschnitte</skos:altLabel>
	<skos:prefLabel xml:lang="de">Linolschnitt</skos:prefLabel>
	<skos:prefLabel xml:lang="sv">linoleumsnitt</skos:prefLabel>
	<skos:prefLabel xml:lang="pt">linótipo</skos:prefLabel>
	<skos:prefLabel xml:lang="fi">linopiirros</skos:prefLabel>
	<skos:inScheme rdf:resource="http://partage.vocnet.org/Objects"/>
	<skos:broader rdf:resource="http://partage.vocnet.org/part00837"/>
	<skos:exactMatch rdf:resource="http://vocab.getty.edu/aat/300041393"/>
	<skos:editorialNote xml:lang="en">PPRefiningObjectType</skos:editorialNote>
	<skos:scopeNote xml:lang="en">Prints made from a design cut in linoleum-faced blocks on which a knife or gouge has been used to recess the non-printing area and leave the image to be printed in relief.</skos:scopeNote>
</skos:Concept>
<skos:Concept rdf:about="http://partage.vocnet.org/part00818">
	<skos:altLabel xml:lang="en">etchings (prints)</skos:altLabel>
	<skos:prefLabel xml:lang="en">etchings</skos:prefLabel>
	<skos:prefLabel xml:lang="pt">água-forte</skos:prefLabel>
	<skos:prefLabel xml:lang="sv">etsningar</skos:prefLabel>
	<skos:altLabel xml:lang="de">Radierungen</skos:altLabel>
	<skos:prefLabel xml:lang="de">Radierung</skos:prefLabel>
	<skos:prefLabel xml:lang="hr">bakropis</skos:prefLabel>
	<skos:prefLabel xml:lang="fi">etsaukset</skos:prefLabel>
	<skos:inScheme rdf:resource="http://partage.vocnet.org/Objects"/>
	<skos:broader rdf:resource="http://partage.vocnet.org/part00836"/>
	<skos:exactMatch rdf:resource="http://vocab.getty.edu/aat/300041365"/>
	<skos:editorialNote xml:lang="en">PPRefiningObjectType</skos:editorialNote>
	<skos:scopeNote xml:lang="en">Prints made from an etched printing plate, which is a metal plate on which a design is made by coating the plate with an acid-resistant substance, creating a design in the coating, and then exposing the plate to acid, which etches the plate where the metal is exposed. For designs incised directly into a copper plate using a burin or graver, use "engravings (prints)."</skos:scopeNote>
</skos:Concept>
<skos:Concept rdf:about="http://partage.vocnet.org/part00819">
	<skos:altLabel xml:lang="en">drypoints (prints)</skos:altLabel>
	<skos:prefLabel xml:lang="en">drypoints</skos:prefLabel>
	<skos:altLabel xml:lang="pt">gravura ponta seca</skos:altLabel>
	<skos:prefLabel xml:lang="pt">ponta seca</skos:prefLabel>
	<skos:altLabel xml:lang="de">Kaltnadelblätter</skos:altLabel>
	<skos:prefLabel xml:lang="de">Kaltnadel</skos:prefLabel>
	<skos:prefLabel xml:lang="sv">torrnålsgravyrer</skos:prefLabel>
	<skos:prefLabel xml:lang="hr">suha igla</skos:prefLabel>
	<skos:prefLabel xml:lang="fi">kuivaneulapiirros</skos:prefLabel>
	<skos:inScheme rdf:resource="http://partage.vocnet.org/Objects"/>
	<skos:broader rdf:resource="http://partage.vocnet.org/part00836"/>
	<skos:exactMatch rdf:resource="http://vocab.getty.edu/aat/300041349"/>
	<skos:editorialNote xml:lang="en">PPRefiningObjectType</skos:editorialNote>
	<skos:scopeNote xml:lang="en">Prints made using the drypoint process.</skos:scopeNote>
</skos:Concept>
<skos:Concept rdf:about="http://partage.vocnet.org/part00820">
	<skos:altLabel xml:lang="en">engravings (prints)</skos:altLabel>
	<skos:prefLabel xml:lang="en">engravings</skos:prefLabel>
	<skos:prefLabel xml:lang="pt">gravura</skos:prefLabel>
	<skos:prefLabel xml:lang="de">Kupferstich</skos:prefLabel>
	<skos:prefLabel xml:lang="sv">gravyrer</skos:prefLabel>
	<skos:altLabel xml:lang="de">Kupferstiche</skos:altLabel>
	<skos:prefLabel xml:lang="hr">bakrorez</skos:prefLabel>
	<skos:prefLabel xml:lang="fi">kaiverrukset</skos:prefLabel>
	<skos:inScheme rdf:resource="http://partage.vocnet.org/Objects"/>
	<skos:broader rdf:resource="http://partage.vocnet.org/part00836"/>
	<skos:narrower rdf:resource="http://partage.vocnet.org/part01245"/>
	<skos:exactMatch rdf:resource="http://vocab.getty.edu/aat/300041340"/>
	<skos:editorialNote xml:lang="en">PPRefiningObjectType</skos:editorialNote>
	<skos:scopeNote xml:lang="en">Prints on paper incorporating impressions of a reverse design created on a printing plate, usually copper, into which the design has been incised (engraved) using burins or gravers. Historically, "engravings" has sometimes been incorrectly used to refer to all prints, regardless of the specific technique. For prints made from designs engraved on a flat wooden block, use "wood cuts"; for prints made from a plate that is etched rather than engraved, use "etchings."</skos:scopeNote>
</skos:Concept>
<skos:Concept rdf:about="http://partage.vocnet.org/part00821">
	<skos:prefLabel xml:lang="en">cartoons (working drawings)</skos:prefLabel>
	<skos:prefLabel xml:lang="sv">kartonger</skos:prefLabel>
	<skos:prefLabel xml:lang="pt">esboços</skos:prefLabel>
	<skos:altLabel xml:lang="de">Kartons (Entwürfe)</skos:altLabel>
	<skos:prefLabel xml:lang="de">Karton (Entwurf)</skos:prefLabel>
	<skos:prefLabel xml:lang="hr">karton</skos:prefLabel>
	<skos:prefLabel xml:lang="fi">luonnokset.</skos:prefLabel>
	<skos:inScheme rdf:resource="http://partage.vocnet.org/Objects"/>
	<skos:broader rdf:resource="http://partage.vocnet.org/part00948"/>
	<skos:exactMatch rdf:resource="http://vocab.getty.edu/aat/300034442"/>
	<skos:editorialNote xml:lang="en">PPRefiningObjectType</skos:editorialNote>
	<skos:scopeNote xml:lang="en">Refers to full-size preparatory drawings made for the purpose of transferring a design to the working surface of a painting, tapestry, or other large work.</skos:scopeNote>
</skos:Concept>
<skos:Concept rdf:about="http://partage.vocnet.org/part00822">
	<skos:altLabel xml:lang="en">aquatints (prints)</skos:altLabel>
	<skos:prefLabel xml:lang="en">aquatints</skos:prefLabel>
	<skos:prefLabel xml:lang="sv">akvatintlavyrer</skos:prefLabel>
	<skos:prefLabel xml:lang="pl">água forte</skos:prefLabel>
	<skos:altLabel xml:lang="de">Aquatintas</skos:altLabel>
	<skos:prefLabel xml:lang="de">Aquatinta</skos:prefLabel>
	<skos:prefLabel xml:lang="hr">akvatinta</skos:prefLabel>
	<skos:prefLabel xml:lang="fi">akvatinta</skos:prefLabel>
	<skos:inScheme rdf:resource="http://partage.vocnet.org/Objects"/>
	<skos:broader rdf:resource="http://partage.vocnet.org/part00836"/>
	<skos:exactMatch rdf:resource="http://vocab.getty.edu/aat/300041366"/>
	<skos:editorialNote xml:lang="en">PPRefiningObjectType</skos:editorialNote>
	<skos:scopeNote xml:lang="en">Prints produced from designs created by the aquatint process, by which a printing plate is covered with a coating and etched with acid so as to create a range of tonal values, often combined with line work. The resulting print resembling a watercolor.</skos:scopeNote>
</skos:Concept>
<skos:Concept rdf:about="http://partage.vocnet.org/part00823">
	<skos:prefLabel xml:lang="en">pedestals</skos:prefLabel>
	<skos:prefLabel xml:lang="hr">postament</skos:prefLabel>
	<skos:prefLabel xml:lang="de">Piedestal</skos:prefLabel>
	<skos:prefLabel xml:lang="sv">pedestaler</skos:prefLabel>
	<skos:prefLabel xml:lang="pt">pedestral</skos:prefLabel>
	<skos:prefLabel xml:lang="fi">jalustat.</skos:prefLabel>
	<skos:inScheme rdf:resource="http://partage.vocnet.org/Objects"/>
	<skos:broader rdf:resource="http://partage.vocnet.org/part00127"/>
	<skos:exactMatch rdf:resource="http://vocab.getty.edu/aat/300001744"/>
	<skos:editorialNote xml:lang="en">PPRefiningObjectType</skos:editorialNote>
	<skos:scopeNote xml:lang="en">Solid, fixed supports found under such architectural elements as columns or balustrades, or built in to hold sculpture; may also be used for freestanding furniture supports, usually for decorative objects, sometimes incorporating cabinets or shelves; usually classically divided by tripartation into base, dado, and cap.</skos:scopeNote>
</skos:Concept>
<skos:Concept rdf:about="http://partage.vocnet.org/part00824">
	<skos:prefLabel xml:lang="en">carbon prints</skos:prefLabel>
	<skos:inScheme rdf:resource="http://partage.vocnet.org/Objects"/>
	<skos:broader rdf:resource="http://partage.vocnet.org/part00921"/>
	<skos:narrower rdf:resource="http://partage.vocnet.org/part00893"/>
	<skos:exactMatch rdf:resource="http://vocab.getty.edu/aat/300127138"/>
	<skos:scopeNote xml:lang="en">Photographic prints made by the carbon process, which uses carbon pigment and gelatin to transfer images to a paper support. Carbon prints show a very slight relief and rarely exhibit signs of aging or image deterioration. During the last quarter of the 19th century they were widely used for book illustrations and the commercial reproduction of conventionally made photographs and prints.</skos:scopeNote>
</skos:Concept>
<skos:Concept rdf:about="http://partage.vocnet.org/part00825">
	<skos:prefLabel xml:lang="en">balusters</skos:prefLabel>
	<skos:altLabel xml:lang="en">balusters (railing components)</skos:altLabel>
	<skos:prefLabel xml:lang="sv">balustrar</skos:prefLabel>
	<skos:prefLabel xml:lang="pt">balaústre</skos:prefLabel>
	<skos:prefLabel xml:lang="de">Baluster</skos:prefLabel>
	<skos:prefLabel xml:lang="hr">balustar</skos:prefLabel>
	<skos:prefLabel xml:lang="fi">pylväät</skos:prefLabel>
	<skos:inScheme rdf:resource="http://partage.vocnet.org/Objects"/>
	<skos:broader rdf:resource="http://partage.vocnet.org/part00127"/>
	<skos:exactMatch rdf:resource="http://vocab.getty.edu/aat/300003287"/>
	<skos:editorialNote xml:lang="en">PPRefiningObjectType</skos:editorialNote>
	<skos:scopeNote xml:lang="en">Short vertical members used to support a stair handrail or coping, often circular in section with a vase-shaped outline. Used also in furniture, as on the backs of chairs.</skos:scopeNote>
</skos:Concept>
<skos:Concept rdf:about="http://partage.vocnet.org/part00826">
	<skos:prefLabel xml:lang="en">railings</skos:prefLabel>
	<skos:altLabel xml:lang="en">railings (balustrades)</skos:altLabel>
	<skos:altLabel xml:lang="hr">rešetka</skos:altLabel>
	<skos:prefLabel xml:lang="hr">ograda</skos:prefLabel>
	<skos:prefLabel xml:lang="pt">grade</skos:prefLabel>
	<skos:prefLabel xml:lang="de">Geländer</skos:prefLabel>
	<skos:prefLabel xml:lang="ru">räcken</skos:prefLabel>
	<skos:prefLabel xml:lang="fi">kaiteet.</skos:prefLabel>
	<skos:inScheme rdf:resource="http://partage.vocnet.org/Objects"/>
	<skos:broader rdf:resource="http://partage.vocnet.org/part00127"/>
	<skos:exactMatch rdf:resource="http://vocab.getty.edu/aat/300002018"/>
	<skos:editorialNote xml:lang="en">PPRefiningObjectType</skos:editorialNote>
	<skos:scopeNote xml:lang="en">Parapets or balustrades of a lightweight, partly open, metal or wood construction.</skos:scopeNote>
</skos:Concept>
<skos:Concept rdf:about="http://partage.vocnet.org/part00827">
	<skos:prefLabel xml:lang="en">balustrades</skos:prefLabel>
	<skos:altLabel xml:lang="de">Balustraden</skos:altLabel>
	<skos:altLabel xml:lang="de">Brüstung</skos:altLabel>
	<skos:prefLabel xml:lang="de">Balustrade</skos:prefLabel>
	<skos:prefLabel xml:lang="pt">balaustrada</skos:prefLabel>
	<skos:prefLabel xml:lang="sv">balustrader</skos:prefLabel>
	<skos:prefLabel xml:lang="hr">balustrada</skos:prefLabel>
	<skos:prefLabel xml:lang="fi">kaiteet</skos:prefLabel>
	<skos:inScheme rdf:resource="http://partage.vocnet.org/Objects"/>
	<skos:broader rdf:resource="http://partage.vocnet.org/part00127"/>
	<skos:exactMatch rdf:resource="http://vocab.getty.edu/aat/300001989"/>
	<skos:editorialNote xml:lang="en">PPRefiningObjectType</skos:editorialNote>
	<skos:scopeNote xml:lang="en">Parapets or low screens composed of balusters and carrying a rail or other horizontal member that is usually heavy in proportion to the balusters themselves.</skos:scopeNote>
</skos:Concept>
<skos:Concept rdf:about="http://partage.vocnet.org/part00828">
	<skos:prefLabel xml:lang="en">radiator enclosures</skos:prefLabel>
	<skos:prefLabel xml:lang="hr">panel za radijator</skos:prefLabel>
	<skos:prefLabel xml:lang="pt">cobertura de aquecedor</skos:prefLabel>
	<skos:altLabel xml:lang="de">Heizkörperverkleidungen</skos:altLabel>
	<skos:prefLabel xml:lang="de">Heizkörperverkleidung</skos:prefLabel>
	<skos:prefLabel xml:lang="sv">elementskydd</skos:prefLabel>
	<skos:prefLabel xml:lang="fi">patterinsuojukset</skos:prefLabel>
	<skos:inScheme rdf:resource="http://partage.vocnet.org/Objects"/>
	<skos:broader rdf:resource="http://partage.vocnet.org/part00116"/>
	<skos:exactMatch rdf:resource="http://vocab.getty.edu/aat/300250349"/>
	<skos:editorialNote xml:lang="en">PPRefiningObjectType</skos:editorialNote>
	<skos:scopeNote xml:lang="en">Boxlike housings, usually of metal, placed over radiators to hide them from view, redirect the flow of warm air, or provide protection from a hot surface.</skos:scopeNote>
</skos:Concept>
<skos:Concept rdf:about="http://partage.vocnet.org/part00829">
	<skos:prefLabel xml:lang="en">fire screens (metal)</skos:prefLabel>
	<skos:altLabel xml:lang="en">fire screens (equipment)</skos:altLabel>
	<skos:prefLabel xml:lang="sv">eldskärmar (metal)</skos:prefLabel>
	<skos:prefLabel xml:lang="pt">guarda fogo (metal)</skos:prefLabel>
	<skos:altLabel xml:lang="de">Feuerschirme</skos:altLabel>
	<skos:altLabel xml:lang="de">Feuerschirm</skos:altLabel>
	<skos:altLabel xml:lang="de">Kaminschirme (Metall)</skos:altLabel>
	<skos:prefLabel xml:lang="de">Kaminschirm (Metall)</skos:prefLabel>
	<skos:prefLabel xml:lang="hr">zaslon za peć.</skos:prefLabel>
	<skos:prefLabel xml:lang="fi">kipinäsuojukset</skos:prefLabel>
	<skos:inScheme rdf:resource="http://partage.vocnet.org/Objects"/>
	<skos:broader rdf:resource="http://partage.vocnet.org/part00218"/>
	<skos:exactMatch rdf:resource="http://vocab.getty.edu/aat/300262203"/>
	<skos:editorialNote xml:lang="en">PPRefiningObjectType</skos:editorialNote>
	<skos:scopeNote xml:lang="en">Protective devices made of woven or linked metal placed in front of fireplace openings to prevent sparks or embers from escaping.</skos:scopeNote>
</skos:Concept>
<skos:Concept rdf:about="http://partage.vocnet.org/part00830">
	<skos:prefLabel xml:lang="en">stoves (heating equipment)</skos:prefLabel>
	<skos:prefLabel xml:lang="sv">kaminer</skos:prefLabel>
	<skos:prefLabel xml:lang="hr">peć</skos:prefLabel>
	<skos:prefLabel xml:lang="pt">fogão</skos:prefLabel>
	<skos:altLabel xml:lang="de">Öfen</skos:altLabel>
	<skos:altLabel xml:lang="de">Herde</skos:altLabel>
	<skos:altLabel xml:lang="de">Ofen</skos:altLabel>
	<skos:prefLabel xml:lang="de">Herd</skos:prefLabel>
	<skos:altLabel xml:lang="fi">hellat</skos:altLabel>
	<skos:prefLabel xml:lang="fi">liedet</skos:prefLabel>
	<skos:inScheme rdf:resource="http://partage.vocnet.org/Objects"/>
	<skos:broader rdf:resource="http://partage.vocnet.org/part00218"/>
	<skos:exactMatch rdf:resource="http://vocab.getty.edu/aat/300052201"/>
	<skos:scopeNote xml:lang="en">Portable or fixed apparatuses that furnish heat for warmth or cooking, commonly using coal, oil, gas, wood, or electricity as a source of power.</skos:scopeNote>
	<skos:editorialNote xml:lang="en">PPRefiningObjectType</skos:editorialNote>
</skos:Concept>
<skos:Concept rdf:about="http://partage.vocnet.org/part00831">
	<skos:prefLabel xml:lang="en">pencils</skos:prefLabel>
	<skos:altLabel xml:lang="en">pencils (drawing and writing equipment)</skos:altLabel>
	<skos:prefLabel xml:lang="hr">olovka</skos:prefLabel>
	<skos:altLabel xml:lang="de">Stift</skos:altLabel>
	<skos:prefLabel xml:lang="de">Bleistift</skos:prefLabel>
	<skos:prefLabel xml:lang="sv">blyertspennor.</skos:prefLabel>
	<skos:prefLabel xml:lang="pt">lápis</skos:prefLabel>
	<skos:prefLabel xml:lang="fi">lyijykynät</skos:prefLabel>
	<skos:inScheme rdf:resource="http://partage.vocnet.org/Objects"/>
	<skos:broader rdf:resource="http://partage.vocnet.org/part00218"/>
	<skos:exactMatch rdf:resource="http://vocab.getty.edu/aat/300022439"/>
	<skos:editorialNote xml:lang="en">PPRefiningObjectType</skos:editorialNote>
	<skos:scopeNote xml:lang="en">Rods of a marking substance, enclosed in wood, plastic, or metal, and used for writing or drawing.</skos:scopeNote>
</skos:Concept>
<skos:Concept rdf:about="http://partage.vocnet.org/part00833">
	<skos:prefLabel xml:lang="en">pens</skos:prefLabel>
	<skos:altLabel xml:lang="en">pens (drawing and writing)</skos:altLabel>
	<skos:prefLabel xml:lang="hr">olovka.</skos:prefLabel>
	<skos:prefLabel xml:lang="de">Feder</skos:prefLabel>
	<skos:prefLabel xml:lang="sv">pennor</skos:prefLabel>
	<skos:prefLabel xml:lang="pt">caneta</skos:prefLabel>
	<skos:prefLabel xml:lang="fi">kynät</skos:prefLabel>
	<skos:inScheme rdf:resource="http://partage.vocnet.org/Objects"/>
	<skos:broader rdf:resource="http://partage.vocnet.org/part00218"/>
	<skos:exactMatch rdf:resource="http://vocab.getty.edu/aat/300022452"/>
	<skos:editorialNote xml:lang="en">PPRefiningObjectType</skos:editorialNote>
	<skos:scopeNote xml:lang="en">Hand-held instruments for writing or drawing with a colored fluid such as ink. A pen generally comprises a handle or holder and a pointed tip for distributing the fluid on the drawing surface. The term may also refer to an instrument for machine-controlled writing or drawing with ink.</skos:scopeNote>
</skos:Concept>
<skos:Concept rdf:about="http://partage.vocnet.org/part00834">
	<skos:prefLabel xml:lang="en">knives</skos:prefLabel>
	<skos:prefLabel xml:lang="hr">nož</skos:prefLabel>
	<skos:prefLabel xml:lang="de">Messer</skos:prefLabel>
	<skos:prefLabel xml:lang="sv">knivar</skos:prefLabel>
	<skos:prefLabel xml:lang="pt">faca</skos:prefLabel>
	<skos:prefLabel xml:lang="fi">veitset</skos:prefLabel>
	<skos:inScheme rdf:resource="http://partage.vocnet.org/Objects"/>
	<skos:broader rdf:resource="http://partage.vocnet.org/part00218"/>
	<skos:exactMatch rdf:resource="http://vocab.getty.edu/aat/300024668"/>
	<skos:editorialNote xml:lang="en">PPRefiningObjectType</skos:editorialNote>
	<skos:scopeNote xml:lang="en">Cutting instruments consisting of a blade with a sharpened longitudinal edge fixed in a handle, either rigidly as in a table-, carving, or sheath-knife, or with a joint as in a pocket- or clasp-knife. Knives may be used to cut food, especially in serving and eating, as weapons, and for other purposes. The blade may be of steel or another metal or stone, as in the flint knives of early man, or of another material such as ivory or wood (as with a paperknife). The term also refers to tools that are shaped or used as knives, even if the edge is not particularly sharp or actually used for cutting.</skos:scopeNote>
</skos:Concept>
<skos:Concept rdf:about="http://partage.vocnet.org/part00835">
	<skos:prefLabel xml:lang="en">forks</skos:prefLabel>
	<skos:prefLabel xml:lang="sv">gafflar</skos:prefLabel>
	<skos:prefLabel xml:lang="pt">garfos</skos:prefLabel>
	<skos:altLabel xml:lang="de">Gabeln</skos:altLabel>
	<skos:prefLabel xml:lang="de">Gabel</skos:prefLabel>
	<skos:prefLabel xml:lang="hr">vilica</skos:prefLabel>
	<skos:prefLabel xml:lang="fi">haarukat</skos:prefLabel>
	<skos:inScheme rdf:resource="http://partage.vocnet.org/Objects"/>
	<skos:broader rdf:resource="http://partage.vocnet.org/part00219"/>
	<skos:exactMatch rdf:resource="http://vocab.getty.edu/aat/300043099"/>
	<skos:editorialNote xml:lang="en">PPRefiningObjectType</skos:editorialNote>
	<skos:scopeNote xml:lang="en">Articles of flatware having a handle with a shank terminating in two or more tines, used to manipulate food especially in serving and eating.</skos:scopeNote>
</skos:Concept>
<skos:Concept rdf:about="http://partage.vocnet.org/part00836">
	<skos:prefLabel xml:lang="en">intaglio prints</skos:prefLabel>
	<skos:inScheme rdf:resource="http://partage.vocnet.org/Objects"/>
	<skos:broader rdf:resource="http://partage.vocnet.org/part00042"/>
	<skos:narrower rdf:resource="http://partage.vocnet.org/part00818"/>
	<skos:narrower rdf:resource="http://partage.vocnet.org/part00819"/>
	<skos:narrower rdf:resource="http://partage.vocnet.org/part00820"/>
	<skos:narrower rdf:resource="http://partage.vocnet.org/part00822"/>
	<skos:exactMatch rdf:resource="http://vocab.getty.edu/aat/300041338"/>
	<skos:scopeNote xml:lang="en">Prints made using the process of intaglio printing.</skos:scopeNote>
</skos:Concept>
<skos:Concept rdf:about="http://partage.vocnet.org/part00837">
	<skos:prefLabel xml:lang="en">relief prints</skos:prefLabel>
	<skos:inScheme rdf:resource="http://partage.vocnet.org/Objects"/>
	<skos:broader rdf:resource="http://partage.vocnet.org/part00042"/>
	<skos:narrower rdf:resource="http://partage.vocnet.org/part00816"/>
	<skos:narrower rdf:resource="http://partage.vocnet.org/part00817"/>
	<skos:exactMatch rdf:resource="http://vocab.getty.edu/aat/300041391"/>
	<skos:scopeNote xml:lang="en">Prints made using a process of relief printing.</skos:scopeNote>
</skos:Concept>
<skos:Concept rdf:about="http://partage.vocnet.org/part00847">
	<skos:prefLabel xml:lang="en">financial institutions (buildings)</skos:prefLabel>
	<skos:inScheme rdf:resource="http://partage.vocnet.org/Objects"/>
	<skos:broader rdf:resource="http://partage.vocnet.org/part00165"/>
	<skos:narrower rdf:resource="http://partage.vocnet.org/part00740"/>
	<skos:exactMatch rdf:resource="http://vocab.getty.edu/aat/300005213"/>
	<skos:scopeNote xml:lang="en">Buildings that house institutions that provide financial services for clients or members, usually able to both accept deposits and make loans. Examples include banks, credit unions, savings associations, trust companies, and industrial loan and thrift companies. The interior space is typically optimized for a reception area and general office space, varying greatly depending upon the functions of the specific institution.</skos:scopeNote>
</skos:Concept>
<skos:Concept rdf:about="http://partage.vocnet.org/part00851">
	<skos:prefLabel xml:lang="en">main garments</skos:prefLabel>
	<skos:inScheme rdf:resource="http://partage.vocnet.org/Objects"/>
	<skos:broader rdf:resource="http://partage.vocnet.org/part00081"/>
	<skos:narrower rdf:resource="http://partage.vocnet.org/part00695"/>
	<skos:narrower rdf:resource="http://partage.vocnet.org/part00696"/>
	<skos:narrower rdf:resource="http://partage.vocnet.org/part00697"/>
	<skos:narrower rdf:resource="http://partage.vocnet.org/part00698"/>
	<skos:narrower rdf:resource="http://partage.vocnet.org/part00702"/>
	<skos:narrower rdf:resource="http://partage.vocnet.org/part00703"/>
	<skos:narrower rdf:resource="http://partage.vocnet.org/part01120"/>
	<skos:narrower rdf:resource="http://partage.vocnet.org/part01127"/>
	<skos:narrower rdf:resource="http://partage.vocnet.org/part01171"/>
	<skos:exactMatch rdf:resource="http://vocab.getty.edu/aat/300209263"/>
	<skos:scopeNote xml:lang="en">Main layer of dress, usually exclusive of accessories.</skos:scopeNote>
</skos:Concept>
<skos:Concept rdf:about="http://partage.vocnet.org/part00853">
	<skos:prefLabel xml:lang="en">entertainment buildings</skos:prefLabel>
	<skos:inScheme rdf:resource="http://partage.vocnet.org/Objects"/>
	<skos:broader rdf:resource="http://partage.vocnet.org/part00158"/>
	<skos:narrower rdf:resource="http://partage.vocnet.org/part00734"/>
	<skos:exactMatch rdf:resource="http://vocab.getty.edu/aat/300007206"/>
	<skos:scopeNote xml:lang="en">Distinguished from "recreation buildings" by more narrowly designating buildings with devices or equipment for amusement or diversion and not active sports, nor for which membership is required.</skos:scopeNote>
</skos:Concept>
<skos:Concept rdf:about="http://partage.vocnet.org/part00876">
	<skos:prefLabel xml:lang="en">bromoil prints</skos:prefLabel>
	<skos:prefLabel xml:lang="sv">bromoljetryck</skos:prefLabel>
	<skos:prefLabel xml:lang="pt">bromoil</skos:prefLabel>
	<skos:altLabel xml:lang="de">Bromöldrucke</skos:altLabel>
	<skos:prefLabel xml:lang="de">Bromöldruck</skos:prefLabel>
	<skos:prefLabel xml:lang="hr">bromouljni tisak</skos:prefLabel>
	<skos:prefLabel xml:lang="fi">bromivedos</skos:prefLabel>
	<skos:inScheme rdf:resource="http://partage.vocnet.org/Objects"/>
	<skos:broader rdf:resource="http://partage.vocnet.org/part00885"/>
	<skos:exactMatch rdf:resource="http://vocab.getty.edu/aat/300138324"/>
	<skos:editorialNote xml:lang="en">PPRefiningObjectType</skos:editorialNote>
	<skos:scopeNote xml:lang="en">Prints made from the photographic process in which the developed silver in a gelatin print is used as a catalyst to tan the gelatin, and the untanned highlights are used as a resist to a greasy ink. The original plate may be the end product or may be used as a master for transferring the image to another support. Resulting prints resemble etchings or lithographs. Though the process was originally described ca. 1907, prints may be made in this way using modern enlarging papers.</skos:scopeNote>
</skos:Concept>
<skos:Concept rdf:about="http://partage.vocnet.org/part00882">
	<skos:prefLabel xml:lang="en">autochromes</skos:prefLabel>
	<skos:altLabel xml:lang="en">autochromes (photographs)</skos:altLabel>
	<skos:prefLabel xml:lang="pt">autocromos</skos:prefLabel>
	<skos:prefLabel xml:lang="sv">autokromfotografier</skos:prefLabel>
	<skos:altLabel xml:lang="de">Autochrome</skos:altLabel>
	<skos:prefLabel xml:lang="de">Autochrom</skos:prefLabel>
	<skos:prefLabel xml:lang="ca">autokrom</skos:prefLabel>
	<skos:prefLabel xml:lang="fi">autochromet</skos:prefLabel>
	<skos:inScheme rdf:resource="http://partage.vocnet.org/Objects"/>
	<skos:broader rdf:resource="http://partage.vocnet.org/part00918"/>
	<skos:exactMatch rdf:resource="http://vocab.getty.edu/aat/300138292"/>
	<skos:editorialNote xml:lang="en">PPRefiningObjectType</skos:editorialNote>
	<skos:scopeNote xml:lang="en">Photographs made by the Autochrome process..</skos:scopeNote>
</skos:Concept>
<skos:Concept rdf:about="http://partage.vocnet.org/part00883">
	<skos:prefLabel xml:lang="en">albumen prints</skos:prefLabel>
	<skos:prefLabel xml:lang="sv">albuminfotografier</skos:prefLabel>
	<skos:altLabel xml:lang="pt">albumina</skos:altLabel>
	<skos:prefLabel xml:lang="pt">albúmen</skos:prefLabel>
	<skos:altLabel xml:lang="de">Albuminpapierabzüge</skos:altLabel>
	<skos:altLabel xml:lang="de">Albuminpapierabzug</skos:altLabel>
	<skos:altLabel xml:lang="de">Albuminabzüge</skos:altLabel>
	<skos:prefLabel xml:lang="de">Albuminabzug</skos:prefLabel>
	<skos:prefLabel xml:lang="hr">albuminska fotografija</skos:prefLabel>
	<skos:prefLabel xml:lang="fi">albumiinivedos</skos:prefLabel>
	<skos:inScheme rdf:resource="http://partage.vocnet.org/Objects"/>
	<skos:broader rdf:resource="http://partage.vocnet.org/part00917"/>
	<skos:exactMatch rdf:resource="http://vocab.getty.edu/aat/300127121"/>
	<skos:scopeNote xml:lang="en">Photographic prints having albumen as the binder; always black-and-white, though they may be toned to a monochrome hue.</skos:scopeNote>
	<skos:editorialNote xml:lang="en">PPRefiningObjectType</skos:editorialNote>
</skos:Concept>
<skos:Concept rdf:about="http://partage.vocnet.org/part00884">
	<skos:prefLabel xml:lang="en">cradles</skos:prefLabel>
	<skos:altLabel xml:lang="en">cradles (children's beds)</skos:altLabel>
	<skos:prefLabel xml:lang="pt">berço</skos:prefLabel>
	<skos:altLabel xml:lang="de">Wiegen</skos:altLabel>
	<skos:prefLabel xml:lang="de">Wiege</skos:prefLabel>
	<skos:prefLabel xml:lang="sv">vaggor</skos:prefLabel>
	<skos:prefLabel xml:lang="hr">kolijevka</skos:prefLabel>
	<skos:prefLabel xml:lang="fi">kehdot</skos:prefLabel>
	<skos:inScheme rdf:resource="http://partage.vocnet.org/Objects"/>
	<skos:broader rdf:resource="http://partage.vocnet.org/part00314"/>
	<skos:exactMatch rdf:resource="http://vocab.getty.edu/aat/300038847"/>
	<skos:scopeNote xml:lang="en">Small beds for infants, usually on bends.</skos:scopeNote>
	<skos:editorialNote xml:lang="en">PPRefiningObjectType</skos:editorialNote>
</skos:Concept>
<skos:Concept rdf:about="http://partage.vocnet.org/part00885">
	<skos:prefLabel xml:lang="en">oil prints</skos:prefLabel>
	<skos:prefLabel xml:lang="hr">uljni tisak</skos:prefLabel>
	<skos:altLabel xml:lang="de">Öldrucke</skos:altLabel>
	<skos:prefLabel xml:lang="de">Öldruck</skos:prefLabel>
	<skos:prefLabel xml:lang="sv">oljetryck</skos:prefLabel>
	<skos:prefLabel xml:lang="pt">cópia a óleo</skos:prefLabel>
	<skos:prefLabel xml:lang="fi">öljypainokuvat</skos:prefLabel>
	<skos:inScheme rdf:resource="http://partage.vocnet.org/Objects"/>
	<skos:broader rdf:resource="http://partage.vocnet.org/part00921"/>
	<skos:narrower rdf:resource="http://partage.vocnet.org/part00876"/>
	<skos:exactMatch rdf:resource="http://vocab.getty.edu/aat/300138319"/>
	<skos:scopeNote xml:lang="en">Hand-inked photographs produced by a bichromate process developed by G.E.H. Rawlins ca. 1904. A sheet of paper is coated with a thin layer of gelatin and sensitized with bichromate, dried in the dark and exposed under a negative. Exposure hardens the gelatin in the shadow areas and partially in mid-tones. Soaking in water subsequently removes sensitizer and causes the mid-tone and highlight areas to absorb moisture. Oil based inks are repelled in these areas, and remain to a greater or lesser degree in others. The plate is then allowed to dry or is transfer-printed to another sheet, then re-inked for more prints.</skos:scopeNote>
	<skos:editorialNote xml:lang="en">PPRefiningObjectType</skos:editorialNote>
</skos:Concept>
<skos:Concept rdf:about="http://partage.vocnet.org/part00886">
	<skos:prefLabel xml:lang="en">photomontages</skos:prefLabel>
	<skos:prefLabel xml:lang="hr">fotomontaža</skos:prefLabel>
	<skos:altLabel xml:lang="de">Photomontage</skos:altLabel>
	<skos:prefLabel xml:lang="de">Fotomontage</skos:prefLabel>
	<skos:prefLabel xml:lang="sv">photomontage</skos:prefLabel>
	<skos:prefLabel xml:lang="pt">fotomontagem</skos:prefLabel>
	<skos:prefLabel xml:lang="fi">valokuvamontaasi</skos:prefLabel>
	<skos:inScheme rdf:resource="http://partage.vocnet.org/Objects"/>
	<skos:broader rdf:resource="http://partage.vocnet.org/part00919"/>
	<skos:exactMatch rdf:resource="http://vocab.getty.edu/aat/300134699"/>
	<skos:editorialNote xml:lang="en">PPRefiningObjectType</skos:editorialNote>
	<skos:scopeNote xml:lang="en">Refers to combinations of photographic images, or photographic with other images, such as architectural drawings, usually arranged into a somewhat unified image. For photographs produced by printing two or more negatives as one unified image, use "composite photographs." When pieces of photographs or other relatively flat materials are pasted together into less unified images, use "collages."</skos:scopeNote>
</skos:Concept>
<skos:Concept rdf:about="http://partage.vocnet.org/part00887">
	<skos:prefLabel xml:lang="en">platinum prints</skos:prefLabel>
	<skos:prefLabel xml:lang="hr">platinotipija</skos:prefLabel>
	<skos:altLabel xml:lang="de">Platinotypie</skos:altLabel>
	<skos:prefLabel xml:lang="de">Platindruck</skos:prefLabel>
	<skos:prefLabel xml:lang="sv">platinumtryck</skos:prefLabel>
	<skos:prefLabel xml:lang="pt">impressão em platina</skos:prefLabel>
	<skos:prefLabel xml:lang="fi">platinavedokset</skos:prefLabel>
	<skos:inScheme rdf:resource="http://partage.vocnet.org/Objects"/>
	<skos:broader rdf:resource="http://partage.vocnet.org/part00917"/>
	<skos:exactMatch rdf:resource="http://vocab.getty.edu/aat/300127145"/>
	<skos:editorialNote xml:lang="en">PPRefiningObjectType</skos:editorialNote>
	<skos:scopeNote xml:lang="en">Photographic prints made by the platinum process.</skos:scopeNote>
</skos:Concept>
<skos:Concept rdf:about="http://partage.vocnet.org/part00888">
	<skos:prefLabel xml:lang="en">gelatin silver prints</skos:prefLabel>
	<skos:prefLabel xml:lang="sv">gelatinsilverfotografi</skos:prefLabel>
	<skos:prefLabel xml:lang="pt">impressão em gelatina de prata</skos:prefLabel>
	<skos:prefLabel xml:lang="de">Silbergelatineabzug</skos:prefLabel>
	<skos:prefLabel xml:lang="hr">želatinasti srebrni print</skos:prefLabel>
	<skos:prefLabel xml:lang="fi">hopeagelatiinivedokset</skos:prefLabel>
	<skos:inScheme rdf:resource="http://partage.vocnet.org/Objects"/>
	<skos:broader rdf:resource="http://partage.vocnet.org/part00917"/>
	<skos:exactMatch rdf:resource="http://vocab.getty.edu/aat/300128695"/>
	<skos:editorialNote xml:lang="en">PPRefiningObjectType</skos:editorialNote>
	<skos:scopeNote xml:lang="en">Refers to photographic prints having gelatin as the binder, holding silver as the final image material; always black-and-white, though they may be toned to a monochrome hue</skos:scopeNote>
</skos:Concept>
<skos:Concept rdf:about="http://partage.vocnet.org/part00890">
	<skos:prefLabel xml:lang="en">stereoscopic photographs</skos:prefLabel>
	<skos:prefLabel xml:lang="sv">stereoskopiska fotografier</skos:prefLabel>
	<skos:prefLabel xml:lang="hr">stereoskopska fotografija</skos:prefLabel>
	<skos:prefLabel xml:lang="pt">fotografia estereostópica</skos:prefLabel>
	<skos:altLabel xml:lang="de">Stereofotografie</skos:altLabel>
	<skos:prefLabel xml:lang="de">Stereophotographie</skos:prefLabel>
	<skos:prefLabel xml:lang="fi">stereokuvat</skos:prefLabel>
	<skos:inScheme rdf:resource="http://partage.vocnet.org/Objects"/>
	<skos:broader rdf:resource="http://partage.vocnet.org/part00419"/>
	<skos:exactMatch rdf:resource="http://vocab.getty.edu/aat/300162872"/>
	<skos:editorialNote xml:lang="en">PPRefiningObjectType</skos:editorialNote>
	<skos:scopeNote xml:lang="en">Refers to double pictures of the same scene that produce the effect of three dimensionality when viewed through a stereoscope. They were first envisioned in 1832 by the English physicist Charles Wheatstone, who described this as a uniquely photographic art form, since a draftsman could not draw two scenes in exact perspective from viewpoints separated only 2 1\/2 inches, which is the normal distance between human eyes necessary for the three-dimensional effect. Wheatstone's mirror stereoscope was not practical for use with photographs, and the invention was not popular until the 1850s, when Sir David Brewster, a Scottish scientist, designed a simpler viewing instrument. The introduction of the collodion process, which simplified exposure and printing techniques, allowed three-dimensional photographs to become a popular craze. They may be daguerreotypes, negatives, or other forms of photographs. For images in the form of photographic prints on cards, use the more specific term "stereographs."</skos:scopeNote>
</skos:Concept>
<skos:Concept rdf:about="http://partage.vocnet.org/part00891">
	<skos:prefLabel xml:lang="en">gum bichromate prints</skos:prefLabel>
	<skos:prefLabel xml:lang="sv">gummitryck</skos:prefLabel>
	<skos:prefLabel xml:lang="pt">impressão em goma bicromada</skos:prefLabel>
	<skos:altLabel xml:lang="de">Gummibichromatabzug</skos:altLabel>
	<skos:prefLabel xml:lang="de">Gummidruck</skos:prefLabel>
	<skos:prefLabel xml:lang="hr">gumnobikromatni tisak</skos:prefLabel>
	<skos:prefLabel xml:lang="fi">kumibikromaattivedokset</skos:prefLabel>
	<skos:inScheme rdf:resource="http://partage.vocnet.org/Objects"/>
	<skos:broader rdf:resource="http://partage.vocnet.org/part00921"/>
	<skos:exactMatch rdf:resource="http://vocab.getty.edu/aat/300134949"/>
	<skos:editorialNote xml:lang="en">PPRefiningObjectType</skos:editorialNote>
	<skos:scopeNote xml:lang="en">Photographic prints made by the gum bichromate process.</skos:scopeNote>
</skos:Concept>
<skos:Concept rdf:about="http://partage.vocnet.org/part00892">
	<skos:prefLabel xml:lang="en">monotypes</skos:prefLabel>
	<skos:altLabel xml:lang="en">monotypes (planographic prints)</skos:altLabel>
	<skos:prefLabel xml:lang="hr">monotipija</skos:prefLabel>
	<skos:altLabel xml:lang="de">Monotypien</skos:altLabel>
	<skos:prefLabel xml:lang="de">Monotypie</skos:prefLabel>
	<skos:prefLabel xml:lang="sv">monotypemaskiner</skos:prefLabel>
	<skos:prefLabel xml:lang="pt">monótipo</skos:prefLabel>
	<skos:prefLabel xml:lang="fi">monotypia</skos:prefLabel>
	<skos:inScheme rdf:resource="http://partage.vocnet.org/Objects"/>
	<skos:broader rdf:resource="http://partage.vocnet.org/part00525"/>
	<skos:exactMatch rdf:resource="http://vocab.getty.edu/aat/300041538"/>
	<skos:editorialNote xml:lang="en">PPRefiningObjectType</skos:editorialNote>
	<skos:scopeNote xml:lang="en">Unique prints made using the process of monotype</skos:scopeNote>
</skos:Concept>
<skos:Concept rdf:about="http://partage.vocnet.org/part00893">
	<skos:prefLabel xml:lang="en">chromotypes (carbon prints)</skos:prefLabel>
	<skos:prefLabel xml:lang="sv">kromotypier</skos:prefLabel>
	<skos:prefLabel xml:lang="pt">cromotipo</skos:prefLabel>
	<skos:altLabel xml:lang="de">Chromotypien</skos:altLabel>
	<skos:prefLabel xml:lang="de">Chromotypie</skos:prefLabel>
	<skos:prefLabel xml:lang="hr">ugljeni tisak</skos:prefLabel>
	<skos:prefLabel xml:lang="fi">kromotyypit</skos:prefLabel>
	<skos:inScheme rdf:resource="http://partage.vocnet.org/Objects"/>
	<skos:broader rdf:resource="http://partage.vocnet.org/part00824"/>
	<skos:exactMatch rdf:resource="http://vocab.getty.edu/aat/300265180"/>
	<skos:editorialNote xml:lang="en">PPRefiningObjectType</skos:editorialNote>
	<skos:scopeNote xml:lang="en">Carbon print developed on collodionised glass, and stripped when dry. The name was given by Claude L\u00e9on and T. S. Lambert, and was in use in the United States from 1876-1880s.</skos:scopeNote>
</skos:Concept>
<skos:Concept rdf:about="http://partage.vocnet.org/part00894">
	<skos:prefLabel xml:lang="en">collodion prints</skos:prefLabel>
	<skos:altLabel xml:lang="de">Kollodiumabzüge</skos:altLabel>
	<skos:prefLabel xml:lang="de">Kollodiumabzug</skos:prefLabel>
	<skos:prefLabel xml:lang="pt">impressões colódio</skos:prefLabel>
	<skos:prefLabel xml:lang="sv">kollodiumtryck</skos:prefLabel>
	<skos:prefLabel xml:lang="hr">kolodijski postupak</skos:prefLabel>
	<skos:prefLabel xml:lang="fi">kollodiumvedokset</skos:prefLabel>
	<skos:inScheme rdf:resource="http://partage.vocnet.org/Objects"/>
	<skos:broader rdf:resource="http://partage.vocnet.org/part00917"/>
	<skos:exactMatch rdf:resource="http://vocab.getty.edu/aat/300134696"/>
	<skos:editorialNote xml:lang="en">PPRefiningObjectType</skos:editorialNote>
	<skos:scopeNote xml:lang="en">Photographic prints having collodion as the binder.</skos:scopeNote>
</skos:Concept>
<skos:Concept rdf:about="http://partage.vocnet.org/part00895">
	<skos:prefLabel xml:lang="en">collotypes</skos:prefLabel>
	<skos:altLabel xml:lang="de">Fototypie</skos:altLabel>
	<skos:prefLabel xml:lang="de">Lichtdruck</skos:prefLabel>
	<skos:altLabel xml:lang="de">Kollotypie</skos:altLabel>
	<skos:prefLabel xml:lang="pt">calótipo</skos:prefLabel>
	<skos:prefLabel xml:lang="sv">kollotypier</skos:prefLabel>
	<skos:altLabel xml:lang="de">Fototypien</skos:altLabel>
	<skos:altLabel xml:lang="de">Lichtdrucke</skos:altLabel>
	<skos:altLabel xml:lang="de">Kollotypien</skos:altLabel>
	<skos:altLabel xml:lang="hr">kolotipija</skos:altLabel>
	<skos:prefLabel xml:lang="hr">svjetlotisak</skos:prefLabel>
	<skos:prefLabel xml:lang="fi">kollotyypit</skos:prefLabel>
	<skos:inScheme rdf:resource="http://partage.vocnet.org/Objects"/>
	<skos:broader rdf:resource="http://partage.vocnet.org/part00943"/>
	<skos:exactMatch rdf:resource="http://vocab.getty.edu/aat/300154355"/>
	<skos:editorialNote xml:lang="en">PPRefiningObjectType</skos:editorialNote>
	<skos:scopeNote xml:lang="en">Photomechanical prints produced by photolithography in which the printing plate is prepared using a bichromate process, gelatin, and greasy ink, which is held in the characteristic wormlike patterns of cracks.</skos:scopeNote>
</skos:Concept>
<skos:Concept rdf:about="http://partage.vocnet.org/part00896">
	<skos:prefLabel xml:lang="en">cyanotypes</skos:prefLabel>
	<skos:altLabel xml:lang="en">cyanotypes (photographic prints)</skos:altLabel>
	<skos:prefLabel xml:lang="pt">cianótipos</skos:prefLabel>
	<skos:altLabel xml:lang="de">Cyanotypien</skos:altLabel>
	<skos:prefLabel xml:lang="de">Cyanotypie</skos:prefLabel>
	<skos:prefLabel xml:lang="sv">cyanotypi</skos:prefLabel>
	<skos:prefLabel xml:lang="hr">cijanotipija</skos:prefLabel>
	<skos:prefLabel xml:lang="fi">sinikopio</skos:prefLabel>
	<skos:inScheme rdf:resource="http://partage.vocnet.org/Objects"/>
	<skos:broader rdf:resource="http://partage.vocnet.org/part00917"/>
	<skos:exactMatch rdf:resource="http://vocab.getty.edu/aat/300134811"/>
	<skos:editorialNote xml:lang="en">PPRefiningObjectType</skos:editorialNote>
	<skos:scopeNote xml:lang="en">Blue-toned photographic prints produced by the blueprint process, not including reproductive prints of architectural or other technical drawings; for these, use "blueprints" or "blueline prints.</skos:scopeNote>
</skos:Concept>
<skos:Concept rdf:about="http://partage.vocnet.org/part00904">
	<skos:prefLabel xml:lang="en">linoleum</skos:prefLabel>
	<skos:prefLabel xml:lang="hr">linoleum</skos:prefLabel>
	<skos:prefLabel xml:lang="de">Linoleum</skos:prefLabel>
	<skos:prefLabel xml:lang="sv">linoleum</skos:prefLabel>
	<skos:prefLabel xml:lang="pt">linóleo</skos:prefLabel>
	<skos:prefLabel xml:lang="fi">linoleum</skos:prefLabel>
	<skos:inScheme rdf:resource="http://partage.vocnet.org/Objects"/>
	<skos:broader rdf:resource="http://partage.vocnet.org/part00180"/>
	<skos:exactMatch rdf:resource="http://vocab.getty.edu/aat/300069563"/>
	<skos:editorialNote xml:lang="en">PPRefiningObjectType</skos:editorialNote>
	<skos:scopeNote xml:lang="en">Durable floor coverings made primarily of linseed oil, with a filler of cork dust or wood flour, and flax, with pigments added to create the desired colors and patterns; also, similar floor coverings made with substitutes for the linseed oil or filler or both.</skos:scopeNote>
</skos:Concept>
<skos:Concept rdf:about="http://partage.vocnet.org/part00914">
	<skos:prefLabel xml:lang="en">negatives (photographic)</skos:prefLabel>
	<skos:prefLabel xml:lang="hr">negativ</skos:prefLabel>
	<skos:altLabel xml:lang="de">Negative</skos:altLabel>
	<skos:prefLabel xml:lang="de">Negativ</skos:prefLabel>
	<skos:prefLabel xml:lang="ru">negativ (fotografiska)</skos:prefLabel>
	<skos:prefLabel xml:lang="pt">negativo</skos:prefLabel>
	<skos:prefLabel xml:lang="fi">negatiivit</skos:prefLabel>
	<skos:inScheme rdf:resource="http://partage.vocnet.org/Objects"/>
	<skos:broader rdf:resource="http://partage.vocnet.org/part00419"/>
	<skos:exactMatch rdf:resource="http://vocab.getty.edu/aat/300127173"/>
	<skos:editorialNote xml:lang="en">PPRefiningObjectType</skos:editorialNote>
	<skos:scopeNote xml:lang="en">Photographs, usually on a transparent support, in which the tones or colors are reversed from their appearance in nature. For prints in which tones or colors are reversed, see "negative prints." When a glass plate is painted or drawn on and a photographic print made from it, see "clich\u00e9s-verre."</skos:scopeNote>
</skos:Concept>
<skos:Concept rdf:about="http://partage.vocnet.org/part00917">
	<skos:prefLabel xml:lang="en">photographic prints</skos:prefLabel>
	<skos:inScheme rdf:resource="http://partage.vocnet.org/Objects"/>
	<skos:broader rdf:resource="http://partage.vocnet.org/part00918"/>
	<skos:narrower rdf:resource="http://partage.vocnet.org/part00883"/>
	<skos:narrower rdf:resource="http://partage.vocnet.org/part00887"/>
	<skos:narrower rdf:resource="http://partage.vocnet.org/part00888"/>
	<skos:narrower rdf:resource="http://partage.vocnet.org/part00894"/>
	<skos:narrower rdf:resource="http://partage.vocnet.org/part00896"/>
	<skos:narrower rdf:resource="http://partage.vocnet.org/part00921"/>
	<skos:exactMatch rdf:resource="http://vocab.getty.edu/aat/300127104"/>
	<skos:scopeNote xml:lang="en">Opaque photographs, usually positive (i.e., reproducing appearances without tonal reversal, otherwise use "negative prints"), usually on paper, and generally, but not always, printed from a negative.</skos:scopeNote>
</skos:Concept>
<skos:Concept rdf:about="http://partage.vocnet.org/part00918">
	<skos:prefLabel xml:lang="en">positives (photographs)</skos:prefLabel>
	<skos:inScheme rdf:resource="http://partage.vocnet.org/Objects"/>
	<skos:broader rdf:resource="http://partage.vocnet.org/part00419"/>
	<skos:narrower rdf:resource="http://partage.vocnet.org/part00882"/>
	<skos:narrower rdf:resource="http://partage.vocnet.org/part00917"/>
	<skos:narrower rdf:resource="http://partage.vocnet.org/part01238"/>
	<skos:exactMatch rdf:resource="http://vocab.getty.edu/aat/300138191"/>
	<skos:scopeNote xml:lang="en">Photographs in which the tones or colors correspond to (that is, are not reversed from) their appearance in nature.</skos:scopeNote>
</skos:Concept>
<skos:Concept rdf:about="http://partage.vocnet.org/part00919">
	<skos:altLabel xml:lang="en">montages (visual works)</skos:altLabel>
	<skos:prefLabel xml:lang="en">montages</skos:prefLabel>
	<skos:inScheme rdf:resource="http://partage.vocnet.org/Objects"/>
	<skos:narrower rdf:resource="http://partage.vocnet.org/part00886"/>
	<skos:exactMatch rdf:resource="http://vocab.getty.edu/aat/300127008"/>
	<skos:scopeNote xml:lang="en">Works produced by the technique of montage. If photographs dominate the composition, use "photomontages.</skos:scopeNote>
</skos:Concept>
<skos:Concept rdf:about="http://partage.vocnet.org/part00921">
	<skos:prefLabel xml:lang="en">pigment prints</skos:prefLabel>
	<skos:inScheme rdf:resource="http://partage.vocnet.org/Objects"/>
	<skos:broader rdf:resource="http://partage.vocnet.org/part00917"/>
	<skos:narrower rdf:resource="http://partage.vocnet.org/part00824"/>
	<skos:narrower rdf:resource="http://partage.vocnet.org/part00885"/>
	<skos:narrower rdf:resource="http://partage.vocnet.org/part00891"/>
	<skos:exactMatch rdf:resource="http://vocab.getty.edu/aat/300128234"/>
	<skos:scopeNote xml:lang="en">Use as a broad term for photographic prints made by any of the pigment processes.</skos:scopeNote>
</skos:Concept>
<skos:Concept rdf:about="http://partage.vocnet.org/part00923">
	<skos:prefLabel xml:lang="en">openings (architectural elements)</skos:prefLabel>
	<skos:inScheme rdf:resource="http://partage.vocnet.org/Objects"/>
	<skos:broader rdf:resource="http://partage.vocnet.org/part00127"/>
	<skos:narrower rdf:resource="http://partage.vocnet.org/part00748"/>
	<skos:narrower rdf:resource="http://partage.vocnet.org/part00749"/>
	<skos:narrower rdf:resource="http://partage.vocnet.org/part00751"/>
	<skos:exactMatch rdf:resource="http://vocab.getty.edu/aat/300114196"/>
	<skos:scopeNote xml:lang="en">Generally denotes apertures or breaks in the surface of a wall or other architectural element.</skos:scopeNote>
</skos:Concept>
<skos:Concept rdf:about="http://partage.vocnet.org/part00928">
	<skos:prefLabel xml:lang="en">stands (support furniture)</skos:prefLabel>
	<skos:prefLabel xml:lang="de">Ständer (Mobiliar)</skos:prefLabel>
	<skos:prefLabel xml:lang="hr">stalak</skos:prefLabel>
	<skos:inScheme rdf:resource="http://partage.vocnet.org/Objects"/>
	<skos:broader rdf:resource="http://partage.vocnet.org/part00099"/>
	<skos:narrower rdf:resource="http://partage.vocnet.org/part00796"/>
	<skos:narrower rdf:resource="http://partage.vocnet.org/part01163"/>
	<skos:narrower rdf:resource="http://partage.vocnet.org/part01179"/>
	<skos:narrower rdf:resource="http://partage.vocnet.org/part01187"/>
	<skos:exactMatch rdf:resource="http://vocab.getty.edu/aat/300039767"/>
	<skos:scopeNote xml:lang="en">Small often tablelike pieces of furniture used for holding or displaying objects.</skos:scopeNote>
	<skos:scopeNote xml:lang="en">PPRefiningObjectType</skos:scopeNote>
</skos:Concept>
<skos:Concept rdf:about="http://partage.vocnet.org/part00939">
	<skos:prefLabel xml:lang="en">planters</skos:prefLabel>
	<skos:altLabel xml:lang="en">planters (containers)</skos:altLabel>
	<skos:inScheme rdf:resource="http://partage.vocnet.org/Objects"/>
	<skos:broader rdf:resource="http://partage.vocnet.org/part00085"/>
	<skos:narrower rdf:resource="http://partage.vocnet.org/part00797"/>
	<skos:exactMatch rdf:resource="http://vocab.getty.edu/aat/300237566"/>
	<skos:scopeNote xml:lang="en">Any of various containers in which plants are grown or placed for decorative purposes.</skos:scopeNote>
</skos:Concept>
<skos:Concept rdf:about="http://partage.vocnet.org/part00943">
	<skos:prefLabel xml:lang="en">photolithographs</skos:prefLabel>
	<skos:inScheme rdf:resource="http://partage.vocnet.org/Objects"/>
	<skos:broader rdf:resource="http://partage.vocnet.org/part00944"/>
	<skos:narrower rdf:resource="http://partage.vocnet.org/part00895"/>
	<skos:exactMatch rdf:resource="http://vocab.getty.edu/aat/300154386"/>
	<skos:scopeNote xml:lang="en">Photomechanical prints produced by photolithography.</skos:scopeNote>
</skos:Concept>
<skos:Concept rdf:about="http://partage.vocnet.org/part00944">
	<skos:prefLabel xml:lang="en">photomechanical prints</skos:prefLabel>
	<skos:inScheme rdf:resource="http://partage.vocnet.org/Objects"/>
	<skos:narrower rdf:resource="http://partage.vocnet.org/part00943"/>
	<skos:narrower rdf:resource="http://partage.vocnet.org/part01259"/>
	<skos:exactMatch rdf:resource="http://vocab.getty.edu/aat/300041424"/>
	<skos:scopeNote xml:lang="en">Images produced by processes that involve a photographic process (that is, employing light-sensitivity) to transfer an image, and then a separate process to produce the print, which was never itself light-sensitive.</skos:scopeNote>
</skos:Concept>
<skos:Concept rdf:about="http://partage.vocnet.org/part00948">
	<skos:prefLabel xml:lang="en">working drawings</skos:prefLabel>
	<skos:inScheme rdf:resource="http://partage.vocnet.org/Objects"/>
	<skos:broader rdf:resource="http://partage.vocnet.org/part00047"/>
	<skos:narrower rdf:resource="http://partage.vocnet.org/part00821"/>
	<skos:exactMatch rdf:resource="http://vocab.getty.edu/aat/300034471"/>
	<skos:scopeNote xml:lang="en">Final drawings from which a structure, object, or work of art is made. For drawings done in developing a work, use "sketches," "studies (visual works)," "preliminary drawings," "preparatory drawings," or "design drawings."</skos:scopeNote>
</skos:Concept>
<skos:Concept rdf:about="http://partage.vocnet.org/part00955">
	<skos:prefLabel xml:lang="en">neckwear</skos:prefLabel>
	<skos:inScheme rdf:resource="http://partage.vocnet.org/Objects"/>
	<skos:broader rdf:resource="http://partage.vocnet.org/part00080"/>
	<skos:narrower rdf:resource="http://partage.vocnet.org/part00780"/>
	<skos:narrower rdf:resource="http://partage.vocnet.org/part01124"/>
	<skos:scopeNote xml:lang="en">Articles of costume worn about the neck.</skos:scopeNote>
</skos:Concept>
<skos:Concept rdf:about="http://partage.vocnet.org/part00958">
	<skos:prefLabel xml:lang="en">ear ornaments</skos:prefLabel>
	<skos:inScheme rdf:resource="http://partage.vocnet.org/Objects"/>
	<skos:broader rdf:resource="http://partage.vocnet.org/part00078"/>
	<skos:narrower rdf:resource="http://partage.vocnet.org/part00777"/>
	<skos:exactMatch rdf:resource="http://vocab.getty.edu/aat/300211279"/>
	<skos:scopeNote xml:lang="en">Decorative items worn in, on, or about the ear.</skos:scopeNote>
</skos:Concept>
<skos:Concept rdf:about="http://partage.vocnet.org/part00965">
	<skos:prefLabel xml:lang="en">headgear</skos:prefLabel>
	<skos:inScheme rdf:resource="http://partage.vocnet.org/Objects"/>
	<skos:broader rdf:resource="http://partage.vocnet.org/part00080"/>
	<skos:narrower rdf:resource="http://partage.vocnet.org/part00717"/>
	<skos:narrower rdf:resource="http://partage.vocnet.org/part00718"/>
	<skos:exactMatch rdf:resource="http://vocab.getty.edu/aat/300209285"/>
	<skos:scopeNote xml:lang="en">Any covering for the head.</skos:scopeNote>
</skos:Concept>
<skos:Concept rdf:about="http://partage.vocnet.org/part00974">
	<skos:prefLabel xml:lang="en">hosiery</skos:prefLabel>
	<skos:inScheme rdf:resource="http://partage.vocnet.org/Objects"/>
	<skos:broader rdf:resource="http://partage.vocnet.org/part00080"/>
	<skos:narrower rdf:resource="http://partage.vocnet.org/part00723"/>
	<skos:exactMatch rdf:resource="http://vocab.getty.edu/aat/300209984"/>
	<skos:scopeNote xml:lang="en">Leg coverings, sometimes woven in one with panties, that extend to the ankle and usually cover the foot; generally knitted or woven, sheer or opaque, and of lightweight or heavy fabric. Distinguish from "footwear", which is primarily worn as coverings for the feet.</skos:scopeNote>
	<skos:editorialNote xml:lang="en">PPRefiningObjectType</skos:editorialNote>
</skos:Concept>
<skos:Concept rdf:about="http://partage.vocnet.org/part00983">
	<skos:prefLabel xml:lang="en">eyeglasses</skos:prefLabel>
	<skos:inScheme rdf:resource="http://partage.vocnet.org/Objects"/>
	<skos:broader rdf:resource="http://partage.vocnet.org/part00218"/>
	<skos:narrower rdf:resource="http://partage.vocnet.org/part00787"/>
	<skos:exactMatch rdf:resource="http://vocab.getty.edu/aat/300266808"/>
	<skos:scopeNote xml:lang="en">Devices to compensate for defective vision or to protect the eyes from light, dust, and the like, consisting usually of two lenses set in a frame that includes a nosepiece for resting on the bridge of the nose and which may also have two sidepieces extending over or around the ears.</skos:scopeNote>
</skos:Concept>
<skos:Concept rdf:about="http://partage.vocnet.org/part00986">
	<skos:prefLabel xml:lang="en">garden structures</skos:prefLabel>
	<skos:inScheme rdf:resource="http://partage.vocnet.org/Objects"/>
	<skos:narrower rdf:resource="http://partage.vocnet.org/part00744"/>
	<skos:exactMatch rdf:resource="http://vocab.getty.edu/aat/300006822"/>
	<skos:scopeNote xml:lang="en">Structures usually associated with or located in gardens or similarly landscaped grounds.</skos:scopeNote>
</skos:Concept>
<skos:Concept rdf:about="http://partage.vocnet.org/part00994">
	<skos:prefLabel xml:lang="en">closures (container components)</skos:prefLabel>
	<skos:inScheme rdf:resource="http://partage.vocnet.org/Objects"/>
	<skos:broader rdf:resource="http://partage.vocnet.org/part00116"/>
	<skos:narrower rdf:resource="http://partage.vocnet.org/part01012"/>
	<skos:exactMatch rdf:resource="http://vocab.getty.edu/aat/300203437"/>
	<skos:scopeNote xml:lang="en">Object components which are used to cover or close a mouth or other openings on containers.</skos:scopeNote>
</skos:Concept>
<skos:Concept rdf:about="http://partage.vocnet.org/part01006">
	<skos:prefLabel xml:lang="en">water distribution structures</skos:prefLabel>
	<skos:inScheme rdf:resource="http://partage.vocnet.org/Objects"/>
	<skos:broader rdf:resource="http://partage.vocnet.org/part01009"/>
	<skos:narrower rdf:resource="http://partage.vocnet.org/part00750"/>
	<skos:narrower rdf:resource="http://partage.vocnet.org/part01064"/>
	<skos:exactMatch rdf:resource="http://vocab.getty.edu/aat/300006164"/>
	<skos:scopeNote xml:lang="en">Irrigation canals, pipes, pumps, and other structures and equipment for distributing water.</skos:scopeNote>
</skos:Concept>
<skos:Concept rdf:about="http://partage.vocnet.org/part01009">
	<skos:prefLabel xml:lang="en">hydraulic structures</skos:prefLabel>
	<skos:inScheme rdf:resource="http://partage.vocnet.org/Objects"/>
	<skos:narrower rdf:resource="http://partage.vocnet.org/part01006"/>
	<skos:exactMatch rdf:resource="http://vocab.getty.edu/aat/300006073"/>
	<skos:scopeNote xml:lang="en">Facilities designed to convey or control the flow of water, including channels, bridges, dams, and other such constructions.</skos:scopeNote>
</skos:Concept>
<skos:Concept rdf:about="http://partage.vocnet.org/part01012">
	<skos:prefLabel xml:lang="en">covers (closures)</skos:prefLabel>
	<skos:altLabel xml:lang="de">Hüllen</skos:altLabel>
	<skos:altLabel xml:lang="de">Hülle</skos:altLabel>
	<skos:altLabel xml:lang="de">Abdeckungen</skos:altLabel>
	<skos:prefLabel xml:lang="de">Abdeckung</skos:prefLabel>
	<skos:inScheme rdf:resource="http://partage.vocnet.org/Objects"/>
	<skos:broader rdf:resource="http://partage.vocnet.org/part00994"/>
	<skos:narrower rdf:resource="http://partage.vocnet.org/part00694"/>
	<skos:exactMatch rdf:resource="http://vocab.getty.edu/aat/300197210"/>
	<skos:scopeNote xml:lang="en">Objects that are placed or that naturally overlie or overspread another object, with the purpose or effect of enclosing, hiding, or sheltering the second object or its contents.</skos:scopeNote>
</skos:Concept>
<skos:Concept rdf:about="http://partage.vocnet.org/part01028">
	<skos:prefLabel xml:lang="en">crayons</skos:prefLabel>
	<skos:altLabel xml:lang="en">crayons (drawing material)</skos:altLabel>
	<skos:inScheme rdf:resource="http://partage.vocnet.org/Objects"/>
	<skos:broader rdf:resource="http://partage.vocnet.org/part00218"/>
	<skos:exactMatch rdf:resource="http://vocab.getty.edu/aat/300022415"/>
	<skos:scopeNote xml:lang="en">A generic term for any drawing material made in stick form.</skos:scopeNote>
</skos:Concept>
<skos:Concept rdf:about="http://partage.vocnet.org/part01034">
	<skos:prefLabel xml:lang="en">welfare buildings</skos:prefLabel>
	<skos:inScheme rdf:resource="http://partage.vocnet.org/Objects"/>
	<skos:narrower rdf:resource="http://partage.vocnet.org/part00730"/>
	<skos:exactMatch rdf:resource="http://vocab.getty.edu/aat/300006742"/>
	<skos:scopeNote xml:lang="en">Buildings containing facilities for record keeping or distribution of care, advice, or publications having to do with the general health and welfare of humans or animals.</skos:scopeNote>
</skos:Concept>
<skos:Concept rdf:about="http://partage.vocnet.org/part01041">
	<skos:prefLabel xml:lang="en">passenger vehicles</skos:prefLabel>
	<skos:inScheme rdf:resource="http://partage.vocnet.org/Objects"/>
	<skos:broader rdf:resource="http://partage.vocnet.org/part01045"/>
	<skos:narrower rdf:resource="http://partage.vocnet.org/part00788"/>
	<skos:exactMatch rdf:resource="http://vocab.getty.edu/aat/300227816"/>
	<skos:scopeNote xml:lang="en">Land vehicles whose primary purpose is to convey travelers.</skos:scopeNote>
</skos:Concept>
<skos:Concept rdf:about="http://partage.vocnet.org/part01045">
	<skos:prefLabel xml:lang="en">land vehicles</skos:prefLabel>
	<skos:inScheme rdf:resource="http://partage.vocnet.org/Objects"/>
	<skos:broader rdf:resource="http://partage.vocnet.org/part01046"/>
	<skos:narrower rdf:resource="http://partage.vocnet.org/part01041"/>
	<skos:exactMatch rdf:resource="http://vocab.getty.edu/aat/300212968"/>
	<skos:scopeNote xml:lang="en">Vehicles for use over land.</skos:scopeNote>
</skos:Concept>
<skos:Concept rdf:about="http://partage.vocnet.org/part01046">
	<skos:prefLabel xml:lang="en">vehicles (transportation)</skos:prefLabel>
	<skos:inScheme rdf:resource="http://partage.vocnet.org/Objects"/>
	<skos:narrower rdf:resource="http://partage.vocnet.org/part01045"/>
	<skos:exactMatch rdf:resource="http://vocab.getty.edu/aat/300219258"/>
	<skos:scopeNote xml:lang="en">Use broadly for devices or contrivances by which people or objects are conveyed or carried.</skos:scopeNote>
</skos:Concept>
<skos:Concept rdf:about="http://partage.vocnet.org/part01052">
	<skos:prefLabel xml:lang="en">walkways</skos:prefLabel>
	<skos:inScheme rdf:resource="http://partage.vocnet.org/Objects"/>
	<skos:broader rdf:resource="http://partage.vocnet.org/part00728"/>
	<skos:narrower rdf:resource="http://partage.vocnet.org/part00727"/>
	<skos:exactMatch rdf:resource="http://vocab.getty.edu/aat/300008312"/>
	<skos:scopeNote xml:lang="en">Outdoor pedestrian pathways, and similar bicycle or horseback riding paths, paved or unpaved, developed as a regular means of access from one point to another within a landscape. For indoor means of access see descriptors collocated under "circulation spaces."</skos:scopeNote>
</skos:Concept>
<skos:Concept rdf:about="http://partage.vocnet.org/part01057">
	<skos:prefLabel xml:lang="en">extended care facilities</skos:prefLabel>
	<skos:inScheme rdf:resource="http://partage.vocnet.org/Objects"/>
	<skos:broader rdf:resource="http://partage.vocnet.org/part00160"/>
	<skos:narrower rdf:resource="http://partage.vocnet.org/part00743"/>
	<skos:exactMatch rdf:resource="http://vocab.getty.edu/aat/300006707"/>
	<skos:scopeNote xml:lang="en">Health facilities specializing in the treatment of and rehabilitation from illnesses and injuries that require prolonged care over an extended period of time.</skos:scopeNote>
</skos:Concept>
<skos:Concept rdf:about="http://partage.vocnet.org/part01064">
	<skos:prefLabel xml:lang="en">reservoirs (water distribution structures)</skos:prefLabel>
	<skos:inScheme rdf:resource="http://partage.vocnet.org/Objects"/>
	<skos:broader rdf:resource="http://partage.vocnet.org/part01006"/>
	<skos:narrower rdf:resource="http://partage.vocnet.org/part00754"/>
	<skos:exactMatch rdf:resource="http://vocab.getty.edu/aat/300006191"/>
</skos:Concept>
<skos:Concept rdf:about="http://partage.vocnet.org/part01066">
	<skos:altLabel xml:lang="de">Kacheln</skos:altLabel>
	<skos:prefLabel xml:lang="de">Fliesen</skos:prefLabel>
	<skos:prefLabel xml:lang="en">tiles</skos:prefLabel>
	<skos:altLabel xml:lang="en">tiles (object genre)</skos:altLabel>
	<skos:inScheme rdf:resource="http://partage.vocnet.org/Objects"/>
	<skos:exactMatch rdf:resource="http://vocab.getty.edu/aat/300379948"/>
	<skos:editorialNote xml:lang="en">PPRefiningObjectType</skos:editorialNote>
	<skos:scopeNote xml:lang="en">Relatively small, flat objects, often rectangular, used to cover roofs, floors or walls, as game pieces, as lids, or for other purposes. Originally referred to such objects made of baked earth or earthenware, but modern usage includes such items made of other materials, including metal or plastic.</skos:scopeNote>
</skos:Concept>
<skos:Concept rdf:about="http://partage.vocnet.org/part01120">
	<skos:prefLabel xml:lang="en">jackets</skos:prefLabel>
	<skos:altLabel xml:lang="en">jackets (garments)</skos:altLabel>
	<skos:inScheme rdf:resource="http://partage.vocnet.org/Objects"/>
	<skos:broader rdf:resource="http://partage.vocnet.org/part00851"/>
	<skos:exactMatch rdf:resource="http://vocab.getty.edu/aat/300046167"/>
	<skos:editorialNote xml:lang="en">PPRefiningObjectType</skos:editorialNote>
	<skos:scopeNote xml:lang="en">A short coat for the upper body made in various forms and lengths but usually no lower than the waist; worn separately or as part of a suit. Also, similar outer garments worn for warmth or protection from the weather.</skos:scopeNote>
</skos:Concept>
<skos:Concept rdf:about="http://partage.vocnet.org/part01121">
	<skos:prefLabel xml:lang="hr">dekoratini pano</skos:prefLabel>
	<skos:prefLabel xml:lang="de">Wandverkleidung</skos:prefLabel>
	<skos:prefLabel xml:lang="en">panelling</skos:prefLabel>
	<skos:altLabel xml:lang="en">paneling</skos:altLabel>
	<skos:altLabel xml:lang="hr">zidna oplata</skos:altLabel>
	<skos:inScheme rdf:resource="http://partage.vocnet.org/Objects"/>
	<skos:broader rdf:resource="http://partage.vocnet.org/part00179"/>
	<skos:exactMatch rdf:resource="http://vocab.getty.edu/aat/300014658"/>
	<skos:editorialNote xml:lang="en">PPRefiningObejctType</skos:editorialNote>
	<skos:scopeNote xml:lang="en">Wall coverings consisting of panels of wood or other material joined in a continuous surface.</skos:scopeNote>
</skos:Concept>
<skos:Concept rdf:about="http://partage.vocnet.org/part01122">
	<skos:prefLabel xml:lang="hr">kalendar</skos:prefLabel>
	<skos:prefLabel xml:lang="de">Kalender</skos:prefLabel>
	<skos:prefLabel xml:lang="en">calendars</skos:prefLabel>
	<skos:inScheme rdf:resource="http://partage.vocnet.org/Objects"/>
	<skos:exactMatch rdf:resource="http://vocab.getty.edu/aat/300026741"/>
	<skos:editorialNote xml:lang="en">PPRefiningObjectType</skos:editorialNote>
	<skos:scopeNote xml:lang="en">Registers of days or other contrivances for reckoning days, months, years, etc., such as a table showing the division of a given year into its months, weeks, days, years, or other divisions of time. A calendar may include important astronomical data, ecclesiastical or other festivals, and other events belonging to specific days.</skos:scopeNote>
</skos:Concept>
<skos:Concept rdf:about="http://partage.vocnet.org/part01123">
	<skos:prefLabel xml:lang="hr">dionica</skos:prefLabel>
	<skos:prefLabel xml:lang="en">stocks (neckcloths)</skos:prefLabel>
	<skos:inScheme rdf:resource="http://partage.vocnet.org/Objects"/>
	<skos:broader rdf:resource="http://partage.vocnet.org/part01124"/>
	<skos:exactMatch rdf:resource="http://vocab.getty.edu/aat/300210073"/>
	<skos:editorialNote xml:lang="en">PPRefiningObjectType</skos:editorialNote>
	<skos:scopeNote xml:lang="en">Men's preformed neckcloths in the form of broad bands, soft or stiffened, usually fastened at the back. Also, similar neckcloths worn by men and women as part of formal riding attire and similar forms, sometimes made of leather, worn by military personnel as an item of uniform.</skos:scopeNote>
</skos:Concept>
<skos:Concept rdf:about="http://partage.vocnet.org/part01124">
	<skos:prefLabel xml:lang="en">neckcloths</skos:prefLabel>
	<skos:inScheme rdf:resource="http://partage.vocnet.org/Objects"/>
	<skos:broader rdf:resource="http://partage.vocnet.org/part00955"/>
	<skos:narrower rdf:resource="http://partage.vocnet.org/part01123"/>
	<skos:exactMatch rdf:resource="http://vocab.getty.edu/aat/300210069"/>
	<skos:scopeNote xml:lang="en">General term for cloths of varying form worn at the neck.</skos:scopeNote>
</skos:Concept>
<skos:Concept rdf:about="http://partage.vocnet.org/part01125">
	<skos:prefLabel xml:lang="hr">flakon</skos:prefLabel>
	<skos:prefLabel xml:lang="en">flacons (perfume bottles)</skos:prefLabel>
	<skos:altLabel xml:lang="en">perfume bottles</skos:altLabel>
	<skos:altLabel xml:lang="de">Parfümfläschchen</skos:altLabel>
	<skos:altLabel xml:lang="de">Flakons</skos:altLabel>
	<skos:altLabel xml:lang="de">Flacons</skos:altLabel>
	<skos:altLabel xml:lang="de">Flacon</skos:altLabel>
	<skos:prefLabel xml:lang="de">Flakon</skos:prefLabel>
	<skos:inScheme rdf:resource="http://partage.vocnet.org/Objects"/>
	<skos:broader rdf:resource="http://partage.vocnet.org/part00085"/>
	<skos:exactMatch rdf:resource="http://vocab.getty.edu/aat/300197635"/>
	<skos:editorialNote xml:lang="en">PPRefiningObjectType</skos:editorialNote>
	<skos:scopeNote xml:lang="en">Term applied to a wide variety of bottles of different size and shape intended primarily for holding or dispersing perfume. Includes those made for sale to cosmetics manufacturers as well as those often decorative forms meant to be placed on the dressing table and sometimes part of a toilet set.</skos:scopeNote>
</skos:Concept>
<skos:Concept rdf:about="http://partage.vocnet.org/part01127">
	<skos:altLabel xml:lang="de">Hosen</skos:altLabel>
	<skos:prefLabel xml:lang="de">Hose</skos:prefLabel>
	<skos:prefLabel xml:lang="hr">hlače</skos:prefLabel>
	<skos:prefLabel xml:lang="en">trousers</skos:prefLabel>
	<skos:inScheme rdf:resource="http://partage.vocnet.org/Objects"/>
	<skos:broader rdf:resource="http://partage.vocnet.org/part00851"/>
	<skos:exactMatch rdf:resource="http://vocab.getty.edu/aat/300209935"/>
	<skos:editorialNote xml:lang="en">PPRefiningObjectType</skos:editorialNote>
	<skos:scopeNote xml:lang="en">Exposed bifurcated garments which extend from waist or hips to the ankle or sometimes to the knee or just below.</skos:scopeNote>
</skos:Concept>
<skos:Concept rdf:about="http://partage.vocnet.org/part01129">
	<skos:altLabel xml:lang="de">Sims</skos:altLabel>
	<skos:prefLabel xml:lang="de">Gesims</skos:prefLabel>
	<skos:prefLabel xml:lang="hr">karniša</skos:prefLabel>
	<skos:prefLabel xml:lang="en">cornices</skos:prefLabel>
	<skos:inScheme rdf:resource="http://partage.vocnet.org/Objects"/>
	<skos:broader rdf:resource="http://partage.vocnet.org/part00127"/>
	<skos:exactMatch rdf:resource="http://vocab.getty.edu/aat/300001788"/>
	<skos:editorialNote xml:lang="en">PPRefiningObjectType</skos:editorialNote>
	<skos:scopeNote xml:lang="en">The projecting, uppermost features of classical entablatures; use also for similar features crowning a window or wall.</skos:scopeNote>
</skos:Concept>
<skos:Concept rdf:about="http://partage.vocnet.org/part01134">
	<skos:altLabel xml:lang="de">Kataloge</skos:altLabel>
	<skos:prefLabel xml:lang="de">Katalog</skos:prefLabel>
	<skos:prefLabel xml:lang="hr">katalog</skos:prefLabel>
	<skos:prefLabel xml:lang="en">catalogs</skos:prefLabel>
	<skos:inScheme rdf:resource="http://partage.vocnet.org/Objects"/>
	<skos:exactMatch rdf:resource="http://vocab.getty.edu/aat/300026059"/>
	<skos:editorialNote xml:lang="en">PPRefiningObjectType</skos:editorialNote>
	<skos:scopeNote xml:lang="en">Enumerations of items, such as a file of bibliographic records or a list of art objects, usually arranged systematically and with descriptive details; may be in book or pamphlet form, on cards, or online. Catalogs are created according to specific and uniform principles of construction and usually under the control of an authority file.</skos:scopeNote>
</skos:Concept>
<skos:Concept rdf:about="http://partage.vocnet.org/part01135">
	<skos:prefLabel xml:lang="de">Sportkleidung</skos:prefLabel>
	<skos:prefLabel xml:lang="en">sports clothing</skos:prefLabel>
	<skos:inScheme rdf:resource="http://partage.vocnet.org/Objects"/>
	<skos:broader rdf:resource="http://partage.vocnet.org/part00081"/>
	<skos:exactMatch rdf:resource="http://vocab.getty.edu/aat/300221269"/>
	<skos:editorialNote xml:lang="en">PPRefiningObjectType</skos:editorialNote>
	<skos:scopeNote xml:lang="en">Garments and accessories designed to be worn while engaged in a specific active sport.</skos:scopeNote>
</skos:Concept>
<skos:Concept rdf:about="http://partage.vocnet.org/part01136">
	<skos:prefLabel xml:lang="hr">lavor</skos:prefLabel>
	<skos:prefLabel xml:lang="en">basins</skos:prefLabel>
	<skos:altLabel xml:lang="en">basins (vessels)</skos:altLabel>
	<skos:inScheme rdf:resource="http://partage.vocnet.org/Objects"/>
	<skos:broader rdf:resource="http://partage.vocnet.org/part00083"/>
	<skos:broader rdf:resource="http://partage.vocnet.org/part00321"/>
	<skos:exactMatch rdf:resource="http://vocab.getty.edu/aat/300045614"/>
	<skos:editorialNote xml:lang="en">PPRefiningObjectType</skos:editorialNote>
	<skos:scopeNote xml:lang="en">Open, rounded vessels of greater width than depth, with sloping or curving sides, used for receiving running water or holding water and other liquids, especially for washing purposes.</skos:scopeNote>
</skos:Concept>
<skos:Concept rdf:about="http://partage.vocnet.org/part01137">
	<skos:prefLabel xml:lang="hr">lutka</skos:prefLabel>
	<skos:altLabel xml:lang="de">Puppen</skos:altLabel>
	<skos:prefLabel xml:lang="de">Puppe</skos:prefLabel>
	<skos:prefLabel xml:lang="en">dolls</skos:prefLabel>
	<skos:inScheme rdf:resource="http://partage.vocnet.org/Objects"/>
	<skos:broader rdf:resource="http://partage.vocnet.org/part00412"/>
	<skos:broader rdf:resource="http://partage.vocnet.org/part01170"/>
	<skos:exactMatch rdf:resource="http://vocab.getty.edu/aat/300211087"/>
	<skos:editorialNote xml:lang="en">PPRefiningObjectType</skos:editorialNote>
	<skos:scopeNote xml:lang="en">Figurines representing humans or animals, including but not restricted to those intended as toys for children, usually girls, or as collectibles for adults. Dolls are commonly in the form of a baby or woman, often with changeable clothes; they may have moveable arms and legs. Doll may be made of cloth (rag dolls), wood, clay, porcelain, wax, paper, plastic, celluloid, corn husks, or other materials. Dolls may also be figurines used for ceremonial, religious, or decorative purposes. Archaeological evidence suggests that dolls were the first playthings; they have been found in Babylonian and Egyptian tombs from ca. 3000 BCE. In ancient Greece and Rome, maturing girls consecrated their childhood dolls to the goddesses. Cloth dolls in the form of animals are generally called "stuffed toys."</skos:scopeNote>
</skos:Concept>
<skos:Concept rdf:about="http://partage.vocnet.org/part01141">
	<skos:altLabel xml:lang="de">Nachtgeschirr</skos:altLabel>
	<skos:prefLabel xml:lang="de">Nachttopf</skos:prefLabel>
	<skos:prefLabel xml:lang="hr">noćna posuda</skos:prefLabel>
	<skos:prefLabel xml:lang="en">chamber pots</skos:prefLabel>
	<skos:altLabel xml:lang="de">Nachttöpfe</skos:altLabel>
	<skos:inScheme rdf:resource="http://partage.vocnet.org/Objects"/>
	<skos:broader rdf:resource="http://partage.vocnet.org/part00682"/>
	<skos:exactMatch rdf:resource="http://vocab.getty.edu/aat/300198893"/>
	<skos:editorialNote xml:lang="en">PPRefiningObjectType</skos:editorialNote>
	<skos:scopeNote xml:lang="en">Portable bowls kept in a bedroom and used for the discharge of urine, etc., especially at night. Usually having shaped convex sides, a flat bottom, and a single loop or scroll handle; some have covers.</skos:scopeNote>
</skos:Concept>
<skos:Concept rdf:about="http://partage.vocnet.org/part01143">
	<skos:altLabel xml:lang="de">Nachttische</skos:altLabel>
	<skos:prefLabel xml:lang="de">Nachttisch</skos:prefLabel>
	<skos:prefLabel xml:lang="hr">noćni ormarić</skos:prefLabel>
	<skos:prefLabel xml:lang="en">night tables</skos:prefLabel>
	<skos:altLabel xml:lang="en">nightstands</skos:altLabel>
	<skos:inScheme rdf:resource="http://partage.vocnet.org/Objects"/>
	<skos:broader rdf:resource="http://partage.vocnet.org/part00316"/>
	<skos:exactMatch rdf:resource="http://vocab.getty.edu/aat/300039745"/>
	<skos:editorialNote xml:lang="en">PPRefiniingObjectType</skos:editorialNote>
	<skos:scopeNote xml:lang="en">Small tables made to stand beside a bed; includes those having a cupboard to hold a chamber pot and those with a close stool that pulls forward in the lower part.</skos:scopeNote>
</skos:Concept>
<skos:Concept rdf:about="http://partage.vocnet.org/part01144">
	<skos:prefLabel xml:lang="de">Löffel</skos:prefLabel>
	<skos:prefLabel xml:lang="en">spoons</skos:prefLabel>
	<skos:inScheme rdf:resource="http://partage.vocnet.org/Objects"/>
	<skos:broader rdf:resource="http://partage.vocnet.org/part00219"/>
	<skos:exactMatch rdf:resource="http://vocab.getty.edu/aat/300043149"/>
	<skos:editorialNote xml:lang="en">PPRefiningObjectType</skos:editorialNote>
	<skos:scopeNote xml:lang="en">Utensils consisting of a shallow bowl with a handle used for preparing, cooking, serving, or eating food.</skos:scopeNote>
</skos:Concept>
<skos:Concept rdf:about="http://partage.vocnet.org/part01146">
	<skos:altLabel xml:lang="de">Büsten</skos:altLabel>
	<skos:prefLabel xml:lang="de">Büste</skos:prefLabel>
	<skos:prefLabel xml:lang="hr">poprsje</skos:prefLabel>
	<skos:prefLabel xml:lang="en">busts (figures)</skos:prefLabel>
	<skos:inScheme rdf:resource="http://partage.vocnet.org/Objects"/>
	<skos:broader rdf:resource="http://partage.vocnet.org/part01201"/>
	<skos:exactMatch rdf:resource="http://vocab.getty.edu/aat/300047457"/>
	<skos:editorialNote xml:lang="en">PPRefiningOnjectType</skos:editorialNote>
	<skos:scopeNote xml:lang="en">Representations of only the head and shoulders of a human figure.</skos:scopeNote>
</skos:Concept>
<skos:Concept rdf:about="http://partage.vocnet.org/part01155">
	<skos:prefLabel xml:lang="hr">posjetnica</skos:prefLabel>
	<skos:altLabel xml:lang="de">Besuchskarten</skos:altLabel>
	<skos:prefLabel xml:lang="de">Besuchskarte</skos:prefLabel>
	<skos:prefLabel xml:lang="en">visiting cards</skos:prefLabel>
	<skos:inScheme rdf:resource="http://partage.vocnet.org/Objects"/>
	<skos:exactMatch rdf:resource="http://vocab.getty.edu/aat/300026823"/>
	<skos:editorialNote xml:lang="en">PPRefiningObjectType</skos:editorialNote>
	<skos:scopeNote xml:lang="en">Small cards bearing the name, and sometimes the address of a person or married couple for presentation, as when formally calling or visiting.</skos:scopeNote>
</skos:Concept>
<skos:Concept rdf:about="http://partage.vocnet.org/part01157">
	<skos:altLabel xml:lang="de">Briefbeschwerer</skos:altLabel>
	<skos:altLabel xml:lang="de">Paperweights</skos:altLabel>
	<skos:prefLabel xml:lang="de">Paperweight</skos:prefLabel>
	<skos:prefLabel xml:lang="hr">pritiskivač za papir</skos:prefLabel>
	<skos:prefLabel xml:lang="en">paperweights</skos:prefLabel>
	<skos:inScheme rdf:resource="http://partage.vocnet.org/Objects"/>
	<skos:broader rdf:resource="http://partage.vocnet.org/part00100"/>
	<skos:exactMatch rdf:resource="http://vocab.getty.edu/aat/300236043"/>
	<skos:editorialNote xml:lang="en">PPRefiningObjectType</skos:editorialNote>
	<skos:scopeNote xml:lang="en">Small, heavy objects of glass, metal, or the like placed on papers to keep them from scattering.</skos:scopeNote>
</skos:Concept>
<skos:Concept rdf:about="http://partage.vocnet.org/part01158">
	<skos:altLabel xml:lang="de">Dokumente</skos:altLabel>
	<skos:prefLabel xml:lang="de">Dokument</skos:prefLabel>
	<skos:prefLabel xml:lang="en">records (documents)</skos:prefLabel>
	<skos:inScheme rdf:resource="http://partage.vocnet.org/Objects"/>
	<skos:exactMatch rdf:resource="http://vocab.getty.edu/aat/300026685"/>
	<skos:editorialNote xml:lang="en">PPRefiningObjectType</skos:editorialNote>
	<skos:scopeNote xml:lang="en">Recorded information, regardless of medium, created, received, and maintained by an agency, institution, organization, or individual in pursuance of its legal obligations or in the transaction of business.</skos:scopeNote>
</skos:Concept>
<skos:Concept rdf:about="http://partage.vocnet.org/part01160">
	<skos:prefLabel xml:lang="de">Bowle (Gefäß)</skos:prefLabel>
	<skos:prefLabel xml:lang="en">punch bowls</skos:prefLabel>
	<skos:altLabel xml:lang="de">Bowlen (Gefäße)</skos:altLabel>
	<skos:inScheme rdf:resource="http://partage.vocnet.org/Objects"/>
	<skos:broader rdf:resource="http://partage.vocnet.org/part00085"/>
	<skos:exactMatch rdf:resource="http://vocab.getty.edu/aat/300043061"/>
	<skos:editorialNote xml:lang="en">PPRefiningObjectType</skos:editorialNote>
	<skos:scopeNote xml:lang="en">Large bowls, usually made of silver, ceramic, or glass, in which a beverage, such as punch or lemonade, is prepared and served. They are frequently accompanied by a ladle and sometimes a set of punch cups.</skos:scopeNote>
</skos:Concept>
<skos:Concept rdf:about="http://partage.vocnet.org/part01161">
	<skos:altLabel xml:lang="de">Gießkannen</skos:altLabel>
	<skos:prefLabel xml:lang="de">Gießkanne</skos:prefLabel>
	<skos:prefLabel xml:lang="en">watering cans</skos:prefLabel>
	<skos:inScheme rdf:resource="http://partage.vocnet.org/Objects"/>
	<skos:broader rdf:resource="http://partage.vocnet.org/part00085"/>
	<skos:exactMatch rdf:resource="http://vocab.getty.edu/aat/300197360"/>
	<skos:scopeNote xml:lang="en">Containers for water, typically of metal or plastic and having a spout with a perforated nozzle, for watering or sprinkling plants.</skos:scopeNote>
	<skos:editorialNote xml:lang="en">PPRefiningObjectType</skos:editorialNote>
</skos:Concept>
<skos:Concept rdf:about="http://partage.vocnet.org/part01162">
	<skos:altLabel xml:lang="de">Kessel</skos:altLabel>
	<skos:prefLabel xml:lang="de">Wasserkessel</skos:prefLabel>
	<skos:prefLabel xml:lang="en">kettles (vessels)</skos:prefLabel>
	<skos:inScheme rdf:resource="http://partage.vocnet.org/Objects"/>
	<skos:broader rdf:resource="http://partage.vocnet.org/part00083"/>
	<skos:broader rdf:resource="http://partage.vocnet.org/part00682"/>
	<skos:exactMatch rdf:resource="http://vocab.getty.edu/aat/300195349"/>
	<skos:scopeNote xml:lang="en">Large wide metal vessels used for boiling or cooking, having a bail handle and sometimes a lid or small feet.</skos:scopeNote>
	<skos:editorialNote xml:lang="en">PPRefiningObjectType</skos:editorialNote>
</skos:Concept>
<skos:Concept rdf:about="http://partage.vocnet.org/part01163">
	<skos:prefLabel xml:lang="de">Schirmständer</skos:prefLabel>
	<skos:prefLabel xml:lang="en">umbrella stands</skos:prefLabel>
	<skos:inScheme rdf:resource="http://partage.vocnet.org/Objects"/>
	<skos:broader rdf:resource="http://partage.vocnet.org/part00928"/>
	<skos:exactMatch rdf:resource="http://vocab.getty.edu/aat/300039852"/>
	<skos:editorialNote xml:lang="en">PPRefiningObjectType</skos:editorialNote>
	<skos:scopeNote xml:lang="en">Stands or receptacles for holding umbrellas, generally located inside a home or other building near an exterior door. The term is used for stands of metal or wood construction as well as for large cylinder-shaped vessels of ceramic, metal, or another material, designed and used for holding umbrellas.</skos:scopeNote>
</skos:Concept>
<skos:Concept rdf:about="http://partage.vocnet.org/part01164">
	<skos:altLabel xml:lang="de">Tischtücher</skos:altLabel>
	<skos:altLabel xml:lang="de">Tischtuch</skos:altLabel>
	<skos:altLabel xml:lang="de">Tischdecken</skos:altLabel>
	<skos:prefLabel xml:lang="de">Tischdecke</skos:prefLabel>
	<skos:prefLabel xml:lang="en">tablecloths</skos:prefLabel>
	<skos:inScheme rdf:resource="http://partage.vocnet.org/Objects"/>
	<skos:broader rdf:resource="http://partage.vocnet.org/part00100"/>
	<skos:exactMatch rdf:resource="http://vocab.getty.edu/aat/300204969"/>
	<skos:editorialNote xml:lang="en">PPRefiningObjectType</skos:editorialNote>
	<skos:scopeNote xml:lang="en">Cloths for covering the top of a table, especially during a meal.</skos:scopeNote>
</skos:Concept>
<skos:Concept rdf:about="http://partage.vocnet.org/part01168">
	<skos:altLabel xml:lang="de">Soßengiesser</skos:altLabel>
	<skos:altLabel xml:lang="de">Saucièren</skos:altLabel>
	<skos:prefLabel xml:lang="de">Saucière</skos:prefLabel>
	<skos:prefLabel xml:lang="en">sauceboats</skos:prefLabel>
	<skos:altLabel xml:lang="en">saucières</skos:altLabel>
	<skos:inScheme rdf:resource="http://partage.vocnet.org/Objects"/>
	<skos:broader rdf:resource="http://partage.vocnet.org/part00085"/>
	<skos:exactMatch rdf:resource="http://vocab.getty.edu/aat/300218762"/>
	<skos:editorialNote xml:lang="en">PPRefiningObjectType</skos:editorialNote>
	<skos:scopeNote xml:lang="en">Boat-shaped vessels, usually with a long pouring lip at one end and a handle at the other or two pouring lips and a central handle, used for serving sauces, gravies, or the like.</skos:scopeNote>
</skos:Concept>
<skos:Concept rdf:about="http://partage.vocnet.org/part01169">
	<skos:altLabel xml:lang="de">Terrinen</skos:altLabel>
	<skos:prefLabel xml:lang="de">Terrine</skos:prefLabel>
	<skos:prefLabel xml:lang="en">tureens</skos:prefLabel>
	<skos:inScheme rdf:resource="http://partage.vocnet.org/Objects"/>
	<skos:broader rdf:resource="http://partage.vocnet.org/part00085"/>
	<skos:exactMatch rdf:resource="http://vocab.getty.edu/aat/300199769"/>
	<skos:editorialNote xml:lang="en">PPRefiningObjectType</skos:editorialNote>
	<skos:scopeNote xml:lang="en">Deep vessels of varying size and shape, and usually having a cover; used for serving soup, sauce, stew, or other foods.</skos:scopeNote>
</skos:Concept>
<skos:Concept rdf:about="http://partage.vocnet.org/part01170">
	<skos:prefLabel xml:lang="de">Spielzeug</skos:prefLabel>
	<skos:prefLabel xml:lang="en">toys (recreational artifacts)</skos:prefLabel>
	<skos:altLabel xml:lang="de">Spielwaren</skos:altLabel>
	<skos:altLabel xml:lang="de">Spielzeuge</skos:altLabel>
	<skos:inScheme rdf:resource="http://partage.vocnet.org/Objects"/>
	<skos:broader rdf:resource="http://partage.vocnet.org/part00181"/>
	<skos:narrower rdf:resource="http://partage.vocnet.org/part01137"/>
	<skos:exactMatch rdf:resource="http://vocab.getty.edu/aat/300211037"/>
	<skos:editorialNote xml:lang="en">PPRefiningObjectType</skos:editorialNote>
	<skos:scopeNote xml:lang="en">Material objects contrived for amusement rather than for practical use by children or pets, or intended as collectibles by adults. Toys are generally miniature versions of real beings or objects that lend themselves to imaginative or imitative play. Toys may also be items for use in games. Among the earliest toys were dolls and balls.</skos:scopeNote>
</skos:Concept>
<skos:Concept rdf:about="http://partage.vocnet.org/part01171">
	<skos:prefLabel xml:lang="en">robes (main garments)</skos:prefLabel>
	<skos:prefLabel xml:lang="hr">ogrtač</skos:prefLabel>
	<skos:altLabel xml:lang="de">Gewänder</skos:altLabel>
	<skos:prefLabel xml:lang="de">Gewand</skos:prefLabel>
	<skos:inScheme rdf:resource="http://partage.vocnet.org/Objects"/>
	<skos:broader rdf:resource="http://partage.vocnet.org/part00851"/>
	<skos:exactMatch rdf:resource="http://vocab.getty.edu/aat/300209852"/>
	<skos:editorialNote xml:lang="en">PPRefiningObjectType</skos:editorialNote>
	<skos:scopeNote xml:lang="en">Long, loose garments, which tend to be of one piece and to open down the front, cut with flowing lines; worn for ordinary wear by men and women during the Middle Ages and until the modern period, especially in Asian and African countries. Also, similar garments often of elegant style worn for ceremonial or official occasions or as a symbol of office or profession. Also, term used generally from the 18th century through the early 20th century for fashionable women's dress of varying form. Prefer "gowns" for women's dresses of varying form, originally closed with a semi-fitted bodice, and which usually have a long, flowing skirt. For loose-fitting garments of varying length, often wraparound and tied with a belt, worn before or after bathing or informally around the house use "bathrobes."</skos:scopeNote>
</skos:Concept>
<skos:Concept rdf:about="http://partage.vocnet.org/part01172">
	<skos:prefLabel xml:lang="hr">predložak</skos:prefLabel>
	<skos:altLabel xml:lang="de">Muster (Vorlagen)</skos:altLabel>
	<skos:altLabel xml:lang="de">Muster (Vorlage)</skos:altLabel>
	<skos:altLabel xml:lang="de">Vorlagen</skos:altLabel>
	<skos:prefLabel xml:lang="de">Vorlage</skos:prefLabel>
	<skos:prefLabel xml:lang="en">templates (shaping tools)</skos:prefLabel>
	<skos:inScheme rdf:resource="http://partage.vocnet.org/Objects"/>
	<skos:broader rdf:resource="http://partage.vocnet.org/part00218"/>
	<skos:exactMatch rdf:resource="http://vocab.getty.edu/aat/300022539"/>
	<skos:scopeNote xml:lang="en">Guiding tools such as stencils, patterns, or overlays used for duplicating shapes or designs in sculpting, woodcrafting, creating architectural details, graphic arts, sewing, and other activities.</skos:scopeNote>
	<skos:editorialNote xml:lang="en">PPRefiningObjectType</skos:editorialNote>
</skos:Concept>
<skos:Concept rdf:about="http://partage.vocnet.org/part01175">
	<skos:prefLabel xml:lang="hr">sjenilo</skos:prefLabel>
	<skos:altLabel xml:lang="de">Lampenschirme</skos:altLabel>
	<skos:prefLabel xml:lang="de">Lampenschirm</skos:prefLabel>
	<skos:prefLabel xml:lang="en">lampshades</skos:prefLabel>
	<skos:inScheme rdf:resource="http://partage.vocnet.org/Objects"/>
	<skos:broader rdf:resource="http://partage.vocnet.org/part00100"/>
	<skos:exactMatch rdf:resource="http://vocab.getty.edu/aat/300037661"/>
	<skos:editorialNote xml:lang="en">PPRefiningObjectType</skos:editorialNote>
	<skos:scopeNote xml:lang="en">Shades placed over or around the light source of a lamp, and that are designed to diffuse or direct light and shield glare. They may be designed to perform a task or to be primarily decorative.</skos:scopeNote>
</skos:Concept>
<skos:Concept rdf:about="http://partage.vocnet.org/part01177">
	<skos:altLabel xml:lang="de">Autographen</skos:altLabel>
	<skos:prefLabel xml:lang="de">Autograph</skos:prefLabel>
	<skos:prefLabel xml:lang="en">autographs (manuscripts)</skos:prefLabel>
	<skos:inScheme rdf:resource="http://partage.vocnet.org/Objects"/>
	<skos:broader rdf:resource="http://partage.vocnet.org/part01178"/>
	<skos:exactMatch rdf:resource="http://vocab.getty.edu/aat/300028571"/>
	<skos:scopeNote xml:lang="en">Documents written in, and usually signed with, the writer's own hand; in certain legal instances, prefer "holographs."</skos:scopeNote>
	<skos:editorialNote xml:lang="en">PPRefiningObjectType</skos:editorialNote>
</skos:Concept>
<skos:Concept rdf:about="http://partage.vocnet.org/part01178">
	<skos:altLabel xml:lang="de">Handschriften</skos:altLabel>
	<skos:prefLabel xml:lang="de">Handschrift</skos:prefLabel>
	<skos:prefLabel xml:lang="en">manuscripts (document genre)</skos:prefLabel>
	<skos:inScheme rdf:resource="http://partage.vocnet.org/Objects"/>
	<skos:narrower rdf:resource="http://partage.vocnet.org/part01177"/>
	<skos:exactMatch rdf:resource="http://vocab.getty.edu/aat/300028569"/>
	<skos:editorialNote xml:lang="en">PPRefiningObjectType</skos:editorialNote>
	<skos:scopeNote xml:lang="en">Handwritten documents, particularly books and other documents created before the invention of the printing press. May also be used to distinguish certain documents from published or otherwise printed documents, as in the cases of typed personal letters or a typescript from which printed versions are made.</skos:scopeNote>
</skos:Concept>
<skos:Concept rdf:about="http://partage.vocnet.org/part01179">
	<skos:altLabel xml:lang="de">Pflanzenständer</skos:altLabel>
	<skos:prefLabel xml:lang="de">Blumenständer</skos:prefLabel>
	<skos:prefLabel xml:lang="hr">stalak za cvijeće</skos:prefLabel>
	<skos:altLabel xml:lang="en">flower stands</skos:altLabel>
	<skos:prefLabel xml:lang="en">plant stands</skos:prefLabel>
	<skos:inScheme rdf:resource="http://partage.vocnet.org/Objects"/>
	<skos:broader rdf:resource="http://partage.vocnet.org/part00928"/>
	<skos:exactMatch rdf:resource="http://vocab.getty.edu/aat/300039835"/>
	<skos:editorialNote xml:lang="en">PPRefiningObjectType</skos:editorialNote>
	<skos:scopeNote xml:lang="en">Small tablelike pieces of furniture used to hold or display plants or flowers.</skos:scopeNote>
</skos:Concept>
<skos:Concept rdf:about="http://partage.vocnet.org/part01180">
	<skos:prefLabel xml:lang="hr">suncobran</skos:prefLabel>
	<skos:altLabel xml:lang="de">Sonnenschirme</skos:altLabel>
	<skos:prefLabel xml:lang="de">Sonnenschirm</skos:prefLabel>
	<skos:prefLabel xml:lang="en">parasols</skos:prefLabel>
	<skos:inScheme rdf:resource="http://partage.vocnet.org/Objects"/>
	<skos:broader rdf:resource="http://partage.vocnet.org/part00080"/>
	<skos:broader rdf:resource="http://partage.vocnet.org/part01181"/>
	<skos:exactMatch rdf:resource="http://vocab.getty.edu/aat/300046218"/>
	<skos:editorialNote xml:lang="en">PPRefiningObjectType</skos:editorialNote>
	<skos:scopeNote xml:lang="en">Small umbrellas used as a sunshade or simply carried as a fashionable accessory.</skos:scopeNote>
</skos:Concept>
<skos:Concept rdf:about="http://partage.vocnet.org/part01181">
	<skos:altLabel xml:lang="de">Schirme</skos:altLabel>
	<skos:prefLabel xml:lang="de">Schirm</skos:prefLabel>
	<skos:prefLabel xml:lang="en">umbrellas</skos:prefLabel>
	<skos:inScheme rdf:resource="http://partage.vocnet.org/Objects"/>
	<skos:broader rdf:resource="http://partage.vocnet.org/part00218"/>
	<skos:narrower rdf:resource="http://partage.vocnet.org/part01180"/>
	<skos:exactMatch rdf:resource="http://vocab.getty.edu/aat/300046227"/>
	<skos:editorialNote xml:lang="en">PPRefiningObjectType</skos:editorialNote>
	<skos:scopeNote xml:lang="en">300046227</skos:scopeNote>
</skos:Concept>
<skos:Concept rdf:about="http://partage.vocnet.org/part01182">
	<skos:prefLabel xml:lang="hr">ulaznica</skos:prefLabel>
	<skos:altLabel xml:lang="de">Eintrittskarten</skos:altLabel>
	<skos:prefLabel xml:lang="de">Eintrittskarte</skos:prefLabel>
	<skos:altLabel xml:lang="de">Tickets</skos:altLabel>
	<skos:altLabel xml:lang="de">Ticket</skos:altLabel>
	<skos:prefLabel xml:lang="en">tickets</skos:prefLabel>
	<skos:inScheme rdf:resource="http://partage.vocnet.org/Objects"/>
	<skos:exactMatch rdf:resource="http://vocab.getty.edu/aat/300027381"/>
	<skos:editorialNote xml:lang="en">PPRefiningObjectType</skos:editorialNote>
	<skos:scopeNote xml:lang="en">Slips of paper or cardboard serving as evidence that the holder has paid a fare or admission or is entitled to some service.</skos:scopeNote>
</skos:Concept>
<skos:Concept rdf:about="http://partage.vocnet.org/part01184">
	<skos:altLabel xml:lang="de">Schatullen</skos:altLabel>
	<skos:prefLabel xml:lang="de">Schatulle</skos:prefLabel>
	<skos:altLabel xml:lang="de">Kästchen</skos:altLabel>
	<skos:prefLabel xml:lang="en">caskets (personal gear)</skos:prefLabel>
	<skos:altLabel xml:lang="de">Kassetten</skos:altLabel>
	<skos:altLabel xml:lang="de">Kassette</skos:altLabel>
	<skos:inScheme rdf:resource="http://partage.vocnet.org/Objects"/>
	<skos:broader rdf:resource="http://partage.vocnet.org/part00302"/>
	<skos:broader rdf:resource="http://partage.vocnet.org/part00318"/>
	<skos:exactMatch rdf:resource="http://vocab.getty.edu/aat/300039006"/>
	<skos:editorialNote xml:lang="en">PPRefiningObjectType</skos:editorialNote>
	<skos:scopeNote xml:lang="en">Small chests or boxes for holding objects of value such as money, letters, and jewels; usually of wood or metal and highly ornamented and often hinged.</skos:scopeNote>
</skos:Concept>
<skos:Concept rdf:about="http://partage.vocnet.org/part01185">
	<skos:altLabel xml:lang="de">Hüllen.</skos:altLabel>
	<skos:altLabel xml:lang="de">Hülle.</skos:altLabel>
	<skos:altLabel xml:lang="de">Überwurf</skos:altLabel>
	<skos:prefLabel xml:lang="de">Bedeckung</skos:prefLabel>
	<skos:prefLabel xml:lang="en">coverings</skos:prefLabel>
	<skos:inScheme rdf:resource="http://partage.vocnet.org/Objects"/>
	<skos:broader rdf:resource="http://partage.vocnet.org/part00100"/>
	<skos:exactMatch rdf:resource="http://vocab.getty.edu/aat/300205009"/>
	<skos:editorialNote xml:lang="en">PPRefiningObjectType</skos:editorialNote>
	<skos:scopeNote xml:lang="en">Artifacts, usually flexible, often textiles, used to cover or conceal interior spaces, surfaces, or furnishings, especially for protection, warmth, or embellishment.</skos:scopeNote>
</skos:Concept>
<skos:Concept rdf:about="http://partage.vocnet.org/part01187">
	<skos:prefLabel xml:lang="de">Notenständer</skos:prefLabel>
	<skos:prefLabel xml:lang="en">music stands</skos:prefLabel>
	<skos:inScheme rdf:resource="http://partage.vocnet.org/Objects"/>
	<skos:broader rdf:resource="http://partage.vocnet.org/part00928"/>
	<skos:exactMatch rdf:resource="http://vocab.getty.edu/aat/300039830"/>
</skos:Concept>
<skos:Concept rdf:about="http://partage.vocnet.org/part01188">
	<skos:prefLabel xml:lang="de">Gitter</skos:prefLabel>
	<skos:prefLabel xml:lang="en">lattices</skos:prefLabel>
	<skos:inScheme rdf:resource="http://partage.vocnet.org/Objects"/>
	<skos:broader rdf:resource="http://partage.vocnet.org/part00127"/>
	<skos:exactMatch rdf:resource="http://vocab.getty.edu/aat/300163920"/>
	<skos:editorialNote xml:lang="en">PPRefiningObjectType</skos:editorialNote>
	<skos:scopeNote xml:lang="en">Networks of small light bars of wood, metal, or other material crossing at regular intervals, usually diagonally.</skos:scopeNote>
</skos:Concept>
<skos:Concept rdf:about="http://partage.vocnet.org/part01189">
	<skos:altLabel xml:lang="de">Bildplatten</skos:altLabel>
	<skos:prefLabel xml:lang="de">Bildplatte</skos:prefLabel>
	<skos:prefLabel xml:lang="en">plaques</skos:prefLabel>
	<skos:inScheme rdf:resource="http://partage.vocnet.org/Objects"/>
	<skos:exactMatch rdf:resource="http://vocab.getty.edu/aat/300010262"/>
	<skos:editorialNote xml:lang="en">PPRefiningObjectType</skos:editorialNote>
	<skos:scopeNote xml:lang="en">Flat, thin, usually small objects, made of metal, clay, ivory, glass, or basketry, sometimes set into a surface for decoration or to bear an inscription.</skos:scopeNote>
</skos:Concept>
<skos:Concept rdf:about="http://partage.vocnet.org/part01190">
	<skos:altLabel xml:lang="de">Zuckerdosen</skos:altLabel>
	<skos:prefLabel xml:lang="de">Zuckerdose</skos:prefLabel>
	<skos:prefLabel xml:lang="en">sugar bowls</skos:prefLabel>
	<skos:prefLabel xml:lang="hr">šećernica</skos:prefLabel>
	<skos:inScheme rdf:resource="http://partage.vocnet.org/Objects"/>
	<skos:broader rdf:resource="http://partage.vocnet.org/part00085"/>
	<skos:exactMatch rdf:resource="http://vocab.getty.edu/aat/300042971"/>
	<skos:editorialNote xml:lang="en">PPRefiningObjectType</skos:editorialNote>
	<skos:scopeNote xml:lang="en">Bowls of varying form intended primarily for holding and serving sugar; made as an individual piece, to match a creamer, or as part of a tea or coffee service.</skos:scopeNote>
</skos:Concept>
<skos:Concept rdf:about="http://partage.vocnet.org/part01191">
	<skos:altLabel xml:lang="de">Statuetten</skos:altLabel>
	<skos:prefLabel xml:lang="de">Statuette</skos:prefLabel>
	<skos:prefLabel xml:lang="en">statuettes (statues)</skos:prefLabel>
	<skos:inScheme rdf:resource="http://partage.vocnet.org/Objects"/>
	<skos:broader rdf:resource="http://partage.vocnet.org/part00410"/>
	<skos:exactMatch rdf:resource="http://vocab.getty.edu/aat/300312262"/>
	<skos:editorialNote xml:lang="en">PPRefiningObjectType</skos:editorialNote>
	<skos:scopeNote xml:lang="en">Three-dimensional, free-standing sculptures that are smaller than life-size and usually but not always figural. They are often reduced versions of larger works. While the term may be used interchangeably with "figurine" in certain situations, it differs in that a statuette is always free-standing while a figurine may be part of a larger work, such as a decorative detail on a candelabra or mirror. Also, a statuette may represent objects other than a figure, while a figurine always represents a human, animal, or mythical figure.</skos:scopeNote>
</skos:Concept>
<skos:Concept rdf:about="http://partage.vocnet.org/part01192">
	<skos:altLabel xml:lang="de">Vorhänge</skos:altLabel>
	<skos:prefLabel xml:lang="de">Vorhang</skos:prefLabel>
	<skos:prefLabel xml:lang="en">curtains</skos:prefLabel>
	<skos:inScheme rdf:resource="http://partage.vocnet.org/Objects"/>
	<skos:broader rdf:resource="http://partage.vocnet.org/part00100"/>
	<skos:exactMatch rdf:resource="http://vocab.getty.edu/aat/300037564"/>
	<skos:editorialNote xml:lang="en">PPRefiningObjectType</skos:editorialNote>
	<skos:scopeNote xml:lang="en">Cloth hangings for windows, doorways, or other openings that are generally finished with hems, casings, pleats, or ruffles and hung by the top edge; used for privacy, control of light and drafts, or decoration.</skos:scopeNote>
</skos:Concept>
<skos:Concept rdf:about="http://partage.vocnet.org/part01193">
	<skos:altLabel xml:lang="de">Samoware</skos:altLabel>
	<skos:prefLabel xml:lang="de">Samowar</skos:prefLabel>
	<skos:prefLabel xml:lang="en">samovars</skos:prefLabel>
	<skos:inScheme rdf:resource="http://partage.vocnet.org/Objects"/>
	<skos:broader rdf:resource="http://partage.vocnet.org/part00085"/>
	<skos:exactMatch rdf:resource="http://vocab.getty.edu/aat/300215736"/>
	<skos:editorialNote xml:lang="en">PPRefiningObjectType</skos:editorialNote>
	<skos:scopeNote xml:lang="en">Metal, often copper, urn-shaped vessels, with a spigot at the base and interior tubes for hot coals; used to boil water for tea. Term used especially with reference to Russian types.</skos:scopeNote>
</skos:Concept>
<skos:Concept rdf:about="http://partage.vocnet.org/part01194">
	<skos:prefLabel xml:lang="de">Türklopfer</skos:prefLabel>
	<skos:prefLabel xml:lang="en">door knockers</skos:prefLabel>
	<skos:inScheme rdf:resource="http://partage.vocnet.org/Objects"/>
	<skos:broader rdf:resource="http://partage.vocnet.org/part00498"/>
	<skos:exactMatch rdf:resource="http://vocab.getty.edu/aat/300080114"/>
	<skos:editorialNote xml:lang="en">PPRefiningObjectType</skos:editorialNote>
	<skos:scopeNote xml:lang="en">Appendages, usually of iron or brass, fastened to a door and hinged so that it may be made to strike against a metal plate or the door itself, to attract the attention of those within. Door knockers are usually placed on exterior doors.</skos:scopeNote>
</skos:Concept>
<skos:Concept rdf:about="http://partage.vocnet.org/part01198">
	<skos:altLabel xml:lang="de">Taschenuhren</skos:altLabel>
	<skos:prefLabel xml:lang="de">Taschenuhr</skos:prefLabel>
	<skos:prefLabel xml:lang="en">pocket watches</skos:prefLabel>
	<skos:prefLabel xml:lang="hr">džepni sat</skos:prefLabel>
	<skos:inScheme rdf:resource="http://partage.vocnet.org/Objects"/>
	<skos:broader rdf:resource="http://partage.vocnet.org/part00789"/>
	<skos:exactMatch rdf:resource="http://vocab.getty.edu/aat/300200088"/>
	<skos:editorialNote xml:lang="en">PPRefiningObjectType</skos:editorialNote>
	<skos:scopeNote xml:lang="en">Watches meant to be carried in pockets, as opposed, for example to be worn on the wrist or carried on chains.</skos:scopeNote>
</skos:Concept>
<skos:Concept rdf:about="http://partage.vocnet.org/part01199">
	<skos:prefLabel xml:lang="hr">naslovna stranica</skos:prefLabel>
	<skos:altLabel xml:lang="de">Titelseiten</skos:altLabel>
	<skos:prefLabel xml:lang="de">Titelseite</skos:prefLabel>
	<skos:prefLabel xml:lang="en">title pages</skos:prefLabel>
	<skos:inScheme rdf:resource="http://partage.vocnet.org/Objects"/>
	<skos:broader rdf:resource="http://partage.vocnet.org/part01200"/>
	<skos:exactMatch rdf:resource="http://vocab.getty.edu/aat/300055033"/>
	<skos:editorialNote xml:lang="en">PPRefiningObjectType</skos:editorialNote>
	<skos:scopeNote xml:lang="en">Pages on the right-hand side, recto of a leaf, at the beginning of a book where the bibliographic information about the work is provided, displaying the book's title and usually the author's name, the publisher, and sometimes the date of publication. Where more than one page giving particulars of the title are present, that giving the fullest information is the title page.</skos:scopeNote>
</skos:Concept>
<skos:Concept rdf:about="http://partage.vocnet.org/part01200">
	<skos:prefLabel xml:lang="en">pages</skos:prefLabel>
	<skos:inScheme rdf:resource="http://partage.vocnet.org/Objects"/>
	<skos:broader rdf:resource="http://partage.vocnet.org/part00116"/>
	<skos:narrower rdf:resource="http://partage.vocnet.org/part01199"/>
	<skos:exactMatch rdf:resource="http://vocab.getty.edu/aat/300194222"/>
	<skos:scopeNote xml:lang="en">Individual sides of a leaf, recto or verso; the individual sides of leaves resulting from folding a sheet, as of paper or parchment, whether blank or containing writing, printing, or other matter. Distinguished from a "folio" in that a folio is numbered on only the front side.</skos:scopeNote>
</skos:Concept>
<skos:Concept rdf:about="http://partage.vocnet.org/part01201">
	<skos:prefLabel xml:lang="en">figures (representations)</skos:prefLabel>
	<skos:inScheme rdf:resource="http://partage.vocnet.org/Objects"/>
	<skos:narrower rdf:resource="http://partage.vocnet.org/part01146"/>
	<skos:exactMatch rdf:resource="http://vocab.getty.edu/aat/300189808"/>
</skos:Concept>
<skos:Concept rdf:about="http://partage.vocnet.org/part01228">
	<skos:prefLabel xml:lang="en">slipware</skos:prefLabel>
	<skos:inScheme rdf:resource="http://partage.vocnet.org/Objects"/>
	<skos:broader rdf:resource="http://partage.vocnet.org/part00224"/>
	<skos:exactMatch rdf:resource="http://vocab.getty.edu/aat/300264955"/>
	<skos:scopeNote xml:lang="en">A general term for wares decorated predominantly with one or more clay slips of greater or lesser iron content than the body clay. The slip clays fire to a contrasting color or shade from that of the body. Slipware can be decorated by pouring, dipping, painting, daubing or trailing slips on to the unfired, or sometimes once-fired, body. After it is applied, the slip can be manipulated by twisting the piece, by combing or feathering the slip into more regular designs or, after drying to a tacky consistency, can be carved in the sgraffito technique. Dipping, trailing, and marbling are other common techniques used for slip-decorated ceramics. The application of slip almost always precedes glazing.</skos:scopeNote>
</skos:Concept>
<skos:Concept rdf:about="http://partage.vocnet.org/part01237">
	<skos:prefLabel xml:lang="hr">ferotipija</skos:prefLabel>
	<skos:altLabel xml:lang="de">Ferrotypien</skos:altLabel>
	<skos:prefLabel xml:lang="de">Ferrotypie</skos:prefLabel>
	<skos:prefLabel xml:lang="en">tintypes (prints)</skos:prefLabel>
	<skos:altLabel xml:lang="en">ferrotypes (prints)</skos:altLabel>
	<skos:inScheme rdf:resource="http://partage.vocnet.org/Objects"/>
	<skos:broader rdf:resource="http://partage.vocnet.org/part01238"/>
	<skos:exactMatch rdf:resource="http://vocab.getty.edu/aat/300134759"/>
	<skos:editorialNote xml:lang="en">PPRefiningObjectType</skos:editorialNote>
	<skos:scopeNote xml:lang="en">Photographs produced by the wet collodion process directly on lacquered metal, usually iron.</skos:scopeNote>
</skos:Concept>
<skos:Concept rdf:about="http://partage.vocnet.org/part01238">
	<skos:prefLabel xml:lang="en">direct positives</skos:prefLabel>
	<skos:inScheme rdf:resource="http://partage.vocnet.org/Objects"/>
	<skos:broader rdf:resource="http://partage.vocnet.org/part00918"/>
	<skos:narrower rdf:resource="http://partage.vocnet.org/part01237"/>
	<skos:exactMatch rdf:resource="http://vocab.getty.edu/aat/300127180"/>
	<skos:scopeNote xml:lang="en">Positive-image photographs produced in the camera without the intervening use of a negative, or produced by a positive-to-positive process.</skos:scopeNote>
</skos:Concept>
<skos:Concept rdf:about="http://partage.vocnet.org/part01244">
	<skos:prefLabel xml:lang="hr">heliogravura</skos:prefLabel>
	<skos:prefLabel xml:lang="de">Heliogravure</skos:prefLabel>
	<skos:prefLabel xml:lang="en">photoaquatints (prints)</skos:prefLabel>
	<skos:inScheme rdf:resource="http://partage.vocnet.org/Objects"/>
	<skos:broader rdf:resource="http://partage.vocnet.org/part01259"/>
	<skos:exactMatch rdf:resource="http://vocab.getty.edu/aat/300264707"/>
	<skos:editorialNote xml:lang="en">PPRefiningObjectType</skos:editorialNote>
	<skos:scopeNote xml:lang="en">Photogravures differing from the ordinary type in that they are made using an aquatint grain and only one density of etching.</skos:scopeNote>
</skos:Concept>
<skos:Concept rdf:about="http://partage.vocnet.org/part01245">
	<skos:altLabel xml:lang="de">Schabkunstblätter</skos:altLabel>
	<skos:prefLabel xml:lang="de">Schabkunstblatt</skos:prefLabel>
	<skos:prefLabel xml:lang="hr">mezzotinta</skos:prefLabel>
	<skos:prefLabel xml:lang="en">mezzotints (prints)</skos:prefLabel>
	<skos:altLabel xml:lang="de">Schwarzkunst</skos:altLabel>
	<skos:altLabel xml:lang="de">Mezzotinto</skos:altLabel>
	<skos:inScheme rdf:resource="http://partage.vocnet.org/Objects"/>
	<skos:broader rdf:resource="http://partage.vocnet.org/part00820"/>
	<skos:exactMatch rdf:resource="http://vocab.getty.edu/aat/300041356"/>
	<skos:editorialNote xml:lang="en">PPRefiningObjectType</skos:editorialNote>
	<skos:scopeNote xml:lang="en">Prints made using the mezzotint process, in which the surface of the plate is methodically roughened with a rocker to produce a dark background; areas may then be lightened using various scrapers.</skos:scopeNote>
</skos:Concept>
<skos:Concept rdf:about="http://partage.vocnet.org/part01259">
	<skos:prefLabel xml:lang="en">photogravures (prints)</skos:prefLabel>
	<skos:inScheme rdf:resource="http://partage.vocnet.org/Objects"/>
	<skos:broader rdf:resource="http://partage.vocnet.org/part00944"/>
	<skos:narrower rdf:resource="http://partage.vocnet.org/part01244"/>
	<skos:exactMatch rdf:resource="http://vocab.getty.edu/aat/300154382"/>
	<skos:scopeNote xml:lang="en">Photomechanical prints produced by the process called photogravure, in which the metal printing plate is prepared using a bichromate process, leaving a gelatin resist of varying thickness. The plate is etched to form cells of varying depth able to hold different amounts of ink. If done with an aquatint grain, use "photoaquatints.".</skos:scopeNote>
</skos:Concept>
<skos:Collection rdf:about="http://partage.vocnet.org/PPObjectType">
	<skos:prefLabel>PPObjectType</skos:prefLabel>
	<skos:member rdf:resource="http://partage.vocnet.org/part00036"/>
	<skos:member rdf:resource="http://partage.vocnet.org/part00040"/>
	<skos:member rdf:resource="http://partage.vocnet.org/part00041"/>
	<skos:member rdf:resource="http://partage.vocnet.org/part00042"/>
	<skos:member rdf:resource="http://partage.vocnet.org/part00043"/>
	<skos:member rdf:resource="http://partage.vocnet.org/part00044"/>
	<skos:member rdf:resource="http://partage.vocnet.org/part00046"/>
	<skos:member rdf:resource="http://partage.vocnet.org/part00047"/>
	<skos:member rdf:resource="http://partage.vocnet.org/part00048"/>
	<skos:member rdf:resource="http://partage.vocnet.org/part00052"/>
	<skos:member rdf:resource="http://partage.vocnet.org/part00055"/>
	<skos:member rdf:resource="http://partage.vocnet.org/part00056"/>
	<skos:member rdf:resource="http://partage.vocnet.org/part00059"/>
	<skos:member rdf:resource="http://partage.vocnet.org/part00060"/>
	<skos:member rdf:resource="http://partage.vocnet.org/part00061"/>
	<skos:member rdf:resource="http://partage.vocnet.org/part00062"/>
	<skos:member rdf:resource="http://partage.vocnet.org/part00063"/>
	<skos:member rdf:resource="http://partage.vocnet.org/part00064"/>
	<skos:member rdf:resource="http://partage.vocnet.org/part00066"/>
	<skos:member rdf:resource="http://partage.vocnet.org/part00078"/>
	<skos:member rdf:resource="http://partage.vocnet.org/part00081"/>
	<skos:member rdf:resource="http://partage.vocnet.org/part00087"/>
	<skos:member rdf:resource="http://partage.vocnet.org/part00094"/>
	<skos:member rdf:resource="http://partage.vocnet.org/part00099"/>
	<skos:member rdf:resource="http://partage.vocnet.org/part00100"/>
	<skos:member rdf:resource="http://partage.vocnet.org/part00109"/>
	<skos:member rdf:resource="http://partage.vocnet.org/part00128"/>
	<skos:member rdf:resource="http://partage.vocnet.org/part00139"/>
	<skos:member rdf:resource="http://partage.vocnet.org/part00151"/>
	<skos:member rdf:resource="http://partage.vocnet.org/part00177"/>
	<skos:member rdf:resource="http://partage.vocnet.org/part00181"/>
	<skos:member rdf:resource="http://partage.vocnet.org/part00185"/>
	<skos:member rdf:resource="http://partage.vocnet.org/part00218"/>
	<skos:member rdf:resource="http://partage.vocnet.org/part00221"/>
	<skos:member rdf:resource="http://partage.vocnet.org/part00222"/>
	<skos:member rdf:resource="http://partage.vocnet.org/part00223"/>
	<skos:member rdf:resource="http://partage.vocnet.org/part00225"/>
	<skos:member rdf:resource="http://partage.vocnet.org/part00226"/>
	<skos:member rdf:resource="http://partage.vocnet.org/part00249"/>
	<skos:member rdf:resource="http://partage.vocnet.org/part00419"/>
	<skos:member rdf:resource="http://partage.vocnet.org/part00470"/>
	<skos:member rdf:resource="http://partage.vocnet.org/part00498"/>
	<skos:member rdf:resource="http://partage.vocnet.org/part00501"/>
	<skos:member rdf:resource="http://partage.vocnet.org/part00502"/>
	<skos:member rdf:resource="http://partage.vocnet.org/part00505"/>
	<skos:member rdf:resource="http://partage.vocnet.org/part00510"/>
	<skos:member rdf:resource="http://partage.vocnet.org/part00511"/>
	<skos:member rdf:resource="http://partage.vocnet.org/part00512"/>
	<skos:member rdf:resource="http://partage.vocnet.org/part00513"/>
</skos:Collection>
<skos:Collection rdf:about="http://partage.vocnet.org/PPRefiningObjectType">
	<skos:prefLabel>PPRefiningObjectType</skos:prefLabel>
	<skos:member rdf:resource="http://partage.vocnet.org/part00053"/>
	<skos:member rdf:resource="http://partage.vocnet.org/part00072"/>
	<skos:member rdf:resource="http://partage.vocnet.org/part00075"/>
	<skos:member rdf:resource="http://partage.vocnet.org/part00080"/>
	<skos:member rdf:resource="http://partage.vocnet.org/part00083"/>
	<skos:member rdf:resource="http://partage.vocnet.org/part00085"/>
	<skos:member rdf:resource="http://partage.vocnet.org/part00091"/>
	<skos:member rdf:resource="http://partage.vocnet.org/part00102"/>
	<skos:member rdf:resource="http://partage.vocnet.org/part00110"/>
	<skos:member rdf:resource="http://partage.vocnet.org/part00118"/>
	<skos:member rdf:resource="http://partage.vocnet.org/part00127"/>
	<skos:member rdf:resource="http://partage.vocnet.org/part00133"/>
	<skos:member rdf:resource="http://partage.vocnet.org/part00134"/>
	<skos:member rdf:resource="http://partage.vocnet.org/part00135"/>
	<skos:member rdf:resource="http://partage.vocnet.org/part00136"/>
	<skos:member rdf:resource="http://partage.vocnet.org/part00140"/>
	<skos:member rdf:resource="http://partage.vocnet.org/part00141"/>
	<skos:member rdf:resource="http://partage.vocnet.org/part00142"/>
	<skos:member rdf:resource="http://partage.vocnet.org/part00152"/>
	<skos:member rdf:resource="http://partage.vocnet.org/part00153"/>
	<skos:member rdf:resource="http://partage.vocnet.org/part00155"/>
	<skos:member rdf:resource="http://partage.vocnet.org/part00156"/>
	<skos:member rdf:resource="http://partage.vocnet.org/part00160"/>
	<skos:member rdf:resource="http://partage.vocnet.org/part00163"/>
	<skos:member rdf:resource="http://partage.vocnet.org/part00164"/>
	<skos:member rdf:resource="http://partage.vocnet.org/part00165"/>
	<skos:member rdf:resource="http://partage.vocnet.org/part00166"/>
	<skos:member rdf:resource="http://partage.vocnet.org/part00167"/>
	<skos:member rdf:resource="http://partage.vocnet.org/part00171"/>
	<skos:member rdf:resource="http://partage.vocnet.org/part00172"/>
	<skos:member rdf:resource="http://partage.vocnet.org/part00180"/>
	<skos:member rdf:resource="http://partage.vocnet.org/part00184"/>
	<skos:member rdf:resource="http://partage.vocnet.org/part00188"/>
	<skos:member rdf:resource="http://partage.vocnet.org/part00190"/>
	<skos:member rdf:resource="http://partage.vocnet.org/part00191"/>
	<skos:member rdf:resource="http://partage.vocnet.org/part00193"/>
	<skos:member rdf:resource="http://partage.vocnet.org/part00195"/>
	<skos:member rdf:resource="http://partage.vocnet.org/part00196"/>
	<skos:member rdf:resource="http://partage.vocnet.org/part00197"/>
	<skos:member rdf:resource="http://partage.vocnet.org/part00198"/>
	<skos:member rdf:resource="http://partage.vocnet.org/part00200"/>
	<skos:member rdf:resource="http://partage.vocnet.org/part00213"/>
	<skos:member rdf:resource="http://partage.vocnet.org/part00215"/>
	<skos:member rdf:resource="http://partage.vocnet.org/part00219"/>
	<skos:member rdf:resource="http://partage.vocnet.org/part00299"/>
	<skos:member rdf:resource="http://partage.vocnet.org/part00301"/>
	<skos:member rdf:resource="http://partage.vocnet.org/part00302"/>
	<skos:member rdf:resource="http://partage.vocnet.org/part00303"/>
	<skos:member rdf:resource="http://partage.vocnet.org/part00304"/>
	<skos:member rdf:resource="http://partage.vocnet.org/part00305"/>
	<skos:member rdf:resource="http://partage.vocnet.org/part00306"/>
	<skos:member rdf:resource="http://partage.vocnet.org/part00308"/>
	<skos:member rdf:resource="http://partage.vocnet.org/part00309"/>
	<skos:member rdf:resource="http://partage.vocnet.org/part00311"/>
	<skos:member rdf:resource="http://partage.vocnet.org/part00312"/>
	<skos:member rdf:resource="http://partage.vocnet.org/part00314"/>
	<skos:member rdf:resource="http://partage.vocnet.org/part00315"/>
	<skos:member rdf:resource="http://partage.vocnet.org/part00316"/>
	<skos:member rdf:resource="http://partage.vocnet.org/part00318"/>
	<skos:member rdf:resource="http://partage.vocnet.org/part00319"/>
	<skos:member rdf:resource="http://partage.vocnet.org/part00320"/>
	<skos:member rdf:resource="http://partage.vocnet.org/part00321"/>
	<skos:member rdf:resource="http://partage.vocnet.org/part00322"/>
	<skos:member rdf:resource="http://partage.vocnet.org/part00323"/>
	<skos:member rdf:resource="http://partage.vocnet.org/part00325"/>
	<skos:member rdf:resource="http://partage.vocnet.org/part00326"/>
	<skos:member rdf:resource="http://partage.vocnet.org/part00327"/>
	<skos:member rdf:resource="http://partage.vocnet.org/part00330"/>
	<skos:member rdf:resource="http://partage.vocnet.org/part00331"/>
	<skos:member rdf:resource="http://partage.vocnet.org/part00332"/>
	<skos:member rdf:resource="http://partage.vocnet.org/part00334"/>
	<skos:member rdf:resource="http://partage.vocnet.org/part00335"/>
	<skos:member rdf:resource="http://partage.vocnet.org/part00338"/>
	<skos:member rdf:resource="http://partage.vocnet.org/part00339"/>
	<skos:member rdf:resource="http://partage.vocnet.org/part00396"/>
	<skos:member rdf:resource="http://partage.vocnet.org/part00400"/>
	<skos:member rdf:resource="http://partage.vocnet.org/part00401"/>
	<skos:member rdf:resource="http://partage.vocnet.org/part00402"/>
	<skos:member rdf:resource="http://partage.vocnet.org/part00403"/>
	<skos:member rdf:resource="http://partage.vocnet.org/part00404"/>
	<skos:member rdf:resource="http://partage.vocnet.org/part00410"/>
	<skos:member rdf:resource="http://partage.vocnet.org/part00412"/>
	<skos:member rdf:resource="http://partage.vocnet.org/part00413"/>
	<skos:member rdf:resource="http://partage.vocnet.org/part00415"/>
	<skos:member rdf:resource="http://partage.vocnet.org/part00465"/>
	<skos:member rdf:resource="http://partage.vocnet.org/part00528"/>
	<skos:member rdf:resource="http://partage.vocnet.org/part00560"/>
	<skos:member rdf:resource="http://partage.vocnet.org/part00562"/>
	<skos:member rdf:resource="http://partage.vocnet.org/part00676"/>
	<skos:member rdf:resource="http://partage.vocnet.org/part00677"/>
	<skos:member rdf:resource="http://partage.vocnet.org/part00678"/>
	<skos:member rdf:resource="http://partage.vocnet.org/part00679"/>
	<skos:member rdf:resource="http://partage.vocnet.org/part00680"/>
	<skos:member rdf:resource="http://partage.vocnet.org/part00681"/>
	<skos:member rdf:resource="http://partage.vocnet.org/part00682"/>
	<skos:member rdf:resource="http://partage.vocnet.org/part00683"/>
	<skos:member rdf:resource="http://partage.vocnet.org/part00684"/>
	<skos:member rdf:resource="http://partage.vocnet.org/part00685"/>
	<skos:member rdf:resource="http://partage.vocnet.org/part00686"/>
	<skos:member rdf:resource="http://partage.vocnet.org/part00688"/>
	<skos:member rdf:resource="http://partage.vocnet.org/part00689"/>
	<skos:member rdf:resource="http://partage.vocnet.org/part00690"/>
	<skos:member rdf:resource="http://partage.vocnet.org/part00691"/>
	<skos:member rdf:resource="http://partage.vocnet.org/part00692"/>
	<skos:member rdf:resource="http://partage.vocnet.org/part00693"/>
	<skos:member rdf:resource="http://partage.vocnet.org/part00694"/>
	<skos:member rdf:resource="http://partage.vocnet.org/part00695"/>
	<skos:member rdf:resource="http://partage.vocnet.org/part00696"/>
	<skos:member rdf:resource="http://partage.vocnet.org/part00697"/>
	<skos:member rdf:resource="http://partage.vocnet.org/part00698"/>
	<skos:member rdf:resource="http://partage.vocnet.org/part00699"/>
	<skos:member rdf:resource="http://partage.vocnet.org/part00700"/>
	<skos:member rdf:resource="http://partage.vocnet.org/part00701"/>
	<skos:member rdf:resource="http://partage.vocnet.org/part00702"/>
	<skos:member rdf:resource="http://partage.vocnet.org/part00703"/>
	<skos:member rdf:resource="http://partage.vocnet.org/part00704"/>
	<skos:member rdf:resource="http://partage.vocnet.org/part00705"/>
	<skos:member rdf:resource="http://partage.vocnet.org/part00706"/>
	<skos:member rdf:resource="http://partage.vocnet.org/part00707"/>
	<skos:member rdf:resource="http://partage.vocnet.org/part00708"/>
	<skos:member rdf:resource="http://partage.vocnet.org/part00709"/>
	<skos:member rdf:resource="http://partage.vocnet.org/part00710"/>
	<skos:member rdf:resource="http://partage.vocnet.org/part00711"/>
	<skos:member rdf:resource="http://partage.vocnet.org/part00712"/>
	<skos:member rdf:resource="http://partage.vocnet.org/part00713"/>
	<skos:member rdf:resource="http://partage.vocnet.org/part00714"/>
	<skos:member rdf:resource="http://partage.vocnet.org/part00715"/>
	<skos:member rdf:resource="http://partage.vocnet.org/part00716"/>
	<skos:member rdf:resource="http://partage.vocnet.org/part00717"/>
	<skos:member rdf:resource="http://partage.vocnet.org/part00718"/>
	<skos:member rdf:resource="http://partage.vocnet.org/part00719"/>
	<skos:member rdf:resource="http://partage.vocnet.org/part00720"/>
	<skos:member rdf:resource="http://partage.vocnet.org/part00721"/>
	<skos:member rdf:resource="http://partage.vocnet.org/part00722"/>
	<skos:member rdf:resource="http://partage.vocnet.org/part00723"/>
	<skos:member rdf:resource="http://partage.vocnet.org/part00724"/>
	<skos:member rdf:resource="http://partage.vocnet.org/part00725"/>
	<skos:member rdf:resource="http://partage.vocnet.org/part00726"/>
	<skos:member rdf:resource="http://partage.vocnet.org/part00727"/>
	<skos:member rdf:resource="http://partage.vocnet.org/part00728"/>
	<skos:member rdf:resource="http://partage.vocnet.org/part00729"/>
	<skos:member rdf:resource="http://partage.vocnet.org/part00730"/>
	<skos:member rdf:resource="http://partage.vocnet.org/part00731"/>
	<skos:member rdf:resource="http://partage.vocnet.org/part00732"/>
	<skos:member rdf:resource="http://partage.vocnet.org/part00733"/>
	<skos:member rdf:resource="http://partage.vocnet.org/part00734"/>
	<skos:member rdf:resource="http://partage.vocnet.org/part00735"/>
	<skos:member rdf:resource="http://partage.vocnet.org/part00736"/>
	<skos:member rdf:resource="http://partage.vocnet.org/part00737"/>
	<skos:member rdf:resource="http://partage.vocnet.org/part00738"/>
	<skos:member rdf:resource="http://partage.vocnet.org/part00739"/>
	<skos:member rdf:resource="http://partage.vocnet.org/part00740"/>
	<skos:member rdf:resource="http://partage.vocnet.org/part00741"/>
	<skos:member rdf:resource="http://partage.vocnet.org/part00742"/>
	<skos:member rdf:resource="http://partage.vocnet.org/part00743"/>
	<skos:member rdf:resource="http://partage.vocnet.org/part00744"/>
	<skos:member rdf:resource="http://partage.vocnet.org/part00745"/>
	<skos:member rdf:resource="http://partage.vocnet.org/part00746"/>
	<skos:member rdf:resource="http://partage.vocnet.org/part00747"/>
	<skos:member rdf:resource="http://partage.vocnet.org/part00748"/>
	<skos:member rdf:resource="http://partage.vocnet.org/part00749"/>
	<skos:member rdf:resource="http://partage.vocnet.org/part00750"/>
	<skos:member rdf:resource="http://partage.vocnet.org/part00751"/>
	<skos:member rdf:resource="http://partage.vocnet.org/part00752"/>
	<skos:member rdf:resource="http://partage.vocnet.org/part00753"/>
	<skos:member rdf:resource="http://partage.vocnet.org/part00754"/>
	<skos:member rdf:resource="http://partage.vocnet.org/part00755"/>
	<skos:member rdf:resource="http://partage.vocnet.org/part00756"/>
	<skos:member rdf:resource="http://partage.vocnet.org/part00757"/>
	<skos:member rdf:resource="http://partage.vocnet.org/part00758"/>
	<skos:member rdf:resource="http://partage.vocnet.org/part00759"/>
	<skos:member rdf:resource="http://partage.vocnet.org/part00760"/>
	<skos:member rdf:resource="http://partage.vocnet.org/part00761"/>
	<skos:member rdf:resource="http://partage.vocnet.org/part00762"/>
	<skos:member rdf:resource="http://partage.vocnet.org/part00763"/>
	<skos:member rdf:resource="http://partage.vocnet.org/part00764"/>
	<skos:member rdf:resource="http://partage.vocnet.org/part00765"/>
	<skos:member rdf:resource="http://partage.vocnet.org/part00766"/>
	<skos:member rdf:resource="http://partage.vocnet.org/part00767"/>
	<skos:member rdf:resource="http://partage.vocnet.org/part00768"/>
	<skos:member rdf:resource="http://partage.vocnet.org/part00769"/>
	<skos:member rdf:resource="http://partage.vocnet.org/part00770"/>
	<skos:member rdf:resource="http://partage.vocnet.org/part00771"/>
	<skos:member rdf:resource="http://partage.vocnet.org/part00772"/>
	<skos:member rdf:resource="http://partage.vocnet.org/part00773"/>
	<skos:member rdf:resource="http://partage.vocnet.org/part00774"/>
	<skos:member rdf:resource="http://partage.vocnet.org/part00775"/>
	<skos:member rdf:resource="http://partage.vocnet.org/part00776"/>
	<skos:member rdf:resource="http://partage.vocnet.org/part00777"/>
	<skos:member rdf:resource="http://partage.vocnet.org/part00778"/>
	<skos:member rdf:resource="http://partage.vocnet.org/part00779"/>
	<skos:member rdf:resource="http://partage.vocnet.org/part00780"/>
	<skos:member rdf:resource="http://partage.vocnet.org/part00781"/>
	<skos:member rdf:resource="http://partage.vocnet.org/part00782"/>
	<skos:member rdf:resource="http://partage.vocnet.org/part00783"/>
	<skos:member rdf:resource="http://partage.vocnet.org/part00784"/>
	<skos:member rdf:resource="http://partage.vocnet.org/part00785"/>
	<skos:member rdf:resource="http://partage.vocnet.org/part00786"/>
	<skos:member rdf:resource="http://partage.vocnet.org/part00787"/>
	<skos:member rdf:resource="http://partage.vocnet.org/part00788"/>
	<skos:member rdf:resource="http://partage.vocnet.org/part00789"/>
	<skos:member rdf:resource="http://partage.vocnet.org/part00790"/>
	<skos:member rdf:resource="http://partage.vocnet.org/part00791"/>
	<skos:member rdf:resource="http://partage.vocnet.org/part00792"/>
	<skos:member rdf:resource="http://partage.vocnet.org/part00793"/>
	<skos:member rdf:resource="http://partage.vocnet.org/part00794"/>
	<skos:member rdf:resource="http://partage.vocnet.org/part00795"/>
	<skos:member rdf:resource="http://partage.vocnet.org/part00796"/>
	<skos:member rdf:resource="http://partage.vocnet.org/part00797"/>
	<skos:member rdf:resource="http://partage.vocnet.org/part00798"/>
	<skos:member rdf:resource="http://partage.vocnet.org/part00799"/>
	<skos:member rdf:resource="http://partage.vocnet.org/part00800"/>
	<skos:member rdf:resource="http://partage.vocnet.org/part00801"/>
	<skos:member rdf:resource="http://partage.vocnet.org/part00802"/>
	<skos:member rdf:resource="http://partage.vocnet.org/part00803"/>
	<skos:member rdf:resource="http://partage.vocnet.org/part00804"/>
	<skos:member rdf:resource="http://partage.vocnet.org/part00805"/>
	<skos:member rdf:resource="http://partage.vocnet.org/part00806"/>
	<skos:member rdf:resource="http://partage.vocnet.org/part00807"/>
	<skos:member rdf:resource="http://partage.vocnet.org/part00808"/>
	<skos:member rdf:resource="http://partage.vocnet.org/part00809"/>
	<skos:member rdf:resource="http://partage.vocnet.org/part00810"/>
	<skos:member rdf:resource="http://partage.vocnet.org/part00811"/>
	<skos:member rdf:resource="http://partage.vocnet.org/part00812"/>
	<skos:member rdf:resource="http://partage.vocnet.org/part00813"/>
	<skos:member rdf:resource="http://partage.vocnet.org/part00814"/>
	<skos:member rdf:resource="http://partage.vocnet.org/part00815"/>
	<skos:member rdf:resource="http://partage.vocnet.org/part00816"/>
	<skos:member rdf:resource="http://partage.vocnet.org/part00817"/>
	<skos:member rdf:resource="http://partage.vocnet.org/part00818"/>
	<skos:member rdf:resource="http://partage.vocnet.org/part00819"/>
	<skos:member rdf:resource="http://partage.vocnet.org/part00820"/>
	<skos:member rdf:resource="http://partage.vocnet.org/part00821"/>
	<skos:member rdf:resource="http://partage.vocnet.org/part00822"/>
	<skos:member rdf:resource="http://partage.vocnet.org/part00823"/>
	<skos:member rdf:resource="http://partage.vocnet.org/part00825"/>
	<skos:member rdf:resource="http://partage.vocnet.org/part00826"/>
	<skos:member rdf:resource="http://partage.vocnet.org/part00827"/>
	<skos:member rdf:resource="http://partage.vocnet.org/part00828"/>
	<skos:member rdf:resource="http://partage.vocnet.org/part00829"/>
	<skos:member rdf:resource="http://partage.vocnet.org/part00830"/>
	<skos:member rdf:resource="http://partage.vocnet.org/part00831"/>
	<skos:member rdf:resource="http://partage.vocnet.org/part00833"/>
	<skos:member rdf:resource="http://partage.vocnet.org/part00834"/>
	<skos:member rdf:resource="http://partage.vocnet.org/part00835"/>
	<skos:member rdf:resource="http://partage.vocnet.org/part00876"/>
	<skos:member rdf:resource="http://partage.vocnet.org/part00882"/>
	<skos:member rdf:resource="http://partage.vocnet.org/part00883"/>
	<skos:member rdf:resource="http://partage.vocnet.org/part00884"/>
	<skos:member rdf:resource="http://partage.vocnet.org/part00885"/>
	<skos:member rdf:resource="http://partage.vocnet.org/part00886"/>
	<skos:member rdf:resource="http://partage.vocnet.org/part00887"/>
	<skos:member rdf:resource="http://partage.vocnet.org/part00888"/>
	<skos:member rdf:resource="http://partage.vocnet.org/part00890"/>
	<skos:member rdf:resource="http://partage.vocnet.org/part00891"/>
	<skos:member rdf:resource="http://partage.vocnet.org/part00892"/>
	<skos:member rdf:resource="http://partage.vocnet.org/part00893"/>
	<skos:member rdf:resource="http://partage.vocnet.org/part00894"/>
	<skos:member rdf:resource="http://partage.vocnet.org/part00895"/>
	<skos:member rdf:resource="http://partage.vocnet.org/part00896"/>
	<skos:member rdf:resource="http://partage.vocnet.org/part00904"/>
	<skos:member rdf:resource="http://partage.vocnet.org/part00914"/>
	<skos:member rdf:resource="http://partage.vocnet.org/part00974"/>
	<skos:member rdf:resource="http://partage.vocnet.org/part01066"/>
	<skos:member rdf:resource="http://partage.vocnet.org/part01120"/>
	<skos:member rdf:resource="http://partage.vocnet.org/part01122"/>
	<skos:member rdf:resource="http://partage.vocnet.org/part01123"/>
	<skos:member rdf:resource="http://partage.vocnet.org/part01125"/>
	<skos:member rdf:resource="http://partage.vocnet.org/part01127"/>
	<skos:member rdf:resource="http://partage.vocnet.org/part01129"/>
	<skos:member rdf:resource="http://partage.vocnet.org/part01134"/>
	<skos:member rdf:resource="http://partage.vocnet.org/part01135"/>
	<skos:member rdf:resource="http://partage.vocnet.org/part01136"/>
	<skos:member rdf:resource="http://partage.vocnet.org/part01137"/>
	<skos:member rdf:resource="http://partage.vocnet.org/part01141"/>
	<skos:member rdf:resource="http://partage.vocnet.org/part01144"/>
	<skos:member rdf:resource="http://partage.vocnet.org/part01155"/>
	<skos:member rdf:resource="http://partage.vocnet.org/part01157"/>
	<skos:member rdf:resource="http://partage.vocnet.org/part01158"/>
	<skos:member rdf:resource="http://partage.vocnet.org/part01160"/>
	<skos:member rdf:resource="http://partage.vocnet.org/part01161"/>
	<skos:member rdf:resource="http://partage.vocnet.org/part01162"/>
	<skos:member rdf:resource="http://partage.vocnet.org/part01163"/>
	<skos:member rdf:resource="http://partage.vocnet.org/part01164"/>
	<skos:member rdf:resource="http://partage.vocnet.org/part01168"/>
	<skos:member rdf:resource="http://partage.vocnet.org/part01169"/>
	<skos:member rdf:resource="http://partage.vocnet.org/part01170"/>
	<skos:member rdf:resource="http://partage.vocnet.org/part01171"/>
	<skos:member rdf:resource="http://partage.vocnet.org/part01172"/>
	<skos:member rdf:resource="http://partage.vocnet.org/part01175"/>
	<skos:member rdf:resource="http://partage.vocnet.org/part01177"/>
	<skos:member rdf:resource="http://partage.vocnet.org/part01178"/>
	<skos:member rdf:resource="http://partage.vocnet.org/part01179"/>
	<skos:member rdf:resource="http://partage.vocnet.org/part01180"/>
	<skos:member rdf:resource="http://partage.vocnet.org/part01181"/>
	<skos:member rdf:resource="http://partage.vocnet.org/part01182"/>
	<skos:member rdf:resource="http://partage.vocnet.org/part01184"/>
	<skos:member rdf:resource="http://partage.vocnet.org/part01185"/>
	<skos:member rdf:resource="http://partage.vocnet.org/part01188"/>
	<skos:member rdf:resource="http://partage.vocnet.org/part01189"/>
	<skos:member rdf:resource="http://partage.vocnet.org/part01190"/>
	<skos:member rdf:resource="http://partage.vocnet.org/part01191"/>
	<skos:member rdf:resource="http://partage.vocnet.org/part01192"/>
	<skos:member rdf:resource="http://partage.vocnet.org/part01193"/>
	<skos:member rdf:resource="http://partage.vocnet.org/part01194"/>
	<skos:member rdf:resource="http://partage.vocnet.org/part01198"/>
	<skos:member rdf:resource="http://partage.vocnet.org/part01199"/>
	<skos:member rdf:resource="http://partage.vocnet.org/part01237"/>
	<skos:member rdf:resource="http://partage.vocnet.org/part01244"/>
	<skos:member rdf:resource="http://partage.vocnet.org/part01245"/>
</skos:Collection>
<skos:Collection rdf:about="http://partage.vocnet.org/IndexingConcepts">
	<skos:prefLabel>IndexingConcepts</skos:prefLabel>
	<skos:member rdf:resource="http://partage.vocnet.org/part00036"/>
	<skos:member rdf:resource="http://partage.vocnet.org/part00040"/>
	<skos:member rdf:resource="http://partage.vocnet.org/part00041"/>
	<skos:member rdf:resource="http://partage.vocnet.org/part00042"/>
	<skos:member rdf:resource="http://partage.vocnet.org/part00043"/>
	<skos:member rdf:resource="http://partage.vocnet.org/part00044"/>
	<skos:member rdf:resource="http://partage.vocnet.org/part00046"/>
	<skos:member rdf:resource="http://partage.vocnet.org/part00047"/>
	<skos:member rdf:resource="http://partage.vocnet.org/part00048"/>
	<skos:member rdf:resource="http://partage.vocnet.org/part00052"/>
	<skos:member rdf:resource="http://partage.vocnet.org/part00053"/>
	<skos:member rdf:resource="http://partage.vocnet.org/part00055"/>
	<skos:member rdf:resource="http://partage.vocnet.org/part00056"/>
	<skos:member rdf:resource="http://partage.vocnet.org/part00059"/>
	<skos:member rdf:resource="http://partage.vocnet.org/part00060"/>
	<skos:member rdf:resource="http://partage.vocnet.org/part00061"/>
	<skos:member rdf:resource="http://partage.vocnet.org/part00062"/>
	<skos:member rdf:resource="http://partage.vocnet.org/part00063"/>
	<skos:member rdf:resource="http://partage.vocnet.org/part00064"/>
	<skos:member rdf:resource="http://partage.vocnet.org/part00066"/>
	<skos:member rdf:resource="http://partage.vocnet.org/part00072"/>
	<skos:member rdf:resource="http://partage.vocnet.org/part00075"/>
	<skos:member rdf:resource="http://partage.vocnet.org/part00078"/>
	<skos:member rdf:resource="http://partage.vocnet.org/part00080"/>
	<skos:member rdf:resource="http://partage.vocnet.org/part00081"/>
	<skos:member rdf:resource="http://partage.vocnet.org/part00083"/>
	<skos:member rdf:resource="http://partage.vocnet.org/part00085"/>
	<skos:member rdf:resource="http://partage.vocnet.org/part00087"/>
	<skos:member rdf:resource="http://partage.vocnet.org/part00091"/>
	<skos:member rdf:resource="http://partage.vocnet.org/part00094"/>
	<skos:member rdf:resource="http://partage.vocnet.org/part00099"/>
	<skos:member rdf:resource="http://partage.vocnet.org/part00100"/>
	<skos:member rdf:resource="http://partage.vocnet.org/part00102"/>
	<skos:member rdf:resource="http://partage.vocnet.org/part00109"/>
	<skos:member rdf:resource="http://partage.vocnet.org/part00110"/>
	<skos:member rdf:resource="http://partage.vocnet.org/part00118"/>
	<skos:member rdf:resource="http://partage.vocnet.org/part00127"/>
	<skos:member rdf:resource="http://partage.vocnet.org/part00128"/>
	<skos:member rdf:resource="http://partage.vocnet.org/part00133"/>
	<skos:member rdf:resource="http://partage.vocnet.org/part00134"/>
	<skos:member rdf:resource="http://partage.vocnet.org/part00135"/>
	<skos:member rdf:resource="http://partage.vocnet.org/part00136"/>
	<skos:member rdf:resource="http://partage.vocnet.org/part00139"/>
	<skos:member rdf:resource="http://partage.vocnet.org/part00140"/>
	<skos:member rdf:resource="http://partage.vocnet.org/part00141"/>
	<skos:member rdf:resource="http://partage.vocnet.org/part00142"/>
	<skos:member rdf:resource="http://partage.vocnet.org/part00151"/>
	<skos:member rdf:resource="http://partage.vocnet.org/part00152"/>
	<skos:member rdf:resource="http://partage.vocnet.org/part00153"/>
	<skos:member rdf:resource="http://partage.vocnet.org/part00155"/>
	<skos:member rdf:resource="http://partage.vocnet.org/part00156"/>
	<skos:member rdf:resource="http://partage.vocnet.org/part00160"/>
	<skos:member rdf:resource="http://partage.vocnet.org/part00163"/>
	<skos:member rdf:resource="http://partage.vocnet.org/part00164"/>
	<skos:member rdf:resource="http://partage.vocnet.org/part00165"/>
	<skos:member rdf:resource="http://partage.vocnet.org/part00166"/>
	<skos:member rdf:resource="http://partage.vocnet.org/part00167"/>
	<skos:member rdf:resource="http://partage.vocnet.org/part00171"/>
	<skos:member rdf:resource="http://partage.vocnet.org/part00172"/>
	<skos:member rdf:resource="http://partage.vocnet.org/part00177"/>
	<skos:member rdf:resource="http://partage.vocnet.org/part00180"/>
	<skos:member rdf:resource="http://partage.vocnet.org/part00181"/>
	<skos:member rdf:resource="http://partage.vocnet.org/part00184"/>
	<skos:member rdf:resource="http://partage.vocnet.org/part00185"/>
	<skos:member rdf:resource="http://partage.vocnet.org/part00188"/>
	<skos:member rdf:resource="http://partage.vocnet.org/part00190"/>
	<skos:member rdf:resource="http://partage.vocnet.org/part00191"/>
	<skos:member rdf:resource="http://partage.vocnet.org/part00193"/>
	<skos:member rdf:resource="http://partage.vocnet.org/part00195"/>
	<skos:member rdf:resource="http://partage.vocnet.org/part00196"/>
	<skos:member rdf:resource="http://partage.vocnet.org/part00197"/>
	<skos:member rdf:resource="http://partage.vocnet.org/part00198"/>
	<skos:member rdf:resource="http://partage.vocnet.org/part00200"/>
	<skos:member rdf:resource="http://partage.vocnet.org/part00213"/>
	<skos:member rdf:resource="http://partage.vocnet.org/part00215"/>
	<skos:member rdf:resource="http://partage.vocnet.org/part00218"/>
	<skos:member rdf:resource="http://partage.vocnet.org/part00219"/>
	<skos:member rdf:resource="http://partage.vocnet.org/part00221"/>
	<skos:member rdf:resource="http://partage.vocnet.org/part00222"/>
	<skos:member rdf:resource="http://partage.vocnet.org/part00223"/>
	<skos:member rdf:resource="http://partage.vocnet.org/part00225"/>
	<skos:member rdf:resource="http://partage.vocnet.org/part00226"/>
	<skos:member rdf:resource="http://partage.vocnet.org/part00249"/>
	<skos:member rdf:resource="http://partage.vocnet.org/part00299"/>
	<skos:member rdf:resource="http://partage.vocnet.org/part00301"/>
	<skos:member rdf:resource="http://partage.vocnet.org/part00302"/>
	<skos:member rdf:resource="http://partage.vocnet.org/part00303"/>
	<skos:member rdf:resource="http://partage.vocnet.org/part00304"/>
	<skos:member rdf:resource="http://partage.vocnet.org/part00305"/>
	<skos:member rdf:resource="http://partage.vocnet.org/part00306"/>
	<skos:member rdf:resource="http://partage.vocnet.org/part00308"/>
	<skos:member rdf:resource="http://partage.vocnet.org/part00309"/>
	<skos:member rdf:resource="http://partage.vocnet.org/part00311"/>
	<skos:member rdf:resource="http://partage.vocnet.org/part00312"/>
	<skos:member rdf:resource="http://partage.vocnet.org/part00314"/>
	<skos:member rdf:resource="http://partage.vocnet.org/part00315"/>
	<skos:member rdf:resource="http://partage.vocnet.org/part00316"/>
	<skos:member rdf:resource="http://partage.vocnet.org/part00318"/>
	<skos:member rdf:resource="http://partage.vocnet.org/part00319"/>
	<skos:member rdf:resource="http://partage.vocnet.org/part00320"/>
	<skos:member rdf:resource="http://partage.vocnet.org/part00321"/>
	<skos:member rdf:resource="http://partage.vocnet.org/part00322"/>
	<skos:member rdf:resource="http://partage.vocnet.org/part00323"/>
	<skos:member rdf:resource="http://partage.vocnet.org/part00325"/>
	<skos:member rdf:resource="http://partage.vocnet.org/part00326"/>
	<skos:member rdf:resource="http://partage.vocnet.org/part00327"/>
	<skos:member rdf:resource="http://partage.vocnet.org/part00330"/>
	<skos:member rdf:resource="http://partage.vocnet.org/part00331"/>
	<skos:member rdf:resource="http://partage.vocnet.org/part00332"/>
	<skos:member rdf:resource="http://partage.vocnet.org/part00334"/>
	<skos:member rdf:resource="http://partage.vocnet.org/part00335"/>
	<skos:member rdf:resource="http://partage.vocnet.org/part00338"/>
	<skos:member rdf:resource="http://partage.vocnet.org/part00339"/>
	<skos:member rdf:resource="http://partage.vocnet.org/part00396"/>
	<skos:member rdf:resource="http://partage.vocnet.org/part00400"/>
	<skos:member rdf:resource="http://partage.vocnet.org/part00401"/>
	<skos:member rdf:resource="http://partage.vocnet.org/part00402"/>
	<skos:member rdf:resource="http://partage.vocnet.org/part00403"/>
	<skos:member rdf:resource="http://partage.vocnet.org/part00404"/>
	<skos:member rdf:resource="http://partage.vocnet.org/part00410"/>
	<skos:member rdf:resource="http://partage.vocnet.org/part00412"/>
	<skos:member rdf:resource="http://partage.vocnet.org/part00413"/>
	<skos:member rdf:resource="http://partage.vocnet.org/part00415"/>
	<skos:member rdf:resource="http://partage.vocnet.org/part00419"/>
	<skos:member rdf:resource="http://partage.vocnet.org/part00465"/>
	<skos:member rdf:resource="http://partage.vocnet.org/part00470"/>
	<skos:member rdf:resource="http://partage.vocnet.org/part00498"/>
	<skos:member rdf:resource="http://partage.vocnet.org/part00501"/>
	<skos:member rdf:resource="http://partage.vocnet.org/part00502"/>
	<skos:member rdf:resource="http://partage.vocnet.org/part00505"/>
	<skos:member rdf:resource="http://partage.vocnet.org/part00510"/>
	<skos:member rdf:resource="http://partage.vocnet.org/part00511"/>
	<skos:member rdf:resource="http://partage.vocnet.org/part00512"/>
	<skos:member rdf:resource="http://partage.vocnet.org/part00513"/>
	<skos:member rdf:resource="http://partage.vocnet.org/part00528"/>
	<skos:member rdf:resource="http://partage.vocnet.org/part00560"/>
	<skos:member rdf:resource="http://partage.vocnet.org/part00562"/>
	<skos:member rdf:resource="http://partage.vocnet.org/part00676"/>
	<skos:member rdf:resource="http://partage.vocnet.org/part00677"/>
	<skos:member rdf:resource="http://partage.vocnet.org/part00678"/>
	<skos:member rdf:resource="http://partage.vocnet.org/part00679"/>
	<skos:member rdf:resource="http://partage.vocnet.org/part00680"/>
	<skos:member rdf:resource="http://partage.vocnet.org/part00681"/>
	<skos:member rdf:resource="http://partage.vocnet.org/part00682"/>
	<skos:member rdf:resource="http://partage.vocnet.org/part00683"/>
	<skos:member rdf:resource="http://partage.vocnet.org/part00684"/>
	<skos:member rdf:resource="http://partage.vocnet.org/part00685"/>
	<skos:member rdf:resource="http://partage.vocnet.org/part00686"/>
	<skos:member rdf:resource="http://partage.vocnet.org/part00688"/>
	<skos:member rdf:resource="http://partage.vocnet.org/part00689"/>
	<skos:member rdf:resource="http://partage.vocnet.org/part00690"/>
	<skos:member rdf:resource="http://partage.vocnet.org/part00691"/>
	<skos:member rdf:resource="http://partage.vocnet.org/part00692"/>
	<skos:member rdf:resource="http://partage.vocnet.org/part00693"/>
	<skos:member rdf:resource="http://partage.vocnet.org/part00694"/>
	<skos:member rdf:resource="http://partage.vocnet.org/part00695"/>
	<skos:member rdf:resource="http://partage.vocnet.org/part00696"/>
	<skos:member rdf:resource="http://partage.vocnet.org/part00697"/>
	<skos:member rdf:resource="http://partage.vocnet.org/part00698"/>
	<skos:member rdf:resource="http://partage.vocnet.org/part00699"/>
	<skos:member rdf:resource="http://partage.vocnet.org/part00700"/>
	<skos:member rdf:resource="http://partage.vocnet.org/part00701"/>
	<skos:member rdf:resource="http://partage.vocnet.org/part00702"/>
	<skos:member rdf:resource="http://partage.vocnet.org/part00703"/>
	<skos:member rdf:resource="http://partage.vocnet.org/part00704"/>
	<skos:member rdf:resource="http://partage.vocnet.org/part00705"/>
	<skos:member rdf:resource="http://partage.vocnet.org/part00706"/>
	<skos:member rdf:resource="http://partage.vocnet.org/part00707"/>
	<skos:member rdf:resource="http://partage.vocnet.org/part00708"/>
	<skos:member rdf:resource="http://partage.vocnet.org/part00709"/>
	<skos:member rdf:resource="http://partage.vocnet.org/part00710"/>
	<skos:member rdf:resource="http://partage.vocnet.org/part00711"/>
	<skos:member rdf:resource="http://partage.vocnet.org/part00712"/>
	<skos:member rdf:resource="http://partage.vocnet.org/part00713"/>
	<skos:member rdf:resource="http://partage.vocnet.org/part00714"/>
	<skos:member rdf:resource="http://partage.vocnet.org/part00715"/>
	<skos:member rdf:resource="http://partage.vocnet.org/part00716"/>
	<skos:member rdf:resource="http://partage.vocnet.org/part00717"/>
	<skos:member rdf:resource="http://partage.vocnet.org/part00718"/>
	<skos:member rdf:resource="http://partage.vocnet.org/part00719"/>
	<skos:member rdf:resource="http://partage.vocnet.org/part00720"/>
	<skos:member rdf:resource="http://partage.vocnet.org/part00721"/>
	<skos:member rdf:resource="http://partage.vocnet.org/part00722"/>
	<skos:member rdf:resource="http://partage.vocnet.org/part00723"/>
	<skos:member rdf:resource="http://partage.vocnet.org/part00724"/>
	<skos:member rdf:resource="http://partage.vocnet.org/part00725"/>
	<skos:member rdf:resource="http://partage.vocnet.org/part00726"/>
	<skos:member rdf:resource="http://partage.vocnet.org/part00727"/>
	<skos:member rdf:resource="http://partage.vocnet.org/part00728"/>
	<skos:member rdf:resource="http://partage.vocnet.org/part00729"/>
	<skos:member rdf:resource="http://partage.vocnet.org/part00730"/>
	<skos:member rdf:resource="http://partage.vocnet.org/part00731"/>
	<skos:member rdf:resource="http://partage.vocnet.org/part00732"/>
	<skos:member rdf:resource="http://partage.vocnet.org/part00733"/>
	<skos:member rdf:resource="http://partage.vocnet.org/part00734"/>
	<skos:member rdf:resource="http://partage.vocnet.org/part00735"/>
	<skos:member rdf:resource="http://partage.vocnet.org/part00736"/>
	<skos:member rdf:resource="http://partage.vocnet.org/part00737"/>
	<skos:member rdf:resource="http://partage.vocnet.org/part00738"/>
	<skos:member rdf:resource="http://partage.vocnet.org/part00739"/>
	<skos:member rdf:resource="http://partage.vocnet.org/part00740"/>
	<skos:member rdf:resource="http://partage.vocnet.org/part00741"/>
	<skos:member rdf:resource="http://partage.vocnet.org/part00742"/>
	<skos:member rdf:resource="http://partage.vocnet.org/part00743"/>
	<skos:member rdf:resource="http://partage.vocnet.org/part00744"/>
	<skos:member rdf:resource="http://partage.vocnet.org/part00745"/>
	<skos:member rdf:resource="http://partage.vocnet.org/part00746"/>
	<skos:member rdf:resource="http://partage.vocnet.org/part00747"/>
	<skos:member rdf:resource="http://partage.vocnet.org/part00748"/>
	<skos:member rdf:resource="http://partage.vocnet.org/part00749"/>
	<skos:member rdf:resource="http://partage.vocnet.org/part00750"/>
	<skos:member rdf:resource="http://partage.vocnet.org/part00751"/>
	<skos:member rdf:resource="http://partage.vocnet.org/part00752"/>
	<skos:member rdf:resource="http://partage.vocnet.org/part00753"/>
	<skos:member rdf:resource="http://partage.vocnet.org/part00754"/>
	<skos:member rdf:resource="http://partage.vocnet.org/part00755"/>
	<skos:member rdf:resource="http://partage.vocnet.org/part00756"/>
	<skos:member rdf:resource="http://partage.vocnet.org/part00757"/>
	<skos:member rdf:resource="http://partage.vocnet.org/part00758"/>
	<skos:member rdf:resource="http://partage.vocnet.org/part00759"/>
	<skos:member rdf:resource="http://partage.vocnet.org/part00760"/>
	<skos:member rdf:resource="http://partage.vocnet.org/part00761"/>
	<skos:member rdf:resource="http://partage.vocnet.org/part00762"/>
	<skos:member rdf:resource="http://partage.vocnet.org/part00763"/>
	<skos:member rdf:resource="http://partage.vocnet.org/part00764"/>
	<skos:member rdf:resource="http://partage.vocnet.org/part00765"/>
	<skos:member rdf:resource="http://partage.vocnet.org/part00766"/>
	<skos:member rdf:resource="http://partage.vocnet.org/part00767"/>
	<skos:member rdf:resource="http://partage.vocnet.org/part00768"/>
	<skos:member rdf:resource="http://partage.vocnet.org/part00769"/>
	<skos:member rdf:resource="http://partage.vocnet.org/part00770"/>
	<skos:member rdf:resource="http://partage.vocnet.org/part00771"/>
	<skos:member rdf:resource="http://partage.vocnet.org/part00772"/>
	<skos:member rdf:resource="http://partage.vocnet.org/part00773"/>
	<skos:member rdf:resource="http://partage.vocnet.org/part00774"/>
	<skos:member rdf:resource="http://partage.vocnet.org/part00775"/>
	<skos:member rdf:resource="http://partage.vocnet.org/part00776"/>
	<skos:member rdf:resource="http://partage.vocnet.org/part00777"/>
	<skos:member rdf:resource="http://partage.vocnet.org/part00778"/>
	<skos:member rdf:resource="http://partage.vocnet.org/part00779"/>
	<skos:member rdf:resource="http://partage.vocnet.org/part00780"/>
	<skos:member rdf:resource="http://partage.vocnet.org/part00781"/>
	<skos:member rdf:resource="http://partage.vocnet.org/part00782"/>
	<skos:member rdf:resource="http://partage.vocnet.org/part00783"/>
	<skos:member rdf:resource="http://partage.vocnet.org/part00784"/>
	<skos:member rdf:resource="http://partage.vocnet.org/part00785"/>
	<skos:member rdf:resource="http://partage.vocnet.org/part00786"/>
	<skos:member rdf:resource="http://partage.vocnet.org/part00787"/>
	<skos:member rdf:resource="http://partage.vocnet.org/part00788"/>
	<skos:member rdf:resource="http://partage.vocnet.org/part00789"/>
	<skos:member rdf:resource="http://partage.vocnet.org/part00790"/>
	<skos:member rdf:resource="http://partage.vocnet.org/part00791"/>
	<skos:member rdf:resource="http://partage.vocnet.org/part00792"/>
	<skos:member rdf:resource="http://partage.vocnet.org/part00793"/>
	<skos:member rdf:resource="http://partage.vocnet.org/part00794"/>
	<skos:member rdf:resource="http://partage.vocnet.org/part00795"/>
	<skos:member rdf:resource="http://partage.vocnet.org/part00796"/>
	<skos:member rdf:resource="http://partage.vocnet.org/part00797"/>
	<skos:member rdf:resource="http://partage.vocnet.org/part00798"/>
	<skos:member rdf:resource="http://partage.vocnet.org/part00799"/>
	<skos:member rdf:resource="http://partage.vocnet.org/part00800"/>
	<skos:member rdf:resource="http://partage.vocnet.org/part00801"/>
	<skos:member rdf:resource="http://partage.vocnet.org/part00802"/>
	<skos:member rdf:resource="http://partage.vocnet.org/part00803"/>
	<skos:member rdf:resource="http://partage.vocnet.org/part00804"/>
	<skos:member rdf:resource="http://partage.vocnet.org/part00805"/>
	<skos:member rdf:resource="http://partage.vocnet.org/part00806"/>
	<skos:member rdf:resource="http://partage.vocnet.org/part00807"/>
	<skos:member rdf:resource="http://partage.vocnet.org/part00808"/>
	<skos:member rdf:resource="http://partage.vocnet.org/part00809"/>
	<skos:member rdf:resource="http://partage.vocnet.org/part00810"/>
	<skos:member rdf:resource="http://partage.vocnet.org/part00811"/>
	<skos:member rdf:resource="http://partage.vocnet.org/part00812"/>
	<skos:member rdf:resource="http://partage.vocnet.org/part00813"/>
	<skos:member rdf:resource="http://partage.vocnet.org/part00814"/>
	<skos:member rdf:resource="http://partage.vocnet.org/part00815"/>
	<skos:member rdf:resource="http://partage.vocnet.org/part00816"/>
	<skos:member rdf:resource="http://partage.vocnet.org/part00817"/>
	<skos:member rdf:resource="http://partage.vocnet.org/part00818"/>
	<skos:member rdf:resource="http://partage.vocnet.org/part00819"/>
	<skos:member rdf:resource="http://partage.vocnet.org/part00820"/>
	<skos:member rdf:resource="http://partage.vocnet.org/part00821"/>
	<skos:member rdf:resource="http://partage.vocnet.org/part00822"/>
	<skos:member rdf:resource="http://partage.vocnet.org/part00823"/>
	<skos:member rdf:resource="http://partage.vocnet.org/part00825"/>
	<skos:member rdf:resource="http://partage.vocnet.org/part00826"/>
	<skos:member rdf:resource="http://partage.vocnet.org/part00827"/>
	<skos:member rdf:resource="http://partage.vocnet.org/part00828"/>
	<skos:member rdf:resource="http://partage.vocnet.org/part00829"/>
	<skos:member rdf:resource="http://partage.vocnet.org/part00830"/>
	<skos:member rdf:resource="http://partage.vocnet.org/part00831"/>
	<skos:member rdf:resource="http://partage.vocnet.org/part00833"/>
	<skos:member rdf:resource="http://partage.vocnet.org/part00834"/>
	<skos:member rdf:resource="http://partage.vocnet.org/part00835"/>
	<skos:member rdf:resource="http://partage.vocnet.org/part00876"/>
	<skos:member rdf:resource="http://partage.vocnet.org/part00882"/>
	<skos:member rdf:resource="http://partage.vocnet.org/part00883"/>
	<skos:member rdf:resource="http://partage.vocnet.org/part00884"/>
	<skos:member rdf:resource="http://partage.vocnet.org/part00885"/>
	<skos:member rdf:resource="http://partage.vocnet.org/part00886"/>
	<skos:member rdf:resource="http://partage.vocnet.org/part00887"/>
	<skos:member rdf:resource="http://partage.vocnet.org/part00888"/>
	<skos:member rdf:resource="http://partage.vocnet.org/part00890"/>
	<skos:member rdf:resource="http://partage.vocnet.org/part00891"/>
	<skos:member rdf:resource="http://partage.vocnet.org/part00892"/>
	<skos:member rdf:resource="http://partage.vocnet.org/part00893"/>
	<skos:member rdf:resource="http://partage.vocnet.org/part00894"/>
	<skos:member rdf:resource="http://partage.vocnet.org/part00895"/>
	<skos:member rdf:resource="http://partage.vocnet.org/part00896"/>
	<skos:member rdf:resource="http://partage.vocnet.org/part00904"/>
	<skos:member rdf:resource="http://partage.vocnet.org/part00914"/>
	<skos:member rdf:resource="http://partage.vocnet.org/part00974"/>
	<skos:member rdf:resource="http://partage.vocnet.org/part01066"/>
	<skos:member rdf:resource="http://partage.vocnet.org/part01120"/>
	<skos:member rdf:resource="http://partage.vocnet.org/part01121"/>
	<skos:member rdf:resource="http://partage.vocnet.org/part01122"/>
	<skos:member rdf:resource="http://partage.vocnet.org/part01123"/>
	<skos:member rdf:resource="http://partage.vocnet.org/part01125"/>
	<skos:member rdf:resource="http://partage.vocnet.org/part01127"/>
	<skos:member rdf:resource="http://partage.vocnet.org/part01129"/>
	<skos:member rdf:resource="http://partage.vocnet.org/part01134"/>
	<skos:member rdf:resource="http://partage.vocnet.org/part01135"/>
	<skos:member rdf:resource="http://partage.vocnet.org/part01136"/>
	<skos:member rdf:resource="http://partage.vocnet.org/part01137"/>
	<skos:member rdf:resource="http://partage.vocnet.org/part01141"/>
	<skos:member rdf:resource="http://partage.vocnet.org/part01143"/>
	<skos:member rdf:resource="http://partage.vocnet.org/part01144"/>
	<skos:member rdf:resource="http://partage.vocnet.org/part01146"/>
	<skos:member rdf:resource="http://partage.vocnet.org/part01155"/>
	<skos:member rdf:resource="http://partage.vocnet.org/part01157"/>
	<skos:member rdf:resource="http://partage.vocnet.org/part01158"/>
	<skos:member rdf:resource="http://partage.vocnet.org/part01160"/>
	<skos:member rdf:resource="http://partage.vocnet.org/part01161"/>
	<skos:member rdf:resource="http://partage.vocnet.org/part01162"/>
	<skos:member rdf:resource="http://partage.vocnet.org/part01163"/>
	<skos:member rdf:resource="http://partage.vocnet.org/part01164"/>
	<skos:member rdf:resource="http://partage.vocnet.org/part01168"/>
	<skos:member rdf:resource="http://partage.vocnet.org/part01169"/>
	<skos:member rdf:resource="http://partage.vocnet.org/part01170"/>
	<skos:member rdf:resource="http://partage.vocnet.org/part01171"/>
	<skos:member rdf:resource="http://partage.vocnet.org/part01172"/>
	<skos:member rdf:resource="http://partage.vocnet.org/part01175"/>
	<skos:member rdf:resource="http://partage.vocnet.org/part01177"/>
	<skos:member rdf:resource="http://partage.vocnet.org/part01178"/>
	<skos:member rdf:resource="http://partage.vocnet.org/part01179"/>
	<skos:member rdf:resource="http://partage.vocnet.org/part01180"/>
	<skos:member rdf:resource="http://partage.vocnet.org/part01181"/>
	<skos:member rdf:resource="http://partage.vocnet.org/part01182"/>
	<skos:member rdf:resource="http://partage.vocnet.org/part01184"/>
	<skos:member rdf:resource="http://partage.vocnet.org/part01185"/>
	<skos:member rdf:resource="http://partage.vocnet.org/part01188"/>
	<skos:member rdf:resource="http://partage.vocnet.org/part01189"/>
	<skos:member rdf:resource="http://partage.vocnet.org/part01190"/>
	<skos:member rdf:resource="http://partage.vocnet.org/part01191"/>
	<skos:member rdf:resource="http://partage.vocnet.org/part01192"/>
	<skos:member rdf:resource="http://partage.vocnet.org/part01193"/>
	<skos:member rdf:resource="http://partage.vocnet.org/part01194"/>
	<skos:member rdf:resource="http://partage.vocnet.org/part01198"/>
	<skos:member rdf:resource="http://partage.vocnet.org/part01199"/>
	<skos:member rdf:resource="http://partage.vocnet.org/part01237"/>
	<skos:member rdf:resource="http://partage.vocnet.org/part01244"/>
	<skos:member rdf:resource="http://partage.vocnet.org/part01245"/>
</skos:Collection>
<skos:Collection rdf:about="http://partage.vocnet.org/NonIndexingConcepts">
	<skos:prefLabel>NonIndexingConcepts</skos:prefLabel>
	<skos:member rdf:resource="http://partage.vocnet.org/part00045"/>
	<skos:member rdf:resource="http://partage.vocnet.org/part00074"/>
	<skos:member rdf:resource="http://partage.vocnet.org/part00089"/>
	<skos:member rdf:resource="http://partage.vocnet.org/part00092"/>
	<skos:member rdf:resource="http://partage.vocnet.org/part00104"/>
	<skos:member rdf:resource="http://partage.vocnet.org/part00116"/>
	<skos:member rdf:resource="http://partage.vocnet.org/part00120"/>
	<skos:member rdf:resource="http://partage.vocnet.org/part00122"/>
	<skos:member rdf:resource="http://partage.vocnet.org/part00158"/>
	<skos:member rdf:resource="http://partage.vocnet.org/part00169"/>
	<skos:member rdf:resource="http://partage.vocnet.org/part00179"/>
	<skos:member rdf:resource="http://partage.vocnet.org/part00202"/>
	<skos:member rdf:resource="http://partage.vocnet.org/part00203"/>
	<skos:member rdf:resource="http://partage.vocnet.org/part00204"/>
	<skos:member rdf:resource="http://partage.vocnet.org/part00224"/>
	<skos:member rdf:resource="http://partage.vocnet.org/part00298"/>
	<skos:member rdf:resource="http://partage.vocnet.org/part00406"/>
	<skos:member rdf:resource="http://partage.vocnet.org/part00504"/>
	<skos:member rdf:resource="http://partage.vocnet.org/part00524"/>
	<skos:member rdf:resource="http://partage.vocnet.org/part00525"/>
	<skos:member rdf:resource="http://partage.vocnet.org/part00644"/>
	<skos:member rdf:resource="http://partage.vocnet.org/part00824"/>
	<skos:member rdf:resource="http://partage.vocnet.org/part00836"/>
	<skos:member rdf:resource="http://partage.vocnet.org/part00837"/>
	<skos:member rdf:resource="http://partage.vocnet.org/part00847"/>
	<skos:member rdf:resource="http://partage.vocnet.org/part00851"/>
	<skos:member rdf:resource="http://partage.vocnet.org/part00853"/>
	<skos:member rdf:resource="http://partage.vocnet.org/part00917"/>
	<skos:member rdf:resource="http://partage.vocnet.org/part00918"/>
	<skos:member rdf:resource="http://partage.vocnet.org/part00919"/>
	<skos:member rdf:resource="http://partage.vocnet.org/part00921"/>
	<skos:member rdf:resource="http://partage.vocnet.org/part00923"/>
	<skos:member rdf:resource="http://partage.vocnet.org/part00928"/>
	<skos:member rdf:resource="http://partage.vocnet.org/part00939"/>
	<skos:member rdf:resource="http://partage.vocnet.org/part00943"/>
	<skos:member rdf:resource="http://partage.vocnet.org/part00944"/>
	<skos:member rdf:resource="http://partage.vocnet.org/part00948"/>
	<skos:member rdf:resource="http://partage.vocnet.org/part00955"/>
	<skos:member rdf:resource="http://partage.vocnet.org/part00958"/>
	<skos:member rdf:resource="http://partage.vocnet.org/part00965"/>
	<skos:member rdf:resource="http://partage.vocnet.org/part00983"/>
	<skos:member rdf:resource="http://partage.vocnet.org/part00986"/>
	<skos:member rdf:resource="http://partage.vocnet.org/part00994"/>
	<skos:member rdf:resource="http://partage.vocnet.org/part01006"/>
	<skos:member rdf:resource="http://partage.vocnet.org/part01009"/>
	<skos:member rdf:resource="http://partage.vocnet.org/part01012"/>
	<skos:member rdf:resource="http://partage.vocnet.org/part01028"/>
	<skos:member rdf:resource="http://partage.vocnet.org/part01034"/>
	<skos:member rdf:resource="http://partage.vocnet.org/part01041"/>
	<skos:member rdf:resource="http://partage.vocnet.org/part01045"/>
	<skos:member rdf:resource="http://partage.vocnet.org/part01046"/>
	<skos:member rdf:resource="http://partage.vocnet.org/part01052"/>
	<skos:member rdf:resource="http://partage.vocnet.org/part01057"/>
	<skos:member rdf:resource="http://partage.vocnet.org/part01064"/>
	<skos:member rdf:resource="http://partage.vocnet.org/part01124"/>
	<skos:member rdf:resource="http://partage.vocnet.org/part01187"/>
	<skos:member rdf:resource="http://partage.vocnet.org/part01200"/>
	<skos:member rdf:resource="http://partage.vocnet.org/part01201"/>
	<skos:member rdf:resource="http://partage.vocnet.org/part01228"/>
	<skos:member rdf:resource="http://partage.vocnet.org/part01238"/>
	<skos:member rdf:resource="http://partage.vocnet.org/part01259"/>
</skos:Collection>
</rdf:RDF>