<?xml version="1.0" encoding="UTF-8"?>
<rdf:RDF xmlns:dcterms="http://purl.org/dc/terms/" xmlns:owl="http://www.w3.org/2002/07/owl#" xmlns:rdf="http://www.w3.org/1999/02/22-rdf-syntax-ns#" xmlns:skos="http://www.w3.org/2004/02/skos/core#" xmlns:xsi="http://www.w3.org/2001/XMLSchema-instance">
	<skos:ConceptScheme rdf:about="http://partage.vocnet.org/MicroObjectTypes">
		<rdf:type rdf:resource="http://www.w3.org/2004/02/skos/core#ConceptScheme"/>
	</skos:ConceptScheme>
	<skos:Concept rdf:about="http://partage.vocnet.org/part00036">
		<skos:inScheme rdf:resource="http://partage.vocnet.org/MicroObjectTypes"/>
		<skos:prefLabel xml:lang="en">works on paper</skos:prefLabel>
		<skos:altLabel xml:lang="de">Kunst auf Papier</skos:altLabel>
		<skos:prefLabel xml:lang="sv">konst på papper</skos:prefLabel>
		<skos:prefLabel xml:lang="fi">paperityöt</skos:prefLabel>
		<skos:altLabel xml:lang="es">obras en papel</skos:altLabel>
		<skos:prefLabel xml:lang="es">obras sobre papel</skos:prefLabel>
		<skos:prefLabel xml:lang="sl">dela na papirju</skos:prefLabel>
		<skos:prefLabel xml:lang="pt">trabalho sobre papel</skos:prefLabel>
		<skos:prefLabel xml:lang="pl">prace na papierze</skos:prefLabel>
		<skos:prefLabel xml:lang="nl">werken op papier</skos:prefLabel>
		<skos:prefLabel xml:lang="it">oggetti di carta</skos:prefLabel>
		<skos:prefLabel xml:lang="cs">práce na papíře</skos:prefLabel>
		<skos:prefLabel xml:lang="ca">obra sobre paper</skos:prefLabel>
		<skos:prefLabel xml:lang="fr">œuvre sur papier</skos:prefLabel>
		<skos:prefLabel xml:lang="hu">papír alapú tárgy</skos:prefLabel>
		<skos:prefLabel xml:lang="no">arbeid på papir</skos:prefLabel>
		<skos:prefLabel xml:lang="hr">radovi na papiru</skos:prefLabel>
		<skos:prefLabel xml:lang="de">Graphik</skos:prefLabel>
		<skos:altLabel xml:lang="de">Arbeiten auf Papier</skos:altLabel>
		<skos:exactMatch rdf:resource="http://vocab.getty.edu/aat/300189621"/>
		<skos:editorialNote xml:lang="en">PPObjectType</skos:editorialNote>
		<skos:scopeNote xml:lang="en">Use collectively to bring together works of art in which paper is the support, only when terms such as "drawings" or "prints" are not appropriate.</skos:scopeNote>
	</skos:Concept>
	<skos:Concept rdf:about="http://partage.vocnet.org/part00040">
		<skos:inScheme rdf:resource="http://partage.vocnet.org/MicroObjectTypes"/>
		<skos:prefLabel xml:lang="en">sketches</skos:prefLabel>
		<skos:altLabel xml:lang="de">Skizze</skos:altLabel>
		<skos:prefLabel xml:lang="sv">skisser</skos:prefLabel>
		<skos:prefLabel xml:lang="fi">luonnokset</skos:prefLabel>
		<skos:prefLabel xml:lang="es">bocetos</skos:prefLabel>
		<skos:prefLabel xml:lang="sl">skice</skos:prefLabel>
		<skos:prefLabel xml:lang="pt">esboço</skos:prefLabel>
		<skos:prefLabel xml:lang="pl">szkice</skos:prefLabel>
		<skos:prefLabel xml:lang="nl">schetsen</skos:prefLabel>
		<skos:altLabel xml:lang="it">schizzi</skos:altLabel>
		<skos:prefLabel xml:lang="it">bozzetti</skos:prefLabel>
		<skos:prefLabel xml:lang="cs">skica</skos:prefLabel>
		<skos:prefLabel xml:lang="ca">esbossos</skos:prefLabel>
		<skos:prefLabel xml:lang="de">Skizzen</skos:prefLabel>
		<skos:prefLabel xml:lang="fr">esquisse</skos:prefLabel>
		<skos:prefLabel xml:lang="hu">vázlat</skos:prefLabel>
		<skos:prefLabel xml:lang="no">skisser</skos:prefLabel>
		<skos:prefLabel xml:lang="hr">skice</skos:prefLabel>
		<skos:exactMatch rdf:resource="http://vocab.getty.edu/aat/300015617"/>
		<skos:editorialNote xml:lang="en">PPObjectType</skos:editorialNote>
		<skos:scopeNote xml:lang="en">Rough or summary art works; less finished than studies. Though sketches are often in the drawing medium, the term "drawings" in general implies more finished works than does "sketches."</skos:scopeNote>
	</skos:Concept>
	<skos:Concept rdf:about="http://partage.vocnet.org/part00041">
		<skos:inScheme rdf:resource="http://partage.vocnet.org/MicroObjectTypes"/>
		<skos:hiddenLabel xml:lang="en">sculpture (visual work)</skos:hiddenLabel>
		<skos:prefLabel xml:lang="en">sculpture</skos:prefLabel>
		<skos:prefLabel xml:lang="de">Skulptur</skos:prefLabel>
		<skos:prefLabel xml:lang="sv">skulpturer</skos:prefLabel>
		<skos:prefLabel xml:lang="fi">veistokset</skos:prefLabel>
		<skos:prefLabel xml:lang="es">escultura</skos:prefLabel>
		<skos:altLabel xml:lang="sl">kipi</skos:altLabel>
		<skos:prefLabel xml:lang="sl">skulpture</skos:prefLabel>
		<skos:prefLabel xml:lang="pt">escultura</skos:prefLabel>
		<skos:prefLabel xml:lang="pl">rzeźba</skos:prefLabel>
		<skos:prefLabel xml:lang="nl">beeldhouwwerken</skos:prefLabel>
		<skos:prefLabel xml:lang="it">scultura</skos:prefLabel>
		<skos:prefLabel xml:lang="cs">sochařství</skos:prefLabel>
		<skos:prefLabel xml:lang="ca">escultura</skos:prefLabel>
		<skos:altLabel xml:lang="de">Plastik</skos:altLabel>
		<skos:prefLabel xml:lang="hr">skulpture</skos:prefLabel>
		<skos:prefLabel xml:lang="hu">szobrászat</skos:prefLabel>
		<skos:prefLabel xml:lang="no">skulptur</skos:prefLabel>
		<skos:prefLabel xml:lang="fr">sculpture</skos:prefLabel>
		<skos:exactMatch rdf:resource="http://vocab.getty.edu/aat/300047090"/>
		<skos:editorialNote xml:lang="en">PPObjectType</skos:editorialNote>
		<skos:scopeNote xml:lang="en">Three-dimensional works of art in which images and forms are produced in relief, in intaglio, or in the round. The term refers particularly to art works created by carving or engraving a hard material, by molding or casting a malleable material (which usually then hardens), or by assembling parts to create a three-dimensional object. It is typically used to refer to large or medium-sized objects made of stone, wood, bronze, or another metal. Small objects are typically referred to as "carvings" or another appropriate term. "Sculpture" refers to works that represent tangible beings, objects, or groups of objects, or are abstract works that have defined edges and boundaries and can be measured. As three-dimensional works become more diffused in space or time, or less tangible, use appropriate specific terms, such as "mail art" or "environmental art."</skos:scopeNote>
	</skos:Concept>
	<skos:Concept rdf:about="http://partage.vocnet.org/part00042">
		<skos:inScheme rdf:resource="http://partage.vocnet.org/MicroObjectTypes"/>
		<skos:hiddenLabel xml:lang="en">prints (visual works)</skos:hiddenLabel>
		<skos:prefLabel xml:lang="en">prints</skos:prefLabel>
		<skos:prefLabel xml:lang="sv">tryck</skos:prefLabel>
		<skos:prefLabel xml:lang="fi">painokuvat</skos:prefLabel>
		<skos:prefLabel xml:lang="es">estampas</skos:prefLabel>
		<skos:prefLabel xml:lang="sl">tiski</skos:prefLabel>
		<skos:prefLabel xml:lang="pt">impressões</skos:prefLabel>
		<skos:prefLabel xml:lang="pl">odbitki graficzne</skos:prefLabel>
		<skos:prefLabel xml:lang="nl">prenten</skos:prefLabel>
		<skos:prefLabel xml:lang="it">stampe</skos:prefLabel>
		<skos:prefLabel xml:lang="cs">tisk</skos:prefLabel>
		<skos:prefLabel xml:lang="ca">estampes</skos:prefLabel>
		<skos:prefLabel xml:lang="de">Druckgraphik</skos:prefLabel>
		<skos:prefLabel xml:lang="fr">imprimé</skos:prefLabel>
		<skos:prefLabel xml:lang="hu">metszet</skos:prefLabel>
		<skos:prefLabel xml:lang="no">trykk</skos:prefLabel>
		<skos:prefLabel xml:lang="hr">grafike</skos:prefLabel>
		<skos:exactMatch rdf:resource="http://vocab.getty.edu/aat/300041273"/>
		<skos:editorialNote xml:lang="en">PPObjectType</skos:editorialNote>
		<skos:scopeNote xml:lang="en">Pictorial works produced by transferring images by means of a matrix such as a plate, block, or screen, using any of various printing processes. When emphasizing the individual printed image, use "impressions." Avoid the controversial expression "original prints," except in reference to discussions of the expression's use. If prints are neither "reproductive prints" nor "popular prints," use just "prints." With regard to photographs, see "photographic prints"; for types of reproductions of technical drawings and documents, see terms found under "reprographic copies."</skos:scopeNote>
	</skos:Concept>
	<skos:Concept rdf:about="http://partage.vocnet.org/part00043">
		<skos:inScheme rdf:resource="http://partage.vocnet.org/MicroObjectTypes"/>
		<skos:hiddenLabel xml:lang="en">pastels (visual works)</skos:hiddenLabel>
		<skos:prefLabel xml:lang="en">pastels</skos:prefLabel>
		<skos:altLabel xml:lang="de">Pastelle</skos:altLabel>
		<skos:prefLabel xml:lang="sv">pasteller</skos:prefLabel>
		<skos:prefLabel xml:lang="fi">pastelli</skos:prefLabel>
		<skos:altLabel xml:lang="es">pinturas al pastel</skos:altLabel>
		<skos:prefLabel xml:lang="es">pasteles</skos:prefLabel>
		<skos:prefLabel xml:lang="sl">pasteli</skos:prefLabel>
		<skos:prefLabel xml:lang="pt">pastel</skos:prefLabel>
		<skos:prefLabel xml:lang="pl">pastele</skos:prefLabel>
		<skos:prefLabel xml:lang="nl">pastels</skos:prefLabel>
		<skos:prefLabel xml:lang="it">disegni a pastello</skos:prefLabel>
		<skos:prefLabel xml:lang="cs">pastel</skos:prefLabel>
		<skos:prefLabel xml:lang="ca">pastels</skos:prefLabel>
		<skos:prefLabel xml:lang="hr">pasteli</skos:prefLabel>
		<skos:prefLabel xml:lang="no">pastell</skos:prefLabel>
		<skos:prefLabel xml:lang="hu">pasztell</skos:prefLabel>
		<skos:prefLabel xml:lang="fr">pastel</skos:prefLabel>
		<skos:prefLabel xml:lang="de">Pastell</skos:prefLabel>
		<skos:exactMatch rdf:resource="http://vocab.getty.edu/aat/300076922"/>
		<skos:editorialNote xml:lang="en">PPObjectType</skos:editorialNote>
		<skos:scopeNote xml:lang="en">Works of art, typically on a paper or vellum support, to which designs are applied using crayons made of ground pigment held together with a binder, typically oil or water and gum. Works in this medium are sometimes classified as drawings, and sometimes as paintings, typically based on the local curatorial department responsible for the work or on the material of the support (pastels on paper may be classified as drawings, while pastels on vellum may be classified as paintings).</skos:scopeNote>
	</skos:Concept>
	<skos:Concept rdf:about="http://partage.vocnet.org/part00044">
		<skos:inScheme rdf:resource="http://partage.vocnet.org/MicroObjectTypes"/>
		<skos:hiddenLabel xml:lang="en">paintings (visual works)</skos:hiddenLabel>
		<skos:prefLabel xml:lang="en">paintings</skos:prefLabel>
		<skos:prefLabel xml:lang="sv">målningar</skos:prefLabel>
		<skos:prefLabel xml:lang="fi">maalaukset</skos:prefLabel>
		<skos:altLabel xml:lang="es">pinturas</skos:altLabel>
		<skos:prefLabel xml:lang="es">pintura</skos:prefLabel>
		<skos:prefLabel xml:lang="sl">slike</skos:prefLabel>
		<skos:altLabel xml:lang="pt">pinturas</skos:altLabel>
		<skos:prefLabel xml:lang="pt">pintura</skos:prefLabel>
		<skos:prefLabel xml:lang="pl">obrazy</skos:prefLabel>
		<skos:prefLabel xml:lang="nl">schilderingen</skos:prefLabel>
		<skos:prefLabel xml:lang="it">dipinti</skos:prefLabel>
		<skos:prefLabel xml:lang="cs">malba</skos:prefLabel>
		<skos:prefLabel xml:lang="ca">pintura</skos:prefLabel>
		<skos:hiddenLabel xml:lang="de">Malerei</skos:hiddenLabel>
		<skos:prefLabel xml:lang="de">Gemälde</skos:prefLabel>
		<skos:prefLabel xml:lang="fr">peinture</skos:prefLabel>
		<skos:prefLabel xml:lang="hu">festmény</skos:prefLabel>
		<skos:prefLabel xml:lang="no">maleri</skos:prefLabel>
		<skos:prefLabel xml:lang="hr">slikarstvo</skos:prefLabel>
		<skos:narrower rdf:resource="http://partage.vocnet.org/part00249"/>
		<skos:narrower rdf:resource="http://partage.vocnet.org/part00470"/>
		<skos:narrower rdf:resource="http://partage.vocnet.org/part00501"/>
		<skos:narrower rdf:resource="http://partage.vocnet.org/part00510"/>
		<skos:exactMatch rdf:resource="http://vocab.getty.edu/aat/300033618"/>
		<skos:editorialNote xml:lang="en">PPObjectType</skos:editorialNote>
		<skos:scopeNote xml:lang="en">Unique works in which images are formed primarily by the direct application of pigments suspended in oil, water, egg yolk, molten wax, or other liquid, arranged in masses of color, onto a generally two-dimensional surface.</skos:scopeNote>
	</skos:Concept>
	<skos:Concept rdf:about="http://partage.vocnet.org/part00046">
		<skos:inScheme rdf:resource="http://partage.vocnet.org/MicroObjectTypes"/>
		<skos:hiddenLabel xml:lang="en">mosaics (visual works)</skos:hiddenLabel>
		<skos:prefLabel xml:lang="en">mosaics</skos:prefLabel>
		<skos:prefLabel xml:lang="sv">mosaiker</skos:prefLabel>
		<skos:prefLabel xml:lang="fi">mosaiikit</skos:prefLabel>
		<skos:prefLabel xml:lang="es">mosaicos</skos:prefLabel>
		<skos:prefLabel xml:lang="sl">mozaiki</skos:prefLabel>
		<skos:prefLabel xml:lang="pt">mosaico</skos:prefLabel>
		<skos:prefLabel xml:lang="pl">mozaiki</skos:prefLabel>
		<skos:prefLabel xml:lang="nl">mozaïeken</skos:prefLabel>
		<skos:prefLabel xml:lang="it">mosaici</skos:prefLabel>
		<skos:prefLabel xml:lang="cs">mozaika</skos:prefLabel>
		<skos:prefLabel xml:lang="ca">mosaics</skos:prefLabel>
		<skos:prefLabel xml:lang="de">Mosaik</skos:prefLabel>
		<skos:prefLabel xml:lang="hr">mozaici</skos:prefLabel>
		<skos:prefLabel xml:lang="no">mosaikk</skos:prefLabel>
		<skos:prefLabel xml:lang="hu">mozaik</skos:prefLabel>
		<skos:prefLabel xml:lang="fr">mosaïque</skos:prefLabel>
		<skos:exactMatch rdf:resource="http://vocab.getty.edu/aat/300015342"/>
		<skos:editorialNote xml:lang="en">PPObjectType</skos:editorialNote>
		<skos:scopeNote xml:lang="en">Images or patterns composed of small, regularly shaped pieces of durable material, usually stone or colored glass. Distinguished from "opus sectile" which is composed of individually shaped pieces of durable material, usually stone or glass, which conform to the design or pattern.</skos:scopeNote>
	</skos:Concept>
	<skos:Concept rdf:about="http://partage.vocnet.org/part00047">
		<skos:inScheme rdf:resource="http://partage.vocnet.org/MicroObjectTypes"/>
		<skos:hiddenLabel xml:lang="en">drawings (visual works)</skos:hiddenLabel>
		<skos:prefLabel xml:lang="en">drawings</skos:prefLabel>
		<skos:altLabel xml:lang="de">Zeichnungen</skos:altLabel>
		<skos:prefLabel xml:lang="de">Zeichnung</skos:prefLabel>
		<skos:prefLabel xml:lang="sv">teckningar</skos:prefLabel>
		<skos:prefLabel xml:lang="fi">piirustukset</skos:prefLabel>
		<skos:prefLabel xml:lang="es">dibujo</skos:prefLabel>
		<skos:prefLabel xml:lang="sl">risbe</skos:prefLabel>
		<skos:altLabel xml:lang="pt">desenhos</skos:altLabel>
		<skos:prefLabel xml:lang="pt">desenho</skos:prefLabel>
		<skos:prefLabel xml:lang="pl">rysunki</skos:prefLabel>
		<skos:prefLabel xml:lang="nl">tekeningen</skos:prefLabel>
		<skos:prefLabel xml:lang="it">disegni</skos:prefLabel>
		<skos:prefLabel xml:lang="cs">kresba</skos:prefLabel>
		<skos:prefLabel xml:lang="ca">dibuix</skos:prefLabel>
		<skos:altLabel xml:lang="de">Handzeichnungen</skos:altLabel>
		<skos:prefLabel xml:lang="fr">dessin</skos:prefLabel>
		<skos:prefLabel xml:lang="hu">rajz</skos:prefLabel>
		<skos:prefLabel xml:lang="no">tegninger</skos:prefLabel>
		<skos:prefLabel xml:lang="hr">crteži</skos:prefLabel>
		<skos:exactMatch rdf:resource="http://vocab.getty.edu/aat/300033973"/>
		<skos:editorialNote xml:lang="en">PPObjectType</skos:editorialNote>
		<skos:scopeNote xml:lang="en">Visual works produced by drawing, which is the application of lines on a surface, often paper, by using a pencil, pen, chalk, or some other tracing instrument to focus on the delineation of form rather than the application of color. This term is often defined broadly to refer to computer-generated images as well.</skos:scopeNote>
	</skos:Concept>
	<skos:Concept rdf:about="http://partage.vocnet.org/part00048">
		<skos:inScheme rdf:resource="http://partage.vocnet.org/MicroObjectTypes"/>
		<skos:hiddenLabel xml:lang="en">calligraphy (visual works)</skos:hiddenLabel>
		<skos:prefLabel xml:lang="en">calligraphy</skos:prefLabel>
		<skos:prefLabel xml:lang="sv">kalligrafi</skos:prefLabel>
		<skos:prefLabel xml:lang="fi">kalligrafia</skos:prefLabel>
		<skos:prefLabel xml:lang="es">caligrafía</skos:prefLabel>
		<skos:prefLabel xml:lang="sl">kaligrafija</skos:prefLabel>
		<skos:prefLabel xml:lang="pt">caligrafia</skos:prefLabel>
		<skos:prefLabel xml:lang="pl">kaligrafia</skos:prefLabel>
		<skos:prefLabel xml:lang="nl">kalligrafie</skos:prefLabel>
		<skos:altLabel xml:lang="it">carattere</skos:altLabel>
		<skos:prefLabel xml:lang="it">calligrafia</skos:prefLabel>
		<skos:prefLabel xml:lang="cs">kaligrafie</skos:prefLabel>
		<skos:prefLabel xml:lang="ca">cal·ligrafia</skos:prefLabel>
		<skos:prefLabel xml:lang="de">Kalligraphie</skos:prefLabel>
		<skos:hiddenLabel xml:lang="de">Kalligrafie</skos:hiddenLabel>
		<skos:prefLabel xml:lang="hr">kaligrafija</skos:prefLabel>
		<skos:prefLabel xml:lang="no">kalligrafi</skos:prefLabel>
		<skos:prefLabel xml:lang="hu">kalligráfia</skos:prefLabel>
		<skos:prefLabel xml:lang="fr">calligraphie</skos:prefLabel>
		<skos:exactMatch rdf:resource="http://vocab.getty.edu/aat/300266660"/>
		<skos:editorialNote xml:lang="en">PPObjectType</skos:editorialNote>
		<skos:scopeNote xml:lang="en">Works composed primarily of beautiful, elegant letters or flourishes that are typically created by hand with a pen, either in unjoined characters or in cursive writing. May also refer to similar works created by computer or another means.</skos:scopeNote>
	</skos:Concept>
	<skos:Concept rdf:about="http://partage.vocnet.org/part00052">
		<skos:inScheme rdf:resource="http://partage.vocnet.org/MicroObjectTypes"/>
		<skos:hiddenLabel xml:lang="en">studies (visual works)</skos:hiddenLabel>
		<skos:prefLabel xml:lang="en">studies</skos:prefLabel>
		<skos:prefLabel xml:lang="sv">studier</skos:prefLabel>
		<skos:prefLabel xml:lang="fi">harjoitelmat</skos:prefLabel>
		<skos:prefLabel xml:lang="es">estudios</skos:prefLabel>
		<skos:prefLabel xml:lang="sl">študije</skos:prefLabel>
		<skos:prefLabel xml:lang="pt">estudos</skos:prefLabel>
		<skos:prefLabel xml:lang="pl">studia</skos:prefLabel>
		<skos:prefLabel xml:lang="nl">studies</skos:prefLabel>
		<skos:prefLabel xml:lang="it">studi</skos:prefLabel>
		<skos:prefLabel xml:lang="cs">studie</skos:prefLabel>
		<skos:prefLabel xml:lang="ca">estudis</skos:prefLabel>
		<skos:prefLabel xml:lang="de">Studien</skos:prefLabel>
		<skos:prefLabel xml:lang="hr">studije</skos:prefLabel>
		<skos:prefLabel xml:lang="fr">étude</skos:prefLabel>
		<skos:prefLabel xml:lang="hu">tanulmányrajz</skos:prefLabel>
		<skos:prefLabel xml:lang="no">studie</skos:prefLabel>
		<skos:exactMatch rdf:resource="http://vocab.getty.edu/aat/300081053"/>
		<skos:editorialNote xml:lang="en">PPObjectType</skos:editorialNote>
		<skos:scopeNote xml:lang="en">Works in any medium of the visual arts that explore a subject or are preliminary to a separate, more finalized work; more finished than sketches. For representations or diagrams that clarify, usually accompanying a text, use "illustrations."</skos:scopeNote>
	</skos:Concept>
	<skos:Concept rdf:about="http://partage.vocnet.org/part00055">
		<skos:inScheme rdf:resource="http://partage.vocnet.org/MicroObjectTypes"/>
		<skos:prefLabel xml:lang="en">tapestries</skos:prefLabel>
		<skos:prefLabel xml:lang="sv">vävar</skos:prefLabel>
		<skos:prefLabel xml:lang="fi">seinätekstiilit</skos:prefLabel>
		<skos:altLabel xml:lang="es">tapiz de Arras</skos:altLabel>
		<skos:prefLabel xml:lang="es">tapices</skos:prefLabel>
		<skos:prefLabel xml:lang="sl">tapiserije</skos:prefLabel>
		<skos:prefLabel xml:lang="pt">tapeçaria</skos:prefLabel>
		<skos:prefLabel xml:lang="pl">tkaniny dekoracyjne</skos:prefLabel>
		<skos:prefLabel xml:lang="nl">tapisserieën</skos:prefLabel>
		<skos:prefLabel xml:lang="it">tappezzerie</skos:prefLabel>
		<skos:prefLabel xml:lang="cs">tapiserie</skos:prefLabel>
		<skos:prefLabel xml:lang="ca">tapissos</skos:prefLabel>
		<skos:prefLabel xml:lang="de">Tapisserie</skos:prefLabel>
		<skos:prefLabel xml:lang="hr">tapiserije</skos:prefLabel>
		<skos:prefLabel xml:lang="no">veggtepper</skos:prefLabel>
		<skos:prefLabel xml:lang="hu">szőnyeg</skos:prefLabel>
		<skos:prefLabel xml:lang="fr">tapisserie</skos:prefLabel>
		<skos:broader rdf:resource="http://partage.vocnet.org/part00100"/>
		<skos:exactMatch rdf:resource="http://vocab.getty.edu/aat/300205002"/>
		<skos:editorialNote xml:lang="en">PPObjectType</skos:editorialNote>
		<skos:scopeNote xml:lang="en">Heavy, woven textiles used as wall hangings, curtains, upholstery, or to hang from windows or balconies. Tapestries are characterized by decoration that may include ornamental or pictorial subjects; they often have details that are painted or embroidered. They are usually of wool and hand-woven on a tapestry loom by a process that differs from cloth-weaving in that the weft travels only to the warp at the edge of a particular color or pattern in the design, rather traveling from edge to edge of the entire piece of fabric. Various techniques are used in mixing and overlaying colors to create shading and patterns. The term also refers to machine-woven imitations of hand-made hangings.</skos:scopeNote>
	</skos:Concept>
	<skos:Concept rdf:about="http://partage.vocnet.org/part00056">
		<skos:inScheme rdf:resource="http://partage.vocnet.org/MicroObjectTypes"/>
		<skos:prefLabel xml:lang="en">medals</skos:prefLabel>
		<skos:prefLabel xml:lang="de">Medaillen</skos:prefLabel>
		<skos:altLabel xml:lang="de">Medaille</skos:altLabel>
		<skos:prefLabel xml:lang="sv">medaljer</skos:prefLabel>
		<skos:prefLabel xml:lang="fi">mitalit</skos:prefLabel>
		<skos:prefLabel xml:lang="es">medallas</skos:prefLabel>
		<skos:prefLabel xml:lang="sl">medalje</skos:prefLabel>
		<skos:altLabel xml:lang="pt">medalhas</skos:altLabel>
		<skos:prefLabel xml:lang="pt">medalha</skos:prefLabel>
		<skos:prefLabel xml:lang="pl">medale</skos:prefLabel>
		<skos:prefLabel xml:lang="nl">medailles</skos:prefLabel>
		<skos:prefLabel xml:lang="it">medaglie</skos:prefLabel>
		<skos:prefLabel xml:lang="cs">medaile</skos:prefLabel>
		<skos:prefLabel xml:lang="ca">medalles</skos:prefLabel>
		<skos:prefLabel xml:lang="hr">medalje</skos:prefLabel>
		<skos:prefLabel xml:lang="no">medaljer</skos:prefLabel>
		<skos:prefLabel xml:lang="hu">medál</skos:prefLabel>
		<skos:prefLabel xml:lang="fr">médaille</skos:prefLabel>
		<skos:exactMatch rdf:resource="http://vocab.getty.edu/aat/300046025"/>
		<skos:editorialNote xml:lang="en">PPObjectType</skos:editorialNote>
		<skos:scopeNote xml:lang="en">Small pieces of metal, usually gold, silver, or bronze, bearing a relief design on one or both sides and having a commemorative purpose; not used as a medium of exchange.</skos:scopeNote>
	</skos:Concept>
	<skos:Concept rdf:about="http://partage.vocnet.org/part00059">
		<skos:inScheme rdf:resource="http://partage.vocnet.org/MicroObjectTypes"/>
		<skos:prefLabel xml:lang="en">lacquerware</skos:prefLabel>
		<skos:prefLabel xml:lang="sv">lackarbete</skos:prefLabel>
		<skos:prefLabel xml:lang="fi">lakkatyöt</skos:prefLabel>
		<skos:hiddenLabel xml:lang="es">obra de laca</skos:hiddenLabel>
		<skos:prefLabel xml:lang="es">lacados</skos:prefLabel>
		<skos:altLabel xml:lang="sl">lak</skos:altLabel>
		<skos:prefLabel xml:lang="sl">lakirani izdelki</skos:prefLabel>
		<skos:prefLabel xml:lang="pt">objetos de laca</skos:prefLabel>
		<skos:prefLabel xml:lang="pl">wyroby z laki</skos:prefLabel>
		<skos:prefLabel xml:lang="nl">lakwerk</skos:prefLabel>
		<skos:prefLabel xml:lang="it">lacche</skos:prefLabel>
		<skos:prefLabel xml:lang="cs">lakované předměty</skos:prefLabel>
		<skos:prefLabel xml:lang="ca">lacats</skos:prefLabel>
		<skos:altLabel xml:lang="de">Lackkunst</skos:altLabel>
		<skos:prefLabel xml:lang="de">Lacke</skos:prefLabel>
		<skos:prefLabel xml:lang="hr">lakirani predmeti</skos:prefLabel>
		<skos:prefLabel xml:lang="no">lakkarbeid</skos:prefLabel>
		<skos:prefLabel xml:lang="hu">lakkbútor</skos:prefLabel>
		<skos:prefLabel xml:lang="fr">laque</skos:prefLabel>
		<skos:exactMatch rdf:resource="http://vocab.getty.edu/aat/300264021"/>
		<skos:editorialNote xml:lang="en">PPObjectType</skos:editorialNote>
		<skos:scopeNote xml:lang="en">Objects, usually made of thin wood, that are coated and decorated with layers of lacquer, often accompanied by inlays of other substances such as mother-of-pearl and metal.</skos:scopeNote>
	</skos:Concept>
	<skos:Concept rdf:about="http://partage.vocnet.org/part00060">
		<skos:inScheme rdf:resource="http://partage.vocnet.org/MicroObjectTypes"/>
		<skos:prefLabel xml:lang="en">woodwork</skos:prefLabel>
		<skos:prefLabel xml:lang="nl">houtwerk</skos:prefLabel>
		<skos:prefLabel xml:lang="it">oggetti di legno lavorato</skos:prefLabel>
		<skos:prefLabel xml:lang="cs">práce ze dřeva</skos:prefLabel>
		<skos:prefLabel xml:lang="ca">obra en fusta</skos:prefLabel>
		<skos:altLabel xml:lang="de">Tischlerarbeit</skos:altLabel>
		<skos:prefLabel xml:lang="de">Holzarbeiten</skos:prefLabel>
		<skos:prefLabel xml:lang="sv">snickerier</skos:prefLabel>
		<skos:prefLabel xml:lang="fi">puutyöt</skos:prefLabel>
		<skos:altLabel xml:lang="es">objeto de madera</skos:altLabel>
		<skos:prefLabel xml:lang="es">obra en madera</skos:prefLabel>
		<skos:prefLabel xml:lang="sl">leseni izdelki</skos:prefLabel>
		<skos:prefLabel xml:lang="pt">carpintaria</skos:prefLabel>
		<skos:prefLabel xml:lang="pl">wyroby z drewna</skos:prefLabel>
		<skos:prefLabel xml:lang="fr">ébénisterie</skos:prefLabel>
		<skos:prefLabel xml:lang="hu">faberendezés</skos:prefLabel>
		<skos:prefLabel xml:lang="no">trearbeid</skos:prefLabel>
		<skos:prefLabel xml:lang="hr">drveni predmeti</skos:prefLabel>
		<skos:altLabel xml:lang="de">Kunsttischlerei</skos:altLabel>
		<skos:exactMatch rdf:resource="http://vocab.getty.edu/aat/300015348"/>
		<skos:editorialNote xml:lang="en">PPObjectType</skos:editorialNote>
		<skos:scopeNote xml:lang="en">Interior fittings of wood, such as moldings and staircases; also any visual work done in wood, or with wooden objects or parts made of wood.</skos:scopeNote>
	</skos:Concept>
	<skos:Concept rdf:about="http://partage.vocnet.org/part00061">
		<skos:inScheme rdf:resource="http://partage.vocnet.org/MicroObjectTypes"/>
		<skos:prefLabel xml:lang="en">textiles</skos:prefLabel>
		<skos:altLabel xml:lang="de">Textilwaren</skos:altLabel>
		<skos:altLabel xml:lang="de">Textilien</skos:altLabel>
		<skos:prefLabel xml:lang="sv">textilier</skos:prefLabel>
		<skos:prefLabel xml:lang="fi">tekstiilit</skos:prefLabel>
		<skos:prefLabel xml:lang="es">textiles</skos:prefLabel>
		<skos:prefLabel xml:lang="sl">tkanine</skos:prefLabel>
		<skos:altLabel xml:lang="pt">produto têxtil</skos:altLabel>
		<skos:prefLabel xml:lang="pt">têxtil</skos:prefLabel>
		<skos:prefLabel xml:lang="pl">tkaniny</skos:prefLabel>
		<skos:prefLabel xml:lang="nl">textilia</skos:prefLabel>
		<skos:prefLabel xml:lang="it">tessuti</skos:prefLabel>
		<skos:prefLabel xml:lang="cs">textil</skos:prefLabel>
		<skos:prefLabel xml:lang="ca">tèxtils</skos:prefLabel>
		<skos:prefLabel xml:lang="fr">textile</skos:prefLabel>
		<skos:prefLabel xml:lang="hu">textil</skos:prefLabel>
		<skos:prefLabel xml:lang="no">tekstil</skos:prefLabel>
		<skos:prefLabel xml:lang="hr">tekstilni predmeti</skos:prefLabel>
		<skos:prefLabel xml:lang="de">Textilkunst</skos:prefLabel>
		<skos:exactMatch rdf:resource="http://vocab.getty.edu/aat/300014063"/>
		<skos:editorialNote xml:lang="en">PPObjectType</skos:editorialNote>
		<skos:scopeNote xml:lang="en">Refers collectively to items made of textile materials. For the general category of these materials, see "textile materials."</skos:scopeNote>
	</skos:Concept>
	<skos:Concept rdf:about="http://partage.vocnet.org/part00062">
		<skos:inScheme rdf:resource="http://partage.vocnet.org/MicroObjectTypes"/>
		<skos:prefLabel xml:lang="en">metalwork</skos:prefLabel>
		<skos:prefLabel xml:lang="nl">metaalwerk</skos:prefLabel>
		<skos:prefLabel xml:lang="it">metalli lavorati</skos:prefLabel>
		<skos:prefLabel xml:lang="cs">práce v kovu</skos:prefLabel>
		<skos:prefLabel xml:lang="ca">obra de metal·listeria</skos:prefLabel>
		<skos:altLabel xml:lang="de">Metallwaren</skos:altLabel>
		<skos:prefLabel xml:lang="de">Metallarbeiten</skos:prefLabel>
		<skos:prefLabel xml:lang="sv">metallarbeten</skos:prefLabel>
		<skos:prefLabel xml:lang="fi">metallityöt</skos:prefLabel>
		<skos:altLabel xml:lang="es">obra de metal</skos:altLabel>
		<skos:prefLabel xml:lang="es">obra de metalistería</skos:prefLabel>
		<skos:prefLabel xml:lang="sl">kovinski izdelki</skos:prefLabel>
		<skos:prefLabel xml:lang="pt">objeto em metal</skos:prefLabel>
		<skos:prefLabel xml:lang="pl">wyroby z metalu</skos:prefLabel>
		<skos:prefLabel xml:lang="fr">œuvre d'art en métal</skos:prefLabel>
		<skos:prefLabel xml:lang="hu">ötvösség</skos:prefLabel>
		<skos:prefLabel xml:lang="no">metallarbeid</skos:prefLabel>
		<skos:prefLabel xml:lang="hr">metalni predmeti</skos:prefLabel>
		<skos:exactMatch rdf:resource="http://vocab.getty.edu/aat/300015336"/>
		<skos:editorialNote xml:lang="en">PPObjectType</skos:editorialNote>
		<skos:scopeNote xml:lang="en">Refers to the products of metalworking, particularly metal objects of artistic merit.</skos:scopeNote>
	</skos:Concept>
	<skos:Concept rdf:about="http://partage.vocnet.org/part00063">
		<skos:inScheme rdf:resource="http://partage.vocnet.org/MicroObjectTypes"/>
		<skos:prefLabel xml:lang="en">glassware</skos:prefLabel>
		<skos:prefLabel xml:lang="de">Glas</skos:prefLabel>
		<skos:prefLabel xml:lang="sv">glasservis</skos:prefLabel>
		<skos:prefLabel xml:lang="fi">lasiesineet</skos:prefLabel>
		<skos:prefLabel xml:lang="es">cristalería</skos:prefLabel>
		<skos:prefLabel xml:lang="sl">stekleno posodje</skos:prefLabel>
		<skos:prefLabel xml:lang="pt">objetos de vidro</skos:prefLabel>
		<skos:prefLabel xml:lang="pl">szkło</skos:prefLabel>
		<skos:prefLabel xml:lang="nl">glaswerk</skos:prefLabel>
		<skos:prefLabel xml:lang="it">oggetti di vetro</skos:prefLabel>
		<skos:prefLabel xml:lang="cs">sklo</skos:prefLabel>
		<skos:prefLabel xml:lang="ca">cristalleria</skos:prefLabel>
		<skos:prefLabel xml:lang="fr">verrerie</skos:prefLabel>
		<skos:prefLabel xml:lang="hu">üveg</skos:prefLabel>
		<skos:prefLabel xml:lang="no">glasstøy</skos:prefLabel>
		<skos:prefLabel xml:lang="hr">stakleni predmeti</skos:prefLabel>
		<skos:exactMatch rdf:resource="http://vocab.getty.edu/aat/300010898"/>
		<skos:editorialNote xml:lang="en">PPObjectType</skos:editorialNote>
		<skos:scopeNote xml:lang="de">Articles made of glass; especially tableware of glass used in serving food and drink.</skos:scopeNote>
	</skos:Concept>
	<skos:Concept rdf:about="http://partage.vocnet.org/part00064">
		<skos:inScheme rdf:resource="http://partage.vocnet.org/MicroObjectTypes"/>
		<skos:hiddenLabel xml:lang="en">ceramics (objects)</skos:hiddenLabel>
		<skos:prefLabel xml:lang="en">ceramics</skos:prefLabel>
		<skos:prefLabel xml:lang="de">Keramik</skos:prefLabel>
		<skos:prefLabel xml:lang="sv">keramik</skos:prefLabel>
		<skos:prefLabel xml:lang="fi">keramiikka</skos:prefLabel>
		<skos:prefLabel xml:lang="es">cerámica</skos:prefLabel>
		<skos:prefLabel xml:lang="sl">keramika</skos:prefLabel>
		<skos:prefLabel xml:lang="pt">cerâmica</skos:prefLabel>
		<skos:prefLabel xml:lang="pl">ceramika</skos:prefLabel>
		<skos:prefLabel xml:lang="nl">keramiek</skos:prefLabel>
		<skos:prefLabel xml:lang="it">ceramica</skos:prefLabel>
		<skos:prefLabel xml:lang="cs">keramika</skos:prefLabel>
		<skos:prefLabel xml:lang="ca">ceràmica</skos:prefLabel>
		<skos:prefLabel xml:lang="fr">céramique</skos:prefLabel>
		<skos:prefLabel xml:lang="hu">kerámia</skos:prefLabel>
		<skos:prefLabel xml:lang="no">keramikk</skos:prefLabel>
		<skos:prefLabel xml:lang="hr">keramika</skos:prefLabel>
		<skos:narrower rdf:resource="http://partage.vocnet.org/part00223"/>
		<skos:narrower rdf:resource="http://partage.vocnet.org/part00225"/>
		<skos:exactMatch rdf:resource="http://vocab.getty.edu/aat/300151343"/>
		<skos:editorialNote xml:lang="en">PPObjectType</skos:editorialNote>
		<skos:scopeNote xml:lang="en">Refers in general to articles made of ceramic, which is any of various hard, brittle, heat-resistant and corrosion-resistant materials made by shaping and then firing a nonmetallic mineral, such as clay, at a high temperature. Earthenware, porcelain, and brick products are examples of ceramics.</skos:scopeNote>
	</skos:Concept>
	<skos:Concept rdf:about="http://partage.vocnet.org/part00066">
		<skos:inScheme rdf:resource="http://partage.vocnet.org/MicroObjectTypes"/>
		<skos:prefLabel xml:lang="en">posters</skos:prefLabel>
		<skos:prefLabel xml:lang="sv">affischer</skos:prefLabel>
		<skos:prefLabel xml:lang="fi">julisteet</skos:prefLabel>
		<skos:prefLabel xml:lang="es">carteles</skos:prefLabel>
		<skos:prefLabel xml:lang="sl">plakati</skos:prefLabel>
		<skos:altLabel xml:lang="pt">posters</skos:altLabel>
		<skos:prefLabel xml:lang="pt">poster</skos:prefLabel>
		<skos:prefLabel xml:lang="pl">plakaty</skos:prefLabel>
		<skos:prefLabel xml:lang="nl">posters</skos:prefLabel>
		<skos:prefLabel xml:lang="it">manifesti</skos:prefLabel>
		<skos:prefLabel xml:lang="cs">plakát</skos:prefLabel>
		<skos:prefLabel xml:lang="ca">cartells</skos:prefLabel>
		<skos:altLabel xml:lang="de">Plakat</skos:altLabel>
		<skos:prefLabel xml:lang="de">Plakate</skos:prefLabel>
		<skos:prefLabel xml:lang="fr">affiche</skos:prefLabel>
		<skos:prefLabel xml:lang="hu">plakát</skos:prefLabel>
		<skos:prefLabel xml:lang="no">plakat</skos:prefLabel>
		<skos:prefLabel xml:lang="hr">plakati</skos:prefLabel>
		<skos:exactMatch rdf:resource="http://vocab.getty.edu/aat/300027221"/>
		<skos:editorialNote xml:lang="en">PPObjectType</skos:editorialNote>
		<skos:scopeNote xml:lang="en">Notices, usually decorative or pictorial, intended to be posted to advertise, promote, or publicize an activity, cause, product, or service; also, decorative, mass-produced prints intended for hanging. For small printed notices or advertisements intended for distribution by hand, use "handbills."</skos:scopeNote>
	</skos:Concept>
	<skos:Concept rdf:about="http://partage.vocnet.org/part00078">
		<skos:inScheme rdf:resource="http://partage.vocnet.org/MicroObjectTypes"/>
		<skos:prefLabel xml:lang="en">jewellery</skos:prefLabel>
		<skos:altLabel xml:lang="en">jewelry</skos:altLabel>
		<skos:prefLabel xml:lang="pt">joalharia</skos:prefLabel>
		<skos:prefLabel xml:lang="pl">biżuteria</skos:prefLabel>
		<skos:prefLabel xml:lang="nl">sieraden</skos:prefLabel>
		<skos:prefLabel xml:lang="it">gioielli</skos:prefLabel>
		<skos:prefLabel xml:lang="cs">šperk</skos:prefLabel>
		<skos:prefLabel xml:lang="ca">joies</skos:prefLabel>
		<skos:prefLabel xml:lang="de">Schmuck</skos:prefLabel>
		<skos:prefLabel xml:lang="sv">smycken</skos:prefLabel>
		<skos:prefLabel xml:lang="fi">korut</skos:prefLabel>
		<skos:hiddenLabel xml:lang="es">joya</skos:hiddenLabel>
		<skos:prefLabel xml:lang="es">joyas</skos:prefLabel>
		<skos:prefLabel xml:lang="sl">nakit</skos:prefLabel>
		<skos:altLabel xml:lang="pt">jóias</skos:altLabel>
		<skos:prefLabel xml:lang="hr">nakit</skos:prefLabel>
		<skos:prefLabel xml:lang="no">smykker</skos:prefLabel>
		<skos:prefLabel xml:lang="hu">ékszer</skos:prefLabel>
		<skos:prefLabel xml:lang="fr">bijou</skos:prefLabel>
		<skos:broader rdf:resource="http://partage.vocnet.org/part00081"/>
		<skos:exactMatch rdf:resource="http://vocab.getty.edu/aat/300209286"/>
		<skos:editorialNote xml:lang="en">PPObjectType</skos:editorialNote>
		<skos:scopeNote xml:lang="en">Ornaments such as bracelets, necklaces, and rings, of precious or semiprecious materials worn or carried on the person for adornment; also includes similar articles worn or carried for devotional or mourning purposes.</skos:scopeNote>
	</skos:Concept>
	<skos:Concept rdf:about="http://partage.vocnet.org/part00081">
		<skos:inScheme rdf:resource="http://partage.vocnet.org/MicroObjectTypes"/>
		<skos:hiddenLabel xml:lang="en">costume (mode of fashion)</skos:hiddenLabel>
		<skos:prefLabel xml:lang="en">costume</skos:prefLabel>
		<skos:hiddenLabel xml:lang="de">Kleidung</skos:hiddenLabel>
		<skos:prefLabel xml:lang="de">Mode</skos:prefLabel>
		<skos:prefLabel xml:lang="sv">dräkt</skos:prefLabel>
		<skos:prefLabel xml:lang="fi">asut</skos:prefLabel>
		<skos:prefLabel xml:lang="es">indumentaria</skos:prefLabel>
		<skos:prefLabel xml:lang="sl">noše</skos:prefLabel>
		<skos:prefLabel xml:lang="pt">traje</skos:prefLabel>
		<skos:prefLabel xml:lang="pl">akcesoria mody</skos:prefLabel>
		<skos:prefLabel xml:lang="nl">kleding</skos:prefLabel>
		<skos:prefLabel xml:lang="it">moda</skos:prefLabel>
		<skos:prefLabel xml:lang="cs">móda</skos:prefLabel>
		<skos:prefLabel xml:lang="ca">indumentària</skos:prefLabel>
		<skos:prefLabel xml:lang="hr">odjeća</skos:prefLabel>
		<skos:prefLabel xml:lang="no">drakt</skos:prefLabel>
		<skos:prefLabel xml:lang="hu">viselet</skos:prefLabel>
		<skos:prefLabel xml:lang="fr">costume</skos:prefLabel>
		<skos:narrower rdf:resource="http://partage.vocnet.org/part00078"/>
		<skos:exactMatch rdf:resource="http://vocab.getty.edu/aat/300178802"/>
		<skos:editorialNote xml:lang="en">PPObjectType</skos:editorialNote>
		<skos:scopeNote xml:lang="en">The mode or fashion of personal attire and dress, including the way of wearing the hair, style of clothing, jewelry, crowns, scepters, and other accessories of personal adornment, belonging to a particular nation, class, period, or special occasion, including all items worn or carried by people for warmth, protection, embellishment, or symbolic purposes. In English, generally expressed in the singular.</skos:scopeNote>
	</skos:Concept>
	<skos:Concept rdf:about="http://partage.vocnet.org/part00087">
		<skos:inScheme rdf:resource="http://partage.vocnet.org/MicroObjectTypes"/>
		<skos:prefLabel xml:lang="en">timepieces</skos:prefLabel>
		<skos:prefLabel xml:lang="it">orologi</skos:prefLabel>
		<skos:prefLabel xml:lang="cs">hodiny a hodinky</skos:prefLabel>
		<skos:prefLabel xml:lang="ca">rellotges</skos:prefLabel>
		<skos:prefLabel xml:lang="de">Uhren</skos:prefLabel>
		<skos:prefLabel xml:lang="sv">ur</skos:prefLabel>
		<skos:prefLabel xml:lang="fi">kellot</skos:prefLabel>
		<skos:altLabel xml:lang="es">indicadores de tiempo</skos:altLabel>
		<skos:prefLabel xml:lang="es">relojes</skos:prefLabel>
		<skos:prefLabel xml:lang="sl">ure</skos:prefLabel>
		<skos:altLabel xml:lang="pt">relógios</skos:altLabel>
		<skos:prefLabel xml:lang="pt">relógio</skos:prefLabel>
		<skos:prefLabel xml:lang="pl">czasomierze</skos:prefLabel>
		<skos:prefLabel xml:lang="nl">uurwerken</skos:prefLabel>
		<skos:prefLabel xml:lang="hr">satovi</skos:prefLabel>
		<skos:prefLabel xml:lang="no">ur</skos:prefLabel>
		<skos:prefLabel xml:lang="hu">óra</skos:prefLabel>
		<skos:prefLabel xml:lang="fr">horlogerie</skos:prefLabel>
		<skos:altLabel xml:lang="de">Uhr</skos:altLabel>
		<skos:exactMatch rdf:resource="http://vocab.getty.edu/aat/300041573"/>
		<skos:editorialNote xml:lang="en">PPObjectType</skos:editorialNote>
		<skos:scopeNote xml:lang="de">Devices for measuring and recording the passage of time.</skos:scopeNote>
	</skos:Concept>
	<skos:Concept rdf:about="http://partage.vocnet.org/part00094">
		<skos:inScheme rdf:resource="http://partage.vocnet.org/MicroObjectTypes"/>
		<skos:prefLabel xml:lang="en">books</skos:prefLabel>
		<skos:prefLabel xml:lang="de">Bücher</skos:prefLabel>
		<skos:altLabel xml:lang="de">Buch</skos:altLabel>
		<skos:prefLabel xml:lang="sv">böcker</skos:prefLabel>
		<skos:prefLabel xml:lang="fi">kirjat</skos:prefLabel>
		<skos:prefLabel xml:lang="es">libros</skos:prefLabel>
		<skos:prefLabel xml:lang="sl">knjige</skos:prefLabel>
		<skos:altLabel xml:lang="pt">livros</skos:altLabel>
		<skos:prefLabel xml:lang="pt">livro</skos:prefLabel>
		<skos:prefLabel xml:lang="pl">książki</skos:prefLabel>
		<skos:prefLabel xml:lang="nl">boeken</skos:prefLabel>
		<skos:prefLabel xml:lang="it">libri</skos:prefLabel>
		<skos:prefLabel xml:lang="cs">kniha</skos:prefLabel>
		<skos:prefLabel xml:lang="ca">llibres</skos:prefLabel>
		<skos:prefLabel xml:lang="fr">livre</skos:prefLabel>
		<skos:prefLabel xml:lang="hu">könyv</skos:prefLabel>
		<skos:prefLabel xml:lang="no">bøker</skos:prefLabel>
		<skos:prefLabel xml:lang="hr">knjige</skos:prefLabel>
		<skos:exactMatch rdf:resource="http://vocab.getty.edu/aat/300028051"/>
		<skos:editorialNote xml:lang="en">PPObjectType</skos:editorialNote>
		<skos:scopeNote xml:lang="en">Items comprising a collection of leaves of paper, parchment, wood, stiffened textile, ivory, metal tablets, or other flat material, that are blank, written on, or printed, and are strung or bound together in a volume.</skos:scopeNote>
	</skos:Concept>
	<skos:Concept rdf:about="http://partage.vocnet.org/part00099">
		<skos:inScheme rdf:resource="http://partage.vocnet.org/MicroObjectTypes"/>
		<skos:prefLabel xml:lang="en">furniture</skos:prefLabel>
		<skos:altLabel xml:lang="de">Mobiliar</skos:altLabel>
		<skos:prefLabel xml:lang="de">Möbel</skos:prefLabel>
		<skos:prefLabel xml:lang="sv">möbler</skos:prefLabel>
		<skos:prefLabel xml:lang="fi">huonekalut</skos:prefLabel>
		<skos:prefLabel xml:lang="es">muebles</skos:prefLabel>
		<skos:prefLabel xml:lang="sl">pohištvo</skos:prefLabel>
		<skos:altLabel xml:lang="pt">mobília</skos:altLabel>
		<skos:prefLabel xml:lang="pt">mobiliário</skos:prefLabel>
		<skos:prefLabel xml:lang="pl">meble</skos:prefLabel>
		<skos:prefLabel xml:lang="nl">meubilair</skos:prefLabel>
		<skos:prefLabel xml:lang="it">mobilia</skos:prefLabel>
		<skos:prefLabel xml:lang="cs">nábytek</skos:prefLabel>
		<skos:prefLabel xml:lang="ca">mobles</skos:prefLabel>
		<skos:prefLabel xml:lang="hr">namještaj</skos:prefLabel>
		<skos:prefLabel xml:lang="no">møbler</skos:prefLabel>
		<skos:prefLabel xml:lang="hu">bútor</skos:prefLabel>
		<skos:prefLabel xml:lang="fr">mobilier</skos:prefLabel>
		<skos:broader rdf:resource="http://partage.vocnet.org/part00100"/>
		<skos:exactMatch rdf:resource="http://vocab.getty.edu/aat/ 300037680"/>
		<skos:editorialNote xml:lang="en">PPObjectType</skos:editorialNote>
		<skos:scopeNote xml:lang="en">Movable or fixed objects or equipment, which may be either functional or ornamental, for use in a dwelling, business, or public space.</skos:scopeNote>
	</skos:Concept>
	<skos:Concept rdf:about="http://partage.vocnet.org/part00100">
		<skos:inScheme rdf:resource="http://partage.vocnet.org/MicroObjectTypes"/>
		<skos:hiddenLabel xml:lang="en">furnishings (artifacts)</skos:hiddenLabel>
		<skos:prefLabel xml:lang="en">furnishings</skos:prefLabel>
		<skos:altLabel xml:lang="de">Raumausstattung</skos:altLabel>
		<skos:prefLabel xml:lang="de">Inneneinrichtung</skos:prefLabel>
		<skos:prefLabel xml:lang="sv">möblemang</skos:prefLabel>
		<skos:prefLabel xml:lang="fi">sisustus</skos:prefLabel>
		<skos:prefLabel xml:lang="es">mobiliario</skos:prefLabel>
		<skos:prefLabel xml:lang="sl">oprema</skos:prefLabel>
		<skos:prefLabel xml:lang="pt">recheio</skos:prefLabel>
		<skos:prefLabel xml:lang="pl">wyroby użytkowe</skos:prefLabel>
		<skos:prefLabel xml:lang="nl">interieurinrichting</skos:prefLabel>
		<skos:prefLabel xml:lang="it">oggetti di uso domestico</skos:prefLabel>
		<skos:prefLabel xml:lang="cs">bytové vybavení</skos:prefLabel>
		<skos:prefLabel xml:lang="ca">mobiliari</skos:prefLabel>
		<skos:prefLabel xml:lang="hu">berendezés</skos:prefLabel>
		<skos:prefLabel xml:lang="no">inventar</skos:prefLabel>
		<skos:prefLabel xml:lang="hr">oprema</skos:prefLabel>
		<skos:narrower rdf:resource="http://partage.vocnet.org/part00055"/>
		<skos:narrower rdf:resource="http://partage.vocnet.org/part00099"/>
		<skos:narrower rdf:resource="http://partage.vocnet.org/part00109"/>
		<skos:narrower rdf:resource="http://partage.vocnet.org/part00177"/>
		<skos:exactMatch rdf:resource="http://vocab.getty.edu/aat/300037336"/>
		<skos:editorialNote xml:lang="en">PPObjectType</skos:editorialNote>
		<skos:scopeNote xml:lang="en">Artifacts originally created to facilitate human activity and to provide for physical needs of people in or around a building generally by offering comfort, convenience, or protection</skos:scopeNote>
	</skos:Concept>
	<skos:Concept rdf:about="http://partage.vocnet.org/part00109">
		<skos:inScheme rdf:resource="http://partage.vocnet.org/MicroObjectTypes"/>
		<skos:prefLabel xml:lang="en">lighting devices</skos:prefLabel>
		<skos:prefLabel xml:lang="de">Beleuchtung</skos:prefLabel>
		<skos:altLabel xml:lang="es">artefactos de iluminación</skos:altLabel>
		<skos:prefLabel xml:lang="es">luces</skos:prefLabel>
		<skos:prefLabel xml:lang="sl">svetila</skos:prefLabel>
		<skos:altLabel xml:lang="pt">candeeiro</skos:altLabel>
		<skos:prefLabel xml:lang="pt">iluminação</skos:prefLabel>
		<skos:prefLabel xml:lang="pl">oświetlenie</skos:prefLabel>
		<skos:prefLabel xml:lang="nl">verlichtingsmiddelen</skos:prefLabel>
		<skos:prefLabel xml:lang="it">illuminazione</skos:prefLabel>
		<skos:prefLabel xml:lang="cs">osvětlovací tělesa</skos:prefLabel>
		<skos:prefLabel xml:lang="ca">llums</skos:prefLabel>
		<skos:prefLabel xml:lang="fi">valaisimet</skos:prefLabel>
		<skos:prefLabel xml:lang="sv">armaturer</skos:prefLabel>
		<skos:altLabel xml:lang="de">Leuchten</skos:altLabel>
		<skos:prefLabel xml:lang="fr">lumière</skos:prefLabel>
		<skos:prefLabel xml:lang="hu">lámpa</skos:prefLabel>
		<skos:prefLabel xml:lang="no">belysning</skos:prefLabel>
		<skos:prefLabel xml:lang="hr">rasvjetna tijela</skos:prefLabel>
		<skos:broader rdf:resource="http://partage.vocnet.org/part00100"/>
		<skos:exactMatch rdf:resource="http://vocab.getty.edu/aat/300037581"/>
		<skos:editorialNote xml:lang="en">PPObjectType</skos:editorialNote>
		<skos:scopeNote xml:lang="en">Apparatus, fixed or portable, whose primary purpose is to produce artificial light.</skos:scopeNote>
	</skos:Concept>
	<skos:Concept rdf:about="http://partage.vocnet.org/part00128">
		<skos:inScheme rdf:resource="http://partage.vocnet.org/MicroObjectTypes"/>
		<skos:prefLabel xml:lang="en">tableware</skos:prefLabel>
		<skos:prefLabel xml:lang="de">Tafelgeschirr</skos:prefLabel>
		<skos:prefLabel xml:lang="sv">serviser</skos:prefLabel>
		<skos:altLabel xml:lang="fi">kattaus</skos:altLabel>
		<skos:prefLabel xml:lang="fi">ruokailuvälineet</skos:prefLabel>
		<skos:altLabel xml:lang="es">servicios de mesa</skos:altLabel>
		<skos:prefLabel xml:lang="es">servicio de mesa</skos:prefLabel>
		<skos:prefLabel xml:lang="sl">namizno posodje</skos:prefLabel>
		<skos:prefLabel xml:lang="pt">artigos para cozinha e sala de jantar</skos:prefLabel>
		<skos:prefLabel xml:lang="pl">zastawa stołowa</skos:prefLabel>
		<skos:prefLabel xml:lang="nl">tafelgerei</skos:prefLabel>
		<skos:prefLabel xml:lang="it">stoviglie da tavola</skos:prefLabel>
		<skos:prefLabel xml:lang="cs">stolní náčiní</skos:prefLabel>
		<skos:prefLabel xml:lang="ca">parament de taula</skos:prefLabel>
		<skos:prefLabel xml:lang="hr">stolno posuđe</skos:prefLabel>
		<skos:prefLabel xml:lang="fr">vaisselle</skos:prefLabel>
		<skos:prefLabel xml:lang="hu">asztali készlet</skos:prefLabel>
		<skos:prefLabel xml:lang="no">dekketøy</skos:prefLabel>
		<skos:exactMatch rdf:resource="http://vocab.getty.edu/aat/300043196"/>
		<skos:editorialNote xml:lang="en">PPObjectType</skos:editorialNote>
		<skos:scopeNote xml:lang="en">Articles, collectively, that are generally used for serving food at the table, including various types of flatware, cutlery, hollowware, plates, and accessories, such as coasters and napkin rings, but not necessarily constituting a service.</skos:scopeNote>
	</skos:Concept>
	<skos:Concept rdf:about="http://partage.vocnet.org/part00139">
		<skos:inScheme rdf:resource="http://partage.vocnet.org/MicroObjectTypes"/>
		<skos:prefLabel xml:lang="en">promotional materials</skos:prefLabel>
		<skos:altLabel xml:lang="de">Werbegrafik</skos:altLabel>
		<skos:altLabel xml:lang="de">Gebrauchsgraphik</skos:altLabel>
		<skos:prefLabel xml:lang="de">Gebrauchsgrafik</skos:prefLabel>
		<skos:prefLabel xml:lang="sv">reklam</skos:prefLabel>
		<skos:prefLabel xml:lang="fi">mainokset</skos:prefLabel>
		<skos:prefLabel xml:lang="es">materiales promocionales</skos:prefLabel>
		<skos:prefLabel xml:lang="sl">promocijska gradiva</skos:prefLabel>
		<skos:prefLabel xml:lang="pt">materiais promocionais</skos:prefLabel>
		<skos:prefLabel xml:lang="pl">materiały reklamowe</skos:prefLabel>
		<skos:prefLabel xml:lang="nl">reclamematerialen</skos:prefLabel>
		<skos:prefLabel xml:lang="it">materiale promozionale</skos:prefLabel>
		<skos:prefLabel xml:lang="cs">propagační materiál</skos:prefLabel>
		<skos:prefLabel xml:lang="ca">materials promocionals</skos:prefLabel>
		<skos:prefLabel xml:lang="hr">promotivni materijali</skos:prefLabel>
		<skos:prefLabel xml:lang="no">markedsføringsmateriale</skos:prefLabel>
		<skos:prefLabel xml:lang="hu">reklámanyag</skos:prefLabel>
		<skos:prefLabel xml:lang="fr">matériel promotionnel</skos:prefLabel>
		<skos:exactMatch rdf:resource="http://vocab.getty.edu/aat/300249572"/>
		<skos:editorialNote xml:lang="en">PPObjectType</skos:editorialNote>
		<skos:scopeNote xml:lang="en">Printed matter or objects devised to advertise or promote products, causes, or other concerns, especially those items given away to prospective consumers, clients, or contributors. Not used with reference to items produced before the late 19th century.</skos:scopeNote>
	</skos:Concept>
	<skos:Concept rdf:about="http://partage.vocnet.org/part00151">
		<skos:inScheme rdf:resource="http://partage.vocnet.org/MicroObjectTypes"/>
		<skos:hiddenLabel xml:lang="en">architecture (object genre)</skos:hiddenLabel>
		<skos:prefLabel xml:lang="en">architecture</skos:prefLabel>
		<skos:prefLabel xml:lang="sv">arkitektur</skos:prefLabel>
		<skos:prefLabel xml:lang="fi">arkkitehtuuri</skos:prefLabel>
		<skos:prefLabel xml:lang="es">arquitectura</skos:prefLabel>
		<skos:prefLabel xml:lang="sl">arhitekturna dela</skos:prefLabel>
		<skos:prefLabel xml:lang="pt">arquitetura</skos:prefLabel>
		<skos:prefLabel xml:lang="pl">architektura</skos:prefLabel>
		<skos:prefLabel xml:lang="nl">architectuur</skos:prefLabel>
		<skos:prefLabel xml:lang="it">architettura</skos:prefLabel>
		<skos:prefLabel xml:lang="cs">architektura</skos:prefLabel>
		<skos:prefLabel xml:lang="de">Architektur</skos:prefLabel>
		<skos:prefLabel xml:lang="ca">arquitectura</skos:prefLabel>
		<skos:altLabel xml:lang="de">Baukunst</skos:altLabel>
		<skos:prefLabel xml:lang="hr">arhitektura</skos:prefLabel>
		<skos:prefLabel xml:lang="fr">architecture</skos:prefLabel>
		<skos:prefLabel xml:lang="hu">építészet</skos:prefLabel>
		<skos:prefLabel xml:lang="no">arkitektur</skos:prefLabel>
		<skos:exactMatch rdf:resource="http://vocab.getty.edu/aat/300263552"/>
		<skos:editorialNote xml:lang="en">PPObjectType</skos:editorialNote>
		<skos:scopeNote xml:lang="en">Structures or parts of structures that are the result of conscious construction, are of practical use, are relatively stable and permanent, and are of a size and scale appropriate for--but not limited to--habitable buildings. Works of architecture are manifestations of the built environment that is typically classified as fine art, meaning it is generally considered to have aesthetic value, was designed by an architect (whether or not his or her name is known), and constructed with skilled labor. For the art or science of designing and building structures, use "architecture (discipline)."</skos:scopeNote>
	</skos:Concept>
	<skos:Concept rdf:about="http://partage.vocnet.org/part00177">
		<skos:inScheme rdf:resource="http://partage.vocnet.org/MicroObjectTypes"/>
		<skos:prefLabel xml:lang="en">wallpapers</skos:prefLabel>
		<skos:prefLabel xml:lang="de">Tapeten</skos:prefLabel>
		<skos:prefLabel xml:lang="sv">tapeter</skos:prefLabel>
		<skos:prefLabel xml:lang="fi">tapetit</skos:prefLabel>
		<skos:altLabel xml:lang="es">papel pintado para paredes</skos:altLabel>
		<skos:prefLabel xml:lang="es">papel pintado</skos:prefLabel>
		<skos:prefLabel xml:lang="sl">tapete</skos:prefLabel>
		<skos:prefLabel xml:lang="pt">papel de parede</skos:prefLabel>
		<skos:prefLabel xml:lang="pl">tapety</skos:prefLabel>
		<skos:prefLabel xml:lang="nl">behang</skos:prefLabel>
		<skos:prefLabel xml:lang="it">carte da parati</skos:prefLabel>
		<skos:prefLabel xml:lang="cs">tapety</skos:prefLabel>
		<skos:prefLabel xml:lang="ca">paper pintat</skos:prefLabel>
		<skos:prefLabel xml:lang="fr">papier peint</skos:prefLabel>
		<skos:prefLabel xml:lang="hu">tapéta</skos:prefLabel>
		<skos:prefLabel xml:lang="no">tapet</skos:prefLabel>
		<skos:prefLabel xml:lang="hr">tapete</skos:prefLabel>
		<skos:altLabel xml:lang="de">Tapete</skos:altLabel>
		<skos:broader rdf:resource="http://partage.vocnet.org/part00100"/>
		<skos:exactMatch rdf:resource="http://vocab.getty.edu/aat/300037366"/>
		<skos:editorialNote xml:lang="en">PPObjectType</skos:editorialNote>
		<skos:scopeNote xml:lang="en">Papers or paperlike materials, often decorative in nature, made primarily for attachment to walls and ceilings but sometimes applied to other surfaces.</skos:scopeNote>
	</skos:Concept>
	<skos:Concept rdf:about="http://partage.vocnet.org/part00181">
		<skos:inScheme rdf:resource="http://partage.vocnet.org/MicroObjectTypes"/>
		<skos:prefLabel xml:lang="en">recreational artifacts</skos:prefLabel>
		<skos:prefLabel xml:lang="de">Freizeitgegenstände</skos:prefLabel>
		<skos:prefLabel xml:lang="sv">rekreationsföremål</skos:prefLabel>
		<skos:prefLabel xml:lang="fi">vapaa-ajan välineet</skos:prefLabel>
		<skos:prefLabel xml:lang="es">artefactos recreativos</skos:prefLabel>
		<skos:prefLabel xml:lang="sl">pribor za rekreacijo</skos:prefLabel>
		<skos:prefLabel xml:lang="pt">objetos recreativos or objetos lúdicos</skos:prefLabel>
		<skos:prefLabel xml:lang="pl">przedmioty rekreacyjne</skos:prefLabel>
		<skos:prefLabel xml:lang="nl">ontspanningsmiddelen</skos:prefLabel>
		<skos:prefLabel xml:lang="it">oggetti per il tempo libero</skos:prefLabel>
		<skos:prefLabel xml:lang="cs">vybavení pro volnočasové aktivity</skos:prefLabel>
		<skos:prefLabel xml:lang="ca">objectes recreatius</skos:prefLabel>
		<skos:prefLabel xml:lang="fr">équipement de loisir</skos:prefLabel>
		<skos:prefLabel xml:lang="hu">szabadidős termékek</skos:prefLabel>
		<skos:prefLabel xml:lang="no">fritidsutstyr</skos:prefLabel>
		<skos:prefLabel xml:lang="hr">oprema za rekreaciju</skos:prefLabel>
		<skos:exactMatch rdf:resource="http://vocab.getty.edu/aat/300218781"/>
		<skos:editorialNote xml:lang="en">PPObjectType</skos:editorialNote>
		<skos:scopeNote xml:lang="en">Equipment and accessories used in any of a large array of activities that are engaged in for personal satisfaction or amusement during leisure time.</skos:scopeNote>
	</skos:Concept>
	<skos:Concept rdf:about="http://partage.vocnet.org/part00185">
		<skos:inScheme rdf:resource="http://partage.vocnet.org/MicroObjectTypes"/>
		<skos:prefLabel xml:lang="en">musical instruments</skos:prefLabel>
		<skos:prefLabel xml:lang="sv">musikinstrument</skos:prefLabel>
		<skos:prefLabel xml:lang="fi">soittimet</skos:prefLabel>
		<skos:prefLabel xml:lang="es">instrumentos musicales</skos:prefLabel>
		<skos:prefLabel xml:lang="sl">glasbila</skos:prefLabel>
		<skos:altLabel xml:lang="pt">instrumentos musicais</skos:altLabel>
		<skos:prefLabel xml:lang="pt">instrumento musical</skos:prefLabel>
		<skos:prefLabel xml:lang="pl">instrumenty muzyczne</skos:prefLabel>
		<skos:prefLabel xml:lang="nl">muziekinstrumenten</skos:prefLabel>
		<skos:prefLabel xml:lang="it">strumenti musicali</skos:prefLabel>
		<skos:prefLabel xml:lang="cs">hudební nástroje</skos:prefLabel>
		<skos:prefLabel xml:lang="ca">instruments musicals</skos:prefLabel>
		<skos:altLabel xml:lang="de">Musikinstrument</skos:altLabel>
		<skos:prefLabel xml:lang="de">Musikinstrumente</skos:prefLabel>
		<skos:prefLabel xml:lang="hr">glazbeni instrumenti</skos:prefLabel>
		<skos:prefLabel xml:lang="no">musikkinstrument</skos:prefLabel>
		<skos:prefLabel xml:lang="hu">hangszer</skos:prefLabel>
		<skos:prefLabel xml:lang="fr">instrument de musique</skos:prefLabel>
		<skos:exactMatch rdf:resource="http://vocab.getty.edu/aat/300041620"/>
		<skos:editorialNote xml:lang="en">PPObjectType</skos:editorialNote>
		<skos:scopeNote xml:lang="en">Sound-producing apparatuses whose primary function is to play music.</skos:scopeNote>
	</skos:Concept>
	<skos:Concept rdf:about="http://partage.vocnet.org/part00218">
		<skos:inScheme rdf:resource="http://partage.vocnet.org/MicroObjectTypes"/>
		<skos:prefLabel xml:lang="en">equipment</skos:prefLabel>
		<skos:prefLabel xml:lang="es">equipo</skos:prefLabel>
		<skos:prefLabel xml:lang="sl">pribor</skos:prefLabel>
		<skos:prefLabel xml:lang="pt">apetrechos</skos:prefLabel>
		<skos:altLabel xml:lang="pt">equipamento</skos:altLabel>
		<skos:prefLabel xml:lang="pl">wyposażenie</skos:prefLabel>
		<skos:prefLabel xml:lang="nl">uitrusting</skos:prefLabel>
		<skos:prefLabel xml:lang="it">strumenti</skos:prefLabel>
		<skos:prefLabel xml:lang="cs">vybavení</skos:prefLabel>
		<skos:prefLabel xml:lang="ca">equip</skos:prefLabel>
		<skos:altLabel xml:lang="fi">välineet</skos:altLabel>
		<skos:prefLabel xml:lang="fi">varusteet</skos:prefLabel>
		<skos:prefLabel xml:lang="de">Gerät</skos:prefLabel>
		<skos:altLabel xml:lang="de">Ausstattung</skos:altLabel>
		<skos:altLabel xml:lang="de">Gerätschaften</skos:altLabel>
		<skos:prefLabel xml:lang="hr">pribor</skos:prefLabel>
		<skos:prefLabel xml:lang="no">utstyr</skos:prefLabel>
		<skos:prefLabel xml:lang="hu">felszerelés</skos:prefLabel>
		<skos:prefLabel xml:lang="fr">équipement</skos:prefLabel>
		<skos:prefLabel xml:lang="sv">utrustning</skos:prefLabel>
		<skos:narrower rdf:resource="http://partage.vocnet.org/part00505"/>
		<skos:exactMatch rdf:resource="http://vocab.getty.edu/aat/300122241"/>
		<skos:editorialNote xml:lang="en">PPObjectType</skos:editorialNote>
		<skos:scopeNote xml:lang="en">Articles or physical resources used to equip a person or thing, such as the instruments used in an activity or operation.</skos:scopeNote>
	</skos:Concept>
	<skos:Concept rdf:about="http://partage.vocnet.org/part00221">
		<skos:inScheme rdf:resource="http://partage.vocnet.org/MicroObjectTypes"/>
		<skos:hiddenLabel xml:lang="en">embroidery (visual works)</skos:hiddenLabel>
		<skos:prefLabel xml:lang="en">embroidery</skos:prefLabel>
		<skos:prefLabel xml:lang="sv">broderi</skos:prefLabel>
		<skos:prefLabel xml:lang="es">bordado</skos:prefLabel>
		<skos:prefLabel xml:lang="sl">vezenine</skos:prefLabel>
		<skos:prefLabel xml:lang="pt">bordado</skos:prefLabel>
		<skos:prefLabel xml:lang="pl">haft</skos:prefLabel>
		<skos:prefLabel xml:lang="nl">borduurwerk</skos:prefLabel>
		<skos:prefLabel xml:lang="it">ricamo</skos:prefLabel>
		<skos:prefLabel xml:lang="cs">výšivka</skos:prefLabel>
		<skos:prefLabel xml:lang="ca">brodat</skos:prefLabel>
		<skos:prefLabel xml:lang="de">Stickerei</skos:prefLabel>
		<skos:prefLabel xml:lang="hr">vezivo</skos:prefLabel>
		<skos:prefLabel xml:lang="no">broderi</skos:prefLabel>
		<skos:prefLabel xml:lang="fr">broderie</skos:prefLabel>
		<skos:prefLabel xml:lang="fi">kirjonta</skos:prefLabel>
		<skos:exactMatch rdf:resource="http://vocab.getty.edu/aat/300264024"/>
		<skos:editorialNote xml:lang="en">PPObjectType</skos:editorialNote>
		<skos:scopeNote xml:lang="en">Refers to works characterized by a pattern or design executed in stitches using thread or fine wire. The designs are typically executed on textiles, but leather, paper, or another media may also be used; the designs may be intended to be framed, or to decorate apparel, bed linens, furniture coverings, pillows, altar cloths, ceremonial hangings, or other items.</skos:scopeNote>
	</skos:Concept>
	<skos:Concept rdf:about="http://partage.vocnet.org/part00222">
		<skos:inScheme rdf:resource="http://partage.vocnet.org/MicroObjectTypes"/>
		<skos:hiddenLabel xml:lang="en">lace (needlework)</skos:hiddenLabel>
		<skos:prefLabel xml:lang="en">lace</skos:prefLabel>
		<skos:hiddenLabel xml:lang="de">Spitze</skos:hiddenLabel>
		<skos:prefLabel xml:lang="de">Spitzen</skos:prefLabel>
		<skos:prefLabel xml:lang="sv">spets</skos:prefLabel>
		<skos:prefLabel xml:lang="fi">pitsit</skos:prefLabel>
		<skos:prefLabel xml:lang="es">encaje</skos:prefLabel>
		<skos:prefLabel xml:lang="sl">čipke</skos:prefLabel>
		<skos:prefLabel xml:lang="pt">renda</skos:prefLabel>
		<skos:prefLabel xml:lang="pl">koronka</skos:prefLabel>
		<skos:prefLabel xml:lang="nl">kant</skos:prefLabel>
		<skos:prefLabel xml:lang="it">merletti</skos:prefLabel>
		<skos:prefLabel xml:lang="cs">krajka</skos:prefLabel>
		<skos:prefLabel xml:lang="ca">puntes</skos:prefLabel>
		<skos:prefLabel xml:lang="fr">dentelle</skos:prefLabel>
		<skos:prefLabel xml:lang="hu">csipke</skos:prefLabel>
		<skos:prefLabel xml:lang="no">lasur</skos:prefLabel>
		<skos:prefLabel xml:lang="hr">čipka</skos:prefLabel>
		<skos:exactMatch rdf:resource="http://vocab.getty.edu/aat/300132861"/>
		<skos:editorialNote xml:lang="en">PPObjectType</skos:editorialNote>
		<skos:scopeNote xml:lang="en">Refers to a fine, openwork ornamental textile work formed by looping, interlacing, twisting, plaiting, or braiding threads of linen, cotton, silk, hair, metal, or another fiber to form designs or patterns. Lace may be made with a needle or with bobbins. Embroidery may be added. Modern lace may be made by machine. Openwork fabrics made on a loom and ornamental openwork knitting are generally not classified as lace. Lace is often white or monochromatic. True lace developed in the fourteenth century in Europe and the Middle East, although ornamented openwork fabrics were known in ancient cultures, including the Egyptian culture. Lace may be used as a border, edging, or insert on linens or apparel; it is also formed into large pieces of cloth used for hangings, draperies, apparel, or other items.</skos:scopeNote>
	</skos:Concept>
	<skos:Concept rdf:about="http://partage.vocnet.org/part00223">
		<skos:inScheme rdf:resource="http://partage.vocnet.org/MicroObjectTypes"/>
		<skos:prefLabel xml:lang="en">earthenware</skos:prefLabel>
		<skos:prefLabel xml:lang="nl">aardewerk</skos:prefLabel>
		<skos:prefLabel xml:lang="it">terracotta</skos:prefLabel>
		<skos:prefLabel xml:lang="cs">pórovina</skos:prefLabel>
		<skos:prefLabel xml:lang="ca">pisa</skos:prefLabel>
		<skos:altLabel xml:lang="de">Töpferware</skos:altLabel>
		<skos:prefLabel xml:lang="de">Irdenware</skos:prefLabel>
		<skos:prefLabel xml:lang="sv">lergods</skos:prefLabel>
		<skos:prefLabel xml:lang="fi">savitavara</skos:prefLabel>
		<skos:prefLabel xml:lang="es">loza</skos:prefLabel>
		<skos:prefLabel xml:lang="sl">lončenina</skos:prefLabel>
		<skos:prefLabel xml:lang="pt">louça de barro</skos:prefLabel>
		<skos:prefLabel xml:lang="pl">wyroby garncarskie</skos:prefLabel>
		<skos:prefLabel xml:lang="fr">faïence</skos:prefLabel>
		<skos:prefLabel xml:lang="hu">agyagkerámia</skos:prefLabel>
		<skos:prefLabel xml:lang="no">leirgods</skos:prefLabel>
		<skos:prefLabel xml:lang="hr">glineno posuđe</skos:prefLabel>
		<skos:broader rdf:resource="http://partage.vocnet.org/part00064"/>
		<skos:narrower rdf:resource="http://partage.vocnet.org/part00226"/>
		<skos:exactMatch rdf:resource="http://vocab.getty.edu/aat/300140803"/>
		<skos:editorialNote xml:lang="en">PPObjectType</skos:editorialNote>
		<skos:scopeNote xml:lang="en">Pottery with a porous body, fired below 1200 degrees Centigrade. It is not vitrified, and must be glazed to render it nonporous.</skos:scopeNote>
	</skos:Concept>
	<skos:Concept rdf:about="http://partage.vocnet.org/part00225">
		<skos:inScheme rdf:resource="http://partage.vocnet.org/MicroObjectTypes"/>
		<skos:hiddenLabel xml:lang="en">stoneware (pottery)</skos:hiddenLabel>
		<skos:prefLabel xml:lang="en">stoneware</skos:prefLabel>
		<skos:prefLabel xml:lang="de">Steingut</skos:prefLabel>
		<skos:prefLabel xml:lang="sv">stengods</skos:prefLabel>
		<skos:prefLabel xml:lang="fi">kivitavara</skos:prefLabel>
		<skos:altLabel xml:lang="es">gres vidriado</skos:altLabel>
		<skos:prefLabel xml:lang="es">gres</skos:prefLabel>
		<skos:altLabel xml:lang="sl">posodje iz kamenine</skos:altLabel>
		<skos:prefLabel xml:lang="sl">kamenina</skos:prefLabel>
		<skos:prefLabel xml:lang="pt">grés</skos:prefLabel>
		<skos:prefLabel xml:lang="pl">kamionka</skos:prefLabel>
		<skos:prefLabel xml:lang="nl">steengoed</skos:prefLabel>
		<skos:prefLabel xml:lang="it">vasellame</skos:prefLabel>
		<skos:prefLabel xml:lang="cs">kamenina</skos:prefLabel>
		<skos:prefLabel xml:lang="ca">gres</skos:prefLabel>
		<skos:prefLabel xml:lang="fr">grès</skos:prefLabel>
		<skos:prefLabel xml:lang="hu">kőedény</skos:prefLabel>
		<skos:prefLabel xml:lang="no">steingods</skos:prefLabel>
		<skos:prefLabel xml:lang="hr">kamenjača</skos:prefLabel>
		<skos:broader rdf:resource="http://partage.vocnet.org/part00064"/>
		<skos:exactMatch rdf:resource="http://vocab.getty.edu/aat/300010672"/>
		<skos:editorialNote xml:lang="en">PPObjectType</skos:editorialNote>
		<skos:scopeNote xml:lang="en">A type of pottery midway between earthenware and porcelain being made of clay and a fusible stone. It is fired to a point where partial vitrification renders it impervious to liquids, but, unlike porcelain, it is very seldom more than faintly translucent. The vitrification makes it unnecessary to add a glaze, but for reasons of utility and appearance decorative glazes are sometimes used, such as salt glaze and lead glaze.</skos:scopeNote>
	</skos:Concept>
	<skos:Concept rdf:about="http://partage.vocnet.org/part00226">
		<skos:inScheme rdf:resource="http://partage.vocnet.org/MicroObjectTypes"/>
		<skos:prefLabel xml:lang="en">maiolica</skos:prefLabel>
		<skos:prefLabel xml:lang="sv">majolika</skos:prefLabel>
		<skos:prefLabel xml:lang="es">mayólica</skos:prefLabel>
		<skos:altLabel xml:lang="sl">posodje iz majolike</skos:altLabel>
		<skos:prefLabel xml:lang="sl">majolika</skos:prefLabel>
		<skos:prefLabel xml:lang="pt">majólica</skos:prefLabel>
		<skos:prefLabel xml:lang="pl">majolika</skos:prefLabel>
		<skos:prefLabel xml:lang="nl">majolica</skos:prefLabel>
		<skos:prefLabel xml:lang="it">maioliche</skos:prefLabel>
		<skos:prefLabel xml:lang="cs">majolika</skos:prefLabel>
		<skos:prefLabel xml:lang="ca">majòlica</skos:prefLabel>
		<skos:prefLabel xml:lang="de">Majolika</skos:prefLabel>
		<skos:prefLabel xml:lang="fi">majolika</skos:prefLabel>
		<skos:prefLabel xml:lang="fr">majolique</skos:prefLabel>
		<skos:prefLabel xml:lang="hu">majolika</skos:prefLabel>
		<skos:prefLabel xml:lang="no">majolika</skos:prefLabel>
		<skos:prefLabel xml:lang="hr">majolika</skos:prefLabel>
		<skos:broader rdf:resource="http://partage.vocnet.org/part00223"/>
		<skos:exactMatch rdf:resource="http://vocab.getty.edu/aat/300021170"/>
		<skos:editorialNote xml:lang="en">PPObjectType</skos:editorialNote>
		<skos:scopeNote xml:lang="en">Refers to tin-glazed earthenware, particularly such ware produced in Italy. The term originally referred to the island of Majorca (or an alternate theory has it referring to Malaga), and designated only Hispano-Moresque lusterware; but since the 16th century it has been used to refer to Italian tin-glazed ware and imitations of the Italian ware. It is characterized by painted decoration of high quality executed in several colors on the dry but unfired tin glaze, generally with a final coating of clear lead glaze. The range of colors is typically limited to cobalt blue, copper green, manganese purple, antimony yellow, and iron red, with white provided by the tin-glaze material. When white is used for painting, it is applied onto a bluish-white glaze or blue ground. The luster is typically a golden color derived from silver or a mother-of-pearl effect.</skos:scopeNote>
	</skos:Concept>
	<skos:Concept rdf:about="http://partage.vocnet.org/part00249">
		<skos:inScheme rdf:resource="http://partage.vocnet.org/MicroObjectTypes"/>
		<skos:hiddenLabel xml:lang="en">stained glass (visual works)</skos:hiddenLabel>
		<skos:prefLabel xml:lang="en">stained glass</skos:prefLabel>
		<skos:prefLabel xml:lang="hr">vitraji</skos:prefLabel>
		<skos:prefLabel xml:lang="no">blyglass</skos:prefLabel>
		<skos:prefLabel xml:lang="hu">ólomüveg</skos:prefLabel>
		<skos:prefLabel xml:lang="fr">vitrail</skos:prefLabel>
		<skos:prefLabel xml:lang="pl">witraże</skos:prefLabel>
		<skos:prefLabel xml:lang="pt">vitral</skos:prefLabel>
		<skos:prefLabel xml:lang="sl">vitraži</skos:prefLabel>
		<skos:prefLabel xml:lang="es">vidriera de colores</skos:prefLabel>
		<skos:prefLabel xml:lang="sv">blyglas</skos:prefLabel>
		<skos:altLabel xml:lang="de">Buntglas</skos:altLabel>
		<skos:altLabel xml:lang="de">Farbglas</skos:altLabel>
		<skos:prefLabel xml:lang="de">Glasmalerei (Glasfenster)</skos:prefLabel>
		<skos:prefLabel xml:lang="ca">vitrall</skos:prefLabel>
		<skos:prefLabel xml:lang="cs">vitráž</skos:prefLabel>
		<skos:prefLabel xml:lang="it">vetri colorati</skos:prefLabel>
		<skos:prefLabel xml:lang="nl">gebrandschilderd glas</skos:prefLabel>
		<skos:prefLabel xml:lang="fi">lasimaalaus</skos:prefLabel>
		<skos:broader rdf:resource="http://partage.vocnet.org/part00044"/>
		<skos:exactMatch rdf:resource="http://vocab.getty.edu/aat/300263722"/>
		<skos:editorialNote xml:lang="en">PPObjectType</skos:editorialNote>
		<skos:scopeNote xml:lang="en">Refers to works made of colored glass, generally in the form of a window, autonomous panel, or lampshade, in which the design is meant to be observed through refracted light and its effect is greatly dependent on the quality of the light. The stages of manufacture were described in a manual written in the early twelfth century by the monk Theophilus and the process has hardly changed since then. The window or other item is made by cutting pieces of colored glass based on a full-scale cartoon and holding the pieces together by strips of lead. Details may be painted on the surface of the pieces of glass and fired in a kiln before piecing the glass together. The method of weatherproofing and fixing the glass in a window is often highly decorative and forms an important element of the design. The highest achievements in stained glass are thought to be those of the Gothic era in Europe and those of the Gothic Revival of the nineteenth century.</skos:scopeNote>
	</skos:Concept>
	<skos:Concept rdf:about="http://partage.vocnet.org/part00419">
		<skos:inScheme rdf:resource="http://partage.vocnet.org/MicroObjectTypes"/>
		<skos:prefLabel xml:lang="en">photographs</skos:prefLabel>
		<skos:prefLabel xml:lang="de">Fotografie</skos:prefLabel>
		<skos:altLabel xml:lang="de">Photographie</skos:altLabel>
		<skos:prefLabel xml:lang="sv">fotografier</skos:prefLabel>
		<skos:prefLabel xml:lang="fi">valokuvat</skos:prefLabel>
		<skos:prefLabel xml:lang="es">fotografías</skos:prefLabel>
		<skos:prefLabel xml:lang="sl">fotografije</skos:prefLabel>
		<skos:altLabel xml:lang="pt">fotografias</skos:altLabel>
		<skos:prefLabel xml:lang="pt">fotografia</skos:prefLabel>
		<skos:prefLabel xml:lang="pl">fotografie</skos:prefLabel>
		<skos:prefLabel xml:lang="nl">foto's</skos:prefLabel>
		<skos:prefLabel xml:lang="it">fotografie</skos:prefLabel>
		<skos:prefLabel xml:lang="cs">fotografie</skos:prefLabel>
		<skos:prefLabel xml:lang="ca">fotografies</skos:prefLabel>
		<skos:prefLabel xml:lang="hr">fotografije</skos:prefLabel>
		<skos:prefLabel xml:lang="no">fotografi</skos:prefLabel>
		<skos:prefLabel xml:lang="hu">fénykép</skos:prefLabel>
		<skos:prefLabel xml:lang="fr">photographie</skos:prefLabel>
		<skos:altLabel xml:lang="de">Photographien</skos:altLabel>
		<skos:altLabel xml:lang="de">Fotografien</skos:altLabel>
		<skos:altLabel xml:lang="de">Fotos</skos:altLabel>
		<skos:exactMatch rdf:resource="http://vocab.getty.edu/aat/300046300"/>
		<skos:editorialNote xml:lang="en">PPObjectType</skos:editorialNote>
		<skos:scopeNote xml:lang="en">Refers to still images produced from radiation-sensitive materials (sensitive to light, electron beams, or nuclear radiation), generally by means of the chemical action of light on a sensitive film, paper, glass, or metal. It does not include reproductive prints of documents and technical drawings, for which descriptors found under "reprographic copies" are more appropriate. Photographs may be positive or negative, opaque or transparent.</skos:scopeNote>
	</skos:Concept>
	<skos:Concept rdf:about="http://partage.vocnet.org/part00470">
		<skos:inScheme rdf:resource="http://partage.vocnet.org/MicroObjectTypes"/>
		<skos:hiddenLabel xml:lang="en">mural paintings (visual works)</skos:hiddenLabel>
		<skos:prefLabel xml:lang="en">mural paintings</skos:prefLabel>
		<skos:prefLabel xml:lang="nl">muurschilderingen</skos:prefLabel>
		<skos:prefLabel xml:lang="it">murali</skos:prefLabel>
		<skos:prefLabel xml:lang="cs">nástěnné malířství</skos:prefLabel>
		<skos:prefLabel xml:lang="ca">pintura mural</skos:prefLabel>
		<skos:prefLabel xml:lang="de">Wandmalerei</skos:prefLabel>
		<skos:prefLabel xml:lang="sv">muralmålningar</skos:prefLabel>
		<skos:altLabel xml:lang="fi">kattomaalaukset</skos:altLabel>
		<skos:prefLabel xml:lang="fi">seinämaalaukset</skos:prefLabel>
		<skos:prefLabel xml:lang="es">pinturas murales</skos:prefLabel>
		<skos:altLabel xml:lang="sl">freske</skos:altLabel>
		<skos:prefLabel xml:lang="sl">stensko slikarstvo</skos:prefLabel>
		<skos:prefLabel xml:lang="pt">pintura mural</skos:prefLabel>
		<skos:prefLabel xml:lang="pl">malarstwo ścienne</skos:prefLabel>
		<skos:prefLabel xml:lang="fr">peinture murale</skos:prefLabel>
		<skos:prefLabel xml:lang="hu">falkép</skos:prefLabel>
		<skos:prefLabel xml:lang="no">muralmaleri</skos:prefLabel>
		<skos:prefLabel xml:lang="hr">zidno slikarstvo</skos:prefLabel>
		<skos:broader rdf:resource="http://partage.vocnet.org/part00044"/>
		<skos:exactMatch rdf:resource="http://vocab.getty.edu/aat/300033644"/>
		<skos:editorialNote xml:lang="en">PPObjectType</skos:editorialNote>
		<skos:scopeNote xml:lang="en">Painted decorations or scenes that dominate a wall (or ceiling) surface. For works in other media that dominate a wall (or ceiling), use the more general term "murals (any medium)".</skos:scopeNote>
	</skos:Concept>
	<skos:Concept rdf:about="http://partage.vocnet.org/part00498">
		<skos:inScheme rdf:resource="http://partage.vocnet.org/MicroObjectTypes"/>
		<skos:hiddenLabel xml:lang="en">hardware (components)</skos:hiddenLabel>
		<skos:prefLabel xml:lang="en">hardware</skos:prefLabel>
		<skos:prefLabel xml:lang="sv">verktyg</skos:prefLabel>
		<skos:prefLabel xml:lang="fi">rakennustarvikkeet</skos:prefLabel>
		<skos:prefLabel xml:lang="es">herraje</skos:prefLabel>
		<skos:altLabel xml:lang="sl">spojke</skos:altLabel>
		<skos:prefLabel xml:lang="sl">okovje</skos:prefLabel>
		<skos:prefLabel xml:lang="pt">ferragens</skos:prefLabel>
		<skos:prefLabel xml:lang="pl">okucia</skos:prefLabel>
		<skos:prefLabel xml:lang="nl">ijzerwaren</skos:prefLabel>
		<skos:prefLabel xml:lang="it">utensili</skos:prefLabel>
		<skos:prefLabel xml:lang="cs">komponenty</skos:prefLabel>
		<skos:prefLabel xml:lang="ca">ferramenta</skos:prefLabel>
		<skos:prefLabel xml:lang="de">Eisenwaren</skos:prefLabel>
		<skos:prefLabel xml:lang="hr">okovi</skos:prefLabel>
		<skos:prefLabel xml:lang="no">jernvare</skos:prefLabel>
		<skos:prefLabel xml:lang="hu">veret</skos:prefLabel>
		<skos:prefLabel xml:lang="fr">quincaillerie</skos:prefLabel>
		<skos:exactMatch rdf:resource="http://vocab.getty.edu/aat/300033260"/>
		<skos:editorialNote xml:lang="en">PPObjectType</skos:editorialNote>
		<skos:scopeNote xml:lang="en">Large and small items that are necessary to attach, anchor, hold, or join materials and components of structures, furniture, and other objects. Also, items used in the finishing of buildings and objects, such as hinges and knobs.</skos:scopeNote>
	</skos:Concept>
	<skos:Concept rdf:about="http://partage.vocnet.org/part00501">
		<skos:inScheme rdf:resource="http://partage.vocnet.org/MicroObjectTypes"/>
		<skos:hiddenLabel xml:lang="en">watercolors (paintings)</skos:hiddenLabel>
		<skos:prefLabel xml:lang="en">watercolours</skos:prefLabel>
		<skos:altLabel xml:lang="de">Aquarelle</skos:altLabel>
		<skos:prefLabel xml:lang="sv">akvareller</skos:prefLabel>
		<skos:prefLabel xml:lang="fi">akvarellimaalaus</skos:prefLabel>
		<skos:prefLabel xml:lang="es">acuarelas</skos:prefLabel>
		<skos:prefLabel xml:lang="sl">akvareli</skos:prefLabel>
		<skos:prefLabel xml:lang="pt">aguarela</skos:prefLabel>
		<skos:prefLabel xml:lang="pl">akwarele</skos:prefLabel>
		<skos:prefLabel xml:lang="nl">aquarellen</skos:prefLabel>
		<skos:prefLabel xml:lang="it">acquarelli</skos:prefLabel>
		<skos:prefLabel xml:lang="cs">akvarel</skos:prefLabel>
		<skos:prefLabel xml:lang="ca">aquarel·les</skos:prefLabel>
		<skos:prefLabel xml:lang="fr">aquarelle</skos:prefLabel>
		<skos:prefLabel xml:lang="hu">akvarell</skos:prefLabel>
		<skos:prefLabel xml:lang="no">akvarell</skos:prefLabel>
		<skos:prefLabel xml:lang="hr">akvareli</skos:prefLabel>
		<skos:prefLabel xml:lang="de">Aquarell</skos:prefLabel>
		<skos:altLabel xml:lang="en">watercolors</skos:altLabel>
		<skos:broader rdf:resource="http://partage.vocnet.org/part00044"/>
		<skos:exactMatch rdf:resource="http://vocab.getty.edu/aat/300078925"/>
		<skos:editorialNote xml:lang="en">PPObjectType</skos:editorialNote>
		<skos:scopeNote xml:lang="en">Refers to two-dimensional works of art, usually on a paper support, to which pigment suspended in water is applied with a brush to create an image or design.</skos:scopeNote>
	</skos:Concept>
	<skos:Concept rdf:about="http://partage.vocnet.org/part00502">
		<skos:inScheme rdf:resource="http://partage.vocnet.org/MicroObjectTypes"/>
		<skos:hiddenLabel xml:lang="en">magazines (periodicals)</skos:hiddenLabel>
		<skos:prefLabel xml:lang="en">magazines</skos:prefLabel>
		<skos:prefLabel xml:lang="sv">tidskrifter</skos:prefLabel>
		<skos:prefLabel xml:lang="fi">aikakauslehdet</skos:prefLabel>
		<skos:prefLabel xml:lang="es">revistas</skos:prefLabel>
		<skos:prefLabel xml:lang="sl">revije</skos:prefLabel>
		<skos:altLabel xml:lang="pt">revistas</skos:altLabel>
		<skos:prefLabel xml:lang="pt">revista</skos:prefLabel>
		<skos:prefLabel xml:lang="pl">czasopisma</skos:prefLabel>
		<skos:prefLabel xml:lang="nl">magazines</skos:prefLabel>
		<skos:prefLabel xml:lang="it">riviste</skos:prefLabel>
		<skos:prefLabel xml:lang="cs">časopisy</skos:prefLabel>
		<skos:prefLabel xml:lang="ca">revistes</skos:prefLabel>
		<skos:altLabel xml:lang="de">Magazin</skos:altLabel>
		<skos:prefLabel xml:lang="de">Zeitschriften</skos:prefLabel>
		<skos:altLabel xml:lang="de">Zeitschrift</skos:altLabel>
		<skos:prefLabel xml:lang="hr">časopisi</skos:prefLabel>
		<skos:prefLabel xml:lang="no">tidsskrift</skos:prefLabel>
		<skos:prefLabel xml:lang="hu">folyóirat</skos:prefLabel>
		<skos:prefLabel xml:lang="fr">revue</skos:prefLabel>
		<skos:altLabel xml:lang="de">Magazine</skos:altLabel>
		<skos:exactMatch rdf:resource="http://vocab.getty.edu/aat/300215389"/>
		<skos:editorialNote xml:lang="en">PPObjectType</skos:editorialNote>
		<skos:scopeNote xml:lang="en">Periodicals containing articles, essays, poems, or other writings by different authors, usually on a variety of topics and intended for a general reading public or treating a particular area of interest for a popular audience.</skos:scopeNote>
	</skos:Concept>
	<skos:Concept rdf:about="http://partage.vocnet.org/part00505">
		<skos:inScheme rdf:resource="http://partage.vocnet.org/MicroObjectTypes"/>
		<skos:prefLabel xml:lang="en">printing plates</skos:prefLabel>
		<skos:prefLabel xml:lang="de">Druckplatten</skos:prefLabel>
		<skos:prefLabel xml:lang="sv">tryckplåtar</skos:prefLabel>
		<skos:prefLabel xml:lang="fi">painolaatat</skos:prefLabel>
		<skos:prefLabel xml:lang="es">planchas de impresión</skos:prefLabel>
		<skos:prefLabel xml:lang="sl">tiskarske plošče</skos:prefLabel>
		<skos:prefLabel xml:lang="pt">chapa de impressão</skos:prefLabel>
		<skos:prefLabel xml:lang="pl">płyty graficzne</skos:prefLabel>
		<skos:prefLabel xml:lang="nl">drukplaten</skos:prefLabel>
		<skos:prefLabel xml:lang="it">matrici di incisione</skos:prefLabel>
		<skos:prefLabel xml:lang="cs">tisková matrice</skos:prefLabel>
		<skos:prefLabel xml:lang="ca">planxes d'impressió</skos:prefLabel>
		<skos:altLabel xml:lang="de">Matritze</skos:altLabel>
		<skos:altLabel xml:lang="de">Druckstock</skos:altLabel>
		<skos:altLabel xml:lang="de">Druckform</skos:altLabel>
		<skos:prefLabel xml:lang="hr">grafičke ploče</skos:prefLabel>
		<skos:prefLabel xml:lang="hu">nyomódúc</skos:prefLabel>
		<skos:prefLabel xml:lang="no">trykkeplater</skos:prefLabel>
		<skos:prefLabel xml:lang="fr">plaque d'imprimerie</skos:prefLabel>
		<skos:altLabel xml:lang="de">Matritzen</skos:altLabel>
		<skos:altLabel xml:lang="de">Druckstöcke</skos:altLabel>
		<skos:altLabel xml:lang="de">Druckformen</skos:altLabel>
		<skos:broader rdf:resource="http://partage.vocnet.org/part00218"/>
		<skos:exactMatch rdf:resource="http://vocab.getty.edu/aat/300022755"/>
		<skos:editorialNote xml:lang="en">PPObjectType</skos:editorialNote>
		<skos:scopeNote xml:lang="en">Flat pieces of metal from which textual or pictorial images are printed. For blocks of other material, usually wood, cut to print an image or used to support other materials that form the printing surface, use "printing blocks" or a more specific term.</skos:scopeNote>
	</skos:Concept>
	<skos:Concept rdf:about="http://partage.vocnet.org/part00510">
		<skos:inScheme rdf:resource="http://partage.vocnet.org/MicroObjectTypes"/>
		<skos:hiddenLabel xml:lang="en">painted glass (visual works)</skos:hiddenLabel>
		<skos:prefLabel xml:lang="en">painted glass</skos:prefLabel>
		<skos:prefLabel xml:lang="de">Glasmalerei</skos:prefLabel>
		<skos:prefLabel xml:lang="sv">målat glas</skos:prefLabel>
		<skos:prefLabel xml:lang="fi">maalattu lasi</skos:prefLabel>
		<skos:altLabel xml:lang="fi">lasimaalaus.</skos:altLabel>
		<skos:altLabel xml:lang="es">pintura en vidrio</skos:altLabel>
		<skos:prefLabel xml:lang="es">vidrio pintado</skos:prefLabel>
		<skos:prefLabel xml:lang="sl">slikano steklo</skos:prefLabel>
		<skos:prefLabel xml:lang="pt">vidro pintado</skos:prefLabel>
		<skos:prefLabel xml:lang="pl">szkło malowane</skos:prefLabel>
		<skos:prefLabel xml:lang="nl">geschilderd glas</skos:prefLabel>
		<skos:prefLabel xml:lang="it">vetri dipinti</skos:prefLabel>
		<skos:prefLabel xml:lang="cs">malované sklo</skos:prefLabel>
		<skos:prefLabel xml:lang="ca">vidre pintat</skos:prefLabel>
		<skos:altLabel xml:lang="de">gefasstes Glas</skos:altLabel>
		<skos:prefLabel xml:lang="fr">peinture sur verre</skos:prefLabel>
		<skos:prefLabel xml:lang="hu">festett üveg</skos:prefLabel>
		<skos:prefLabel xml:lang="no">glassmaleri</skos:prefLabel>
		<skos:prefLabel xml:lang="hr">oslikano staklo</skos:prefLabel>
		<skos:broader rdf:resource="http://partage.vocnet.org/part00044"/>
		<skos:exactMatch rdf:resource="http://vocab.getty.edu/aat/300343822"/>
		<skos:editorialNote xml:lang="en">PPObjectType</skos:editorialNote>
		<skos:scopeNote xml:lang="en">Works done by painting on the front or the reverse of glass, whether or not the paint is then fired onto the glass. Painted glass mirrors and other glass decoration, and painted works in the manner of painting on canvas or wooden panels were known since ancient times. In the context of stained glass windows and panels, refers to parts of the image that are painted on glass (often stained glass), especially the smaller details.</skos:scopeNote>
	</skos:Concept>
	<skos:Concept rdf:about="http://partage.vocnet.org/part00511">
		<skos:inScheme rdf:resource="http://partage.vocnet.org/MicroObjectTypes"/>
		<skos:prefLabel xml:lang="en">fine bindings</skos:prefLabel>
		<skos:altLabel xml:lang="de">Bucheinband</skos:altLabel>
		<skos:prefLabel xml:lang="sv">bokband</skos:prefLabel>
		<skos:prefLabel xml:lang="fi">taidesidokset</skos:prefLabel>
		<skos:prefLabel xml:lang="es">encuadernación de lujo</skos:prefLabel>
		<skos:prefLabel xml:lang="sl">bibliofilske vezave</skos:prefLabel>
		<skos:prefLabel xml:lang="pt">encadernação</skos:prefLabel>
		<skos:prefLabel xml:lang="pl">oprawy artystyczne</skos:prefLabel>
		<skos:prefLabel xml:lang="nl">kunstboekbanden</skos:prefLabel>
		<skos:prefLabel xml:lang="it">legature</skos:prefLabel>
		<skos:prefLabel xml:lang="cs">knižní vazba</skos:prefLabel>
		<skos:prefLabel xml:lang="ca">enquadernació de luxe</skos:prefLabel>
		<skos:altLabel xml:lang="de">Buchkunst</skos:altLabel>
		<skos:prefLabel xml:lang="de">Bucheinbände</skos:prefLabel>
		<skos:prefLabel xml:lang="hr">umjetničko knjigoveštvo</skos:prefLabel>
		<skos:prefLabel xml:lang="no">kunstbokbind</skos:prefLabel>
		<skos:prefLabel xml:lang="hu">művészi könyvkötés</skos:prefLabel>
		<skos:prefLabel xml:lang="fr">reliure d'art</skos:prefLabel>
		<skos:exactMatch rdf:resource="http://vocab.getty.edu/aat/300311788"/>
		<skos:editorialNote xml:lang="en">PPObjectType</skos:editorialNote>
		<skos:scopeNote xml:lang="en">Bindings produced as unique or limited editions and intended to be works of art in themselves.</skos:scopeNote>
	</skos:Concept>
	<skos:Concept rdf:about="http://partage.vocnet.org/part00512">
		<skos:inScheme rdf:resource="http://partage.vocnet.org/MicroObjectTypes"/>
		<skos:prefLabel xml:lang="en">wickerwork</skos:prefLabel>
		<skos:prefLabel xml:lang="de">Flechtwerk</skos:prefLabel>
		<skos:prefLabel xml:lang="sv">korgarbete</skos:prefLabel>
		<skos:prefLabel xml:lang="fi">punontatyöt</skos:prefLabel>
		<skos:prefLabel xml:lang="es">obra de mimbre</skos:prefLabel>
		<skos:prefLabel xml:lang="sl">pletarski izdelki</skos:prefLabel>
		<skos:prefLabel xml:lang="pt">trabalho de verga</skos:prefLabel>
		<skos:prefLabel xml:lang="pl">wyroby wyplatane</skos:prefLabel>
		<skos:prefLabel xml:lang="nl">vlechtwerk</skos:prefLabel>
		<skos:prefLabel xml:lang="it">oggetti di vimini</skos:prefLabel>
		<skos:prefLabel xml:lang="cs">práce z proutí</skos:prefLabel>
		<skos:prefLabel xml:lang="ca">obra de vímet</skos:prefLabel>
		<skos:prefLabel xml:lang="hr">predmeti od šiblja</skos:prefLabel>
		<skos:prefLabel xml:lang="no">kurvfletting</skos:prefLabel>
		<skos:prefLabel xml:lang="hu">fonás</skos:prefLabel>
		<skos:prefLabel xml:lang="fr">vannerie</skos:prefLabel>
		<skos:exactMatch rdf:resource="http://vocab.getty.edu/aat/300044074"/>
		<skos:editorialNote xml:lang="en">PPObjectType</skos:editorialNote>
		<skos:scopeNote xml:lang="en">Objects created with real or simulated flexible twigs, plaited together.</skos:scopeNote>
	</skos:Concept>
	<skos:Concept rdf:about="http://partage.vocnet.org/part00513">
		<skos:inScheme rdf:resource="http://partage.vocnet.org/MicroObjectTypes"/>
		<skos:hiddenLabel xml:lang="en">illustrations (layout features)</skos:hiddenLabel>
		<skos:prefLabel xml:lang="en">illustrations</skos:prefLabel>
		<skos:prefLabel xml:lang="de">Illustration</skos:prefLabel>
		<skos:altLabel xml:lang="pt">ilustraçãos</skos:altLabel>
		<skos:prefLabel xml:lang="pt">ilustração</skos:prefLabel>
		<skos:prefLabel xml:lang="pl">ilustracje</skos:prefLabel>
		<skos:prefLabel xml:lang="nl">illustraties</skos:prefLabel>
		<skos:prefLabel xml:lang="it">illustrazioni</skos:prefLabel>
		<skos:prefLabel xml:lang="cs">ilustrace</skos:prefLabel>
		<skos:prefLabel xml:lang="ca">il·lustracions</skos:prefLabel>
		<skos:prefLabel xml:lang="sv">illustrationer</skos:prefLabel>
		<skos:prefLabel xml:lang="fi">kuvitus</skos:prefLabel>
		<skos:prefLabel xml:lang="fr">illustrations</skos:prefLabel>
		<skos:prefLabel xml:lang="hu">illusztráció</skos:prefLabel>
		<skos:prefLabel xml:lang="no">illustrasjoner</skos:prefLabel>
		<skos:prefLabel xml:lang="hr">ilustracije</skos:prefLabel>
		<skos:prefLabel xml:lang="es">ilustraciones</skos:prefLabel>
		<skos:prefLabel xml:lang="sl">ilustracije</skos:prefLabel>
		<skos:exactMatch rdf:resource="http://vocab.getty.edu/aat/300015578"/>
		<skos:editorialNote xml:lang="en">PPObjectType</skos:editorialNote>
		<skos:scopeNote xml:lang="en">Pictures or diagrams that clarify or provide an example or visualization. They usually accompany a text; the term is most often used to refer to pictures in books or published journal. For works that explore a subject or are preliminary to a separate, more finalized work, use "studies (visual works)." For paintings in manuscripts, use "illuminations" or "miniatures (paintings)."</skos:scopeNote>
	</skos:Concept>
</rdf:RDF>
